<?xml version="1.0" encoding="UTF-8"?>
<rdf:RDF
   xmlns:dc="http://purl.org/dc/elements/1.1/"
   xmlns:odm2="http://vocabulary.odm2.org/ODM2/ODM2Terms/"
   xmlns:rdf="http://www.w3.org/1999/02/22-rdf-syntax-ns#"
   xmlns:skos="http://www.w3.org/2004/02/skos/core#"
>
  <rdf:Description rdf:about="http://vocabulary.odm2.org/unitstype/magneticPermeability">
    <odm2:dimensionTime>1</odm2:dimensionTime>
    <skos:definition>Permeability is the degree of magnetization of a material that responds linearly to an applied magnetic field. In general permeability is a tensor-valued quantity.</skos:definition>
    <odm2:defaultUnit>Henry per meter (H/m)</odm2:defaultUnit>
    <odm2:dimensionAmount>0</odm2:dimensionAmount>
    <odm2:dimensionLength>0</odm2:dimensionLength>
    <skos:prefLabel>Magnetic permeability</skos:prefLabel>
    <rdf:type rdf:resource="http://www.w3.org/2004/02/skos/core#Concept"/>
    <odm2:dimensionLight>0</odm2:dimensionLight>
    <odm2:dimensionSymbol>L1M1T-2I-2</odm2:dimensionSymbol>
    <odm2:category>Electricity and Magnetism</odm2:category>
    <odm2:dimensionMass>1</odm2:dimensionMass>
    <skos:exactMatch>http://qudt.org/schema/qudt#PermeabilityUnit</skos:exactMatch>
    <odm2:dimensionCurrent>-2</odm2:dimensionCurrent>
    <skos:inScheme rdf:resource="http://vocabulary.odm2.org/unitstype"/>
    <odm2:dimensionTemperature>-2</odm2:dimensionTemperature>
    <skos:historyNote>QUDT</skos:historyNote>
  </rdf:Description>
  <rdf:Description rdf:about="http://vocabulary.odm2.org/unitstype/lengthMass">
    <rdf:type rdf:resource="http://www.w3.org/2004/02/skos/core#Concept"/>
    <odm2:dimensionSymbol>L1M1</odm2:dimensionSymbol>
    <odm2:dimensionCurrent>0</odm2:dimensionCurrent>
    <odm2:dimensionTime>1</odm2:dimensionTime>
    <odm2:dimensionLength>0</odm2:dimensionLength>
    <skos:inScheme rdf:resource="http://vocabulary.odm2.org/unitstype"/>
    <skos:exactMatch>http://qudt.org/vocab/quantity#Lengthmass</skos:exactMatch>
    <odm2:dimensionMass>1</odm2:dimensionMass>
    <odm2:dimensionAmount>0</odm2:dimensionAmount>
    <skos:prefLabel>Length mass</skos:prefLabel>
    <odm2:category>Mechanics</odm2:category>
    <odm2:dimensionLight>0</odm2:dimensionLight>
    <odm2:defaultUnit>Meter kilogram (m-kg)</odm2:defaultUnit>
    <odm2:dimensionTemperature>0</odm2:dimensionTemperature>
    <skos:historyNote>QUDT</skos:historyNote>
  </rdf:Description>
  <rdf:Description rdf:about="http://vocabulary.odm2.org/unitstype/lengthEnergy">
    <odm2:defaultUnit>Joule meter</odm2:defaultUnit>
    <rdf:type rdf:resource="http://www.w3.org/2004/02/skos/core#Concept"/>
    <odm2:dimensionTemperature>0</odm2:dimensionTemperature>
    <skos:prefLabel>Length energy</skos:prefLabel>
    <odm2:dimensionSymbol>L3M1T-2</odm2:dimensionSymbol>
    <odm2:dimensionLight>0</odm2:dimensionLight>
    <odm2:dimensionTime>1</odm2:dimensionTime>
    <skos:historyNote>QUDT</skos:historyNote>
    <odm2:dimensionMass>3</odm2:dimensionMass>
    <odm2:dimensionCurrent>-2</odm2:dimensionCurrent>
    <skos:exactMatch>http://qudt.org/vocab/quantity#Lengthenergy; http://qudt.org/vocab/quantity#ThermalEnergyLength</skos:exactMatch>
    <skos:inScheme rdf:resource="http://vocabulary.odm2.org/unitstype"/>
    <odm2:dimensionLength>0</odm2:dimensionLength>
    <odm2:category>Mechanics</odm2:category>
    <odm2:dimensionAmount>0</odm2:dimensionAmount>
    <skos:note>redundant with thermalEnergyLength</skos:note>
  </rdf:Description>
  <rdf:Description rdf:about="http://vocabulary.odm2.org/unitstype/jerk">
    <odm2:category>Mechanics</odm2:category>
    <odm2:dimensionSymbol>L1T-3</odm2:dimensionSymbol>
    <odm2:defaultUnit>Meters per second cubed (m/s^3)</odm2:defaultUnit>
    <skos:inScheme rdf:resource="http://vocabulary.odm2.org/unitstype"/>
    <odm2:dimensionMass>1</odm2:dimensionMass>
    <skos:historyNote>Aquarius</skos:historyNote>
    <skos:definition>In physics, jerk, also known as jolt, surge, or lurch, is the rate of change of acceleration; that is, the derivative of acceleration with respect to time, and as such the second derivative of velocity, or the third derivative of position. [Wikipedia: https://en.wikipedia.org/wiki/Jerk_%28physics%29]</skos:definition>
    <odm2:dimensionTemperature>0</odm2:dimensionTemperature>
    <rdf:type rdf:resource="http://www.w3.org/2004/02/skos/core#Concept"/>
    <odm2:dimensionLight>0</odm2:dimensionLight>
    <odm2:dimensionAmount>0</odm2:dimensionAmount>
    <skos:prefLabel>Jerk</skos:prefLabel>
    <odm2:dimensionTime>0</odm2:dimensionTime>
    <odm2:dimensionCurrent>-3</odm2:dimensionCurrent>
    <odm2:dimensionLength>0</odm2:dimensionLength>
  </rdf:Description>
  <rdf:Description rdf:about="http://vocabulary.odm2.org/unitstype/thermalConductivity">
    <odm2:dimensionCurrent>-3</odm2:dimensionCurrent>
    <odm2:dimensionAmount>-1</odm2:dimensionAmount>
    <odm2:category>Thermodynamics</odm2:category>
    <odm2:dimensionSymbol>L1M1T-3?-1</odm2:dimensionSymbol>
    <odm2:dimensionTemperature>0</odm2:dimensionTemperature>
    <odm2:dimensionLength>0</odm2:dimensionLength>
    <odm2:dimensionLight>0</odm2:dimensionLight>
    <rdf:type rdf:resource="http://www.w3.org/2004/02/skos/core#Concept"/>
    <skos:exactMatch>http://qudt.org/vocab/quantity#Thermalconductivity</skos:exactMatch>
    <odm2:dimensionMass>1</odm2:dimensionMass>
    <skos:prefLabel>Thermal conductivity</skos:prefLabel>
    <skos:inScheme rdf:resource="http://vocabulary.odm2.org/unitstype"/>
    <odm2:defaultUnit>Watt per meter kelvin (W/(m*K))</odm2:defaultUnit>
    <odm2:dimensionTime>1</odm2:dimensionTime>
    <skos:historyNote>QUDT</skos:historyNote>
    <skos:definition>In physics, thermal conductivity (often denoted k, ?, or ?) is the property of a material to conduct heat. Thermal conductivity of materials is temperature dependent. The reciprocal of thermal conductivity is called thermal resistivity.</skos:definition>
  </rdf:Description>
  <rdf:Description rdf:about="http://vocabulary.odm2.org/unitstype/energyDensity">
    <odm2:dimensionCurrent>-2</odm2:dimensionCurrent>
    <odm2:dimensionLight>0</odm2:dimensionLight>
    <rdf:type rdf:resource="http://www.w3.org/2004/02/skos/core#Concept"/>
    <odm2:dimensionAmount>0</odm2:dimensionAmount>
    <skos:inScheme rdf:resource="http://vocabulary.odm2.org/unitstype"/>
    <skos:historyNote>QUDT</skos:historyNote>
    <skos:prefLabel>Energy density</skos:prefLabel>
    <skos:note>Has identical dimensionality to pressure or stress</skos:note>
    <odm2:dimensionMass>-1</odm2:dimensionMass>
    <skos:definition>Energy density is the amount of energy stored in a given system or region of space per unit volume or mass, though the latter is more accurately termed specific energy.</skos:definition>
    <odm2:dimensionTime>1</odm2:dimensionTime>
    <odm2:dimensionTemperature>0</odm2:dimensionTemperature>
    <odm2:dimensionLength>0</odm2:dimensionLength>
    <skos:exactMatch>http://qudt.org/vocab/quantity#Energydensity</skos:exactMatch>
    <odm2:dimensionSymbol>L-1M1T-2</odm2:dimensionSymbol>
    <odm2:category>Mechanics</odm2:category>
    <odm2:defaultUnit>Joule per cubic meter (J/m^3)</odm2:defaultUnit>
  </rdf:Description>
  <rdf:Description rdf:about="http://vocabulary.odm2.org/unitstype/concentrationCountPerVolume">
    <odm2:dimensionAmount>0</odm2:dimensionAmount>
    <skos:exactMatch>http://qudt.org/vocab/quantity#AmountOfSubstancePerUnitVolume</skos:exactMatch>
    <odm2:dimensionMass>-3</odm2:dimensionMass>
    <odm2:dimensionSymbol>L-3N1</odm2:dimensionSymbol>
    <skos:inScheme rdf:resource="http://vocabulary.odm2.org/unitstype"/>
    <skos:note>Distinct from inverse volume in that there is something specific being counted within each unit volume.  Inverse volume implies a truly dimensionless numerator.</skos:note>
    <odm2:dimensionLength>0</odm2:dimensionLength>
    <odm2:dimensionLight>1</odm2:dimensionLight>
    <rdf:type rdf:resource="http://www.w3.org/2004/02/skos/core#Concept"/>
    <odm2:dimensionTemperature>0</odm2:dimensionTemperature>
    <skos:definition>Amount of substance or a count/number of items per unit volume. Concentration impliles the amount of one substance/item within another substance.</skos:definition>
    <odm2:dimensionTime>0</odm2:dimensionTime>
    <odm2:dimensionCurrent>0</odm2:dimensionCurrent>
    <skos:prefLabel>Concentration count per volume</skos:prefLabel>
    <odm2:category>Chemistry</odm2:category>
    <odm2:defaultUnit>Mole per cubic meter (mol/m^3) or per cubic meter (1/m^3)</odm2:defaultUnit>
    <skos:historyNote>QUDT</skos:historyNote>
  </rdf:Description>
  <rdf:Description rdf:about="http://vocabulary.odm2.org/unitstype/frequency">
    <rdf:type rdf:resource="http://www.w3.org/2004/02/skos/core#Concept"/>
    <odm2:dimensionLight>0</odm2:dimensionLight>
    <odm2:dimensionCurrent>-1</odm2:dimensionCurrent>
    <skos:inScheme rdf:resource="http://vocabulary.odm2.org/unitstype"/>
    <odm2:defaultUnit>Hertz (Hz) or Inverse second time (s^-1)</odm2:defaultUnit>
    <odm2:dimensionTime>0</odm2:dimensionTime>
    <skos:exactMatch>http://qudt.org/vocab/quantity#Frequency</skos:exactMatch>
    <odm2:dimensionTemperature>0</odm2:dimensionTemperature>
    <odm2:dimensionMass>0</odm2:dimensionMass>
    <skos:definition>Frequency is the number of occurrences of a repeating event per unit time. The repetition of the events may be periodic (i.e. the length of time between event repetitions is fixed) or aperiodic (i.e. the length of time between event repetitions varies). Therefore, we distinguish between periodic and aperiodic frequencies. In the SI system, periodic frequency is measured in hertz (Hz) or multiples of hertz, while aperiodic frequency is measured in becquerel (Bq).</skos:definition>
    <skos:prefLabel>Frequency</skos:prefLabel>
    <skos:historyNote>QUDT</skos:historyNote>
    <odm2:dimensionSymbol>T-1 or N1T-1</odm2:dimensionSymbol>
    <odm2:category>Space and Time</odm2:category>
    <odm2:dimensionLength>0</odm2:dimensionLength>
    <odm2:dimensionAmount>0</odm2:dimensionAmount>
  </rdf:Description>
  <rdf:Description rdf:about="http://vocabulary.odm2.org/unitstype/yank">
    <odm2:dimensionTemperature>0</odm2:dimensionTemperature>
    <rdf:type rdf:resource="http://www.w3.org/2004/02/skos/core#Concept"/>
    <skos:definition>Yank is the rate of change of force.</skos:definition>
    <odm2:defaultUnit>Newtons per second (N/s)</odm2:defaultUnit>
    <odm2:dimensionLight>0</odm2:dimensionLight>
    <skos:inScheme rdf:resource="http://vocabulary.odm2.org/unitstype"/>
    <odm2:dimensionMass>1</odm2:dimensionMass>
    <odm2:category>Mechanics</odm2:category>
    <odm2:dimensionAmount>0</odm2:dimensionAmount>
    <odm2:dimensionCurrent>-3</odm2:dimensionCurrent>
    <odm2:dimensionLength>0</odm2:dimensionLength>
    <skos:historyNote>Aquarius</skos:historyNote>
    <skos:prefLabel>Yank</skos:prefLabel>
    <odm2:dimensionTime>1</odm2:dimensionTime>
    <odm2:dimensionSymbol>L1M1T-3</odm2:dimensionSymbol>
  </rdf:Description>
  <rdf:Description rdf:about="http://vocabulary.odm2.org/unitstype/electricalQuadrupoleMoment">
    <odm2:dimensionAmount>0</odm2:dimensionAmount>
    <odm2:dimensionSymbol>L2T1I1</odm2:dimensionSymbol>
    <odm2:dimensionLength>0</odm2:dimensionLength>
    <odm2:dimensionTemperature>1</odm2:dimensionTemperature>
    <odm2:dimensionMass>2</odm2:dimensionMass>
    <rdf:type rdf:resource="http://www.w3.org/2004/02/skos/core#Concept"/>
    <odm2:dimensionCurrent>1</odm2:dimensionCurrent>
    <odm2:dimensionLight>0</odm2:dimensionLight>
    <odm2:defaultUnit>Coulomb square meter (C-m^2)</odm2:defaultUnit>
    <skos:prefLabel>Electrical quadrupole moment</skos:prefLabel>
    <odm2:category>Electricity and Magnetism</odm2:category>
    <odm2:dimensionTime>0</odm2:dimensionTime>
    <skos:note>&lt;http://dbpedia.org/resource/Quadrupole&gt;</skos:note>
    <skos:inScheme rdf:resource="http://vocabulary.odm2.org/unitstype"/>
    <skos:exactMatch>http://qudt.org/vocab/quantity#ElectricQuadrupoleMoment</skos:exactMatch>
    <skos:definition>The Electric Quadrupole Moment is a quantity which describes the effective shape of the ellipsoid of nuclear charge distribution. A non-zero quadrupole moment Q indicates that the charge distribution is not spherically symmetric. By convention, the value of Q is taken to be positive if the ellipsoid is prolate and negative if it is oblate. In general, the electric quadrupole moment is tensor-valued.</skos:definition>
    <skos:historyNote>QUDT</skos:historyNote>
  </rdf:Description>
  <rdf:Description rdf:about="http://vocabulary.odm2.org/unitstype/magneticFlux">
    <skos:inScheme rdf:resource="http://vocabulary.odm2.org/unitstype"/>
    <odm2:dimensionAmount>0</odm2:dimensionAmount>
    <odm2:dimensionLength>0</odm2:dimensionLength>
    <skos:historyNote>QUDT</skos:historyNote>
    <odm2:dimensionLight>0</odm2:dimensionLight>
    <rdf:type rdf:resource="http://www.w3.org/2004/02/skos/core#Concept"/>
    <skos:exactMatch>http://qudt.org/vocab/quantity#Magneticflux</skos:exactMatch>
    <odm2:dimensionTemperature>-1</odm2:dimensionTemperature>
    <odm2:dimensionCurrent>-2</odm2:dimensionCurrent>
    <odm2:dimensionMass>2</odm2:dimensionMass>
    <odm2:dimensionTime>1</odm2:dimensionTime>
    <odm2:category>Electricity and Magnetism</odm2:category>
    <odm2:dimensionSymbol>L2M1T-2I-1</odm2:dimensionSymbol>
    <odm2:defaultUnit>Weber (Wb)</odm2:defaultUnit>
    <skos:prefLabel>Magnetic flux</skos:prefLabel>
    <skos:definition>Magnetic Flux is the product of the average magnetic field times the perpendicular area that it penetrates.</skos:definition>
  </rdf:Description>
  <rdf:Description rdf:about="http://vocabulary.odm2.org/unitstype/magneticDipoleMoment">
    <odm2:category>Electricity and Magnetism</odm2:category>
    <odm2:dimensionTime>0</odm2:dimensionTime>
    <odm2:dimensionCurrent>0</odm2:dimensionCurrent>
    <odm2:dimensionSymbol>L2I1</odm2:dimensionSymbol>
    <skos:exactMatch>http://qudt.org/vocab/quantity#Magneticdipolemoment</skos:exactMatch>
    <skos:inScheme rdf:resource="http://vocabulary.odm2.org/unitstype"/>
    <odm2:defaultUnit>Joule per Tesla (J/T)</odm2:defaultUnit>
    <skos:historyNote>QUDT</skos:historyNote>
    <odm2:dimensionAmount>0</odm2:dimensionAmount>
    <odm2:dimensionLength>0</odm2:dimensionLength>
    <odm2:dimensionTemperature>1</odm2:dimensionTemperature>
    <odm2:dimensionMass>2</odm2:dimensionMass>
    <skos:definition>The magnetic moment of a system is a measure of the magnitude and the direction of its magnetism. Magnetic moment usually refers to its Magnetic Dipole Moment, and quantifies the contribution of the system's internal magnetism to the external dipolar magnetic field produced by the system (that is, the component of the external magnetic field that is inversely proportional to the cube of the distance to the observer). The Magnetic Dipole Moment is a vector-valued quantity.</skos:definition>
    <rdf:type rdf:resource="http://www.w3.org/2004/02/skos/core#Concept"/>
    <skos:prefLabel>Magnetic dipole moment</skos:prefLabel>
    <odm2:dimensionLight>0</odm2:dimensionLight>
  </rdf:Description>
  <rdf:Description rdf:about="http://vocabulary.odm2.org/unitstype/torque">
    <odm2:dimensionSymbol>L2M1T-2</odm2:dimensionSymbol>
    <odm2:dimensionLength>0</odm2:dimensionLength>
    <odm2:category>Mechanics</odm2:category>
    <odm2:dimensionAmount>0</odm2:dimensionAmount>
    <skos:prefLabel>Torque</skos:prefLabel>
    <skos:historyNote>QUDT</skos:historyNote>
    <skos:exactMatch>http://qudt.org/vocab/quantity#Torque</skos:exactMatch>
    <rdf:type rdf:resource="http://www.w3.org/2004/02/skos/core#Concept"/>
    <odm2:dimensionMass>2</odm2:dimensionMass>
    <skos:note>Has the same dimensionality as energy/work</skos:note>
    <skos:inScheme rdf:resource="http://vocabulary.odm2.org/unitstype"/>
    <odm2:dimensionTemperature>0</odm2:dimensionTemperature>
    <odm2:dimensionTime>1</odm2:dimensionTime>
    <odm2:dimensionLight>0</odm2:dimensionLight>
    <odm2:defaultUnit>Newton meter (N-m)</odm2:defaultUnit>
    <odm2:dimensionCurrent>-2</odm2:dimensionCurrent>
    <skos:definition>In physics, a torque (?) is a vector that measures the tendency of a force to rotate an object about some axis [1]. The magnitude of a torque is defined as force times its lever arm [2]. Just as a force is a push or a pull, a torque can be thought of as a twist. The SI unit for torque is newton meters (N m). In U.S. customary units, it is measured in foot pounds (ft lbf) (also known as 'pounds feet'). Mathematically, the torque on a particle (which has the position r in some reference frame) can be defined as the cross product: ? = r x F where r is the particle's position vector relative to the fulcrum F is the force acting on the particles, or, more generally, torque can be defined as the rate of change of angular momentum, ? = dL/dt where L is the angular momentum vector t stands for time.</skos:definition>
  </rdf:Description>
  <rdf:Description rdf:about="http://vocabulary.odm2.org/unitstype/energy">
    <rdf:type rdf:resource="http://www.w3.org/2004/02/skos/core#Concept"/>
    <skos:exactMatch>http://qudt.org/schema/qudt#EnergyAndWorkUnit</skos:exactMatch>
    <skos:definition>In physics, energy is a property of objects which can be transferred to other objects or converted into different forms, but cannot be created or destroyed.  Energy, work, and heat all have identical units.</skos:definition>
    <skos:note>Has the same dimensionality as torque</skos:note>
    <skos:prefLabel>Energy</skos:prefLabel>
    <odm2:category>Space and Time</odm2:category>
    <odm2:dimensionTemperature>0</odm2:dimensionTemperature>
    <odm2:dimensionTime>1</odm2:dimensionTime>
    <skos:historyNote>QUDT</skos:historyNote>
    <odm2:dimensionCurrent>-2</odm2:dimensionCurrent>
    <odm2:defaultUnit>Joule (J)</odm2:defaultUnit>
    <odm2:dimensionMass>2</odm2:dimensionMass>
    <skos:inScheme rdf:resource="http://vocabulary.odm2.org/unitstype"/>
    <odm2:dimensionSymbol>L2M1T-2</odm2:dimensionSymbol>
    <odm2:dimensionLength>0</odm2:dimensionLength>
    <odm2:dimensionAmount>0</odm2:dimensionAmount>
    <odm2:dimensionLight>0</odm2:dimensionLight>
  </rdf:Description>
  <rdf:Description rdf:about="http://vocabulary.odm2.org/unitstype/massNormalizedParticleLoading">
    <odm2:dimensionAmount>0</odm2:dimensionAmount>
    <odm2:defaultUnit>Moles per second per kilogram (mol/s*kg)</odm2:defaultUnit>
    <odm2:dimensionSymbol>M-1T-1N1</odm2:dimensionSymbol>
    <skos:historyNote>CUAHSI</skos:historyNote>
    <odm2:dimensionCurrent>-1</odm2:dimensionCurrent>
    <odm2:dimensionLength>0</odm2:dimensionLength>
    <odm2:dimensionLight>1</odm2:dimensionLight>
    <odm2:dimensionTime>-1</odm2:dimensionTime>
    <skos:definition>The number of particles or organisms per unit time per unit mass.</skos:definition>
    <odm2:dimensionMass>0</odm2:dimensionMass>
    <skos:prefLabel>Mass normalized particle loading</skos:prefLabel>
    <odm2:category>Chemistry</odm2:category>
    <odm2:dimensionTemperature>0</odm2:dimensionTemperature>
    <rdf:type rdf:resource="http://www.w3.org/2004/02/skos/core#Concept"/>
    <skos:inScheme rdf:resource="http://vocabulary.odm2.org/unitstype"/>
  </rdf:Description>
  <rdf:Description rdf:about="http://vocabulary.odm2.org/unitstype/molarMass">
    <odm2:dimensionAmount>0</odm2:dimensionAmount>
    <odm2:dimensionLight>-1</odm2:dimensionLight>
    <odm2:dimensionCurrent>0</odm2:dimensionCurrent>
    <skos:inScheme rdf:resource="http://vocabulary.odm2.org/unitstype"/>
    <odm2:dimensionSymbol>M1N-1</odm2:dimensionSymbol>
    <skos:exactMatch>http://qudt.org/vocab/quantity#MolarMass</skos:exactMatch>
    <odm2:category>Chemistry</odm2:category>
    <odm2:dimensionTemperature>0</odm2:dimensionTemperature>
    <skos:prefLabel>Molar mass</skos:prefLabel>
    <odm2:defaultUnit>kilogram per mol (kg/mol)</odm2:defaultUnit>
    <odm2:dimensionLength>0</odm2:dimensionLength>
    <skos:note>&lt;http://dbpedia.org/resource/Molar_mass&gt;</skos:note>
    <rdf:type rdf:resource="http://www.w3.org/2004/02/skos/core#Concept"/>
    <odm2:dimensionMass>0</odm2:dimensionMass>
    <skos:historyNote>QUDT</skos:historyNote>
    <skos:definition>In chemistry, the molar mass M is a physical property defined as the mass of a given substance (chemical element or chemical compound) divided by its amount of substance.  The base SI unit for molar mass is kg/mol. However, for historical reasons, molar masses are almost always expressed in g/mol. [Wikipedia: https://en.wikipedia.org/wiki/Molar_mass]</skos:definition>
    <odm2:dimensionTime>1</odm2:dimensionTime>
  </rdf:Description>
  <rdf:Description rdf:about="http://vocabulary.odm2.org/unitstype/linearAcceleration">
    <skos:definition>Linear acceleration, in physics, is the rate at which the velocity of an object changes over time. Velocity and acceleration are vector quantities, with magnitude and direction that add according to the parallelogram law. The SI unit for acceleration is the metre per second squared (m/s2).</skos:definition>
    <odm2:dimensionLength>0</odm2:dimensionLength>
    <odm2:category>Mechanics</odm2:category>
    <odm2:dimensionAmount>0</odm2:dimensionAmount>
    <odm2:dimensionSymbol>L1T-2</odm2:dimensionSymbol>
    <skos:prefLabel>Linear acceleration</skos:prefLabel>
    <skos:note>Same dimensionality as Thrust to mass ratio</skos:note>
    <skos:historyNote>QUDT</skos:historyNote>
    <odm2:dimensionMass>1</odm2:dimensionMass>
    <rdf:type rdf:resource="http://www.w3.org/2004/02/skos/core#Concept"/>
    <skos:inScheme rdf:resource="http://vocabulary.odm2.org/unitstype"/>
    <odm2:dimensionTime>0</odm2:dimensionTime>
    <odm2:dimensionTemperature>0</odm2:dimensionTemperature>
    <odm2:defaultUnit>Meter per second squared (m/s^2)</odm2:defaultUnit>
    <odm2:dimensionLight>0</odm2:dimensionLight>
    <skos:exactMatch>http://qudt.org/vocab/quantity#Linearacceleration</skos:exactMatch>
    <odm2:dimensionCurrent>-2</odm2:dimensionCurrent>
  </rdf:Description>
  <rdf:Description rdf:about="http://vocabulary.odm2.org/unitstype/specificHeatVolume">
    <rdf:type rdf:resource="http://www.w3.org/2004/02/skos/core#Concept"/>
    <skos:prefLabel>Specific heat volume</skos:prefLabel>
    <odm2:defaultUnit>Joule per kilogram kelvin per cubic meter (J/(kg-K-m^3))</odm2:defaultUnit>
    <skos:definition>Specific heat per constant volume.</skos:definition>
    <odm2:dimensionCurrent>-2</odm2:dimensionCurrent>
    <skos:inScheme rdf:resource="http://vocabulary.odm2.org/unitstype"/>
    <odm2:dimensionMass>-1</odm2:dimensionMass>
    <odm2:dimensionTime>0</odm2:dimensionTime>
    <skos:historyNote>QUDT</skos:historyNote>
    <odm2:dimensionSymbol>L-1T-2?-1</odm2:dimensionSymbol>
    <odm2:dimensionTemperature>0</odm2:dimensionTemperature>
    <odm2:dimensionAmount>-1</odm2:dimensionAmount>
    <odm2:category>Thermodynamics</odm2:category>
    <skos:exactMatch>http://qudt.org/vocab/quantity#Specificheatvolume</skos:exactMatch>
    <odm2:dimensionLength>0</odm2:dimensionLength>
    <odm2:dimensionLight>0</odm2:dimensionLight>
  </rdf:Description>
  <rdf:Description rdf:about="http://vocabulary.odm2.org/unitstype/satelliteResolution">
    <rdf:type rdf:resource="http://www.w3.org/2004/02/skos/core#Concept"/>
    <odm2:dimensionSymbol>L1N-1</odm2:dimensionSymbol>
    <odm2:dimensionTemperature>0</odm2:dimensionTemperature>
    <skos:prefLabel>Satellite resolution</skos:prefLabel>
    <odm2:dimensionMass>1</odm2:dimensionMass>
    <odm2:dimensionAmount>0</odm2:dimensionAmount>
    <odm2:dimensionLight>-1</odm2:dimensionLight>
    <odm2:category>Space and Time</odm2:category>
    <skos:definition>In remote sensing, a satellite's resolution is defined as the size on the earth of the smallest individual component or dot (called a pixel) from which the image is constituted.  This is also reffered to as the ground sample distance.</skos:definition>
    <skos:inScheme rdf:resource="http://vocabulary.odm2.org/unitstype"/>
    <odm2:dimensionCurrent>0</odm2:dimensionCurrent>
    <odm2:dimensionTime>0</odm2:dimensionTime>
    <odm2:dimensionLength>0</odm2:dimensionLength>
    <skos:historyNote>CUAHSI</skos:historyNote>
    <odm2:defaultUnit>meter per pixel</odm2:defaultUnit>
  </rdf:Description>
  <rdf:Description rdf:about="http://vocabulary.odm2.org/unitstype/electricalCharge">
    <rdf:type rdf:resource="http://www.w3.org/2004/02/skos/core#Concept"/>
    <odm2:dimensionMass>0</odm2:dimensionMass>
    <odm2:dimensionTime>0</odm2:dimensionTime>
    <skos:definition>Electric charge is the physical property of matter that causes it to experience a force when placed in an electromagnetic field. The SI derived unit of electric charge is the coulomb (C), although in electrical engineering it is also common to use the ampere-hour (Ah), and in chemistry it is common to use the elementary charge (e) as a unit. The symbol Q is often used to denote charge. [Wikipedia: https://en.wikipedia.org/wiki/Electric_charge]</skos:definition>
    <odm2:dimensionLight>0</odm2:dimensionLight>
    <odm2:dimensionLength>0</odm2:dimensionLength>
    <odm2:dimensionSymbol>T1I1</odm2:dimensionSymbol>
    <skos:prefLabel>Electrical charge</skos:prefLabel>
    <odm2:dimensionTemperature>1</odm2:dimensionTemperature>
    <skos:historyNote>QUDT</skos:historyNote>
    <odm2:dimensionCurrent>1</odm2:dimensionCurrent>
    <skos:inScheme rdf:resource="http://vocabulary.odm2.org/unitstype"/>
    <odm2:defaultUnit>Coulomb (C)</odm2:defaultUnit>
    <odm2:category>Electricity and Magnetism</odm2:category>
    <odm2:dimensionAmount>0</odm2:dimensionAmount>
    <skos:exactMatch>http://qudt.org/vocab/quantity#ElectricCharge</skos:exactMatch>
  </rdf:Description>
  <rdf:Description rdf:about="http://vocabulary.odm2.org/unitstype/luminousEfficacy">
    <rdf:type rdf:resource="http://www.w3.org/2004/02/skos/core#Concept"/>
    <odm2:dimensionTemperature>0</odm2:dimensionTemperature>
    <odm2:dimensionCurrent>3</odm2:dimensionCurrent>
    <odm2:dimensionMass>-2</odm2:dimensionMass>
    <odm2:defaultUnit>Lumen per Watt</odm2:defaultUnit>
    <skos:inScheme rdf:resource="http://vocabulary.odm2.org/unitstype"/>
    <odm2:category>Photometry</odm2:category>
    <odm2:dimensionLight>0</odm2:dimensionLight>
    <skos:exactMatch>http://qudt.org/schema/qudt#LuminousEfficacyUnit</skos:exactMatch>
    <odm2:dimensionAmount>0</odm2:dimensionAmount>
    <skos:historyNote>QUDT</skos:historyNote>
    <odm2:dimensionLength>1</odm2:dimensionLength>
    <odm2:dimensionSymbol>U1L-2M-1T3J1</odm2:dimensionSymbol>
    <odm2:dimensionTime>-1</odm2:dimensionTime>
    <skos:prefLabel>Luminous efficacy</skos:prefLabel>
    <skos:definition>Luminous Efficacy is the ratio of luminous flux (in lumens) to power (usually measured in watts). Depending on context, the power can be either the radiant flux of the source's output, or it can be the total electric power consumed by the source.</skos:definition>
  </rdf:Description>
  <rdf:Description rdf:about="http://vocabulary.odm2.org/unitstype/energyFlux">
    <rdf:type rdf:resource="http://www.w3.org/2004/02/skos/core#Concept"/>
    <odm2:dimensionMass>0</odm2:dimensionMass>
    <odm2:dimensionTemperature>0</odm2:dimensionTemperature>
    <skos:prefLabel>Energy flux</skos:prefLabel>
    <skos:historyNote>See https://en.wikipedia.org/wiki/Energy_flux</skos:historyNote>
    <odm2:dimensionTime>0</odm2:dimensionTime>
    <odm2:dimensionCurrent>0</odm2:dimensionCurrent>
    <skos:inScheme rdf:resource="http://vocabulary.odm2.org/unitstype"/>
    <odm2:defaultUnit>W*m-2</odm2:defaultUnit>
    <odm2:dimensionAmount>0</odm2:dimensionAmount>
    <odm2:dimensionLength>0</odm2:dimensionLength>
    <odm2:dimensionLight>0</odm2:dimensionLight>
    <skos:definition>Energy flux is the rate of transfer of energy through a surface. The quantity is defined in two different ways, depending on the context.  In the first context, it is the rate of energy transfer per unit area (SI units: W·m?2 = J·m?2·s?1). This is a vector quantity, its components being determined in terms of the normal (perpendicular) direction to the surface of measurement. This is sometimes called energy flux density, to distinguish it from the second definition. Radiative flux, heat flux, and sound energy flux are specific cases of energy flux density. In the second context, it is the total rate of energy transfer (SI units: W = J·s?1). This is sometimes informally called energy current.</skos:definition>
  </rdf:Description>
  <rdf:Description rdf:about="http://vocabulary.odm2.org/unitstype/electricalResistivity">
    <odm2:dimensionLength>0</odm2:dimensionLength>
    <odm2:dimensionTemperature>-2</odm2:dimensionTemperature>
    <odm2:dimensionSymbol>L3M1I-2</odm2:dimensionSymbol>
    <odm2:dimensionLight>0</odm2:dimensionLight>
    <odm2:dimensionTime>1</odm2:dimensionTime>
    <rdf:type rdf:resource="http://www.w3.org/2004/02/skos/core#Concept"/>
    <odm2:dimensionCurrent>0</odm2:dimensionCurrent>
    <skos:exactMatch>http://dbpedia.org/page/Electrical_resistivity_and_conductivity</skos:exactMatch>
    <skos:inScheme rdf:resource="http://vocabulary.odm2.org/unitstype"/>
    <odm2:category>Electricity and Magnetism</odm2:category>
    <odm2:dimensionAmount>0</odm2:dimensionAmount>
    <odm2:defaultUnit>Ohm metres (Ohm m)</odm2:defaultUnit>
    <skos:prefLabel>Electrical resistivity</skos:prefLabel>
    <skos:definition>Electrical resistivity (also known as resistivity, specific electrical resistance, or volume resistivity) is an intrinsic property that quantifies how strongly a given material opposes the flow of electric current. A low resistivity indicates a material that readily allows the movement of electric charge. Resistivity is commonly represented by the Greek letter ? (rho). The SI unit of electrical resistivity is the ohm?metre (??m)[1][2][3] although other units like ohm?centimetre (??cm) are also in use. [Wikipedia: https://en.wikipedia.org/wiki/Electrical_resistivity_and_conductivity]</skos:definition>
    <skos:historyNote>Wikipedia</skos:historyNote>
    <odm2:dimensionMass>3</odm2:dimensionMass>
  </rdf:Description>
  <rdf:Description rdf:about="http://vocabulary.odm2.org/unitstype/particleLoading">
    <odm2:dimensionLength>0</odm2:dimensionLength>
    <odm2:dimensionSymbol>T-1N1</odm2:dimensionSymbol>
    <skos:inScheme rdf:resource="http://vocabulary.odm2.org/unitstype"/>
    <odm2:dimensionMass>0</odm2:dimensionMass>
    <odm2:dimensionAmount>0</odm2:dimensionAmount>
    <odm2:category>Chemistry</odm2:category>
    <rdf:type rdf:resource="http://www.w3.org/2004/02/skos/core#Concept"/>
    <odm2:dimensionTime>0</odm2:dimensionTime>
    <odm2:defaultUnit>Number per second (#/s)</odm2:defaultUnit>
    <odm2:dimensionCurrent>-1</odm2:dimensionCurrent>
    <skos:prefLabel>Particle loading</skos:prefLabel>
    <skos:historyNote>CUAHSI</skos:historyNote>
    <odm2:dimensionTemperature>0</odm2:dimensionTemperature>
    <skos:definition>The number of particles, organisms, or moles of substance appearing in a given amount of time.</skos:definition>
    <skos:note>Uses units that are similar, if not identical, to catalytic activity.  Both have the same dimensionality.</skos:note>
    <odm2:dimensionLight>1</odm2:dimensionLight>
  </rdf:Description>
  <rdf:Description rdf:about="http://vocabulary.odm2.org/unitstype/electricalCurrentPerEnergy">
    <odm2:dimensionTemperature>1</odm2:dimensionTemperature>
    <odm2:dimensionMass>-2</odm2:dimensionMass>
    <odm2:dimensionTime>-1</odm2:dimensionTime>
    <skos:exactMatch>http://qudt.org/vocab/quantity#Electricalcurrentperunitenergy</skos:exactMatch>
    <skos:prefLabel>Electrical current per energy</skos:prefLabel>
    <rdf:type rdf:resource="http://www.w3.org/2004/02/skos/core#Concept"/>
    <odm2:dimensionAmount>0</odm2:dimensionAmount>
    <skos:note>Has identical dimensionality to Inverse Magnetic Flux</skos:note>
    <odm2:dimensionSymbol>L-2M-1T2I1</odm2:dimensionSymbol>
    <skos:inScheme rdf:resource="http://vocabulary.odm2.org/unitstype"/>
    <odm2:defaultUnit>Ampere per Joule (A/J)</odm2:defaultUnit>
    <skos:historyNote>QUDT</skos:historyNote>
    <odm2:category>Electricity and Magnetism</odm2:category>
    <odm2:dimensionLight>0</odm2:dimensionLight>
    <odm2:dimensionCurrent>2</odm2:dimensionCurrent>
    <odm2:dimensionLength>0</odm2:dimensionLength>
  </rdf:Description>
  <rdf:Description rdf:about="http://vocabulary.odm2.org/unitstype/luminousFlux">
    <odm2:dimensionLength>1</odm2:dimensionLength>
    <skos:prefLabel>Luminous flux</skos:prefLabel>
    <odm2:dimensionMass>0</odm2:dimensionMass>
    <skos:exactMatch>http://qudt.org/vocab/quantity#Luminousflux</skos:exactMatch>
    <odm2:dimensionTime>0</odm2:dimensionTime>
    <odm2:dimensionCurrent>0</odm2:dimensionCurrent>
    <skos:inScheme rdf:resource="http://vocabulary.odm2.org/unitstype"/>
    <skos:definition>Luminous Flux or Luminous Power is the measure of the perceived power of light. It differs from radiant flux, the measure of the total power of light emitted, in that luminous flux is adjusted to reflect the varying sensitivity of the human eye to different wavelengths of light.</skos:definition>
    <skos:historyNote>QUDT</skos:historyNote>
    <odm2:category>Photometry</odm2:category>
    <odm2:dimensionAmount>0</odm2:dimensionAmount>
    <odm2:defaultUnit>Lumen (lm)</odm2:defaultUnit>
    <rdf:type rdf:resource="http://www.w3.org/2004/02/skos/core#Concept"/>
    <odm2:dimensionTemperature>0</odm2:dimensionTemperature>
    <odm2:dimensionSymbol>U1J1</odm2:dimensionSymbol>
    <odm2:dimensionLight>0</odm2:dimensionLight>
  </rdf:Description>
  <rdf:Description rdf:about="http://vocabulary.odm2.org/unitstype/radiantIntensity">
    <odm2:category>Radiology</odm2:category>
    <odm2:dimensionLength>-1</odm2:dimensionLength>
    <skos:inScheme rdf:resource="http://vocabulary.odm2.org/unitstype"/>
    <odm2:dimensionMass>2</odm2:dimensionMass>
    <odm2:dimensionAmount>0</odm2:dimensionAmount>
    <skos:exactMatch>http://qudt.org/schema/qudt#RadiantIntensityUnit</skos:exactMatch>
    <skos:prefLabel>Radiant Intensity</skos:prefLabel>
    <rdf:type rdf:resource="http://www.w3.org/2004/02/skos/core#Concept"/>
    <skos:definition>Radiant flux emitted, reflected, transmitted or received, per unit solid angle. This is a directional quantity. [Wikipedia: https://en.wikipedia.org/wiki/Radiant_intensity]</skos:definition>
    <odm2:dimensionSymbol>U-1L2M1T-3</odm2:dimensionSymbol>
    <odm2:dimensionCurrent>-3</odm2:dimensionCurrent>
    <odm2:dimensionTemperature>0</odm2:dimensionTemperature>
    <odm2:dimensionLight>0</odm2:dimensionLight>
    <odm2:defaultUnit>Watt per steradian (W/sr)</odm2:defaultUnit>
    <skos:historyNote>QUDT</skos:historyNote>
    <odm2:dimensionTime>1</odm2:dimensionTime>
  </rdf:Description>
  <rdf:Description rdf:about="http://vocabulary.odm2.org/unitstype/time">
    <odm2:category>Base Quantity</odm2:category>
    <skos:exactMatch>http://qudt.org/vocab/quantity#Time</skos:exactMatch>
    <odm2:defaultUnit>second (s)</odm2:defaultUnit>
    <odm2:dimensionSymbol>T1</odm2:dimensionSymbol>
    <odm2:dimensionAmount>0</odm2:dimensionAmount>
    <odm2:dimensionCurrent>1</odm2:dimensionCurrent>
    <odm2:dimensionTemperature>0</odm2:dimensionTemperature>
    <odm2:dimensionLength>0</odm2:dimensionLength>
    <skos:definition>Time is a basic component of the measuring system used to sequence events, to compare the durations of events and the intervals between them, and to quantify the motions of objects.</skos:definition>
    <rdf:type rdf:resource="http://www.w3.org/2004/02/skos/core#Concept"/>
    <skos:inScheme rdf:resource="http://vocabulary.odm2.org/unitstype"/>
    <skos:historyNote>QUDT</skos:historyNote>
    <odm2:dimensionLight>0</odm2:dimensionLight>
    <skos:prefLabel>Time</skos:prefLabel>
    <odm2:dimensionTime>0</odm2:dimensionTime>
    <odm2:dimensionMass>0</odm2:dimensionMass>
  </rdf:Description>
  <rdf:Description rdf:about="http://vocabulary.odm2.org/unitstype/luminousIntensity">
    <odm2:defaultUnit>Candela (cd)</odm2:defaultUnit>
    <skos:inScheme rdf:resource="http://vocabulary.odm2.org/unitstype"/>
    <rdf:type rdf:resource="http://www.w3.org/2004/02/skos/core#Concept"/>
    <odm2:dimensionTemperature>0</odm2:dimensionTemperature>
    <odm2:dimensionAmount>0</odm2:dimensionAmount>
    <odm2:dimensionSymbol>J1</odm2:dimensionSymbol>
    <skos:definition>Luminous Intensity is a measure of the wavelength-weighted power emitted by a light source in a particular direction per unit solid angle. The weighting is determined by the luminosity function, a standardized model of the sensitivity of the human eye to different wavelengths.</skos:definition>
    <odm2:dimensionMass>0</odm2:dimensionMass>
    <skos:historyNote>QUDT</skos:historyNote>
    <odm2:dimensionLight>0</odm2:dimensionLight>
    <odm2:category>Base Quantity</odm2:category>
    <skos:exactMatch>http://qudt.org/vocab/quantity#Luminousintensity</skos:exactMatch>
    <skos:prefLabel>Luminous intensity</skos:prefLabel>
    <odm2:dimensionTime>0</odm2:dimensionTime>
    <odm2:dimensionCurrent>0</odm2:dimensionCurrent>
    <odm2:dimensionLength>0</odm2:dimensionLength>
  </rdf:Description>
  <rdf:Description rdf:about="http://vocabulary.odm2.org/unitstype/force">
    <odm2:dimensionMass>1</odm2:dimensionMass>
    <odm2:dimensionAmount>0</odm2:dimensionAmount>
    <skos:historyNote>QUDT</skos:historyNote>
    <rdf:type rdf:resource="http://www.w3.org/2004/02/skos/core#Concept"/>
    <odm2:defaultUnit>Newton (N)</odm2:defaultUnit>
    <odm2:dimensionLight>0</odm2:dimensionLight>
    <skos:inScheme rdf:resource="http://vocabulary.odm2.org/unitstype"/>
    <skos:exactMatch>http://qudt.org/vocab/quantity#Force</skos:exactMatch>
    <odm2:dimensionTemperature>0</odm2:dimensionTemperature>
    <odm2:category>Mechanics</odm2:category>
    <odm2:dimensionTime>1</odm2:dimensionTime>
    <skos:definition>Force is an influence that causes mass to accelerate. It may be experienced as a lift, a push, or a pull. Force is defined by Newton's Second Law as F = m · a, where F is force, m is mass and a is acceleration. Net force is mathematically equal to the time rate of change of the momentum of the body on which it acts. Since momentum is a vector quantity (has both a magnitude and direction), force also is a vector quantity.</skos:definition>
    <skos:prefLabel>Force</skos:prefLabel>
    <odm2:dimensionCurrent>-2</odm2:dimensionCurrent>
    <odm2:dimensionSymbol>L1M1T-2</odm2:dimensionSymbol>
    <odm2:dimensionLength>0</odm2:dimensionLength>
  </rdf:Description>
  <rdf:Description rdf:about="http://vocabulary.odm2.org/unitstype/inverseLength">
    <odm2:category>Space and Time</odm2:category>
    <odm2:dimensionAmount>0</odm2:dimensionAmount>
    <skos:historyNote>QUDT</skos:historyNote>
    <skos:exactMatch>http://qudt.org/vocab/quantity#Inverselength</skos:exactMatch>
    <rdf:type rdf:resource="http://www.w3.org/2004/02/skos/core#Concept"/>
    <odm2:dimensionCurrent>0</odm2:dimensionCurrent>
    <skos:prefLabel>Inverse length</skos:prefLabel>
    <odm2:dimensionSymbol>L-1</odm2:dimensionSymbol>
    <odm2:dimensionLight>0</odm2:dimensionLight>
    <skos:inScheme rdf:resource="http://vocabulary.odm2.org/unitstype"/>
    <odm2:dimensionTime>0</odm2:dimensionTime>
    <odm2:dimensionTemperature>0</odm2:dimensionTemperature>
    <skos:definition>The inverse of length - frequently used for absorption or attenuation coefficients and wave numbers.  This can also be used to for extrinsic curvature where the unit 'diopter' is used.</skos:definition>
    <odm2:defaultUnit>per meter</odm2:defaultUnit>
    <odm2:dimensionMass>-1</odm2:dimensionMass>
    <skos:note>This should not be used for linear densities, but only for quantities with a truly dimensionless numerator. For linear densities, use "Count per length"</skos:note>
    <odm2:dimensionLength>0</odm2:dimensionLength>
  </rdf:Description>
  <rdf:Description rdf:about="http://vocabulary.odm2.org/unitstype/potentialVorticity">
    <skos:exactMatch>http://dbpedia.org/page/Potential_vorticity</skos:exactMatch>
    <odm2:category>Fluid Mechanics</odm2:category>
    <odm2:dimensionLength>0</odm2:dimensionLength>
    <odm2:dimensionSymbol>L2M-1T-1?1</odm2:dimensionSymbol>
    <odm2:dimensionMass>2</odm2:dimensionMass>
    <rdf:type rdf:resource="http://www.w3.org/2004/02/skos/core#Concept"/>
    <odm2:dimensionTemperature>0</odm2:dimensionTemperature>
    <odm2:dimensionLight>0</odm2:dimensionLight>
    <skos:historyNote>UDUnits</skos:historyNote>
    <skos:prefLabel>Potential vorticity</skos:prefLabel>
    <odm2:dimensionAmount>1</odm2:dimensionAmount>
    <skos:definition>Potential vorticity (PV) is a quantity which is proportional to the dot product of vorticity and stratification that, following a parcel of air or water, can only be changed by diabatic or frictional processes. It is a useful concept for understanding the generation of vorticity in cyclogenesis (the birth and development of a cyclone), especially along the polar front, and in analyzing flow in the ocean. [Wikipedia: https://en.wikipedia.org/wiki/Potential_vorticity]</skos:definition>
    <odm2:dimensionCurrent>-1</odm2:dimensionCurrent>
    <odm2:dimensionTime>-1</odm2:dimensionTime>
    <skos:inScheme rdf:resource="http://vocabulary.odm2.org/unitstype"/>
    <odm2:defaultUnit>Meter squared Kelvin per kilogram per second</odm2:defaultUnit>
  </rdf:Description>
  <rdf:Description rdf:about="http://vocabulary.odm2.org/unitstype/volumetricHeatCapacity">
    <odm2:dimensionTemperature>0</odm2:dimensionTemperature>
    <odm2:dimensionAmount>-1</odm2:dimensionAmount>
    <skos:prefLabel>Volumetric heat capacity</skos:prefLabel>
    <skos:historyNote>QUDT</skos:historyNote>
    <odm2:dimensionLength>0</odm2:dimensionLength>
    <odm2:defaultUnit>Joule per cubic meter kelvin (J/(m^3 K))</odm2:defaultUnit>
    <odm2:dimensionSymbol>L-1M1T-2?-1</odm2:dimensionSymbol>
    <odm2:dimensionTime>1</odm2:dimensionTime>
    <rdf:type rdf:resource="http://www.w3.org/2004/02/skos/core#Concept"/>
    <skos:exactMatch>http://qudt.org/vocab/quantity#Volumetricheatcapacity</skos:exactMatch>
    <odm2:dimensionMass>-1</odm2:dimensionMass>
    <odm2:dimensionCurrent>-2</odm2:dimensionCurrent>
    <odm2:category>Thermodynamics</odm2:category>
    <odm2:dimensionLight>0</odm2:dimensionLight>
    <skos:definition>Volumetric heat capacity (VHC), also termed volume-specific heat capacity, describes the ability of a given volume of a substance to store internal energy while undergoing a given temperature change, but without undergoing a phase transition. It is different from specific heat capacity in that the VHC is a 'per unit volume' measure of the relationship between thermal energy and temperature of a material, while the specific heat is a 'per unit mass' measure (or occasionally per molar quantity of the material).</skos:definition>
    <skos:inScheme rdf:resource="http://vocabulary.odm2.org/unitstype"/>
  </rdf:Description>
  <rdf:Description rdf:about="http://vocabulary.odm2.org/unitstype/specificVolume">
    <odm2:dimensionCurrent>0</odm2:dimensionCurrent>
    <skos:prefLabel>Specific volume</skos:prefLabel>
    <skos:definition>Specific volume (?) is the volume occupied by a unit of mass of a material. It is equal to the inverse of density.</skos:definition>
    <odm2:dimensionMass>3</odm2:dimensionMass>
    <odm2:dimensionLight>0</odm2:dimensionLight>
    <odm2:dimensionSymbol>L3M-1</odm2:dimensionSymbol>
    <odm2:dimensionLength>0</odm2:dimensionLength>
    <skos:exactMatch>http://qudt.org/vocab/quantity#Specificvolume</skos:exactMatch>
    <odm2:dimensionTime>-1</odm2:dimensionTime>
    <odm2:dimensionTemperature>0</odm2:dimensionTemperature>
    <odm2:category>Mechanics</odm2:category>
    <odm2:defaultUnit>meter cubed per kg</odm2:defaultUnit>
    <odm2:dimensionAmount>0</odm2:dimensionAmount>
    <rdf:type rdf:resource="http://www.w3.org/2004/02/skos/core#Concept"/>
    <skos:inScheme rdf:resource="http://vocabulary.odm2.org/unitstype"/>
    <skos:historyNote>QUDT</skos:historyNote>
  </rdf:Description>
  <rdf:Description rdf:about="http://vocabulary.odm2.org/unitstype/angle">
    <odm2:dimensionCurrent>0</odm2:dimensionCurrent>
    <skos:definition>In geometry, an angle (or plane angle) is the figure formed by two rays or line segments, called the sides of the angle, sharing a common endpoint, called the vertex of the angle. Euclid defines a plane angle as the inclination to each other, in a plane, of two lines which meet each other, and do not lie straight with respect to each other.</skos:definition>
    <odm2:defaultUnit>Radian (rad)</odm2:defaultUnit>
    <odm2:dimensionLight>0</odm2:dimensionLight>
    <odm2:dimensionMass>0</odm2:dimensionMass>
    <skos:prefLabel>Angle</skos:prefLabel>
    <odm2:category>Space and Time</odm2:category>
    <odm2:dimensionTemperature>0</odm2:dimensionTemperature>
    <odm2:dimensionSymbol>U1</odm2:dimensionSymbol>
    <skos:exactMatch>http://qudt.org/vocab/quantity#Angle</skos:exactMatch>
    <odm2:dimensionAmount>0</odm2:dimensionAmount>
    <rdf:type rdf:resource="http://www.w3.org/2004/02/skos/core#Concept"/>
    <odm2:dimensionLength>1</odm2:dimensionLength>
    <skos:inScheme rdf:resource="http://vocabulary.odm2.org/unitstype"/>
    <skos:historyNote>QUDT</skos:historyNote>
    <odm2:dimensionTime>0</odm2:dimensionTime>
  </rdf:Description>
  <rdf:Description rdf:about="http://vocabulary.odm2.org/unitstype/dataRate">
    <odm2:category>Information</odm2:category>
    <odm2:dimensionCurrent>-1</odm2:dimensionCurrent>
    <odm2:defaultUnit>Bits per Second (pbs)</odm2:defaultUnit>
    <odm2:dimensionAmount>0</odm2:dimensionAmount>
    <odm2:dimensionMass>0</odm2:dimensionMass>
    <odm2:dimensionTemperature>0</odm2:dimensionTemperature>
    <skos:exactMatch>http://qudt.org/schema/qudt#DataRateUnit</skos:exactMatch>
    <rdf:type rdf:resource="http://www.w3.org/2004/02/skos/core#Concept"/>
    <skos:inScheme rdf:resource="http://vocabulary.odm2.org/unitstype"/>
    <skos:historyNote>QUDT</skos:historyNote>
    <odm2:dimensionLight>0</odm2:dimensionLight>
    <odm2:dimensionLength>1</odm2:dimensionLength>
    <skos:definition>The frequency derived from the period of time required to transmit one bit. This represents the amount of data transferred per second by a communications channel or a computing or storage device. Data rate is measured in units of bits per second (written "b/s" or "bps"), bytes per second (Bps), or baud. When applied to data rate, the multiplier prefixes "kilo-", "mega-", "giga-", etc. (and their abbreviations, "k", "M", "G", etc.) always denote powers of 1000. For example, 64 kbps is 64,000 bits per second. This contrasts with units of storage which use different prefixes to denote multiplication by powers of 1024, e.g. 1 kibibit = 1024 bits.</skos:definition>
    <odm2:dimensionSymbol>U1T-1</odm2:dimensionSymbol>
    <odm2:dimensionTime>0</odm2:dimensionTime>
    <skos:prefLabel>Data rate</skos:prefLabel>
  </rdf:Description>
  <rdf:Description rdf:about="http://vocabulary.odm2.org/unitstype/molarEnergy">
    <odm2:dimensionLight>-1</odm2:dimensionLight>
    <skos:prefLabel>Molar energy</skos:prefLabel>
    <odm2:dimensionSymbol>L2M1T-2N-1</odm2:dimensionSymbol>
    <odm2:dimensionTemperature>0</odm2:dimensionTemperature>
    <skos:exactMatch>http://qudt.org/schema/qudt#MolarEnergyUnit</skos:exactMatch>
    <odm2:dimensionTime>1</odm2:dimensionTime>
    <skos:definition>The amount of energy per mole of substance</skos:definition>
    <odm2:dimensionLength>0</odm2:dimensionLength>
    <odm2:dimensionCurrent>-2</odm2:dimensionCurrent>
    <odm2:defaultUnit>Joule per mole (J/mol)</odm2:defaultUnit>
    <odm2:dimensionAmount>0</odm2:dimensionAmount>
    <rdf:type rdf:resource="http://www.w3.org/2004/02/skos/core#Concept"/>
    <odm2:category>Chemistry</odm2:category>
    <odm2:dimensionMass>2</odm2:dimensionMass>
    <skos:inScheme rdf:resource="http://vocabulary.odm2.org/unitstype"/>
    <skos:historyNote>QUDT</skos:historyNote>
  </rdf:Description>
  <rdf:Description rdf:about="http://vocabulary.odm2.org/unitstype/electricalPermittivity">
    <skos:definition>In electromagnetism, absolute permittivity is the measure of the resistance that is encountered when forming an electric field in a medium. In other words, permittivity is a measure of how an electric field affects, and is affected by, a dielectric medium. The permittivity of a medium describes how much electric field (more correctly, flux) is 'generated' per unit charge in that medium. More electric flux exists in a medium with a low permittivity (per unit charge) because of polarization effects. Permittivity is directly related to electric susceptibility, which is a measure of how easily a dielectric polarizes in response to an electric field. Thus, permittivity relates to a material's ability to resist an electric field and "permit" is a misnomer.  In SI units, permittivity ? is measured in farads per meter (F/m)</skos:definition>
    <skos:inScheme rdf:resource="http://vocabulary.odm2.org/unitstype"/>
    <skos:prefLabel>Electrical permittivity</skos:prefLabel>
    <odm2:defaultUnit>Farad per meter (F/m)</odm2:defaultUnit>
    <odm2:dimensionTime>-1</odm2:dimensionTime>
    <rdf:type rdf:resource="http://www.w3.org/2004/02/skos/core#Concept"/>
    <odm2:dimensionAmount>0</odm2:dimensionAmount>
    <odm2:dimensionSymbol>L-3M-1T4I2</odm2:dimensionSymbol>
    <skos:historyNote>QUDT</skos:historyNote>
    <odm2:dimensionTemperature>2</odm2:dimensionTemperature>
    <odm2:dimensionCurrent>4</odm2:dimensionCurrent>
    <odm2:dimensionMass>-3</odm2:dimensionMass>
    <skos:exactMatch>http://qudt.org/vocab/quantity#Permittivity</skos:exactMatch>
    <odm2:category>Electricity and Magnetism</odm2:category>
    <odm2:dimensionLight>0</odm2:dimensionLight>
    <odm2:dimensionLength>0</odm2:dimensionLength>
  </rdf:Description>
  <rdf:Description rdf:about="http://vocabulary.odm2.org/unitstype/molarVolume">
    <odm2:dimensionLight>-1</odm2:dimensionLight>
    <skos:prefLabel>Molar volume</skos:prefLabel>
    <odm2:category>Chemistry</odm2:category>
    <rdf:type rdf:resource="http://www.w3.org/2004/02/skos/core#Concept"/>
    <odm2:dimensionMass>3</odm2:dimensionMass>
    <odm2:dimensionTime>0</odm2:dimensionTime>
    <odm2:dimensionTemperature>0</odm2:dimensionTemperature>
    <skos:definition>The molar volume, symbol Vm, is the volume occupied by one mole of a substance (chemical element or chemical compound) at a given temperature and pressure. It is equal to the molar mass (M) divided by the mass density (?). [Wikipedia: https://en.wikipedia.org/wiki/Molar_volume]</skos:definition>
    <skos:inScheme rdf:resource="http://vocabulary.odm2.org/unitstype"/>
    <skos:historyNote>New for ODM2</skos:historyNote>
    <odm2:dimensionCurrent>0</odm2:dimensionCurrent>
    <odm2:dimensionAmount>0</odm2:dimensionAmount>
    <odm2:dimensionSymbol>L3N-1</odm2:dimensionSymbol>
    <odm2:dimensionLength>0</odm2:dimensionLength>
    <odm2:defaultUnit>cubic meters per mol (m^3/mol)</odm2:defaultUnit>
    <skos:exactMatch>http://dbpedia.org/page/Molar_volume</skos:exactMatch>
  </rdf:Description>
  <rdf:Description rdf:about="http://vocabulary.odm2.org/unitstype/countPerLength">
    <skos:inScheme rdf:resource="http://vocabulary.odm2.org/unitstype"/>
    <odm2:dimensionTime>0</odm2:dimensionTime>
    <odm2:dimensionAmount>0</odm2:dimensionAmount>
    <odm2:dimensionLight>1</odm2:dimensionLight>
    <skos:historyNote>Aquarius</skos:historyNote>
    <odm2:category>Space and Time</odm2:category>
    <odm2:dimensionTemperature>0</odm2:dimensionTemperature>
    <odm2:dimensionMass>-1</odm2:dimensionMass>
    <odm2:dimensionSymbol>L-1N1</odm2:dimensionSymbol>
    <odm2:dimensionLength>0</odm2:dimensionLength>
    <odm2:defaultUnit>Count per meter (#/m)</odm2:defaultUnit>
    <skos:prefLabel>Count per length</skos:prefLabel>
    <rdf:type rdf:resource="http://www.w3.org/2004/02/skos/core#Concept"/>
    <odm2:dimensionCurrent>0</odm2:dimensionCurrent>
    <skos:definition>The length density of a given amount of a substance.  This unit group is also used for image and TV resolutions measured in lines.  This is distinct from "inverse length" in that there is something specific being counted per unit length, that is, the numerator is not dimensionless.</skos:definition>
  </rdf:Description>
  <rdf:Description rdf:about="http://vocabulary.odm2.org/unitstype/dimensionless">
    <odm2:dimensionCurrent>0</odm2:dimensionCurrent>
    <skos:inScheme rdf:resource="http://vocabulary.odm2.org/unitstype"/>
    <skos:exactMatch>http://qudt.org/schema/qudt#DimensionlessUnit</skos:exactMatch>
    <odm2:dimensionMass>0</odm2:dimensionMass>
    <odm2:dimensionAmount>0</odm2:dimensionAmount>
    <skos:definition>Any unit or combination of units that has no dimensions.  A Dimensionless Unit is a quantity for which all the exponents of the factors corresponding to the base quantities in its quantity dimension are zero.</skos:definition>
    <odm2:defaultUnit>unitless</odm2:defaultUnit>
    <odm2:dimensionLength>1</odm2:dimensionLength>
    <odm2:dimensionSymbol>U1</odm2:dimensionSymbol>
    <rdf:type rdf:resource="http://www.w3.org/2004/02/skos/core#Concept"/>
    <odm2:category>Dimensionless</odm2:category>
    <odm2:dimensionTime>0</odm2:dimensionTime>
    <skos:prefLabel>Dimensionless</skos:prefLabel>
    <odm2:dimensionLight>0</odm2:dimensionLight>
    <odm2:dimensionTemperature>0</odm2:dimensionTemperature>
    <skos:historyNote>QUDT</skos:historyNote>
  </rdf:Description>
  <rdf:Description rdf:about="http://vocabulary.odm2.org/unitstype/inverseSquareEnergy">
    <skos:inScheme rdf:resource="http://vocabulary.odm2.org/unitstype"/>
    <odm2:dimensionSymbol>L-4M-2T4</odm2:dimensionSymbol>
    <rdf:type rdf:resource="http://www.w3.org/2004/02/skos/core#Concept"/>
    <odm2:dimensionTemperature>0</odm2:dimensionTemperature>
    <odm2:dimensionTime>-2</odm2:dimensionTime>
    <skos:prefLabel>Inverse square energy</skos:prefLabel>
    <odm2:dimensionCurrent>4</odm2:dimensionCurrent>
    <odm2:dimensionLength>0</odm2:dimensionLength>
    <odm2:category>Mechanics</odm2:category>
    <odm2:dimensionAmount>0</odm2:dimensionAmount>
    <skos:exactMatch>http://qudt.org/vocab/quantity#Inversesquareenergy</skos:exactMatch>
    <odm2:dimensionLight>0</odm2:dimensionLight>
    <skos:historyNote>QUDT</skos:historyNote>
    <odm2:defaultUnit>per square Joule (J-2)</odm2:defaultUnit>
    <odm2:dimensionMass>-4</odm2:dimensionMass>
  </rdf:Description>
  <rdf:Description rdf:about="http://vocabulary.odm2.org/unitstype/standardGravitationalParameter">
    <rdf:type rdf:resource="http://www.w3.org/2004/02/skos/core#Concept"/>
    <odm2:dimensionLight>0</odm2:dimensionLight>
    <odm2:dimensionCurrent>-2</odm2:dimensionCurrent>
    <odm2:dimensionMass>3</odm2:dimensionMass>
    <odm2:dimensionTime>0</odm2:dimensionTime>
    <odm2:defaultUnit>Cubic Meter per Second Squared</odm2:defaultUnit>
    <skos:inScheme rdf:resource="http://vocabulary.odm2.org/unitstype"/>
    <skos:prefLabel>Standard gravitational parameter</skos:prefLabel>
    <odm2:dimensionTemperature>0</odm2:dimensionTemperature>
    <odm2:dimensionSymbol>L3T-2</odm2:dimensionSymbol>
    <skos:historyNote>QUDT</skos:historyNote>
    <skos:definition>In celestial mechanics, the standard gravitational parameter ? of a celestial body is the product of the gravitational constant G and the mass M of the body. [Wikipedia: https://en.wikipedia.org/wiki/Standard_gravitational_parameter]</skos:definition>
    <odm2:category>Mechanics</odm2:category>
    <odm2:dimensionLength>0</odm2:dimensionLength>
    <skos:exactMatch>http://qudt.org/vocab/quantity#StandardGravitationalParameter</skos:exactMatch>
    <skos:note>&lt;http://dbpedia.org/resource/Standard_gravitational_parameter&gt;</skos:note>
    <odm2:dimensionAmount>0</odm2:dimensionAmount>
  </rdf:Description>
  <rdf:Description rdf:about="http://vocabulary.odm2.org/unitstype/electricalFieldStrength">
    <odm2:dimensionMass>1</odm2:dimensionMass>
    <odm2:dimensionTemperature>-1</odm2:dimensionTemperature>
    <odm2:dimensionLight>0</odm2:dimensionLight>
    <skos:exactMatch>http://qudt.org/schema/qudt#ElectricFieldStrengthUnit</skos:exactMatch>
    <skos:inScheme rdf:resource="http://vocabulary.odm2.org/unitstype"/>
    <rdf:type rdf:resource="http://www.w3.org/2004/02/skos/core#Concept"/>
    <odm2:dimensionTime>1</odm2:dimensionTime>
    <skos:definition>The strength of the electric field at a given point is defined as the force that would be exerted on a positive test charge of +1 coulomb placed at that point; the direction of the field is given by the direction of that force. Electric fields contain electrical energy with energy density proportional to the square of the field intensity. The electric field is to charge as gravitational acceleration is to mass and force density is to volume.</skos:definition>
    <odm2:category>Electricity and Magnetism</odm2:category>
    <odm2:defaultUnit>Volt per Meter (V/m) or Newton per coulomb (N/C)</odm2:defaultUnit>
    <skos:prefLabel>Electrical field strength</skos:prefLabel>
    <odm2:dimensionAmount>0</odm2:dimensionAmount>
    <skos:historyNote>QUDT</skos:historyNote>
    <odm2:dimensionLength>0</odm2:dimensionLength>
    <odm2:dimensionSymbol>L1M1T-3I-1</odm2:dimensionSymbol>
    <odm2:dimensionCurrent>-3</odm2:dimensionCurrent>
  </rdf:Description>
  <rdf:Description rdf:about="http://vocabulary.odm2.org/unitstype/inverseVolume">
    <skos:note>This should only be used for quantities with a truly dimensionless numerator. For other concentrations and densities, use "Concentration count per volume."</skos:note>
    <skos:historyNote>QUDT</skos:historyNote>
    <odm2:dimensionLight>0</odm2:dimensionLight>
    <odm2:dimensionTemperature>0</odm2:dimensionTemperature>
    <odm2:dimensionSymbol>L-3</odm2:dimensionSymbol>
    <odm2:dimensionMass>-3</odm2:dimensionMass>
    <skos:prefLabel>Inverse volume</skos:prefLabel>
    <odm2:dimensionCurrent>0</odm2:dimensionCurrent>
    <odm2:dimensionLength>0</odm2:dimensionLength>
    <skos:inScheme rdf:resource="http://vocabulary.odm2.org/unitstype"/>
    <skos:exactMatch>http://qudt.org/vocab/quantity#Inversevolume</skos:exactMatch>
    <rdf:type rdf:resource="http://www.w3.org/2004/02/skos/core#Concept"/>
    <odm2:dimensionAmount>0</odm2:dimensionAmount>
    <odm2:defaultUnit>per cubic meter</odm2:defaultUnit>
    <odm2:category>Space and Time</odm2:category>
    <odm2:dimensionTime>0</odm2:dimensionTime>
  </rdf:Description>
  <rdf:Description rdf:about="http://vocabulary.odm2.org/unitstype/concentrationCountPerMass">
    <odm2:dimensionLength>0</odm2:dimensionLength>
    <odm2:dimensionAmount>0</odm2:dimensionAmount>
    <skos:prefLabel>Concentration count per mass</skos:prefLabel>
    <skos:historyNote>QUDT</skos:historyNote>
    <rdf:type rdf:resource="http://www.w3.org/2004/02/skos/core#Concept"/>
    <odm2:dimensionCurrent>0</odm2:dimensionCurrent>
    <skos:exactMatch>http://qudt.org/vocab/quantity#AmountOfSubstancePerUnitMass; http://dbpedia.org/page/Molality</skos:exactMatch>
    <odm2:dimensionSymbol>M-1N1</odm2:dimensionSymbol>
    <skos:inScheme rdf:resource="http://vocabulary.odm2.org/unitstype"/>
    <odm2:defaultUnit>molal (moles per kg)</odm2:defaultUnit>
    <odm2:dimensionLight>1</odm2:dimensionLight>
    <odm2:dimensionTemperature>0</odm2:dimensionTemperature>
    <odm2:dimensionMass>0</odm2:dimensionMass>
    <odm2:category>Chemistry</odm2:category>
    <odm2:dimensionTime>-1</odm2:dimensionTime>
    <skos:definition>Amount of substance or a count/number of items per unit mass.  This is most often called molality or molal concentration. This contrasts with the definition of molarity which is based on a specified volume of solution. A commonly used unit for molality used in chemistry is mol/kg. A solution of concentration 1 mol/kg is also sometimes denoted as 1 molal.</skos:definition>
  </rdf:Description>
  <rdf:Description rdf:about="http://vocabulary.odm2.org/unitstype/turbidity">
    <odm2:defaultUnit>Nephelometric Turbidity Units (NTU)</odm2:defaultUnit>
    <odm2:dimensionAmount>0</odm2:dimensionAmount>
    <skos:prefLabel>Turbidity</skos:prefLabel>
    <odm2:dimensionTime>0</odm2:dimensionTime>
    <skos:inScheme rdf:resource="http://vocabulary.odm2.org/unitstype"/>
    <odm2:category>Chemistry</odm2:category>
    <odm2:dimensionCurrent>0</odm2:dimensionCurrent>
    <skos:definition>Turbidity is the cloudiness or haziness of a fluid, or of air, caused by individual particles (suspended solids) that are generally invisible to the naked eye, similar to smoke in air. Turbidity in open water is often caused by phytoplankton and the measurement of turbidity is a key test of water quality. The higher the turbidity, the higher the risk of the drinkers developing gastrointestinal diseases, especially for immune-compromised people, because contaminants like virus or bacteria can become attached to the suspended solid. The suspended solids interfere with water disinfection with chlorine because the particles act as shields for the virus and bacteria. Similarly suspended solids can protect bacteria from UV sterilisation of water. Fluids can contain suspended solid matter consisting of particles of many different sizes. While some suspended material will be large enough and heavy enough to settle rapidly to the bottom container if a liquid sample is left to stand (the settleable solids), very small particles will settle only very slowly or not at all if the sample is regularly agitated or the particles are colloidal. These small solid particles cause the liquid to appear turbid.</skos:definition>
    <odm2:dimensionSymbol>U1</odm2:dimensionSymbol>
    <odm2:dimensionLength>1</odm2:dimensionLength>
    <odm2:dimensionMass>0</odm2:dimensionMass>
    <odm2:dimensionLight>0</odm2:dimensionLight>
    <skos:historyNote>QUDT</skos:historyNote>
    <odm2:dimensionTemperature>0</odm2:dimensionTemperature>
    <skos:exactMatch>http://qudt.org/vocab/quantity#Turbidity</skos:exactMatch>
    <rdf:type rdf:resource="http://www.w3.org/2004/02/skos/core#Concept"/>
  </rdf:Description>
  <rdf:Description rdf:about="http://vocabulary.odm2.org/unitstype/thrustToMassRatio">
    <odm2:category>Mechanics</odm2:category>
    <skos:historyNote>QUDT</skos:historyNote>
    <odm2:dimensionSymbol>L1T-2</odm2:dimensionSymbol>
    <odm2:dimensionTemperature>0</odm2:dimensionTemperature>
    <odm2:dimensionLight>0</odm2:dimensionLight>
    <skos:note>Same dimensionality as linear accelleration</skos:note>
    <skos:exactMatch>http://qudt.org/vocab/quantity#ThrustToMassRatio</skos:exactMatch>
    <skos:prefLabel>Thrust to mass ratio</skos:prefLabel>
    <odm2:dimensionLength>0</odm2:dimensionLength>
    <skos:inScheme rdf:resource="http://vocabulary.odm2.org/unitstype"/>
    <odm2:dimensionMass>1</odm2:dimensionMass>
    <rdf:type rdf:resource="http://www.w3.org/2004/02/skos/core#Concept"/>
    <odm2:dimensionAmount>0</odm2:dimensionAmount>
    <odm2:defaultUnit>Newton per kilogram (N/kg)</odm2:defaultUnit>
    <skos:definition>Thrust-to-weight ratio is a dimensionless ratio of thrust to weight of a rocket, jet engine, propeller engine, or a vehicle propelled by such an engine that indicates the performance of the engine or vehicle. [Wikipedia: https://en.wikipedia.org/wiki/Thrust-to-weight_ratio]</skos:definition>
    <odm2:dimensionCurrent>-2</odm2:dimensionCurrent>
    <odm2:dimensionTime>0</odm2:dimensionTime>
  </rdf:Description>
  <rdf:Description rdf:about="http://vocabulary.odm2.org/unitstype/radioactivityPerVolume">
    <odm2:dimensionCurrent>-1</odm2:dimensionCurrent>
    <odm2:dimensionTemperature>0</odm2:dimensionTemperature>
    <skos:historyNote>New for ODM2</skos:historyNote>
    <odm2:dimensionAmount>0</odm2:dimensionAmount>
    <odm2:dimensionTime>0</odm2:dimensionTime>
    <odm2:dimensionSymbol>L-3T-1</odm2:dimensionSymbol>
    <odm2:defaultUnit>Becquerels per meter cubed (Bq/m^3)</odm2:defaultUnit>
    <odm2:category>Quantum Mechanics</odm2:category>
    <skos:definition>The amount of radioactivity per unit volume</skos:definition>
    <rdf:type rdf:resource="http://www.w3.org/2004/02/skos/core#Concept"/>
    <skos:prefLabel>Radioactivity per volume</skos:prefLabel>
    <odm2:dimensionMass>-3</odm2:dimensionMass>
    <odm2:dimensionLight>0</odm2:dimensionLight>
    <skos:inScheme rdf:resource="http://vocabulary.odm2.org/unitstype"/>
    <odm2:dimensionLength>0</odm2:dimensionLength>
  </rdf:Description>
  <rdf:Description rdf:about="http://vocabulary.odm2.org/unitstype/pressureOrStressRate">
    <odm2:dimensionMass>-1</odm2:dimensionMass>
    <odm2:dimensionTime>1</odm2:dimensionTime>
    <skos:exactMatch>http://qudt.org/schema/qudt#PressureOrStressRateUnit</skos:exactMatch>
    <odm2:dimensionAmount>0</odm2:dimensionAmount>
    <odm2:dimensionLight>0</odm2:dimensionLight>
    <odm2:dimensionCurrent>-3</odm2:dimensionCurrent>
    <odm2:dimensionLength>0</odm2:dimensionLength>
    <odm2:dimensionTemperature>0</odm2:dimensionTemperature>
    <skos:inScheme rdf:resource="http://vocabulary.odm2.org/unitstype"/>
    <skos:historyNote>QUDT</skos:historyNote>
    <odm2:dimensionSymbol>L-1M1T-3</odm2:dimensionSymbol>
    <odm2:defaultUnit>Pascal per second (Pa/s)</odm2:defaultUnit>
    <rdf:type rdf:resource="http://www.w3.org/2004/02/skos/core#Concept"/>
    <odm2:category>Space and Time</odm2:category>
    <skos:prefLabel>Pressure or stress rate</skos:prefLabel>
  </rdf:Description>
  <rdf:Description rdf:about="http://vocabulary.odm2.org/unitstype/other">
    <skos:prefLabel>Other</skos:prefLabel>
    <rdf:type rdf:resource="http://www.w3.org/2004/02/skos/core#Concept"/>
    <odm2:dimensionCurrent>0</odm2:dimensionCurrent>
    <odm2:category>Dimensionless</odm2:category>
    <skos:inScheme rdf:resource="http://vocabulary.odm2.org/unitstype"/>
    <odm2:dimensionTime>0</odm2:dimensionTime>
    <skos:note>Catch-all for units I don't know how to deal with</skos:note>
    <odm2:dimensionTemperature>0</odm2:dimensionTemperature>
    <odm2:dimensionLength>0</odm2:dimensionLength>
    <odm2:dimensionMass>0</odm2:dimensionMass>
    <skos:historyNote>New for ODM2</skos:historyNote>
    <odm2:dimensionAmount>0</odm2:dimensionAmount>
    <odm2:dimensionLight>0</odm2:dimensionLight>
    <skos:definition>A unit that does not belong in any of the other groups.  These units have dimensionality, but are generally strangely compounded or calculated</skos:definition>
  </rdf:Description>
  <rdf:Description rdf:about="http://vocabulary.odm2.org/unitstype/massCount">
    <skos:prefLabel>Mass count</skos:prefLabel>
    <odm2:dimensionCurrent>0</odm2:dimensionCurrent>
    <odm2:category>Chemistry</odm2:category>
    <rdf:type rdf:resource="http://www.w3.org/2004/02/skos/core#Concept"/>
    <odm2:dimensionAmount>0</odm2:dimensionAmount>
    <skos:exactMatch>http://qudt.org/vocab/quantity#MassAmountOfSubstance</skos:exactMatch>
    <odm2:dimensionMass>0</odm2:dimensionMass>
    <odm2:dimensionTemperature>0</odm2:dimensionTemperature>
    <odm2:defaultUnit>kilogram mole (kg*mol)</odm2:defaultUnit>
    <odm2:dimensionTime>1</odm2:dimensionTime>
    <odm2:dimensionSymbol>M1N1</odm2:dimensionSymbol>
    <skos:historyNote>QUDT</skos:historyNote>
    <odm2:dimensionLength>0</odm2:dimensionLength>
    <skos:inScheme rdf:resource="http://vocabulary.odm2.org/unitstype"/>
    <odm2:dimensionLight>1</odm2:dimensionLight>
  </rdf:Description>
  <rdf:Description rdf:about="http://vocabulary.odm2.org/unitstype/powerArea">
    <odm2:defaultUnit>Watt Square Meter</odm2:defaultUnit>
    <skos:exactMatch>http://qudt.org/vocab/quantity#PowerArea</skos:exactMatch>
    <odm2:dimensionTemperature>0</odm2:dimensionTemperature>
    <odm2:dimensionTime>1</odm2:dimensionTime>
    <skos:historyNote>QUDT</skos:historyNote>
    <odm2:dimensionLength>0</odm2:dimensionLength>
    <odm2:dimensionMass>4</odm2:dimensionMass>
    <skos:inScheme rdf:resource="http://vocabulary.odm2.org/unitstype"/>
    <odm2:dimensionSymbol>L4M1T-3</odm2:dimensionSymbol>
    <odm2:dimensionCurrent>-3</odm2:dimensionCurrent>
    <odm2:dimensionAmount>0</odm2:dimensionAmount>
    <skos:prefLabel>Power area</skos:prefLabel>
    <odm2:dimensionLight>0</odm2:dimensionLight>
    <rdf:type rdf:resource="http://www.w3.org/2004/02/skos/core#Concept"/>
    <odm2:category>Mechanics</odm2:category>
  </rdf:Description>
  <rdf:Description rdf:about="http://vocabulary.odm2.org/unitstype/solidAngle">
    <rdf:type rdf:resource="http://www.w3.org/2004/02/skos/core#Concept"/>
    <odm2:dimensionMass>0</odm2:dimensionMass>
    <odm2:dimensionSymbol>U1</odm2:dimensionSymbol>
    <odm2:dimensionCurrent>0</odm2:dimensionCurrent>
    <skos:prefLabel>Solid angle</skos:prefLabel>
    <odm2:category>Space and Time</odm2:category>
    <skos:inScheme rdf:resource="http://vocabulary.odm2.org/unitstype"/>
    <odm2:dimensionTime>0</odm2:dimensionTime>
    <skos:historyNote>QUDT</skos:historyNote>
    <odm2:dimensionTemperature>0</odm2:dimensionTemperature>
    <skos:definition>The solid angle subtended by a surface S is defined as the surface area of a unit sphere covered by the surface S's projection onto the sphere. A solid angle is related to the surface of a sphere in the same way an ordinary angle is related to the circumference of a circle. Since the total surface area of the unit sphere is 4*pi, the measure of solid angle will always be between 0 and 4*pi.</skos:definition>
    <odm2:dimensionLength>1</odm2:dimensionLength>
    <skos:exactMatch>http://qudt.org/vocab/quantity#Solidangle</skos:exactMatch>
    <odm2:dimensionAmount>0</odm2:dimensionAmount>
    <odm2:dimensionLight>0</odm2:dimensionLight>
    <odm2:defaultUnit>Steradian (sr)</odm2:defaultUnit>
  </rdf:Description>
  <rdf:Description rdf:about="http://vocabulary.odm2.org/unitstype/linearThermalExpansion">
    <skos:inScheme rdf:resource="http://vocabulary.odm2.org/unitstype"/>
    <odm2:dimensionCurrent>0</odm2:dimensionCurrent>
    <rdf:type rdf:resource="http://www.w3.org/2004/02/skos/core#Concept"/>
    <odm2:dimensionAmount>-1</odm2:dimensionAmount>
    <skos:exactMatch>http://qudt.org/vocab/quantity#Linearthermalexpansion</skos:exactMatch>
    <odm2:dimensionTemperature>0</odm2:dimensionTemperature>
    <odm2:dimensionTime>0</odm2:dimensionTime>
    <odm2:defaultUnit>Meter per kelvin (m/K)</odm2:defaultUnit>
    <skos:historyNote>QUDT</skos:historyNote>
    <skos:prefLabel>Linear thermal expansion</skos:prefLabel>
    <odm2:dimensionMass>1</odm2:dimensionMass>
    <odm2:dimensionSymbol>L1?-1</odm2:dimensionSymbol>
    <odm2:dimensionLight>0</odm2:dimensionLight>
    <odm2:category>Thermodynamics</odm2:category>
    <odm2:dimensionLength>0</odm2:dimensionLength>
    <skos:definition>When the temperature of a substance changes, the energy that is stored in the intermolecular bonds between atoms changes. When the stored energy increases, so does the length of the molecular bonds. As a result, solids typically expand in response to heating and contract on cooling; this dimensional response to temperature change is expressed by its coefficient of thermal expansion. Different coefficients of thermal expansion can be defined for a substance depending on whether the expansion is measured by: * linear thermal expansion * area thermal expansion * volumetric thermal expansion These characteristics are closely related. The volumetric thermal expansion coefficient can be defined for both liquids and solids. The linear thermal expansion can only be defined for solids, and is common in engineering applications. Some substances expand when cooled, such as freezing water, so they have negative thermal expansion coefficients. [Wikipedia: https://en.wikipedia.org/wiki/Thermal_expansion]</skos:definition>
  </rdf:Description>
  <rdf:Description rdf:about="http://vocabulary.odm2.org/unitstype/power">
    <odm2:dimensionTemperature>0</odm2:dimensionTemperature>
    <odm2:dimensionTime>1</odm2:dimensionTime>
    <odm2:dimensionLength>0</odm2:dimensionLength>
    <skos:inScheme rdf:resource="http://vocabulary.odm2.org/unitstype"/>
    <rdf:type rdf:resource="http://www.w3.org/2004/02/skos/core#Concept"/>
    <odm2:dimensionMass>2</odm2:dimensionMass>
    <skos:exactMatch>http://qudt.org/vocab/quantity#Power</skos:exactMatch>
    <odm2:dimensionLight>0</odm2:dimensionLight>
    <skos:historyNote>QUDT</skos:historyNote>
    <odm2:dimensionSymbol>L2M1T-3</odm2:dimensionSymbol>
    <odm2:category>Mechanics</odm2:category>
    <skos:definition>Power is the rate at which work is performed or energy is transmitted, or the amount of energy required or expended for a given unit of time. As a rate of change of work done or the energy of a subsystem, power is: P = W/t where P is power W is work t is time.  Heat flow rate follows identical units to Power</skos:definition>
    <skos:prefLabel>Power</skos:prefLabel>
    <odm2:defaultUnit>Watt (W)</odm2:defaultUnit>
    <odm2:dimensionCurrent>-3</odm2:dimensionCurrent>
    <odm2:dimensionAmount>0</odm2:dimensionAmount>
  </rdf:Description>
  <rdf:Description rdf:about="http://vocabulary.odm2.org/unitstype/area">
    <odm2:dimensionTemperature>0</odm2:dimensionTemperature>
    <odm2:defaultUnit>Square meter (m^2)</odm2:defaultUnit>
    <skos:definition>Area is a quantity expressing the two-dimensional size of a defined part of a surface, typically a region bounded by a closed curve.</skos:definition>
    <skos:historyNote>QUDT</skos:historyNote>
    <odm2:dimensionTime>0</odm2:dimensionTime>
    <skos:exactMatch>http://qudt.org/vocab/quantity#Area</skos:exactMatch>
    <odm2:dimensionLight>0</odm2:dimensionLight>
    <odm2:dimensionAmount>0</odm2:dimensionAmount>
    <skos:prefLabel>Area</skos:prefLabel>
    <odm2:dimensionMass>2</odm2:dimensionMass>
    <odm2:dimensionLength>0</odm2:dimensionLength>
    <odm2:dimensionSymbol>L2</odm2:dimensionSymbol>
    <odm2:category>Space and Time</odm2:category>
    <rdf:type rdf:resource="http://www.w3.org/2004/02/skos/core#Concept"/>
    <odm2:dimensionCurrent>0</odm2:dimensionCurrent>
    <skos:inScheme rdf:resource="http://vocabulary.odm2.org/unitstype"/>
  </rdf:Description>
  <rdf:Description rdf:about="http://vocabulary.odm2.org/unitstype/lengthFraction">
    <odm2:dimensionAmount>0</odm2:dimensionAmount>
    <odm2:category>Space and Time</odm2:category>
    <odm2:dimensionMass>0</odm2:dimensionMass>
    <odm2:dimensionTemperature>0</odm2:dimensionTemperature>
    <skos:definition>The ratio or two lengths, often used to measure slope or scale.</skos:definition>
    <odm2:dimensionLength>0</odm2:dimensionLength>
    <odm2:dimensionTime>0</odm2:dimensionTime>
    <odm2:dimensionSymbol>L1L-1</odm2:dimensionSymbol>
    <odm2:defaultUnit>unitless</odm2:defaultUnit>
    <skos:inScheme rdf:resource="http://vocabulary.odm2.org/unitstype"/>
    <rdf:type rdf:resource="http://www.w3.org/2004/02/skos/core#Concept"/>
    <odm2:dimensionCurrent>0</odm2:dimensionCurrent>
    <skos:historyNote>CSN</skos:historyNote>
    <skos:prefLabel>Length fraction</skos:prefLabel>
    <odm2:dimensionLight>0</odm2:dimensionLight>
  </rdf:Description>
  <rdf:Description rdf:about="http://vocabulary.odm2.org/unitstype/molarAngularMomentum">
    <rdf:type rdf:resource="http://www.w3.org/2004/02/skos/core#Concept"/>
    <odm2:dimensionSymbol>L2M1T-1N-1</odm2:dimensionSymbol>
    <skos:exactMatch>http://qudt.org/vocab/quantity#MolarAngularMomentum</skos:exactMatch>
    <odm2:defaultUnit>Joule Second per Mole</odm2:defaultUnit>
    <skos:inScheme rdf:resource="http://vocabulary.odm2.org/unitstype"/>
    <odm2:dimensionTime>1</odm2:dimensionTime>
    <skos:definition>The angular momentum per mole of substance.  Used for measuring electron orbitals.</skos:definition>
    <odm2:dimensionCurrent>-1</odm2:dimensionCurrent>
    <skos:historyNote>QUDT</skos:historyNote>
    <odm2:category>Chemistry</odm2:category>
    <odm2:dimensionLight>-1</odm2:dimensionLight>
    <odm2:dimensionMass>2</odm2:dimensionMass>
    <skos:prefLabel>Molar angular momentum</skos:prefLabel>
    <odm2:dimensionAmount>0</odm2:dimensionAmount>
    <odm2:dimensionLength>0</odm2:dimensionLength>
    <odm2:dimensionTemperature>0</odm2:dimensionTemperature>
  </rdf:Description>
  <rdf:Description rdf:about="http://vocabulary.odm2.org/unitstype/electricalConductance">
    <skos:prefLabel>Electrical conductance</skos:prefLabel>
    <odm2:dimensionSymbol>L-2M-1T3I2</odm2:dimensionSymbol>
    <skos:exactMatch>http://qudt.org/schema/qudt#ConductanceUnit</skos:exactMatch>
    <odm2:category>Electricity and Magnetism</odm2:category>
    <odm2:dimensionAmount>0</odm2:dimensionAmount>
    <odm2:dimensionTemperature>2</odm2:dimensionTemperature>
    <skos:historyNote>QUDT</skos:historyNote>
    <odm2:dimensionLength>0</odm2:dimensionLength>
    <odm2:dimensionCurrent>3</odm2:dimensionCurrent>
    <odm2:dimensionTime>-1</odm2:dimensionTime>
    <rdf:type rdf:resource="http://www.w3.org/2004/02/skos/core#Concept"/>
    <odm2:dimensionMass>-2</odm2:dimensionMass>
    <odm2:dimensionLight>0</odm2:dimensionLight>
    <odm2:defaultUnit>Siemens (S)</odm2:defaultUnit>
    <skos:definition>Conductance is the reciprocal of resistance and is different from conductivitiy (specific conductance).  Conductance is the ease with which an electric current passes through a conductor.  The SI unit of electrical resistance is the ohm (?), while electrical conductance is measured in siemens (S).  [Wikipedia: https://en.wikipedia.org/wiki/Electrical_resistance_and_conductance]</skos:definition>
    <skos:inScheme rdf:resource="http://vocabulary.odm2.org/unitstype"/>
  </rdf:Description>
  <rdf:Description rdf:about="http://vocabulary.odm2.org/unitstype/concentrationVolumePerVolume">
    <skos:definition>The volume of one substance per unit volume of another substance. This is used for volume percents or the ppm of a gas mixture.</skos:definition>
    <odm2:dimensionCurrent>0</odm2:dimensionCurrent>
    <odm2:dimensionTemperature>0</odm2:dimensionTemperature>
    <odm2:category>Dimensionless Ratio</odm2:category>
    <odm2:defaultUnit>unitless</odm2:defaultUnit>
    <rdf:type rdf:resource="http://www.w3.org/2004/02/skos/core#Concept"/>
    <odm2:dimensionAmount>0</odm2:dimensionAmount>
    <skos:prefLabel>Concentration volume per volume</skos:prefLabel>
    <odm2:dimensionMass>0</odm2:dimensionMass>
    <odm2:dimensionTime>0</odm2:dimensionTime>
    <odm2:dimensionLight>0</odm2:dimensionLight>
    <odm2:dimensionSymbol>L3L-3</odm2:dimensionSymbol>
    <skos:historyNote>new for ODM2</skos:historyNote>
    <odm2:dimensionLength>0</odm2:dimensionLength>
    <skos:inScheme rdf:resource="http://vocabulary.odm2.org/unitstype"/>
  </rdf:Description>
  <rdf:Description rdf:about="http://vocabulary.odm2.org/unitstype/massPerArea">
    <skos:note>Has same dimensionality as length integrated mass concentration</skos:note>
    <skos:inScheme rdf:resource="http://vocabulary.odm2.org/unitstype"/>
    <odm2:category>Chemistry</odm2:category>
    <odm2:dimensionSymbol>L-2M1</odm2:dimensionSymbol>
    <rdf:type rdf:resource="http://www.w3.org/2004/02/skos/core#Concept"/>
    <odm2:dimensionLight>0</odm2:dimensionLight>
    <odm2:dimensionAmount>0</odm2:dimensionAmount>
    <odm2:dimensionTime>1</odm2:dimensionTime>
    <odm2:dimensionMass>-2</odm2:dimensionMass>
    <skos:exactMatch>http://qudt.org/vocab/quantity#Massperarea</skos:exactMatch>
    <skos:historyNote>QUDT</skos:historyNote>
    <odm2:dimensionTemperature>0</odm2:dimensionTemperature>
    <odm2:defaultUnit>Kilogram per square meter (kg/m^2)</odm2:defaultUnit>
    <skos:prefLabel>Mass per area</skos:prefLabel>
    <odm2:dimensionCurrent>0</odm2:dimensionCurrent>
    <odm2:dimensionLength>0</odm2:dimensionLength>
  </rdf:Description>
  <rdf:Description rdf:about="http://vocabulary.odm2.org/unitstype/magneticFluxPerLength">
    <odm2:dimensionLight>0</odm2:dimensionLight>
    <odm2:category>Electricity and Magnetism</odm2:category>
    <odm2:dimensionTime>1</odm2:dimensionTime>
    <odm2:dimensionTemperature>-1</odm2:dimensionTemperature>
    <skos:prefLabel>Magnetic flux per length</skos:prefLabel>
    <skos:definition>Magnetic Flux Per Unit Length</skos:definition>
    <odm2:dimensionCurrent>-2</odm2:dimensionCurrent>
    <odm2:dimensionLength>0</odm2:dimensionLength>
    <odm2:dimensionMass>1</odm2:dimensionMass>
    <odm2:dimensionAmount>0</odm2:dimensionAmount>
    <odm2:defaultUnit>Tesla Meter</odm2:defaultUnit>
    <skos:historyNote>QUDT</skos:historyNote>
    <odm2:dimensionSymbol>L1M1T-2I-1</odm2:dimensionSymbol>
    <rdf:type rdf:resource="http://www.w3.org/2004/02/skos/core#Concept"/>
    <skos:exactMatch>http://qudt.org/vocab/quantity#Magneticfluxperunitlength</skos:exactMatch>
    <skos:inScheme rdf:resource="http://vocabulary.odm2.org/unitstype"/>
  </rdf:Description>
  <rdf:Description rdf:about="http://vocabulary.odm2.org/unitstype/inverseLengthTemperature">
    <odm2:dimensionTime>0</odm2:dimensionTime>
    <skos:historyNote>QUDT</skos:historyNote>
    <odm2:dimensionLight>0</odm2:dimensionLight>
    <odm2:defaultUnit>per meter Kelvin</odm2:defaultUnit>
    <skos:exactMatch>http://qudt.org/vocab/quantity#Inverselengthtemperature</skos:exactMatch>
    <odm2:dimensionTemperature>0</odm2:dimensionTemperature>
    <rdf:type rdf:resource="http://www.w3.org/2004/02/skos/core#Concept"/>
    <odm2:dimensionAmount>-1</odm2:dimensionAmount>
    <skos:inScheme rdf:resource="http://vocabulary.odm2.org/unitstype"/>
    <skos:prefLabel>Inverse length temperature</skos:prefLabel>
    <odm2:dimensionCurrent>0</odm2:dimensionCurrent>
    <odm2:dimensionMass>-1</odm2:dimensionMass>
    <odm2:category>Thermodynamics</odm2:category>
    <odm2:dimensionSymbol>L-1?-1</odm2:dimensionSymbol>
    <odm2:dimensionLength>0</odm2:dimensionLength>
  </rdf:Description>
  <rdf:Description rdf:about="http://vocabulary.odm2.org/unitstype/massPerTime">
    <odm2:dimensionTemperature>0</odm2:dimensionTemperature>
    <skos:definition>In physics and engineering, mass flow rate is the mass of a substance which passes per unit of time. [Wikipedia: https://en.wikipedia.org/wiki/Mass_flow_rate]</skos:definition>
    <odm2:dimensionSymbol>M1T-1</odm2:dimensionSymbol>
    <odm2:dimensionLength>0</odm2:dimensionLength>
    <skos:inScheme rdf:resource="http://vocabulary.odm2.org/unitstype"/>
    <odm2:defaultUnit>Kilogram per second (kg/s)</odm2:defaultUnit>
    <rdf:type rdf:resource="http://www.w3.org/2004/02/skos/core#Concept"/>
    <odm2:dimensionMass>0</odm2:dimensionMass>
    <skos:note>Also known as loading.</skos:note>
    <odm2:category>Mechanics</odm2:category>
    <odm2:dimensionCurrent>-1</odm2:dimensionCurrent>
    <skos:historyNote>QUDT</skos:historyNote>
    <odm2:dimensionLight>0</odm2:dimensionLight>
    <odm2:dimensionTime>1</odm2:dimensionTime>
    <odm2:dimensionAmount>0</odm2:dimensionAmount>
    <skos:exactMatch>http://qudt.org/vocab/quantity#Masspertime</skos:exactMatch>
    <skos:prefLabel>Mass per time</skos:prefLabel>
  </rdf:Description>
  <rdf:Description rdf:about="http://vocabulary.odm2.org/unitstype/electricalFluxDensity">
    <odm2:dimensionCurrent>1</odm2:dimensionCurrent>
    <odm2:dimensionLength>0</odm2:dimensionLength>
    <odm2:dimensionTemperature>1</odm2:dimensionTemperature>
    <odm2:dimensionMass>-2</odm2:dimensionMass>
    <skos:historyNote>QUDT</skos:historyNote>
    <odm2:category>Electricity and Magnetism</odm2:category>
    <rdf:type rdf:resource="http://www.w3.org/2004/02/skos/core#Concept"/>
    <skos:exactMatch>http://qudt.org/schema/qudt#ElectricFluxDensityUnit</skos:exactMatch>
    <odm2:dimensionAmount>0</odm2:dimensionAmount>
    <odm2:dimensionSymbol>L-2T1I1</odm2:dimensionSymbol>
    <skos:prefLabel>Electrical flux density</skos:prefLabel>
    <odm2:defaultUnit>Coulomb per Square Meter (C/m^2)</odm2:defaultUnit>
    <odm2:dimensionTime>0</odm2:dimensionTime>
    <skos:definition>In physics, the electric flux density (or electric displacement field), denoted by D, is a vector field that appears in Maxwell's equations. It accounts for the effects of free and bound charge within materials. "D" stands for "displacement", as in the related concept of displacement current in dielectrics. In free space, the electric displacement field is equivalent to flux density, a concept that lends understanding to Gauss's law.</skos:definition>
    <skos:inScheme rdf:resource="http://vocabulary.odm2.org/unitstype"/>
    <odm2:dimensionLight>0</odm2:dimensionLight>
  </rdf:Description>
  <rdf:Description rdf:about="http://vocabulary.odm2.org/unitstype/heatCapacity">
    <skos:inScheme rdf:resource="http://vocabulary.odm2.org/unitstype"/>
    <skos:exactMatch>http://qudt.org/vocab/quantity#Heatcapacity</skos:exactMatch>
    <rdf:type rdf:resource="http://www.w3.org/2004/02/skos/core#Concept"/>
    <odm2:dimensionAmount>-1</odm2:dimensionAmount>
    <odm2:dimensionSymbol>L2M1T-2?-1</odm2:dimensionSymbol>
    <odm2:dimensionTime>1</odm2:dimensionTime>
    <odm2:dimensionTemperature>0</odm2:dimensionTemperature>
    <skos:definition>Heat capacity, or thermal capacity, is a measurable physical quantity equal to the ratio of the heat added to (or removed from) an object to the resulting temperature change. The SI unit of heat capacity is joule per kelvin and the dimensional form is L2MT?2??1. [Wikipedia: https://en.wikipedia.org/wiki/Heat_capacity]</skos:definition>
    <odm2:dimensionMass>2</odm2:dimensionMass>
    <odm2:dimensionCurrent>-2</odm2:dimensionCurrent>
    <skos:historyNote>QUDT</skos:historyNote>
    <skos:prefLabel>Heat capacity</skos:prefLabel>
    <odm2:defaultUnit>Joule per kelvin (J/K)</odm2:defaultUnit>
    <odm2:dimensionLight>0</odm2:dimensionLight>
    <odm2:category>Thermodynamics</odm2:category>
    <odm2:dimensionLength>0</odm2:dimensionLength>
  </rdf:Description>
  <rdf:Description rdf:about="http://vocabulary.odm2.org/unitstype/linearEnergyTransfer">
    <skos:definition>Linear energy transfer (LET) is a term used in dosimetry. It describes the action of radiation upon matter. It is identical to the retarding force acting on a charged ionizing particle travelling through the matter.  It describes how much energy an ionising particle transfers to the material transversed per unit distance. By definition, LET is a positive quantity. LET depends on the nature of the radiation as well as on the material traversed. [Wikipedia: https://en.wikipedia.org/wiki/Linear_energy_transfer]</skos:definition>
    <odm2:dimensionCurrent>-2</odm2:dimensionCurrent>
    <odm2:dimensionLight>0</odm2:dimensionLight>
    <odm2:dimensionTime>1</odm2:dimensionTime>
    <skos:prefLabel>Linear energy transfer</skos:prefLabel>
    <odm2:category>Atomic Physics</odm2:category>
    <odm2:defaultUnit>Joules per meter (J/m)</odm2:defaultUnit>
    <odm2:dimensionMass>1</odm2:dimensionMass>
    <skos:note>Has identical dimensionality to force, but is generally expressed differently. https://en.wikipedia.org/wiki/Linear_energy_transfer</skos:note>
    <skos:inScheme rdf:resource="http://vocabulary.odm2.org/unitstype"/>
    <odm2:dimensionAmount>0</odm2:dimensionAmount>
    <odm2:dimensionSymbol>L1M1T-2</odm2:dimensionSymbol>
    <skos:historyNote>QUDT</skos:historyNote>
    <odm2:dimensionTemperature>0</odm2:dimensionTemperature>
    <rdf:type rdf:resource="http://www.w3.org/2004/02/skos/core#Concept"/>
    <odm2:dimensionLength>0</odm2:dimensionLength>
    <skos:exactMatch>http://qudt.org/vocab/quantity#LinearEnergyTransfer</skos:exactMatch>
  </rdf:Description>
  <rdf:Description rdf:about="http://vocabulary.odm2.org/unitstype/particleFlux">
    <odm2:dimensionTemperature>0</odm2:dimensionTemperature>
    <odm2:category>Chemistry</odm2:category>
    <odm2:dimensionCurrent>-1</odm2:dimensionCurrent>
    <odm2:defaultUnit>moles per meter squared per second</odm2:defaultUnit>
    <skos:inScheme rdf:resource="http://vocabulary.odm2.org/unitstype"/>
    <odm2:dimensionMass>-2</odm2:dimensionMass>
    <odm2:dimensionTime>0</odm2:dimensionTime>
    <skos:definition>The number of particles, organisms, or moles of substance going through a specific area in a given amount of time.</skos:definition>
    <odm2:dimensionLight>1</odm2:dimensionLight>
    <skos:prefLabel>Particle flux</skos:prefLabel>
    <skos:historyNote>CUAHSI</skos:historyNote>
    <odm2:dimensionSymbol>L-2T-1N1</odm2:dimensionSymbol>
    <odm2:dimensionAmount>0</odm2:dimensionAmount>
    <odm2:dimensionLength>0</odm2:dimensionLength>
    <rdf:type rdf:resource="http://www.w3.org/2004/02/skos/core#Concept"/>
  </rdf:Description>
  <rdf:Description rdf:about="http://vocabulary.odm2.org/unitstype/electricalChargePerMass">
    <skos:definition>Unit group for radiation exposure and gyromagnetic ratios</skos:definition>
    <odm2:dimensionCurrent>1</odm2:dimensionCurrent>
    <odm2:defaultUnit>Coulomb per kilogram (C/kg)</odm2:defaultUnit>
    <odm2:dimensionTime>-1</odm2:dimensionTime>
    <skos:historyNote>QUDT</skos:historyNote>
    <odm2:dimensionLight>0</odm2:dimensionLight>
    <skos:prefLabel>Electrical charge per mass</skos:prefLabel>
    <skos:inScheme rdf:resource="http://vocabulary.odm2.org/unitstype"/>
    <odm2:dimensionAmount>0</odm2:dimensionAmount>
    <skos:exactMatch>http://qudt.org/vocab/quantity#Electricalchargepermass</skos:exactMatch>
    <odm2:dimensionMass>0</odm2:dimensionMass>
    <odm2:dimensionLength>0</odm2:dimensionLength>
    <odm2:dimensionTemperature>1</odm2:dimensionTemperature>
    <rdf:type rdf:resource="http://www.w3.org/2004/02/skos/core#Concept"/>
    <odm2:category>Electricity and Magnetism</odm2:category>
    <odm2:dimensionSymbol>M-1T1I1</odm2:dimensionSymbol>
  </rdf:Description>
  <rdf:Description rdf:about="http://vocabulary.odm2.org/unitstype/areaThermalExpansion">
    <skos:exactMatch>http://qudt.org/vocab/quantity#AreaThermalExpansion</skos:exactMatch>
    <odm2:dimensionAmount>-1</odm2:dimensionAmount>
    <odm2:category>Thermodynamics</odm2:category>
    <odm2:dimensionSymbol>L2?-1</odm2:dimensionSymbol>
    <odm2:dimensionMass>2</odm2:dimensionMass>
    <odm2:dimensionTime>0</odm2:dimensionTime>
    <odm2:dimensionLength>0</odm2:dimensionLength>
    <odm2:dimensionLight>0</odm2:dimensionLight>
    <odm2:defaultUnit>Square meter per kelvin (m^2/K)</odm2:defaultUnit>
    <odm2:dimensionTemperature>0</odm2:dimensionTemperature>
    <rdf:type rdf:resource="http://www.w3.org/2004/02/skos/core#Concept"/>
    <skos:prefLabel>Area thermal expansion</skos:prefLabel>
    <odm2:dimensionCurrent>0</odm2:dimensionCurrent>
    <skos:inScheme rdf:resource="http://vocabulary.odm2.org/unitstype"/>
    <skos:definition>When the temperature of a substance changes, the energy that is stored in the intermolecular bonds between atoms changes. When the stored energy increases, so does the length of the molecular bonds. As a result, solids typically expand in response to heating and contract on cooling; this dimensional response to temperature change is expressed by its coefficient of thermal expansion. Different coefficients of thermal expansion can be defined for a substance depending on whether the expansion is measured by: * linear thermal expansion * area thermal expansion * volumetric thermal expansion These characteristics are closely related. The volumetric thermal expansion coefficient can be defined for both liquids and solids. The linear thermal expansion can only be defined for solids, and is common in engineering applications. Some substances expand when cooled, such as freezing water, so they have negative thermal expansion coefficients. [Wikipedia: https://en.wikipedia.org/wiki/Thermal_expansion]</skos:definition>
    <skos:historyNote>QUDT</skos:historyNote>
  </rdf:Description>
  <rdf:Description rdf:about="http://vocabulary.odm2.org/unitstype/areaTime">
    <odm2:dimensionCurrent>1</odm2:dimensionCurrent>
    <odm2:dimensionAmount>0</odm2:dimensionAmount>
    <odm2:dimensionSymbol>L2T1</odm2:dimensionSymbol>
    <rdf:type rdf:resource="http://www.w3.org/2004/02/skos/core#Concept"/>
    <odm2:category>Space and Time</odm2:category>
    <odm2:dimensionTime>0</odm2:dimensionTime>
    <skos:prefLabel>Area time</skos:prefLabel>
    <skos:exactMatch>http://qudt.org/vocab/quantity#AreaTime</skos:exactMatch>
    <skos:inScheme rdf:resource="http://vocabulary.odm2.org/unitstype"/>
    <skos:historyNote>QUDT</skos:historyNote>
    <odm2:defaultUnit>Square meter second (m^2 s)</odm2:defaultUnit>
    <odm2:dimensionLight>0</odm2:dimensionLight>
    <odm2:dimensionLength>0</odm2:dimensionLength>
    <odm2:dimensionTemperature>0</odm2:dimensionTemperature>
    <odm2:dimensionMass>2</odm2:dimensionMass>
  </rdf:Description>
  <rdf:Description rdf:about="http://vocabulary.odm2.org/unitstype/count">
    <rdf:type rdf:resource="http://www.w3.org/2004/02/skos/core#Concept"/>
    <odm2:category>Base Quantity</odm2:category>
    <skos:prefLabel>Count</skos:prefLabel>
    <odm2:dimensionTime>0</odm2:dimensionTime>
    <odm2:dimensionLight>1</odm2:dimensionLight>
    <odm2:dimensionAmount>0</odm2:dimensionAmount>
    <odm2:dimensionMass>0</odm2:dimensionMass>
    <odm2:defaultUnit>Mole (mol)</odm2:defaultUnit>
    <skos:exactMatch>http://qudt.org/vocab/quantity#AmountOfSubstance</skos:exactMatch>
    <odm2:dimensionSymbol>N1</odm2:dimensionSymbol>
    <odm2:dimensionCurrent>0</odm2:dimensionCurrent>
    <odm2:dimensionLength>0</odm2:dimensionLength>
    <skos:inScheme rdf:resource="http://vocabulary.odm2.org/unitstype"/>
    <skos:definition>Count or amount of substance is a standards-defined quantity that measures the size of an ensemble of elementary entities, such as atoms, molecules, electrons, and other particles. It is a macroscopic property and it is sometimes referred to as chemical amount. The International System of Units (SI) defines the amount of substance to be proportional to the number of elementary entities present. The SI unit for amount of substance is the mole. It has the unit symbol mol.</skos:definition>
    <odm2:dimensionTemperature>0</odm2:dimensionTemperature>
    <skos:historyNote>QUDT</skos:historyNote>
  </rdf:Description>
  <rdf:Description rdf:about="http://vocabulary.odm2.org/unitstype/electricalCurrentPerAngle">
    <rdf:type rdf:resource="http://www.w3.org/2004/02/skos/core#Concept"/>
    <odm2:dimensionCurrent>0</odm2:dimensionCurrent>
    <odm2:dimensionMass>0</odm2:dimensionMass>
    <odm2:dimensionLength>-1</odm2:dimensionLength>
    <skos:inScheme rdf:resource="http://vocabulary.odm2.org/unitstype"/>
    <odm2:dimensionTime>0</odm2:dimensionTime>
    <odm2:defaultUnit>Ampere per radian (A/rad)</odm2:defaultUnit>
    <skos:prefLabel>Electrical current per angle</skos:prefLabel>
    <odm2:dimensionLight>0</odm2:dimensionLight>
    <odm2:category>Electricity and Magnetism</odm2:category>
    <odm2:dimensionAmount>0</odm2:dimensionAmount>
    <odm2:dimensionTemperature>1</odm2:dimensionTemperature>
    <skos:exactMatch>http://qudt.org/vocab/quantity#Electricalcurrentperangle</skos:exactMatch>
    <skos:historyNote>QUDT</skos:historyNote>
    <odm2:dimensionSymbol>U-1I1</odm2:dimensionSymbol>
  </rdf:Description>
  <rdf:Description rdf:about="http://vocabulary.odm2.org/unitstype/volumetricFlux">
    <rdf:type rdf:resource="http://www.w3.org/2004/02/skos/core#Concept"/>
    <skos:historyNote>Wikipedia</skos:historyNote>
    <odm2:dimensionLength>0</odm2:dimensionLength>
    <skos:prefLabel>Volumetric flux</skos:prefLabel>
    <odm2:dimensionAmount>0</odm2:dimensionAmount>
    <odm2:category>Mechanics</odm2:category>
    <odm2:defaultUnit>meters cubed per second per meter squared (m^3/s*m^2)</odm2:defaultUnit>
    <odm2:dimensionSymbol>L1T-1</odm2:dimensionSymbol>
    <skos:note>Has identical dimensionality to linear velocity, but is expressed differently.</skos:note>
    <skos:exactMatch>http://dbpedia.org/page/Volumetric_flux</skos:exactMatch>
    <skos:definition>In fluid dynamics, the volumetric flux is the rate of volume flow across a unit area (m3·s?1·m?2). Volumetric flux = liters/(second*area). The density of a particular property in a fluid's volume, multiplied with the volumetric flux of the fluid, thus defines the advective flux of that property.  The volumetric flux through a porous medium is often modelled using Darcy's law. Volumetric flux is not to be confused with volumetric flow rate, which is the volume of fluid that passes through a given surface per unit of time (as opposed to a unit surface).  [Wikipedia: https://en.wikipedia.org/wiki/Volumetric_flux] Also used for hydraulic conductivity.</skos:definition>
    <odm2:dimensionTemperature>0</odm2:dimensionTemperature>
    <odm2:dimensionTime>0</odm2:dimensionTime>
    <odm2:dimensionCurrent>-1</odm2:dimensionCurrent>
    <skos:inScheme rdf:resource="http://vocabulary.odm2.org/unitstype"/>
    <odm2:dimensionMass>1</odm2:dimensionMass>
    <odm2:dimensionLight>0</odm2:dimensionLight>
  </rdf:Description>
  <rdf:Description rdf:about="http://vocabulary.odm2.org/unitstype/concentrationPercentSaturation">
    <odm2:dimensionTime>0</odm2:dimensionTime>
    <odm2:dimensionCurrent>0</odm2:dimensionCurrent>
    <odm2:dimensionLength>0</odm2:dimensionLength>
    <rdf:type rdf:resource="http://www.w3.org/2004/02/skos/core#Concept"/>
    <odm2:category>Chemistry</odm2:category>
    <odm2:dimensionAmount>0</odm2:dimensionAmount>
    <odm2:dimensionTemperature>0</odm2:dimensionTemperature>
    <odm2:dimensionLight>0</odm2:dimensionLight>
    <odm2:dimensionMass>0</odm2:dimensionMass>
    <odm2:defaultUnit>Percent (%)</odm2:defaultUnit>
    <skos:inScheme rdf:resource="http://vocabulary.odm2.org/unitstype"/>
    <skos:definition>The amount of a substance dissolved in a solution compared with the amount dissolved in the solution at saturation concentration, expressed as a percent. </skos:definition>
    <skos:prefLabel>Concentration percent saturation</skos:prefLabel>
  </rdf:Description>
  <rdf:Description rdf:about="http://vocabulary.odm2.org/unitstype/angularAcceleration">
    <odm2:dimensionTemperature>0</odm2:dimensionTemperature>
    <odm2:category>Space and Time</odm2:category>
    <odm2:dimensionTime>0</odm2:dimensionTime>
    <odm2:dimensionSymbol>U1T-2</odm2:dimensionSymbol>
    <skos:exactMatch>http://qudt.org/vocab/quantity#AngularAcceleration</skos:exactMatch>
    <rdf:type rdf:resource="http://www.w3.org/2004/02/skos/core#Concept"/>
    <skos:definition>Angular acceleration is the rate of change of angular velocity over time. Measurement of the change made in the rate of change of an angle that a spinning object undergoes per unit time. It is a vector quantity. Also called Rotational acceleration. In SI units, it is measured in radians per second squared (rad/s^2), and is usually denoted by the Greek letter alpha.</skos:definition>
    <odm2:dimensionLight>0</odm2:dimensionLight>
    <skos:historyNote>QUDT</skos:historyNote>
    <odm2:dimensionLength>1</odm2:dimensionLength>
    <odm2:dimensionAmount>0</odm2:dimensionAmount>
    <skos:prefLabel>Angular acceleration</skos:prefLabel>
    <skos:inScheme rdf:resource="http://vocabulary.odm2.org/unitstype"/>
    <odm2:dimensionCurrent>-2</odm2:dimensionCurrent>
    <odm2:defaultUnit>Radian per second squared (rad/s^2)</odm2:defaultUnit>
    <odm2:dimensionMass>0</odm2:dimensionMass>
  </rdf:Description>
  <rdf:Description rdf:about="http://vocabulary.odm2.org/unitstype/salinity">
    <odm2:dimensionMass>0</odm2:dimensionMass>
    <skos:definition>Salinity is the saltiness or dissolved salt content of a body of water. Salinity is an important factor in determining many aspects of the chemistryof natural waters and of biological processes within it, and is a thermodynamic state variable that, along with temperature and pressure, governs physical characteristics like the density and heat capacity of the water. The use of electrical conductivity measurements to estimate the ionic content of seawater led to the development of the so-called practical salinity scale 1978 (PSS-78). Salinities measured using PSS-78 do not have units. The 'unit' of PSU (denoting practical salinity unit) is sometimes added to PSS-78 measurements, however this is officially discouraged.</skos:definition>
    <odm2:dimensionLength>1</odm2:dimensionLength>
    <skos:inScheme rdf:resource="http://vocabulary.odm2.org/unitstype"/>
    <odm2:dimensionLight>0</odm2:dimensionLight>
    <odm2:dimensionCurrent>0</odm2:dimensionCurrent>
    <skos:exactMatch>http://dbpedia.org/page/Salinity</skos:exactMatch>
    <rdf:type rdf:resource="http://www.w3.org/2004/02/skos/core#Concept"/>
    <odm2:dimensionTemperature>0</odm2:dimensionTemperature>
    <skos:prefLabel>Salinity</skos:prefLabel>
    <odm2:dimensionTime>0</odm2:dimensionTime>
    <odm2:defaultUnit>Practical salinity units (PSU)</odm2:defaultUnit>
    <skos:historyNote>Wikipedia</skos:historyNote>
    <odm2:dimensionSymbol>U1</odm2:dimensionSymbol>
    <odm2:category>Chemistry</odm2:category>
    <odm2:dimensionAmount>0</odm2:dimensionAmount>
  </rdf:Description>
  <rdf:Description rdf:about="http://vocabulary.odm2.org/unitstype/inverseCount">
    <odm2:defaultUnit>Per mole (mol^(-1))</odm2:defaultUnit>
    <odm2:dimensionLight>-1</odm2:dimensionLight>
    <rdf:type rdf:resource="http://www.w3.org/2004/02/skos/core#Concept"/>
    <odm2:dimensionCurrent>0</odm2:dimensionCurrent>
    <odm2:category>Chemistry</odm2:category>
    <skos:prefLabel>Inverse count</skos:prefLabel>
    <skos:inScheme rdf:resource="http://vocabulary.odm2.org/unitstype"/>
    <odm2:dimensionTime>0</odm2:dimensionTime>
    <skos:exactMatch>http://qudt.org/vocab/quantity#Inversecount</skos:exactMatch>
    <odm2:dimensionTemperature>0</odm2:dimensionTemperature>
    <odm2:dimensionLength>0</odm2:dimensionLength>
    <odm2:dimensionMass>0</odm2:dimensionMass>
    <odm2:dimensionAmount>0</odm2:dimensionAmount>
    <odm2:dimensionSymbol>N-1</odm2:dimensionSymbol>
    <skos:historyNote>QUDT</skos:historyNote>
  </rdf:Description>
  <rdf:Description rdf:about="http://vocabulary.odm2.org/unitstype/electricalCapacitance">
    <odm2:dimensionAmount>0</odm2:dimensionAmount>
    <odm2:defaultUnit>Farad (F)</odm2:defaultUnit>
    <odm2:dimensionTime>-1</odm2:dimensionTime>
    <skos:prefLabel>Electrical capacitance</skos:prefLabel>
    <odm2:dimensionLight>0</odm2:dimensionLight>
    <odm2:dimensionMass>-2</odm2:dimensionMass>
    <skos:inScheme rdf:resource="http://vocabulary.odm2.org/unitstype"/>
    <skos:historyNote>QUDT</skos:historyNote>
    <odm2:dimensionLength>0</odm2:dimensionLength>
    <odm2:dimensionTemperature>2</odm2:dimensionTemperature>
    <skos:definition>Capacitance is the ability of a body to store an electrical charge.</skos:definition>
    <odm2:dimensionCurrent>4</odm2:dimensionCurrent>
    <odm2:dimensionSymbol>L-2M-1T4I2</odm2:dimensionSymbol>
    <rdf:type rdf:resource="http://www.w3.org/2004/02/skos/core#Concept"/>
    <skos:exactMatch>http://qudt.org/vocab/quantity#Capacitance</skos:exactMatch>
    <odm2:category>Electricity and Magnetism</odm2:category>
  </rdf:Description>
  <rdf:Description rdf:about="http://vocabulary.odm2.org/unitstype/countPerArea">
    <odm2:dimensionSymbol>L-2N1</odm2:dimensionSymbol>
    <odm2:dimensionMass>-2</odm2:dimensionMass>
    <skos:historyNote>Aquarius</skos:historyNote>
    <odm2:defaultUnit>Count per square meter (#/m^2)</odm2:defaultUnit>
    <skos:definition>The areal density of a given amount of a substance.  This unit group is also used for pixel densities (often incorrectly called resolution).</skos:definition>
    <odm2:category>Space and Time</odm2:category>
    <odm2:dimensionLight>1</odm2:dimensionLight>
    <skos:inScheme rdf:resource="http://vocabulary.odm2.org/unitstype"/>
    <odm2:dimensionTime>0</odm2:dimensionTime>
    <odm2:dimensionCurrent>0</odm2:dimensionCurrent>
    <rdf:type rdf:resource="http://www.w3.org/2004/02/skos/core#Concept"/>
    <skos:prefLabel>Count per area</skos:prefLabel>
    <odm2:dimensionTemperature>0</odm2:dimensionTemperature>
    <odm2:dimensionLength>0</odm2:dimensionLength>
    <odm2:dimensionAmount>0</odm2:dimensionAmount>
  </rdf:Description>
  <rdf:Description rdf:about="http://vocabulary.odm2.org/unitstype/energyPerAreaElectricalCharge">
    <odm2:dimensionLength>0</odm2:dimensionLength>
    <skos:historyNote>QUDT</skos:historyNote>
    <rdf:type rdf:resource="http://www.w3.org/2004/02/skos/core#Concept"/>
    <odm2:category>Electricity and Magnetism</odm2:category>
    <skos:inScheme rdf:resource="http://vocabulary.odm2.org/unitstype"/>
    <odm2:dimensionSymbol>M1T-3I-1</odm2:dimensionSymbol>
    <skos:exactMatch>http://qudt.org/vocab/quantity#EnergyPerAreaElectricCharge</skos:exactMatch>
    <odm2:dimensionLight>0</odm2:dimensionLight>
    <odm2:dimensionCurrent>-3</odm2:dimensionCurrent>
    <odm2:dimensionAmount>0</odm2:dimensionAmount>
    <odm2:dimensionMass>0</odm2:dimensionMass>
    <skos:note>Magnetic current density?</skos:note>
    <odm2:dimensionTime>1</odm2:dimensionTime>
    <skos:prefLabel>Energy per area electrical charge</skos:prefLabel>
    <odm2:dimensionTemperature>-1</odm2:dimensionTemperature>
    <odm2:defaultUnit>Volt per Square Meter</odm2:defaultUnit>
  </rdf:Description>
  <rdf:Description rdf:about="http://vocabulary.odm2.org/unitstype/electricalResistance">
    <rdf:type rdf:resource="http://www.w3.org/2004/02/skos/core#Concept"/>
    <skos:historyNote>Wikipedia</skos:historyNote>
    <skos:definition>Electrical resistance is a ratio of the degree to which an object opposes an electric current through it, measured in ohms. Its reciprocal quantity is electrical conductance measured in siemens.</skos:definition>
    <odm2:dimensionSymbol>L2M1T-3I-2</odm2:dimensionSymbol>
    <skos:inScheme rdf:resource="http://vocabulary.odm2.org/unitstype"/>
    <odm2:dimensionLight>0</odm2:dimensionLight>
    <skos:prefLabel>Electrical resistance</skos:prefLabel>
    <skos:exactMatch>http://dbpedia.org/page/Electrical_resistance_and_conductance</skos:exactMatch>
    <odm2:defaultUnit>Ohm (Ohm)</odm2:defaultUnit>
    <odm2:dimensionCurrent>-3</odm2:dimensionCurrent>
    <odm2:dimensionLength>0</odm2:dimensionLength>
    <odm2:dimensionMass>2</odm2:dimensionMass>
    <odm2:dimensionTime>1</odm2:dimensionTime>
    <odm2:dimensionTemperature>-2</odm2:dimensionTemperature>
    <odm2:dimensionAmount>0</odm2:dimensionAmount>
    <odm2:category>Electricity and Magnetism</odm2:category>
  </rdf:Description>
  <rdf:Description rdf:about="http://vocabulary.odm2.org/unitstype/specificEnergy">
    <skos:prefLabel>Specific energy</skos:prefLabel>
    <skos:note>Absorbed dose, does equivalent, and specific energy all have the same dimensionality.</skos:note>
    <odm2:dimensionMass>2</odm2:dimensionMass>
    <odm2:dimensionSymbol>L2T-2</odm2:dimensionSymbol>
    <odm2:dimensionAmount>0</odm2:dimensionAmount>
    <odm2:dimensionLength>0</odm2:dimensionLength>
    <skos:exactMatch>http://qudt.org/vocab/quantity#Specificenergy</skos:exactMatch>
    <rdf:type rdf:resource="http://www.w3.org/2004/02/skos/core#Concept"/>
    <odm2:dimensionTemperature>0</odm2:dimensionTemperature>
    <odm2:category>Mechanics</odm2:category>
    <skos:definition>Specific energy is energy per unit mass. (It is also sometimes called "energy density," though "energy density" more precisely means energy per unit volume.) The SI unit for specific energy is the joule per kilogram (J/kg). Other units still in use in some contexts are the kilocalorie per gram (Cal/g or kcal/g), mostly in food-related topics, watt hours per kilogram in the field of batteries, and the Imperial unit BTU per pound (BTU/lb), in some engineering and applied technical fields.</skos:definition>
    <odm2:dimensionCurrent>-2</odm2:dimensionCurrent>
    <skos:inScheme rdf:resource="http://vocabulary.odm2.org/unitstype"/>
    <odm2:defaultUnit>Joule per kilogram (J/kg); Gray (Gy); Sievert (Sv)</odm2:defaultUnit>
    <odm2:dimensionTime>0</odm2:dimensionTime>
    <skos:historyNote>QUDT</skos:historyNote>
    <odm2:dimensionLight>0</odm2:dimensionLight>
  </rdf:Description>
  <rdf:Description rdf:about="http://vocabulary.odm2.org/unitstype/inverseEnergy">
    <odm2:category>Mechanics</odm2:category>
    <odm2:dimensionLength>0</odm2:dimensionLength>
    <skos:historyNote>QUDT</skos:historyNote>
    <odm2:dimensionTemperature>0</odm2:dimensionTemperature>
    <skos:prefLabel>Inverse energy</skos:prefLabel>
    <odm2:dimensionAmount>0</odm2:dimensionAmount>
    <rdf:type rdf:resource="http://www.w3.org/2004/02/skos/core#Concept"/>
    <odm2:defaultUnit>per Joule</odm2:defaultUnit>
    <odm2:dimensionMass>-2</odm2:dimensionMass>
    <odm2:dimensionSymbol>L-2M-1T2</odm2:dimensionSymbol>
    <odm2:dimensionLight>0</odm2:dimensionLight>
    <skos:inScheme rdf:resource="http://vocabulary.odm2.org/unitstype"/>
    <odm2:dimensionCurrent>2</odm2:dimensionCurrent>
    <skos:exactMatch>http://qudt.org/vocab/quantity#Inverseenergy</skos:exactMatch>
    <odm2:dimensionTime>-1</odm2:dimensionTime>
  </rdf:Description>
  <rdf:Description rdf:about="http://vocabulary.odm2.org/unitstype/concentrationCountPerCount">
    <odm2:category>Dimensionless Ratio</odm2:category>
    <odm2:defaultUnit>mole per mole</odm2:defaultUnit>
    <rdf:type rdf:resource="http://www.w3.org/2004/02/skos/core#Concept"/>
    <skos:definition>The count of one substance per unit count of another substance, also known as mole fraction or numeric concentration.</skos:definition>
    <skos:inScheme rdf:resource="http://vocabulary.odm2.org/unitstype"/>
    <skos:prefLabel>Concentration count per count</skos:prefLabel>
    <odm2:dimensionSymbol>N1N-1</odm2:dimensionSymbol>
    <odm2:dimensionTemperature>0</odm2:dimensionTemperature>
    <odm2:dimensionAmount>0</odm2:dimensionAmount>
    <odm2:dimensionMass>0</odm2:dimensionMass>
    <skos:historyNote>New for ODM2</skos:historyNote>
    <odm2:dimensionLight>0</odm2:dimensionLight>
    <odm2:dimensionTime>0</odm2:dimensionTime>
    <odm2:dimensionLength>0</odm2:dimensionLength>
    <odm2:dimensionCurrent>0</odm2:dimensionCurrent>
  </rdf:Description>
  <rdf:Description rdf:about="http://vocabulary.odm2.org/unitstype/specificHeatCapacity">
    <odm2:dimensionTemperature>0</odm2:dimensionTemperature>
    <odm2:dimensionLight>0</odm2:dimensionLight>
    <odm2:dimensionMass>2</odm2:dimensionMass>
    <skos:inScheme rdf:resource="http://vocabulary.odm2.org/unitstype"/>
    <skos:historyNote>QUDT</skos:historyNote>
    <odm2:dimensionLength>0</odm2:dimensionLength>
    <odm2:dimensionCurrent>-2</odm2:dimensionCurrent>
    <odm2:category>Thermodynamics</odm2:category>
    <odm2:dimensionSymbol>L2T-2?-1</odm2:dimensionSymbol>
    <skos:prefLabel>Specific heat capacity</skos:prefLabel>
    <rdf:type rdf:resource="http://www.w3.org/2004/02/skos/core#Concept"/>
    <odm2:dimensionTime>0</odm2:dimensionTime>
    <skos:definition>The specific heat capacity, often simply called specific heat, is the heat capacity per unit mass of a material.  It is the amount of heat needed to raise the temperature of a certain mass 1 degree Celsius.</skos:definition>
    <odm2:dimensionAmount>-1</odm2:dimensionAmount>
    <skos:exactMatch>http://qudt.org/vocab/quantity#Specificheatcapacity</skos:exactMatch>
    <odm2:defaultUnit>Joule per kilogram kelvin (J/(kg-K))</odm2:defaultUnit>
  </rdf:Description>
  <rdf:Description rdf:about="http://vocabulary.odm2.org/unitstype/areaTemperature">
    <rdf:type rdf:resource="http://www.w3.org/2004/02/skos/core#Concept"/>
    <odm2:dimensionMass>2</odm2:dimensionMass>
    <odm2:dimensionAmount>1</odm2:dimensionAmount>
    <odm2:dimensionTemperature>0</odm2:dimensionTemperature>
    <odm2:dimensionLight>0</odm2:dimensionLight>
    <odm2:dimensionTime>0</odm2:dimensionTime>
    <skos:historyNote>QUDT</skos:historyNote>
    <odm2:defaultUnit>Square meter kelvin (m^2-K)</odm2:defaultUnit>
    <skos:prefLabel>Area temperature</skos:prefLabel>
    <odm2:category>Thermodynamics</odm2:category>
    <odm2:dimensionSymbol>L2?1</odm2:dimensionSymbol>
    <odm2:dimensionCurrent>0</odm2:dimensionCurrent>
    <skos:exactMatch>http://qudt.org/schema/qudt#AreaTemperatureUnit</skos:exactMatch>
    <odm2:dimensionLength>0</odm2:dimensionLength>
    <skos:inScheme rdf:resource="http://vocabulary.odm2.org/unitstype"/>
  </rdf:Description>
  <rdf:Description rdf:about="http://vocabulary.odm2.org/unitstype/absorbedDose">
    <odm2:dimensionLength>0</odm2:dimensionLength>
    <skos:note>Absorbed dose, does equivalent, and specific energy all have the same dimensionality.</skos:note>
    <odm2:dimensionTemperature>0</odm2:dimensionTemperature>
    <skos:prefLabel>Absorbed dose</skos:prefLabel>
    <rdf:type rdf:resource="http://www.w3.org/2004/02/skos/core#Concept"/>
    <odm2:dimensionMass>2</odm2:dimensionMass>
    <odm2:dimensionTime>0</odm2:dimensionTime>
    <skos:inScheme rdf:resource="http://vocabulary.odm2.org/unitstype"/>
    <odm2:dimensionAmount>0</odm2:dimensionAmount>
    <skos:historyNote>QUDT</skos:historyNote>
    <odm2:defaultUnit>Gray (Gy)</odm2:defaultUnit>
    <odm2:dimensionCurrent>-2</odm2:dimensionCurrent>
    <skos:exactMatch>http://qudt.org/vocab/quantity#AbsorbedDose</skos:exactMatch>
    <skos:definition>Absorbed dose (also known as Total Ionizing Dose, TID) is a measure of the energy deposited in a medium by ionizing radiation. It is equal to the energy deposited per unit mass of medium, and so has the unit J/kg, which is given the special name Gray (Gy). Note that the absorbed dose is not a good indicator of the likely biological effect. 1 Gy of alpha radiation would be much more biologically damaging than 1 Gy of photon radiation for example. Appropriate weighting factors can be applied reflecting the different relative biological effects to find the equivalent dose. The risk of stoctic effects due to radiation exposure can be quantified using the effective dose, which is a weighted average of the equivalent dose to each organ depending upon its radiosensitivity. When ionising radiation is used to treat cancer, the doctor will usually prescribe the radiotherapy treatment in Gy. When risk from ionising radiation is being discussed, a related unit, the Sievert is used.</skos:definition>
    <odm2:dimensionSymbol>L2T-2</odm2:dimensionSymbol>
    <odm2:dimensionLight>0</odm2:dimensionLight>
    <odm2:category>Radiology</odm2:category>
  </rdf:Description>
  <rdf:Description rdf:about="http://vocabulary.odm2.org/unitstype/electricalChargePerCount">
    <odm2:dimensionSymbol>T1I1N-1</odm2:dimensionSymbol>
    <odm2:dimensionAmount>0</odm2:dimensionAmount>
    <odm2:dimensionLight>-1</odm2:dimensionLight>
    <skos:definition>The amount of electrical charge within a given count of something.</skos:definition>
    <odm2:dimensionLength>0</odm2:dimensionLength>
    <odm2:dimensionTemperature>1</odm2:dimensionTemperature>
    <skos:prefLabel>Electrical charge per count</skos:prefLabel>
    <odm2:defaultUnit>Coulomb per mole (C/mol)</odm2:defaultUnit>
    <rdf:type rdf:resource="http://www.w3.org/2004/02/skos/core#Concept"/>
    <odm2:dimensionCurrent>1</odm2:dimensionCurrent>
    <odm2:category>Electricity and Magnetism</odm2:category>
    <odm2:dimensionMass>0</odm2:dimensionMass>
    <odm2:dimensionTime>0</odm2:dimensionTime>
    <skos:inScheme rdf:resource="http://vocabulary.odm2.org/unitstype"/>
    <skos:exactMatch>http://qudt.org/vocab/quantity#Electricalchargepercount</skos:exactMatch>
    <skos:historyNote>QUDT</skos:historyNote>
  </rdf:Description>
  <rdf:Description rdf:about="http://vocabulary.odm2.org/unitstype/angularMass">
    <odm2:dimensionTemperature>0</odm2:dimensionTemperature>
    <odm2:category>Space and Time</odm2:category>
    <skos:exactMatch>http://qudt.org/schema/qudt#AngularMassUnit</skos:exactMatch>
    <odm2:defaultUnit>Kilogram Meter Squared (kg-m^2)</odm2:defaultUnit>
    <skos:historyNote>QUDT</skos:historyNote>
    <odm2:dimensionLight>0</odm2:dimensionLight>
    <odm2:dimensionTime>1</odm2:dimensionTime>
    <odm2:dimensionAmount>0</odm2:dimensionAmount>
    <skos:inScheme rdf:resource="http://vocabulary.odm2.org/unitstype"/>
    <odm2:dimensionCurrent>0</odm2:dimensionCurrent>
    <skos:prefLabel>Angular mass</skos:prefLabel>
    <odm2:dimensionSymbol>L2M1</odm2:dimensionSymbol>
    <odm2:dimensionLength>0</odm2:dimensionLength>
    <odm2:dimensionMass>2</odm2:dimensionMass>
    <skos:definition>The units of angular mass have dimensions of mass * area. They are used to measure the moment of inertia or rotational inertia.</skos:definition>
    <rdf:type rdf:resource="http://www.w3.org/2004/02/skos/core#Concept"/>
  </rdf:Description>
  <rdf:Description rdf:about="http://vocabulary.odm2.org/unitstype/absorbedDoseRate">
    <odm2:dimensionSymbol>L2T-3</odm2:dimensionSymbol>
    <odm2:dimensionTime>0</odm2:dimensionTime>
    <odm2:dimensionCurrent>-3</odm2:dimensionCurrent>
    <odm2:defaultUnit>Gray per second (Gy/s)</odm2:defaultUnit>
    <odm2:category>Radiology</odm2:category>
    <odm2:dimensionLight>0</odm2:dimensionLight>
    <odm2:dimensionTemperature>0</odm2:dimensionTemperature>
    <odm2:dimensionAmount>0</odm2:dimensionAmount>
    <skos:exactMatch>http://qudt.org/vocab/quantity#AbsorbedDoseRate</skos:exactMatch>
    <odm2:dimensionLength>0</odm2:dimensionLength>
    <skos:inScheme rdf:resource="http://vocabulary.odm2.org/unitstype"/>
    <rdf:type rdf:resource="http://www.w3.org/2004/02/skos/core#Concept"/>
    <odm2:dimensionMass>2</odm2:dimensionMass>
    <skos:definition>Absorbed dose per unit time.</skos:definition>
    <skos:historyNote>QUDT</skos:historyNote>
    <skos:prefLabel>Absorbed dose rate</skos:prefLabel>
  </rdf:Description>
  <rdf:Description rdf:about="http://vocabulary.odm2.org/unitstype/areaTimeTemperature">
    <rdf:type rdf:resource="http://www.w3.org/2004/02/skos/core#Concept"/>
    <odm2:dimensionMass>2</odm2:dimensionMass>
    <odm2:dimensionAmount>1</odm2:dimensionAmount>
    <odm2:dimensionSymbol>L2T1?1</odm2:dimensionSymbol>
    <odm2:dimensionLight>0</odm2:dimensionLight>
    <odm2:defaultUnit>Square Meter Second Kelvin</odm2:defaultUnit>
    <odm2:dimensionTime>0</odm2:dimensionTime>
    <skos:historyNote>QUDT</skos:historyNote>
    <skos:exactMatch>http://qudt.org/vocab/quantity#AreaTimeTemperature</skos:exactMatch>
    <odm2:dimensionTemperature>0</odm2:dimensionTemperature>
    <odm2:category>Thermodynamics</odm2:category>
    <skos:prefLabel>Area time temperature</skos:prefLabel>
    <odm2:dimensionCurrent>1</odm2:dimensionCurrent>
    <odm2:dimensionLength>0</odm2:dimensionLength>
    <skos:inScheme rdf:resource="http://vocabulary.odm2.org/unitstype"/>
  </rdf:Description>
  <rdf:Description rdf:about="http://vocabulary.odm2.org/unitstype/lengthIntegratedMassConcentration">
    <skos:note>Has same dimensionality as mass per unit area</skos:note>
    <odm2:dimensionSymbol>L-2M1</odm2:dimensionSymbol>
    <skos:prefLabel>Length integrated mass concentration</skos:prefLabel>
    <odm2:dimensionAmount>0</odm2:dimensionAmount>
    <rdf:type rdf:resource="http://www.w3.org/2004/02/skos/core#Concept"/>
    <odm2:dimensionLength>0</odm2:dimensionLength>
    <odm2:dimensionLight>0</odm2:dimensionLight>
    <skos:exactMatch>http://his.cuahsi.org/mastercvreg/edit_cv11.aspx?tbl=Units&amp;id=1125579048</skos:exactMatch>
    <skos:historyNote>CUAHSI</skos:historyNote>
    <odm2:dimensionTemperature>0</odm2:dimensionTemperature>
    <odm2:defaultUnit>kilograms per meter cubed per meter</odm2:defaultUnit>
    <odm2:dimensionMass>-2</odm2:dimensionMass>
    <skos:inScheme rdf:resource="http://vocabulary.odm2.org/unitstype"/>
    <odm2:category>Chemistry</odm2:category>
    <odm2:dimensionTime>1</odm2:dimensionTime>
    <odm2:dimensionCurrent>0</odm2:dimensionCurrent>
    <skos:definition>A mass concentration per unit length.  These units can be used to measure concentration inputs of a chemical along the length of a waterway.</skos:definition>
  </rdf:Description>
  <rdf:Description rdf:about="http://vocabulary.odm2.org/unitstype/temperaturePerTime">
    <odm2:dimensionMass>0</odm2:dimensionMass>
    <odm2:dimensionLight>0</odm2:dimensionLight>
    <odm2:dimensionCurrent>-1</odm2:dimensionCurrent>
    <skos:historyNote>QUDT</skos:historyNote>
    <odm2:dimensionTime>0</odm2:dimensionTime>
    <skos:inScheme rdf:resource="http://vocabulary.odm2.org/unitstype"/>
    <odm2:dimensionTemperature>0</odm2:dimensionTemperature>
    <odm2:dimensionSymbol>T-1?1</odm2:dimensionSymbol>
    <odm2:category>Thermodynamics</odm2:category>
    <odm2:dimensionLength>0</odm2:dimensionLength>
    <skos:exactMatch>http://qudt.org/vocab/quantity#TemperaturePerTime</skos:exactMatch>
    <skos:prefLabel>Temperature per time</skos:prefLabel>
    <odm2:defaultUnit>Kelvin per second (K/s)</odm2:defaultUnit>
    <odm2:dimensionAmount>1</odm2:dimensionAmount>
    <rdf:type rdf:resource="http://www.w3.org/2004/02/skos/core#Concept"/>
  </rdf:Description>
  <rdf:Description rdf:about="http://vocabulary.odm2.org/unitstype/fluidPermeance">
    <odm2:category>Fluid Mechanics</odm2:category>
    <odm2:dimensionSymbol>L-1T1</odm2:dimensionSymbol>
    <skos:historyNote>Wikipedia</skos:historyNote>
    <rdf:type rdf:resource="http://www.w3.org/2004/02/skos/core#Concept"/>
    <skos:inScheme rdf:resource="http://vocabulary.odm2.org/unitstype"/>
    <skos:prefLabel>Fluid permeance</skos:prefLabel>
    <skos:definition>Permeance is closely related to permeability, but it refers to the extent of penetration of a specific object with given thickness by a liquid or a gas.  It is the degee to which a materal or membrane transmits another substance.  Units of permeance are volumetric output per unit membrane area per unit trans-membrane pressure. Permeance is also referred to as pressure-normalized flux.</skos:definition>
    <odm2:dimensionCurrent>1</odm2:dimensionCurrent>
    <odm2:dimensionTemperature>0</odm2:dimensionTemperature>
    <odm2:defaultUnit>Kilograms per pascal per second per meter squared</odm2:defaultUnit>
    <odm2:dimensionAmount>0</odm2:dimensionAmount>
    <odm2:dimensionMass>-1</odm2:dimensionMass>
    <odm2:dimensionTime>0</odm2:dimensionTime>
    <odm2:dimensionLight>0</odm2:dimensionLight>
    <odm2:dimensionLength>0</odm2:dimensionLength>
  </rdf:Description>
  <rdf:Description rdf:about="http://vocabulary.odm2.org/unitstype/inverseTimeTemperature">
    <odm2:dimensionAmount>-1</odm2:dimensionAmount>
    <odm2:category>Thermodynamics</odm2:category>
    <odm2:dimensionMass>0</odm2:dimensionMass>
    <odm2:dimensionSymbol>T-1?-1</odm2:dimensionSymbol>
    <odm2:dimensionTime>0</odm2:dimensionTime>
    <odm2:defaultUnit>Hertz per Kelvin (Hz/K)</odm2:defaultUnit>
    <skos:exactMatch>http://qudt.org/vocab/quantity#Inversetimetemperature</skos:exactMatch>
    <rdf:type rdf:resource="http://www.w3.org/2004/02/skos/core#Concept"/>
    <odm2:dimensionCurrent>-1</odm2:dimensionCurrent>
    <skos:inScheme rdf:resource="http://vocabulary.odm2.org/unitstype"/>
    <skos:prefLabel>Inverse time temperature</skos:prefLabel>
    <odm2:dimensionTemperature>0</odm2:dimensionTemperature>
    <skos:historyNote>QUDT</skos:historyNote>
    <odm2:dimensionLength>0</odm2:dimensionLength>
    <odm2:dimensionLight>0</odm2:dimensionLight>
  </rdf:Description>
  <rdf:Description rdf:about="http://vocabulary.odm2.org/unitstype/magneticFluxDensity">
    <odm2:dimensionAmount>0</odm2:dimensionAmount>
    <skos:exactMatch>http://qudt.org/schema/qudt#MagneticFluxDensityUnit</skos:exactMatch>
    <odm2:dimensionLength>0</odm2:dimensionLength>
    <skos:inScheme rdf:resource="http://vocabulary.odm2.org/unitstype"/>
    <odm2:defaultUnit>Tesla (T)</odm2:defaultUnit>
    <odm2:dimensionCurrent>-2</odm2:dimensionCurrent>
    <skos:definition>The Magnetic flux density, B (also called magnetic induction or magnetic field), is a fundamental field in electrodynamics which characterizes the magnetic force exerted by electric currents. It is closely related to the auxillary magnetic field H.</skos:definition>
    <odm2:category>Electricity and Magnetism</odm2:category>
    <odm2:dimensionLight>0</odm2:dimensionLight>
    <skos:prefLabel>Magnetic flux density</skos:prefLabel>
    <skos:historyNote>QUDT</skos:historyNote>
    <rdf:type rdf:resource="http://www.w3.org/2004/02/skos/core#Concept"/>
    <odm2:dimensionSymbol>M1T-2I-1</odm2:dimensionSymbol>
    <odm2:dimensionTime>1</odm2:dimensionTime>
    <odm2:dimensionTemperature>-1</odm2:dimensionTemperature>
    <odm2:dimensionMass>0</odm2:dimensionMass>
  </rdf:Description>
  <rdf:Description rdf:about="http://vocabulary.odm2.org/unitstype/volumetricProductivity">
    <odm2:dimensionSymbol>L-3M1T-1</odm2:dimensionSymbol>
    <odm2:dimensionTemperature>0</odm2:dimensionTemperature>
    <odm2:dimensionCurrent>-1</odm2:dimensionCurrent>
    <odm2:dimensionTime>1</odm2:dimensionTime>
    <odm2:dimensionLength>0</odm2:dimensionLength>
    <skos:inScheme rdf:resource="http://vocabulary.odm2.org/unitstype"/>
    <skos:prefLabel>Volumetric productivity</skos:prefLabel>
    <odm2:dimensionLight>0</odm2:dimensionLight>
    <odm2:defaultUnit>Kilograms per cubic meter per second</odm2:defaultUnit>
    <skos:definition>In ecology, productivity or production refers to the rate of generation of biomass in an ecosystem. It is usually expressed in units of mass per unit surface (or volume) per unit time, for instance grams per square metre per day (g m?2 d?1). The mass unit may relate to dry matter or to the mass of carbon generated. Productivity of autotrophs such as plants is called primary productivity, while that of heterotrophs such as animals is called secondary productivity. [Wikipedia: https://en.wikipedia.org/wiki/Productivity_%28ecology%29]</skos:definition>
    <skos:historyNote>CUAHSI</skos:historyNote>
    <odm2:category>Chemistry</odm2:category>
    <rdf:type rdf:resource="http://www.w3.org/2004/02/skos/core#Concept"/>
    <odm2:dimensionAmount>0</odm2:dimensionAmount>
    <odm2:dimensionMass>-3</odm2:dimensionMass>
  </rdf:Description>
  <rdf:Description rdf:about="http://vocabulary.odm2.org/unitstype/temperatureCount">
    <odm2:category>Thermodynamics</odm2:category>
    <odm2:dimensionTemperature>0</odm2:dimensionTemperature>
    <odm2:dimensionAmount>1</odm2:dimensionAmount>
    <odm2:dimensionMass>0</odm2:dimensionMass>
    <odm2:dimensionLight>1</odm2:dimensionLight>
    <skos:historyNote>QUDT</skos:historyNote>
    <odm2:defaultUnit>Mole kelvin (mol-K)</odm2:defaultUnit>
    <odm2:dimensionSymbol>?1N1</odm2:dimensionSymbol>
    <rdf:type rdf:resource="http://www.w3.org/2004/02/skos/core#Concept"/>
    <odm2:dimensionCurrent>0</odm2:dimensionCurrent>
    <odm2:dimensionTime>0</odm2:dimensionTime>
    <skos:exactMatch>http://qudt.org/schema/qudt#AmountOfSubstanceTemperatureUnit</skos:exactMatch>
    <skos:prefLabel>Temperature count</skos:prefLabel>
    <skos:inScheme rdf:resource="http://vocabulary.odm2.org/unitstype"/>
    <odm2:dimensionLength>0</odm2:dimensionLength>
  </rdf:Description>
  <rdf:Description rdf:about="http://vocabulary.odm2.org/unitstype/thermalInsulance">
    <rdf:type rdf:resource="http://www.w3.org/2004/02/skos/core#Concept"/>
    <odm2:dimensionAmount>1</odm2:dimensionAmount>
    <odm2:dimensionMass>0</odm2:dimensionMass>
    <odm2:dimensionLight>0</odm2:dimensionLight>
    <odm2:dimensionCurrent>3</odm2:dimensionCurrent>
    <odm2:category>Thermodynamics</odm2:category>
    <skos:inScheme rdf:resource="http://vocabulary.odm2.org/unitstype"/>
    <odm2:dimensionTemperature>0</odm2:dimensionTemperature>
    <skos:definition>The inverse of the heat transfer coefficient.</skos:definition>
    <skos:prefLabel>Thermal insulance</skos:prefLabel>
    <skos:historyNote>QUDT</skos:historyNote>
    <odm2:dimensionSymbol>M-1T3?1</odm2:dimensionSymbol>
    <skos:exactMatch>http://qudt.org/vocab/quantity#Thermalinsulance</skos:exactMatch>
    <odm2:dimensionTime>-1</odm2:dimensionTime>
    <odm2:dimensionLength>0</odm2:dimensionLength>
    <odm2:defaultUnit>Square meter Kelvin per watt (K(m^2)/W)</odm2:defaultUnit>
  </rdf:Description>
  <rdf:Description rdf:about="http://vocabulary.odm2.org/unitstype/linearVelocity">
    <odm2:dimensionTemperature>0</odm2:dimensionTemperature>
    <odm2:dimensionLight>0</odm2:dimensionLight>
    <odm2:category>Mechanics</odm2:category>
    <odm2:dimensionCurrent>-1</odm2:dimensionCurrent>
    <skos:inScheme rdf:resource="http://vocabulary.odm2.org/unitstype"/>
    <skos:historyNote>QUDT</skos:historyNote>
    <odm2:dimensionLength>0</odm2:dimensionLength>
    <skos:definition>Velocity is the rate of change of the position of an object, equivalent to a specification of its speed and direction of motion.Velocity is an important concept in kinematics, the branch of classical mechanics which describes the motion of bodies.Velocity is a vector physical quantity; both magnitude and direction are required to define it. The scalar absolute value (magnitude) of velocity is called "speed", a quantity that is measured in metres per second (m/s or m·s?1) in the SI (metric) system.</skos:definition>
    <skos:note>This has the same dimensionality as volumetric flux, but is expressed differently.</skos:note>
    <odm2:dimensionSymbol>L1T-1</odm2:dimensionSymbol>
    <skos:exactMatch>http://qudt.org/vocab/quantity#Linearvelocity</skos:exactMatch>
    <odm2:dimensionAmount>0</odm2:dimensionAmount>
    <rdf:type rdf:resource="http://www.w3.org/2004/02/skos/core#Concept"/>
    <odm2:defaultUnit>Meter per second (m/s)</odm2:defaultUnit>
    <odm2:dimensionTime>0</odm2:dimensionTime>
    <odm2:dimensionMass>1</odm2:dimensionMass>
    <skos:prefLabel>Linear velocity</skos:prefLabel>
  </rdf:Description>
  <rdf:Description rdf:about="http://vocabulary.odm2.org/unitstype/massPerElectricalCharge">
    <odm2:dimensionTemperature>-1</odm2:dimensionTemperature>
    <odm2:dimensionTime>1</odm2:dimensionTime>
    <skos:prefLabel>Mass per electrical charge</skos:prefLabel>
    <odm2:dimensionCurrent>1</odm2:dimensionCurrent>
    <skos:exactMatch>http://qudt.org/vocab/quantity#MassPerElectricCharge</skos:exactMatch>
    <odm2:dimensionLength>0</odm2:dimensionLength>
    <skos:inScheme rdf:resource="http://vocabulary.odm2.org/unitstype"/>
    <odm2:category>Chemistry</odm2:category>
    <rdf:type rdf:resource="http://www.w3.org/2004/02/skos/core#Concept"/>
    <odm2:defaultUnit>Tesla Second (T s)</odm2:defaultUnit>
    <odm2:dimensionMass>0</odm2:dimensionMass>
    <odm2:dimensionLight>0</odm2:dimensionLight>
    <odm2:dimensionSymbol>M1T-1I-1</odm2:dimensionSymbol>
    <odm2:dimensionAmount>0</odm2:dimensionAmount>
    <skos:historyNote>QUDT</skos:historyNote>
  </rdf:Description>
  <rdf:Description rdf:about="http://vocabulary.odm2.org/unitstype/doseEquivalent">
    <odm2:dimensionTime>0</odm2:dimensionTime>
    <odm2:dimensionLight>0</odm2:dimensionLight>
    <odm2:dimensionAmount>0</odm2:dimensionAmount>
    <odm2:category>Radiology</odm2:category>
    <odm2:defaultUnit>Sievert (Sv)</odm2:defaultUnit>
    <odm2:dimensionTemperature>0</odm2:dimensionTemperature>
    <skos:exactMatch>http://qudt.org/vocab/quantity#DoseEquivalent</skos:exactMatch>
    <skos:note>Absorbed dose, does equivalent, and specific energy all have the same dimensionality.</skos:note>
    <odm2:dimensionLength>0</odm2:dimensionLength>
    <skos:historyNote>QUDT</skos:historyNote>
    <odm2:dimensionSymbol>L2T-2</odm2:dimensionSymbol>
    <odm2:dimensionMass>2</odm2:dimensionMass>
    <rdf:type rdf:resource="http://www.w3.org/2004/02/skos/core#Concept"/>
    <skos:inScheme rdf:resource="http://vocabulary.odm2.org/unitstype"/>
    <odm2:dimensionCurrent>-2</odm2:dimensionCurrent>
    <skos:prefLabel>Dose equivalent</skos:prefLabel>
    <skos:definition>Equivalent dose or radiation dosage is a dose quantity used in radiological protection to represent the stochastic health effects (probability of cancer induction and genetic damage) of low levels of ionizing radiation on the human body. It is based on the physical quantity absorbed dose, but takes into account the biological effectiveness of the radiation, which is dependent on the radiation type and energy. [Wikipedia: https://en.wikipedia.org/wiki/Absorbed_dose]</skos:definition>
  </rdf:Description>
  <rdf:Description rdf:about="http://vocabulary.odm2.org/unitstype/lengthPerMagneticFlux">
    <odm2:dimensionCurrent>2</odm2:dimensionCurrent>
    <odm2:dimensionMass>-1</odm2:dimensionMass>
    <odm2:defaultUnit>per Tesla Meter</odm2:defaultUnit>
    <odm2:dimensionTime>-1</odm2:dimensionTime>
    <skos:prefLabel>Length per magnetic flux</skos:prefLabel>
    <odm2:dimensionLength>0</odm2:dimensionLength>
    <skos:inScheme rdf:resource="http://vocabulary.odm2.org/unitstype"/>
    <odm2:category>Electricity and Magnetism</odm2:category>
    <rdf:type rdf:resource="http://www.w3.org/2004/02/skos/core#Concept"/>
    <odm2:dimensionLight>0</odm2:dimensionLight>
    <odm2:dimensionSymbol>L-1M-1T2I1</odm2:dimensionSymbol>
    <odm2:dimensionAmount>0</odm2:dimensionAmount>
    <skos:historyNote>QUDT</skos:historyNote>
    <skos:exactMatch>http://qudt.org/vocab/quantity#Lengthperunitmagneticflux</skos:exactMatch>
    <odm2:dimensionTemperature>1</odm2:dimensionTemperature>
  </rdf:Description>
  <rdf:Description rdf:about="http://vocabulary.odm2.org/unitstype/dynamicViscosity">
    <skos:exactMatch>http://qudt.org/vocab/quantity#Dynamicviscosity</skos:exactMatch>
    <skos:prefLabel>Dynamic viscosity</skos:prefLabel>
    <odm2:defaultUnit>Pascal second (Pa-s)</odm2:defaultUnit>
    <odm2:dimensionCurrent>-1</odm2:dimensionCurrent>
    <odm2:dimensionLength>0</odm2:dimensionLength>
    <skos:inScheme rdf:resource="http://vocabulary.odm2.org/unitstype"/>
    <odm2:dimensionLight>0</odm2:dimensionLight>
    <odm2:dimensionTemperature>0</odm2:dimensionTemperature>
    <odm2:dimensionMass>-1</odm2:dimensionMass>
    <skos:historyNote>QUDT</skos:historyNote>
    <odm2:dimensionSymbol>L-1M1T-1</odm2:dimensionSymbol>
    <rdf:type rdf:resource="http://www.w3.org/2004/02/skos/core#Concept"/>
    <skos:definition>The dynamic (shear) viscosity of a fluid expresses its resistance to shearing flows, where adjacent layers move parallel to each other with different speeds. Both the physical unit of dynamic viscosity in SI Poiseuille (Pl) and the cgs units Poise (P) come from Jean Léonard Marie Poiseuille. The poiseuille, which is never used, is equivalent to the pascal-second (Pa·s), or (N·s)/m2, or kg/(m·s).</skos:definition>
    <odm2:category>Fluid Mechanics</odm2:category>
    <skos:note>Also https://en.wikipedia.org/wiki/Viscosity#Dynamic_viscosity_.CE.BC</skos:note>
    <odm2:dimensionAmount>0</odm2:dimensionAmount>
    <odm2:dimensionTime>1</odm2:dimensionTime>
  </rdf:Description>
  <rdf:Description rdf:about="http://vocabulary.odm2.org/unitstype/concentrationOrDensityMassPerVolume">
    <odm2:dimensionTemperature>0</odm2:dimensionTemperature>
    <odm2:dimensionLength>0</odm2:dimensionLength>
    <skos:definition>The mass of one substance per unit volume of another substance.  These units are commonly used in both density and concentration measurements</skos:definition>
    <odm2:defaultUnit>Kilogram per cubic meter (kg/m^3)</odm2:defaultUnit>
    <odm2:dimensionMass>-3</odm2:dimensionMass>
    <skos:exactMatch>http://dbpedia.org/page/Gram_per_litre</skos:exactMatch>
    <rdf:type rdf:resource="http://www.w3.org/2004/02/skos/core#Concept"/>
    <odm2:dimensionTime>1</odm2:dimensionTime>
    <odm2:dimensionSymbol>L-3M1</odm2:dimensionSymbol>
    <odm2:dimensionAmount>0</odm2:dimensionAmount>
    <skos:inScheme rdf:resource="http://vocabulary.odm2.org/unitstype"/>
    <skos:historyNote>Wikipedia</skos:historyNote>
    <skos:prefLabel>Concentration or density mass per volume</skos:prefLabel>
    <odm2:dimensionLight>0</odm2:dimensionLight>
    <odm2:category>Chemistry</odm2:category>
    <odm2:dimensionCurrent>0</odm2:dimensionCurrent>
  </rdf:Description>
  <rdf:Description rdf:about="http://vocabulary.odm2.org/unitstype/volumetricFlowRate">
    <odm2:dimensionLight>0</odm2:dimensionLight>
    <odm2:dimensionTime>0</odm2:dimensionTime>
    <odm2:dimensionSymbol>L3T-1</odm2:dimensionSymbol>
    <odm2:dimensionMass>3</odm2:dimensionMass>
    <skos:prefLabel>Volumetric flow rate</skos:prefLabel>
    <odm2:category>Mechanics</odm2:category>
    <skos:inScheme rdf:resource="http://vocabulary.odm2.org/unitstype"/>
    <skos:exactMatch>http://qudt.org/vocab/quantity#Volumepertime</skos:exactMatch>
    <skos:definition>Volume Per Unit Time, or Volumetric flow rate, is the volume of fluid that passes through a given surface per unit of time (as opposed to a unit surface).</skos:definition>
    <odm2:dimensionAmount>0</odm2:dimensionAmount>
    <odm2:dimensionLength>0</odm2:dimensionLength>
    <skos:historyNote>QUDT</skos:historyNote>
    <odm2:dimensionTemperature>0</odm2:dimensionTemperature>
    <rdf:type rdf:resource="http://www.w3.org/2004/02/skos/core#Concept"/>
    <odm2:dimensionCurrent>-1</odm2:dimensionCurrent>
    <odm2:defaultUnit>Cubic meter per second (m^3/s)</odm2:defaultUnit>
  </rdf:Description>
  <rdf:Description rdf:about="http://vocabulary.odm2.org/unitstype/specificHeatPressure">
    <skos:prefLabel>Specific heat pressure</skos:prefLabel>
    <odm2:dimensionMass>3</odm2:dimensionMass>
    <odm2:defaultUnit>Joule per kilogram kelvin per pascal (J/(km-K-Pa))</odm2:defaultUnit>
    <odm2:dimensionSymbol>L3M-1?-1</odm2:dimensionSymbol>
    <odm2:dimensionLight>0</odm2:dimensionLight>
    <skos:definition>Specific heat at a constant pressure.</skos:definition>
    <odm2:category>Thermodynamics</odm2:category>
    <odm2:dimensionCurrent>0</odm2:dimensionCurrent>
    <odm2:dimensionLength>0</odm2:dimensionLength>
    <skos:inScheme rdf:resource="http://vocabulary.odm2.org/unitstype"/>
    <rdf:type rdf:resource="http://www.w3.org/2004/02/skos/core#Concept"/>
    <skos:exactMatch>http://qudt.org/vocab/quantity#Specificheatpressure</skos:exactMatch>
    <odm2:dimensionTemperature>0</odm2:dimensionTemperature>
    <skos:historyNote>QUDT</skos:historyNote>
    <odm2:dimensionAmount>-1</odm2:dimensionAmount>
    <odm2:dimensionTime>-1</odm2:dimensionTime>
  </rdf:Description>
  <rdf:Description rdf:about="http://vocabulary.odm2.org/unitstype/forcePerLength">
    <odm2:dimensionTime>1</odm2:dimensionTime>
    <skos:exactMatch>http://qudt.org/vocab/quantity#Forceperlength</skos:exactMatch>
    <odm2:dimensionAmount>0</odm2:dimensionAmount>
    <odm2:dimensionLength>0</odm2:dimensionLength>
    <odm2:dimensionSymbol>M1T-2</odm2:dimensionSymbol>
    <rdf:type rdf:resource="http://www.w3.org/2004/02/skos/core#Concept"/>
    <odm2:dimensionLight>0</odm2:dimensionLight>
    <skos:note>Has the same dimensionality as energy per area.</skos:note>
    <odm2:defaultUnit>Newton per meter (N/m)</odm2:defaultUnit>
    <odm2:dimensionMass>0</odm2:dimensionMass>
    <odm2:category>Mechanics</odm2:category>
    <odm2:dimensionCurrent>-2</odm2:dimensionCurrent>
    <skos:definition>The amount of force applied per unit length.  Frequenty used for surface tension.</skos:definition>
    <skos:inScheme rdf:resource="http://vocabulary.odm2.org/unitstype"/>
    <skos:prefLabel>Force per length</skos:prefLabel>
    <odm2:dimensionTemperature>0</odm2:dimensionTemperature>
    <skos:historyNote>QUDT</skos:historyNote>
  </rdf:Description>
  <rdf:Description rdf:about="http://vocabulary.odm2.org/unitstype/biologicalActivity">
    <skos:historyNote>Wikipedia</skos:historyNote>
    <skos:exactMatch>http://dbpedia.org/page/Biological_activity</skos:exactMatch>
    <odm2:dimensionAmount>0</odm2:dimensionAmount>
    <rdf:type rdf:resource="http://www.w3.org/2004/02/skos/core#Concept"/>
    <odm2:category>Chemistry</odm2:category>
    <skos:prefLabel>Biological activity</skos:prefLabel>
    <skos:definition>Units used mainly in chemical and biochemical laboratories.</skos:definition>
    <skos:inScheme rdf:resource="http://vocabulary.odm2.org/unitstype"/>
    <odm2:dimensionTime>0</odm2:dimensionTime>
    <odm2:dimensionSymbol>T-1</odm2:dimensionSymbol>
    <odm2:dimensionTemperature>0</odm2:dimensionTemperature>
    <skos:note>Medical term - many specific arbitrary units based on different substances.  Do not use conversions within this unit group!</skos:note>
    <odm2:dimensionLight>0</odm2:dimensionLight>
    <odm2:dimensionMass>0</odm2:dimensionMass>
    <odm2:dimensionCurrent>-1</odm2:dimensionCurrent>
    <odm2:dimensionLength>0</odm2:dimensionLength>
  </rdf:Description>
  <rdf:Description rdf:about="http://vocabulary.odm2.org/unitstype/illuminance">
    <skos:prefLabel>Illuminance</skos:prefLabel>
    <odm2:defaultUnit>Lux (lx); Lumen per square meter (lm/m^2)</odm2:defaultUnit>
    <skos:exactMatch>http://qudt.org/vocab/quantity#Illuminance</skos:exactMatch>
    <odm2:dimensionLength>1</odm2:dimensionLength>
    <odm2:dimensionAmount>0</odm2:dimensionAmount>
    <odm2:dimensionSymbol>U1L-2J1</odm2:dimensionSymbol>
    <skos:definition>Illuminance (also know as luminous emittance or luminous flux per area), is the total luminous flux incident on a surface, per unit area. It is a measure of the intensity of the incident light, wavelength-weighted by the luminosity function to correlate with human brightness perception.</skos:definition>
    <rdf:type rdf:resource="http://www.w3.org/2004/02/skos/core#Concept"/>
    <odm2:dimensionLight>0</odm2:dimensionLight>
    <odm2:dimensionTemperature>0</odm2:dimensionTemperature>
    <odm2:dimensionCurrent>0</odm2:dimensionCurrent>
    <skos:inScheme rdf:resource="http://vocabulary.odm2.org/unitstype"/>
    <odm2:category>Photometry</odm2:category>
    <odm2:dimensionTime>0</odm2:dimensionTime>
    <skos:historyNote>QUDT</skos:historyNote>
    <odm2:dimensionMass>-2</odm2:dimensionMass>
  </rdf:Description>
  <rdf:Description rdf:about="http://vocabulary.odm2.org/unitstype/energyPerArea">
    <odm2:dimensionTime>1</odm2:dimensionTime>
    <skos:definition>Energy per area density is the amount of energy stored in a given system or region of space per unit area.  Has the same dimensionality as force per unit length.</skos:definition>
    <odm2:dimensionAmount>0</odm2:dimensionAmount>
    <odm2:defaultUnit>Joule per square meter (J/m^2)</odm2:defaultUnit>
    <odm2:dimensionLength>0</odm2:dimensionLength>
    <odm2:dimensionSymbol>M1T-2</odm2:dimensionSymbol>
    <rdf:type rdf:resource="http://www.w3.org/2004/02/skos/core#Concept"/>
    <odm2:dimensionLight>0</odm2:dimensionLight>
    <odm2:dimensionTemperature>0</odm2:dimensionTemperature>
    <odm2:dimensionMass>0</odm2:dimensionMass>
    <odm2:category>Mechanics</odm2:category>
    <odm2:dimensionCurrent>-2</odm2:dimensionCurrent>
    <skos:inScheme rdf:resource="http://vocabulary.odm2.org/unitstype"/>
    <skos:prefLabel>Energy per area</skos:prefLabel>
    <skos:exactMatch>http://qudt.org/vocab/quantity#Energyperarea</skos:exactMatch>
    <skos:historyNote>QUDT</skos:historyNote>
  </rdf:Description>
  <rdf:Description rdf:about="http://vocabulary.odm2.org/unitstype/electricalCurrentDensity">
    <odm2:dimensionLength>0</odm2:dimensionLength>
    <skos:historyNote>QUDT</skos:historyNote>
    <odm2:dimensionSymbol>L-2I1</odm2:dimensionSymbol>
    <rdf:type rdf:resource="http://www.w3.org/2004/02/skos/core#Concept"/>
    <skos:inScheme rdf:resource="http://vocabulary.odm2.org/unitstype"/>
    <skos:definition>Electric current density is a measure of the density of flow of electric charge; it is the electric current per unit area of cross section. Electric current density is a vector-valued quantity.</skos:definition>
    <odm2:dimensionCurrent>0</odm2:dimensionCurrent>
    <odm2:dimensionTemperature>1</odm2:dimensionTemperature>
    <odm2:defaultUnit>Ampere per square meter (A/m^2)</odm2:defaultUnit>
    <skos:prefLabel>Electrical current density</skos:prefLabel>
    <odm2:dimensionTime>0</odm2:dimensionTime>
    <odm2:dimensionLight>0</odm2:dimensionLight>
    <odm2:dimensionAmount>0</odm2:dimensionAmount>
    <odm2:category>Electricity and Magnetism</odm2:category>
    <odm2:dimensionMass>-2</odm2:dimensionMass>
    <skos:exactMatch>http://qudt.org/vocab/quantity#Electricalcurrentdensity</skos:exactMatch>
  </rdf:Description>
  <rdf:Description rdf:about="http://vocabulary.odm2.org/unitstype/temperaturePerMagneticFluxDensity">
    <odm2:dimensionLength>0</odm2:dimensionLength>
    <odm2:defaultUnit>Kelvin per Tesla</odm2:defaultUnit>
    <skos:inScheme rdf:resource="http://vocabulary.odm2.org/unitstype"/>
    <odm2:dimensionTemperature>1</odm2:dimensionTemperature>
    <odm2:category>Thermodynamics</odm2:category>
    <odm2:dimensionAmount>1</odm2:dimensionAmount>
    <odm2:dimensionMass>0</odm2:dimensionMass>
    <skos:prefLabel>Temperature per magnetic flux density</skos:prefLabel>
    <odm2:dimensionCurrent>2</odm2:dimensionCurrent>
    <skos:historyNote>QUDT</skos:historyNote>
    <rdf:type rdf:resource="http://www.w3.org/2004/02/skos/core#Concept"/>
    <odm2:dimensionTime>-1</odm2:dimensionTime>
    <skos:exactMatch>http://qudt.org/vocab/quantity#TemperaturePerMagneticFluxDensity</skos:exactMatch>
    <odm2:dimensionLight>0</odm2:dimensionLight>
    <odm2:dimensionSymbol>M-1T2I1?1</odm2:dimensionSymbol>
  </rdf:Description>
  <rdf:Description rdf:about="http://vocabulary.odm2.org/unitstype/molarConductivity">
    <odm2:category>Chemistry</odm2:category>
    <odm2:dimensionCurrent>0</odm2:dimensionCurrent>
    <rdf:type rdf:resource="http://www.w3.org/2004/02/skos/core#Concept"/>
    <odm2:dimensionTime>-1</odm2:dimensionTime>
    <odm2:dimensionLight>-1</odm2:dimensionLight>
    <skos:definition>Molar conductivity is defined as the conductivity of an electrolyte solution divided by the molar concentration of the electrolyte, and so measures the efficiency with which a given electrolyte conducts electricity in solution. Its units are siemens per meter per molarity, or siemens meter-squared per mole. The usual symbol is a capital lambda, ?, or ?m. Or Molar conductivity of a solution at a given concentration is the conductance of the volume (V) of the solution containing one mole of electrolyte kept between two electrodes with area of cross section (A) and at a distance of unit length. [Wikipedia: https://en.wikipedia.org/wiki/Molar_conductivity]</skos:definition>
    <skos:inScheme rdf:resource="http://vocabulary.odm2.org/unitstype"/>
    <skos:historyNote>Aquarius</skos:historyNote>
    <odm2:defaultUnit>Siemen Square Meter per Mole (Sm^2/mol)</odm2:defaultUnit>
    <odm2:dimensionLength>0</odm2:dimensionLength>
    <odm2:dimensionAmount>0</odm2:dimensionAmount>
    <odm2:dimensionMass>0</odm2:dimensionMass>
    <skos:prefLabel>Molar conductivity</skos:prefLabel>
    <odm2:dimensionSymbol>M-1I2N-1</odm2:dimensionSymbol>
    <odm2:dimensionTemperature>2</odm2:dimensionTemperature>
  </rdf:Description>
  <rdf:Description rdf:about="http://vocabulary.odm2.org/unitstype/timeSquared">
    <skos:inScheme rdf:resource="http://vocabulary.odm2.org/unitstype"/>
    <odm2:defaultUnit>Second time squared (s^2)</odm2:defaultUnit>
    <odm2:dimensionSymbol>T2</odm2:dimensionSymbol>
    <rdf:type rdf:resource="http://www.w3.org/2004/02/skos/core#Concept"/>
    <skos:exactMatch>http://qudt.org/vocab/quantity#Timesquared</skos:exactMatch>
    <odm2:dimensionTime>0</odm2:dimensionTime>
    <skos:prefLabel>Time squared</skos:prefLabel>
    <odm2:dimensionTemperature>0</odm2:dimensionTemperature>
    <odm2:dimensionLength>0</odm2:dimensionLength>
    <odm2:dimensionAmount>0</odm2:dimensionAmount>
    <skos:historyNote>QUDT</skos:historyNote>
    <odm2:category>Space and Time</odm2:category>
    <odm2:dimensionLight>0</odm2:dimensionLight>
    <odm2:dimensionMass>0</odm2:dimensionMass>
    <odm2:dimensionCurrent>2</odm2:dimensionCurrent>
  </rdf:Description>
  <rdf:Description rdf:about="http://vocabulary.odm2.org/unitstype/massFraction">
    <odm2:dimensionSymbol>M1M-1</odm2:dimensionSymbol>
    <odm2:dimensionTemperature>0</odm2:dimensionTemperature>
    <odm2:dimensionLight>0</odm2:dimensionLight>
    <odm2:dimensionLength>0</odm2:dimensionLength>
    <skos:historyNote>Wikipedia</skos:historyNote>
    <odm2:category>Dimensionless Ratio</odm2:category>
    <skos:inScheme rdf:resource="http://vocabulary.odm2.org/unitstype"/>
    <odm2:defaultUnit>g/kg</odm2:defaultUnit>
    <skos:prefLabel>Mass fraction</skos:prefLabel>
    <odm2:dimensionCurrent>0</odm2:dimensionCurrent>
    <rdf:type rdf:resource="http://www.w3.org/2004/02/skos/core#Concept"/>
    <skos:exactMatch>http://dbpedia.org/page/Mass_fraction_(chemistry)</skos:exactMatch>
    <odm2:dimensionMass>0</odm2:dimensionMass>
    <odm2:dimensionAmount>0</odm2:dimensionAmount>
    <skos:definition>In chemistry, the mass fraction is the ratio of one substance with mass to the mass of the total mixture , defined asThe sum of all the mass fractions is equal to 1:Mass fraction can also be expressed, with a denominator of 100, as percentage by weight (wt%). It is one way of expressing the composition of a mixture in a dimensionless size; mole fraction (percentage by moles, mol%) and volume fraction (percentage by volume, vol%) are others. For elemental analysis, mass fraction (or "mass percent composition") can also refer to the ratio of the mass of one element to the total mass of a compound. It can be calculated for any compound using its empirical formula. or its chemical formula</skos:definition>
    <odm2:dimensionTime>0</odm2:dimensionTime>
  </rdf:Description>
  <rdf:Description rdf:about="http://vocabulary.odm2.org/unitstype/energyPerSquareMagneticFluxDensity">
    <odm2:dimensionAmount>0</odm2:dimensionAmount>
    <odm2:defaultUnit>Joule per Square Tesla (J/T^2)</odm2:defaultUnit>
    <odm2:dimensionCurrent>2</odm2:dimensionCurrent>
    <odm2:dimensionLength>0</odm2:dimensionLength>
    <odm2:dimensionTemperature>1</odm2:dimensionTemperature>
    <rdf:type rdf:resource="http://www.w3.org/2004/02/skos/core#Concept"/>
    <skos:exactMatch>http://qudt.org/vocab/quantity#EnergyPerSquareMagneticFluxDensity</skos:exactMatch>
    <odm2:dimensionLight>0</odm2:dimensionLight>
    <skos:historyNote>QUDT</skos:historyNote>
    <odm2:dimensionTime>-1</odm2:dimensionTime>
    <odm2:category>Electricity and Magnetism</odm2:category>
    <skos:prefLabel>Energy per square magnetic flux density</skos:prefLabel>
    <odm2:dimensionMass>2</odm2:dimensionMass>
    <odm2:dimensionSymbol>L2M-1T2I1</odm2:dimensionSymbol>
    <skos:inScheme rdf:resource="http://vocabulary.odm2.org/unitstype"/>
  </rdf:Description>
  <rdf:Description rdf:about="http://vocabulary.odm2.org/unitstype/specificRadioactivity">
    <odm2:category>Quantum Mechanics</odm2:category>
    <odm2:dimensionAmount>0</odm2:dimensionAmount>
    <odm2:dimensionLength>0</odm2:dimensionLength>
    <odm2:dimensionLight>0</odm2:dimensionLight>
    <skos:definition>Specific activity is the activity per mass quantity of a radionuclide and is a physical property of that radionuclide. [Wikipedia: https://en.wikipedia.org/wiki/Specific_activity]</skos:definition>
    <skos:exactMatch>http://dbpedia.org/page/Specific_activity</skos:exactMatch>
    <rdf:type rdf:resource="http://www.w3.org/2004/02/skos/core#Concept"/>
    <odm2:dimensionMass>0</odm2:dimensionMass>
    <odm2:dimensionTemperature>0</odm2:dimensionTemperature>
    <skos:historyNote>CUAHSI</skos:historyNote>
    <odm2:defaultUnit>Becquerels per gram (Bq/g)</odm2:defaultUnit>
    <odm2:dimensionSymbol>M-1T-1</odm2:dimensionSymbol>
    <skos:prefLabel>Specific radioactivity</skos:prefLabel>
    <skos:inScheme rdf:resource="http://vocabulary.odm2.org/unitstype"/>
    <odm2:dimensionCurrent>-1</odm2:dimensionCurrent>
    <odm2:dimensionTime>-1</odm2:dimensionTime>
  </rdf:Description>
  <rdf:Description rdf:about="http://vocabulary.odm2.org/unitstype/radioactivity">
    <skos:exactMatch>http://qudt.org/vocab/quantity#Activity</skos:exactMatch>
    <odm2:dimensionLength>0</odm2:dimensionLength>
    <odm2:dimensionAmount>0</odm2:dimensionAmount>
    <skos:historyNote>QUDT</skos:historyNote>
    <rdf:type rdf:resource="http://www.w3.org/2004/02/skos/core#Concept"/>
    <skos:inScheme rdf:resource="http://vocabulary.odm2.org/unitstype"/>
    <skos:definition>Activity is the term used to characterise the number of nuclei which disintegrate in a radioactive substance per unit time. Activity is usually measured in Becquerels (Bq), where 1 Bq is 1 disintegration per second.</skos:definition>
    <odm2:dimensionTime>0</odm2:dimensionTime>
    <odm2:dimensionSymbol>T-1</odm2:dimensionSymbol>
    <odm2:dimensionTemperature>0</odm2:dimensionTemperature>
    <odm2:dimensionMass>0</odm2:dimensionMass>
    <odm2:category>Quantum Mechanics</odm2:category>
    <skos:prefLabel>Radioactivity</skos:prefLabel>
    <odm2:dimensionLight>0</odm2:dimensionLight>
    <odm2:defaultUnit>Becquerel (Bq)</odm2:defaultUnit>
    <odm2:dimensionCurrent>-1</odm2:dimensionCurrent>
  </rdf:Description>
  <rdf:Description rdf:about="http://vocabulary.odm2.org/unitstype/color">
    <odm2:dimensionTemperature>0</odm2:dimensionTemperature>
    <odm2:dimensionTime>0</odm2:dimensionTime>
    <odm2:dimensionMass>0</odm2:dimensionMass>
    <skos:historyNote>CUAHSI</skos:historyNote>
    <odm2:dimensionCurrent>0</odm2:dimensionCurrent>
    <skos:prefLabel>Color</skos:prefLabel>
    <skos:inScheme rdf:resource="http://vocabulary.odm2.org/unitstype"/>
    <odm2:dimensionLength>1</odm2:dimensionLength>
    <odm2:dimensionAmount>0</odm2:dimensionAmount>
    <odm2:dimensionLight>0</odm2:dimensionLight>
    <odm2:defaultUnit>Hazen units (HU)</odm2:defaultUnit>
    <rdf:type rdf:resource="http://www.w3.org/2004/02/skos/core#Concept"/>
    <odm2:dimensionSymbol>U1</odm2:dimensionSymbol>
    <skos:note>Do not use conversions within this unit group!</skos:note>
    <skos:definition>Units used to describe hue and coloration.</skos:definition>
    <odm2:category>Dimensionless</odm2:category>
  </rdf:Description>
  <rdf:Description rdf:about="http://vocabulary.odm2.org/unitstype/diffusivity">
    <odm2:dimensionSymbol>L2T-1</odm2:dimensionSymbol>
    <odm2:dimensionCurrent>-1</odm2:dimensionCurrent>
    <skos:prefLabel>Diffusivity</skos:prefLabel>
    <odm2:dimensionAmount>0</odm2:dimensionAmount>
    <rdf:type rdf:resource="http://www.w3.org/2004/02/skos/core#Concept"/>
    <skos:inScheme rdf:resource="http://vocabulary.odm2.org/unitstype"/>
    <odm2:defaultUnit>Square meter per second (m^2/sec)</odm2:defaultUnit>
    <odm2:dimensionMass>2</odm2:dimensionMass>
    <odm2:category>Fluid Mechanics</odm2:category>
    <odm2:dimensionTime>0</odm2:dimensionTime>
    <odm2:dimensionTemperature>0</odm2:dimensionTemperature>
    <skos:note>Encompases both kinematic viscosity and thermal diffusivity</skos:note>
    <odm2:dimensionLight>0</odm2:dimensionLight>
    <skos:definition>Used for kinematic viscosity (also known as momentum diffusivity) and thermal diffusivity.  The Kinematic Viscosity of a fluid is the dynamic viscosity divided by the fluid density.  In heat transfer analysis, thermal diffusivity (usually denoted ? but a, ?, and D are also used) is the thermal conductivity divided by density and specific heat capacity at constant pressure. It measures the ability of a material to conduct thermal energy relative to its ability to store thermal energy.</skos:definition>
    <skos:historyNote>new for ODM2</skos:historyNote>
    <odm2:dimensionLength>0</odm2:dimensionLength>
  </rdf:Description>
  <rdf:Description rdf:about="http://vocabulary.odm2.org/unitstype/heatTransferCoefficient">
    <skos:inScheme rdf:resource="http://vocabulary.odm2.org/unitstype"/>
    <odm2:category>Thermodynamics</odm2:category>
    <odm2:dimensionTemperature>0</odm2:dimensionTemperature>
    <odm2:dimensionSymbol>M1T-3?-1</odm2:dimensionSymbol>
    <odm2:dimensionMass>0</odm2:dimensionMass>
    <odm2:dimensionTime>1</odm2:dimensionTime>
    <skos:exactMatch>http://qudt.org/vocab/quantity#CoefficientOfHeatTransfer</skos:exactMatch>
    <skos:definition>The heat transfer coefficient or film coefficient, in thermodynamics and in mechanics is the proportionality coefficient between the heat flux and the thermodynamic driving force for the flow of heat (i.e., the temperature difference, ?T)</skos:definition>
    <odm2:defaultUnit>Watt per square meter kelvin (W/(m^2-K))</odm2:defaultUnit>
    <odm2:dimensionLength>0</odm2:dimensionLength>
    <odm2:dimensionCurrent>-3</odm2:dimensionCurrent>
    <skos:historyNote>QUDT</skos:historyNote>
    <odm2:dimensionLight>0</odm2:dimensionLight>
    <odm2:dimensionAmount>-1</odm2:dimensionAmount>
    <rdf:type rdf:resource="http://www.w3.org/2004/02/skos/core#Concept"/>
    <skos:prefLabel>Heat transfer Coefficient</skos:prefLabel>
  </rdf:Description>
  <rdf:Description rdf:about="http://vocabulary.odm2.org/unitstype/electricalConductivity">
    <odm2:dimensionAmount>0</odm2:dimensionAmount>
    <odm2:dimensionMass>-3</odm2:dimensionMass>
    <odm2:dimensionCurrent>3</odm2:dimensionCurrent>
    <skos:historyNote>Wikipedia</skos:historyNote>
    <skos:inScheme rdf:resource="http://vocabulary.odm2.org/unitstype"/>
    <odm2:dimensionTemperature>2</odm2:dimensionTemperature>
    <odm2:dimensionLight>0</odm2:dimensionLight>
    <odm2:defaultUnit>microsiemens per centimeter (µS/cm)</odm2:defaultUnit>
    <skos:exactMatch>http://dbpedia.org/page/Electrical_resistivity_and_conductivity</skos:exactMatch>
    <odm2:dimensionLength>0</odm2:dimensionLength>
    <odm2:dimensionSymbol>L-3M-1T3I2</odm2:dimensionSymbol>
    <rdf:type rdf:resource="http://www.w3.org/2004/02/skos/core#Concept"/>
    <odm2:category>Electricity and Magnetism</odm2:category>
    <skos:prefLabel>Electrical conductivity</skos:prefLabel>
    <skos:definition>Electrical conductivity or specific conductance is the reciprocal of electrical resistivity, and measures a material's ability to conduct an electric current. It is commonly represented by the Greek letter ? (sigma), but ? (kappa) (especially in electrical engineering) or ? (gamma) are also occasionally used. Its SI unit is siemens per metre (S/m) and CGSE unit is reciprocal second (s?1).  [Wikipedia: https://en.wikipedia.org/wiki/Electrical_resistivity_and_conductivity]</skos:definition>
    <odm2:dimensionTime>-1</odm2:dimensionTime>
  </rdf:Description>
  <rdf:Description rdf:about="http://vocabulary.odm2.org/unitstype/luminousEnergy">
    <skos:historyNote>QUDT</skos:historyNote>
    <odm2:dimensionCurrent>1</odm2:dimensionCurrent>
    <skos:prefLabel>Luminous Energy</skos:prefLabel>
    <skos:inScheme rdf:resource="http://vocabulary.odm2.org/unitstype"/>
    <odm2:dimensionTemperature>0</odm2:dimensionTemperature>
    <skos:exactMatch>http://qudt.org/schema/qudt#LuminousEnergyUnit</skos:exactMatch>
    <odm2:dimensionAmount>0</odm2:dimensionAmount>
    <skos:definition>In photometry, luminous energy is the perceived energy of light. This is sometimes called the quantity of light. Luminous energy is not the same as radiant energy, the corresponding objective physical quantity. This is because the human eye can only see light in the visible spectrum and has different sensitivities to light of different wavelengths within the spectrum. When adapted for bright conditions (photopic vision), the eye is most sensitive to light at a wavelength of 555 nm. Light with a given amount of radiant energy will have more luminous energy if the wavelength is 555 nm than if the wavelength is longer or shorter. Light whose wavelength is well outside the visible spectrum has a luminous energy of zero, regardless of the amount of radiant energy present.</skos:definition>
    <odm2:dimensionMass>0</odm2:dimensionMass>
    <odm2:dimensionLength>1</odm2:dimensionLength>
    <odm2:defaultUnit>Lumen Second (lm s)</odm2:defaultUnit>
    <rdf:type rdf:resource="http://www.w3.org/2004/02/skos/core#Concept"/>
    <odm2:dimensionTime>0</odm2:dimensionTime>
    <odm2:dimensionSymbol>U1T1J1</odm2:dimensionSymbol>
    <odm2:dimensionLight>0</odm2:dimensionLight>
    <odm2:category>Photometry</odm2:category>
  </rdf:Description>
  <rdf:Description rdf:about="http://vocabulary.odm2.org/unitstype/massCountTemperature">
    <odm2:dimensionSymbol>M1?1N1</odm2:dimensionSymbol>
    <odm2:dimensionCurrent>0</odm2:dimensionCurrent>
    <odm2:category>Chemistry</odm2:category>
    <rdf:type rdf:resource="http://www.w3.org/2004/02/skos/core#Concept"/>
    <skos:prefLabel>Mass count temperature</skos:prefLabel>
    <odm2:dimensionMass>0</odm2:dimensionMass>
    <odm2:dimensionTemperature>0</odm2:dimensionTemperature>
    <odm2:dimensionTime>1</odm2:dimensionTime>
    <odm2:defaultUnit>Kilogram mole Kelvin (kg*mol*K)</odm2:defaultUnit>
    <odm2:dimensionLength>0</odm2:dimensionLength>
    <skos:historyNote>QUDT</skos:historyNote>
    <odm2:dimensionLight>1</odm2:dimensionLight>
    <skos:inScheme rdf:resource="http://vocabulary.odm2.org/unitstype"/>
    <skos:exactMatch>http://qudt.org/vocab/quantity#MassAmountOfSubstanceTemperature</skos:exactMatch>
    <odm2:dimensionAmount>1</odm2:dimensionAmount>
  </rdf:Description>
  <rdf:Description rdf:about="http://vocabulary.odm2.org/unitstype/massTemperature">
    <odm2:dimensionSymbol>M1?1</odm2:dimensionSymbol>
    <odm2:dimensionLength>0</odm2:dimensionLength>
    <skos:inScheme rdf:resource="http://vocabulary.odm2.org/unitstype"/>
    <odm2:defaultUnit>Kilogram kelvin (kg-K)</odm2:defaultUnit>
    <rdf:type rdf:resource="http://www.w3.org/2004/02/skos/core#Concept"/>
    <odm2:dimensionAmount>1</odm2:dimensionAmount>
    <skos:prefLabel>Mass temperature</skos:prefLabel>
    <odm2:dimensionCurrent>0</odm2:dimensionCurrent>
    <odm2:dimensionTime>1</odm2:dimensionTime>
    <skos:historyNote>QUDT</skos:historyNote>
    <odm2:dimensionTemperature>0</odm2:dimensionTemperature>
    <skos:exactMatch>http://qudt.org/vocab/quantity#Masstemperature</skos:exactMatch>
    <odm2:category>Thermodynamics</odm2:category>
    <odm2:dimensionMass>0</odm2:dimensionMass>
    <odm2:dimensionLight>0</odm2:dimensionLight>
  </rdf:Description>
  <rdf:Description rdf:about="http://vocabulary.odm2.org/unitstype/inductance">
    <odm2:category>Electricity and Magnetism</odm2:category>
    <odm2:dimensionSymbol>L2M1T-2I-2</odm2:dimensionSymbol>
    <odm2:dimensionAmount>0</odm2:dimensionAmount>
    <skos:historyNote>QUDT</skos:historyNote>
    <odm2:dimensionLength>0</odm2:dimensionLength>
    <rdf:type rdf:resource="http://www.w3.org/2004/02/skos/core#Concept"/>
    <skos:definition>Inductance is an electromagentic quantity that characterizes a circuit's resistance to any change of electric current; a change in the electric current through induces an opposing electromotive force (EMF). Quantitatively, inductance is proportional to the magnetic flux per unit of electric current.</skos:definition>
    <skos:prefLabel>Inductance</skos:prefLabel>
    <odm2:dimensionCurrent>-2</odm2:dimensionCurrent>
    <skos:exactMatch>http://qudt.org/vocab/quantity#Inductance</skos:exactMatch>
    <odm2:dimensionLight>0</odm2:dimensionLight>
    <odm2:dimensionTemperature>-2</odm2:dimensionTemperature>
    <skos:inScheme rdf:resource="http://vocabulary.odm2.org/unitstype"/>
    <odm2:dimensionTime>1</odm2:dimensionTime>
    <odm2:dimensionMass>2</odm2:dimensionMass>
    <odm2:defaultUnit>Henry (H)</odm2:defaultUnit>
  </rdf:Description>
  <rdf:Description rdf:about="http://vocabulary.odm2.org/unitstype/inversePermittivity">
    <rdf:type rdf:resource="http://www.w3.org/2004/02/skos/core#Concept"/>
    <odm2:dimensionSymbol>L3M1T-4I-2</odm2:dimensionSymbol>
    <skos:prefLabel>Inverse permittivity</skos:prefLabel>
    <odm2:defaultUnit>Meter per farad (m/F)</odm2:defaultUnit>
    <skos:exactMatch>http://qudt.org/vocab/quantity#Inversepermittivity</skos:exactMatch>
    <odm2:dimensionCurrent>-4</odm2:dimensionCurrent>
    <odm2:dimensionLength>0</odm2:dimensionLength>
    <skos:inScheme rdf:resource="http://vocabulary.odm2.org/unitstype"/>
    <odm2:category>Electricity and Magnetism</odm2:category>
    <odm2:dimensionAmount>0</odm2:dimensionAmount>
    <odm2:dimensionMass>3</odm2:dimensionMass>
    <odm2:dimensionTemperature>-2</odm2:dimensionTemperature>
    <odm2:dimensionLight>0</odm2:dimensionLight>
    <odm2:dimensionTime>1</odm2:dimensionTime>
    <skos:historyNote>QUDT</skos:historyNote>
  </rdf:Description>
  <rdf:Description rdf:about="http://vocabulary.odm2.org/unitstype/powerPerArea">
    <rdf:type rdf:resource="http://www.w3.org/2004/02/skos/core#Concept"/>
    <skos:prefLabel>Power per area</skos:prefLabel>
    <odm2:dimensionSymbol>M1T-3</odm2:dimensionSymbol>
    <odm2:dimensionMass>0</odm2:dimensionMass>
    <odm2:dimensionCurrent>-3</odm2:dimensionCurrent>
    <skos:definition>A general term for heat flow rate per unit area, power per unit area, irradiance, radient emmitance, and radiosity.  All these terms are sometimes referred to as "intensity."</skos:definition>
    <odm2:dimensionAmount>0</odm2:dimensionAmount>
    <odm2:defaultUnit>Watt per square meter (W/m^2)</odm2:defaultUnit>
    <odm2:dimensionTemperature>0</odm2:dimensionTemperature>
    <odm2:dimensionLength>0</odm2:dimensionLength>
    <skos:inScheme rdf:resource="http://vocabulary.odm2.org/unitstype"/>
    <odm2:category>Mechanics</odm2:category>
    <odm2:dimensionLight>0</odm2:dimensionLight>
    <odm2:dimensionTime>1</odm2:dimensionTime>
    <skos:exactMatch>http://qudt.org/vocab/quantity#Powerperarea</skos:exactMatch>
    <skos:historyNote>QUDT</skos:historyNote>
  </rdf:Description>
  <rdf:Description rdf:about="http://vocabulary.odm2.org/unitstype/electricalChargeLineDensity">
    <odm2:dimensionAmount>0</odm2:dimensionAmount>
    <odm2:dimensionLength>0</odm2:dimensionLength>
    <odm2:dimensionTemperature>1</odm2:dimensionTemperature>
    <rdf:type rdf:resource="http://www.w3.org/2004/02/skos/core#Concept"/>
    <skos:prefLabel>Electrical charge line density</skos:prefLabel>
    <odm2:defaultUnit>Coulomb per meter (C/m)</odm2:defaultUnit>
    <odm2:dimensionCurrent>1</odm2:dimensionCurrent>
    <odm2:dimensionLight>0</odm2:dimensionLight>
    <skos:exactMatch>http://qudt.org/vocab/quantity#Electricalchargelinedensity</skos:exactMatch>
    <odm2:category>Electricity and Magnetism</odm2:category>
    <odm2:dimensionTime>0</odm2:dimensionTime>
    <odm2:dimensionSymbol>L-1T1I1</odm2:dimensionSymbol>
    <skos:definition>The linear charge density is the amount of electric charge in a line. It is measured in coulombs per metre (C/m). Since there are positive as well as negative charges, the charge density can take on negative values. [Wikipedia]</skos:definition>
    <skos:inScheme rdf:resource="http://vocabulary.odm2.org/unitstype"/>
    <skos:historyNote>QUDT</skos:historyNote>
    <odm2:dimensionMass>-1</odm2:dimensionMass>
  </rdf:Description>
  <rdf:Description rdf:about="http://vocabulary.odm2.org/unitstype/Hyperpolarizability">
    <skos:inScheme rdf:resource="http://vocabulary.odm2.org/unitstype"/>
    <skos:exactMatch>http://qudt.org/vocab/quantity#CubicElectricDipoleMomentPerSquareEnergy</skos:exactMatch>
    <odm2:category>Electricity and Magnetism</odm2:category>
    <odm2:dimensionAmount>0</odm2:dimensionAmount>
    <skos:prefLabel>Hyperpolarizability</skos:prefLabel>
    <skos:historyNote>QUDT</skos:historyNote>
    <odm2:dimensionCurrent>7</odm2:dimensionCurrent>
    <odm2:dimensionMass>-1</odm2:dimensionMass>
    <skos:definition>The hyperpolarizability, a nonlinear-optical property of a molecule, is the second-order electric susceptibility per unit volume. [Wikipedia: https://en.wikipedia.org/wiki/Hyperpolarizability]</skos:definition>
    <odm2:dimensionTime>-2</odm2:dimensionTime>
    <odm2:defaultUnit>Cubic Coulomb Cubic Meter Per Square Joule (C3-m3/J2)</odm2:defaultUnit>
    <odm2:dimensionLength>0</odm2:dimensionLength>
    <odm2:dimensionLight>0</odm2:dimensionLight>
    <skos:note>http://dbpedia.org/page/Hyperpolarizability</skos:note>
    <odm2:dimensionTemperature>3</odm2:dimensionTemperature>
    <rdf:type rdf:resource="http://www.w3.org/2004/02/skos/core#Concept"/>
    <odm2:dimensionSymbol>L-1M-2T7I3</odm2:dimensionSymbol>
  </rdf:Description>
  <rdf:Description rdf:about="http://vocabulary.odm2.org/unitstype/fluidResistance">
    <skos:historyNote>UCUM</skos:historyNote>
    <odm2:dimensionSymbol>L-4M1T-1</odm2:dimensionSymbol>
    <odm2:category>Fluid Mechanics</odm2:category>
    <odm2:defaultUnit>Pascal seconds per cubic metre (Pa·s/m³)</odm2:defaultUnit>
    <odm2:dimensionAmount>0</odm2:dimensionAmount>
    <odm2:dimensionLength>0</odm2:dimensionLength>
    <odm2:dimensionLight>0</odm2:dimensionLight>
    <rdf:type rdf:resource="http://www.w3.org/2004/02/skos/core#Concept"/>
    <odm2:dimensionTemperature>0</odm2:dimensionTemperature>
    <skos:exactMatch>http://unitsofmeasure.org/ucum.html#para-44</skos:exactMatch>
    <skos:definition>In fluid dynamics, drag (sometimes called air resistance, a type of friction, or fluid resistance, another type of friction or fluid friction) refers to forces acting opposite to the relative motion of any object moving with respect to a surrounding fluid. [Wikipedia: https://en.wikipedia.org/wiki/Drag_%28physics%29]</skos:definition>
    <skos:inScheme rdf:resource="http://vocabulary.odm2.org/unitstype"/>
    <odm2:dimensionTime>1</odm2:dimensionTime>
    <odm2:dimensionMass>-4</odm2:dimensionMass>
    <odm2:dimensionCurrent>-1</odm2:dimensionCurrent>
    <skos:prefLabel>Fluid resistance</skos:prefLabel>
  </rdf:Description>
  <rdf:Description rdf:about="http://vocabulary.odm2.org/unitstype/thermalResistivity">
    <odm2:dimensionSymbol>L-1M-1T3?1</odm2:dimensionSymbol>
    <odm2:dimensionAmount>1</odm2:dimensionAmount>
    <odm2:dimensionLight>0</odm2:dimensionLight>
    <rdf:type rdf:resource="http://www.w3.org/2004/02/skos/core#Concept"/>
    <odm2:category>Thermodynamics</odm2:category>
    <odm2:dimensionMass>-1</odm2:dimensionMass>
    <skos:definition>The reciprocal of thermal conductivity is thermal resistivity, measured in kelvin-metres per watt (K*m/W). Also called Specific Thermal Resistance.</skos:definition>
    <skos:inScheme rdf:resource="http://vocabulary.odm2.org/unitstype"/>
    <odm2:dimensionTemperature>0</odm2:dimensionTemperature>
    <odm2:dimensionLength>0</odm2:dimensionLength>
    <odm2:dimensionCurrent>3</odm2:dimensionCurrent>
    <skos:exactMatch>http://qudt.org/vocab/quantity#Thermalresistivity</skos:exactMatch>
    <skos:prefLabel>Thermal resistivity</skos:prefLabel>
    <odm2:defaultUnit>Meter Kelvin per watt (K-m/W)</odm2:defaultUnit>
    <odm2:dimensionTime>-1</odm2:dimensionTime>
    <skos:historyNote>QUDT</skos:historyNote>
  </rdf:Description>
  <rdf:Description rdf:about="http://vocabulary.odm2.org/unitstype/fluidity">
    <odm2:dimensionCurrent>1</odm2:dimensionCurrent>
    <skos:exactMatch>ftp://ftp.unidata.ucar.edu/pub/udunits/</skos:exactMatch>
    <odm2:dimensionLength>0</odm2:dimensionLength>
    <skos:prefLabel>Fluidity</skos:prefLabel>
    <skos:definition>The reciprocal of viscosity is fluidity, usually symbolized by ? = 1 / ? or F = 1 / ?, depending on the convention used, measured in reciprocal poise (cm·s·g?1), sometimes called the rhe. Fluidity is seldom used in engineering practice. [Wikipedia: https://en.wikipedia.org/wiki/Viscosity]</skos:definition>
    <odm2:defaultUnit>Per Pascal Second (1/Pa·s)</odm2:defaultUnit>
    <rdf:type rdf:resource="http://www.w3.org/2004/02/skos/core#Concept"/>
    <odm2:dimensionAmount>0</odm2:dimensionAmount>
    <odm2:dimensionSymbol>L1M-1T1</odm2:dimensionSymbol>
    <odm2:dimensionTemperature>0</odm2:dimensionTemperature>
    <odm2:category>Fluid Mechanics</odm2:category>
    <skos:historyNote>UDUnits</skos:historyNote>
    <odm2:dimensionTime>-1</odm2:dimensionTime>
    <odm2:dimensionMass>1</odm2:dimensionMass>
    <odm2:dimensionLight>0</odm2:dimensionLight>
    <skos:inScheme rdf:resource="http://vocabulary.odm2.org/unitstype"/>
  </rdf:Description>
  <rdf:Description rdf:about="http://vocabulary.odm2.org/unitstype/linearMomentum">
    <odm2:dimensionTemperature>0</odm2:dimensionTemperature>
    <skos:prefLabel>Linear momentum</skos:prefLabel>
    <skos:exactMatch>http://qudt.org/vocab/quantity#Linearmomentum</skos:exactMatch>
    <odm2:dimensionTime>1</odm2:dimensionTime>
    <skos:definition>In classical mechanics, linear momentum or translational momentum (pl. momenta; SI unit kg m/s, or equivalently, N s) is the product of the mass and velocity of an object.</skos:definition>
    <odm2:dimensionLight>0</odm2:dimensionLight>
    <odm2:defaultUnit>Kilogram Meter Per Second (kg-m/s)</odm2:defaultUnit>
    <odm2:dimensionLength>0</odm2:dimensionLength>
    <odm2:dimensionCurrent>-1</odm2:dimensionCurrent>
    <odm2:dimensionSymbol>L1M1T-1</odm2:dimensionSymbol>
    <odm2:dimensionMass>1</odm2:dimensionMass>
    <odm2:dimensionAmount>0</odm2:dimensionAmount>
    <odm2:category>Mechanics</odm2:category>
    <skos:historyNote>QUDT</skos:historyNote>
    <rdf:type rdf:resource="http://www.w3.org/2004/02/skos/core#Concept"/>
    <skos:inScheme rdf:resource="http://vocabulary.odm2.org/unitstype"/>
  </rdf:Description>
  <rdf:Description rdf:about="http://vocabulary.odm2.org/unitstype/mass">
    <odm2:category>Base Quantity</odm2:category>
    <odm2:dimensionTemperature>0</odm2:dimensionTemperature>
    <odm2:dimensionCurrent>0</odm2:dimensionCurrent>
    <skos:prefLabel>Mass</skos:prefLabel>
    <odm2:dimensionLength>0</odm2:dimensionLength>
    <skos:inScheme rdf:resource="http://vocabulary.odm2.org/unitstype"/>
    <odm2:dimensionSymbol>M1</odm2:dimensionSymbol>
    <rdf:type rdf:resource="http://www.w3.org/2004/02/skos/core#Concept"/>
    <odm2:dimensionLight>0</odm2:dimensionLight>
    <odm2:defaultUnit>kilogram (kg)</odm2:defaultUnit>
    <skos:historyNote>QUDT</skos:historyNote>
    <odm2:dimensionTime>1</odm2:dimensionTime>
    <skos:exactMatch>http://qudt.org/vocab/quantity#Mass</skos:exactMatch>
    <skos:definition>In physics, mass is a property of a physical body which determines the strength of its mutual gravitational attraction to other bodies, its resistance to being accelerated by a force, and in the theory of relativity gives the mass–energy content of a system. The SI unit of mass is the kilogram (kg).</skos:definition>
    <odm2:dimensionMass>0</odm2:dimensionMass>
    <odm2:dimensionAmount>0</odm2:dimensionAmount>
  </rdf:Description>
  <rdf:Description rdf:about="http://vocabulary.odm2.org/unitstype/areaPerLength">
    <odm2:dimensionAmount>0</odm2:dimensionAmount>
    <skos:historyNote>Aquarius</skos:historyNote>
    <odm2:dimensionTime>0</odm2:dimensionTime>
    <odm2:category>Space and Time</odm2:category>
    <odm2:dimensionMass>1</odm2:dimensionMass>
    <odm2:defaultUnit>meters squared per meter (m^2/m)</odm2:defaultUnit>
    <odm2:dimensionLight>0</odm2:dimensionLight>
    <skos:inScheme rdf:resource="http://vocabulary.odm2.org/unitstype"/>
    <odm2:dimensionLength>0</odm2:dimensionLength>
    <skos:prefLabel>Area per length</skos:prefLabel>
    <odm2:dimensionTemperature>0</odm2:dimensionTemperature>
    <odm2:dimensionCurrent>0</odm2:dimensionCurrent>
    <skos:definition>A type of Linear Density.</skos:definition>
    <odm2:dimensionSymbol>L2L-1</odm2:dimensionSymbol>
    <rdf:type rdf:resource="http://www.w3.org/2004/02/skos/core#Concept"/>
    <skos:exactMatch>http://dbpedia.org/page/Linear_density</skos:exactMatch>
  </rdf:Description>
  <rdf:Description rdf:about="http://vocabulary.odm2.org/unitstype/fluorescence">
    <odm2:category>Dimensionless</odm2:category>
    <skos:prefLabel>Fluorescence</skos:prefLabel>
    <skos:historyNote>CUAHSI</skos:historyNote>
    <odm2:dimensionMass>0</odm2:dimensionMass>
    <odm2:dimensionTemperature>0</odm2:dimensionTemperature>
    <odm2:dimensionTime>0</odm2:dimensionTime>
    <odm2:dimensionLight>0</odm2:dimensionLight>
    <skos:inScheme rdf:resource="http://vocabulary.odm2.org/unitstype"/>
    <rdf:type rdf:resource="http://www.w3.org/2004/02/skos/core#Concept"/>
    <odm2:dimensionCurrent>0</odm2:dimensionCurrent>
    <skos:definition>Fluorescence is the emission of light by a substance that has absorbed light or other electromagnetic radiation.</skos:definition>
    <odm2:dimensionSymbol>U1</odm2:dimensionSymbol>
    <odm2:dimensionAmount>0</odm2:dimensionAmount>
    <odm2:defaultUnit>relative fluorescence units (RFU)</odm2:defaultUnit>
    <skos:note>https://en.wikipedia.org/wiki/Fluorescence</skos:note>
    <odm2:dimensionLength>1</odm2:dimensionLength>
  </rdf:Description>
  <rdf:Description rdf:about="http://vocabulary.odm2.org/unitstype/snap">
    <odm2:dimensionTime>0</odm2:dimensionTime>
    <odm2:dimensionLength>0</odm2:dimensionLength>
    <skos:inScheme rdf:resource="http://vocabulary.odm2.org/unitstype"/>
    <skos:prefLabel>Snap</skos:prefLabel>
    <odm2:dimensionMass>1</odm2:dimensionMass>
    <odm2:dimensionAmount>0</odm2:dimensionAmount>
    <odm2:category>Mechanics</odm2:category>
    <odm2:dimensionTemperature>0</odm2:dimensionTemperature>
    <odm2:defaultUnit>Meters per quartic second (m/s^4)</odm2:defaultUnit>
    <rdf:type rdf:resource="http://www.w3.org/2004/02/skos/core#Concept"/>
    <odm2:dimensionSymbol>L1T-4</odm2:dimensionSymbol>
    <skos:historyNote>Aquarius</skos:historyNote>
    <skos:definition>In physics, jounce or snap is the fourth derivative of the position vector with respect to time, with the first, second, and third derivatives being velocity, acceleration, and jerk, respectively; hence, the jounce is the rate of change of the jerk with respect to time. [Wikipedia: https://en.wikipedia.org/wiki/Jounce]</skos:definition>
    <odm2:dimensionLight>0</odm2:dimensionLight>
    <odm2:dimensionCurrent>-4</odm2:dimensionCurrent>
  </rdf:Description>
  <rdf:Description rdf:about="http://vocabulary.odm2.org/unitstype/massPerLength">
    <odm2:dimensionTemperature>0</odm2:dimensionTemperature>
    <rdf:type rdf:resource="http://www.w3.org/2004/02/skos/core#Concept"/>
    <odm2:dimensionSymbol>L-1M1</odm2:dimensionSymbol>
    <odm2:dimensionLight>0</odm2:dimensionLight>
    <odm2:dimensionMass>-1</odm2:dimensionMass>
    <skos:exactMatch>http://qudt.org/vocab/quantity#Massperlength</skos:exactMatch>
    <skos:historyNote>QUDT</skos:historyNote>
    <skos:prefLabel>Mass per length</skos:prefLabel>
    <odm2:category>Mechanics</odm2:category>
    <odm2:dimensionCurrent>0</odm2:dimensionCurrent>
    <odm2:dimensionLength>0</odm2:dimensionLength>
    <odm2:defaultUnit>Kilogram per meter (kg/m)</odm2:defaultUnit>
    <skos:inScheme rdf:resource="http://vocabulary.odm2.org/unitstype"/>
    <odm2:dimensionTime>1</odm2:dimensionTime>
    <odm2:dimensionAmount>0</odm2:dimensionAmount>
  </rdf:Description>
  <rdf:Description rdf:about="http://vocabulary.odm2.org/unitstype/powerPerElectricalCharge">
    <skos:historyNote>QUDT</skos:historyNote>
    <odm2:defaultUnit>Volt per Second</odm2:defaultUnit>
    <odm2:dimensionCurrent>-4</odm2:dimensionCurrent>
    <rdf:type rdf:resource="http://www.w3.org/2004/02/skos/core#Concept"/>
    <odm2:dimensionMass>2</odm2:dimensionMass>
    <skos:inScheme rdf:resource="http://vocabulary.odm2.org/unitstype"/>
    <skos:prefLabel>Power per electrical charge</skos:prefLabel>
    <odm2:dimensionLength>0</odm2:dimensionLength>
    <skos:exactMatch>http://qudt.org/vocab/quantity#PowerPerElectricCharge</skos:exactMatch>
    <odm2:dimensionAmount>0</odm2:dimensionAmount>
    <odm2:dimensionLight>0</odm2:dimensionLight>
    <odm2:category>Electricity and Magnetism</odm2:category>
    <odm2:dimensionTime>1</odm2:dimensionTime>
    <odm2:dimensionTemperature>-1</odm2:dimensionTemperature>
    <odm2:dimensionSymbol>L2M1T-4I-1</odm2:dimensionSymbol>
  </rdf:Description>
  <rdf:Description rdf:about="http://vocabulary.odm2.org/unitstype/gravitationalAttraction">
    <odm2:dimensionTemperature>0</odm2:dimensionTemperature>
    <odm2:dimensionLight>0</odm2:dimensionLight>
    <odm2:dimensionSymbol>L3M-1T-2</odm2:dimensionSymbol>
    <skos:inScheme rdf:resource="http://vocabulary.odm2.org/unitstype"/>
    <skos:historyNote>QUDT</skos:historyNote>
    <odm2:dimensionLength>0</odm2:dimensionLength>
    <odm2:dimensionCurrent>-2</odm2:dimensionCurrent>
    <skos:exactMatch>http://qudt.org/vocab/quantity#Gravitationalattraction</skos:exactMatch>
    <odm2:dimensionAmount>0</odm2:dimensionAmount>
    <rdf:type rdf:resource="http://www.w3.org/2004/02/skos/core#Concept"/>
    <skos:prefLabel>Gravitational attraction</skos:prefLabel>
    <odm2:defaultUnit>Cubic meter per kilogram second squared (m^3/(kg-s^2))</odm2:defaultUnit>
    <odm2:category>Mechanics</odm2:category>
    <odm2:dimensionTime>-1</odm2:dimensionTime>
    <odm2:dimensionMass>3</odm2:dimensionMass>
    <skos:definition>Gravity or gravitation is a natural phenomenon by which all things attract one another including stars, planets, galaxies and even light and sub-atomic particles. Gravity is responsible for the formation of the universe (e.g. creating spheres of hydrogen, igniting them under pressure to form stars and grouping them in to galaxies). Without gravity, the universe would be without thermal energy and composed only of equally spaced particles. On Earth, gravity gives weight to physical objects and causes the tides. Gravity has an infinite range, and it cannot be absorbed, transformed, or shielded against. [Wikipedia: https://en.wikipedia.org/wiki/Gravity]</skos:definition>
  </rdf:Description>
  <rdf:Description rdf:about="http://vocabulary.odm2.org/unitstype/electromotiveForce">
    <skos:exactMatch>http://qudt.org/vocab/quantity#Electromotiveforce</skos:exactMatch>
    <skos:definition>In physics, electromotive force, or most commonly emf (seldom capitalized), voltage, or (occasionally) electromotance is "that which tends to cause current (actual electrons and ions) to flow.". More formally, emf is the external work expended per unit of charge to produce an electric potential difference across two open-circuited terminals.[2][3] The electric potential difference is created by separating positive and negative charges, thereby generating an electric field.[4][5] The created electrical potential difference drives current flow if a circuit is attached to the source of emf. When current flows, however, the voltage across the terminals of the source of emf is no longer the open-circuit value, due to voltage drops inside the device due to its internal resistance. [Wikipedia: https://en.wikipedia.org/wiki/Electromotive_force]</skos:definition>
    <odm2:dimensionLight>0</odm2:dimensionLight>
    <skos:prefLabel>Electromotive force</skos:prefLabel>
    <odm2:category>Electricity and Magnetism</odm2:category>
    <skos:inScheme rdf:resource="http://vocabulary.odm2.org/unitstype"/>
    <odm2:defaultUnit>Volt (V) = Joule per coulomb</odm2:defaultUnit>
    <odm2:dimensionTime>1</odm2:dimensionTime>
    <odm2:dimensionAmount>0</odm2:dimensionAmount>
    <odm2:dimensionTemperature>-1</odm2:dimensionTemperature>
    <skos:historyNote>QUDT</skos:historyNote>
    <odm2:dimensionCurrent>-3</odm2:dimensionCurrent>
    <odm2:dimensionMass>2</odm2:dimensionMass>
    <odm2:dimensionLength>0</odm2:dimensionLength>
    <rdf:type rdf:resource="http://www.w3.org/2004/02/skos/core#Concept"/>
    <odm2:dimensionSymbol>L2M1T-3I-1</odm2:dimensionSymbol>
  </rdf:Description>
  <rdf:Description rdf:about="http://vocabulary.odm2.org/unitstype/arealFlux">
    <skos:prefLabel>Areal flux</skos:prefLabel>
    <odm2:dimensionAmount>1</odm2:dimensionAmount>
    <odm2:dimensionLength>-2</odm2:dimensionLength>
    <odm2:defaultUnit>Micromoles per square meter per second (umol/m^2 s)</odm2:defaultUnit>
    <odm2:category>Mechanics</odm2:category>
    <skos:inScheme rdf:resource="http://vocabulary.odm2.org/unitstype"/>
    <odm2:dimensionMass>0</odm2:dimensionMass>
    <skos:definition>Areal flux is the rate of flow of mass across a unit area per time</skos:definition>
    <rdf:type rdf:resource="http://www.w3.org/2004/02/skos/core#Concept"/>
    <odm2:dimensionTime>-1</odm2:dimensionTime>
  </rdf:Description>
  <rdf:Description rdf:about="http://vocabulary.odm2.org/unitstype/luminance">
    <odm2:dimensionTime>0</odm2:dimensionTime>
    <odm2:dimensionLength>0</odm2:dimensionLength>
    <skos:inScheme rdf:resource="http://vocabulary.odm2.org/unitstype"/>
    <odm2:dimensionAmount>0</odm2:dimensionAmount>
    <skos:definition>Luminance is a photometric measure of the luminous intensity per unit area of light travelling in a given direction. It describes the amount of light that passes through or is emitted from a particular area, and falls within a given solid angle.</skos:definition>
    <skos:historyNote>QUDT</skos:historyNote>
    <skos:exactMatch>http://qudt.org/vocab/quantity#Luminance</skos:exactMatch>
    <odm2:dimensionSymbol>L-2J1</odm2:dimensionSymbol>
    <odm2:dimensionMass>-2</odm2:dimensionMass>
    <odm2:dimensionTemperature>0</odm2:dimensionTemperature>
    <odm2:category>Photometry</odm2:category>
    <skos:prefLabel>Luminance</skos:prefLabel>
    <rdf:type rdf:resource="http://www.w3.org/2004/02/skos/core#Concept"/>
    <odm2:dimensionCurrent>0</odm2:dimensionCurrent>
    <odm2:dimensionLight>0</odm2:dimensionLight>
    <odm2:defaultUnit>Candela per square meter (cd/m^2)</odm2:defaultUnit>
  </rdf:Description>
  <rdf:Description rdf:about="http://vocabulary.odm2.org/unitstype/length">
    <skos:exactMatch>http://qudt.org/vocab/quantity#Length</skos:exactMatch>
    <odm2:dimensionLight>0</odm2:dimensionLight>
    <odm2:dimensionLength>0</odm2:dimensionLength>
    <odm2:defaultUnit>meter (m)</odm2:defaultUnit>
    <skos:historyNote>QUDT</skos:historyNote>
    <odm2:dimensionCurrent>0</odm2:dimensionCurrent>
    <rdf:type rdf:resource="http://www.w3.org/2004/02/skos/core#Concept"/>
    <skos:definition>In the International System of Quantities, length is any quantity with dimension distance.  [Wikipedia: https://en.wikipedia.org/wiki/Length]</skos:definition>
    <odm2:dimensionAmount>0</odm2:dimensionAmount>
    <odm2:dimensionMass>1</odm2:dimensionMass>
    <odm2:dimensionTime>0</odm2:dimensionTime>
    <odm2:dimensionTemperature>0</odm2:dimensionTemperature>
    <skos:inScheme rdf:resource="http://vocabulary.odm2.org/unitstype"/>
    <skos:prefLabel>Length</skos:prefLabel>
    <odm2:dimensionSymbol>L1</odm2:dimensionSymbol>
    <odm2:category>Base Quantity</odm2:category>
  </rdf:Description>
  <rdf:Description rdf:about="http://vocabulary.odm2.org/unitstype/stableIsotopeDelta">
    <odm2:dimensionLight>0</odm2:dimensionLight>
    <odm2:defaultUnit>Per Mille (‰; per mil) relative to a standard reference material</odm2:defaultUnit>
    <odm2:dimensionTemperature>0</odm2:dimensionTemperature>
    <odm2:dimensionMass>0</odm2:dimensionMass>
    <skos:prefLabel>Stable isotope delta</skos:prefLabel>
    <skos:definition>For stable isotopes, isotope ratios are typically reported using the delta (?) notation where ? represents the ratio of heavy isotope to light isotope in the sample over the same ratio of a standard reference material, reported using units of in "per mil" (‰, parts per thousand) and reported relative to the specific standard reference material.</skos:definition>
    <skos:historyNote>Wikipedia</skos:historyNote>
    <odm2:dimensionSymbol>U1</odm2:dimensionSymbol>
    <rdf:type rdf:resource="http://www.w3.org/2004/02/skos/core#Concept"/>
    <odm2:category>Chemistry</odm2:category>
    <odm2:dimensionAmount>0</odm2:dimensionAmount>
    <skos:inScheme rdf:resource="http://vocabulary.odm2.org/unitstype"/>
    <odm2:dimensionTime>0</odm2:dimensionTime>
    <odm2:dimensionLength>1</odm2:dimensionLength>
    <skos:exactMatch>https://en.wikipedia.org/wiki/Isotope_geochemistry#Stable_isotope_geochemistry</skos:exactMatch>
    <odm2:dimensionCurrent>0</odm2:dimensionCurrent>
  </rdf:Description>
  <rdf:Description rdf:about="http://vocabulary.odm2.org/unitstype/specificSurfaceArea">
    <odm2:dimensionCurrent>0</odm2:dimensionCurrent>
    <odm2:defaultUnit>Meters squared per kilogram (m²/kg)</odm2:defaultUnit>
    <odm2:dimensionMass>2</odm2:dimensionMass>
    <odm2:dimensionSymbol>L2M-1</odm2:dimensionSymbol>
    <odm2:dimensionAmount>0</odm2:dimensionAmount>
    <odm2:dimensionLength>0</odm2:dimensionLength>
    <odm2:dimensionLight>0</odm2:dimensionLight>
    <skos:exactMatch>http://dbpedia.org/page/Specific_surface_area</skos:exactMatch>
    <rdf:type rdf:resource="http://www.w3.org/2004/02/skos/core#Concept"/>
    <odm2:dimensionTemperature>0</odm2:dimensionTemperature>
    <skos:definition>Specific surface area "SSA" is a property of solids which is the total surface area of a material per unit of mass. It is a derived scientific value that can be used to determine the type and properties of a material (e.g. soil, snow). It is defined by surface area divided by mass (with units of m²/kg).</skos:definition>
    <odm2:dimensionTime>-1</odm2:dimensionTime>
    <odm2:category>Mechanics</odm2:category>
    <skos:historyNote>Wikipedia</skos:historyNote>
    <skos:inScheme rdf:resource="http://vocabulary.odm2.org/unitstype"/>
    <skos:prefLabel>Specific surface area</skos:prefLabel>
  </rdf:Description>
  <rdf:Description rdf:about="http://vocabulary.odm2.org/unitstype/electricalCurrent">
    <skos:inScheme rdf:resource="http://vocabulary.odm2.org/unitstype"/>
    <skos:historyNote>QUDT</skos:historyNote>
    <odm2:dimensionLength>0</odm2:dimensionLength>
    <skos:prefLabel>Electrical current</skos:prefLabel>
    <odm2:dimensionCurrent>0</odm2:dimensionCurrent>
    <odm2:dimensionSymbol>I1</odm2:dimensionSymbol>
    <rdf:type rdf:resource="http://www.w3.org/2004/02/skos/core#Concept"/>
    <odm2:dimensionMass>0</odm2:dimensionMass>
    <skos:exactMatch>http://qudt.org/vocab/quantity#ElectricCurrent</skos:exactMatch>
    <odm2:dimensionAmount>0</odm2:dimensionAmount>
    <odm2:category>Base Quantity</odm2:category>
    <odm2:dimensionTime>0</odm2:dimensionTime>
    <odm2:defaultUnit>ampere (A) = Coulombs per second</odm2:defaultUnit>
    <odm2:dimensionTemperature>1</odm2:dimensionTemperature>
    <skos:definition>An electric current is a flow of electric charge. In electric circuits this charge is often carried by moving electrons in a wire. It can also be carried by ions in an electrolyte, or by both ions and electrons such as in a plasma.  The SI unit for measuring an electric current is the ampere, which is the flow of electric charge across a surface at the rate of one coulomb per second. [Wikipedia: https://en.wikipedia.org/wiki/Electric_current]</skos:definition>
    <odm2:dimensionLight>0</odm2:dimensionLight>
  </rdf:Description>
  <rdf:Description rdf:about="http://vocabulary.odm2.org/unitstype/temperature">
    <odm2:dimensionLength>0</odm2:dimensionLength>
    <odm2:dimensionAmount>1</odm2:dimensionAmount>
    <odm2:dimensionMass>0</odm2:dimensionMass>
    <odm2:dimensionTemperature>0</odm2:dimensionTemperature>
    <skos:definition>A temperature is a numerical measure of hot and cold. Its measurement is by detection of heat radiation or particle velocity or kinetic energy, or by the bulk behavior of a thermometric material. It may be calibrated in any of various temperature scales, Celsius, Fahrenheit, Kelvin, etc. The fundamental physical definition of temperature is provided by thermodynamics.</skos:definition>
    <rdf:type rdf:resource="http://www.w3.org/2004/02/skos/core#Concept"/>
    <odm2:dimensionCurrent>0</odm2:dimensionCurrent>
    <skos:prefLabel>Temperature</skos:prefLabel>
    <odm2:dimensionTime>0</odm2:dimensionTime>
    <skos:inScheme rdf:resource="http://vocabulary.odm2.org/unitstype"/>
    <odm2:dimensionSymbol>?1</odm2:dimensionSymbol>
    <skos:historyNote>QUDT</skos:historyNote>
    <skos:exactMatch>http://qudt.org/vocab/quantity#ThermodynamicTemperature</skos:exactMatch>
    <odm2:category>Base Quantity</odm2:category>
    <odm2:dimensionLight>0</odm2:dimensionLight>
    <odm2:defaultUnit>Kelvin (K)</odm2:defaultUnit>
  </rdf:Description>
  <rdf:Description rdf:about="http://vocabulary.odm2.org/unitstype/electricalDipoleMoment">
    <rdf:type rdf:resource="http://www.w3.org/2004/02/skos/core#Concept"/>
    <odm2:dimensionCurrent>1</odm2:dimensionCurrent>
    <skos:prefLabel>Electrical dipole moment</skos:prefLabel>
    <odm2:dimensionLength>0</odm2:dimensionLength>
    <odm2:dimensionAmount>0</odm2:dimensionAmount>
    <skos:historyNote>QUDT</skos:historyNote>
    <skos:definition>In physics, the electric dipole moment is a measure of the separation of positive and negative electrical charges in a system of electric charges, that is, a measure of the charge system's overall polarity. The SI units are Coulomb-meter (C m). [Wikipedia: https://en.wikipedia.org/wiki/Electric_dipole_moment]</skos:definition>
    <odm2:defaultUnit>Coulomb meter (C-m)</odm2:defaultUnit>
    <odm2:category>Electricity and Magnetism</odm2:category>
    <odm2:dimensionLight>0</odm2:dimensionLight>
    <odm2:dimensionTime>0</odm2:dimensionTime>
    <odm2:dimensionTemperature>1</odm2:dimensionTemperature>
    <odm2:dimensionSymbol>L1T1I1</odm2:dimensionSymbol>
    <skos:exactMatch>http://qudt.org/vocab/quantity#ElectricDipoleMoment</skos:exactMatch>
    <skos:inScheme rdf:resource="http://vocabulary.odm2.org/unitstype"/>
    <odm2:dimensionMass>1</odm2:dimensionMass>
  </rdf:Description>
  <rdf:Description rdf:about="http://vocabulary.odm2.org/unitstype/polarizability">
    <odm2:dimensionTemperature>2</odm2:dimensionTemperature>
    <odm2:category>Electricity and Magnetism</odm2:category>
    <odm2:defaultUnit>Square Coulomb Meter per Joule</odm2:defaultUnit>
    <skos:exactMatch>http://qudt.org/vocab/quantity#Polarizability</skos:exactMatch>
    <odm2:dimensionAmount>0</odm2:dimensionAmount>
    <odm2:dimensionMass>0</odm2:dimensionMass>
    <skos:prefLabel>Polarizability</skos:prefLabel>
    <odm2:dimensionLight>0</odm2:dimensionLight>
    <odm2:dimensionLength>0</odm2:dimensionLength>
    <rdf:type rdf:resource="http://www.w3.org/2004/02/skos/core#Concept"/>
    <skos:inScheme rdf:resource="http://vocabulary.odm2.org/unitstype"/>
    <odm2:dimensionTime>-1</odm2:dimensionTime>
    <skos:historyNote>QUDT</skos:historyNote>
    <skos:definition>Polarizability is the relative tendency of a charge distribution, like the electron cloud of an atom or molecule, to be distorted from its normal shape by an external electric field, which may be caused by the presence of a nearby ion or dipole.  The electronic polarizability ? is defined as the ratio of the induced dipole moment of an atom to the electric field that produces this dipole moment. Polarizability is often a scalar valued quantity, however in the general case it is tensor-valued.</skos:definition>
    <skos:note>&lt;http://dbpedia.org/resource/Polarizability&gt;</skos:note>
    <odm2:dimensionCurrent>4</odm2:dimensionCurrent>
    <odm2:dimensionSymbol>M-1T4I2</odm2:dimensionSymbol>
  </rdf:Description>
  <rdf:Description rdf:about="http://vocabulary.odm2.org/unitstype/lengthTemperatureTime">
    <odm2:dimensionTemperature>0</odm2:dimensionTemperature>
    <odm2:dimensionCurrent>1</odm2:dimensionCurrent>
    <skos:prefLabel>Length temperature time</skos:prefLabel>
    <odm2:dimensionTime>0</odm2:dimensionTime>
    <skos:inScheme rdf:resource="http://vocabulary.odm2.org/unitstype"/>
    <skos:historyNote>QUDT</skos:historyNote>
    <odm2:dimensionLight>0</odm2:dimensionLight>
    <odm2:dimensionAmount>1</odm2:dimensionAmount>
    <rdf:type rdf:resource="http://www.w3.org/2004/02/skos/core#Concept"/>
    <odm2:category>Thermodynamics</odm2:category>
    <odm2:defaultUnit>Meter Second Kelvin</odm2:defaultUnit>
    <skos:exactMatch>http://qudt.org/vocab/quantity#Lengthtemperaturetime</skos:exactMatch>
    <odm2:dimensionMass>1</odm2:dimensionMass>
    <odm2:dimensionLength>0</odm2:dimensionLength>
    <odm2:dimensionSymbol>L1T1?1</odm2:dimensionSymbol>
  </rdf:Description>
  <rdf:Description rdf:about="http://vocabulary.odm2.org/unitstype/powerPerAreaQuarticTemperature">
    <skos:definition>The units of the Stefan-Boltzmann constant.  The Stefan–Boltzmann law states that the total energy radiated per unit surface area of a black body across all wavelengths per unit time (also known as the black-body radiant exitance or emissive power), j*, is directly proportional to the fourth power of the black body's thermodynamic temperature.  The constant of proportionality ?, called the Stefan–Boltzmann constant or Stefan's constant, derives from other known constants of nature. The value of the constant is5.670373 x 10^8 Wm^-2K^-4.  [Wikipedia: https://en.wikipedia.org/wiki/Stefan%E2%80%93Boltzmann_constant]</skos:definition>
    <odm2:dimensionAmount>-4</odm2:dimensionAmount>
    <odm2:dimensionTemperature>0</odm2:dimensionTemperature>
    <odm2:dimensionCurrent>-3</odm2:dimensionCurrent>
    <odm2:dimensionMass>0</odm2:dimensionMass>
    <odm2:dimensionTime>1</odm2:dimensionTime>
    <skos:exactMatch>http://qudt.org/vocab/quantity#PowerPerAreaQuarticTemperature</skos:exactMatch>
    <odm2:defaultUnit>Watt per Square Meter Quartic Kelvin</odm2:defaultUnit>
    <odm2:dimensionLength>0</odm2:dimensionLength>
    <skos:historyNote>QUDT</skos:historyNote>
    <odm2:dimensionSymbol>M1T-3?-4</odm2:dimensionSymbol>
    <odm2:dimensionLight>0</odm2:dimensionLight>
    <rdf:type rdf:resource="http://www.w3.org/2004/02/skos/core#Concept"/>
    <skos:inScheme rdf:resource="http://vocabulary.odm2.org/unitstype"/>
    <skos:prefLabel>Power per area quartic temperature</skos:prefLabel>
    <odm2:category>Thermodynamics</odm2:category>
  </rdf:Description>
  <rdf:Description rdf:about="http://vocabulary.odm2.org/unitstype/volume">
    <skos:historyNote>QUDT</skos:historyNote>
    <odm2:dimensionLength>0</odm2:dimensionLength>
    <odm2:defaultUnit>Cubic Meter (m^3)</odm2:defaultUnit>
    <odm2:dimensionLight>0</odm2:dimensionLight>
    <skos:exactMatch>http://qudt.org/vocab/quantity#LiquidVolume</skos:exactMatch>
    <skos:prefLabel>Volume</skos:prefLabel>
    <odm2:dimensionTemperature>0</odm2:dimensionTemperature>
    <odm2:category>Space and Time</odm2:category>
    <skos:inScheme rdf:resource="http://vocabulary.odm2.org/unitstype"/>
    <skos:note>This includes dry, liquid, and gas volumes.</skos:note>
    <odm2:dimensionTime>0</odm2:dimensionTime>
    <odm2:dimensionCurrent>0</odm2:dimensionCurrent>
    <odm2:dimensionMass>3</odm2:dimensionMass>
    <odm2:dimensionSymbol>L3</odm2:dimensionSymbol>
    <rdf:type rdf:resource="http://www.w3.org/2004/02/skos/core#Concept"/>
    <odm2:dimensionAmount>0</odm2:dimensionAmount>
  </rdf:Description>
  <rdf:Description rdf:about="http://vocabulary.odm2.org/unitstype/catalyticActivity">
    <skos:note>Uses units that are similar, if not identical, to particle loading.  Both have the same dimensionality.</skos:note>
    <odm2:category>Chemistry</odm2:category>
    <odm2:dimensionCurrent>-1</odm2:dimensionCurrent>
    <odm2:defaultUnit>Katal (kat)</odm2:defaultUnit>
    <odm2:dimensionLength>0</odm2:dimensionLength>
    <skos:inScheme rdf:resource="http://vocabulary.odm2.org/unitstype"/>
    <odm2:dimensionTemperature>0</odm2:dimensionTemperature>
    <skos:historyNote>QUDT</skos:historyNote>
    <skos:exactMatch>http://qudt.org/vocab/quantity#CatalyticActivity</skos:exactMatch>
    <rdf:type rdf:resource="http://www.w3.org/2004/02/skos/core#Concept"/>
    <skos:definition>Catalytic activity is usually denoted by the symbol z and measured in mol/s, a unit which was called katal and defined the SI unit for catalytic activity since 1999. Catalytic activity is not a kind of reaction rate, but a property of the catalyst under certain conditions, in relation to a specific chemical reaction. Catalytic activity of one katal (Symbol 1 kat = 1mol/s) of a catalyst means an amount of that catalyst (substance, in Mol) that leads to a net reaction of one Mol per second of the reactants to the resulting reagents or other outcome which was intended for this chemical reaction. A catalyst may and usually will have different catalytic activity for distinct reactions. [Wikipedia: https://en.wikipedia.org/wiki/Catalysis]</skos:definition>
    <odm2:dimensionTime>0</odm2:dimensionTime>
    <odm2:dimensionLight>1</odm2:dimensionLight>
    <odm2:dimensionAmount>0</odm2:dimensionAmount>
    <odm2:dimensionMass>0</odm2:dimensionMass>
    <skos:prefLabel>Catalytic activity</skos:prefLabel>
    <odm2:dimensionSymbol>T-1N1</odm2:dimensionSymbol>
  </rdf:Description>
  <rdf:Description rdf:about="http://vocabulary.odm2.org/unitstype/currency">
    <skos:inScheme rdf:resource="http://vocabulary.odm2.org/unitstype"/>
    <odm2:dimensionAmount>0</odm2:dimensionAmount>
    <odm2:dimensionLength>0</odm2:dimensionLength>
    <skos:historyNote>QUDT</skos:historyNote>
    <odm2:dimensionTemperature>0</odm2:dimensionTemperature>
    <rdf:type rdf:resource="http://www.w3.org/2004/02/skos/core#Concept"/>
    <odm2:category>Financial</odm2:category>
    <odm2:defaultUnit>United States Dollar</odm2:defaultUnit>
    <skos:exactMatch>http://qudt.org/vocab/quantity#Currency</skos:exactMatch>
    <odm2:dimensionLight>0</odm2:dimensionLight>
    <skos:definition>A currency (from Middle English: curraunt, "in circulation", from Latin: currens, -entis) in the most specific use of the word refers to money in any form when in actual use or circulation as a medium of exchange, especially circulating banknotes and coins.  A more general definition is that a currency is a system of money (monetary units) in common use, especially in a nation. [Wikipedia; https://en.wikipedia.org/wiki/Currency]</skos:definition>
    <skos:note>Conversions in this unit need access to the latest financial data.</skos:note>
    <skos:prefLabel>Currency</skos:prefLabel>
    <odm2:dimensionMass>0</odm2:dimensionMass>
    <odm2:dimensionTime>0</odm2:dimensionTime>
    <odm2:dimensionCurrent>0</odm2:dimensionCurrent>
  </rdf:Description>
  <rdf:Description rdf:about="http://vocabulary.odm2.org/unitstype/level">
    <skos:definition>"Psuedo Units" defined from a log ratio.  This includes any number of units like deciBels where the unit is derived as a log ratio of two other units.  The logarithm distinguishes these from other dimensionless ratios.</skos:definition>
    <odm2:dimensionTime>0</odm2:dimensionTime>
    <odm2:dimensionTemperature>0</odm2:dimensionTemperature>
    <odm2:defaultUnit>Decibel (Db)</odm2:defaultUnit>
    <odm2:dimensionAmount>0</odm2:dimensionAmount>
    <odm2:dimensionMass>0</odm2:dimensionMass>
    <skos:prefLabel>Level</skos:prefLabel>
    <skos:exactMatch>http://unitsofmeasure.org/ucum.html#para-46</skos:exactMatch>
    <skos:note>"Psuedo Units" defined from a log ratio</skos:note>
    <odm2:dimensionLength>0</odm2:dimensionLength>
    <odm2:dimensionLight>0</odm2:dimensionLight>
    <rdf:type rdf:resource="http://www.w3.org/2004/02/skos/core#Concept"/>
    <skos:historyNote>UCUM</skos:historyNote>
    <skos:inScheme rdf:resource="http://vocabulary.odm2.org/unitstype"/>
    <odm2:dimensionCurrent>0</odm2:dimensionCurrent>
    <odm2:category>Dimensionless Ratio</odm2:category>
  </rdf:Description>
  <rdf:Description rdf:about="http://vocabulary.odm2.org/unitstype/amountOfInformation">
    <skos:definition>In computing and telecommunications, a unit of information is the capacity of some standard data storage system or communication channel, used to measure the capacities of other systems and channels. In information theory, units of information are also used to measure the information contents or entropy of random variables.</skos:definition>
    <skos:historyNote>UCUM</skos:historyNote>
    <odm2:dimensionSymbol>U1</odm2:dimensionSymbol>
    <odm2:dimensionLength>1</odm2:dimensionLength>
    <odm2:dimensionTemperature>0</odm2:dimensionTemperature>
    <odm2:dimensionLight>0</odm2:dimensionLight>
    <odm2:category>Information</odm2:category>
    <skos:inScheme rdf:resource="http://vocabulary.odm2.org/unitstype"/>
    <odm2:defaultUnit>Bit</odm2:defaultUnit>
    <odm2:dimensionCurrent>0</odm2:dimensionCurrent>
    <rdf:type rdf:resource="http://www.w3.org/2004/02/skos/core#Concept"/>
    <odm2:dimensionMass>0</odm2:dimensionMass>
    <skos:prefLabel>Amount of Information</skos:prefLabel>
    <odm2:dimensionAmount>0</odm2:dimensionAmount>
    <odm2:dimensionTime>0</odm2:dimensionTime>
    <skos:exactMatch>http://unitsofmeasure.org/ucum.html#para-48</skos:exactMatch>
  </rdf:Description>
  <rdf:Description rdf:about="http://vocabulary.odm2.org/unitstype/powerAreaPerSolidAngle">
    <odm2:dimensionAmount>0</odm2:dimensionAmount>
    <skos:prefLabel>Power area per solid angle</skos:prefLabel>
    <odm2:dimensionCurrent>-3</odm2:dimensionCurrent>
    <odm2:dimensionTemperature>0</odm2:dimensionTemperature>
    <rdf:type rdf:resource="http://www.w3.org/2004/02/skos/core#Concept"/>
    <odm2:dimensionLight>0</odm2:dimensionLight>
    <odm2:dimensionSymbol>U-1L4M1T-3</odm2:dimensionSymbol>
    <odm2:dimensionMass>4</odm2:dimensionMass>
    <skos:inScheme rdf:resource="http://vocabulary.odm2.org/unitstype"/>
    <skos:historyNote>QUDT</skos:historyNote>
    <odm2:dimensionTime>1</odm2:dimensionTime>
    <odm2:defaultUnit>Watt Square Meter per Steradian</odm2:defaultUnit>
    <skos:exactMatch>http://qudt.org/vocab/quantity#PowerAreaPerSolidAngle</skos:exactMatch>
    <odm2:dimensionLength>1</odm2:dimensionLength>
    <odm2:category>Mechanics</odm2:category>
  </rdf:Description>
  <rdf:Description rdf:about="http://vocabulary.odm2.org/unitstype/electricalChargeVolumeDensity">
    <odm2:dimensionLight>0</odm2:dimensionLight>
    <odm2:dimensionMass>-3</odm2:dimensionMass>
    <skos:exactMatch>http://qudt.org/vocab/quantity#Electricalchargevolumedensity</skos:exactMatch>
    <skos:inScheme rdf:resource="http://vocabulary.odm2.org/unitstype"/>
    <skos:historyNote>QUDT</skos:historyNote>
    <odm2:dimensionLength>0</odm2:dimensionLength>
    <odm2:dimensionSymbol>L-3T1I1</odm2:dimensionSymbol>
    <skos:definition>In electromagnetism, charge density is a measure of electric charge per unit volume of space, in one, two or three dimensions. More specifically: the linear, surface, or volume charge density is the amount of electric charge per unit length, surface area, or volume, respectively. The respective SI units are C·m?1, C·m?2 or C·m?3.</skos:definition>
    <odm2:defaultUnit>Coulomb per cubic meter (C/m^3)</odm2:defaultUnit>
    <odm2:dimensionAmount>0</odm2:dimensionAmount>
    <rdf:type rdf:resource="http://www.w3.org/2004/02/skos/core#Concept"/>
    <odm2:category>Electricity and Magnetism</odm2:category>
    <odm2:dimensionTime>0</odm2:dimensionTime>
    <odm2:dimensionTemperature>1</odm2:dimensionTemperature>
    <skos:note>Also https://en.wikipedia.org/wiki/Charge_density</skos:note>
    <skos:prefLabel>Electrical charge volume density</skos:prefLabel>
    <odm2:dimensionCurrent>1</odm2:dimensionCurrent>
  </rdf:Description>
  <rdf:Description rdf:about="http://vocabulary.odm2.org/unitstype/areaAngle">
    <odm2:dimensionAmount>0</odm2:dimensionAmount>
    <skos:prefLabel>Area angle</skos:prefLabel>
    <skos:inScheme rdf:resource="http://vocabulary.odm2.org/unitstype"/>
    <skos:historyNote>QUDT</skos:historyNote>
    <odm2:dimensionTime>0</odm2:dimensionTime>
    <odm2:dimensionLength>1</odm2:dimensionLength>
    <odm2:dimensionMass>2</odm2:dimensionMass>
    <odm2:dimensionTemperature>0</odm2:dimensionTemperature>
    <odm2:category>Space and Time</odm2:category>
    <odm2:dimensionCurrent>0</odm2:dimensionCurrent>
    <odm2:defaultUnit>Square meter steradian (m^2-sr)</odm2:defaultUnit>
    <skos:exactMatch>http://qudt.org/vocab/quantity#AreaAngle</skos:exactMatch>
    <odm2:dimensionSymbol>U1L2</odm2:dimensionSymbol>
    <rdf:type rdf:resource="http://www.w3.org/2004/02/skos/core#Concept"/>
    <odm2:dimensionLight>0</odm2:dimensionLight>
  </rdf:Description>
  <rdf:Description rdf:about="http://vocabulary.odm2.org/unitstype/radiance">
    <odm2:dimensionSymbol>U-1M1T-3</odm2:dimensionSymbol>
    <odm2:dimensionMass>0</odm2:dimensionMass>
    <odm2:dimensionTemperature>0</odm2:dimensionTemperature>
    <skos:exactMatch>http://qudt.org/schema/qudt#RadianceUnit</skos:exactMatch>
    <odm2:dimensionLight>0</odm2:dimensionLight>
    <skos:inScheme rdf:resource="http://vocabulary.odm2.org/unitstype"/>
    <rdf:type rdf:resource="http://www.w3.org/2004/02/skos/core#Concept"/>
    <odm2:dimensionTime>1</odm2:dimensionTime>
    <skos:definition>In radiometry, radiance is the radiant flux emitted, reflected, transmitted or received by a surface, per unit solid angle per unit projected area. Radiance is used to characterize diffuse emission and reflection of electromagnetic radiation, or to quantify emission of neutrinos and other particles. This is a directional quantity. Historically, radiance is called "intensity" and spectral radiance is called "specific intensity". [Wikipedia: https://en.wikipedia.org/wiki/Radiance]</skos:definition>
    <odm2:dimensionLength>-1</odm2:dimensionLength>
    <odm2:defaultUnit>Watt per square meter steradian (W/(m^2-sr))</odm2:defaultUnit>
    <odm2:dimensionAmount>0</odm2:dimensionAmount>
    <skos:historyNote>QUDT</skos:historyNote>
    <odm2:category>Radiology</odm2:category>
    <odm2:dimensionCurrent>-3</odm2:dimensionCurrent>
    <skos:prefLabel>Radiance</skos:prefLabel>
  </rdf:Description>
  <rdf:Description rdf:about="http://vocabulary.odm2.org/unitstype/quarticElectricDipoleMomentPerCubicEnergy">
    <odm2:dimensionSymbol>L-2M-3T10I4</odm2:dimensionSymbol>
    <skos:prefLabel>Quartic electrical dipole moment per cubic energy</skos:prefLabel>
    <skos:exactMatch>http://qudt.org/vocab/quantity#QuarticElectricDipoleMomentPerCubicEnergy</skos:exactMatch>
    <odm2:dimensionTime>-3</odm2:dimensionTime>
    <skos:historyNote>QUDT</skos:historyNote>
    <odm2:category>Electricity and Magnetism</odm2:category>
    <rdf:type rdf:resource="http://www.w3.org/2004/02/skos/core#Concept"/>
    <odm2:dimensionMass>-2</odm2:dimensionMass>
    <odm2:dimensionLight>0</odm2:dimensionLight>
    <odm2:dimensionAmount>0</odm2:dimensionAmount>
    <odm2:dimensionTemperature>4</odm2:dimensionTemperature>
    <odm2:dimensionLength>0</odm2:dimensionLength>
    <skos:inScheme rdf:resource="http://vocabulary.odm2.org/unitstype"/>
    <odm2:defaultUnit>Quartic Coulomb Meter per Cubic Joule (C^4 m^4 J^-3)</odm2:defaultUnit>
    <odm2:dimensionCurrent>10</odm2:dimensionCurrent>
  </rdf:Description>
  <rdf:Description rdf:about="http://vocabulary.odm2.org/unitstype/angularMomentum">
    <odm2:dimensionAmount>0</odm2:dimensionAmount>
    <odm2:dimensionSymbol>L2M1T-1</odm2:dimensionSymbol>
    <odm2:dimensionLength>0</odm2:dimensionLength>
    <skos:inScheme rdf:resource="http://vocabulary.odm2.org/unitstype"/>
    <odm2:dimensionCurrent>-1</odm2:dimensionCurrent>
    <odm2:dimensionMass>2</odm2:dimensionMass>
    <odm2:defaultUnit>Joule Second (J s)</odm2:defaultUnit>
    <skos:exactMatch>http://qudt.org/vocab/quantity#AngularMomentum</skos:exactMatch>
    <odm2:category>Mechanics</odm2:category>
    <odm2:dimensionLight>0</odm2:dimensionLight>
    <skos:historyNote>QUDT</skos:historyNote>
    <skos:definition>Quantity of rotational motion. Linear momentum is the quantity obtained by multiplying the mass of a body by its linear velocity. Angular momentum is the quantity obtained by multiplying the moment of inertia of a body by its angular velocity. The momentum of a system of particles is given by the sum of the momenta of the individual particles which make up the system or by the product of the total mass of the system and the velocity of the center of gravity of the system. The momentum of a continuous medium is given by the integral of the velocity over the mass of the medium or by the product of the total mass of the medium and the velocity of the center of gravity of the medium. In physics, the angular momentum of an object rotating about some reference point is the measure of the extent to which the object will continue to rotate about that point unless acted upon by an external torque. In particular, if a point mass rotates about an axis, then the angular momentum with respect to a point on the axis is related to the mass of the object, the velocity and the distance of the mass to the axis. While the motion associated with linear momentum has no absolute frame of reference, the rotation associated with angular momentum is sometimes spoken of as being measured relative to the fixed stars.  The physical quantity "action" has the same units as angular momentum.</skos:definition>
    <rdf:type rdf:resource="http://www.w3.org/2004/02/skos/core#Concept"/>
    <skos:prefLabel>Angular momentum</skos:prefLabel>
    <odm2:dimensionTemperature>0</odm2:dimensionTemperature>
    <odm2:dimensionTime>1</odm2:dimensionTime>
  </rdf:Description>
  <rdf:Description rdf:about="http://vocabulary.odm2.org/unitstype/magneticFieldStrength">
    <odm2:dimensionLight>0</odm2:dimensionLight>
    <odm2:dimensionTime>0</odm2:dimensionTime>
    <odm2:dimensionTemperature>1</odm2:dimensionTemperature>
    <odm2:defaultUnit>Ampere Turn per Meter (At/m) or Ampere per meter (A/m)</odm2:defaultUnit>
    <skos:exactMatch>http://qudt.org/schema/qudt#MagneticFieldStrengthUnit</skos:exactMatch>
    <rdf:type rdf:resource="http://www.w3.org/2004/02/skos/core#Concept"/>
    <skos:historyNote>QUDT</skos:historyNote>
    <odm2:category>Electricity and Magnetism</odm2:category>
    <odm2:dimensionMass>-1</odm2:dimensionMass>
    <odm2:dimensionLength>0</odm2:dimensionLength>
    <odm2:dimensionAmount>0</odm2:dimensionAmount>
    <skos:definition>The magnetic field strength, H (also called magnetic field intensity, magnetizing field, or magnetic field), characterizes how the true Magnetic Field B influences the organization of magnetic dipoles in a given medium.</skos:definition>
    <skos:inScheme rdf:resource="http://vocabulary.odm2.org/unitstype"/>
    <skos:prefLabel>Magnetic field strength</skos:prefLabel>
    <odm2:dimensionSymbol>L-1I1</odm2:dimensionSymbol>
    <odm2:dimensionCurrent>0</odm2:dimensionCurrent>
  </rdf:Description>
  <rdf:Description rdf:about="http://vocabulary.odm2.org/unitstype/pressureOrStress">
    <rdf:type rdf:resource="http://www.w3.org/2004/02/skos/core#Concept"/>
    <odm2:dimensionLight>0</odm2:dimensionLight>
    <odm2:dimensionMass>-1</odm2:dimensionMass>
    <odm2:dimensionCurrent>-2</odm2:dimensionCurrent>
    <skos:exactMatch>http://qudt.org/vocab/quantity#Pressureorstress</skos:exactMatch>
    <skos:inScheme rdf:resource="http://vocabulary.odm2.org/unitstype"/>
    <odm2:dimensionSymbol>L-1M1T-2</odm2:dimensionSymbol>
    <skos:definition>Pressure is an effect which occurs when a force is applied on a surface. Pressure is the amount of force acting on a unit area. Pressure is distinct from stress, as the former is the ratio of the component of force normal to a surface to the surface area. Stress is a tensor that relates the vector force to the vector area.</skos:definition>
    <odm2:dimensionTime>1</odm2:dimensionTime>
    <odm2:defaultUnit>Pascal (Pa)</odm2:defaultUnit>
    <odm2:dimensionTemperature>0</odm2:dimensionTemperature>
    <skos:historyNote>QUDT</skos:historyNote>
    <skos:prefLabel>Pressure or stress</skos:prefLabel>
    <odm2:category>Space and Time</odm2:category>
    <odm2:dimensionLength>0</odm2:dimensionLength>
    <skos:note>Has identical dimensionality to energy density</skos:note>
    <odm2:dimensionAmount>0</odm2:dimensionAmount>
  </rdf:Description>
  <rdf:Description rdf:about="http://vocabulary.odm2.org/unitstype/inverseMagneticFlux">
    <odm2:dimensionMass>-2</odm2:dimensionMass>
    <skos:exactMatch>http://qudt.org/vocab/quantity#Inversemagneticflux</skos:exactMatch>
    <skos:inScheme rdf:resource="http://vocabulary.odm2.org/unitstype"/>
    <skos:historyNote>QUDT</skos:historyNote>
    <odm2:dimensionLength>0</odm2:dimensionLength>
    <skos:prefLabel>Inverse magnetic flux</skos:prefLabel>
    <odm2:dimensionCurrent>2</odm2:dimensionCurrent>
    <rdf:type rdf:resource="http://www.w3.org/2004/02/skos/core#Concept"/>
    <odm2:category>Electricity and Magnetism</odm2:category>
    <odm2:dimensionAmount>0</odm2:dimensionAmount>
    <skos:note>Has identical dimensionality to electric current per unit energy</skos:note>
    <odm2:dimensionSymbol>L-2M-1T2I1</odm2:dimensionSymbol>
    <odm2:dimensionTime>-1</odm2:dimensionTime>
    <odm2:dimensionTemperature>1</odm2:dimensionTemperature>
    <odm2:defaultUnit>Hertz per Volt (Hz/V)</odm2:defaultUnit>
    <odm2:dimensionLight>0</odm2:dimensionLight>
  </rdf:Description>
  <rdf:Description rdf:about="http://vocabulary.odm2.org/unitstype/electricalFlux">
    <odm2:dimensionTemperature>-1</odm2:dimensionTemperature>
    <skos:historyNote>QUDT</skos:historyNote>
    <odm2:dimensionCurrent>-3</odm2:dimensionCurrent>
    <skos:prefLabel>Electrical flux</skos:prefLabel>
    <odm2:dimensionLength>0</odm2:dimensionLength>
    <skos:exactMatch>http://qudt.org/vocab/quantity#ElectricFlux</skos:exactMatch>
    <rdf:type rdf:resource="http://www.w3.org/2004/02/skos/core#Concept"/>
    <odm2:dimensionSymbol>L3M1T-3I-1</odm2:dimensionSymbol>
    <odm2:defaultUnit>Volt Meter (Vm)</odm2:defaultUnit>
    <odm2:dimensionLight>0</odm2:dimensionLight>
    <odm2:category>Electricity and Magnetism</odm2:category>
    <skos:inScheme rdf:resource="http://vocabulary.odm2.org/unitstype"/>
    <skos:definition>The Electric Flux through an area is defined as the electric field multiplied by the area of the surface projected in a plane perpendicular to the field. Electric Flux is a scalar-valued quantity.</skos:definition>
    <odm2:dimensionMass>3</odm2:dimensionMass>
    <odm2:dimensionTime>1</odm2:dimensionTime>
    <odm2:dimensionAmount>0</odm2:dimensionAmount>
  </rdf:Description>
  <rdf:Description rdf:about="http://vocabulary.odm2.org/unitstype">
    <dc:creator>ODM2 Working Group</dc:creator>
    <dc:description>A vocabulary for describing the type of the Unit or the more general quantity that the Unit represents.</dc:description>
    <rdf:type rdf:resource="http://www.w3.org/2004/02/skos/core#ConceptScheme"/>
    <dc:title>ODM2 Units Type Controlled Vocabulary</dc:title>
  </rdf:Description>
  <rdf:Description rdf:about="http://vocabulary.odm2.org/unitstype/molarHeatCapacity">
    <skos:inScheme rdf:resource="http://vocabulary.odm2.org/unitstype"/>
    <odm2:dimensionTime>1</odm2:dimensionTime>
    <odm2:dimensionTemperature>0</odm2:dimensionTemperature>
    <odm2:dimensionSymbol>L2M1T-2?-1N-1</odm2:dimensionSymbol>
    <skos:definition>The molar heat capacity is the heat capacity per unit amount of a pure substance. [Wikipedia: https://en.wikipedia.org/wiki/Heat_capacity]</skos:definition>
    <rdf:type rdf:resource="http://www.w3.org/2004/02/skos/core#Concept"/>
    <odm2:dimensionCurrent>-2</odm2:dimensionCurrent>
    <skos:prefLabel>Molar heat capacity</skos:prefLabel>
    <skos:historyNote>QUDT</skos:historyNote>
    <odm2:dimensionMass>2</odm2:dimensionMass>
    <odm2:dimensionAmount>-1</odm2:dimensionAmount>
    <odm2:defaultUnit>Joule per mole kelvin (J/(mol-K))</odm2:defaultUnit>
    <odm2:dimensionLight>-1</odm2:dimensionLight>
    <skos:exactMatch>http://qudt.org/schema/qudt#MolarHeatCapacityUnit</skos:exactMatch>
    <odm2:category>Thermodynamics</odm2:category>
    <odm2:dimensionLength>0</odm2:dimensionLength>
  </rdf:Description>
  <rdf:Description rdf:about="http://vocabulary.odm2.org/unitstype/pH">
    <rdf:type rdf:resource="http://www.w3.org/2004/02/skos/core#Concept"/>
    <odm2:dimensionMass>0</odm2:dimensionMass>
    <odm2:dimensionSymbol>U1</odm2:dimensionSymbol>
    <odm2:dimensionCurrent>0</odm2:dimensionCurrent>
    <skos:inScheme rdf:resource="http://vocabulary.odm2.org/unitstype"/>
    <odm2:dimensionTime>0</odm2:dimensionTime>
    <skos:exactMatch>http://environment.data.gov.au/def/unit/pH</skos:exactMatch>
    <odm2:category>Chemistry</odm2:category>
    <odm2:dimensionLight>0</odm2:dimensionLight>
    <odm2:defaultUnit>pH</odm2:defaultUnit>
    <skos:historyNote>QUDT-WQ</skos:historyNote>
    <skos:prefLabel>pH</skos:prefLabel>
    <odm2:dimensionLength>1</odm2:dimensionLength>
    <odm2:dimensionAmount>0</odm2:dimensionAmount>
    <odm2:dimensionTemperature>0</odm2:dimensionTemperature>
    <skos:definition>In chemistry, pH (/pi??e?t?/) is a numeric scale used to specify the acidity or alkalinity of an aqueous solution. It is the negative of the logarithm to base 10 of the activity of the hydrogen ion. Solutions with a pH less than 7 are acidic and solutions with a pH greater than 7 are alkaline or basic. Pure water is neutral, being neither an acid nor a base. Contrary to popular belief, the pH value can be less than 0 or greater than 14 for very strong acids and bases respectively. [Wikipedia: https://en.wikipedia.org/wiki/PH]</skos:definition>
  </rdf:Description>
  <rdf:Description rdf:about="http://vocabulary.odm2.org/unitstype/massFlux">
    <skos:inScheme rdf:resource="http://vocabulary.odm2.org/unitstype"/>
    <odm2:dimensionCurrent>-1</odm2:dimensionCurrent>
    <odm2:dimensionMass>-2</odm2:dimensionMass>
    <odm2:dimensionSymbol>L-2M1T-1</odm2:dimensionSymbol>
    <odm2:category>Chemistry</odm2:category>
    <rdf:type rdf:resource="http://www.w3.org/2004/02/skos/core#Concept"/>
    <skos:prefLabel>Mass flux</skos:prefLabel>
    <odm2:defaultUnit>kilograms per meter squared per second (kg/m^2s)</odm2:defaultUnit>
    <odm2:dimensionTime>1</odm2:dimensionTime>
    <odm2:dimensionTemperature>0</odm2:dimensionTemperature>
    <odm2:dimensionAmount>0</odm2:dimensionAmount>
    <skos:historyNote>CUAHSI</skos:historyNote>
    <skos:definition>In physics and engineering, mass flux is the rate of mass flow per unit area, perfectly overlapping with the momentum density, the momentum per unit volume. The common symbols are j, J, q, Q, ?, or ? (Greek lower or capital Phi), sometimes with subscript m to indicate mass is the flowing quantity. Its SI units are kg s?1 m?2. Mass flux can also refer to an alternate form of flux in Fick's law that includes the molecular mass, or in Darcy's law that includes the mass density.  [Wikipedia: https://en.wikipedia.org/wiki/Mass_flux]</skos:definition>
    <odm2:dimensionLight>0</odm2:dimensionLight>
    <odm2:dimensionLength>0</odm2:dimensionLength>
  </rdf:Description>
  <rdf:Description rdf:about="http://vocabulary.odm2.org/unitstype/magnetomotiveForce">
    <skos:prefLabel>Magnetomotive force</skos:prefLabel>
    <odm2:dimensionSymbol>U1I1</odm2:dimensionSymbol>
    <odm2:dimensionAmount>0</odm2:dimensionAmount>
    <odm2:category>Electricity and Magnetism</odm2:category>
    <odm2:defaultUnit>Ampere Turn (At)</odm2:defaultUnit>
    <odm2:dimensionTemperature>1</odm2:dimensionTemperature>
    <odm2:dimensionCurrent>0</odm2:dimensionCurrent>
    <rdf:type rdf:resource="http://www.w3.org/2004/02/skos/core#Concept"/>
    <skos:definition>Magnetomotive force is any physical cause that produces magnetic flux. In other words, it is a field of magnetism (measured in tesla) that has area (measured in square meters), so that (Tesla)(Area)= Flux. It is analogous to electromotive force or voltage in electricity. MMF usually describes electric wire coils in a way so scientists can measure or predict the actual force a wire coil can generate. [Wikipedia: https://en.wikipedia.org/wiki/Magnetomotive_force]</skos:definition>
    <skos:inScheme rdf:resource="http://vocabulary.odm2.org/unitstype"/>
    <skos:historyNote>QUDT</skos:historyNote>
    <odm2:dimensionLight>0</odm2:dimensionLight>
    <odm2:dimensionLength>1</odm2:dimensionLength>
    <skos:exactMatch>http://qudt.org/schema/qudt#MagnetomotiveForceUnit</skos:exactMatch>
    <odm2:dimensionTime>0</odm2:dimensionTime>
    <odm2:dimensionMass>0</odm2:dimensionMass>
  </rdf:Description>
  <rdf:Description rdf:about="http://vocabulary.odm2.org/unitstype/volumeThermalExpansion">
    <odm2:dimensionTemperature>0</odm2:dimensionTemperature>
    <odm2:defaultUnit>Cubic meter per kelvin (m^3/K)</odm2:defaultUnit>
    <odm2:dimensionLight>0</odm2:dimensionLight>
    <odm2:dimensionMass>3</odm2:dimensionMass>
    <skos:prefLabel>Volume thermal expansion</skos:prefLabel>
    <odm2:dimensionLength>0</odm2:dimensionLength>
    <odm2:dimensionSymbol>L3?-1</odm2:dimensionSymbol>
    <odm2:category>Thermodynamics</odm2:category>
    <odm2:dimensionAmount>-1</odm2:dimensionAmount>
    <rdf:type rdf:resource="http://www.w3.org/2004/02/skos/core#Concept"/>
    <skos:inScheme rdf:resource="http://vocabulary.odm2.org/unitstype"/>
    <skos:historyNote>QUDT</skos:historyNote>
    <odm2:dimensionTime>0</odm2:dimensionTime>
    <skos:definition>When the temperature of a substance changes, the energy that is stored in the intermolecular bonds between atoms changes. When the stored energy increases, so does the length of the molecular bonds. As a result, solids typically expand in response to heating and contract on cooling; this dimensional response to temperature change is expressed by its coefficient of thermal expansion. Different coefficients of thermal expansion can be defined for a substance depending on whether the expansion is measured by: * linear thermal expansion * area thermal expansion * volumetric thermal expansion These characteristics are closely related. The volumetric thermal expansion coefficient can be defined for both liquids and solids. The linear thermal expansion can only be defined for solids, and is common in engineering applications. Some substances expand when cooled, such as freezing water, so they have negative thermal expansion coefficients.</skos:definition>
    <odm2:dimensionCurrent>0</odm2:dimensionCurrent>
    <skos:exactMatch>http://qudt.org/vocab/quantity#Volumethermalexpansion</skos:exactMatch>
  </rdf:Description>
  <rdf:Description rdf:about="http://vocabulary.odm2.org/unitstype/lengthTemperature">
    <odm2:dimensionAmount>1</odm2:dimensionAmount>
    <odm2:dimensionCurrent>0</odm2:dimensionCurrent>
    <odm2:dimensionMass>1</odm2:dimensionMass>
    <odm2:dimensionTime>0</odm2:dimensionTime>
    <skos:prefLabel>Length temperature</skos:prefLabel>
    <odm2:defaultUnit>Meter kelvin (m-K)</odm2:defaultUnit>
    <odm2:dimensionTemperature>0</odm2:dimensionTemperature>
    <skos:inScheme rdf:resource="http://vocabulary.odm2.org/unitstype"/>
    <odm2:category>Thermodynamics</odm2:category>
    <rdf:type rdf:resource="http://www.w3.org/2004/02/skos/core#Concept"/>
    <odm2:dimensionLight>0</odm2:dimensionLight>
    <odm2:dimensionSymbol>L1?1</odm2:dimensionSymbol>
    <odm2:dimensionLength>0</odm2:dimensionLength>
    <skos:exactMatch>http://qudt.org/schema/qudt#LengthTemperatureUnit</skos:exactMatch>
    <skos:historyNote>QUDT</skos:historyNote>
  </rdf:Description>
  <rdf:Description rdf:about="http://vocabulary.odm2.org/unitstype/lengthMolarEnergy">
    <odm2:dimensionMass>3</odm2:dimensionMass>
    <odm2:dimensionLight>-1</odm2:dimensionLight>
    <odm2:dimensionAmount>0</odm2:dimensionAmount>
    <skos:prefLabel>Length molar energy</skos:prefLabel>
    <skos:exactMatch>http://qudt.org/vocab/quantity#Lengthmolarenergy</skos:exactMatch>
    <rdf:type rdf:resource="http://www.w3.org/2004/02/skos/core#Concept"/>
    <odm2:dimensionTemperature>0</odm2:dimensionTemperature>
    <odm2:category>Chemistry</odm2:category>
    <odm2:dimensionTime>1</odm2:dimensionTime>
    <odm2:dimensionSymbol>L3M1T-2N-1</odm2:dimensionSymbol>
    <odm2:defaultUnit>Joule meter per mole</odm2:defaultUnit>
    <skos:inScheme rdf:resource="http://vocabulary.odm2.org/unitstype"/>
    <skos:historyNote>QUDT</skos:historyNote>
    <odm2:dimensionLength>0</odm2:dimensionLength>
    <odm2:dimensionCurrent>-2</odm2:dimensionCurrent>
  </rdf:Description>
  <rdf:Description rdf:about="http://vocabulary.odm2.org/unitstype/thermalResistance">
    <skos:historyNote>Wikipedia</skos:historyNote>
    <rdf:type rdf:resource="http://www.w3.org/2004/02/skos/core#Concept"/>
    <skos:inScheme rdf:resource="http://vocabulary.odm2.org/unitstype"/>
    <odm2:dimensionTemperature>0</odm2:dimensionTemperature>
    <odm2:category>Thermodynamics</odm2:category>
    <skos:definition>Thermal resistance is a heat property and a measurement of a temperature difference by which an object or material resists a heat flow. Thermal resistance is the reciprocal of thermal conductance. (Absolute) thermal resistance R in K/W is a property of a particular component. For example, a characteristic of a heat sink. Specific thermal resistance or specific thermal resistivity R? in (K·m)/W is a material constant.</skos:definition>
    <odm2:dimensionAmount>1</odm2:dimensionAmount>
    <odm2:dimensionLight>0</odm2:dimensionLight>
    <odm2:dimensionCurrent>3</odm2:dimensionCurrent>
    <skos:exactMatch>http://dbpedia.org/page/Thermal_resistance</skos:exactMatch>
    <odm2:dimensionTime>-1</odm2:dimensionTime>
    <skos:prefLabel>Thermal resistance</skos:prefLabel>
    <odm2:dimensionSymbol>L-2M-1T3?1</odm2:dimensionSymbol>
    <odm2:defaultUnit>Kelvin per watt (K/W)</odm2:defaultUnit>
    <odm2:dimensionMass>-2</odm2:dimensionMass>
    <odm2:dimensionLength>0</odm2:dimensionLength>
  </rdf:Description>
  <rdf:Description rdf:about="http://vocabulary.odm2.org/unitstype/angularVelocityOrFrequency">
    <skos:exactMatch>http://qudt.org/vocab/quantity#AngularVelocity</skos:exactMatch>
    <skos:note>Angular frequency uses the same units as that of angular velocity.</skos:note>
    <skos:historyNote>QUDT</skos:historyNote>
    <odm2:dimensionSymbol>U1T-1</odm2:dimensionSymbol>
    <skos:definition>The change of angle per unit time; specifically, in celestial mechanics, the change in angle of the radius vector per unit time.  Angular frequency is a scalar measure of rotation rate. It is the magnitude of the vector quantity angular velocity.</skos:definition>
    <odm2:dimensionLight>0</odm2:dimensionLight>
    <odm2:dimensionLength>1</odm2:dimensionLength>
    <odm2:dimensionTime>0</odm2:dimensionTime>
    <odm2:defaultUnit>Radian per second (rad/s)</odm2:defaultUnit>
    <skos:inScheme rdf:resource="http://vocabulary.odm2.org/unitstype"/>
    <skos:prefLabel>Angular velocity or frequency</skos:prefLabel>
    <rdf:type rdf:resource="http://www.w3.org/2004/02/skos/core#Concept"/>
    <odm2:dimensionMass>0</odm2:dimensionMass>
    <odm2:category>Space and Time</odm2:category>
    <odm2:dimensionAmount>0</odm2:dimensionAmount>
    <odm2:dimensionCurrent>-1</odm2:dimensionCurrent>
    <odm2:dimensionTemperature>0</odm2:dimensionTemperature>
  </rdf:Description>
</rdf:RDF>
