@prefix : <http://purl.org/iow/WaterBudgetingFramework/> .
@prefix dc: <http://purl.org/dc/elements/1.1/> .
@prefix dct: <http://purl.org/dc/terms/> .
@prefix fn: <http://www.w3.org/2005/xpath-functions#> .
@prefix gn: <http://www.geonames.org/ontology#> .
@prefix grddl: <http://www.w3.org/2003/g/data-view#> .
@prefix luc: <http://www.ontotext.com/owlim/lucene#> .
@prefix owl: <http://www.w3.org/2002/07/owl#> .
@prefix rdf: <http://www.w3.org/1999/02/22-rdf-syntax-ns#> .
@prefix rdfs: <http://www.w3.org/2000/01/rdf-schema#> .
@prefix sesame: <http://www.openrdf.org/schema/sesame#> .
@prefix skos: <http://www.w3.org/2004/02/skos/core#> .
@prefix wgs: <http://www.w3.org/2003/01/geo/wgs84_pos#> .
@prefix xml: <http://www.w3.org/XML/1998/namespace> .
@prefix xsd: <http://www.w3.org/2001/XMLSchema#> .

rdf:type a rdf:Property .

rdf:Property a rdfs:Class, owl:ObjectProperty .

rdfs:Class a rdfs:Class .

rdfs:Resource a rdfs:Class .

rdfs:subPropertyOf a rdf:Property .

rdfs:subClassOf a rdf:Property .

rdfs:domain a rdf:Property .

rdfs:range a rdf:Property .

owl:sameAs a rdf:Property .

owl:SymmetricProperty a rdfs:Class .

owl:TransitiveProperty a rdfs:Class .

owl:equivalentProperty a rdf:Property .

owl:equivalentClass a rdf:Property .

rdfs:Datatype a rdfs:Class .

owl:intersectionOf a rdf:Property .

owl:FunctionalProperty a rdfs:Class .

rdfs:ContainerMembershipProperty a rdfs:Class .

owl:someValuesFrom a rdf:Property .

owl:allValuesFrom a rdf:Property .

owl:inverseOf a rdf:Property .

rdfs:member a rdf:Property .

owl:hasValue a rdf:Property .

rdf:first a rdf:Property .

owl:onProperty a rdf:Property .

rdf:rest a rdf:Property .

owl:InverseFunctionalProperty a rdfs:Class .

rdfs:Literal a rdfs:Class .

rdf:nil a rdf:List .

rdf:subject a rdf:Property .

rdf:predicate a rdf:Property .

rdf:object a rdf:Property .

rdf:value a rdf:Property .

rdf:List a rdfs:Class .

rdf:Statement a rdfs:Class .

rdfs:comment a rdf:Property .

rdfs:label a rdf:Property .

rdf:Alt a rdfs:Class .

rdfs:Container a rdfs:Class .

rdf:Bag a rdfs:Class .

rdf:Seq a rdfs:Class .

rdfs:isDefinedBy a rdf:Property, owl:AnnotationProperty .

rdfs:seeAlso a rdf:Property .

rdf:XMLLiteral a rdfs:Datatype .

owl:differentFrom a rdf:Property .

<http://www.w3.org/1999/02/22-rdf-syntax-ns#> a owl:Ontology .

owl:Ontology a rdfs:Class .

dc:description a owl:AnnotationProperty .

rdf:HTML a rdfs:Datatype .

rdf:langString a rdfs:Datatype .

rdf:PlainLiteral a rdfs:Datatype .

<http://www.w3.org/2002/07/owl> a owl:Ontology .

owl:versionIRI a owl:OntologyProperty .

owl:imports a owl:OntologyProperty .

owl:versionInfo a owl:AnnotationProperty .

owl:AllDifferent a rdfs:Class .

owl:AllDisjointClasses a rdfs:Class .

owl:AllDisjointProperties a rdfs:Class .

owl:Annotation a rdfs:Class .

owl:AnnotationProperty a rdfs:Class .

owl:AsymmetricProperty a rdfs:Class .

owl:ObjectProperty a rdfs:Class .

owl:Axiom a rdfs:Class .

owl:Class a rdfs:Class .

owl:DataRange a rdfs:Class .

owl:DatatypeProperty a rdfs:Class .

owl:DeprecatedClass a rdfs:Class .

owl:DeprecatedProperty a rdfs:Class .

owl:IrreflexiveProperty a rdfs:Class .

owl:NamedIndividual a rdfs:Class .

owl:Thing a owl:Class .

owl:NegativePropertyAssertion a rdfs:Class .

owl:Nothing a owl:Class .

owl:OntologyProperty a rdfs:Class .

owl:ReflexiveProperty a rdfs:Class .

owl:Restriction a rdfs:Class .

owl:annotatedProperty a rdf:Property .

owl:annotatedSource a rdf:Property .

owl:annotatedTarget a rdf:Property .

owl:assertionProperty a rdf:Property .

owl:backwardCompatibleWith a owl:AnnotationProperty, owl:OntologyProperty .

owl:bottomDataProperty a owl:DatatypeProperty .

owl:bottomObjectProperty a owl:ObjectProperty .

owl:cardinality a rdf:Property .

owl:complementOf a rdf:Property .

owl:datatypeComplementOf a rdf:Property .

owl:deprecated a owl:AnnotationProperty .

owl:disjointUnionOf a rdf:Property .

owl:disjointWith a rdf:Property .

owl:distinctMembers a rdf:Property .

owl:hasKey a rdf:Property .

owl:hasSelf a rdf:Property .

owl:incompatibleWith a owl:AnnotationProperty, owl:OntologyProperty .

owl:maxCardinality a rdf:Property .

owl:maxQualifiedCardinality a rdf:Property .

owl:members a rdf:Property .

owl:minCardinality a rdf:Property .

owl:minQualifiedCardinality a rdf:Property .

owl:onClass a rdf:Property .

owl:onDataRange a rdf:Property .

owl:onDatatype a rdf:Property .

owl:oneOf a rdf:Property .

owl:onProperties a rdf:Property .

owl:priorVersion a owl:AnnotationProperty, owl:OntologyProperty .

owl:propertyChainAxiom a rdf:Property .

owl:propertyDisjointWith a rdf:Property .

owl:qualifiedCardinality a rdf:Property .

owl:sourceIndividual a rdf:Property .

owl:targetIndividual a rdf:Property .

owl:targetValue a rdf:Property .

owl:topDataProperty a owl:DatatypeProperty .

owl:topObjectProperty a owl:ObjectProperty .

owl:unionOf a rdf:Property .

owl:withRestrictions a rdf:Property .

<http://www.w3.org/2000/01/rdf-schema#> a owl:Ontology .

<http://www.w3.org/2004/02/skos/core> a owl:Ontology .

skos:Concept a owl:Class .

skos:definition a rdf:Property, owl:AnnotationProperty, owl:AnnotationProperty .

skos:ConceptScheme a owl:Class .

skos:scopeNote a rdf:Property, owl:AnnotationProperty .

skos:example a rdf:Property, owl:AnnotationProperty .

skos:Collection a owl:Class .

skos:OrderedCollection a owl:Class .

skos:inScheme a rdf:Property, owl:ObjectProperty .

skos:hasTopConcept a rdf:Property, owl:ObjectProperty .

skos:topConceptOf a rdf:Property, owl:ObjectProperty .

skos:prefLabel a rdf:Property, owl:AnnotationProperty, owl:AnnotationProperty .

skos:altLabel a rdf:Property, owl:AnnotationProperty .

skos:hiddenLabel a rdf:Property, owl:AnnotationProperty .

skos:notation a rdf:Property, owl:DatatypeProperty .

skos:note a rdf:Property, owl:AnnotationProperty, owl:AnnotationProperty .

skos:changeNote a rdf:Property, owl:AnnotationProperty .

skos:editorialNote a rdf:Property, owl:AnnotationProperty .

skos:historyNote a rdf:Property, owl:AnnotationProperty .

skos:semanticRelation a rdf:Property, owl:ObjectProperty .

skos:broader a rdf:Property, owl:ObjectProperty, owl:ObjectProperty .

skos:broaderTransitive a rdf:Property, owl:ObjectProperty, owl:TransitiveProperty .

skos:narrower a rdf:Property, owl:ObjectProperty .

skos:narrowerTransitive a rdf:Property, owl:ObjectProperty, owl:TransitiveProperty .

skos:related a rdf:Property, owl:ObjectProperty, owl:SymmetricProperty .

skos:member a rdf:Property, owl:ObjectProperty .

skos:memberList a rdf:Property, owl:FunctionalProperty, owl:ObjectProperty .

skos:mappingRelation a rdf:Property, owl:ObjectProperty .

skos:broadMatch a rdf:Property, owl:ObjectProperty .

skos:narrowMatch a rdf:Property, owl:ObjectProperty .

skos:relatedMatch a rdf:Property, owl:ObjectProperty, owl:SymmetricProperty .

skos:exactMatch a rdf:Property, owl:ObjectProperty, owl:SymmetricProperty, owl:TransitiveProperty .

skos:closeMatch a rdf:Property, owl:ObjectProperty, owl:SymmetricProperty .

<http://purl.org/iow/WaterBudgetingFramework/> a owl:Ontology .

<http://webprotege.stanford.edu/project/qrUilGBx2x8YZBCY6iSVG> a owl:Ontology .

dc:source a owl:AnnotationProperty .

:flowSink a owl:ObjectProperty .

:Component a owl:Class .

:flowDomain a owl:Class .

:flowSource a owl:ObjectProperty .

:hasDataSource a owl:ObjectProperty .

:Parameter a owl:Class .

:DataSource a owl:Class .

:hasEstimationMethod a owl:ObjectProperty .

:EstimationMethod a owl:Class .

:hasParameter a owl:ObjectProperty .

:isFlowType a owl:ObjectProperty .

:flowType a owl:Class .

:isPartialSubComponentOf a owl:ObjectProperty, owl:SymmetricProperty .

:isSubComponentOf a owl:ObjectProperty, owl:TransitiveProperty .

:type a owl:ObjectProperty .

:usedBy a owl:ObjectProperty .

:Jurisdiction a owl:Class .

skos:isExactMatch a owl:ObjectProperty, owl:SymmetricProperty, owl:TransitiveProperty .

:flowProportion a owl:DatatypeProperty .

<http://geoconnex.us/iow/WaterBudgetingFramework/ClosureTerm> a owl:Class .

:Basin a owl:Class .

:Element a owl:Class .

:External a owl:Class .

:SubtotalTerm a owl:Class .

:Zone a owl:Class .

:AZ a :Jurisdiction, owl:NamedIndividual .

:AgriculturalAndMunicipalDepletions-UT a :Component, owl:NamedIndividual .

:Atmosphere a :External, owl:NamedIndividual .

:ZoneGroundwater a :Zone, owl:NamedIndividual .

:ZoneSurfaceWater a :Zone, owl:NamedIndividual .

:Outflow a :flowType, owl:NamedIndividual .

:CropConsumptiveUse-CO a :Component, owl:NamedIndividual .

:GroundwaterExtraction-CA a :Component, owl:NamedIndividual .

:LivestockConsumptiveUse-CO a :Component, owl:NamedIndividual .

:MunicipalAndIndustrialConsumptiveUse-CO a :Component, owl:NamedIndividual .

:MunicipalConsumptiveUse-WY a :Component, owl:NamedIndividual .

:MunicipalTotalUse-WY a :Component, owl:NamedIndividual .

:SurfaceWaterDiversions-CA a :Component, owl:NamedIndividual .

:AgriculturalAndMunicipalDiversions-UT a :Component, owl:NamedIndividual .

:AppliedWater-CA a :Component, owl:NamedIndividual .

:UT a :Jurisdiction, owl:NamedIndividual .

:ZoneLandSystem a :Zone, owl:NamedIndividual .

:USGSStreamGages a :DataSource, owl:NamedIndividual .

:UTDiversionRecordsFromRiverCommissioners a :DataSource, owl:NamedIndividual .

:UTMunicipalPotableAndSecondaryDiversionRecords a :DataSource, owl:NamedIndividual .

:UTOtherIrrigationCompanyRecords a :DataSource, owl:NamedIndividual .

:UTReservoirStorageAndReleaseRecords a :DataSource, owl:NamedIndividual .

:UTWaterRights a :DataSource, owl:NamedIndividual .

:USGSStreamStats a :EstimationMethod, owl:NamedIndividual .

:UTDivisionOfWaterResourcesArea-AltitudeMethod a :EstimationMethod, owl:NamedIndividual .

:USGSMeanAnnualReachEstimates a :Parameter, owl:NamedIndividual .

:InternalTransfer a :flowType, owl:NamedIndividual .

:AgriculturalConsumptiveUse-WY a :Component, owl:NamedIndividual .

:WYConsumptiveUseMethod a :EstimationMethod, owl:NamedIndividual .

:Evapotranspiration-CA a :Component, owl:NamedIndividual .

:IrrigationSurfaceWaterDiversions-WY a :Component, owl:NamedIndividual .

:TotalDiversions-WY a :Component, owl:NamedIndividual .

:BearRiver a :Basin, owl:NamedIndividual .

:GreenRiver a :Basin, owl:NamedIndividual .

:NortheastRiver a :Basin, owl:NamedIndividual .

:PlatteRiver a :Basin, owl:NamedIndividual .

:Powder-TongueRiver a :Basin, owl:NamedIndividual .

:Salt-SnakeRiver a :Basin, owl:NamedIndividual .

:WY a :Jurisdiction, owl:NamedIndividual .

:Wind-BighornRiver a :Basin, owl:NamedIndividual .

:AgriculturalDepletions-UT a :Component, owl:NamedIndividual .

:UTConsumptiveUseMethod a :EstimationMethod, owl:NamedIndividual .

:SurfaceDiversionToCropland-UT a :Component, owl:NamedIndividual .

:AgriculturalPotentialConsumptiveUse-UT a :Component, owl:NamedIndividual .

:NationalOceanicAndAtmosphericAdministrationStations a :DataSource, owl:NamedIndividual .

:PRISM a :DataSource, owl:NamedIndividual .

:USBureauOfReclamationAgriMetStations a :DataSource, owl:NamedIndividual .

:USUResearchReport145 a :DataSource, owl:NamedIndividual .

:DailyPenman-Monteith a :EstimationMethod, owl:NamedIndividual .

:ModifiedBlaney-Criddle a :EstimationMethod, owl:NamedIndividual .

:SolarRadiation a :Parameter, owl:NamedIndividual .

:Temperature a :Parameter, owl:NamedIndividual .

:VaporPressure a :Parameter, owl:NamedIndividual .

:WindRun a :Parameter, owl:NamedIndividual .

:ClimateCoefficient%28kt%29 a :Parameter, owl:NamedIndividual .

:CropGrowthStateCoefficient%28Kc%29 a :Parameter, owl:NamedIndividual .

:MeanMonthlyAirTemperatures%28T%29 a :Parameter, owl:NamedIndividual .

:MonthlyPercentageOfAnnualDaylightHours%28P%29 a :Parameter, owl:NamedIndividual .

:AnnualEmployeeHours a :Parameter, owl:NamedIndividual .

:MineSafetyAndHealthAdministration%28MSHA%29 a :DataSource, owl:NamedIndividual .

:AnnualEvaporation a :Parameter, owl:NamedIndividual .

:MonthlyEvaporation a :Parameter, owl:NamedIndividual .

:NM a :Jurisdiction, owl:NamedIndividual .

:AnnualSodaAshProduction a :Parameter, owl:NamedIndividual .

:USGeologicalSurvey%28USGS%29 a :DataSource, owl:NamedIndividual .

:TotalLandSystemInflow-CA a :Component, :SubtotalTerm, owl:NamedIndividual .

:CA a :Jurisdiction, owl:NamedIndividual .

:AreaOutflows a :Component, owl:NamedIndividual .

:BasinOutflow-UT a :Component, owl:NamedIndividual .

:ExternalSurfaceWater a :External, owl:NamedIndividual .

:GagedStreamOutflow-WY a :Component, owl:NamedIndividual .

:StreamOutfow-CA a :Component, owl:NamedIndividual .

:Exports-CO a :Component, owl:NamedIndividual .

:TotalSurfaceWaterOutflow-CA a :Component, :SubtotalTerm, owl:NamedIndividual .

:AverageMonthlyReservoirGageHeight a :Parameter, owl:NamedIndividual .

:IrrigationDistricts a :DataSource, owl:NamedIndividual .

:USArmyCorpsOfEngineers a :DataSource, owl:NamedIndividual .

:USBureauOfReclamationStations a :DataSource, owl:NamedIndividual .

:NewMexicoInterstateStreamCommission%28NMISC%29 a :DataSource, owl:NamedIndividual .

:AverageUseRate a :Parameter, owl:NamedIndividual .

:MidwestPlanServiceStructuresAndEnvironmentalHandbook%2C1977 a :DataSource, owl:NamedIndividual .

:CO a :Jurisdiction, owl:NamedIndividual .

:Baseflow a :Parameter, owl:NamedIndividual .

:HistoricalData a :DataSource, :EstimationMethod, owl:NamedIndividual .

:BasinInflow-UT a :Component, owl:NamedIndividual .

:RiverInflow-UT a :Component, owl:NamedIndividual .

:Inflow a :flowType, owl:NamedIndividual .

:GagedStreamInflow-WY a :Component, owl:NamedIndividual .

:GagedSurfaceWaterInflow-CO a :Component, owl:NamedIndividual .

:UngagedSurfaceWaterInflow-CO a :Component, owl:NamedIndividual .

:TotalSurfaceWaterInflow-CA a :Component, :SubtotalTerm, owl:NamedIndividual .

:StreamInflow-CA a :Component, owl:NamedIndividual .

:COAgriculturalMeteorologyNetworkStation a :DataSource, owl:NamedIndividual .

:COConsumptiveUseMethod a :EstimationMethod, owl:NamedIndividual .

:CODiversionRecords a :DataSource, owl:NamedIndividual .

:CODivisionOfWaterResourcesGages a :DataSource, owl:NamedIndividual .

:HydroBase a :DataSource, owl:NamedIndividual .

:SCSTR21 a :DataSource, :EstimationMethod, owl:NamedIndividual .

:SatelliteAndAerialPhotos a :DataSource, owl:NamedIndividual .

:SnotelNetworkOfWeatherStations a :DataSource, owl:NamedIndividual .

:WeatherStations a :DataSource, owl:NamedIndividual .

:CommunityCollaborativeRain%2CHailAndSnowNetwork%28CoCoRaHS%29 a :DataSource, owl:NamedIndividual .

:NationalAgriculturalStatisticsService%28NASS%29CroplandDataLayer a :DataSource, owl:NamedIndividual .

:RemoteAutomatedWeatherStations%28RAWS%29 a :DataSource, owl:NamedIndividual .

:COIrrigatedAcreageAssessment a :EstimationMethod, owl:NamedIndividual .

:CropIrrigationRequirementEstimationMethod a :EstimationMethod, owl:NamedIndividual .

:EnergyBalanceRemoteSensing a :EstimationMethod, owl:NamedIndividual .

:METRIC a :EstimationMethod, owl:NamedIndividual .

:ModifiedBlaney-CriddleWithETElevationAdjustment a :EstimationMethod, owl:NamedIndividual .

:NDVIRemoteSensing a :EstimationMethod, owl:NamedIndividual .

:NDVIstar a :EstimationMethod, owl:NamedIndividual .

:On-FarmWaterBalance a :EstimationMethod, owl:NamedIndividual .

:OriginalBlaney-Criddle a :EstimationMethod, owl:NamedIndividual .

:OriginalBlaney-CriddleWithETElevationAdjustment a :EstimationMethod, owl:NamedIndividual .

:RESET a :EstimationMethod, owl:NamedIndividual .

:StateCU a :EstimationMethod, owl:NamedIndividual .

:CropIrrigationRequirement a :Parameter, owl:NamedIndividual .

:CropType a :Parameter, owl:NamedIndividual .

:EffectivePrecipitation a :Parameter, owl:NamedIndividual .

:IrrigatedAcreage a :Parameter, owl:NamedIndividual .

:IrrigationMethod a :Parameter, owl:NamedIndividual .

:PotentialConsumptiveUse a :Parameter, owl:NamedIndividual .

:Precipitation a :Parameter, owl:NamedIndividual .

:SupplySource a :Parameter, owl:NamedIndividual .

:SupplyType a :Parameter, owl:NamedIndividual .

:WaterSupply a :Parameter, owl:NamedIndividual .

:CODivisionOfWaterResources a :DataSource, owl:NamedIndividual .

:COGISExercise a :DataSource, owl:NamedIndividual .

:COLivestockMethod a :EstimationMethod, owl:NamedIndividual .

:StateAgriculturalStatistics a :DataSource, owl:NamedIndividual .

:LivestockCount a :Parameter, owl:NamedIndividual .

:COMunicipalAndIndustrialMethod a :EstimationMethod, owl:NamedIndividual .

:ConsumptiveRatio a :Parameter, owl:NamedIndividual .

:GrossUsage a :Parameter, owl:NamedIndividual .

:Population a :Parameter, owl:NamedIndividual .

:CONativeVegetationMethod a :EstimationMethod, owl:NamedIndividual .

:HistoricalDiversionsFile a :DataSource, owl:NamedIndividual .

:Unknown a :DataSource, owl:NamedIndividual .

:Diversions a :Parameter, owl:NamedIndividual .

:NativeVegetationCoefficient a :Parameter, owl:NamedIndividual .

:ReturnFlow a :Parameter, owl:NamedIndividual .

:ChangeInGroundWaterStorage-CO a :Component, owl:NamedIndividual, _:node1e55oknkkx676 .

_:node1e55oknkkx676 a owl:Restriction .

:ChangeInGroundWaterStorage-CO a _:node1e55oknkkx773 .

:StorageChange a :flowType, owl:NamedIndividual .

:ChangeInGroundwaterStorage-CA a :Component, owl:NamedIndividual .

:ChangeInGroundwaterStorage-AUS a :Component, owl:NamedIndividual .

:ChangeInTotalSystemStorage-CA a :Component, owl:NamedIndividual .

:ChangeInLandSystemStorage-CA a :Component, owl:NamedIndividual .

:ChangeInSurfaceWaterStorage-AUS a :Component, owl:NamedIndividual .

:ChangeInSurfaceWaterStorage-CA a :Component, owl:NamedIndividual .

:ChangeInSurfaceWaterStorage-CO a :Component, owl:NamedIndividual, _:node1e55oknkkx678 .

_:node1e55oknkkx678 a owl:Restriction .

:ChangeInSurfaceWaterStorage-CO a _:node1e55oknkkx775 .

:Class a owl:NamedIndividual .

:ClassAPanEvaporationData a :Parameter, owl:NamedIndividual .

:CoalProductionQuantities a :Parameter, owl:NamedIndividual .

:ColoradoCensusBureau a :DataSource, owl:NamedIndividual .

:ColoradoStateMod a :EstimationMethod, owl:NamedIndividual .

:ColoradoWaterConservationBoard%28CWCB%29 a :DataSource, owl:NamedIndividual .

:DirectFlowDemand-Annual a :Parameter, owl:NamedIndividual .

:DirectFlowDemand-Monthly a :Parameter, owl:NamedIndividual .

:Evaporation a :Parameter, owl:NamedIndividual .

:InstreamFlowDemand-Annual a :Parameter, owl:NamedIndividual .

:InstreamFlowDemand-Monthly a :Parameter, owl:NamedIndividual .

:ReservoirTargets a :Parameter, owl:NamedIndividual .

:Streamflow a :Parameter, owl:NamedIndividual .

:WellDemand-Monthly a :Parameter, owl:NamedIndividual .

:Commercial-NMOSE a :Component, owl:NamedIndividual .

:MunicipalAndIndustrialDiversions-UT a :Component, owl:NamedIndividual .

:ConservancyDistricts a :DataSource, owl:NamedIndividual .

:ConveyanceEvaporation-CA a :Component, owl:NamedIndividual .

:HumanConsumption-NM a :Component, owl:NamedIndividual .

:ConveyanceLossesForAllocatedDiversions-AUS a :Component, owl:NamedIndividual .

:SurfaceWaterOutflows-AUS a :Component, owl:NamedIndividual .

:ConveyanceSeepage-CA a :Component, owl:NamedIndividual .

:TotalGroundwaterSystemInflow-CA a :Component, :SubtotalTerm, owl:NamedIndividual .

:CoplandPrecipitation-UT a :Component, owl:NamedIndividual .

:Precipitation-CA a :Component, owl:NamedIndividual .

:Precipitation-CO a :Component, owl:NamedIndividual .

:Precipitation-NM a :Component, owl:NamedIndividual .

:Precipitation-UT a :Component, owl:NamedIndividual .

:Precipitation-WY a :Component, owl:NamedIndividual .

:IrrigatedAgricultureDepletions-NMOSE a :Component, owl:NamedIndividual .

:EmeryWaterConservancyDistrictStations a :DataSource, owl:NamedIndividual .

:MesoWestStations a :DataSource, owl:NamedIndividual .

:NationalWeatherServiceStations a :DataSource, owl:NamedIndividual .

:NewMexicoClimateCenterStations a :DataSource, owl:NamedIndividual .

:CooperativeObserverNetwork%28COOP%29 a :DataSource, owl:NamedIndividual .

:FruitGrowersNetworkStations%28FGNET%29 a :DataSource, owl:NamedIndividual .

:NationalClimaticDataCenter%27sClimatographyOfTheUnitedStatesNo.81 a :DataSource,
    owl:NamedIndividual .

:NaturalResourcesConservationServiceStations%28NRCS%29 a :DataSource, owl:NamedIndividual .

:SoilClimateAnalysisNetwork%28SCAN%29 a :DataSource, owl:NamedIndividual .

:USBureauOfLandManagement%28BLM%29 a :DataSource, owl:NamedIndividual .

:WYDepartmentOfEnvironmentalQuality%28DEQ%29 a :DataSource, owl:NamedIndividual .

:WesternRegionalClimateCenter%28WRCC%29Stations a :DataSource, owl:NamedIndividual .

:WyomingStateEngineer%27sOfficeStations a :DataSource, owl:NamedIndividual .

:USBR a :Jurisdiction, owl:NamedIndividual .

:CropTypeStateAssessments a :DataSource, owl:NamedIndividual .

:FieldSurvey a :DataSource, owl:NamedIndividual .

:GroundSurvey a :DataSource, owl:NamedIndividual .

:USDACroplandDataLayer%28CDL%29 a :DataSource, owl:NamedIndividual .

:DailyASCEStandardizedPenman-Monteith a :EstimationMethod, owl:NamedIndividual .

:DailyEffectivePrecipitation a :Parameter, owl:NamedIndividual .

:DailyModifiedHargreaves a :EstimationMethod, owl:NamedIndividual .

:DaytimeHours a :Parameter, owl:NamedIndividual .

:DirectCommunication a :EstimationMethod, owl:NamedIndividual .

:WyomingWaterDevelopmentCommission%28WWDC%292002WaterSystemSurveyReport a :DataSource,
    owl:NamedIndividual .

:WYDiversionDataFromWaterUsers a :DataSource, owl:NamedIndividual .

:WYOfficeOfTheStateEngineer a :DataSource, owl:NamedIndividual .

:DivertibleFlow-WY a :Parameter, owl:NamedIndividual .

:DomesticTotalUse-WY a :Component, owl:NamedIndividual .

:USCensusBureau a :DataSource, owl:NamedIndividual .

:WithdrawalMethod a :EstimationMethod, owl:NamedIndividual .

:GallonsPerCapitaPerDay%28GPCD%29 a :Parameter, owl:NamedIndividual .

:DownstreamFlow a :Parameter, owl:NamedIndividual .

:WyomingWaterResourcesDataSystem%28WRDS%29 a :DataSource, owl:NamedIndividual .

:UTEffectivePrecipitationMethod a :EstimationMethod, owl:NamedIndividual .

:EffectivePrecipitationFactor a :Parameter, owl:NamedIndividual .

:ElectricalGenerationData a :Parameter, owl:NamedIndividual .

:USEnergyInformationAdministration%28USEIA%29 a :DataSource, owl:NamedIndividual .

:Elevation-Area-CapacityTables a :Parameter, owl:NamedIndividual .

:USBureauOfReclamation a :DataSource, owl:NamedIndividual .

:UTStateEngineerData a :DataSource, owl:NamedIndividual .

:WaterResourcesStudies a :DataSource, owl:NamedIndividual .

:EmpiricalDataForSmallReservoirs a :EstimationMethod, owl:NamedIndividual .

:MonthlyPrecipitationVolume a :Parameter, owl:NamedIndividual .

:Rainfall a :Parameter, owl:NamedIndividual .

:ReservoirSurfaceArea a :Parameter, owl:NamedIndividual .

:Evaporation-AUS a :Component, owl:NamedIndividual .

:Evaporation-NM a :Component, owl:NamedIndividual .

:TotalEvaporation-NM a :Component, :SubtotalTerm, owl:NamedIndividual .

:EvaporationFromReservoirs-NMOSE a :Component, owl:NamedIndividual .

:PanApproach a :EstimationMethod, owl:NamedIndividual .

:MonthlyGrossEvaporationRate a :Parameter, owl:NamedIndividual .

:WinterIceSurfaceArea a :Parameter, owl:NamedIndividual .

:LakeEvaporation-CA a :Component, owl:NamedIndividual .

:ReservoirEvaporation-CO a :Component, owl:NamedIndividual .

:ReservoirEvaporation-UT a :Component, owl:NamedIndividual .

:TotalLandSystemOutflow-CA a :Component, :SubtotalTerm, owl:NamedIndividual .

:ExternalGroundwater a :External, owl:NamedIndividual .

:GroundwaterExport-CA a :Component, owl:NamedIndividual .

:StoredWaterExport-CA a :Component, owl:NamedIndividual .

:SurfaceWaterExports-CA a :Component, owl:NamedIndividual .

:ExternalLandSystem a :External, owl:NamedIndividual .

:FacilityDirectorOrOperator a :DataSource, owl:NamedIndividual .

:FederalArchives a :DataSource, owl:NamedIndividual .

:FloodReturn-AUS a :Component, owl:NamedIndividual .

:SurfaceWaterInflows-AUS a :Component, owl:NamedIndividual .

:Flow a :Parameter, owl:NamedIndividual .

:GPSPopulationData a :DataSource, owl:NamedIndividual .

:GageHeight a :Parameter, owl:NamedIndividual .

:TotalInflow-CA a :Component, :SubtotalTerm, owl:NamedIndividual .

:TotalOutflow-CA a :Component, :SubtotalTerm, owl:NamedIndividual .

:GagedSurfaceWaterOutflow-CO a :Component, owl:NamedIndividual .

:GrossActivelyIrrigatedAcreage a :Parameter, owl:NamedIndividual .

:NationalAgriculturalStatisticsService a :DataSource, owl:NamedIndividual .

:USDAFarmServiceAgency a :DataSource, owl:NamedIndividual .

:NMOfficeOfTheStateEngineer%28NMOSE%29 a :DataSource, owl:NamedIndividual .

:GrossMonthlyFreeWaterSurfaceEvaporation a :Parameter, owl:NamedIndividual .

:NOAATechnicalReportNWS33 a :DataSource, owl:NamedIndividual .

:GroundWaterInflow-CO a :Component, owl:NamedIndividual .

:SubsurfaceInflow-CA a :Component, owl:NamedIndividual .

:GroundWaterOutflow-CO a :Component, owl:NamedIndividual .

:TotalGroundwaterSystemOutflow-CA a :Component, :SubtotalTerm, owl:NamedIndividual .

:SubsurfaceOutflow-CA a :Component, owl:NamedIndividual .

:GroundwaterDischarge-AUS a :Component, owl:NamedIndividual .

:Discharge%3AGroundwater-AUS a :Component, owl:NamedIndividual .

:GroundwaterDiversions-NM a :Component, owl:NamedIndividual .

:GroundwaterET-NM a :Component, owl:NamedIndividual .

:RiparianConsumption-NM a :Component, owl:NamedIndividual .

:LakeGainFromGroundwater-CA a :Component, owl:NamedIndividual .

:GroundwaterInflows-AUS a :Component, owl:NamedIndividual .

:GroundwaterInflows-NM a :Component, owl:NamedIndividual .

:GroundwaterOutflows-AUS a :Component, owl:NamedIndividual .

:GroundwaterOutflows-NM a :Component, owl:NamedIndividual .

:GroundwaterReturn-NM a :Component, owl:NamedIndividual .

:GroundwaterStock-NM a :Component, owl:NamedIndividual .

:GroundwaterUse a :Parameter, owl:NamedIndividual .

:MunicipalAndIndustrialDiversionReports a :DataSource, owl:NamedIndividual .

:USGSEstimatesOfBasinGroundwaterFlows a :DataSource, owl:NamedIndividual .

:USGSGroundwaterReports a :DataSource, owl:NamedIndividual .

:GroundwaterUse-UT a :Component, owl:NamedIndividual .

:PumpedGroundwater-UT a :Component, owl:NamedIndividual .

:GroundwaterWithdrawals a owl:NamedIndividual .

:HighPlainsClimateCenter-UniversityOfNebraska a :DataSource, owl:NamedIndividual .

:UTStateArchives a :DataSource, owl:NamedIndividual .

:HumanPopulationModel-NM a :DataSource, owl:NamedIndividual .

:HumanReturns-NM a :Component, owl:NamedIndividual .

:HumanStorageAndDistributionSystemStock-NM a :Component, owl:NamedIndividual .

:ImportedWater-CA a :Component, owl:NamedIndividual .

:Imports-CO a :Component, owl:NamedIndividual .

:IndicatorGageApproach a :EstimationMethod, owl:NamedIndividual .

:Industrial-NMOSE a :Component, owl:NamedIndividual .

:Metered a :EstimationMethod, owl:NamedIndividual .

:IndustrialConsumptiveUse-WY a :Component, owl:NamedIndividual .

:IndustrialTotalUse-WY a :Component, owl:NamedIndividual .

:WyomingOilAndGasConservationCommission%28WYOGCC%29 a :DataSource, owl:NamedIndividual .

:MonthlyCoalbedMethaneGasProductionAndProducedWater a :Parameter, owl:NamedIndividual .

:NaturalGasProcessingVolumes a :Parameter, owl:NamedIndividual .

:MonthlyOil%2CGas%2CAndProducedWater a :Parameter, owl:NamedIndividual .

:SurfaceWaterDelivery-CA a :Component, owl:NamedIndividual .

:Inflow-OutflowApproach a :EstimationMethod, owl:NamedIndividual .

:Inter-regionCoastalInflow-AUS a :Component, owl:NamedIndividual .

:Inter-regionCoastalOutflow-AUS a :Component, owl:NamedIndividual .

:InterpolationFromOtherRecords a :EstimationMethod, owl:NamedIndividual .

:NMIrrigatedAcreageAssessment a :EstimationMethod, owl:NamedIndividual .

:USBRIrrigatedAcreageAssessment a :EstimationMethod, owl:NamedIndividual .

:UTIrrigatedAcreageAssessment a :EstimationMethod, owl:NamedIndividual .

:WYIrrigatedAcreageAssessment a :EstimationMethod, owl:NamedIndividual .

:SupplyStructure a :Parameter, owl:NamedIndividual .

:IrrigatedAgriculture-NMOSE a :Component, owl:NamedIndividual .

:NMConsumptiveUseMethod a :EstimationMethod, owl:NamedIndividual .

:IrrigatedAgricultureDiversions-NMOSE a :Component, owl:NamedIndividual .

:NMOSECropAcreageFile a :DataSource, owl:NamedIndividual .

:NMOSEGrowingSeasonFile a :DataSource, owl:NamedIndividual .

:NMOSETemperatureAndPrecipitationFile a :DataSource, owl:NamedIndividual .

:ConsumptiveIrrigationRequirement%28CIR%29 a :Parameter, owl:NamedIndividual .

:IrrigationSchemeInflows-AUS a :Component, owl:NamedIndividual .

:IrrigationSchemeOutflows-AUS a :Component, owl:NamedIndividual .

:LCRAS a :Jurisdiction, owl:NamedIndividual .

:LakeLossToGroundwater-CA a :Component, owl:NamedIndividual .

:Recharge-NM a :Component, owl:NamedIndividual .

:LandSurfaceExapotranspiration-NM a :Component, owl:NamedIndividual .

:LandSurfaceStock-NM a :Component, owl:NamedIndividual .

:Livestock-NMOSE a :Component, owl:NamedIndividual .

:LivestockConsumptiveUse-WY a :Component, owl:NamedIndividual .

:LivestockPopulation a :Parameter, owl:NamedIndividual .

:NewMexicoDepartmentOfAgriculture a :DataSource, owl:NamedIndividual .

:ManagedAquiferRecharge-AUS a :Component, owl:NamedIndividual .

:UrbanWaterSystemOutflows-AUS a :Component, owl:NamedIndividual .

:ManagedAquiferRecharge-CA a :Component, owl:NamedIndividual .

:MilitaryBasePopulationData a :DataSource, owl:NamedIndividual .

:Mining-NMOSE a :Component, owl:NamedIndividual .

:Industrial%3AMineProduction-WY a :Component, owl:NamedIndividual .

:SumOfMonthlyConsumptiveUseFactorsForGrowingSeason%28F%29 a :Parameter, owl:NamedIndividual .

:MonthlyEffectivePrecipitation a :Parameter, owl:NamedIndividual .

:Power-NMOSE a :Component, owl:NamedIndividual .

:PublicWaterSupply-NMOSE a :Component, owl:NamedIndividual .

:MunicipalAndIndustrialDepeltion-UT a :Component, owl:NamedIndividual .

:MunicipalAndIndustrialReturnFlow-UT a :Component, owl:NamedIndividual .

:ReturnFlow-CA a :Component, owl:NamedIndividual .

:MunicipalAndSelfSuppliedDomestic-NM a :Component, owl:NamedIndividual .

:NDVI a :Parameter, owl:NamedIndividual .

:NMDiversionRecords a :DataSource, owl:NamedIndividual .

:NMSpreadsheet-BasedConsumptiveUseModel a :EstimationMethod, owl:NamedIndividual .

:OriginalHargreaves a :EstimationMethod, owl:NamedIndividual .

:NMIrrigationWithdrawals a :EstimationMethod, owl:NamedIndividual .

:NMOSEWaterRightsDatabase a :DataSource, owl:NamedIndividual .

:NMOSETechnicalReportNo.48 a :DataSource, owl:NamedIndividual .

:NativeVegetationConsumptiveUse-CO a :Component, owl:NamedIndividual .

:NaturalSystemUse-UT a :Component, owl:NamedIndividual .

:RiparianDepletions-UT a :Component, owl:NamedIndividual .

:NaturalFlowGainDistribution a :EstimationMethod, owl:NamedIndividual .

:ProrationFactors a :Parameter, owl:NamedIndividual .

:Non-allocatedExtraction-AUS a :Component, owl:NamedIndividual .

:OtherIncreases-AUS a :Component, owl:NamedIndividual, _:node1e55oknkkx680 .

_:node1e55oknkkx680 a owl:Restriction .

:OtherIncreases-AUS a _:node1e55oknkkx777 .

:OtherStatutoryRights-AUS a :Component, owl:NamedIndividual .

:Outflow-AUS a :Component, owl:NamedIndividual .

:OverbankFloodSpilling-AUS a :Component, owl:NamedIndividual .

:OverbankFlow-AUS a :Component, owl:NamedIndividual .

:PersonalOutreach a :EstimationMethod, owl:NamedIndividual .

:WaterUseEstimate a :Parameter, owl:NamedIndividual .

:PopulationServedByPublicWaterSupply a :Parameter, owl:NamedIndividual .

:NewMexicoEnvironmentDepartment%28NMED%29 a :DataSource, owl:NamedIndividual .

:UniversityOfNewMexicoGeospatialAndPopulationStudies%28UNMGPS%29 a :DataSource, owl:NamedIndividual .

:PotentialEvapotranspiration a :Parameter, owl:NamedIndividual .

:Industrial%3AElectricalGeneration-WY a :Component, owl:NamedIndividual .

:WyomingWaterResourcesDataSystemsWaterAndClimateMapServer a :DataSource, owl:NamedIndividual .

:Precipitation-AUS a :Component, owl:NamedIndividual .

:PrecipitationOnLakes-CA a :Component, owl:NamedIndividual .

:RechargeOfAppliedWater-CA a :Component, owl:NamedIndividual .

:RechargeOfPrecipitation-CA a :Component, owl:NamedIndividual .

:RecycledWaterExport-CA a :Component, owl:NamedIndividual .

:ReservoirEstimationMethod a :EstimationMethod, owl:NamedIndividual .

:SurfaceAreaOfReservoir a :Parameter, owl:NamedIndividual .

:ReservoirEvaporation-WY a :Component, owl:NamedIndividual .

:PanMethod%28NetEvaporation%29 a :EstimationMethod, owl:NamedIndividual .

:GrossPanEvaportation%28inches%29 a :Parameter, owl:NamedIndividual .

:RiverAndFloodplainLosses-AUS a :Component, owl:NamedIndividual .

:RiverEvaporation-NM a :Component, owl:NamedIndividual .

:RiverUseByWetPasture-UT a :Component, owl:NamedIndividual .

:Runoff-AUS a :Component, owl:NamedIndividual .

:Runoff-CA a :Component, owl:NamedIndividual .

:Runoff-NM a :Component, owl:NamedIndividual .

:STATSGOSoilsData a :DataSource, owl:NamedIndividual .

:Self-SuppliedDomestic-NMOSE a :Component, owl:NamedIndividual .

:SelfSuppliedDomesticPopulation a :Parameter, owl:NamedIndividual .

:SoilMoistureHoldingCapacity a :Parameter, owl:NamedIndividual .

:WaterResourcesIrrigatedLandUseDatabase a :DataSource, owl:NamedIndividual .

:StateCUOutput a :Parameter, owl:NamedIndividual .

:StateData a :DataSource, owl:NamedIndividual .

:StoredWaterExtraction-CA a :Component, owl:NamedIndividual .

:StreamEvaporation-CA a :Component, owl:NamedIndividual .

:StreamGainFromGroundwater-CA a :Component, owl:NamedIndividual .

:StreamLossToGroundwater-CA a :Component, owl:NamedIndividual .

:StudentPopulation a :Parameter, owl:NamedIndividual .

:SurfaceWaterDiversions-NM a :Component, owl:NamedIndividual .

:SurfaceWaterEvaporation-NM a :Component, owl:NamedIndividual .

:SurfaceWaterFlows-UT a :Component, owl:NamedIndividual .

:SurfaceWaterGroundwaterInteractions-NM a :Component, owl:NamedIndividual, _:node1e55oknkkx682 .

_:node1e55oknkkx682 a owl:Restriction .

:SurfaceWaterGroundwaterInteractions-NM a _:node1e55oknkkx779 .

:SurfaceWaterInflows-NM a :Component, owl:NamedIndividual .

:SurfaceWaterOutflows-NM a :Component, owl:NamedIndividual .

:SurfaceWaterReturns-NM a :Component, owl:NamedIndividual .

:SurfaceWaterStock-NM a :Component, owl:NamedIndividual .

:TotalLandReturnFlow-UT a :Component, owl:NamedIndividual .

:TributaryInflow-UT a :Component, owl:NamedIndividual .

:USBRConsumptiveUseMethod a :EstimationMethod, owl:NamedIndividual .

:XCONS a :EstimationMethod, owl:NamedIndividual .

:USGS a :Jurisdiction, owl:NamedIndividual .

:UngagedLosses a :Component, owl:NamedIndividual .

:UngagedStreamGains-WY a :Component, owl:NamedIndividual .

:WyomingGain%2FLossEstimationMethod a :EstimationMethod, owl:NamedIndividual .

:UpstreamFlow a :Parameter, owl:NamedIndividual .

:UngagedStreamLosses-WY a :Component, owl:NamedIndividual .

:UniversityOfNewMexico a :DataSource, owl:NamedIndividual .

:UrbanWaterSystemInflows-AUS a :Component, owl:NamedIndividual .

:WYAgricultureConsumptiveUseEstimationMethod a :EstimationMethod, owl:NamedIndividual .

:WYDiversionRecords a :DataSource, owl:NamedIndividual .

:WYElectricalGenerationMethod a :EstimationMethod, owl:NamedIndividual .

:WYIndustrialProductionMethod a :EstimationMethod, owl:NamedIndividual .

:WYIrrigatedAcreageConsumptiveUseModel a :EstimationMethod, owl:NamedIndividual .

:WYMineProductionMethod a :EstimationMethod, owl:NamedIndividual .

:WYOfficeOfTheStateEngineerHydrographerCommissionerReports a :Element, owl:NamedIndividual .

:WYVariousWaterSupplyReports a :DataSource, owl:NamedIndividual .

:WastewaterCollected-AUS a :Component, owl:NamedIndividual .

:WaterReleaseCausedByLandSubsidence-CA a :Component, owl:NamedIndividual .

:WaterUse-NM a :Component, :SubtotalTerm, owl:NamedIndividual .

:BrownAndCaldwell%2C1984 a :DataSource, owl:NamedIndividual .

:atmost a owl:NamedIndividual .

:cropGrowh a owl:NamedIndividual .

:weater a owl:NamedIndividual .

:AllocatedDiversion%3AEnvironmentalPurposes-AUS a :Component, owl:NamedIndividual .

:AllocatedDiversion%3AIndividualUsers-AUS a :Component, owl:NamedIndividual .

:AllocatedDiversion%3AInter-region-AUS a :Component, owl:NamedIndividual .

:AllocatedDiversion%3AIrrigation-AUS a :Component, owl:NamedIndividual .

:AllocatedDiversion%3AIrrigationScheme-AUS a :Component, owl:NamedIndividual .

:AllocatedDiversion%3AUrbanSystem-AUS a :Component, owl:NamedIndividual .

:AllocatedDiversions%3ASurfaceWater-AUS a :Component, owl:NamedIndividual .

:AllocatedExtraction%3AEnvironmentalPurposes-AUS a :Component, owl:NamedIndividual .

:AllocatedExtraction%3AGroundwater-AUS a :Component, owl:NamedIndividual .

:AllocatedExtraction%3AIndividualUsers-AUS a :Component, owl:NamedIndividual .

:AllocatedExtraction%3AIrrigation-AUS a :Component, owl:NamedIndividual .

:AllocatedExtraction%3AUrbanSystem-AUS a :Component, owl:NamedIndividual .

:AllocationExtraction%3ASalinityAndWaterTableManagement-AUS a :Component, owl:NamedIndividual .

:AppliedWaterReuse%2FRecycledWater-CA a :Component, owl:NamedIndividual .

:Commercial%3AGolfCourses-NMOSE a :Component, owl:NamedIndividual .

:Commercial%3AUnmetered-NMOSE a :Component, owl:NamedIndividual .

:Commercial%3AIncompleteMetered-NMOSE a :Component, owl:NamedIndividual .

:Commercial%3AMetered-NMOSE a :Component, owl:NamedIndividual .

:Commercial%3ASchools-NMOSE a :Component, owl:NamedIndividual .

:Delivery%3ADesalinatedWater-AUS a :Component, owl:NamedIndividual .

:Delivery%3AInter-region-AUS a :Component, owl:NamedIndividual .

:Delivery%3AInter-regionAgreement-AUS a :Component, owl:NamedIndividual .

:Delivery%3AIrrigationScheme-AUS a :Component, owl:NamedIndividual .

:Delivery%3ARecycledWater-AUS a :Component, owl:NamedIndividual .

:Delivery%3AUrbanUsers-AUS a :Component, owl:NamedIndividual .

:Discharge%3ALandscape-AUS a :Component, owl:NamedIndividual .

:Discharge%3ASea-AUS a :Component, owl:NamedIndividual .

:Discharge%3ASurfaceWater-AUS a :Component, owl:NamedIndividual .

:Discharge%3AUrbanSupply-AUS a :Component, owl:NamedIndividual .

:Discharge%3AUrbanSupplySystem-AUS a :Component, owl:NamedIndividual .

:Discharge%3AUser-AUS a :Component, owl:NamedIndividual .

:Discharge%3AWastewater-AUS a :Component, owl:NamedIndividual .

:Diversions%3AStatutoryRights-AUS a :Component, owl:NamedIndividual .

:Extraction%3AStatutoryRights-AUS a :Component, owl:NamedIndividual .

:Industrial%3ACoalbedMethandProduction-WY a :Component, owl:NamedIndividual .

:Industrial%3AMiscellaneous-WY a :Component, owl:NamedIndividual .

:Industrial%3ANaturalGas-WY a :Component, owl:NamedIndividual .

:Industrial%3AOilAndGas-WY a :Component, owl:NamedIndividual .

:Inter-regionInflow%3AGroundwater-AUS a :Component, owl:NamedIndividual .

:Inter-regionInflow%3ASurfaceWater-AUS a :Component, owl:NamedIndividual .

:Inter-regionOutflow%3AGroundwater-AUS a :Component, owl:NamedIndividual .

:IrrigationWaterSupplyLimitedConsumptiveUse%28Depletions%29-WY a :Component, owl:NamedIndividual .

:Leakage%3AFarmDams-AUS a :Component, owl:NamedIndividual .

:Leakage%3AGroundwater-AUS a :Component, owl:NamedIndividual .

:Leakage%3ALandscape-AUS a :Component, owl:NamedIndividual .

:Leakage%3AUrbanSystem-AUS a :Component, owl:NamedIndividual .

:Livestock%3AMetered-NMOSE a :Component, owl:NamedIndividual .

:Livestock%3AUnmetered-NMOSE a :Component, owl:NamedIndividual .

:ManagedAquiferRecharge%3AIndividualUser-AUS a :Component, owl:NamedIndividual .

:ManagedAquiferRecharge%3AUrban-AUS a :Component, owl:NamedIndividual .

:Mining%3AReported-NMOSE a :Component, owl:NamedIndividual .

:Mining%3AUnreported-NMOSE a :Component, owl:NamedIndividual .

:MonthlyConsumptiveUseCoefficient%28k%29 a :Parameter, owl:NamedIndividual .

:NMOSE%E2%80%99sWaterUseAndConservationBureau%28WUCB%29Survey a :DataSource, owl:NamedIndividual .

:Non-AllocatedDiversion%3ASurfaceWater-AUS a :Component, owl:NamedIndividual .

:Non-AllocatedExtraction%3AGroundwater-AUS a :Component, owl:NamedIndividual .

:Non-AllocatedExtraction%3AIndividualUsers-AUS a :Component, owl:NamedIndividual .

:Non-AllocatedExtraction%3AIrrigation-AUS a :Component, owl:NamedIndividual .

:Non-AllocatedExtraction%3AUrbanSystem-AUS a :Component, owl:NamedIndividual .

:Non-allocatedDiversion%3AEnvironmentalPurposes-AUS a :Component, owl:NamedIndividual .

:Non-allocatedDiversion%3AIndividualUsers-AUS a :Component, owl:NamedIndividual .

:Non-allocatedDiversion%3AUrbanSystem-AUS a :Component, owl:NamedIndividual .

:PointReturn%3AIrrigation-AUS a :Component, owl:NamedIndividual .

:Power%3AReported-NMOSE a :Component, owl:NamedIndividual .

:Power%3AUnreported-NMOSE a :Component, owl:NamedIndividual .

:PublicWaterSupply%3AMetered-NMOSE a :Component, owl:NamedIndividual .

:PublicWaterSupply%3AUnmetered-NMOSE a :Component, owl:NamedIndividual .

:Recharge%3AGroundwater-AUS a :Component, owl:NamedIndividual .

:Recharge%3ALandscape-AUS a :Component, owl:NamedIndividual .

:Recharge%3ASurfaceWater-AUS a :Component, owl:NamedIndividual .

:RecycledWaterDelivery%3AUrbanUsers-AUS a :Component, owl:NamedIndividual .

:ReturnFlow%3AEnvironmentalPurposes-AUS a :Component, owl:NamedIndividual .

:RiparianRelease%3AUrbanSupply-AUS a :Component, owl:NamedIndividual .

:SeasonalConsumptiveUseCoefficients%28K%29 a :Parameter, owl:NamedIndividual .

:SupplySystemDelivery%3AInter-Region-AUS a :Component, owl:NamedIndividual .

:SupplySystemDelivery%3AUrbanUsers-AUS a :Component, owl:NamedIndividual .

:SupplySystemDischarge%3AReservoirs-AUS a :Component, owl:NamedIndividual .

:SupplySystemTransfer%3AInter-region-AUS a :Component, owl:NamedIndividual .

:Transfer%3AInter-region-AUS a :Component, owl:NamedIndividual .

:USCensusBureau%22CityAndTown%28IncorporatedPlacesAndMinorCivilDivisions%29%22DataSet
  a :DataSource, owl:NamedIndividual .

:WastewaterDischarge%3ALandscape-AUS a :Component, owl:NamedIndividual .

:WyomingDepartmentOfEnvironmentalQuality%28WYDEQ%29 a :DataSource, owl:NamedIndividual .

<http://purl.org/iow/WaterBudgetingFramework/California_State_Water_Resources_Control_Board_(SWRCB)_Urban_Water_Supply_Statistics>
  a :DataSource .

:CaliforniaStateWaterResourcesControlBoardUrbanWaterSupplyStatistics a :DataSource,
    owl:Thing .

:AUS a :Jurisdiction, owl:NamedIndividual .

:AUSBureauOfMeteorology a :DataSource, owl:NamedIndividual .

:Adelaide a :Basin, owl:NamedIndividual .

:Burdekin a :Basin, owl:NamedIndividual .

:Canberra a :Basin, owl:NamedIndividual .

:Daly a :Basin, owl:NamedIndividual .

:Fitzroy a :Basin, owl:NamedIndividual .

:Melbourne a :Basin, owl:NamedIndividual .

:MurrayDarling a :Basin, owl:NamedIndividual .

:Ord a :Basin, owl:NamedIndividual .

:Perth a :Basin, owl:NamedIndividual .

:SouthEastQueensland a :Basin, owl:NamedIndividual .

:Sydney a :Basin, owl:NamedIndividual .

:AUSDepartmentOfEnvironmentAndNaturalResources a :DataSource, owl:NamedIndividual .

:AUSDepartmentOfIndustry a :DataSource, owl:NamedIndividual .

:AWRA-LModel a :DataSource, owl:NamedIndividual .

:AWRA-RModel a :DataSource, owl:NamedIndividual .

:AcreageByCropType a :Parameter, owl:NamedIndividual .

:AgriculturalAppliedWater-CA a :Component, owl:NamedIndividual .

:CAAgriculturalWaterManagementPlans a :DataSource, owl:NamedIndividual .

:CALocalAgencyWaterDeliveryRecords a :DataSource, owl:NamedIndividual .

:CAPreviousReports a :DataSource, owl:NamedIndividual .

:Cal-SIMETAWUnitValues a :DataSource, owl:NamedIndividual .

:ExistingCaliforniaWaterPlan a :DataSource, owl:NamedIndividual .

:On-farmWaterUseData a :DataSource, owl:NamedIndividual .

:UniversityOfCaliforniaCooperativeExtensionFarmAdvisors a :DataSource, owl:NamedIndividual .

:CaliforniaCentralValleySimulation%28C2VSim%29 a :DataSource, owl:NamedIndividual .

:CentralValleyHydrologicModel%28CVHM%29 a :EstimationMethod, owl:NamedIndividual .

:Cal-SIMETAWModel a :EstimationMethod, owl:NamedIndividual .

:CropETApproach a :EstimationMethod, owl:NamedIndividual .

:Water-DutyBasedApproach a :EstimationMethod, owl:NamedIndividual .

:CropETRequirements a :Parameter, owl:NamedIndividual .

:ETOfAppliedWater a :Parameter, owl:NamedIndividual .

:IrrigationEfficiency a :Parameter, owl:NamedIndividual .

:IrrigationRecharge a :Parameter, owl:NamedIndividual .

:PrecipitationVolumeForAgriculturalArea a :Parameter, owl:NamedIndividual .

:RunoffVolume a :Parameter, owl:NamedIndividual .

:WaterDutyRateByCrop a :Parameter, owl:NamedIndividual .

:ApparentLosses a :Parameter, owl:NamedIndividual .

:CADWRDemographicData a :DataSource, owl:NamedIndividual .

:CADWRIrrigationMethodsSurvey a :DataSource, owl:NamedIndividual .

:CADWRLandUseViewer a :DataSource, owl:NamedIndividual .

:CADWRSGMADataViewer a :DataSource, owl:NamedIndividual .

:CALSIM2 a :DataSource, owl:NamedIndividual .

:CAUrbanWaterManagementPlans a :DataSource, owl:NamedIndividual .

:CaliforniaAgriculturalLandAndWaterUseEstimates a :DataSource, owl:NamedIndividual .

:CaliforniaDepartmentOfFinance a :DataSource, owl:NamedIndividual .

:CaliforniaPesticideInformationPortal a :DataSource, owl:NamedIndividual .

:CaliforniaWaterPlanPortfolio a :DataSource, owl:NamedIndividual .

:DWRLandUseSurveys a :DataSource, owl:NamedIndividual .

:SWRCBWaterConservationPortal a :DataSource, owl:NamedIndividual .

:USDACropScape a :DataSource, owl:NamedIndividual .

:USDANaturalResourcesConservationServiceGeospatialWebSoilSurvey a :DataSource, owl:NamedIndividual .

:CAIntegratedWaterFlowModel%28IWFM%29 a :DataSource, owl:NamedIndividual .

:CAIntegratedWaterFlowModel%28IWFM%29DemandCalculator a :DataSource, owl:NamedIndividual .

:CaliforniaStateGroundwaterElevationMonitoring%28CASGEM%29 a :DataSource, owl:NamedIndividual .

:MODFLOW-OWHM%3AOneWaterHydrologicFlowModel a :DataSource, :EstimationMethod, owl:NamedIndividual .

:NationalLandCoverDataBase%28NLCD%29 a :DataSource, owl:NamedIndividual .

:USDACountyAgCommissioner%27sDataListing a :DataSource, owl:NamedIndividual .

:VegetationConditionExplorer%28VegScape%29 a :DataSource, owl:NamedIndividual .

:WaterUseClassificationOfLandscapeSpecies%28WUCOLS%29 a :DataSource, owl:NamedIndividual .

:AquiferAttribution a :Parameter, owl:NamedIndividual .

:AUSDepartmentOfEnvironment%2CLand%2CWaterAndPlanning a :DataSource, owl:NamedIndividual .

:AquiferThickness a :Parameter, owl:NamedIndividual .

:PortPhillipCatchmentManagementAuthority a :DataSource, owl:NamedIndividual .

:AssumedDiversionRate a :Parameter, owl:NamedIndividual .

:AustralianBureauOfStatisticsSurveys a :DataSource, owl:NamedIndividual .

:WesternMountLoftyRangesPrescribedWaterResourcesAreaWaterAllocationPlan a :DataSource,
    owl:NamedIndividual .

:BaseflowSeparationTechniques a :EstimationMethod, owl:NamedIndividual .

:BillingMeters a :DataSource, owl:NamedIndividual .

:BoreLocation a :Parameter, owl:NamedIndividual .

:BudgetZoneArea a :Parameter, owl:NamedIndividual .

:CACountyAgriculturalCommissionerCropReports a :DataSource, owl:NamedIndividual .

:CADWRExtensometer a :DataSource, owl:NamedIndividual .

:CALSIM3 a :DataSource, owl:NamedIndividual .

:CARecycledWaterDataFromIndustrialUsers a :DataSource, owl:NamedIndividual .

:CAValidatedWaterLossReporting a :DataSource, owl:NamedIndividual .

:CAWastewaterDataAndDispositionOfTheWater a :DataSource, owl:NamedIndividual .

:CSIROWavesModel a :EstimationMethod, owl:NamedIndividual .

:CaliforniaNevadaRiverForecastCenter a :DataSource, owl:NamedIndividual .

:CaliforniaWaterPlanUpdateData a :DataSource, owl:NamedIndividual .

:CaliforniaWaterPlanWaterPortfolioManagedWetlandsWaterUseData a :DataSource, owl:NamedIndividual .

:ChangeInGroundwaterLevel a :EstimationMethod, owl:NamedIndividual .

:GroundwaterElevation a :Parameter, owl:NamedIndividual .

:SpecificYield a :Parameter, owl:NamedIndividual .

:WaterStorageProduct a :EstimationMethod, owl:NamedIndividual .

:CADWRBulletin118%3AGroundwaterReport a :DataSource, owl:NamedIndividual .

:CaliforniaDataExchangeCenter%28CDEC%29 a :DataSource, owl:NamedIndividual .

:DWRWaterDataLibrary%3ASurfaceWaterAndGroundwaterData a :DataSource, owl:NamedIndividual .

:GravityRecoveryAndClimateExperiment%28GRACE%29 a :DataSource, owl:NamedIndividual .

:MassBalance a :EstimationMethod, owl:NamedIndividual .

:USGSCaliforniaWaterScienceCenter-GroundwaterModeling a :EstimationMethod, owl:NamedIndividual .

:ChangeInLakeStorage a :Parameter, owl:NamedIndividual .

:WaterBalanceForUnsaturatedZoneStorage a :EstimationMethod, owl:NamedIndividual .

:WaterUseModels a :EstimationMethod, owl:NamedIndividual .

:ChangeInPondedWaterStorage a :Parameter, owl:NamedIndividual .

:ChangeInRootZoneSoilMoisture a :Parameter, owl:NamedIndividual .

:ChangeInSoilMoisture a :Parameter, owl:NamedIndividual .

:ChangeInUnsaturatedZoneStorage a :Parameter, owl:NamedIndividual .

:HYDRODatabase a :DataSource, owl:NamedIndividual .

:WaterLevel a :Parameter, owl:NamedIndividual .

:USBRCentralValleyProjectRefugeWaterDeliveryData a :DataSource, owl:NamedIndividual .

:USGSSurface-WaterDataForCalifornia a :DataSource, owl:NamedIndividual .

:CenterForHydrometeorologyAndRemoteSensingDataPortal%28CHRS%29 a :DataSource, owl:NamedIndividual .

:LakeInflowFromStreams-CA a :Component, owl:NamedIndividual .

:LakeOutflowToStreams-CA a :Component, owl:NamedIndividual .

:CityWestWaterAnnualReport a :DataSource, owl:NamedIndividual .

:ConstantPercentage a :EstimationMethod, owl:NamedIndividual .

:ConstantSeepagePercentage a :EstimationMethod, owl:NamedIndividual .

:NOAANationalCentersForEnvironmentalInformation-ClimateDataOnline a :DataSource, owl:NamedIndividual .

:NOAANationalCentersForEnvironmentalInformation-ClimatologicalDataPublications a :DataSource,
    owl:NamedIndividual .

:NWSCLIMATEPREDICTIONCENTEREVAPORATION a :DataSource, owl:NamedIndividual .

:CADWRBulletin132%3AManagementOfTheCaliforniaStateWaterProject a :DataSource, owl:NamedIndividual .

:CaliforniaIrrigationManagementInformationSystem%28CIMIS%29 a :DataSource, owl:NamedIndividual .

:DWRBulletin73%3AEvaporationFromWaterSurfaceInCalifornia%281979%29 a :DataSource,
    owl:NamedIndividual .

:Evapotranspiration%28ET%29Rates a :EstimationMethod, owl:NamedIndividual .

:s.71WaterResourceReport a :DataSource, owl:NamedIndividual .

:EstimateConveyanceSeepageRateBasedOnCanalCharacteristics a :EstimationMethod, owl:NamedIndividual .

:CropCoefficientApproach a :EstimationMethod, owl:NamedIndividual .

:CAIrrigationTrainingAndResearchCenter%28ITRC%29EvapotranspirationData a :DataSource,
    owl:NamedIndividual .

:FAO56Chapter6SingleCropCoefficients%28Kc%29 a :DataSource, owl:NamedIndividual .

:SpatialCaliforniaIrrigationManagementInformationSystem%28CIMIS%29 a :DataSource,
    owl:NamedIndividual .

:ReferenceCropET%28ETo%29 a :Parameter, owl:NamedIndividual .

:CulturalPractices a :Parameter, owl:NamedIndividual .

:DataFromPrivateWetlandsOrDuckClubs a :DataSource, owl:NamedIndividual .

:USFishAndWildlifeServices a :DataSource, owl:NamedIndividual .

:CaliforniaDepartmentOfFishAndWildlife%28CDFW%29 a :DataSource, owl:NamedIndividual .

:CumulativeWaterMeter a :DataSource, owl:NamedIndividual .

:CustomerMeters a :DataSource, owl:NamedIndividual .

:SAWaterGISDatabase a :DataSource, owl:NamedIndividual .

:DWRGuideToEstimatingIrrigationWaterNeedsOfLandscapePlantingsInCalifornia1 a :DataSource,
    owl:NamedIndividual .

:DWRPublicWaterSupplyStatisticsData-Historical a :DataSource, owl:NamedIndividual .

:DailyMaxAndMinAirTemperature a :Parameter, owl:NamedIndividual .

:DailyPrecipitation a :Parameter, owl:NamedIndividual .

:DailyShort-WaveSolarRadiation a :Parameter, owl:NamedIndividual .

:DailyWaterBalanceApproach a :EstimationMethod, owl:NamedIndividual .

:DepartmentOfWaterAndEnvironmentalRegulation a :DataSource, owl:NamedIndividual .

:DrainageAreaOfSiteOfInterest a :Parameter, owl:NamedIndividual .

:DrainageAreaRatioMethod a :EstimationMethod, owl:NamedIndividual .

:DrainageAreaOfStreamflowGagingStation%28Ax%29 a :Parameter, owl:NamedIndividual .

:MeasureStreamflow%28Xij%29 a :Parameter, owl:NamedIndividual .

:EntitlementVolume a :DataSource, owl:NamedIndividual .

:EstimateAppliedWaterReuseAndRecycledWaterVolumes a :EstimationMethod, owl:NamedIndividual .

:EstimatedNon-revenueWaterVolumes a :DataSource, owl:NamedIndividual .

:EstimationOfAbstraction a :EstimationMethod, owl:NamedIndividual .

:Morton%27sShallowLakeFormulation a :EstimationMethod, owl:NamedIndividual .

:EvaporationPanMethod a :EstimationMethod, owl:NamedIndividual .

:MeasuredPanEvaporationRate a :Parameter, owl:NamedIndividual .

:PanCoefficient a :Parameter, owl:NamedIndividual .

:SurfaceAreaOfWaterBody a :Parameter, owl:NamedIndividual .

:METRIC-EarthEngineEvapotranspirationFlux a :DataSource, owl:NamedIndividual .

:USGSBasinCharacterizationModel a :DataSource, owl:NamedIndividual .

:CADWRBulletin113%3ACropWaterUse a :DataSource, owl:NamedIndividual .

:MOD16%3AMODISGlobalEvapotranspirationProject a :DataSource, owl:NamedIndividual .

:NOAAOfficeOfSatelliteAndProductOperationsALEXI%3AAtmosphere-LandExchangeInverseModel
  a :DataSource, owl:NamedIndividual .

:NorthAmericanLandDataAssimilationSystem%28NLDAS-2%29 a :DataSource, owl:NamedIndividual .

:OperationalSimplifiedSurfaceEnergyBalance%28SSEBop%29 a :DataSource, owl:NamedIndividual .

:TOPS-SIMS%3ASatelliteIrrigationManagementSupport a :DataSource, owl:NamedIndividual .

:FloodplainModule a :EstimationMethod, owl:NamedIndividual .

:FlowData a :Parameter, owl:NamedIndividual .

:FlowNetAnalysis a :EstimationMethod, owl:NamedIndividual .

:EffectiveThicknessOfTheAquifer%28b%29 a :Parameter, owl:NamedIndividual .

:FlowThroughAVerticalPlaneThatExtendsBeneathTheShorelineOfASurfaceWaterBody%28Q%29
  a :Parameter, owl:NamedIndividual .

:HorizonalHydraulicConductivityOfTheAquiferAtTheBoundary%28K%29 a :Parameter, owl:NamedIndividual .

:NumberOfEquipotentialHeadDropsOverTheAreaOfInterest%28n%29 a :Parameter, owl:NamedIndividual .

:NumberOfStreamtubesAcrossAFlowNet%28M%29 a :Parameter, owl:NamedIndividual .

:TotalHeadDropAcrossTheAreaOfInterest%28H%29 a :Parameter, owl:NamedIndividual .

:GISGroundwaterModelling a owl:NamedIndividual .

:PortPhillipCatchmentManagementAuthorityGroundwaterModel a :EstimationMethod, owl:NamedIndividual .

:GroundwaterLevel a :Parameter, owl:NamedIndividual .

:HydraulicConductivity a :Parameter, owl:NamedIndividual .

:Darcy%27sLaw a :EstimationMethod, owl:NamedIndividual .

:GippslandWaterAnnualReport a :DataSource, owl:NamedIndividual .

:Peel-HarveyRegionalAquiferModelingSystem%28PHRAMS%29 a :EstimationMethod, owl:NamedIndividual .

:PerthRegionalAquiferModelingSystems%28PRAMS%29 a :EstimationMethod, owl:NamedIndividual .

:LandUseAndAppliedWaterEstimationMethod a :EstimationMethod, owl:NamedIndividual .

:LocalAgencyRecords a :DataSource, owl:NamedIndividual .

:CaliforniaDepartmentOfWaterResources%28DWR%29UrbanWaterSupplyStatistics a owl:NamedIndividual .

:CaliforniaStateWaterResourcesControlBoard%28SWRCB%29UrbanWaterSupplyStatistics a
    :DataSource, owl:NamedIndividual .

:GroundwaterExtractionUnderStatutoryRightsEstimationMethod a :EstimationMethod, owl:NamedIndividual .

:GroundwaterModelling a :EstimationMethod, owl:NamedIndividual .

:HabitatAcreage a :Parameter, owl:NamedIndividual .

:ExistingWaterRightInformationFromStateWaterResourcesControlBoard%28SWRCB%29 a :DataSource,
    owl:NamedIndividual .

:ManagedWetlandAppliedWater-CA a :Component, owl:NamedIndividual .

:OperationalSpill a :Parameter, owl:NamedIndividual .

:UrbanAppliedWater-CA a :Component, owl:NamedIndividual .

:IndividualUserLicenses a :DataSource, owl:NamedIndividual .

:KimberelyAgriculturalInvestment%3AGoomingFarmlands a :DataSource, owl:NamedIndividual .

:OrdIrrigationCooperative%3APacksaddleAndIvanhoePlains a :DataSource, owl:NamedIndividual .

:WaterCorporation%3AM1Channel a :DataSource, owl:NamedIndividual .

:IndustrialWaterUse a :Parameter, owl:NamedIndividual .

:WaterUseSurveys a :DataSource, owl:NamedIndividual .

:InflowFromContributingOrTributaryStreams a :Parameter, owl:NamedIndividual .

:InflowToWaterTreatmentPlants a :DataSource, owl:NamedIndividual .

:GeographicInformationSystem%28GIS%29 a :EstimationMethod, owl:NamedIndividual .

:MassTransferEquations a :EstimationMethod, owl:NamedIndividual .

:MassTransferCoefficient a :Parameter, owl:NamedIndividual .

:SaturationVaporPressure a :Parameter, owl:NamedIndividual .

:WindFunction a :Parameter, owl:NamedIndividual .

:BottomElevationOfTheLakebedSediments%28HlakebedBottom%29 a :Parameter, owl:NamedIndividual .

:DistanceBetweenTwoPointsWithKnownHead%28I%29 a :Parameter, owl:NamedIndividual .

:GroundwaterLevel%28Haquifer%29 a :Parameter, owl:NamedIndividual .

:SurfaceAreaOfLake%28Al%29 a :Parameter, owl:NamedIndividual .

:VerticalHydraulicConductivityOfTheSurroundingAquifer%28Kv%29 a :Parameter, owl:NamedIndividual .

:WaterLevelInLake%28Hlake%29 a :Parameter, owl:NamedIndividual .

:WettedPerimeterOfLakeMultipliedByTheAverageSaturatedThicknessOfAquiferAroundTheLake%28Awpl%29
  a :Parameter, owl:NamedIndividual .

:USGSPublications a :DataSource, owl:NamedIndividual .

:MassCurve a :EstimationMethod, owl:NamedIndividual .

:ReservoirOperationRuleCurve a :EstimationMethod, owl:NamedIndividual .

:ConsumptiveUseOfPrecipitation%28EP%29 a :Parameter, owl:NamedIndividual .

:LandscapeIrrigation a :Parameter, owl:NamedIndividual .

:LandscapeModelledRunoff a :EstimationMethod, owl:NamedIndividual .

:LyneAndHollickFilter a :EstimationMethod, owl:NamedIndividual .

:MIKE11 a :EstimationMethod, owl:NamedIndividual .

:MeteredWaterData a :EstimationMethod, :Parameter, owl:NamedIndividual .

:USFWSAndCDFWRefugeWaterManagementPlans a :DataSource, owl:NamedIndividual .

:ManagedWetlandsAppliedWaterEstimation a :EstimationMethod, owl:NamedIndividual .

:UnitETOfAppliedWater a :Parameter, owl:NamedIndividual .

:StreamflowAtDownstreamGauge a :Parameter, owl:NamedIndividual .

:StreamflowAtUpstreamGauge a :Parameter, owl:NamedIndividual .

:MelbourneWaterAnnualReport a :DataSource, owl:NamedIndividual .

:SnowyHydro a :DataSource, owl:NamedIndividual .

:SouthEastWaterAnnualReport a :DataSource, owl:NamedIndividual .

:UltrasonicFlowMeters a :DataSource, owl:NamedIndividual .

:YarraValleyWaterAnnualReport a :DataSource, owl:NamedIndividual .

:ModelledRunoff a :EstimationMethod, owl:NamedIndividual .

:MoretonAndLoganBasinResourceOperatingLicenses a :DataSource, owl:NamedIndividual .

:MunicipalWaterUseRecords a owl:NamedIndividual .

:NetworkRealLossesAndApparentLossesModelingSoftware a :EstimationMethod, owl:NamedIndividual .

:NewSouthWalesDepartmentOfWater a :DataSource, owl:NamedIndividual .

:Observation a :EstimationMethod, owl:NamedIndividual .

:OnsiteRe-useMeters a :DataSource, owl:NamedIndividual .

:OtherSupplySystemDecreases-AUS a :Component, owl:NamedIndividual .

:RealLossesEquation a :EstimationMethod, owl:NamedIndividual .

:OtherWastewaterDecreases-AUS a :Component, owl:NamedIndividual .

:StreamGages a :DataSource, owl:NamedIndividual .

:PopulationAndPer-CapitaWaterUse a :EstimationMethod, owl:NamedIndividual .

:CentralValleySpatialDatabase-partOfTheCentralValleyHydrologicModel%5BCVHM%5DProject
  a :DataSource, owl:NamedIndividual .

:SpatialAveragingTechniques a :EstimationMethod, owl:NamedIndividual .

:PropertyAreaEstimationMethodsForSurfaceWaterDiversions a :EstimationMethod, owl:NamedIndividual .

:Rainfall-RunoffMethod a :EstimationMethod, owl:NamedIndividual .

:UnmeteredAuthorisedConsumption a :Parameter, owl:NamedIndividual .

:RechargeAsPercentageOfRainfall a :EstimationMethod, owl:NamedIndividual .

:RechargeCreditBalance a :EstimationMethod, owl:NamedIndividual .

:AUSDepartmentForEnvironmentAndWater%28DEW%29 a :DataSource, owl:NamedIndividual .

:WaterRecyclingSurvey%282015%29 a :DataSource, owl:NamedIndividual .

:ReportFromBowenBrokenAndBurdekinHaughtonWaterSupplySchemes a :DataSource, owl:NamedIndividual .

:ResourceOperatingLicenseTables a :DataSource, owl:NamedIndividual .

:ReturnFlowEstimationMethod a :EstimationMethod, owl:NamedIndividual .

:RiparianWaterAuthorisations a :Parameter, owl:NamedIndividual .

:RiverAndGroundwaterInteractionModule a :EstimationMethod, owl:NamedIndividual .

:RiverLosses-AUS a :Component, owl:NamedIndividual .

:CaliforniaDepartmentOfTransportation%27sHighwayDesignManual a :DataSource, owl:NamedIndividual .

:RunoffCurveNumberMethod a :EstimationMethod, owl:NamedIndividual .

:U.C.DavisSoilResourceLab a :DataSource, owl:NamedIndividual .

:Precipitation-RunoffModelingSystem%28PRMS%29 a :EstimationMethod, owl:NamedIndividual .

:PublicPolicyInstituteOfCalifornia%28PPIC%29Map a :EstimationMethod, owl:NamedIndividual .

:SAWaterStorageVolumeRelationship a :EstimationMethod, owl:NamedIndividual .

:SWRCBElectronicAnnualReport a :DataSource, owl:NamedIndividual .

:SWRCBMonthlyUrbanWaterProductionReporting a :DataSource, owl:NamedIndividual .

:Seqwater a :DataSource, owl:NamedIndividual .

:SpatialAssessments a :EstimationMethod, owl:NamedIndividual .

:AverageThicknessOfStreambed%28Bstream%29 a :Parameter, owl:NamedIndividual .

:BottomElevationOfStreambedSediments%28HstreambedBottom%29 a :Parameter, owl:NamedIndividual .

:EffectiveAreaOfFlowExchange%28Awps%29 a :Parameter, owl:NamedIndividual .

:HydraulicConductivityOfTheStreambedMaterial%28Ks%29 a :Parameter, owl:NamedIndividual .

:WaterStageInStream%28Hstream%29 a :Parameter, owl:NamedIndividual .

:USGSDR3M a :EstimationMethod, owl:NamedIndividual .

:WaterResourceAssociatesHYSIM a :EstimationMethod, owl:NamedIndividual .

<http://purl.org/iow/WaterBudgetingFramework/UniversityOfWashington%E2%80%99sVariableInfiltrationCapacityModel%28VIC%29.>
  a :EstimationMethod, owl:NamedIndividual .

:Vieux%26Associates%27Vflo a :EstimationMethod, owl:NamedIndividual .

:DescriptiveDataOfTopography%2CSoils%2CAndVegetation a :Parameter, owl:NamedIndividual .

:Cross-sectionalAreaSubjectToBoundaryFlow%28Ab%29 a :Parameter, owl:NamedIndividual .

:DepthOfCrossSection%28b%29 a :Parameter, owl:NamedIndividual .

:HydraulicConductivityOfTheAquiferBoundary%28K%29 a :Parameter, owl:NamedIndividual .

:HydraulicGradientThroughTheCrossSection%28i%29 a :Parameter, owl:NamedIndividual .

:KnownGroundwaterElevationInsideTheBoundary%28hg%29 a :Parameter, owl:NamedIndividual .

:KnownGroundwaterElevationOutsideTheBoundary%28hb%29 a :Parameter, owl:NamedIndividual .

:SubsurfaceFlowAcrossTheBoundary%28Qb%29 a :Parameter, owl:NamedIndividual .

:TransmissivityOfTheAquiferAtTheBoundary%28T%29 a :Parameter, owl:NamedIndividual .

:WidthOfCrossSection%28w%29 a :Parameter, owl:NamedIndividual .

:SurplusIrrigationAssumption a :EstimationMethod, owl:NamedIndividual .

:USGSExtensometer a :DataSource, owl:NamedIndividual .

:VerticalFluxModel a :EstimationMethod, owl:NamedIndividual .

:VirginiaPipelineSchemePumpStation a :DataSource, owl:NamedIndividual .

:WaterAllocationPlans a :EstimationMethod, owl:NamedIndividual .

:WaterCorporationSurveys a :DataSource, owl:NamedIndividual .

:WaterSharingPlanForTheGreaterMetropolitanRegionUnregulatedRiverWaterSources a :DataSource,
    owl:NamedIndividual .

:WaterSharingPlanForTheKangarooRiverWaterSource a owl:NamedIndividual .

:WaterTableFluctuationModelling a :EstimationMethod, owl:NamedIndividual .

:WillungaBasinWaterCompany a :DataSource, owl:NamedIndividual .

:syde a owl:NamedIndividual .

:yara a owl:NamedIndividual .

:WaterIndustryLicensingManagementDatabase%28WILMA%29 a :DataSource, owl:NamedIndividual .

:SupervisoryControlAndDataAcquisitions%28SCADA%29 a :DataSource, owl:NamedIndividual .

:CARecycledWaterDataFromLocal%2FMunicipalWaterSuppliers a :DataSource, owl:NamedIndividual .

:BarossaInfrastructureLimited%28BIL%29AnnualReport a :DataSource, owl:NamedIndividual .

:FiniteElementSubsurfaceFlowSystem%28FEFLOW%29 a :EstimationMethod, owl:NamedIndividual .

:WaterTrackingAndElectronicReportingSystem%28WaTERS%29 a :DataSource, owl:NamedIndividual .

:Losses%3AManagementOfTreatedWater-AUS a :Component, owl:NamedIndividual .

:Losses%3AWastewaterTreatmentSystem-AUS a :Component, owl:NamedIndividual .

:Non-allocatedDiversion%3AUrbanWaterSystemEstimationMethod a :EstimationMethod, owl:NamedIndividual .

:SAWater%27sTotalLicensedDiversionVolumeFromWesternMountLoftyRangesPWRA a :Parameter,
    owl:NamedIndividual .

:RecycledWaterDelivery%3AIrrigation-AUS a :Component, owl:NamedIndividual .

:SupplySystemDelivery%3AIrrigation-AUS a :Component, owl:NamedIndividual .

:SupplySystemDischarge%3ASurfaceWater-AUS a :Component, owl:NamedIndividual .

:WastewaterAndRecycledWaterDischarge%3ASurfaceWater-AUS a :Component, owl:NamedIndividual .

:WastewaterDischarge%3ASurfaceWater-AUS a :Component, owl:NamedIndividual .

rdf:Property rdfs:subPropertyOf owl:topObjectProperty .

rdfs:isDefinedBy rdfs:subPropertyOf rdfs:seeAlso .

skos:definition rdfs:subPropertyOf skos:note .

skos:scopeNote rdfs:subPropertyOf skos:note .

skos:example rdfs:subPropertyOf skos:note .

skos:topConceptOf rdfs:subPropertyOf skos:inScheme .

skos:prefLabel rdfs:subPropertyOf rdfs:label .

skos:altLabel rdfs:subPropertyOf rdfs:label .

skos:hiddenLabel rdfs:subPropertyOf rdfs:label .

skos:changeNote rdfs:subPropertyOf skos:note .

skos:editorialNote rdfs:subPropertyOf skos:note .

skos:historyNote rdfs:subPropertyOf skos:note .

skos:broader rdfs:subPropertyOf rdf:Property, skos:broaderTransitive .

skos:broaderTransitive rdfs:subPropertyOf skos:semanticRelation .

skos:narrower rdfs:subPropertyOf skos:narrowerTransitive .

skos:narrowerTransitive rdfs:subPropertyOf skos:semanticRelation .

skos:related rdfs:subPropertyOf skos:semanticRelation .

skos:mappingRelation rdfs:subPropertyOf skos:semanticRelation .

skos:broadMatch rdfs:subPropertyOf skos:broader, skos:mappingRelation .

skos:narrowMatch rdfs:subPropertyOf skos:mappingRelation, skos:narrower .

skos:relatedMatch rdfs:subPropertyOf skos:mappingRelation, skos:related .

skos:exactMatch rdfs:subPropertyOf skos:closeMatch .

skos:closeMatch rdfs:subPropertyOf skos:mappingRelation .

:flowSink rdfs:subPropertyOf rdf:Property .

:flowSource rdfs:subPropertyOf rdf:Property .

:hasDataSource rdfs:subPropertyOf rdf:Property .

:hasEstimationMethod rdfs:subPropertyOf rdf:Property .

:hasParameter rdfs:subPropertyOf rdf:Property .

:isFlowType rdfs:subPropertyOf rdf:Property .

:isPartialSubComponentOf rdfs:subPropertyOf rdf:Property .

:isSubComponentOf rdfs:subPropertyOf rdf:Property .

:usedBy rdfs:subPropertyOf rdf:Property .

skos:isExactMatch rdfs:subPropertyOf rdf:Property .

:flowProportion rdfs:subPropertyOf owl:topDataProperty .

rdf:Property rdfs:subClassOf rdfs:Resource .

rdfs:Class rdfs:subClassOf rdfs:Resource .

owl:SymmetricProperty rdfs:subClassOf owl:ObjectProperty .

owl:TransitiveProperty rdfs:subClassOf owl:ObjectProperty .

rdfs:Datatype rdfs:subClassOf rdfs:Class .

owl:FunctionalProperty rdfs:subClassOf rdf:Property .

rdfs:ContainerMembershipProperty rdfs:subClassOf rdf:Property .

owl:InverseFunctionalProperty rdfs:subClassOf owl:ObjectProperty .

rdfs:Literal rdfs:subClassOf rdfs:Resource .

rdf:List rdfs:subClassOf rdfs:Resource .

rdf:Statement rdfs:subClassOf rdfs:Resource .

rdf:Alt rdfs:subClassOf rdfs:Container .

rdfs:Container rdfs:subClassOf rdfs:Resource .

rdf:Bag rdfs:subClassOf rdfs:Container .

rdf:Seq rdfs:subClassOf rdfs:Container .

rdf:XMLLiteral rdfs:subClassOf rdfs:Literal .

owl:Ontology rdfs:subClassOf rdfs:Resource .

rdf:HTML rdfs:subClassOf rdfs:Literal .

rdf:langString rdfs:subClassOf rdfs:Literal .

rdf:PlainLiteral rdfs:subClassOf rdfs:Literal .

owl:AllDifferent rdfs:subClassOf rdfs:Resource .

owl:AllDisjointClasses rdfs:subClassOf rdfs:Resource .

owl:AllDisjointProperties rdfs:subClassOf rdfs:Resource .

owl:Annotation rdfs:subClassOf rdfs:Resource .

owl:AnnotationProperty rdfs:subClassOf rdf:Property .

owl:AsymmetricProperty rdfs:subClassOf owl:ObjectProperty .

owl:ObjectProperty rdfs:subClassOf rdf:Property .

owl:Axiom rdfs:subClassOf rdfs:Resource .

owl:Class rdfs:subClassOf rdfs:Class .

owl:DataRange rdfs:subClassOf rdfs:Datatype .

owl:DatatypeProperty rdfs:subClassOf rdf:Property .

owl:DeprecatedClass rdfs:subClassOf rdfs:Class .

owl:DeprecatedProperty rdfs:subClassOf rdf:Property .

owl:IrreflexiveProperty rdfs:subClassOf owl:ObjectProperty .

owl:NamedIndividual rdfs:subClassOf owl:Thing .

owl:NegativePropertyAssertion rdfs:subClassOf rdfs:Resource .

owl:Nothing rdfs:subClassOf owl:Thing .

owl:OntologyProperty rdfs:subClassOf rdf:Property .

owl:ReflexiveProperty rdfs:subClassOf owl:ObjectProperty .

owl:Restriction rdfs:subClassOf owl:Class .

skos:OrderedCollection rdfs:subClassOf skos:Collection .

:Component rdfs:subClassOf :Element .

:flowDomain rdfs:subClassOf :Element .

:Parameter rdfs:subClassOf :Element .

:DataSource rdfs:subClassOf :Element .

:EstimationMethod rdfs:subClassOf :Element .

:flowType rdfs:subClassOf :Element .

:Jurisdiction rdfs:subClassOf :Element .

<http://geoconnex.us/iow/WaterBudgetingFramework/ClosureTerm> rdfs:subClassOf :Component .

:Basin rdfs:subClassOf :Jurisdiction .

:External rdfs:subClassOf :flowDomain .

:SubtotalTerm rdfs:subClassOf :Component .

:Zone rdfs:subClassOf :flowDomain .

rdf:type rdfs:domain rdfs:Resource;
  rdfs:range rdfs:Class .

rdfs:subPropertyOf rdfs:domain rdf:Property;
  rdfs:range rdf:Property .

rdfs:subClassOf rdfs:domain rdfs:Class;
  rdfs:range rdfs:Class .

rdfs:domain rdfs:domain rdf:Property;
  rdfs:range rdfs:Class .

rdfs:range rdfs:domain rdf:Property;
  rdfs:range rdfs:Class .

owl:sameAs rdfs:domain owl:Thing;
  rdfs:range owl:Thing .

owl:equivalentProperty rdfs:domain rdf:Property;
  rdfs:range rdf:Property .

owl:equivalentClass rdfs:domain rdfs:Class;
  rdfs:range rdfs:Class .

owl:intersectionOf rdfs:domain rdfs:Class;
  rdfs:range rdf:List .

owl:someValuesFrom rdfs:domain owl:Restriction;
  rdfs:range rdfs:Class .

owl:allValuesFrom rdfs:domain owl:Restriction;
  rdfs:range rdfs:Class .

owl:inverseOf rdfs:domain owl:ObjectProperty;
  rdfs:range owl:ObjectProperty .

rdfs:member rdfs:domain rdfs:Resource;
  rdfs:range rdfs:Resource .

owl:hasValue rdfs:domain owl:Restriction;
  rdfs:range rdfs:Resource .

rdf:first rdfs:domain rdf:List;
  rdfs:range rdfs:Resource .

owl:onProperty rdfs:domain owl:Restriction;
  rdfs:range rdf:Property .

rdf:rest rdfs:domain rdf:List;
  rdfs:range rdf:List .

rdf:subject rdfs:domain rdf:Statement;
  rdfs:range rdfs:Resource .

rdf:predicate rdfs:domain rdf:Statement;
  rdfs:range rdfs:Resource .

rdf:object rdfs:domain rdf:Statement;
  rdfs:range rdfs:Resource .

rdf:value rdfs:domain rdfs:Resource;
  rdfs:range rdfs:Resource .

rdfs:comment rdfs:domain rdfs:Resource;
  rdfs:range rdfs:Literal .

rdfs:label rdfs:domain rdfs:Resource;
  rdfs:range rdfs:Literal .

rdfs:isDefinedBy rdfs:domain rdfs:Resource;
  rdfs:range rdfs:Resource .

rdfs:seeAlso rdfs:domain rdfs:Resource;
  rdfs:range rdfs:Resource .

owl:differentFrom rdfs:domain owl:Thing;
  rdfs:range owl:Thing .

owl:versionIRI rdfs:domain owl:Ontology;
  rdfs:range owl:Ontology .

owl:imports rdfs:domain owl:Ontology;
  rdfs:range owl:Ontology .

owl:versionInfo rdfs:domain rdfs:Resource;
  rdfs:range rdfs:Resource .

owl:annotatedProperty rdfs:domain rdfs:Resource;
  rdfs:range rdfs:Resource .

owl:annotatedSource rdfs:domain rdfs:Resource;
  rdfs:range rdfs:Resource .

owl:annotatedTarget rdfs:domain rdfs:Resource;
  rdfs:range rdfs:Resource .

owl:assertionProperty rdfs:domain owl:NegativePropertyAssertion;
  rdfs:range rdf:Property .

owl:backwardCompatibleWith rdfs:domain owl:Ontology;
  rdfs:range owl:Ontology .

owl:bottomDataProperty rdfs:domain owl:Thing;
  rdfs:range rdfs:Literal .

owl:bottomObjectProperty rdfs:domain owl:Thing;
  rdfs:range owl:Thing .

owl:cardinality rdfs:domain owl:Restriction;
  rdfs:range xsd:nonNegativeInteger .

owl:complementOf rdfs:domain owl:Class;
  rdfs:range owl:Class .

owl:datatypeComplementOf rdfs:domain rdfs:Datatype;
  rdfs:range rdfs:Datatype .

owl:deprecated rdfs:domain rdfs:Resource;
  rdfs:range rdfs:Resource .

owl:disjointUnionOf rdfs:domain owl:Class;
  rdfs:range rdf:List .

owl:disjointWith rdfs:domain owl:Class;
  rdfs:range owl:Class .

owl:distinctMembers rdfs:domain owl:AllDifferent;
  rdfs:range rdf:List .

owl:hasKey rdfs:domain owl:Class;
  rdfs:range rdf:List .

owl:hasSelf rdfs:domain owl:Restriction;
  rdfs:range rdfs:Resource .

owl:incompatibleWith rdfs:domain owl:Ontology;
  rdfs:range owl:Ontology .

owl:maxCardinality rdfs:domain owl:Restriction;
  rdfs:range xsd:nonNegativeInteger .

owl:maxQualifiedCardinality rdfs:domain owl:Restriction;
  rdfs:range xsd:nonNegativeInteger .

owl:members rdfs:domain rdfs:Resource;
  rdfs:range rdf:List .

owl:minCardinality rdfs:domain owl:Restriction;
  rdfs:range xsd:nonNegativeInteger .

owl:minQualifiedCardinality rdfs:domain owl:Restriction;
  rdfs:range xsd:nonNegativeInteger .

owl:onClass rdfs:domain owl:Restriction;
  rdfs:range owl:Class .

owl:onDataRange rdfs:domain owl:Restriction;
  rdfs:range rdfs:Datatype .

owl:onDatatype rdfs:domain rdfs:Datatype;
  rdfs:range rdfs:Datatype .

owl:oneOf rdfs:domain rdfs:Class;
  rdfs:range rdf:List .

owl:onProperties rdfs:domain owl:Restriction;
  rdfs:range rdf:List .

owl:priorVersion rdfs:domain owl:Ontology;
  rdfs:range owl:Ontology .

owl:propertyChainAxiom rdfs:domain owl:ObjectProperty;
  rdfs:range rdf:List .

owl:propertyDisjointWith rdfs:domain rdf:Property;
  rdfs:range rdf:Property .

owl:qualifiedCardinality rdfs:domain owl:Restriction;
  rdfs:range xsd:nonNegativeInteger .

owl:sourceIndividual rdfs:domain owl:NegativePropertyAssertion;
  rdfs:range owl:Thing .

owl:targetIndividual rdfs:domain owl:NegativePropertyAssertion;
  rdfs:range owl:Thing .

owl:targetValue rdfs:domain owl:NegativePropertyAssertion;
  rdfs:range rdfs:Literal .

owl:topDataProperty rdfs:domain owl:Thing;
  rdfs:range rdfs:Literal .

owl:topObjectProperty rdfs:domain owl:Thing;
  rdfs:range owl:Thing .

owl:unionOf rdfs:domain rdfs:Class;
  rdfs:range rdf:List .

owl:withRestrictions rdfs:domain rdfs:Datatype;
  rdfs:range rdf:List .

skos:hasTopConcept rdfs:domain skos:ConceptScheme;
  rdfs:range skos:Concept;
  owl:inverseOf skos:topConceptOf .

skos:topConceptOf rdfs:domain skos:Concept;
  rdfs:range skos:ConceptScheme;
  owl:inverseOf skos:hasTopConcept .

skos:semanticRelation rdfs:domain skos:Concept;
  rdfs:range skos:Concept .

skos:member rdfs:domain skos:Collection;
  rdfs:range _:node1 .

_:node1 a owl:Class .

skos:memberList rdfs:domain skos:OrderedCollection;
  rdfs:range rdf:List .

:flowSink rdfs:domain :Component;
  rdfs:range :flowDomain .

:flowSource rdfs:domain :Component;
  rdfs:range :flowDomain .

:hasDataSource rdfs:domain :Component, :EstimationMethod, :Parameter;
  rdfs:range :DataSource .

:hasEstimationMethod rdfs:domain :Component;
  rdfs:range :EstimationMethod .

:hasParameter rdfs:domain :EstimationMethod;
  rdfs:range :Parameter .

:isFlowType rdfs:domain :Component;
  rdfs:range :flowType .

:isSubComponentOf rdfs:domain :Component;
  rdfs:range :Component .

:usedBy rdfs:domain :Component, :DataSource, :EstimationMethod, :Parameter;
  rdfs:range :Jurisdiction .

:flowProportion rdfs:domain :Component;
  rdfs:range xsd:positiveInteger .

skos:inScheme rdfs:range skos:ConceptScheme .

:AreaOutflows owl:sameAs :BasinOutflow-UT .

:BasinInflow-UT owl:sameAs :RiverInflow-UT .

:GroundwaterExport-CA owl:sameAs :LakeGainFromGroundwater-CA .

:GroundwaterDischarge-AUS owl:sameAs :Discharge%3AGroundwater-AUS .

:GroundwaterET-NM owl:sameAs :RiparianConsumption-NM .

:GroundwaterUse-UT owl:sameAs :PumpedGroundwater-UT .

:Delivery%3AInter-region-AUS owl:sameAs :Delivery%3AInter-regionAgreement-AUS .

:Recharge%3AGroundwater-AUS owl:sameAs :Recharge%3ASurfaceWater-AUS .

skos:broader owl:inverseOf skos:narrower .

skos:broaderTransitive owl:inverseOf skos:narrowerTransitive .

skos:narrower owl:inverseOf skos:broader .

skos:narrowerTransitive owl:inverseOf skos:broaderTransitive .

skos:broadMatch owl:inverseOf skos:narrowMatch .

skos:narrowMatch owl:inverseOf skos:broadMatch .

rdf:type rdfs:comment "The subject is an instance of a class." .

rdf:Property rdfs:comment "The class of RDF properties." .

rdfs:Class rdfs:comment "The class of classes." .

rdfs:Resource rdfs:comment "The class resource, everything." .

rdfs:subPropertyOf rdfs:comment "The subject is a subproperty of a property." .

rdfs:subClassOf rdfs:comment "The subject is a subclass of a class." .

rdfs:domain rdfs:comment "A domain of the subject property." .

rdfs:range rdfs:comment "A range of the subject property." .

owl:sameAs rdfs:comment "The property that determines that two given individuals are equal." .

owl:SymmetricProperty rdfs:comment "The class of symmetric properties." .

owl:TransitiveProperty rdfs:comment "The class of transitive properties." .

owl:equivalentProperty rdfs:comment "The property that determines that two given properties are equivalent." .

owl:equivalentClass rdfs:comment "The property that determines that two given classes are equivalent, and that is used to specify datatype definitions." .

rdfs:Datatype rdfs:comment "The class of RDF datatypes." .

owl:intersectionOf rdfs:comment "The property that determines the collection of classes or data ranges that build an intersection." .

owl:FunctionalProperty rdfs:comment "The class of functional properties." .

rdfs:ContainerMembershipProperty rdfs:comment """The class of container membership properties, rdf:_1, rdf:_2, ...,
                    all of which are sub-properties of 'member'.""" .

owl:someValuesFrom rdfs:comment "The property that determines the class that an existential property restriction refers to." .

owl:allValuesFrom rdfs:comment "The property that determines the class that a universal property restriction refers to." .

owl:inverseOf rdfs:comment "The property that determines that two given properties are inverse." .

rdfs:member rdfs:comment "A member of the subject resource." .

owl:hasValue rdfs:comment "The property that determines the individual that a has-value restriction refers to." .

rdf:first rdfs:comment "The first item in the subject RDF list." .

owl:onProperty rdfs:comment "The property that determines the property that a property restriction refers to." .

rdf:rest rdfs:comment "The rest of the subject RDF list after the first item." .

owl:InverseFunctionalProperty rdfs:comment "The class of inverse-functional properties." .

rdfs:Literal rdfs:comment "The class of literal values, eg. textual strings and integers." .

rdf:nil rdfs:comment "The empty list, with no items in it. If the rest of a list is nil then the list has no more items in it." .

rdf:subject rdfs:comment "The subject of the subject RDF statement." .

rdf:predicate rdfs:comment "The predicate of the subject RDF statement." .

rdf:object rdfs:comment "The object of the subject RDF statement." .

rdf:value rdfs:comment "Idiomatic property used for structured values." .

rdf:List rdfs:comment "The class of RDF Lists." .

rdf:Statement rdfs:comment "The class of RDF statements." .

rdfs:comment rdfs:comment "A description of the subject resource." .

rdfs:label rdfs:comment "A human-readable name for the subject." .

rdf:Alt rdfs:comment "The class of containers of alternatives." .

rdfs:Container rdfs:comment "The class of RDF containers." .

rdf:Bag rdfs:comment "The class of unordered containers." .

rdf:Seq rdfs:comment "The class of ordered containers." .

rdfs:isDefinedBy rdfs:comment "The defininition of the subject resource." .

rdfs:seeAlso rdfs:comment "Further information about the subject resource." .

rdf:XMLLiteral rdfs:comment "The datatype of XML literal values." .

owl:differentFrom rdfs:comment "The property that determines that two given individuals are different." .

owl:Ontology rdfs:comment "The class of ontologies." .

rdf:HTML rdfs:comment "The datatype of RDF literals storing fragments of HTML content" .

rdf:langString rdfs:comment "The datatype of language-tagged string values" .

rdf:PlainLiteral rdfs:comment "The class of plain (i.e. untyped) literal values, as used in RIF and OWL 2" .

<http://www.w3.org/2002/07/owl> rdfs:comment """
  This ontology partially describes the built-in classes and
  properties that together form the basis of the RDF/XML syntax of OWL 2.
  The content of this ontology is based on Tables 6.1 and 6.2
  in Section 6.4 of the OWL 2 RDF-Based Semantics specification,
  available at http://www.w3.org/TR/owl2-rdf-based-semantics/.
  Please note that those tables do not include the different annotations
  (labels, comments and rdfs:isDefinedBy links) used in this file.
  Also note that the descriptions provided in this ontology do not
  provide a complete and correct formal description of either the syntax
  or the semantics of the introduced terms (please see the OWL 2
  recommendations for the complete and normative specifications).
  Furthermore, the information provided by this ontology may be
  misleading if not used with care. This ontology SHOULD NOT be imported
  into OWL ontologies. Importing this file into an OWL 2 DL ontology
  will cause it to become an OWL 2 Full ontology and may have other,
  unexpected, consequences.
   """ .

owl:versionIRI rdfs:comment "The property that identifies the version IRI of an ontology." .

owl:imports rdfs:comment "The property that is used for importing other ontologies into a given ontology." .

owl:versionInfo rdfs:comment "The annotation property that provides version information for an ontology or another OWL construct." .

owl:AllDifferent rdfs:comment "The class of collections of pairwise different individuals." .

owl:AllDisjointClasses rdfs:comment "The class of collections of pairwise disjoint classes." .

owl:AllDisjointProperties rdfs:comment "The class of collections of pairwise disjoint properties." .

owl:Annotation rdfs:comment "The class of annotated annotations for which the RDF serialization consists of an annotated subject, predicate and object." .

owl:AnnotationProperty rdfs:comment "The class of annotation properties." .

owl:AsymmetricProperty rdfs:comment "The class of asymmetric properties." .

owl:ObjectProperty rdfs:comment "The class of object properties." .

owl:Axiom rdfs:comment "The class of annotated axioms for which the RDF serialization consists of an annotated subject, predicate and object." .

owl:Class rdfs:comment "The class of OWL classes." .

owl:DataRange rdfs:comment "The class of OWL data ranges, which are special kinds of datatypes. Note: The use of the IRI owl:DataRange has been deprecated as of OWL 2. The IRI rdfs:Datatype SHOULD be used instead." .

owl:DatatypeProperty rdfs:comment "The class of data properties." .

owl:DeprecatedClass rdfs:comment "The class of deprecated classes." .

owl:DeprecatedProperty rdfs:comment "The class of deprecated properties." .

owl:IrreflexiveProperty rdfs:comment "The class of irreflexive properties." .

owl:NamedIndividual rdfs:comment "The class of named individuals." .

owl:Thing rdfs:comment "The class of OWL individuals." .

owl:NegativePropertyAssertion rdfs:comment "The class of negative property assertions." .

owl:Nothing rdfs:comment "This is the empty class." .

owl:OntologyProperty rdfs:comment "The class of ontology properties." .

owl:ReflexiveProperty rdfs:comment "The class of reflexive properties." .

owl:Restriction rdfs:comment "The class of property restrictions." .

owl:annotatedProperty rdfs:comment "The property that determines the predicate of an annotated axiom or annotated annotation." .

owl:annotatedSource rdfs:comment "The property that determines the subject of an annotated axiom or annotated annotation." .

owl:annotatedTarget rdfs:comment "The property that determines the object of an annotated axiom or annotated annotation." .

owl:assertionProperty rdfs:comment "The property that determines the predicate of a negative property assertion." .

owl:backwardCompatibleWith rdfs:comment "The annotation property that indicates that a given ontology is backward compatible with another ontology." .

owl:bottomDataProperty rdfs:comment "The data property that does not relate any individual to any data value." .

owl:bottomObjectProperty rdfs:comment "The object property that does not relate any two individuals." .

owl:cardinality rdfs:comment "The property that determines the cardinality of an exact cardinality restriction." .

owl:complementOf rdfs:comment "The property that determines that a given class is the complement of another class." .

owl:datatypeComplementOf rdfs:comment "The property that determines that a given data range is the complement of another data range with respect to the data domain." .

owl:deprecated rdfs:comment "The annotation property that indicates that a given entity has been deprecated." .

owl:disjointUnionOf rdfs:comment "The property that determines that a given class is equivalent to the disjoint union of a collection of other classes." .

owl:disjointWith rdfs:comment "The property that determines that two given classes are disjoint." .

owl:distinctMembers rdfs:comment "The property that determines the collection of pairwise different individuals in a owl:AllDifferent axiom." .

owl:hasKey rdfs:comment "The property that determines the collection of properties that jointly build a key." .

owl:hasSelf rdfs:comment "The property that determines the property that a self restriction refers to." .

owl:incompatibleWith rdfs:comment "The annotation property that indicates that a given ontology is incompatible with another ontology." .

owl:maxCardinality rdfs:comment "The property that determines the cardinality of a maximum cardinality restriction." .

owl:maxQualifiedCardinality rdfs:comment "The property that determines the cardinality of a maximum qualified cardinality restriction." .

owl:members rdfs:comment "The property that determines the collection of members in either a owl:AllDifferent, owl:AllDisjointClasses or owl:AllDisjointProperties axiom." .

owl:minCardinality rdfs:comment "The property that determines the cardinality of a minimum cardinality restriction." .

owl:minQualifiedCardinality rdfs:comment "The property that determines the cardinality of a minimum qualified cardinality restriction." .

owl:onClass rdfs:comment "The property that determines the class that a qualified object cardinality restriction refers to." .

owl:onDataRange rdfs:comment "The property that determines the data range that a qualified data cardinality restriction refers to." .

owl:onDatatype rdfs:comment "The property that determines the datatype that a datatype restriction refers to." .

owl:oneOf rdfs:comment "The property that determines the collection of individuals or data values that build an enumeration." .

owl:onProperties rdfs:comment "The property that determines the n-tuple of properties that a property restriction on an n-ary data range refers to." .

owl:priorVersion rdfs:comment "The annotation property that indicates the predecessor ontology of a given ontology." .

owl:propertyChainAxiom rdfs:comment "The property that determines the n-tuple of properties that build a sub property chain of a given property." .

owl:propertyDisjointWith rdfs:comment "The property that determines that two given properties are disjoint." .

owl:qualifiedCardinality rdfs:comment "The property that determines the cardinality of an exact qualified cardinality restriction." .

owl:sourceIndividual rdfs:comment "The property that determines the subject of a negative property assertion." .

owl:targetIndividual rdfs:comment "The property that determines the object of a negative object property assertion." .

owl:targetValue rdfs:comment "The property that determines the value of a negative data property assertion." .

owl:topDataProperty rdfs:comment "The data property that relates every individual to every data value." .

owl:topObjectProperty rdfs:comment "The object property that relates every two individuals." .

owl:unionOf rdfs:comment "The property that determines the collection of classes or data ranges that build a union." .

owl:withRestrictions rdfs:comment "The property that determines the collection of facet-value pairs that define a datatype restriction." .

skos:prefLabel rdfs:comment "A resource has no more than one value of skos:prefLabel per language tag, and no more than one value of skos:prefLabel without language tag."@en,
    "The range of skos:prefLabel is the class of RDF plain literals."@en, """skos:prefLabel, skos:altLabel and skos:hiddenLabel are pairwise
      disjoint properties."""@en .

skos:altLabel rdfs:comment "The range of skos:altLabel is the class of RDF plain literals."@en,
    "skos:prefLabel, skos:altLabel and skos:hiddenLabel are pairwise disjoint properties."@en .

skos:hiddenLabel rdfs:comment "The range of skos:hiddenLabel is the class of RDF plain literals."@en,
    "skos:prefLabel, skos:altLabel and skos:hiddenLabel are pairwise disjoint properties."@en .

skos:broader rdfs:comment "Broader concepts are typically rendered as parents in a concept hierarchy (tree)."@en .

skos:narrower rdfs:comment "Narrower concepts are typically rendered as children in a concept hierarchy (tree)."@en .

skos:related rdfs:comment "skos:related is disjoint with skos:broaderTransitive"@en .

skos:memberList rdfs:comment """For any resource, every item in the list given as the value of the
      skos:memberList property is also a value of the skos:member property."""@en .

skos:mappingRelation rdfs:comment "These concept mapping relations mirror semantic relations, and the data model defined below is similar (with the exception of skos:exactMatch) to the data model defined for semantic relations. A distinct vocabulary is provided for concept mapping relations, to provide a convenient way to differentiate links within a concept scheme from links between concept schemes. However, this pattern of usage is not a formal requirement of the SKOS data model, and relies on informal definitions of best practice."@en .

skos:exactMatch rdfs:comment "skos:exactMatch is disjoint with each of the properties skos:broadMatch and skos:relatedMatch."@en .

rdf:type rdfs:label "type" .

rdf:Property rdfs:label "Property" .

rdfs:Class rdfs:label "Class" .

rdfs:Resource rdfs:label "Resource" .

rdfs:subPropertyOf rdfs:label "subPropertyOf" .

rdfs:subClassOf rdfs:label "subClassOf" .

rdfs:domain rdfs:label "domain" .

rdfs:range rdfs:label "range" .

owl:sameAs rdfs:label "sameAs" .

owl:SymmetricProperty rdfs:label "SymmetricProperty" .

owl:TransitiveProperty rdfs:label "TransitiveProperty" .

owl:equivalentProperty rdfs:label "equivalentProperty" .

owl:equivalentClass rdfs:label "equivalentClass" .

rdfs:Datatype rdfs:label "Datatype" .

owl:intersectionOf rdfs:label "intersectionOf" .

owl:FunctionalProperty rdfs:label "FunctionalProperty" .

rdfs:ContainerMembershipProperty rdfs:label "ContainerMembershipProperty" .

owl:someValuesFrom rdfs:label "someValuesFrom" .

owl:allValuesFrom rdfs:label "allValuesFrom" .

owl:inverseOf rdfs:label "inverseOf" .

rdfs:member rdfs:label "member" .

owl:hasValue rdfs:label "hasValue" .

rdf:first rdfs:label "first" .

owl:onProperty rdfs:label "onProperty" .

rdf:rest rdfs:label "rest" .

owl:InverseFunctionalProperty rdfs:label "InverseFunctionalProperty" .

rdfs:Literal rdfs:label "Literal" .

rdf:nil rdfs:label "nil" .

rdf:subject rdfs:label "subject" .

rdf:predicate rdfs:label "predicate" .

rdf:object rdfs:label "object" .

rdf:value rdfs:label "value" .

rdf:List rdfs:label "List" .

rdf:Statement rdfs:label "Statement" .

rdfs:comment rdfs:label "comment" .

rdfs:label rdfs:label "label" .

rdf:Alt rdfs:label "Alt" .

rdfs:Container rdfs:label "Container" .

rdf:Bag rdfs:label "Bag" .

rdf:Seq rdfs:label "Seq" .

rdfs:isDefinedBy rdfs:label "isDefinedBy" .

rdfs:seeAlso rdfs:label "seeAlso" .

rdf:XMLLiteral rdfs:label "XMLLiteral" .

owl:differentFrom rdfs:label "differentFrom" .

owl:Ontology rdfs:label "Ontology" .

rdf:HTML rdfs:label "HTML" .

rdf:langString rdfs:label "langString" .

rdf:PlainLiteral rdfs:label "PlainLiteral" .

owl:versionIRI rdfs:label "versionIRI" .

owl:imports rdfs:label "imports" .

owl:versionInfo rdfs:label "versionInfo" .

owl:AllDifferent rdfs:label "AllDifferent" .

owl:AllDisjointClasses rdfs:label "AllDisjointClasses" .

owl:AllDisjointProperties rdfs:label "AllDisjointProperties" .

owl:Annotation rdfs:label "Annotation" .

owl:AnnotationProperty rdfs:label "AnnotationProperty" .

owl:AsymmetricProperty rdfs:label "AsymmetricProperty" .

owl:ObjectProperty rdfs:label "ObjectProperty" .

owl:Axiom rdfs:label "Axiom" .

owl:Class rdfs:label "Class" .

owl:DataRange rdfs:label "DataRange" .

owl:DatatypeProperty rdfs:label "DatatypeProperty" .

owl:DeprecatedClass rdfs:label "DeprecatedClass" .

owl:DeprecatedProperty rdfs:label "DeprecatedProperty" .

owl:IrreflexiveProperty rdfs:label "IrreflexiveProperty" .

owl:NamedIndividual rdfs:label "NamedIndividual" .

owl:Thing rdfs:label "Thing" .

owl:NegativePropertyAssertion rdfs:label "NegativePropertyAssertion" .

owl:Nothing rdfs:label "Nothing" .

owl:OntologyProperty rdfs:label "OntologyProperty" .

owl:ReflexiveProperty rdfs:label "ReflexiveProperty" .

owl:Restriction rdfs:label "Restriction" .

owl:annotatedProperty rdfs:label "annotatedProperty" .

owl:annotatedSource rdfs:label "annotatedSource" .

owl:annotatedTarget rdfs:label "annotatedTarget" .

owl:assertionProperty rdfs:label "assertionProperty" .

owl:backwardCompatibleWith rdfs:label "backwardCompatibleWith" .

owl:bottomDataProperty rdfs:label "bottomDataProperty" .

owl:bottomObjectProperty rdfs:label "bottomObjectProperty" .

owl:cardinality rdfs:label "cardinality" .

owl:complementOf rdfs:label "complementOf" .

owl:datatypeComplementOf rdfs:label "datatypeComplementOf" .

owl:deprecated rdfs:label "deprecated" .

owl:disjointUnionOf rdfs:label "disjointUnionOf" .

owl:disjointWith rdfs:label "disjointWith" .

owl:distinctMembers rdfs:label "distinctMembers" .

owl:hasKey rdfs:label "hasKey" .

owl:hasSelf rdfs:label "hasSelf" .

owl:incompatibleWith rdfs:label "incompatibleWith" .

owl:maxCardinality rdfs:label "maxCardinality" .

owl:maxQualifiedCardinality rdfs:label "maxQualifiedCardinality" .

owl:members rdfs:label "members" .

owl:minCardinality rdfs:label "minCardinality" .

owl:minQualifiedCardinality rdfs:label "minQualifiedCardinality" .

owl:onClass rdfs:label "onClass" .

owl:onDataRange rdfs:label "onDataRange" .

owl:onDatatype rdfs:label "onDatatype" .

owl:oneOf rdfs:label "oneOf" .

owl:onProperties rdfs:label "onProperties" .

owl:priorVersion rdfs:label "priorVersion" .

owl:propertyChainAxiom rdfs:label "propertyChainAxiom" .

owl:propertyDisjointWith rdfs:label "propertyDisjointWith" .

owl:qualifiedCardinality rdfs:label "qualifiedCardinality" .

owl:sourceIndividual rdfs:label "sourceIndividual" .

owl:targetIndividual rdfs:label "targetIndividual" .

owl:targetValue rdfs:label "targetValue" .

owl:topDataProperty rdfs:label "topDataProperty" .

owl:topObjectProperty rdfs:label "topObjectProperty" .

owl:unionOf rdfs:label "unionOf" .

owl:withRestrictions rdfs:label "withRestrictions" .

skos:Concept rdfs:label "Concept"@en .

skos:definition rdfs:label "definition"@en .

skos:ConceptScheme rdfs:label "Concept Scheme"@en .

skos:scopeNote rdfs:label "scope note"@en .

skos:example rdfs:label "example"@en .

skos:Collection rdfs:label "Collection"@en .

skos:OrderedCollection rdfs:label "Ordered Collection"@en .

skos:inScheme rdfs:label "is in scheme"@en .

skos:hasTopConcept rdfs:label "has top concept"@en .

skos:topConceptOf rdfs:label "is top concept in scheme"@en .

skos:prefLabel rdfs:label "preferred label"@en .

skos:altLabel rdfs:label "alternative label"@en .

skos:hiddenLabel rdfs:label "hidden label"@en .

skos:notation rdfs:label "notation"@en .

skos:note rdfs:label "note"@en .

skos:changeNote rdfs:label "change note"@en .

skos:editorialNote rdfs:label "editorial note"@en .

skos:historyNote rdfs:label "history note"@en .

skos:semanticRelation rdfs:label "is in semantic relation with"@en .

skos:broader rdfs:label "has broader"@en, "broader" .

skos:broaderTransitive rdfs:label "has broader transitive"@en .

skos:narrower rdfs:label "has narrower"@en .

skos:narrowerTransitive rdfs:label "has narrower transitive"@en .

skos:related rdfs:label "has related"@en .

skos:member rdfs:label "has member"@en .

skos:memberList rdfs:label "has member list"@en .

skos:mappingRelation rdfs:label "is in mapping relation with"@en .

skos:broadMatch rdfs:label "has broader match"@en .

skos:narrowMatch rdfs:label "has narrower match"@en .

skos:relatedMatch rdfs:label "has related match"@en .

skos:exactMatch rdfs:label "has exact match"@en .

skos:closeMatch rdfs:label "has close match"@en .

:flowSink rdfs:label "flowSink" .

:Component rdfs:label "Component" .

:flowDomain rdfs:label "flowDomain" .

:flowSource rdfs:label "flowSource" .

:hasDataSource rdfs:label "hasDataSource" .

:DataSource rdfs:label "DataSource" .

:hasEstimationMethod rdfs:label "hasEstimationMethod" .

:EstimationMethod rdfs:label "Estimation Method" .

:hasParameter rdfs:label "hasParameter" .

:isFlowType rdfs:label "isFlowType" .

:flowType rdfs:label "flowType" .

:isPartialSubComponentOf rdfs:label "isPartialSubComponentOf" .

:isSubComponentOf rdfs:label "isSubComponentOf" .

:type rdfs:label "type" .

:usedBy rdfs:label "usedBy" .

:Jurisdiction rdfs:label "Jurisdiction" .

<http://geoconnex.us/iow/WaterBudgetingFramework/ClosureTerm> rdfs:label "Closure Term" .

:Basin rdfs:label "Basin" .

:Element rdfs:label "Element"@en .

:External rdfs:label "External" .

:SubtotalTerm rdfs:label "Subtotal Term" .

:Zone rdfs:label "Zone" .

:AZ rdfs:label "AZ" .

:AgriculturalAndMunicipalDepletions-UT rdfs:label "Agricultural and Municipal Depletions-UT" .

:Atmosphere rdfs:label "Atmosphere" .

:ZoneGroundwater rdfs:label "Zone Groundwater" .

:ZoneSurfaceWater rdfs:label "Zone Surface Water" .

:Outflow rdfs:label "Outflow" .

:CropConsumptiveUse-CO rdfs:label "Crop Consumptive Use-CO" .

:GroundwaterExtraction-CA rdfs:label "Groundwater Extraction-CA" .

:LivestockConsumptiveUse-CO rdfs:label "Livestock Consumptive Use-CO" .

:MunicipalAndIndustrialConsumptiveUse-CO rdfs:label "Municipal and Industrial Consumptive Use-CO" .

:MunicipalConsumptiveUse-WY rdfs:label "Municipal Consumptive Use-WY" .

:MunicipalTotalUse-WY rdfs:label "Municipal Total Use-WY" .

:SurfaceWaterDiversions-CA rdfs:label "Surface Water Diversions-CA" .

:AgriculturalAndMunicipalDiversions-UT rdfs:label "Agricultural and Municipal Diversions-UT" .

:AppliedWater-CA rdfs:label "Applied Water-CA" .

:UT rdfs:label "UT"@en .

:ZoneLandSystem rdfs:label "Zone Land System" .

:USGSStreamGages rdfs:label "USGS Stream Gages" .

:UTDiversionRecordsFromRiverCommissioners rdfs:label "UT Diversion Records from River Commissioners" .

:UTMunicipalPotableAndSecondaryDiversionRecords rdfs:label "UT Municipal Potable and Secondary Diversion Records" .

:UTOtherIrrigationCompanyRecords rdfs:label "UT Other Irrigation Company Records" .

:UTReservoirStorageAndReleaseRecords rdfs:label "UT Reservoir Storage and Release Records" .

:UTWaterRights rdfs:label "UT Water Rights Database" .

:USGSStreamStats rdfs:label "USGS StreamStats" .

:UTDivisionOfWaterResourcesArea-AltitudeMethod rdfs:label "UT Division of Water Resources Area-Altitude Method" .

:USGSMeanAnnualReachEstimates rdfs:label "USGS Mean Annual Reach Estimates" .

:InternalTransfer rdfs:label "Internal Transfer" .

:AgriculturalConsumptiveUse-WY rdfs:label "Agricultural Consumptive Use-WY" .

:WYConsumptiveUseMethod rdfs:label "WY Consumptive Use Method" .

:Evapotranspiration-CA rdfs:label "Evapotranspiration-CA" .

:IrrigationSurfaceWaterDiversions-WY rdfs:label "Irrigation Surface Water Diversions-WY" .

:TotalDiversions-WY rdfs:label "Total Diversions-WY" .

:BearRiver rdfs:label "Bear River" .

:GreenRiver rdfs:label "Green River" .

:NortheastRiver rdfs:label "Northeast River" .

:PlatteRiver rdfs:label "Platte River" .

:Powder-TongueRiver rdfs:label "Powder-Tongue River" .

:Salt-SnakeRiver rdfs:label "Salt-Snake River" .

:WY rdfs:label "WY" .

:Wind-BighornRiver rdfs:label "Wind-Bighorn River" .

:AgriculturalDepletions-UT rdfs:label "Agricultural Depletions-UT" .

:UTConsumptiveUseMethod rdfs:label "UT Consumptive Use Method" .

:SurfaceDiversionToCropland-UT rdfs:label "Surface Diversion to Cropland-UT" .

:AgriculturalPotentialConsumptiveUse-UT rdfs:label "Agricultural Potential Consumptive Use-UT" .

:NationalOceanicAndAtmosphericAdministrationStations rdfs:label "National Oceanic and Atmospheric Administration Stations" .

:PRISM rdfs:label "PRISM" .

:USBureauOfReclamationAgriMetStations rdfs:label "US Bureau of Reclamation AgriMet Stations" .

:USUResearchReport145 rdfs:label "USU Research Report 145" .

:DailyPenman-Monteith rdfs:label "Daily Penman-Monteith" .

:ModifiedBlaney-Criddle rdfs:label "Modified Blaney-Criddle" .

:SolarRadiation rdfs:label "Solar Radiation" .

:Temperature rdfs:label "Temperature" .

:VaporPressure rdfs:label "Vapor Pressure" .

:WindRun rdfs:label "Wind Run" .

:ClimateCoefficient%28kt%29 rdfs:label "Climate Coefficient (kt)" .

:CropGrowthStateCoefficient%28Kc%29 rdfs:label "Crop Growth State Coefficient (Kc)" .

:MeanMonthlyAirTemperatures%28T%29 rdfs:label "Mean Monthly Air Temperatures (T)" .

:MonthlyPercentageOfAnnualDaylightHours%28P%29 rdfs:label "Monthly Percentage of Annual Daylight Hours (P)" .

:AnnualEmployeeHours rdfs:label "Annual Employee Hours" .

:MineSafetyAndHealthAdministration%28MSHA%29 rdfs:label "Mine Safety and Health Administration (MSHA)" .

:AnnualEvaporation rdfs:label "Annual Evaporation" .

:MonthlyEvaporation rdfs:label "Monthly Evaporation" .

:NM rdfs:label "NM"@en .

:AnnualSodaAshProduction rdfs:label "Annual Soda Ash Production" .

:USGeologicalSurvey%28USGS%29 rdfs:label "US Geological Survey (USGS)" .

:TotalLandSystemInflow-CA rdfs:label "Total Land System Inflow-CA" .

:CA rdfs:label "CA" .

:AreaOutflows rdfs:label "Area Outflows-UT" .

:BasinOutflow-UT rdfs:label "Basin Outflow-UT" .

:ExternalSurfaceWater rdfs:label "External Surface Water" .

:GagedStreamOutflow-WY rdfs:label "Gaged Stream Outflow-WY" .

:StreamOutfow-CA rdfs:label "Stream Outflow-CA" .

:Exports-CO rdfs:label "Exports-CO" .

:TotalSurfaceWaterOutflow-CA rdfs:label "Total Surface Water Outflow-CA" .

:AverageMonthlyReservoirGageHeight rdfs:label "Average Monthly Reservoir Gage Height" .

:IrrigationDistricts rdfs:label "Irrigation Districts" .

:USArmyCorpsOfEngineers rdfs:label "US Army Corps of Engineers" .

:USBureauOfReclamationStations rdfs:label "US Bureau of Reclamation Stations" .

:NewMexicoInterstateStreamCommission%28NMISC%29 rdfs:label "New Mexico Interstate Stream Commission (NMISC)" .

:AverageUseRate rdfs:label "Average Use Rate" .

:MidwestPlanServiceStructuresAndEnvironmentalHandbook%2C1977 rdfs:label "Midwest Plan Service Structures and Environmental Handbook, 1977" .

:CO rdfs:label "CO"@en .

:Baseflow rdfs:label "Baseflow" .

:HistoricalData rdfs:label "Historical Data" .

:BasinInflow-UT rdfs:label "Basin Inflow-UT" .

:RiverInflow-UT rdfs:label "River Inflow-UT" .

:Inflow rdfs:label "Inflow" .

:GagedStreamInflow-WY rdfs:label "Gaged Stream Inflow-WY" .

:GagedSurfaceWaterInflow-CO rdfs:label "Gaged Surface Water Inflow-CO" .

:UngagedSurfaceWaterInflow-CO rdfs:label "Ungaged Surface Water Inflow-CO" .

:TotalSurfaceWaterInflow-CA rdfs:label "Total Surface Water Inflow-CA" .

:StreamInflow-CA rdfs:label "Stream Inflow-CA" .

:COAgriculturalMeteorologyNetworkStation rdfs:label "CO Agricultural Meteorology Network Station (COAGM)" .

:COConsumptiveUseMethod rdfs:label "CO Consumptive Use Method" .

:CODiversionRecords rdfs:label "CO Diversion Records" .

:CODivisionOfWaterResourcesGages rdfs:label "CO Division of Water Resources Gages" .

:HydroBase rdfs:label "HydroBase" .

:SCSTR21 rdfs:label "SCS TR21" .

:SatelliteAndAerialPhotos rdfs:label "Satellite and Aerial Photos" .

:SnotelNetworkOfWeatherStations rdfs:label "Snotel Network of Weather Stations" .

:WeatherStations rdfs:label "Weather Stations" .

:CommunityCollaborativeRain%2CHailAndSnowNetwork%28CoCoRaHS%29 rdfs:label "Community Collaborative Rain, Hail and Snow Network (CoCoRaHS)" .

:NationalAgriculturalStatisticsService%28NASS%29CroplandDataLayer rdfs:label "National Agricultural Statistics Service (NASS) Cropland Data Layer" .

:RemoteAutomatedWeatherStations%28RAWS%29 rdfs:label "Remote Automated Weather Stations (RAWS)" .

:COIrrigatedAcreageAssessment rdfs:label "CO Irrigated Acreage Assessment" .

:CropIrrigationRequirementEstimationMethod rdfs:label "Crop Irrigation Requirement Estimation Method" .

:EnergyBalanceRemoteSensing rdfs:label "Energy Balance Remote Sensing" .

:METRIC rdfs:label "METRIC" .

:ModifiedBlaney-CriddleWithETElevationAdjustment rdfs:label "Modified Blaney-Criddle with ET Elevation Adjustment" .

:NDVIRemoteSensing rdfs:label "NDVI Remote Sensing" .

:NDVIstar rdfs:label "NDVIstar" .

:On-FarmWaterBalance rdfs:label "On-Farm Water Balance" .

:OriginalBlaney-Criddle rdfs:label "Original Blaney-Criddle" .

:OriginalBlaney-CriddleWithETElevationAdjustment rdfs:label "Original Blaney-Criddle with ET Elevation Adjustment" .

:RESET rdfs:label "RESET" .

:StateCU rdfs:label "State CU" .

:CropIrrigationRequirement rdfs:label "Crop Irrigation Requirement" .

:CropType rdfs:label "Crop Type" .

:EffectivePrecipitation rdfs:label "Effective Precipitation" .

:IrrigatedAcreage rdfs:label "Irrigated Acreage" .

:IrrigationMethod rdfs:label "Irrigation Method" .

:PotentialConsumptiveUse rdfs:label "Potential Consumptive Use" .

:Precipitation rdfs:label "Precipitation" .

:SupplySource rdfs:label "Supply Source" .

:SupplyType rdfs:label "Supply Type" .

:WaterSupply rdfs:label "Water Supply" .

:CODivisionOfWaterResources rdfs:label "CO Division of Water Resources" .

:COGISExercise rdfs:label "CO GIS Exercise" .

:COLivestockMethod rdfs:label "CO Livestock Method" .

:StateAgriculturalStatistics rdfs:label "State Agricultural Statistics" .

:LivestockCount rdfs:label "Livestock Count" .

:COMunicipalAndIndustrialMethod rdfs:label "CO Municipal and Industrial Method" .

:ConsumptiveRatio rdfs:label "Consumptive Ratio" .

:GrossUsage rdfs:label "Gross Usage" .

:Population rdfs:label "Population" .

:CONativeVegetationMethod rdfs:label "CO Native Vegetation Method" .

:HistoricalDiversionsFile rdfs:label "Historical Diversions File" .

:Unknown rdfs:label "Unknown" .

:Diversions rdfs:label "Diversions" .

:NativeVegetationCoefficient rdfs:label "Native Vegetation Coefficient" .

:ReturnFlow rdfs:label "Return Flow" .

:ChangeInGroundWaterStorage-CO rdfs:label "Change in Ground Water Storage-CO" .

:StorageChange rdfs:label "Storage Change" .

:ChangeInGroundwaterStorage-CA rdfs:label "Change in Groundwater Storage-CA" .

:ChangeInGroundwaterStorage-AUS rdfs:label "Change in Groundwater Storage-AUS" .

:ChangeInTotalSystemStorage-CA rdfs:label "Change in Total System Storage-CA" .

:ChangeInLandSystemStorage-CA rdfs:label "Change in Land System Storage-CA" .

:ChangeInSurfaceWaterStorage-AUS rdfs:label "Change in Surface Water Storage-AUS" .

:ChangeInSurfaceWaterStorage-CA rdfs:label "Change in Surface Water Storage-CA" .

:ChangeInSurfaceWaterStorage-CO rdfs:label "Change in Surface Water Storage-CO" .

:Class rdfs:label "Class " .

:ClassAPanEvaporationData rdfs:label "Class A Pan Evaporation Data" .

:CoalProductionQuantities rdfs:label "Coal Production Quantities" .

:ColoradoCensusBureau rdfs:label "Colorado Census Bureau" .

:ColoradoStateMod rdfs:label "Colorado StateMod" .

:ColoradoWaterConservationBoard%28CWCB%29 rdfs:label "Colorado Water Conservation Board (CWCB)" .

:DirectFlowDemand-Annual rdfs:label "Direct Flow Demand - Annual" .

:DirectFlowDemand-Monthly rdfs:label "Direct Flow Demand - Monthly" .

:Evaporation rdfs:label "Evaporation" .

:InstreamFlowDemand-Annual rdfs:label "Instream Flow Demand - Annual" .

:InstreamFlowDemand-Monthly rdfs:label "Instream Flow Demand-Monthly" .

:ReservoirTargets rdfs:label "Reservoir Targets" .

:Streamflow rdfs:label "Streamflow" .

:WellDemand-Monthly rdfs:label "Well Demand - Monthly" .

:Commercial-NMOSE rdfs:label "Commercial-NMOSE" .

:MunicipalAndIndustrialDiversions-UT rdfs:label "Municipal and Industrial Diversions-UT" .

:ConservancyDistricts rdfs:label "Conservancy Districts" .

:ConveyanceEvaporation-CA rdfs:label "Conveyance Evaporation-CA" .

:HumanConsumption-NM rdfs:label "Human Consumption-NM" .

:ConveyanceLossesForAllocatedDiversions-AUS rdfs:label "Conveyance Losses for Allocated Diversions-AUS" .

:SurfaceWaterOutflows-AUS rdfs:label "Surface Water Outflows-AUS" .

:ConveyanceSeepage-CA rdfs:label "Conveyance Seepage-CA" .

:TotalGroundwaterSystemInflow-CA rdfs:label "Total Groundwater System Inflow-CA" .

:CoplandPrecipitation-UT rdfs:label "Cropland Precipitation-UT" .

:Precipitation-CA rdfs:label "Precipitation-CA" .

:Precipitation-CO rdfs:label "Precipitation-CO" .

:Precipitation-NM rdfs:label "Precipitation-NM" .

:Precipitation-UT rdfs:label "Precipitation-UT" .

:Precipitation-WY rdfs:label "Precipitation-WY" .

:IrrigatedAgricultureDepletions-NMOSE rdfs:label "Irrigated Agriculture Depletions-NMOSE" .

:EmeryWaterConservancyDistrictStations rdfs:label "Emery Water Conservancy District Stations" .

:MesoWestStations rdfs:label "MesoWest Stations" .

:NationalWeatherServiceStations rdfs:label "National Weather Service Stations" .

:NewMexicoClimateCenterStations rdfs:label "New Mexico Climate Center Stations" .

:CooperativeObserverNetwork%28COOP%29 rdfs:label "Cooperative Observer Network (COOP)" .

:FruitGrowersNetworkStations%28FGNET%29 rdfs:label "Fruit Growers Network Stations (FGNET)" .

:NationalClimaticDataCenter%27sClimatographyOfTheUnitedStatesNo.81 rdfs:label "National Climatic Data Center's Climatography of the United States No. 81" .

:NaturalResourcesConservationServiceStations%28NRCS%29 rdfs:label "Natural Resources Conservation Service Stations (NRCS)" .

:SoilClimateAnalysisNetwork%28SCAN%29 rdfs:label "Soil Climate Analysis Network (SCAN)" .

:USBureauOfLandManagement%28BLM%29 rdfs:label "US Bureau of Land Management (BLM)" .

:WYDepartmentOfEnvironmentalQuality%28DEQ%29 rdfs:label "WY Department of Environmental Quality (DEQ)" .

:WesternRegionalClimateCenter%28WRCC%29Stations rdfs:label "Western Regional Climate Center (WRCC) Stations" .

:WyomingStateEngineer%27sOfficeStations rdfs:label "Wyoming State Engineer's Office Stations" .

:USBR rdfs:label "USBR" .

:CropTypeStateAssessments rdfs:label "Crop Type State Assessments" .

:FieldSurvey rdfs:label "Field Survey" .

:GroundSurvey rdfs:label "Ground Survey" .

:USDACroplandDataLayer%28CDL%29 rdfs:label "USDA Cropland Data Layer (CDL)" .

:DailyASCEStandardizedPenman-Monteith rdfs:label "Daily ASCE Standardized Penman-Monteith" .

:DailyEffectivePrecipitation rdfs:label "Daily Effective Precipitation" .

:DailyModifiedHargreaves rdfs:label "Daily Modified Hargreaves" .

:DaytimeHours rdfs:label "Daytime Hours" .

:DirectCommunication rdfs:label "Direct Communication" .

:WyomingWaterDevelopmentCommission%28WWDC%292002WaterSystemSurveyReport rdfs:label
    "Wyoming Water Development Commission (WWDC) 2002 Water System Survey Report" .

:WYDiversionDataFromWaterUsers rdfs:label "WY Diversion Data from Water Users" .

:WYOfficeOfTheStateEngineer rdfs:label "WY Office of the State Engineer" .

:DivertibleFlow-WY rdfs:label "Divertible Flow" .

:DomesticTotalUse-WY rdfs:label "Domestic Total Use-WY" .

:USCensusBureau rdfs:label "US Census Bureau" .

:WithdrawalMethod rdfs:label "Withdrawal Method" .

:GallonsPerCapitaPerDay%28GPCD%29 rdfs:label "Gallons Per Capita Per Day (GPDPC)" .

:DownstreamFlow rdfs:label "Downstream Flow" .

:WyomingWaterResourcesDataSystem%28WRDS%29 rdfs:label "Wyoming Water Resources Data System (WRDS)" .

:UTEffectivePrecipitationMethod rdfs:label "UT Effective Precipitation Method" .

:EffectivePrecipitationFactor rdfs:label "Effective Precipitation Factor" .

:ElectricalGenerationData rdfs:label "Electrical Generation Data" .

:USEnergyInformationAdministration%28USEIA%29 rdfs:label "US Energy Information Administration (USEIA)" .

:Elevation-Area-CapacityTables rdfs:label "Elevation-Area-Capacity Tables" .

:USBureauOfReclamation rdfs:label "US Bureau of Reclamation" .

:UTStateEngineerData rdfs:label "UT State Engineer Data" .

:WaterResourcesStudies rdfs:label "Water Resources Studies" .

:EmpiricalDataForSmallReservoirs rdfs:label "Empirical Data for Small Reservoirs" .

:MonthlyPrecipitationVolume rdfs:label "Monthly Precipitation Volume" .

:Rainfall rdfs:label "Rainfall" .

:ReservoirSurfaceArea rdfs:label "Reservoir Surface Area" .

:Evaporation-AUS rdfs:label "Evaporation-AUS" .

:Evaporation-NM rdfs:label "Evaporation-NM" .

:TotalEvaporation-NM rdfs:label "Total Evaporation-NM" .

:EvaporationFromReservoirs-NMOSE rdfs:label "Evaporation from Reservoirs-NMOSE" .

:PanApproach rdfs:label "Pan Approach" .

:MonthlyGrossEvaporationRate rdfs:label "Monthly Gross Evaporation Rate" .

:WinterIceSurfaceArea rdfs:label "Winter Ice Surface Area" .

:LakeEvaporation-CA rdfs:label "Lake Evaporation-CA" .

:ReservoirEvaporation-CO rdfs:label "Reservoir Evaporation-CO" .

:ReservoirEvaporation-UT rdfs:label "Reservoir Evaporation-UT" .

:TotalLandSystemOutflow-CA rdfs:label "Total Land System Outflow-CA" .

:ExternalGroundwater rdfs:label "External Groundwater" .

:GroundwaterExport-CA rdfs:label "Groundwater Export-CA" .

:StoredWaterExport-CA rdfs:label "Stored Water Export-CA" .

:SurfaceWaterExports-CA rdfs:label "Surface Water Exports-CA" .

:ExternalLandSystem rdfs:label "External Land System" .

:FacilityDirectorOrOperator rdfs:label "Facility Director or Operator" .

:FederalArchives rdfs:label "Federal Archives" .

:FloodReturn-AUS rdfs:label "Flood Return-AUS" .

:SurfaceWaterInflows-AUS rdfs:label "Surface Water Inflows-AUS" .

:Flow rdfs:label "Flow" .

:GPSPopulationData rdfs:label "GPS Population Data" .

:GageHeight rdfs:label "Gage Height" .

:TotalInflow-CA rdfs:label "Total Inflow-CA" .

:TotalOutflow-CA rdfs:label "Total Outflow-CA" .

:GagedSurfaceWaterOutflow-CO rdfs:label "Gaged Surface Water Outflow-CO" .

:GrossActivelyIrrigatedAcreage rdfs:label "Gross Actively Irrigated Acreage" .

:NationalAgriculturalStatisticsService rdfs:label "National Agricultural Statistics Service" .

:USDAFarmServiceAgency rdfs:label "USDA Farm Service Agency" .

:NMOfficeOfTheStateEngineer%28NMOSE%29 rdfs:label "NM Office of the State Engineer (NMOSE)" .

:GrossMonthlyFreeWaterSurfaceEvaporation rdfs:label "Gross Monthly Free Water Surface Evaporation" .

:NOAATechnicalReportNWS33 rdfs:label "NOAA Technical Report NWS 33" .

:GroundWaterInflow-CO rdfs:label "Ground Water Inflow-CO" .

:SubsurfaceInflow-CA rdfs:label "Subsurface Inflow-CA" .

:GroundWaterOutflow-CO rdfs:label "Ground Water Outflow-CO" .

:TotalGroundwaterSystemOutflow-CA rdfs:label "Total Groundwater System Outflow-CA" .

:SubsurfaceOutflow-CA rdfs:label "Subsurface Outflow-CA" .

:GroundwaterDischarge-AUS rdfs:label "Groundwater Discharge-AUS" .

:Discharge%3AGroundwater-AUS rdfs:label "Discharge: Groundwater-AUS" .

:GroundwaterDiversions-NM rdfs:label "Groundwater Diversions-NM" .

:GroundwaterET-NM rdfs:label "Groundwater ET-NM" .

:RiparianConsumption-NM rdfs:label "Riparian Consumption-NM" .

:LakeGainFromGroundwater-CA rdfs:label "Lake Gain from Groundwater-CA" .

:GroundwaterInflows-AUS rdfs:label "Groundwater Inflows-AUS" .

:GroundwaterInflows-NM rdfs:label "Groundwater Inflows-NM" .

:GroundwaterOutflows-AUS rdfs:label "Groundwater Outflows-AUS" .

:GroundwaterOutflows-NM rdfs:label "Groundwater Outflows-NM" .

:GroundwaterReturn-NM rdfs:label "Groundwater Return-NM" .

:GroundwaterStock-NM rdfs:label "Groundwater Stock-NM" .

:GroundwaterUse rdfs:label "Groundwater Use" .

:MunicipalAndIndustrialDiversionReports rdfs:label "Municipal and Industrial Diversion Reports" .

:USGSEstimatesOfBasinGroundwaterFlows rdfs:label "USGS Estimates of Basin Groundwater Flows" .

:USGSGroundwaterReports rdfs:label "USGS Groundwater Reports" .

:GroundwaterUse-UT rdfs:label "Groundwater Use-UT" .

:PumpedGroundwater-UT rdfs:label "Pumped Groundwater-UT" .

:GroundwaterWithdrawals rdfs:label "Groundwater Withdrawals" .

:HighPlainsClimateCenter-UniversityOfNebraska rdfs:label "High Plains Climate Center - University of Nebraska" .

:UTStateArchives rdfs:label "UT State Archives" .

:HumanPopulationModel-NM rdfs:label "Human Population Model-NM" .

:HumanReturns-NM rdfs:label "Human Returns-NM" .

:HumanStorageAndDistributionSystemStock-NM rdfs:label "Human Storage and Distribution System Stock-NM" .

:ImportedWater-CA rdfs:label "Imported Water-CA" .

:Imports-CO rdfs:label "Imports-CO" .

:IndicatorGageApproach rdfs:label "Indicator Gage Approach" .

:Industrial-NMOSE rdfs:label "Industrial-NMOSE" .

:Metered rdfs:label "Metered" .

:IndustrialConsumptiveUse-WY rdfs:label "Industrial Consumptive Use-WY" .

:IndustrialTotalUse-WY rdfs:label "Industrial Total Use-WY" .

:WyomingOilAndGasConservationCommission%28WYOGCC%29 rdfs:label "Wyoming Oil and Gas Conservation Commission (WYOGCC)" .

:MonthlyCoalbedMethaneGasProductionAndProducedWater rdfs:label "Monthly Coalbed Methane Gas Production and Produced Water" .

:NaturalGasProcessingVolumes rdfs:label "Natural Gas Processing Volumes" .

:MonthlyOil%2CGas%2CAndProducedWater rdfs:label "Monthly Oil, Gas, and Produced Water" .

:SurfaceWaterDelivery-CA rdfs:label "Surface Water Delivery-CA" .

:Inflow-OutflowApproach rdfs:label "Inflow-Outflow Approach" .

:Inter-regionCoastalInflow-AUS rdfs:label "Inter-region Coastal Inflow-AUS" .

:Inter-regionCoastalOutflow-AUS rdfs:label "Inter-region Coastal Outflow-AUS" .

:InterpolationFromOtherRecords rdfs:label "Interpolation from Other Records" .

:NMIrrigatedAcreageAssessment rdfs:label "NM Irrigated Acreage Assessment" .

:USBRIrrigatedAcreageAssessment rdfs:label "USBR Irrigated Acreage Assessment" .

:UTIrrigatedAcreageAssessment rdfs:label "UT Irrigated Acreage Assessment" .

:WYIrrigatedAcreageAssessment rdfs:label "WY Irrigated Acreage Assessment" .

:SupplyStructure rdfs:label "Supply Structure" .

:IrrigatedAgriculture-NMOSE rdfs:label "Irrigated Agriculture-NMOSE" .

:NMConsumptiveUseMethod rdfs:label "NM Consumptive Use Method" .

:IrrigatedAgricultureDiversions-NMOSE rdfs:label "Irrigated Agriculture Diversions-NMOSE" .

:NMOSECropAcreageFile rdfs:label "NMOSE Crop Acreage File" .

:NMOSEGrowingSeasonFile rdfs:label "NMOSE Growing Season File" .

:NMOSETemperatureAndPrecipitationFile rdfs:label "NMOSE Temperature and Precipitation File" .

:ConsumptiveIrrigationRequirement%28CIR%29 rdfs:label "Consumptive Irrigation Requirement (CIR)" .

:IrrigationSchemeInflows-AUS rdfs:label "Irrigation Scheme Inflows-AUS" .

:IrrigationSchemeOutflows-AUS rdfs:label "Irrigation Scheme Outflows-AUS" .

:LCRAS rdfs:label "LCRAS" .

:LakeLossToGroundwater-CA rdfs:label "Lake Loss to Groundwater-CA" .

:Recharge-NM rdfs:label "Recharge-NM" .

:LandSurfaceExapotranspiration-NM rdfs:label "Land Surface Evapotranspiration-NM" .

:LandSurfaceStock-NM rdfs:label "Land Surface Stock-NM" .

:Livestock-NMOSE rdfs:label "Livestock-NMOSE" .

:LivestockConsumptiveUse-WY rdfs:label "Livestock Consumptive Use-WY" .

:LivestockPopulation rdfs:label "Livestock Population" .

:NewMexicoDepartmentOfAgriculture rdfs:label "New Mexico Department of Agriculture" .

:ManagedAquiferRecharge-AUS rdfs:label "Managed Aquifer Recharge-AUS" .

:UrbanWaterSystemOutflows-AUS rdfs:label "Urban Water System Outflows-AUS" .

:ManagedAquiferRecharge-CA rdfs:label "Managed Aquifer Recharge-CA" .

:MilitaryBasePopulationData rdfs:label "Military Base Population Data" .

:Mining-NMOSE rdfs:label "Mining-NMOSE" .

:Industrial%3AMineProduction-WY rdfs:label "Industrial: Mine Production-WY" .

:SumOfMonthlyConsumptiveUseFactorsForGrowingSeason%28F%29 rdfs:label "Sum of Monthly Consumptive Use Factors for Growing Season (F)" .

:MonthlyEffectivePrecipitation rdfs:label "Monthly Effective Precipitation" .

:Power-NMOSE rdfs:label "Power-NMOSE" .

:PublicWaterSupply-NMOSE rdfs:label "Public Water Supply-NMOSE" .

:MunicipalAndIndustrialDepeltion-UT rdfs:label "Municipal and Industrial Depeltion-UT" .

:MunicipalAndIndustrialReturnFlow-UT rdfs:label "Municipal and Industrial Return Flow-UT" .

:ReturnFlow-CA rdfs:label "Return Flow-CA" .

:MunicipalAndSelfSuppliedDomestic-NM rdfs:label "Municipal and Self Supplied Domestic-NM" .

:NDVI rdfs:label "NDVI" .

:NMDiversionRecords rdfs:label "NM Diversion Records" .

:NMSpreadsheet-BasedConsumptiveUseModel rdfs:label "NM Spreadsheet-Based Consumptive Use Model" .

:OriginalHargreaves rdfs:label "Original Hargreaves" .

:NMIrrigationWithdrawals rdfs:label "NM Irrigation Withdrawals" .

:NMOSEWaterRightsDatabase rdfs:label "NMOSE Water Rights Database" .

:NMOSETechnicalReportNo.48 rdfs:label "NMOSE Technical Report No. 48" .

:NativeVegetationConsumptiveUse-CO rdfs:label "Native Vegetation Consumptive Use-CO" .

:NaturalSystemUse-UT rdfs:label "Natural System Use-UT" .

:RiparianDepletions-UT rdfs:label "Riparian Depletions-UT" .

:NaturalFlowGainDistribution rdfs:label "Natural Flow Gain Distribution" .

:ProrationFactors rdfs:label "Proration Factors" .

:Non-allocatedExtraction-AUS rdfs:label "Non-allocated Extraction-AUS" .

:OtherIncreases-AUS rdfs:label "Other Increases-AUS" .

:OtherStatutoryRights-AUS rdfs:label "Other Statutory Rights-AUS" .

:Outflow-AUS rdfs:label "Outflow-AUS" .

:OverbankFloodSpilling-AUS rdfs:label "Overbank Flood Spilling-AUS" .

:OverbankFlow-AUS rdfs:label "Overbank Flow-AUS" .

:PersonalOutreach rdfs:label "Personal Outreach" .

:WaterUseEstimate rdfs:label "Water Use Estimate" .

:PopulationServedByPublicWaterSupply rdfs:label "Population Served by Public Water Supply" .

:NewMexicoEnvironmentDepartment%28NMED%29 rdfs:label "New Mexico Environment Department (NMED)" .

:UniversityOfNewMexicoGeospatialAndPopulationStudies%28UNMGPS%29 rdfs:label "University of New Mexico Geospatial and Population Studies (UNM GPS)" .

:PotentialEvapotranspiration rdfs:label "Potential Evapotranspiration" .

:Industrial%3AElectricalGeneration-WY rdfs:label "Industrial: Electrical Generation-WY" .

:WyomingWaterResourcesDataSystemsWaterAndClimateMapServer rdfs:label "Wyoming Water Resources Data Systems Water and Climate Map Server" .

:Precipitation-AUS rdfs:label "Precipitation-AUS" .

:PrecipitationOnLakes-CA rdfs:label "Precipitation on Lakes-CA" .

:RechargeOfAppliedWater-CA rdfs:label "Recharge of Applied Water-CA" .

:RechargeOfPrecipitation-CA rdfs:label "Recharge of Precipitation-CA" .

:RecycledWaterExport-CA rdfs:label "Recycled Water Export-CA" .

:ReservoirEstimationMethod rdfs:label "Reservoir Estimation Method" .

:SurfaceAreaOfReservoir rdfs:label "Surface Area of Reservoir" .

:ReservoirEvaporation-WY rdfs:label "Reservoir Evaporation-WY" .

:PanMethod%28NetEvaporation%29 rdfs:label "Pan Method (Net Evaporation)" .

:GrossPanEvaportation%28inches%29 rdfs:label "Gross Pan Evaportation (inches)" .

:RiverAndFloodplainLosses-AUS rdfs:label "River and Floodplain Losses-AUS" .

:RiverEvaporation-NM rdfs:label "River Evaporation-NM" .

:RiverUseByWetPasture-UT rdfs:label "River Use By Wet Pasture-UT" .

:Runoff-AUS rdfs:label "Runoff-AUS" .

:Runoff-CA rdfs:label "Runoff-CA" .

:Runoff-NM rdfs:label "Runoff-NM" .

:STATSGOSoilsData rdfs:label "STATSGO Soils Data" .

:Self-SuppliedDomestic-NMOSE rdfs:label "Self-Supplied Domestic-NMOSE" .

:SelfSuppliedDomesticPopulation rdfs:label "Self Supplied Domestic Population" .

:SoilMoistureHoldingCapacity rdfs:label "Soil Moisture Holding Capacity" .

:WaterResourcesIrrigatedLandUseDatabase rdfs:label "Water Resources irrigated land use database" .

:StateCUOutput rdfs:label "State CU Output" .

:StateData rdfs:label "State Data" .

:StoredWaterExtraction-CA rdfs:label "Stored Water Extraction-CA" .

:StreamEvaporation-CA rdfs:label "Stream Evaporation-CA" .

:StreamGainFromGroundwater-CA rdfs:label "Stream Gain from Groundwater-CA" .

:StreamLossToGroundwater-CA rdfs:label "Stream Loss to Groundwater-CA" .

:StudentPopulation rdfs:label "Student Population" .

:SurfaceWaterDiversions-NM rdfs:label "Surface Water Diversions-NM" .

:SurfaceWaterEvaporation-NM rdfs:label "Surface Water Evaporation-NM" .

:SurfaceWaterFlows-UT rdfs:label "Surface Water Flows-UT" .

:SurfaceWaterGroundwaterInteractions-NM rdfs:label "Surface Water Groundwater Interactions-NM" .

:SurfaceWaterInflows-NM rdfs:label "Surface Water Inflows-NM" .

:SurfaceWaterOutflows-NM rdfs:label "Surface Water Outflows-NM" .

:SurfaceWaterReturns-NM rdfs:label "Surface Water Returns-NM" .

:SurfaceWaterStock-NM rdfs:label "Surface Water Stock-NM" .

:TotalLandReturnFlow-UT rdfs:label "Total Land Return Flow-UT" .

:TributaryInflow-UT rdfs:label "Tributary Inflow-UT" .

:USBRConsumptiveUseMethod rdfs:label "USBR Consumptive Use Method" .

:XCONS rdfs:label "XCONS" .

:USGS rdfs:label "USGS"@en .

:UngagedLosses rdfs:label "Ungaged Losses" .

:UngagedStreamGains-WY rdfs:label "Ungaged Stream Gains-WY" .

:WyomingGain%2FLossEstimationMethod rdfs:label "Wyoming Gain/Loss Estimation Method" .

:UpstreamFlow rdfs:label "Upstream Flow" .

:UngagedStreamLosses-WY rdfs:label "Ungaged Stream Losses-WY" .

:UniversityOfNewMexico rdfs:label "University of New Mexico" .

:UrbanWaterSystemInflows-AUS rdfs:label "Urban Water System Inflows-AUS" .

:WYAgricultureConsumptiveUseEstimationMethod rdfs:label "WY Agriculture Consumptive Use Estimation Method" .

:WYDiversionRecords rdfs:label "WY Diversion Records" .

:WYElectricalGenerationMethod rdfs:label "WY Electrical Generation Method" .

:WYIndustrialProductionMethod rdfs:label "WY Industrial Production Method" .

:WYIrrigatedAcreageConsumptiveUseModel rdfs:label "WY Irrigated Acreage Consumptive Use Model" .

:WYMineProductionMethod rdfs:label "WY Mine Production Method" .

:WYOfficeOfTheStateEngineerHydrographerCommissionerReports rdfs:label "WY Office of the State Engineer Hydrographer Commissioner Reports" .

:WYVariousWaterSupplyReports rdfs:label "WY Various Water Supply Reports" .

:WastewaterCollected-AUS rdfs:label "Wastewater Collected-AUS" .

:WaterReleaseCausedByLandSubsidence-CA rdfs:label "Water Release Caused by Land Subsidence-CA"@en .

:WaterUse-NM rdfs:label "Water Use-NM" .

:BrownAndCaldwell%2C1984 rdfs:label "Brown and Caldwell,1984" .

:atmost rdfs:label "atmost" .

:cropGrowh rdfs:label "crop growh" .

:weater rdfs:label "weater" .

:AllocatedDiversion%3AEnvironmentalPurposes-AUS rdfs:label "Allocated Diversion: Environmental Purposes-AUS" .

:AllocatedDiversion%3AIndividualUsers-AUS rdfs:label "Allocated Diversion: Individual Users-AUS" .

:AllocatedDiversion%3AInter-region-AUS rdfs:label "Allocated Diversion: Inter-region-AUS" .

:AllocatedDiversion%3AIrrigation-AUS rdfs:label "Allocated Diversion: Irrigation-AUS" .

:AllocatedDiversion%3AIrrigationScheme-AUS rdfs:label "Allocated Diversion: Irrigation Scheme-AUS" .

:AllocatedDiversion%3AUrbanSystem-AUS rdfs:label "Allocated Diversion: Urban System-AUS" .

:AllocatedDiversions%3ASurfaceWater-AUS rdfs:label "Allocated Diversions:Surface Water-AUS" .

:AllocatedExtraction%3AEnvironmentalPurposes-AUS rdfs:label "Allocated Extraction: Environmental Purposes-AUS" .

:AllocatedExtraction%3AGroundwater-AUS rdfs:label "Allocated Extraction: Groundwater-AUS" .

:AllocatedExtraction%3AIndividualUsers-AUS rdfs:label "Allocated Extraction: Individual Users-AUS" .

:AllocatedExtraction%3AIrrigation-AUS rdfs:label "Allocated Extraction: Irrigation-AUS" .

:AllocatedExtraction%3AUrbanSystem-AUS rdfs:label "Allocated Extraction: Urban System-AUS" .

:AllocationExtraction%3ASalinityAndWaterTableManagement-AUS rdfs:label "Allocation Extraction: Salinity and Water Table Management-AUS" .

:AppliedWaterReuse%2FRecycledWater-CA rdfs:label "Applied Water Reuse/Recycled Water-CA" .

:Commercial%3AGolfCourses-NMOSE rdfs:label "Commercial: Golf Courses-NMOSE" .

:Commercial%3AUnmetered-NMOSE rdfs:label "Commercial: Unmetered-NMOSE" .

:Commercial%3AIncompleteMetered-NMOSE rdfs:label "Commercial: Incomplete Metered-NMOSE" .

:Commercial%3AMetered-NMOSE rdfs:label "Commercial: Metered-NMOSE" .

:Commercial%3ASchools-NMOSE rdfs:label "Commercial: Schools-NMOSE" .

:Delivery%3ADesalinatedWater-AUS rdfs:label "Delivery: Desalinated Water-AUS" .

:Delivery%3AInter-region-AUS rdfs:label "Delivery: Inter-region-AUS" .

:Delivery%3AInter-regionAgreement-AUS rdfs:label "Delivery: Inter-region Agreement-AUS" .

:Delivery%3AIrrigationScheme-AUS rdfs:label "Delivery: Irrigation Scheme-AUS" .

:Delivery%3ARecycledWater-AUS rdfs:label "Delivery: Recycled Water-AUS" .

:Delivery%3AUrbanUsers-AUS rdfs:label "Delivery:Urban Users-AUS" .

:Discharge%3ALandscape-AUS rdfs:label "Discharge: Landscape-AUS" .

:Discharge%3ASea-AUS rdfs:label "Discharge: Sea-AUS" .

:Discharge%3ASurfaceWater-AUS rdfs:label "Discharge: Surface Water-AUS" .

:Discharge%3AUrbanSupply-AUS rdfs:label "Discharge: Urban Supply-AUS" .

:Discharge%3AUrbanSupplySystem-AUS rdfs:label "Discharge: Urban Supply System-AUS" .

:Discharge%3AUser-AUS rdfs:label "Discharge: User-AUS" .

:Discharge%3AWastewater-AUS rdfs:label "Discharge: Wastewater-AUS" .

:Diversions%3AStatutoryRights-AUS rdfs:label "Diversions: Statutory Rights-AUS" .

:Extraction%3AStatutoryRights-AUS rdfs:label "Extraction: Statutory Rights-AUS" .

:Industrial%3ACoalbedMethandProduction-WY rdfs:label "Industrial: Coalbed Methand Production-WY" .

:Industrial%3AMiscellaneous-WY rdfs:label "Industrial: Miscellaneous-WY" .

:Industrial%3ANaturalGas-WY rdfs:label "Industrial: Natural Gas-WY" .

:Industrial%3AOilAndGas-WY rdfs:label "Industrial: Oil and Gas-WY" .

:Inter-regionInflow%3AGroundwater-AUS rdfs:label "Inter-region Inflow: Groundwater-AUS" .

:Inter-regionInflow%3ASurfaceWater-AUS rdfs:label "Inter-region Inflow: Surface Water-AUS" .

:Inter-regionOutflow%3AGroundwater-AUS rdfs:label "Inter-region Outflow: Groundwater-AUS" .

:IrrigationWaterSupplyLimitedConsumptiveUse%28Depletions%29-WY rdfs:label "Irrigation Water Supply Limited Consumptive Use (Depletions)-WY" .

:Leakage%3AFarmDams-AUS rdfs:label "Leakage: Farm Dams-AUS" .

:Leakage%3AGroundwater-AUS rdfs:label "Leakage: Groundwater-AUS" .

:Leakage%3ALandscape-AUS rdfs:label "Leakage: Landscape-AUS" .

:Leakage%3AUrbanSystem-AUS rdfs:label "Leakage: Urban System-AUS" .

:Livestock%3AMetered-NMOSE rdfs:label "Livestock: Metered-NMOSE" .

:Livestock%3AUnmetered-NMOSE rdfs:label "Livestock: Unmetered-NMOSE" .

:ManagedAquiferRecharge%3AIndividualUser-AUS rdfs:label "Managed Aquifer Recharge: Individual User-AUS" .

:ManagedAquiferRecharge%3AUrban-AUS rdfs:label "Managed Aquifer Recharge: Urban-AUS" .

:Mining%3AReported-NMOSE rdfs:label "Mining: Reported-NMOSE" .

:Mining%3AUnreported-NMOSE rdfs:label "Mining: Unreported-NMOSE" .

:MonthlyConsumptiveUseCoefficient%28k%29 rdfs:label "Monthly Consumptive Use Coefficient (k)" .

:NMOSE%E2%80%99sWaterUseAndConservationBureau%28WUCB%29Survey rdfs:label "NMOSEs Water Use and Conservation Bureau (WUCB) Survey" .

:Non-AllocatedDiversion%3ASurfaceWater-AUS rdfs:label "Non-Allocated Diversion: Surface Water-AUS" .

:Non-AllocatedExtraction%3AGroundwater-AUS rdfs:label "Non-Allocated Extraction: Groundwater-AUS" .

:Non-AllocatedExtraction%3AIndividualUsers-AUS rdfs:label "Non-Allocated Extraction: Individual Users-AUS" .

:Non-AllocatedExtraction%3AIrrigation-AUS rdfs:label "Non-Allocated Extraction: Irrigation-AUS" .

:Non-AllocatedExtraction%3AUrbanSystem-AUS rdfs:label "Non-Allocated Extraction: Urban System-AUS" .

:Non-allocatedDiversion%3AEnvironmentalPurposes-AUS rdfs:label "Non-allocated Diversion: Environmental Purposes-AUS" .

:Non-allocatedDiversion%3AIndividualUsers-AUS rdfs:label "Non-allocated Diversion: Individual Users-AUS" .

:Non-allocatedDiversion%3AUrbanSystem-AUS rdfs:label "Non-allocated Diversion: Urban System-AUS" .

:PointReturn%3AIrrigation-AUS rdfs:label "Point Return: Irrigation-AUS" .

:Power%3AReported-NMOSE rdfs:label "Power: Reported-NMOSE" .

:Power%3AUnreported-NMOSE rdfs:label "Power: Unreported-NMOSE" .

:PublicWaterSupply%3AMetered-NMOSE rdfs:label "Public Water Supply: Metered-NMOSE" .

:PublicWaterSupply%3AUnmetered-NMOSE rdfs:label "Public Water Supply: Unmetered-NMOSE" .

:Recharge%3AGroundwater-AUS rdfs:label "Recharge: Groundwater-AUS" .

:Recharge%3ALandscape-AUS rdfs:label "Recharge: Landscape-AUS", "Recharge:Landscape-AUS" .

:Recharge%3ASurfaceWater-AUS rdfs:label "Recharge: Surface Water-AUS" .

:RecycledWaterDelivery%3AUrbanUsers-AUS rdfs:label "Recycled Water Delivery: Urban Users-AUS" .

:ReturnFlow%3AEnvironmentalPurposes-AUS rdfs:label "Return Flow: Environmental Purposes-AUS" .

:RiparianRelease%3AUrbanSupply-AUS rdfs:label "Riparian Release: Urban Supply-AUS" .

:SeasonalConsumptiveUseCoefficients%28K%29 rdfs:label "Seasonal Consumptive Use Coefficients (K)" .

:SupplySystemDelivery%3AInter-Region-AUS rdfs:label "Supply System Delivery: Inter-Region-AUS" .

:SupplySystemDelivery%3AUrbanUsers-AUS rdfs:label "Supply System Delivery: Urban Users-AUS" .

:SupplySystemDischarge%3AReservoirs-AUS rdfs:label "Supply System Discharge: Reservoirs-AUS" .

:SupplySystemTransfer%3AInter-region-AUS rdfs:label "Supply System Transfer: Inter-region-AUS" .

:Transfer%3AInter-region-AUS rdfs:label "Transfer: Inter-region-AUS" .

:USCensusBureau%22CityAndTown%28IncorporatedPlacesAndMinorCivilDivisions%29%22DataSet
  rdfs:label "US Census Bureau \"City and Town (Incorporated Places and Minor Civil Divisions)\" data set" .

:WastewaterDischarge%3ALandscape-AUS rdfs:label "Wastewater Discharge: Landscape-AUS" .

:WyomingDepartmentOfEnvironmentalQuality%28WYDEQ%29 rdfs:label "Wyoming Department of Environmental Quality (WYDEQ)" .

:AUS rdfs:label "AUS" .

:AUSBureauOfMeteorology rdfs:label "AUS Bureau of Meteorology" .

:Adelaide rdfs:label "Adelaide" .

:Burdekin rdfs:label "Burdekin" .

:Canberra rdfs:label "Canberra" .

:Daly rdfs:label "Daly" .

:Fitzroy rdfs:label "Fitzroy" .

:Melbourne rdfs:label "Melbourne" .

:MurrayDarling rdfs:label "Murray Darling" .

:Ord rdfs:label "Ord" .

:Perth rdfs:label "Perth" .

:SouthEastQueensland rdfs:label "South East Queensland" .

:Sydney rdfs:label "Sydney" .

:AUSDepartmentOfEnvironmentAndNaturalResources rdfs:label "AUS Department of Environment and Natural Resources" .

:AUSDepartmentOfIndustry rdfs:label "AUS Department of Industry" .

:AWRA-LModel rdfs:label "AWRA-L model" .

:AWRA-RModel rdfs:label "AWRA-R model" .

:AcreageByCropType rdfs:label "Acreage by Crop Type" .

:AgriculturalAppliedWater-CA rdfs:label "Agricultural Applied Water-CA" .

:CAAgriculturalWaterManagementPlans rdfs:label "CA Agricultural Water Management Plans" .

:CALocalAgencyWaterDeliveryRecords rdfs:label "CA Local Agency Water Delivery Records" .

:CAPreviousReports rdfs:label "CA Previous Reports" .

:Cal-SIMETAWUnitValues rdfs:label "Cal-SIMETAW Unit Values" .

:ExistingCaliforniaWaterPlan rdfs:label "Existing California Water Plan" .

:On-farmWaterUseData rdfs:label "On-farm water use data" .

:UniversityOfCaliforniaCooperativeExtensionFarmAdvisors rdfs:label "University of California Cooperative Extension Farm  Advisors" .

:CaliforniaCentralValleySimulation%28C2VSim%29 rdfs:label "California Central Valley Simulation (C2VSim)" .

:CentralValleyHydrologicModel%28CVHM%29 rdfs:label "Central Valley Hydrologic Model (CVHM)" .

:Cal-SIMETAWModel rdfs:label "Cal-SIMETAW Model" .

:CropETApproach rdfs:label "Crop ET Approach" .

:Water-DutyBasedApproach rdfs:label "Water-Duty Based Approach" .

:CropETRequirements rdfs:label "Crop ET Requirements" .

:ETOfAppliedWater rdfs:label "ET of Applied Water" .

:IrrigationEfficiency rdfs:label "Irrigation Efficiency" .

:IrrigationRecharge rdfs:label "Irrigation Recharge" .

:PrecipitationVolumeForAgriculturalArea rdfs:label "Precipitation Volume for Agricultural Area" .

:RunoffVolume rdfs:label "Runoff Volume" .

:WaterDutyRateByCrop rdfs:label "Water Duty Rate by Crop" .

:ApparentLosses rdfs:label "Apparent Losses" .

:CADWRDemographicData rdfs:label "CA DWR Demographic Data" .

:CADWRIrrigationMethodsSurvey rdfs:label "CA DWR Irrigation Methods Survey" .

:CADWRLandUseViewer rdfs:label "CA DWR Land Use Viewer" .

:CADWRSGMADataViewer rdfs:label "CA DWR SGMA Data Viewer" .

:CALSIM2 rdfs:label "CALSIM2" .

:CAUrbanWaterManagementPlans rdfs:label "CA Urban Water Management Plans" .

:CaliforniaAgriculturalLandAndWaterUseEstimates rdfs:label "California Agricultural Land and Water Use Estimates" .

:CaliforniaDepartmentOfFinance rdfs:label "California Department of Finance" .

:CaliforniaPesticideInformationPortal rdfs:label "California Pesticide Information Portal" .

:CaliforniaWaterPlanPortfolio rdfs:label "California Water Plan Portfolio" .

:DWRLandUseSurveys rdfs:label "CA DWR Land Use Surveys" .

:SWRCBWaterConservationPortal rdfs:label "SWRCB Water Conservation Portal" .

:USDACropScape rdfs:label "USDA CropScape" .

:USDANaturalResourcesConservationServiceGeospatialWebSoilSurvey rdfs:label "USDA Natural Resources Conservation Service Geospatial Web Soil Survey" .

:CAIntegratedWaterFlowModel%28IWFM%29 rdfs:label "CA Integrated Water Flow Model (IWFM)" .

:CAIntegratedWaterFlowModel%28IWFM%29DemandCalculator rdfs:label "CA Integrated Water Flow Model (IWFM) Demand Calculator" .

:CaliforniaStateGroundwaterElevationMonitoring%28CASGEM%29 rdfs:label "California State Groundwater Elevation Monitoring (CASGEM)" .

:MODFLOW-OWHM%3AOneWaterHydrologicFlowModel rdfs:label "MODFLOW-OWHM: One Water Hydrologic Flow Model" .

:NationalLandCoverDataBase%28NLCD%29 rdfs:label "National Land Cover Data Base (NLCD)" .

:USDACountyAgCommissioner%27sDataListing rdfs:label "USDA County Ag Commissioner's Data Listing" .

:VegetationConditionExplorer%28VegScape%29 rdfs:label "Vegetation Condition Explorer (VegScape)" .

:WaterUseClassificationOfLandscapeSpecies%28WUCOLS%29 rdfs:label "Water Use Classification of Landscape Species (WUCOLS)" .

:AquiferAttribution rdfs:label "Aquifer Attribution" .

:AUSDepartmentOfEnvironment%2CLand%2CWaterAndPlanning rdfs:label "AUS Department of Environment, Land, Water and Planning" .

:AquiferThickness rdfs:label "Aquifer Thickness" .

:PortPhillipCatchmentManagementAuthority rdfs:label "Port Phillip Catchment Management Authority" .

:AssumedDiversionRate rdfs:label "Assumed Diversion Rate" .

:AustralianBureauOfStatisticsSurveys rdfs:label "Australian Bureau of Statistics Surveys" .

:WesternMountLoftyRangesPrescribedWaterResourcesAreaWaterAllocationPlan rdfs:label
    "Western Mount Lofty Ranges Prescribed Water Resources Area Water Allocation Plan" .

:BaseflowSeparationTechniques rdfs:label "Baseflow Separation Techniques" .

:BillingMeters rdfs:label "Billing Meters" .

:BoreLocation rdfs:label "Bore Location" .

:BudgetZoneArea rdfs:label "Budget Zone Area" .

:CACountyAgriculturalCommissionerCropReports rdfs:label "CA County Agricultural Commissioner Crop Reports" .

:CADWRExtensometer rdfs:label "CA DWR Extensometer" .

:CALSIM3 rdfs:label "CALSIM 3" .

:CARecycledWaterDataFromIndustrialUsers rdfs:label "CA Recycled Water Data from Industrial Users" .

:CAValidatedWaterLossReporting rdfs:label "CA Validated Water Loss Reporting" .

:CAWastewaterDataAndDispositionOfTheWater rdfs:label "CA Wastewater Data and Disposition of the Water" .

:CSIROWavesModel rdfs:label "CSIRO Waves Model" .

:CaliforniaNevadaRiverForecastCenter rdfs:label "California Nevada River Forecast Center" .

:CaliforniaWaterPlanUpdateData rdfs:label "California Water Plan Update Data" .

:CaliforniaWaterPlanWaterPortfolioManagedWetlandsWaterUseData rdfs:label "California Water Plan Water Portfolio Managed Wetlands Water Use Data" .

:ChangeInGroundwaterLevel rdfs:label "Change in Groundwater Level" .

:GroundwaterElevation rdfs:label "Groundwater Elevation" .

:SpecificYield rdfs:label "Specific Yield" .

:WaterStorageProduct rdfs:label "Water Storage Product" .

:CADWRBulletin118%3AGroundwaterReport rdfs:label "CA DWR Bulletin 118: Groundwater Report" .

:CaliforniaDataExchangeCenter%28CDEC%29 rdfs:label "California Data Exchange Center (CDEC)" .

:DWRWaterDataLibrary%3ASurfaceWaterAndGroundwaterData rdfs:label "CA DWR Water Data Library: Surface Water and Groundwater Data" .

:GravityRecoveryAndClimateExperiment%28GRACE%29 rdfs:label "Gravity Recovery and Climate Experiment (GRACE)" .

:MassBalance rdfs:label "Mass Balance" .

:USGSCaliforniaWaterScienceCenter-GroundwaterModeling rdfs:label "USGS California Water Science Center - Groundwater Modeling" .

:ChangeInLakeStorage rdfs:label "Change in Lake Storage" .

:WaterBalanceForUnsaturatedZoneStorage rdfs:label "Water Balance for Unsaturated Zone Storage" .

:WaterUseModels rdfs:label "Water Use Models" .

:ChangeInPondedWaterStorage rdfs:label "Change in Ponded Water Storage" .

:ChangeInRootZoneSoilMoisture rdfs:label "Change in Root Zone Soil Moisture" .

:ChangeInSoilMoisture rdfs:label "Change in Soil Moisture" .

:ChangeInUnsaturatedZoneStorage rdfs:label "Change in Unsaturated Zone Storage" .

:HYDRODatabase rdfs:label "HYDRO Database" .

:WaterLevel rdfs:label "Water Level" .

:USBRCentralValleyProjectRefugeWaterDeliveryData rdfs:label "USBR Central Valley Project Refuge Water Delivery Data" .

:USGSSurface-WaterDataForCalifornia rdfs:label "USGS Surface-Water Data for California" .

:CenterForHydrometeorologyAndRemoteSensingDataPortal%28CHRS%29 rdfs:label "Center for Hydrometeorology and Remote Sensing Data Portal (CHRS)" .

:LakeInflowFromStreams-CA rdfs:label "Lake Inflow from Streams-CA" .

:LakeOutflowToStreams-CA rdfs:label "Lake Outflow to Streams-CA" .

:CityWestWaterAnnualReport rdfs:label "City West Water Annual Report" .

:ConstantPercentage rdfs:label "Constant Percentage" .

:ConstantSeepagePercentage rdfs:label "Constant Seepage Percentage" .

:NOAANationalCentersForEnvironmentalInformation-ClimateDataOnline rdfs:label "NOAA National Centers for Environmental Information - Climate Data Online" .

:NOAANationalCentersForEnvironmentalInformation-ClimatologicalDataPublications rdfs:label
    "NOAA National Centers for Environmental Information - Climatological Data Publications" .

:NWSCLIMATEPREDICTIONCENTEREVAPORATION rdfs:label "NWS Climate Prediction Center Evaporation" .

:CADWRBulletin132%3AManagementOfTheCaliforniaStateWaterProject rdfs:label "CA DWR Bulletin 132: Management of the California State Water Project" .

:CaliforniaIrrigationManagementInformationSystem%28CIMIS%29 rdfs:label "California Irrigation Management Information System (CIMIS)" .

:DWRBulletin73%3AEvaporationFromWaterSurfaceInCalifornia%281979%29 rdfs:label "CA DWR Bulletin 73: Evaporation from Water Surface in California (1979)" .

:Evapotranspiration%28ET%29Rates rdfs:label "Evapotranspiration (ET) Rates" .

:s.71WaterResourceReport rdfs:label "s.71 Water Resource Report" .

:EstimateConveyanceSeepageRateBasedOnCanalCharacteristics rdfs:label "Estimate Conveyance Seepage Rate based on Canal Characteristics" .

:CropCoefficientApproach rdfs:label "Crop Coefficient Approach" .

:CAIrrigationTrainingAndResearchCenter%28ITRC%29EvapotranspirationData rdfs:label
    "CA Irrigation Training and Research Center (ITRC) Evapotranspiration Data" .

:FAO56Chapter6SingleCropCoefficients%28Kc%29 rdfs:label "FAO 56 Chapter 6 Single Crop Coefficients (Kc)" .

:SpatialCaliforniaIrrigationManagementInformationSystem%28CIMIS%29 rdfs:label "Spatial California Irrigation Management Information System (CIMIS)" .

:ReferenceCropET%28ETo%29 rdfs:label "Reference Crop ET (ETo)" .

:CulturalPractices rdfs:label "Cultural Practices" .

:DataFromPrivateWetlandsOrDuckClubs rdfs:label "Data from Private Wetlands or Duck Clubs" .

:USFishAndWildlifeServices rdfs:label "US Fish and Wildlife Services (USFWS)" .

:CaliforniaDepartmentOfFishAndWildlife%28CDFW%29 rdfs:label "California Department of Fish and Wildlife (CDFW)" .

:CumulativeWaterMeter rdfs:label "Cumulative Water Meter" .

:CustomerMeters rdfs:label "Customer Meters" .

:SAWaterGISDatabase rdfs:label "SA Water GIS Database" .

:DWRGuideToEstimatingIrrigationWaterNeedsOfLandscapePlantingsInCalifornia1 rdfs:label
    "CA DWR Guide to Estimating Irrigation Water Needs of Landscape Plantings in California 1" .

:DWRPublicWaterSupplyStatisticsData-Historical rdfs:label "CA DWR Public Water Supply Statistics Data-Historical" .

:DailyMaxAndMinAirTemperature rdfs:label "Daily Max and Min Air Temperature" .

:DailyPrecipitation rdfs:label "Daily Precipitation" .

:DailyShort-WaveSolarRadiation rdfs:label "Daily Short-Wave Solar Radiation" .

:DailyWaterBalanceApproach rdfs:label "Daily Water Balance Approach" .

:DepartmentOfWaterAndEnvironmentalRegulation rdfs:label "Department of Water and Environmental Regulation" .

:DrainageAreaOfSiteOfInterest rdfs:label "Drainage area of site of interest (Ay)" .

:DrainageAreaRatioMethod rdfs:label "Drainage Area Ratio Method" .

:DrainageAreaOfStreamflowGagingStation%28Ax%29 rdfs:label "Drainage area of streamflow gaging station (Ax)" .

:MeasureStreamflow%28Xij%29 rdfs:label "Measure streamflow (Xij)" .

:EntitlementVolume rdfs:label "Entitlement Volume" .

:EstimateAppliedWaterReuseAndRecycledWaterVolumes rdfs:label "Estimate Applied Water Reuse and Recycled Water Volumes" .

:EstimatedNon-revenueWaterVolumes rdfs:label "Estimated non-revenue water volumes" .

:EstimationOfAbstraction rdfs:label "Estimation of Abstraction" .

:Morton%27sShallowLakeFormulation rdfs:label "Morton's Shallow Lake Formulation" .

:EvaporationPanMethod rdfs:label "Evaporation Pan Method" .

:MeasuredPanEvaporationRate rdfs:label "Measured Pan Evaporation Rate" .

:PanCoefficient rdfs:label "Pan Coefficient" .

:SurfaceAreaOfWaterBody rdfs:label "Surface Area of Water Body" .

:METRIC-EarthEngineEvapotranspirationFlux rdfs:label "METRIC-Earth Engine Evapotranspiration Flux" .

:USGSBasinCharacterizationModel rdfs:label "USGS Basin Characterization Model" .

:CADWRBulletin113%3ACropWaterUse rdfs:label "CA DWR Bulletin 113: Crop Water Use" .

:MOD16%3AMODISGlobalEvapotranspirationProject rdfs:label "MOD 16: MODIS Global Evapotranspiration Project" .

:NOAAOfficeOfSatelliteAndProductOperationsALEXI%3AAtmosphere-LandExchangeInverseModel
  rdfs:label "NOAA Office of Satellite and Product Operations ALEXI: Atmosphere-Land Exchange Inverse Model" .

:NorthAmericanLandDataAssimilationSystem%28NLDAS-2%29 rdfs:label "North American Land Data Assimilation System (NLDAS-2)" .

:OperationalSimplifiedSurfaceEnergyBalance%28SSEBop%29 rdfs:label "Operational Simplified Surface Energy Balance (SSEBop)" .

:TOPS-SIMS%3ASatelliteIrrigationManagementSupport rdfs:label "TOPS-SIMS: Satellite Irrigation Management Support" .

:FloodplainModule rdfs:label "Floodplain Module" .

:FlowData rdfs:label "Flow Data" .

:FlowNetAnalysis rdfs:label "Flow Net Analysis" .

:EffectiveThicknessOfTheAquifer%28b%29 rdfs:label "Effective thickness of the aquifer (b)" .

:FlowThroughAVerticalPlaneThatExtendsBeneathTheShorelineOfASurfaceWaterBody%28Q%29
  rdfs:label "Flow through a vertical plane that extends beneath the shoreline of a surface water body (Q)" .

:HorizonalHydraulicConductivityOfTheAquiferAtTheBoundary%28K%29 rdfs:label "Horizontal hydraulic conductivity of the aquifer at the boundary (K)" .

:NumberOfEquipotentialHeadDropsOverTheAreaOfInterest%28n%29 rdfs:label "Number of equipotential head drops over the area of interest (n)" .

:NumberOfStreamtubesAcrossAFlowNet%28M%29 rdfs:label "Number of streamtubes across a flow net (M)" .

:TotalHeadDropAcrossTheAreaOfInterest%28H%29 rdfs:label "Total head drop across the area of interest (H)" .

:GISGroundwaterModelling rdfs:label "GIS Groundwater Modelling" .

:PortPhillipCatchmentManagementAuthorityGroundwaterModel rdfs:label "Port Phillip Catchment Management Authority Groundwater Model" .

:GroundwaterLevel rdfs:label "Groundwater Level" .

:HydraulicConductivity rdfs:label "Hydraulic Conductivity" .

:Darcy%27sLaw rdfs:label "Darcy's Law" .

:GippslandWaterAnnualReport rdfs:label "Gippsland Water Annual Report" .

:Peel-HarveyRegionalAquiferModelingSystem%28PHRAMS%29 rdfs:label "Peel-Harvey Regional Aquifer Modeling System (PHRAMS)" .

:PerthRegionalAquiferModelingSystems%28PRAMS%29 rdfs:label "Perth Regional Aquifer Modeling Systems (PRAMS)" .

:LandUseAndAppliedWaterEstimationMethod rdfs:label "Applied Water Estimation Method" .

:LocalAgencyRecords rdfs:label "Local Agency Records" .

:CaliforniaDepartmentOfWaterResources%28DWR%29UrbanWaterSupplyStatistics rdfs:label
    "California Department of Water Resources (DWR) Urban Water Supply Statistics" .

:CaliforniaStateWaterResourcesControlBoard%28SWRCB%29UrbanWaterSupplyStatistics rdfs:label
    "California State Water Resources Control Board (SWRCB) Urban Water Supply Statistics" .

:GroundwaterExtractionUnderStatutoryRightsEstimationMethod rdfs:label "Groundwater Extraction Under Statutory Rights Estimation Method" .

:GroundwaterModelling rdfs:label "Groundwater Modelling" .

:HabitatAcreage rdfs:label "Habitat Acreage" .

:ExistingWaterRightInformationFromStateWaterResourcesControlBoard%28SWRCB%29 rdfs:label
    "Existing Water Right Information from State Water Resources Control Board (SWRCB)" .

:ManagedWetlandAppliedWater-CA rdfs:label "Managed Wetland Applied Water-CA" .

:OperationalSpill rdfs:label "Operational Spill" .

:UrbanAppliedWater-CA rdfs:label "Urban Applied Water-CA" .

:IndividualUserLicenses rdfs:label "Individual User Licenses" .

:KimberelyAgriculturalInvestment%3AGoomingFarmlands rdfs:label "Kimberely Agricultural Investment: Gooming Farmlands" .

:OrdIrrigationCooperative%3APacksaddleAndIvanhoePlains rdfs:label "Ord Irrigation Cooperative: Packsaddle and Ivanhoe Plains" .

:WaterCorporation%3AM1Channel rdfs:label "Water Corporation: M1 Channel" .

:IndustrialWaterUse rdfs:label "Industrial Water Use" .

:WaterUseSurveys rdfs:label "Water Use Surveys" .

:InflowFromContributingOrTributaryStreams rdfs:label "Inflow from contributing or tributary streams" .

:InflowToWaterTreatmentPlants rdfs:label "Inflow to Water Treatment Plants" .

:GeographicInformationSystem%28GIS%29 rdfs:label "Geographic information system (GIS)" .

:MassTransferEquations rdfs:label "Mass Transfer Equations" .

:MassTransferCoefficient rdfs:label "Mass Transfer Coefficient" .

:SaturationVaporPressure rdfs:label "Saturation Vapor Pressure " .

:WindFunction rdfs:label "Wind Function" .

:BottomElevationOfTheLakebedSediments%28HlakebedBottom%29 rdfs:label "Bottom elevation of the lakebed sediments (Hlakebed bottom)" .

:DistanceBetweenTwoPointsWithKnownHead%28I%29 rdfs:label "Distance between two points with known head (I)" .

:GroundwaterLevel%28Haquifer%29 rdfs:label "Groundwater Level (Haquifer)" .

:SurfaceAreaOfLake%28Al%29 rdfs:label "Surface area of lake (Al)" .

:VerticalHydraulicConductivityOfTheSurroundingAquifer%28Kv%29 rdfs:label "Vertical hydraulic conductivity of the surrounding aquifer (Kv)" .

:WaterLevelInLake%28Hlake%29 rdfs:label "Water level in lake (Hlake)" .

:WettedPerimeterOfLakeMultipliedByTheAverageSaturatedThicknessOfAquiferAroundTheLake%28Awpl%29
  rdfs:label "Wetted perimeter of lake multiplied by the average saturated thickness of aquifer around the lake (Awpl)" .

:USGSPublications rdfs:label "USGS Publications" .

:MassCurve rdfs:label "Mass Curve" .

:ReservoirOperationRuleCurve rdfs:label "Reservoir Operation Rule Curve" .

:ConsumptiveUseOfPrecipitation%28EP%29 rdfs:label "Consumptive Use of Precipitation (EP)" .

:LandscapeIrrigation rdfs:label "Landscape Irrigation" .

:LandscapeModelledRunoff rdfs:label "Landscape Modelled Runoff" .

:LyneAndHollickFilter rdfs:label "Lyne and Hollick Filter" .

:MIKE11 rdfs:label "MIKE 11" .

:MeteredWaterData rdfs:label "Metered Water Data" .

:USFWSAndCDFWRefugeWaterManagementPlans rdfs:label "USFWS and CDFW Refuge Water Management Plans" .

:ManagedWetlandsAppliedWaterEstimation rdfs:label "Managed Wetlands Applied Water Estimation" .

:UnitETOfAppliedWater rdfs:label "Unit ET of Applied Water" .

:StreamflowAtDownstreamGauge rdfs:label "Streamflow at downstream gauge" .

:StreamflowAtUpstreamGauge rdfs:label "Streamflow at upstream gauge" .

:MelbourneWaterAnnualReport rdfs:label "Melbourne Water Annual Report" .

:SnowyHydro rdfs:label "Snowy Hydro" .

:SouthEastWaterAnnualReport rdfs:label "South East Water Annual Report" .

:UltrasonicFlowMeters rdfs:label "Ultrasonic Flow Meters" .

:YarraValleyWaterAnnualReport rdfs:label "Yarra Valley Water Annual Report" .

:ModelledRunoff rdfs:label "Modelled Runoff" .

:MoretonAndLoganBasinResourceOperatingLicenses rdfs:label "Moreton and Logan Basin Resource Operating Licenses" .

:MunicipalWaterUseRecords rdfs:label "Municipal Water Use Records" .

:NetworkRealLossesAndApparentLossesModelingSoftware rdfs:label "Network real losses and apparent losses modeling software" .

:NewSouthWalesDepartmentOfWater rdfs:label "New South Wales Department of Water" .

:Observation rdfs:label "Observation" .

:OnsiteRe-useMeters rdfs:label "Onsite re-use meters" .

:OtherSupplySystemDecreases-AUS rdfs:label "Other Supply System Decreases-AUS" .

:RealLossesEquation rdfs:label "Real Losses Equation" .

:OtherWastewaterDecreases-AUS rdfs:label "Other Wastewater Decreases-AUS" .

:StreamGages rdfs:label "Stream Gages" .

:PopulationAndPer-CapitaWaterUse rdfs:label "Population and Per-Capita Water Use" .

:CentralValleySpatialDatabase-partOfTheCentralValleyHydrologicModel%5BCVHM%5DProject
  rdfs:label "Central Valley Spatial Database-part of the Central Valley Hydrologic Model [CVHM] project" .

:SpatialAveragingTechniques rdfs:label "Spatial Averaging Techniques" .

:PropertyAreaEstimationMethodsForSurfaceWaterDiversions rdfs:label "Property Area Estimation Methods for Surface Water Diversions" .

:Rainfall-RunoffMethod rdfs:label "Rainfall-Runoff Method" .

:UnmeteredAuthorisedConsumption rdfs:label "Unmetered Authorised Consumption" .

:RechargeAsPercentageOfRainfall rdfs:label "Recharge as percentage of rainfall" .

:RechargeCreditBalance rdfs:label "Recharge Credit Balance" .

:AUSDepartmentForEnvironmentAndWater%28DEW%29 rdfs:label "AUS Department for Environment and Water (DEW)" .

:WaterRecyclingSurvey%282015%29 rdfs:label "Water Recycling Survey (2015)" .

:ReportFromBowenBrokenAndBurdekinHaughtonWaterSupplySchemes rdfs:label "Report from Bowen Broken and Burdekin Haughton water supply schemes" .

:ResourceOperatingLicenseTables rdfs:label "Resource Operating License Tables" .

:ReturnFlowEstimationMethod rdfs:label "Return Flow Estimation Method" .

:RiparianWaterAuthorisations rdfs:label "Riparian Water Authorisations" .

:RiverAndGroundwaterInteractionModule rdfs:label "River and Groundwater Interaction Module" .

:RiverLosses-AUS rdfs:label "River Losses-AUS" .

:CaliforniaDepartmentOfTransportation%27sHighwayDesignManual rdfs:label "California Department of Transportation's Highway Design Manual" .

:RunoffCurveNumberMethod rdfs:label "Runoff Curve Number Method" .

:U.C.DavisSoilResourceLab rdfs:label "U.C. Davis Soil Resource Lab" .

:Precipitation-RunoffModelingSystem%28PRMS%29 rdfs:label "USGS Precipitation-Runoff Modeling System (PRMS)" .

:PublicPolicyInstituteOfCalifornia%28PPIC%29Map rdfs:label "Public Policy Institute of California (PPIC) map" .

:SAWaterStorageVolumeRelationship rdfs:label "SA Water Storage Volume Relationship" .

:SWRCBElectronicAnnualReport rdfs:label "SWRCB Electronic Annual Report" .

:SWRCBMonthlyUrbanWaterProductionReporting rdfs:label "SWRCB Monthly Urban Water Production Reporting" .

:Seqwater rdfs:label "Seqwater" .

:SpatialAssessments rdfs:label "Spatial Assessments" .

:AverageThicknessOfStreambed%28Bstream%29 rdfs:label "Average thickness of streambed (Bstream)" .

:BottomElevationOfStreambedSediments%28HstreambedBottom%29 rdfs:label "Bottom Elevation of Streambed Sediments (Hstreambed bottom)" .

:EffectiveAreaOfFlowExchange%28Awps%29 rdfs:label "Effective area of flow exchange (Awps)" .

:HydraulicConductivityOfTheStreambedMaterial%28Ks%29 rdfs:label "Hydraulic conductivity of the streambed material (Ks)" .

:WaterStageInStream%28Hstream%29 rdfs:label "Water Stage in stream (Hstream)" .

:USGSDR3M rdfs:label "USGS DR3M" .

:WaterResourceAssociatesHYSIM rdfs:label "Water Resource Associates HYSIM" .

<http://purl.org/iow/WaterBudgetingFramework/UniversityOfWashington%E2%80%99sVariableInfiltrationCapacityModel%28VIC%29.>
  rdfs:label "University of Washingtons Variable Infiltration Capacity Model (VIC)." .

:Vieux%26Associates%27Vflo rdfs:label "Vieux & Associates' Vflo" .

:DescriptiveDataOfTopography%2CSoils%2CAndVegetation rdfs:label "Descriptive Data of Topography, Soils, and Vegetation" .

:Cross-sectionalAreaSubjectToBoundaryFlow%28Ab%29 rdfs:label "Cross-sectional area subject to boundary flow (Ab)" .

:DepthOfCrossSection%28b%29 rdfs:label "Depth of cross section (b)" .

:HydraulicConductivityOfTheAquiferBoundary%28K%29 rdfs:label "Hydraulic conductivity of the aquifer boundary (K)" .

:HydraulicGradientThroughTheCrossSection%28i%29 rdfs:label "Hydraulic gradient through the cross section (i)" .

:KnownGroundwaterElevationInsideTheBoundary%28hg%29 rdfs:label "Known groundwater elevation inside the boundary (hg)" .

:KnownGroundwaterElevationOutsideTheBoundary%28hb%29 rdfs:label "Known groundwater elevation outside the boundary (hb)" .

:SubsurfaceFlowAcrossTheBoundary%28Qb%29 rdfs:label "Subsurface flow across the boundary (Qb)" .

:TransmissivityOfTheAquiferAtTheBoundary%28T%29 rdfs:label "Transmissivity of the Aquifer at the boundary (T)" .

:WidthOfCrossSection%28w%29 rdfs:label "Width of cross section (w)" .

:SurplusIrrigationAssumption rdfs:label "Surplus Irrigation Assumption" .

:USGSExtensometer rdfs:label "USGS Extensometer" .

:VerticalFluxModel rdfs:label "Vertical Flux Model" .

:VirginiaPipelineSchemePumpStation rdfs:label "Virginia Pipeline Scheme pump station" .

:WaterAllocationPlans rdfs:label "Water Allocation Plans" .

:WaterCorporationSurveys rdfs:label "Water Corporation Surveys" .

:WaterSharingPlanForTheGreaterMetropolitanRegionUnregulatedRiverWaterSources rdfs:label
    "Water Sharing Plan for the Greater Metropolitan Region Unregulated River Water Sources" .

:WaterSharingPlanForTheKangarooRiverWaterSource rdfs:label "Water Sharing Plan for the Kangaroo River Water Source" .

:WaterTableFluctuationModelling rdfs:label "Water table fluctuation modelling" .

:WillungaBasinWaterCompany rdfs:label "Willunga Basin Water Company" .

:syde rdfs:label "syde" .

:yara rdfs:label "yara" .

:WaterIndustryLicensingManagementDatabase%28WILMA%29 rdfs:label "Water Industry Licensing Management Database (WILMA)" .

:SupervisoryControlAndDataAcquisitions%28SCADA%29 rdfs:label "Supervisory Control and Data Acquisitions (SCADA)" .

:CARecycledWaterDataFromLocal%2FMunicipalWaterSuppliers rdfs:label "CA Recycled Water Data from Local/Municipal Water Suppliers" .

:BarossaInfrastructureLimited%28BIL%29AnnualReport rdfs:label "Barossa Infrastructure Limited (BIL) Annual Report" .

:FiniteElementSubsurfaceFlowSystem%28FEFLOW%29 rdfs:label "Finite Element Subsurface Flow system (FEFLOW)" .

:WaterTrackingAndElectronicReportingSystem%28WaTERS%29 rdfs:label "Water Tracking and Electronic Reporting System (WaTERS)" .

:Losses%3AManagementOfTreatedWater-AUS rdfs:label "Losses: Management of Treated Water-AUS" .

:Losses%3AWastewaterTreatmentSystem-AUS rdfs:label "Losses: Wastewater Treatment System-AUS" .

:Non-allocatedDiversion%3AUrbanWaterSystemEstimationMethod rdfs:label "Non-allocated diversion: urban water system estimation method" .

:SAWater%27sTotalLicensedDiversionVolumeFromWesternMountLoftyRangesPWRA rdfs:label
    "SA Water's Total Licensed Diversion Volume from Western Mount Lofty Ranges PWRA" .

:RecycledWaterDelivery%3AIrrigation-AUS rdfs:label "Recycled Water Delivery: Irrigation-AUS" .

:SupplySystemDelivery%3AIrrigation-AUS rdfs:label "Supply System Delivery: Irrigation-AUS" .

:SupplySystemDischarge%3ASurfaceWater-AUS rdfs:label "Supply System Discharge: Surface Water-AUS" .

:WastewaterAndRecycledWaterDischarge%3ASurfaceWater-AUS rdfs:label "Wastewater and Recycled Water Discharge: Surface Water-AUS" .

:WastewaterDischarge%3ASurfaceWater-AUS rdfs:label "Wastewater Discharge: Surface Water-AUS" .

rdf:type rdfs:isDefinedBy <http://www.w3.org/1999/02/22-rdf-syntax-ns#> .

rdf:Property rdfs:isDefinedBy <http://www.w3.org/1999/02/22-rdf-syntax-ns#> .

rdfs:Class rdfs:isDefinedBy <http://www.w3.org/2000/01/rdf-schema#> .

rdfs:Resource rdfs:isDefinedBy <http://www.w3.org/2000/01/rdf-schema#> .

rdfs:subPropertyOf rdfs:isDefinedBy <http://www.w3.org/2000/01/rdf-schema#> .

rdfs:subClassOf rdfs:isDefinedBy <http://www.w3.org/2000/01/rdf-schema#> .

rdfs:domain rdfs:isDefinedBy <http://www.w3.org/2000/01/rdf-schema#> .

rdfs:range rdfs:isDefinedBy <http://www.w3.org/2000/01/rdf-schema#> .

owl:sameAs rdfs:isDefinedBy <http://www.w3.org/2002/07/owl#> .

owl:SymmetricProperty rdfs:isDefinedBy <http://www.w3.org/2002/07/owl#> .

owl:TransitiveProperty rdfs:isDefinedBy <http://www.w3.org/2002/07/owl#> .

owl:equivalentProperty rdfs:isDefinedBy <http://www.w3.org/2002/07/owl#> .

owl:equivalentClass rdfs:isDefinedBy <http://www.w3.org/2002/07/owl#> .

rdfs:Datatype rdfs:isDefinedBy <http://www.w3.org/2000/01/rdf-schema#> .

owl:intersectionOf rdfs:isDefinedBy <http://www.w3.org/2002/07/owl#> .

owl:FunctionalProperty rdfs:isDefinedBy <http://www.w3.org/2002/07/owl#> .

rdfs:ContainerMembershipProperty rdfs:isDefinedBy <http://www.w3.org/2000/01/rdf-schema#> .

owl:someValuesFrom rdfs:isDefinedBy <http://www.w3.org/2002/07/owl#> .

owl:allValuesFrom rdfs:isDefinedBy <http://www.w3.org/2002/07/owl#> .

owl:inverseOf rdfs:isDefinedBy <http://www.w3.org/2002/07/owl#> .

rdfs:member rdfs:isDefinedBy <http://www.w3.org/2000/01/rdf-schema#> .

owl:hasValue rdfs:isDefinedBy <http://www.w3.org/2002/07/owl#> .

rdf:first rdfs:isDefinedBy <http://www.w3.org/1999/02/22-rdf-syntax-ns#> .

owl:onProperty rdfs:isDefinedBy <http://www.w3.org/2002/07/owl#> .

rdf:rest rdfs:isDefinedBy <http://www.w3.org/1999/02/22-rdf-syntax-ns#> .

owl:InverseFunctionalProperty rdfs:isDefinedBy <http://www.w3.org/2002/07/owl#> .

rdfs:Literal rdfs:isDefinedBy <http://www.w3.org/2000/01/rdf-schema#> .

rdf:nil rdfs:isDefinedBy <http://www.w3.org/1999/02/22-rdf-syntax-ns#> .

rdf:subject rdfs:isDefinedBy <http://www.w3.org/1999/02/22-rdf-syntax-ns#> .

rdf:predicate rdfs:isDefinedBy <http://www.w3.org/1999/02/22-rdf-syntax-ns#> .

rdf:object rdfs:isDefinedBy <http://www.w3.org/1999/02/22-rdf-syntax-ns#> .

rdf:value rdfs:isDefinedBy <http://www.w3.org/1999/02/22-rdf-syntax-ns#> .

rdf:List rdfs:isDefinedBy <http://www.w3.org/1999/02/22-rdf-syntax-ns#> .

rdf:Statement rdfs:isDefinedBy <http://www.w3.org/1999/02/22-rdf-syntax-ns#> .

rdfs:comment rdfs:isDefinedBy <http://www.w3.org/2000/01/rdf-schema#> .

rdfs:label rdfs:isDefinedBy <http://www.w3.org/2000/01/rdf-schema#> .

rdf:Alt rdfs:isDefinedBy <http://www.w3.org/1999/02/22-rdf-syntax-ns#> .

rdfs:Container rdfs:isDefinedBy <http://www.w3.org/2000/01/rdf-schema#> .

rdf:Bag rdfs:isDefinedBy <http://www.w3.org/1999/02/22-rdf-syntax-ns#> .

rdf:Seq rdfs:isDefinedBy <http://www.w3.org/1999/02/22-rdf-syntax-ns#> .

rdfs:isDefinedBy rdfs:isDefinedBy <http://www.w3.org/2000/01/rdf-schema#> .

rdfs:seeAlso rdfs:isDefinedBy <http://www.w3.org/2000/01/rdf-schema#> .

rdf:XMLLiteral rdfs:isDefinedBy <http://www.w3.org/1999/02/22-rdf-syntax-ns#> .

owl:differentFrom rdfs:isDefinedBy <http://www.w3.org/2002/07/owl#> .

owl:Ontology rdfs:isDefinedBy <http://www.w3.org/2002/07/owl#> .

rdf:HTML rdfs:isDefinedBy <http://www.w3.org/1999/02/22-rdf-syntax-ns#> .

rdf:langString rdfs:isDefinedBy <http://www.w3.org/1999/02/22-rdf-syntax-ns#> .

rdf:PlainLiteral rdfs:isDefinedBy <http://www.w3.org/1999/02/22-rdf-syntax-ns#> .

<http://www.w3.org/2002/07/owl> rdfs:isDefinedBy <http://www.w3.org/TR/owl2-mapping-to-rdf/>,
    <http://www.w3.org/TR/owl2-rdf-based-semantics/>, <http://www.w3.org/TR/owl2-syntax/> .

owl:versionIRI rdfs:isDefinedBy <http://www.w3.org/2002/07/owl#> .

owl:imports rdfs:isDefinedBy <http://www.w3.org/2002/07/owl#> .

owl:versionInfo rdfs:isDefinedBy <http://www.w3.org/2002/07/owl#> .

owl:AllDifferent rdfs:isDefinedBy <http://www.w3.org/2002/07/owl#> .

owl:AllDisjointClasses rdfs:isDefinedBy <http://www.w3.org/2002/07/owl#> .

owl:AllDisjointProperties rdfs:isDefinedBy <http://www.w3.org/2002/07/owl#> .

owl:Annotation rdfs:isDefinedBy <http://www.w3.org/2002/07/owl#> .

owl:AnnotationProperty rdfs:isDefinedBy <http://www.w3.org/2002/07/owl#> .

owl:AsymmetricProperty rdfs:isDefinedBy <http://www.w3.org/2002/07/owl#> .

owl:ObjectProperty rdfs:isDefinedBy <http://www.w3.org/2002/07/owl#> .

owl:Axiom rdfs:isDefinedBy <http://www.w3.org/2002/07/owl#> .

owl:Class rdfs:isDefinedBy <http://www.w3.org/2002/07/owl#> .

owl:DataRange rdfs:isDefinedBy <http://www.w3.org/2002/07/owl#> .

owl:DatatypeProperty rdfs:isDefinedBy <http://www.w3.org/2002/07/owl#> .

owl:DeprecatedClass rdfs:isDefinedBy <http://www.w3.org/2002/07/owl#> .

owl:DeprecatedProperty rdfs:isDefinedBy <http://www.w3.org/2002/07/owl#> .

owl:IrreflexiveProperty rdfs:isDefinedBy <http://www.w3.org/2002/07/owl#> .

owl:NamedIndividual rdfs:isDefinedBy <http://www.w3.org/2002/07/owl#> .

owl:Thing rdfs:isDefinedBy <http://www.w3.org/2002/07/owl#> .

owl:NegativePropertyAssertion rdfs:isDefinedBy <http://www.w3.org/2002/07/owl#> .

owl:Nothing rdfs:isDefinedBy <http://www.w3.org/2002/07/owl#> .

owl:OntologyProperty rdfs:isDefinedBy <http://www.w3.org/2002/07/owl#> .

owl:ReflexiveProperty rdfs:isDefinedBy <http://www.w3.org/2002/07/owl#> .

owl:Restriction rdfs:isDefinedBy <http://www.w3.org/2002/07/owl#> .

owl:annotatedProperty rdfs:isDefinedBy <http://www.w3.org/2002/07/owl#> .

owl:annotatedSource rdfs:isDefinedBy <http://www.w3.org/2002/07/owl#> .

owl:annotatedTarget rdfs:isDefinedBy <http://www.w3.org/2002/07/owl#> .

owl:assertionProperty rdfs:isDefinedBy <http://www.w3.org/2002/07/owl#> .

owl:backwardCompatibleWith rdfs:isDefinedBy <http://www.w3.org/2002/07/owl#> .

owl:bottomDataProperty rdfs:isDefinedBy <http://www.w3.org/2002/07/owl#> .

owl:bottomObjectProperty rdfs:isDefinedBy <http://www.w3.org/2002/07/owl#> .

owl:cardinality rdfs:isDefinedBy <http://www.w3.org/2002/07/owl#> .

owl:complementOf rdfs:isDefinedBy <http://www.w3.org/2002/07/owl#> .

owl:datatypeComplementOf rdfs:isDefinedBy <http://www.w3.org/2002/07/owl#> .

owl:deprecated rdfs:isDefinedBy <http://www.w3.org/2002/07/owl#> .

owl:disjointUnionOf rdfs:isDefinedBy <http://www.w3.org/2002/07/owl#> .

owl:disjointWith rdfs:isDefinedBy <http://www.w3.org/2002/07/owl#> .

owl:distinctMembers rdfs:isDefinedBy <http://www.w3.org/2002/07/owl#> .

owl:hasKey rdfs:isDefinedBy <http://www.w3.org/2002/07/owl#> .

owl:hasSelf rdfs:isDefinedBy <http://www.w3.org/2002/07/owl#> .

owl:incompatibleWith rdfs:isDefinedBy <http://www.w3.org/2002/07/owl#> .

owl:maxCardinality rdfs:isDefinedBy <http://www.w3.org/2002/07/owl#> .

owl:maxQualifiedCardinality rdfs:isDefinedBy <http://www.w3.org/2002/07/owl#> .

owl:members rdfs:isDefinedBy <http://www.w3.org/2002/07/owl#> .

owl:minCardinality rdfs:isDefinedBy <http://www.w3.org/2002/07/owl#> .

owl:minQualifiedCardinality rdfs:isDefinedBy <http://www.w3.org/2002/07/owl#> .

owl:onClass rdfs:isDefinedBy <http://www.w3.org/2002/07/owl#> .

owl:onDataRange rdfs:isDefinedBy <http://www.w3.org/2002/07/owl#> .

owl:onDatatype rdfs:isDefinedBy <http://www.w3.org/2002/07/owl#> .

owl:oneOf rdfs:isDefinedBy <http://www.w3.org/2002/07/owl#> .

owl:onProperties rdfs:isDefinedBy <http://www.w3.org/2002/07/owl#> .

owl:priorVersion rdfs:isDefinedBy <http://www.w3.org/2002/07/owl#> .

owl:propertyChainAxiom rdfs:isDefinedBy <http://www.w3.org/2002/07/owl#> .

owl:propertyDisjointWith rdfs:isDefinedBy <http://www.w3.org/2002/07/owl#> .

owl:qualifiedCardinality rdfs:isDefinedBy <http://www.w3.org/2002/07/owl#> .

owl:sourceIndividual rdfs:isDefinedBy <http://www.w3.org/2002/07/owl#> .

owl:targetIndividual rdfs:isDefinedBy <http://www.w3.org/2002/07/owl#> .

owl:targetValue rdfs:isDefinedBy <http://www.w3.org/2002/07/owl#> .

owl:topDataProperty rdfs:isDefinedBy <http://www.w3.org/2002/07/owl#> .

owl:topObjectProperty rdfs:isDefinedBy <http://www.w3.org/2002/07/owl#> .

owl:unionOf rdfs:isDefinedBy <http://www.w3.org/2002/07/owl#> .

owl:withRestrictions rdfs:isDefinedBy <http://www.w3.org/2002/07/owl#> .

skos:Concept rdfs:isDefinedBy <http://www.w3.org/2004/02/skos/core>;
  skos:definition "An idea or notion; a unit of thought."@en .

skos:definition rdfs:isDefinedBy <http://www.w3.org/2004/02/skos/core>;
  skos:definition "A statement or formal explanation of the meaning of a concept."@en .

skos:ConceptScheme rdfs:isDefinedBy <http://www.w3.org/2004/02/skos/core>;
  owl:disjointWith skos:Concept;
  skos:definition "A set of concepts, optionally including statements about semantic relationships between those concepts."@en .

skos:scopeNote rdfs:isDefinedBy <http://www.w3.org/2004/02/skos/core>;
  skos:definition "A note that helps to clarify the meaning and/or the use of a concept."@en .

skos:example rdfs:isDefinedBy <http://www.w3.org/2004/02/skos/core>;
  skos:definition "An example of the use of a concept."@en .

skos:Collection rdfs:isDefinedBy <http://www.w3.org/2004/02/skos/core>;
  owl:disjointWith skos:Concept, skos:ConceptScheme;
  skos:definition "A meaningful collection of concepts."@en .

skos:OrderedCollection rdfs:isDefinedBy <http://www.w3.org/2004/02/skos/core>;
  skos:definition "An ordered collection of concepts, where both the grouping and the ordering are meaningful."@en .

skos:inScheme rdfs:isDefinedBy <http://www.w3.org/2004/02/skos/core>;
  skos:definition "Relates a resource (for example a concept) to a concept scheme in which it is included."@en .

skos:hasTopConcept rdfs:isDefinedBy <http://www.w3.org/2004/02/skos/core>;
  skos:definition "Relates, by convention, a concept scheme to a concept which is topmost in the broader/narrower concept hierarchies for that scheme, providing an entry point to these hierarchies."@en .

skos:topConceptOf rdfs:isDefinedBy <http://www.w3.org/2004/02/skos/core>;
  skos:definition "Relates a concept to the concept scheme that it is a top level concept of."@en .

skos:prefLabel rdfs:isDefinedBy <http://www.w3.org/2004/02/skos/core>;
  skos:definition "The preferred lexical label for a resource, in a given language."@en .

skos:altLabel rdfs:isDefinedBy <http://www.w3.org/2004/02/skos/core>;
  skos:definition "An alternative lexical label for a resource."@en .

skos:hiddenLabel rdfs:isDefinedBy <http://www.w3.org/2004/02/skos/core>;
  skos:definition "A lexical label for a resource that should be hidden when generating visual displays of the resource, but should still be accessible to free text search operations."@en .

skos:notation rdfs:isDefinedBy <http://www.w3.org/2004/02/skos/core>;
  skos:definition "A notation, also known as classification code, is a string of characters such as \"T58.5\" or \"303.4833\" used to uniquely identify a concept within the scope of a given concept scheme."@en .

skos:note rdfs:isDefinedBy <http://www.w3.org/2004/02/skos/core>;
  skos:definition "A general note, for any purpose."@en .

skos:changeNote rdfs:isDefinedBy <http://www.w3.org/2004/02/skos/core>;
  skos:definition "A note about a modification to a concept."@en .

skos:editorialNote rdfs:isDefinedBy <http://www.w3.org/2004/02/skos/core>;
  skos:definition "A note for an editor, translator or maintainer of the vocabulary."@en .

skos:historyNote rdfs:isDefinedBy <http://www.w3.org/2004/02/skos/core>;
  skos:definition "A note about the past state/use/meaning of a concept."@en .

skos:semanticRelation rdfs:isDefinedBy <http://www.w3.org/2004/02/skos/core>;
  skos:definition "Links a concept to a concept related by meaning."@en .

skos:broader rdfs:isDefinedBy <http://www.w3.org/2004/02/skos/core>;
  skos:definition "Relates a concept to a concept that is more general in meaning."@en .

skos:broaderTransitive rdfs:isDefinedBy <http://www.w3.org/2004/02/skos/core>;
  skos:definition "skos:broaderTransitive is a transitive superproperty of skos:broader." .

skos:narrower rdfs:isDefinedBy <http://www.w3.org/2004/02/skos/core>;
  skos:definition "Relates a concept to a concept that is more specific in meaning."@en .

skos:narrowerTransitive rdfs:isDefinedBy <http://www.w3.org/2004/02/skos/core>;
  skos:definition "skos:narrowerTransitive is a transitive superproperty of skos:narrower." .

skos:related rdfs:isDefinedBy <http://www.w3.org/2004/02/skos/core>;
  skos:definition "Relates a concept to a concept with which there is an associative semantic relationship."@en .

skos:member rdfs:isDefinedBy <http://www.w3.org/2004/02/skos/core>;
  skos:definition "Relates a collection to one of its members."@en .

skos:memberList rdfs:isDefinedBy <http://www.w3.org/2004/02/skos/core>;
  skos:definition "Relates an ordered collection to the RDF list containing its members."@en .

skos:mappingRelation rdfs:isDefinedBy <http://www.w3.org/2004/02/skos/core>;
  skos:definition "Relates two concepts coming, by convention, from different schemes, and that have comparable meanings"@en .

skos:broadMatch rdfs:isDefinedBy <http://www.w3.org/2004/02/skos/core>;
  skos:definition "skos:broadMatch is used to state a hierarchical mapping link between two conceptual resources in different concept schemes."@en .

skos:narrowMatch rdfs:isDefinedBy <http://www.w3.org/2004/02/skos/core>;
  skos:definition "skos:narrowMatch is used to state a hierarchical mapping link between two conceptual resources in different concept schemes."@en .

skos:relatedMatch rdfs:isDefinedBy <http://www.w3.org/2004/02/skos/core>;
  skos:definition "skos:relatedMatch is used to state an associative mapping link between two conceptual resources in different concept schemes."@en .

skos:exactMatch rdfs:isDefinedBy <http://www.w3.org/2004/02/skos/core>;
  skos:definition "skos:exactMatch is used to link two concepts, indicating a high degree of confidence that the concepts can be used interchangeably across a wide range of information retrieval applications. skos:exactMatch is a transitive property, and is a sub-property of skos:closeMatch."@en .

skos:closeMatch rdfs:isDefinedBy <http://www.w3.org/2004/02/skos/core>;
  skos:definition "skos:closeMatch is used to link two concepts that are sufficiently similar that they can be used interchangeably in some information retrieval applications. In order to avoid the possibility of \"compound errors\" when combining mappings across more than two concept schemes, skos:closeMatch is not declared to be a transitive property."@en .

:CA rdfs:isDefinedBy "Handbook for Water Budget Development With or Without Models. California Deparment of Water Resources. Draft April 2019" .

<http://www.w3.org/1999/02/22-rdf-syntax-ns#> dc:description "This is the RDF Schema for the RDF vocabulary terms in the RDF Namespace, defined in RDF 1.1 Concepts.";
  dc:title "The RDF Concepts Vocabulary (RDF)";
  rdfs:seeAlso <http://www.w3.org/2000/01/rdf-schema-more> .

rdf:HTML rdfs:seeAlso <http://www.w3.org/TR/rdf11-concepts/#section-html> .

rdf:langString rdfs:seeAlso <http://www.w3.org/TR/rdf11-concepts/#section-Graph-Literal> .

rdf:PlainLiteral rdfs:seeAlso <http://www.w3.org/TR/rdf-plain-literal/> .

<http://www.w3.org/2002/07/owl> dc:title "The OWL 2 Schema vocabulary (OWL 2)";
  rdfs:seeAlso <http://www.w3.org/TR/owl2-rdf-based-semantics/#table-axiomatic-classes>,
    <http://www.w3.org/TR/owl2-rdf-based-semantics/#table-axiomatic-properties>;
  owl:imports <http://www.w3.org/2000/01/rdf-schema>;
  owl:versionIRI <http://www.w3.org/2002/07/owl>;
  owl:versionInfo "$Date: 2009/11/15 10:54:12 $";
  grddl:namespaceTransformation <http://dev.w3.org/cvsweb/2009/owl-grddl/owx2rdf.xsl> .

<http://www.w3.org/2000/01/rdf-schema#> dc:title "The RDF Schema vocabulary (RDFS)";
  rdfs:seeAlso <http://www.w3.org/2000/01/rdf-schema-more> .

<http://www.w3.org/2004/02/skos/core> dct:contributor "Dave Beckett", "Nikki Rogers",
    "Participants in W3C's Semantic Web Deployment Working Group.";
  dct:creator "Alistair Miles", "Sean Bechhofer";
  dct:description "An RDF vocabulary for describing the basic structure and content of concept schemes such as thesauri, classification schemes, subject heading lists, taxonomies, 'folksonomies', other types of controlled vocabulary, and also concept schemes embedded in glossaries and terminologies."@en;
  dct:title "SKOS Vocabulary"@en;
  rdfs:seeAlso <http://www.w3.org/TR/skos-reference/> .

:Mining%3AReported-NMOSE dc:description "Before opening any mining operation, the operator must register the mine, mill, smelter, or pit with the Mining and Minerals Division of the New Mexico Energy, Minerals, and Natural Resources Department. A directory of all of the mining facilities registered in the state is updated annually." .

:METRIC-EarthEngineEvapotranspirationFlux dc:description """EEFlux (Earth Engine Evapotranspiration Flux) is a version of
METRIC that operates on the Google Earth Engine system. The
model METRIC, Mapping Evapotranspiration at High Resolution
with Internalized Calibration, uses satellite-based image
processing to calculate actual ET (ETa). Landsat satellite images
are used to calculate actual ET as a residual of the surface
energy balance. EEFlux uses North American Land Data
Assimilation System (NLDAS) and GridMET gridded weather
data to calibrate the surface energy balance in the US. The
model also uses STATSGO soils data, National Land Cover
Database (NLCD) land use data, PRISM precipitation data, and
USGS Digital Elevation Models (DEMs).""" .

:PublicPolicyInstituteOfCalifornia%28PPIC%29Map dc:description """The Public Policy Institute of California (PPIC) published a map of relative runoff as a percentage of annual runoff. The map uses data from PRISM, CIMIS, and the U.C. Davis Soil Resource Laboratory. The description states that the map shows the distribution of runoff  the amount of local precipitation that flows into
streams and recharges groundwater. Relative runoff is depicted as a percentage of annual runoff, calculated by adjusting average monthly precipitation (PRISM 19702000) by losses to soil storage capacity (U.C. Davis Soil Resource Laboratory, Beaudette, and OGeen) and average monthly reference ET (CIMIS 20002005, Hart).""" .

:flowSink skos:definition "Location where the flow is going" .

:flowSource skos:definition "Location where flow is coming from" .

:isPartialSubComponentOf skos:definition "a part of the subject component is accounted for by the object component" .

:isSubComponentOf skos:definition "the entirety of the subject is accounted for within the object component" .

:usedBy skos:definition "The State (or Federal Agency) that uses this element in a formalized water budgeting calculation or process" .

:AgriculturalAndMunicipalDepletions-UT skos:definition "Water from surface or groundwater supplied for municipal and agricultural uses provided through a municipal distribution system that is consumed by agriculture and municipal use and does not return to a natural water source or another body of water." .

:CropConsumptiveUse-CO skos:definition "Amount of water that does not return to its source after it has been diverted and put to beneficial use by agriculture." .

:GroundwaterExtraction-CA skos:definition """Volume of groundwater pumped (extracted) from the underlying
aquifer(s) for use within the water budget zone. It does not include
groundwater export, stored water extraction, and stored water export.""" .

:LivestockConsumptiveUse-CO skos:definition "Amount of water that does not return to its source after it has been diverted and put to beneficial use by livestock." .

:MunicipalAndIndustrialConsumptiveUse-CO skos:definition "Amount of water that does not return to its source after it has been diverted and put to beneficial use by municipal and industrial use." .

:MunicipalConsumptiveUse-WY skos:definition """Municipal water use is water supplied by a municipality for personal, commercial, and other purposes. Municipal water use is principally
driven by the number of people living and working in a community.""" .

:MunicipalTotalUse-WY skos:definition """Municipal water use is water supplied by a municipality for personal, commercial, and other purposes. Municipal water use is principally
driven by the number of people living and working in a community.""" .

:SurfaceWaterDiversions-CA skos:definition """Volume of water taken from the surface water system within a water
budget zone for use within the zone.""" .

:AgriculturalAndMunicipalDiversions-UT skos:definition "Water from surface or groundwater supplied for municipal and agricultural uses provided through a municipal distribution system that remains in the budget zone" .

:AppliedWater-CA skos:definition """Volume of water delivered to the intake of a city water system, a factory, a
farm headgate, managed wetlands, or managed aquifer recharge; it
includes all sources of supply (surface water, groundwater, applied water
reuse, and recycled water).""" .

:UTDiversionRecordsFromRiverCommissioners skos:definition "The Utah Division of Water Rights (UDWR) regulates the appropriation and distribution of water in the State of Utah. Some basins maintain surface water diversion records using automated recorders and field readings. Commissioners responsible for maintaining diversion records are hired by the State Engineer; however assigned commissioners are requested by, and funded by, the water users in each subbasin. For basins with commissioners, it often takes 2 to 3 years for collected diversion records to be provided to the State. In general, few diversions are recorded in the Green River and Colorado River basins in Utah." .

:USGSStreamStats skos:definition "For estimating inflow in ungaged basins" .

:UTDivisionOfWaterResourcesArea-AltitudeMethod skos:definition "For estimating inflow in ungaged basins" .

:Evapotranspiration-CA skos:definition """Volume of water entering the atmosphere through the combined process
of evaporation from soil and plant surfaces and transpiration from plants.""" .

:AgriculturalDepletions-UT skos:definition "Portion of water withdrawn from a surface or groundwater source that is consumed by agriculture and does not return to a natural water source or another body of water." .

:SurfaceDiversionToCropland-UT skos:definition "All land area diversions other than groundwater" .

:AgriculturalPotentialConsumptiveUse-UT skos:definition "Portion of water withdrawn from a surface or groundwater source that is might be consumed by agriculture and might not return to a natural water source or another body of water. This could include consumptive use and return flow." .

:PRISM skos:definition """PRISM (Parameter elevation Regression on Independent Slopes
Model) Gridded Precipitation is the result of sophisticated
climatological modeling of a large network of historic and active
weather stations and radar data. The PRISM model accounts for
complex climatological factors including orography, rain
shadows, temperature inversions, slope aspect, coastal
proximity, and others. PRISM climate data are widely used for
modeling and analysis at multiple scales.""" .

:DailyPenman-Monteith skos:definition "The Penman-Monteith method for determining daily reference crop ET uses minimum and maximum temperature, vapor pressure, solar radiation and wind run data. Reference crop ET for alfalfa is the rate at which water, if available, is removed by the processes of evaporation and transpiration from soil and plant surfaces expressed as the depth of water used by a standard reference crop per unit time." .

:ModifiedBlaney-Criddle skos:definition """The procedure used to calculate the final monthly consumptive use coefficient (k) distinguishes
the MBC method from the OBC method, which uses a seasonal consumptive use coefficient.""" .

:ClimateCoefficient%28kt%29 skos:definition "Climatic coefficients that are directly related to the mean air temperature for each of the consecutive short periods which constitutes the growing season",
    "The climatic coefficient (kt) equals 0.0173t-0.314" .

:MonthlyEvaporation skos:definition "The net evaporation rate for each month, expressed as a depth of water in feet, is calculated by subtracting the measured rainfall, in feet, from the gross evaporation rate." .

:AreaOutflows skos:definition "Volume of water leaving through rivers at the periphery of a water budget zone" .

:BasinOutflow-UT skos:definition "Volume of water leaving through rivers at the periphery of a water budget zone" .

:StreamOutfow-CA skos:definition """Volume of water leaving through streams at the periphery of a water
budget zone.""" .

:Exports-CO skos:definition "Water exported from the water budget zone as surface or groundwater" .

:AverageMonthlyReservoirGageHeight skos:definition "Compute the average gage height of the water surface level, or the average reservoir content for each month, from daily measurements reported by the agency responsible for managing the reservoir. Sources of data include the NMISC, the U.S. Army Corps of Engineers, the USBR, the USGS, the National Oceanic and Atmospheric Administration (NOAA), and irrigation districts." .

:Baseflow skos:definition """Base flow data is used by the baseflow module to estimate base flows at river nodes that do not have
hisoric records using the following formula:""" .

:BasinInflow-UT skos:definition "Volume of water entering through rivers at the periphery of a water budget zone" .

:RiverInflow-UT skos:definition "Volume of water entering through rivers from an upstream subarea." .

:GagedSurfaceWaterInflow-CO skos:definition "Volume of water entering through surface waters at the periphery of a water budget zone that is measured by gages." .

:UngagedSurfaceWaterInflow-CO skos:definition "Volume of water entering through suface waters at the periphery of a water budget zone that is not measured by gages." .

:StreamInflow-CA skos:definition """Volume of water entering through streams at the periphery of a water
budget zone.""" .

:CODiversionRecords skos:definition "The Division Engineer for each major river basin, along with Water Commissioners and other staff, is responsible for administering the water rights and taking measurements of streamflow and diversions in their basin. The responsibility of recording diversions extends to both surface and ground water use, however there is very little ground water used for irrigation in the Western Slope river basins, therefore this discussion will focus on surface water diversions. The daily diversion records are stored in HydroBase, and can be accessed either through the CDSS website or through data management interfaces." .

:HydroBase skos:definition "The State of Colorado's relational database used in the CDSS efforts. HydroBase contains historic, realtime, and administrative water resources data." .

:SCSTR21 skos:definition """Re = (0.7091*Rt0.82416  0.11556)*(10(0.02426*cu) )*F 
- Re - monthly effective precipitation 
- Rt - total monthly precipitation 
- cu - monthly consumptive use (potential ET) 
- F - function of D 
- D - the net depth of application 
- F = 0.531747 + 0.295164(D)  0.057697(D2 ) + 0.003804(D3 )""" .

:SnotelNetworkOfWeatherStations skos:definition "Managed by the National Resources Conservation Service (NRCS) in the high elevation mountains surrounding the Green River basin. Climate data, along with maps and summary reports from these climate stations, are available online (http://www.wcc.nrcs.usda.gov/snow/)." .

:RemoteAutomatedWeatherStations%28RAWS%29 skos:definition "Managed by several Federal entities including the U.S. Bureau of Land Management and the U.S. Fish and Wildlife Service. These stations are located in remote areas to assist in assessing wild fire vulnerability. The hourly climate data information from these climate stations is available online from the RAWS website, generally beginning in the mid-1990s" .

:COIrrigatedAcreageAssessment skos:definition "Irrigated acreage assessments define the amount of acreage that was actively irrigated and cultivated in any given year. Irrigated acreage assessments can range in the level of attribution;" .

:CropIrrigationRequirementEstimationMethod skos:definition "Crop irrigation requirement is calculated as PCU less effective precipitation." .

:METRIC skos:definition "Mapping evapotranspiration at high resolution with internalized calibration, publically available system developed through the University of Idaho. Mapping Evapotranspiration at high Resolution with Internalized Calibration (METRIC) is a model that utilizes satellite imagery and the energy balance method to spatially estimate actual ET. LandSat satellite imagery records thermal infrared light that is used in the energy balance to determine net radiation and the model utilizes local climate data to determine the remaining factors in the energy balance equation and calibrate the ET results. METRIC was recently used in the South Platte River basin in comparison to StateCU results for varying crop and irrigation practices." .

:ModifiedBlaney-CriddleWithETElevationAdjustment skos:definition "The ASCE Manuals and Reports on Engineering Practice No. 70, Evapotranspiration and Irrigation Water Requirements (1990), recommends elevation adjustments for both the SCS and the FAO-24 Blaney-Criddle methods of 10% adjustment upward for each 1,000 meters increase in elevation above sea level. The adjustment corrects for lower mean temperatures that occur at higher elevations at a given level of solar radiation (i.e. mean temperatures do not reflect crops reactions to warm daytime temperatures and cool nights). The adjustment is applied to the potential consumptive use estimate and can be applied to any crop type. Note, however, that if locally calibrated crop coefficients are used in lieu of standard SCS or FAO-24 crop coefficients, the mean temperature correction is represented, and an additional elevation adjustment should not be applied." .

:NDVIstar skos:definition "The NDVI StateCU methodology utilizes the normalized difference vegetative index (NDVI) measure of greenness within satellite images to apply a scaled measure of supply limitation to monthly actual ET estimates derived by the StateCU model when well diversions are an unknown. Linear scaling follows the NDVIstar approach proposed by D.P. Groeneveld and W.M. Baugh that can be overridden by measures of standing water. It is currently being developed by the State of Colorado to estimate water Actual ET and improve historic pumping estimates for the Rio Grande Basin over extended historical time periods, and has also been tested in the South Platte basin." .

:OriginalBlaney-Criddle skos:definition "Blaney Criddle relates ET with mean air temperature and mean percentage daytime hours. Formula: ETo = p (0.46 T mean +8)" .

:OriginalBlaney-CriddleWithETElevationAdjustment skos:definition "The ASCE Manuals and Reports on Engineering Practice No. 70, Evapotranspiration and Irrigation Water Requirements (1990), recommends elevation adjustments for both the SCS and the FAO-24 Blaney-Criddle methods of 10% adjustment upward for each 1,000 meters increase in elevation above sea level. The adjustment corrects for lower mean temperatures that occur at higher elevations at a given level of solar radiation (i.e. mean temperatures do not reflect crops reactions to warm daytime temperatures and cool nights). The adjustment is applied to the potential consumptive use estimate and can be applied to any crop type. Note, however, that if locally calibrated crop coefficients are used in lieu of standard SCS or FAO-24 crop coefficients, the mean temperature correction is represented, and an additional elevation adjustment should not be applied." .

:RESET skos:definition "Remote sensing of evapotranspiration, publically available system developed at Colorado State University. Remote Sensing of Evapotranspiration (RESET) is a remote sensing algorithm similar to the Surface Energy Balance Algorithm for Land (SEBAL) which is a satellite image-processing methodology used for computing actual ET for an entire satellite image. RESET, however, accounts for spatial and temporal variability by allowing more input from climate stations. RESET was developed by the IDS Group at Colorado State University. It is currently being used by Reclamation to investigate ET in the Uncompahgre River basin, and has been applied to areas of the Arkansas River Basin." .

:StateCU skos:definition "Publically available model developed by State of Colorado)" .

:CropIrrigationRequirement skos:definition "Crop irrigation requirement is calculated as PCU less effective precipitation.The amount of water crops could consume from a full irrigation supply." .

:EffectivePrecipitation skos:definition "Effective precipitation is the amount of precipitation during the irrigation season that is effective in satisfying a portion of PCU. The amount of water crops consume from precipitation." .

:IrrigationMethod skos:definition "Flood or sprinkler irrigation practices" .

:PotentialConsumptiveUse skos:definition "The amount of water crops could consume if provided a full supply, also called potential evapotranspiration (potential ET)." .

:Precipitation skos:definition "Parameter for StateMod" .

:SupplySource skos:definition "Including name or unique identifier of the water permit or water right, diversion structure, well, or reservoir" .

:SupplyType skos:definition "surface water, ground water, reservoir releases, or multiple sources" .

:ChangeInGroundWaterStorage-CO skos:definition "Calculation of inflows minus outflows to the groundwater system" .

:ChangeInGroundwaterStorage-CA skos:definition """Net change in the volume of groundwater stored within the underlying
aquifer of the water budget zone.""" .

:ChangeInGroundwaterStorage-AUS skos:definition "Calculation of inflows minus outflows to the groundwater system" .

:ChangeInLandSystemStorage-CA skos:definition """Net change in the volume of water stored within the land system, which
includes ponded water on the land surface (not including streams, lakes,
and conveyance facilities) and soil moisture within the unsaturated zone,
which includes the root zone.""" .

:ChangeInSurfaceWaterStorage-CA skos:definition """Net change in the volume of water stored within the surface water
system, which includes lakes and reservoirs, streams, and conveyance
facilities.""" .

:ChangeInSurfaceWaterStorage-CO skos:definition "Change in the amount of water stored as groundwater" .

:ClassAPanEvaporationData skos:definition "Obtain Class A pan evaporation data recorded for each month from the weather station that best represents climate conditions in the study area. Measurements of monthly and annual evaporation from U.S. Weather Bureau Class A pans are generally available from NOAA." .

:ColoradoStateMod skos:definition "State of Colorado's Stream Simulation Model (StateMod) is a water allocation and accounting model capable of making comparative analyses of various historical and future water management policies in a river basin. It is designed to be applied to any river basin through appropriate input data preparation." .

:DirectFlowDemand-Monthly skos:definition """The monthly direct flow demand file contains demands for direct diversions for each month of the
simulation period. Monthly data is required when the diversion station variable idvcom is set to 1
(monthly total demand) or 3 (monthly irrigation water requirement).""" .

:Evaporation skos:definition "Parameter used in CO StateMod" .

:ReservoirTargets skos:definition """Target (im) = Current Storage (im) - (Current Storage (im) - Forecast (im) - End Target) /
(Months Remaining +1)""",
    "The reservoir target file contains monthly targets for a reservoir's minimum and maximum contents." .

:Streamflow skos:definition "The streamflow file may contain total baseflows or gains for each month of the simulation period. The control variable iopflo identifies which is expected; total baseflow (1) or gains (2)." .

:Commercial-NMOSE skos:definition "The Commercial category includes: Self-supplied businesses (e.g., motels, restaurants, recreational resorts, and campgrounds), Public and private institutions (e.g., public and private schools and hospitals) involved in the trade of goods or provision of services, Self-supplied golf courses that are not supplied by entities covered in the Public Water Supply category, Greenhouses and nurseries that both produce and sell products to the general public on the same premises, Off-stream fish hatcheries that produce fish for release, and Non-metered schools." .

:MunicipalAndIndustrialDiversions-UT skos:definition "Water Supplied for municipal and industrial uses, other than agriculture, provided through a municipal distribution system that remains in the budget zone" .

:ConveyanceEvaporation-CA skos:definition """Volume of water evaporated into the atmosphere from conveyance
facilities, other than streams, during water delivery.""" .

:HumanConsumption-NM skos:definition "In the default setting of the NMDSWB human consumption is calculated for public and domestic water supplies (section 4.4.3), Irrigated agriculture (section 5.1), and livestock (4.4.4). Commercial, Industrial, Mining, and Power uses of water are provided by the OSE water use by categories report for counties and river basins" .

:ConveyanceLossesForAllocatedDiversions-AUS skos:definition "Water diverted primarily to operate regulated rivers and utility supply networks to enable the delivery of water for which an allocation has been recognised." .

:SurfaceWaterOutflows-AUS skos:definition "Volume of physical outflows from surface water during the reporting period to outside the region or to other stores." .

:ConveyanceSeepage-CA skos:definition """Volume of water recharged to the groundwater system from the
conveyance facilities, other than streams, during water delivery.""" .

:CoplandPrecipitation-UT skos:definition "Volume of water vapor that falls  to the earth specifically on cropland area, as rain, snow, hail, or is formed on the earth as dew, and frost" .

:Precipitation-CA skos:definition """Volume of water vapor that falls to the earth (land and surface water
systems) as rain, snow, hail, or is formed on the earth as dew, and frost. -- Excepting Lakes""" .

:Precipitation-CO skos:definition "Volume of water vapor that falls to the earth (land and surface water systems) as rain, snow, hail, or is formed on the earth as dew, and frost." .

:Precipitation-NM skos:definition "Volume of water vapor that falls to the earth (land and surface water systems) as rain, snow, hail, or is formed on the earth as dew, and frost." .

:Precipitation-UT skos:definition "Volume of water vapor that falls to the earth as rain, snow, hail, or is formed on the earth as dew, and frost." .

:Precipitation-WY skos:definition "Volume of water vapor that falls to the earth as rain, snow, hail, or is formed on the earth as dew, and frost." .

:IrrigatedAgricultureDepletions-NMOSE skos:definition "Consumptive Use" .

:USDACroplandDataLayer%28CDL%29 skos:definition """The CDL is a georeferenced crop-specific land cover classification product
with a 30 meter resolution that is produced annually. GIS was used to integrate the CDL crop types with a layer of potentially irrigated polygons covering the entire state.""" .

:DailyASCEStandardizedPenman-Monteith skos:definition """In 1999, the Irrigation Association requested a technical committee of the American Society of Civil Engineers (ASCE) that is involved with evapotranspiration to propose one standardized equation and set of procedures for calculating evapotranspiration. The result of this process was that two equations (one for a short crop named 
ETo and one for a taller crop named ETr) were developed. These equations were based on framework suggested in a FAO56 (Allen, 1998) document that assumed a constant for the psychometric constant, simplified the air density term and simplified the vapor aerodynamic resistance term. For each type of reference crop (short or tall), constants were assigned in the ASCE Standardized Penman-Monteith equation for the vegetation height, latent heat of vaporization, and surface resistance.""" .

:DailyEffectivePrecipitation skos:definition """The portion of precipitation falling during the cropgrowing season that is available to meet the evapotranspiration requirements of
the crop.""" .

:DailyModifiedHargreaves skos:definition """StateCU uses a Modified Hargreaves radiation method to estimate ET that was developed by Agro Engineering, Inc. This method was specifically developed for the San Luis Valley and should be used with caution in other areas. The original Hargreaves method used temperature and radiation data to estimate ET for an Alta fescue grass crop. The Modified Hargreaves approach includes a wind function to recognize the advective transfer of water away from plant stomatal openings under windy conditions as follows:

ETo=(FRsTavg)/1498.6""" .

:DivertibleFlow-WY skos:definition "Portion of inflow that can be diverted in the budget zone under compact allocation" .

:DomesticTotalUse-WY skos:definition """Domestic water use is water used for personal, commercial, and other purposes that
is not supplied by a municipality. Examples of domestic water use are rural singlefamily
residences and highway rest-stops.""" .

:WithdrawalMethod skos:definition "W = (POP)(GPCD)/892.74 (NM)" .

:UTEffectivePrecipitationMethod skos:definition "UT estimates effective precipitation to be 80% of total precipitation during the irrigation season" .

:EffectivePrecipitationFactor skos:definition """F - a user-specified factor with the value ranging
from 0 to 1""" .

:EmpiricalDataForSmallReservoirs skos:definition """In some areas there are small reservoirs that are not monitored on a regular basis. Many of these are not equipped with a gage to measure the water level, and area capacity curves are frequently not available. The NMOSE Dam Safety Bureau provided the most up-to-date area capacity data where possible for use in estimating evaporation. Because these reservoirs are small, and
hydrological and meteorological data are typically unavailable, spending extensive time and effort to estimate annual evaporation is not recommended.""" .

:Rainfall skos:definition "Obtain the total rainfall recorded for each month. These data are published monthly for most weather stations operated by the NOAA. When a reservoir is completely covered with ice for part of a month, recorded precipitation should include only those days when the water surface was exposed." .

:ReservoirSurfaceArea skos:definition "Determine the average water surface area in acres for each month from a curve or equation that correlates gage height or content with surface area. Area-gage height or area-capacity data can be obtained from the agencies mentioned in Step 1." .

:Evaporation-AUS skos:definition "Movement of water from theregion'ssurface waterto the atmosphere (water vapour)" .

:Evaporation-NM skos:definition "Volume of water evaporated from the land surface into the atmosphere" .

:EvaporationFromReservoirs-NMOSE skos:definition "The Power category includes all self-supplied power generating facilities and water used in conjunction with coal-mining operations that are directly associated with a power generating facility that owns and/or operates the coal mines. Section 5.6 describes some power generating facilities and their associated water use." .

:PanApproach skos:definition "The National Weather Service Class A Pan is 4 feet in diameter and 10 inches deep, It is made of unpainted, 22-gage galvanized iron and sits on a wooden pallet so that the bottom of the pan is raised 6 inches above the ground, allowing air to circulate. Site requirements specify that the pan be located on level ground, unobstructed by trees or buildings, so maximum exposure to sunlight is possible. The pan is filled with water to within 2 inches of the top and is refilled as soon as the water level drops 1 inch. The depth of water is measured with a micrometer hook gage located in a stilling well that supports the gage. An anemometer, which is used to measure wind movement, is mounted on the pallet, with the cups positioned 24 inches above the base of the pan. Maximum/minimum thermometers (which are stored in an instrument shelter) and a rain gage are also installed at the site. A 5-foot-high wire mesh fence encloses the entire installation. A pan reading is taken every morning." .

:MonthlyGrossEvaporationRate skos:definition "The gross evaporation rate for each month is computed by multiplying the pan evaporation, which is expressed as a depth of water in feet, by the pan coefficient. In winter, if the evaporation pan is iced over, but the water surface of a nearby reservoir remains unfrozen, agencies such as the USBR have developed empirical equations based on temperature that can be used to estimate gross evaporation." .

:WinterIceSurfaceArea skos:definition "Winter evaporation estimates must take into account the possible effects of ice cover. Partial ice cover will inhibit evaporation; complete ice cover will reduce water surface evaporation to zero. Thus, the average surface area computed in Step 2 must be adjusted to reflect the surface area covered by ice. For large reservoirs, daily measurements of ice cover may be available. Some agencies have developed tables showing the percentage of ice cover by month, based on historical records, which may be used when no other data are available." .

:LakeEvaporation-CA skos:definition "Volume of evaporation from lakes and reservoirs." .

:ReservoirEvaporation-CO skos:definition "Volume of water evaporated into the atmosphere from reservoirs." .

:ReservoirEvaporation-UT skos:definition "Volume of water evaporated into the atmosphere from reservoirs." .

:GroundwaterExport-CA skos:definition """Volume of groundwater pumped (extracted) from the underlying aquifer
for use outside the water budget zone. It does not include groundwater
extraction, stored water extraction, and stored water export.""" .

:StoredWaterExport-CA skos:definition """Volume of groundwater pumped (extracted) from the underlying
aquifer(s) through a defined recharge and extraction program for use
outside the water budget zone. For example, a water bank with dedicated
extraction wells can provide data for stored water export. It does not
include stored water extraction, groundwater extraction, and
groundwater export. Groundwater export and stored water export will be
combined if stored water export amounts are unknown or are not
separately measured. In such a case, the total volume of combined
exports will be reported as groundwater export.""" .

:SurfaceWaterExports-CA skos:definition """Volume of water diverted from the surface water system within a water
budget zone for use outside the zone.""" .

:FloodReturn-AUS skos:definition "Return of flood waters from the flood plains. It excludes flood waters returning from seasonally connected wetlands and other surface water bodies." .

:SurfaceWaterInflows-AUS skos:definition "Volume of physical inflows tosurface waterduring thereporting periodfrom outside theregionor from other stores" .

:GagedSurfaceWaterOutflow-CO skos:definition "Volume of water exiting through surface waters at the periphery of a water budget zone that is measured by gages." .

:GrossActivelyIrrigatedAcreage skos:definition """Irrigated acreage for the Report was compiled using the USDA Cropland
Data Layer (CDL). The CDL is a georeferenced crop-specific land cover classification product with a 30 meter resolution that is produced annually. GIS was used to integrate the CDL crop types with a layer of potentially irrigated polygons covering the entire state. WUCB staff analyzed the results using aerial imagery to ensure accuracy. During this process, edits were made as needed to reflect on-the-ground conditions. For example, areas in the eastern part of the state that appeared to be dryland farmed were removed from the analysis. Ancillary data from the USBR, USDA Farm Service Agency, National Agricultural Statistics Service, NMISC, NMOSE district offices, irrigation districts, conservancy districts, and county extension agents were used to help validate and refine the totals obtained from the CDL and subsequent analysis.""" .

:GroundWaterInflow-CO skos:definition "Volume of water entering as groundwater from a water budget zone through its subsurface boundaries." .

:SubsurfaceInflow-CA skos:definition """Volume of water entering as groundwater into a water budget zone
through its subsurface boundaries.""" .

:GroundWaterOutflow-CO skos:definition "Volume of water leaving as groundwater from a water budget zone through its subsurface boundaries." .

:SubsurfaceOutflow-CA skos:definition """Volume of water leaving as groundwater from a water budget zone
through its subsurface boundaries.""" .

:GroundwaterDischarge-AUS skos:definition "Groundwater discharge to the region's surface water." .

:Discharge%3AGroundwater-AUS skos:definition "Groundwater discharge to the region's surface water." .

:GroundwaterDiversions-NM skos:definition "Water diverted from groundwater to human storage and distribution systems" .

:GroundwaterET-NM skos:definition "Groundwater ET is calculated based on a calculated riparian ET rate multiplied by a remote sensing based estimate of riparian area." .

:RiparianConsumption-NM skos:definition "Volume of water lost due to ET in the riparian zone" .

:LakeGainFromGroundwater-CA skos:definition """Volume of water entering lakes and reservoirs from the groundwater
system.""" .

:GroundwaterInflows-NM skos:definition "As used in the NMDSWB, groundwater inflows into a given MBAU flow in from outside of the MBAU. FOr the purposes of the NBMDSWB, we assume that basin scale groundwater divides are the same as surface water divides" .

:GroundwaterOutflows-AUS skos:definition "Lateral flow of groundwater out of the region's groundwater to inland groundwater aquifers that extend outside the region. It excludes lateral flow of groundwater to coastal aquifers." .

:GroundwaterOutflows-NM skos:definition "Groundwater flow across a political or watershed boundary cannot be directly measured, and must be calculated based on observed groundwater elevations and inferred geologic information, or extracted from regional groundwater models based on the same. In the 2015 version of the NMDSWB, groundwater outflows are largely unknown. The user has the option of setting groundwater outflows to a user selected constant value (with a default of zero), allowing a change in groundwater storage over the selected period to be calculated. However, this change would be averaged over the entire region being modeled (i.e. watershed, WPR, or county). This change in storage cannot be related to a change in groundwater elevation without detailed knowledge of aquifer characteristics, pumping and recharge, and developing a mechanistic groundwater model of the basin." .

:GroundwaterReturn-NM skos:definition "Volume of water returned to groundwater from human storage and distribution systems" .

:GroundwaterStock-NM skos:definition """The groundwatersystem conceptually representsall sub-surface water that is below the water table (saturated soil and rock).Total groundwater storage for the state of New Mexico is largely unknown. However, for select aquifers throughout the state, estimates of total groundwater storage do exist. Where these estimates are known they areused as input into the NMDSWB. Future work by other 
17members of the New Mexico Water Resources Research Institute led Statewide Water Assessment includes plans to quantify total groundwater storage on a statewide basis.The NMDSWBdoes track groundwater storage changes over time. When groundwater storage estimates are not available the default initial storage is set to zero.""" .

:USGSGroundwaterReports skos:definition "Groundwater use from USGS groundwater reports allocated annual to each water budget study area from 1989 to 2009. Water Rights irrigation wells were used to proportion water from USGS groundwater use areas to water budget study areas. USGS groundwater use areas were modified to spatially account for where their study wells were actually located in association with irrigated agriculture." .

:GroundwaterUse-UT skos:definition "Volume of groundwater extracted from the underlying aquifer(s) for use within the water budget zone" .

:PumpedGroundwater-UT skos:definition "Volume of groundwater pumped (extracted) from the underlying aquifer(s) for use within the water budget zone" .

:HumanReturns-NM skos:definition "In the NMDSWB return flows are calculated as the difference between withdrawals and consumption (depletions).  The surface water return flux from human storage also includes releases from reservoir storage." .

:HumanStorageAndDistributionSystemStock-NM skos:definition "The human storage and distribution system (HSDS)stockrepresents water at any given time residing in manmade storage impoundments or distribution systems, such as public water supplies, irrigation canals, and reservoirs.Currently, only reservoir storage is tracked.For purposes of this mass balance, when water is added to storage in a reservoir, it is considered a diversion of available surface water to the HSDS, and when it is released from storage, it is considered a return to the available surface water system.Reservoirvolumes in the NMDSWBare calculated as the previous storage pluschange in storage which iscalculated as the difference between knownor calculatedinflows (gaged inflow, precipitation) and known or calculated outflows (gaged outflows, evaporation" .

:ImportedWater-CA skos:definition """Volume of water brought from outside the water budget zone for use
within the water budget zone, such as State Water Project water, Central
Valley Project water, water produced from desalination of ocean water,
and water produced from desalination of deep groundwater from below
the base of freshwater.""" .

:Imports-CO skos:definition """Volume of water brought from outside the water budget zone for use
within the water budget zone.""" .

:Industrial-NMOSE skos:definition "The Industrial category includes self-supplied enterprises that process raw materials or manufacture durable or nondurable goods. This category also includes water used for the construction of highways, subdivisions, and other construction projects. 100% of industrial withdrawals are metered." .

:IndustrialConsumptiveUse-WY skos:definition """Industrial water use is indexed to a variety of data sources depending on the
industries present in a given river planning basin (Table 1). Common industrial uses
include electrical generation, oil and gas production, and mining.""" .

:IndustrialTotalUse-WY skos:definition """Industrial water use is indexed to a variety of data sources depending on the
industries present in a given river planning basin (Table 1). Common industrial uses
include electrical generation, oil and gas production, and mining.""" .

:SurfaceWaterDelivery-CA skos:definition """Volume of surface water delivered to a water budget zone. This does not
equal the volume of surface water diversion and imported water because
the latter also include conveyance seepage and evaporation during
transport of the water.""" .

:Inter-regionCoastalInflow-AUS skos:definition "Groundwater transferred into the region through salt water intrusion" .

:Inter-regionCoastalOutflow-AUS skos:definition "Groundwater discharged into coastal waters" .

:InterpolationFromOtherRecords skos:definition """When metered records for the water-use inventory year are incomplete, water use is estimated based on earlier records (as with other categories in this Report) or prorated based on
similar operations.""" .

:NMIrrigatedAcreageAssessment skos:definition "Irrigated acreage assessments define the amount of acreage that was actively irrigated and cultivated in any given year. Irrigated acreage assessments can range in the level of attribution;" .

:UTIrrigatedAcreageAssessment skos:definition "Irrigated acreage assessments define the amount of acreage that was actively irrigated and cultivated in any given year. Irrigated acreage assessments can range in the level of attribution;" .

:IrrigatedAgriculture-NMOSE skos:definition "The Irrigated Agriculture category includes all withdrawals of water for the irrigation of crops grown on farms, ranches, and wildlife refuges." .

:ConsumptiveIrrigationRequirement%28CIR%29 skos:definition "The quantity of irrigation water expressed as a depth or volume per unit area, exclusive of effective rainfall, that is consumptively used by plants or is evaporated from the soil surface in a specific period of time. It does not include water requirements for leaching, frost protection, wind erosion protection, or plant cooling. Such requirements are accounted for in on-farm efficiency values. The consumptive irrigation requirement may be numerically determined by subtracting effective rainfall from the consumptive use." .

:IrrigationSchemeInflows-AUS skos:definition "Inflows into theregion'sirrigation schemeor increase ofclaims to waterthat may result in inflows into theregion'sirrigation scheme." .

:IrrigationSchemeOutflows-AUS skos:definition "Outflows from theregion'sirrigation schemeor decrease ofclaims to waterthat may result in outflows from theregion'sirrigation scheme." .

:LakeLossToGroundwater-CA skos:definition """Volume of water entering the groundwater system from lakes and
reservoirs.""" .

:Recharge-NM skos:definition "Recharge in the NMDSWB is calculated by assuming that without human diversions and returns, the groundwater system would be in steady state. Under this assumption, non-anthropogenic inflows (groundwater inflows from another MBAU and recharge) are equal to non-human related outflows (groundwater outflows to another MBAU, ET, and baseflow). Baseflow is water moving to the surface water system from the groundwater system, and is calculated as the portion of the total gains to the surface water system not attributed to runoff as described above. For each MBAU at each timestep, recharge is set equal to a moving 10 year average of the sum of the baseflow terms (calculated above as headwaters baseflow and baseflow of net gains between gages) plus groundwater ET and groundwater out minus groundwater in. Without averaging this term of a long time period it would ignore a basic characteristic of temporal lags in groundwater systems. Additionally, human impacts that change mass balance groundwater fluxes are at play across the state. Thus, both the assumption that recharge is equal to baseflow plus groundwater ET, and the assumption that non-human related groundwater fluxes are in balance are both open to legitimate criticism. These assumptions have provided the NMDSWB with a self-consistent way to estimate recharge which results in state level mass balance terms (especially groundwater storage change) that are reasonable, but as will be seen, produces some basin scale results that do not seem reasonable. The assumptions are in theory worse in regions of higher levels of groundwater pumping." .

:LandSurfaceExapotranspiration-NM skos:definition "Land surface evaporation is calculated by setting evaporation equal to precipitation less surface water runoff and recharge. In other words, of the rain that falls in an area in a given period of time, we assume that what doesnt runoff or recharge evaporates to the atmosphere." .

:LandSurfaceStock-NM skos:definition "For the purposes of the NMDSWB, the landsurface system conceptually representsmoisture stored in non-saturated soilsor geologic formations(the vadose zone),in vegetation, orany other surface water source that cannot be practicably diverted for human use.The water stored in this stock is difficult to measure at large scale and changes rapidly, and isnot calculated in this effort.Change in storage of this stock isset to zeroin the NMDSWBfor all timesteps.Thus, the land surface stock for purposes of this conceptual mass balance is a construct which allows precipitation to be partitioned into recharge, evaporation, and runoffat each timestep." .

:Livestock-NMOSE skos:definition "The Livestock category includes water used to raise livestock, maintain self-supplied livestock facilities, and provide for on-farm processing of poultry and dairy products." .

:ManagedAquiferRecharge-AUS skos:definition "The volume of water intentionally transferred toground water assets(e.g. via injection wells) from otherwater assets: eithersurface water,urban water systemorirrigation scheme." .

:UrbanWaterSystemOutflows-AUS skos:definition "Outflows from theurban water system; to outside theregionor to other stores. For example the discharge of treated wastewater to a river or to the sea." .

:ManagedAquiferRecharge-CA skos:definition """Volume of water intentionally added to the groundwater system as part of
defined recharge and water banking programs through spreading basins,
injection wells, and other means.""" .

:Mining-NMOSE skos:definition "The Mining category includes the following self-supplied enterprises that extract minerals occurring naturally in the earths crust: Solids, such as potash, coal, and smelting ores, Liquids, such as crude petroleum, Gases, such as natural gas. This category includes water used for oil and gas production (well drilling and secondary recovery of oil), quarrying, milling (crushing, screening, washing, flotation, etc.), and other processing done at the mine site or as part of a mining activity, as well as water removed from underground excavations (mine dewatering) and stored inand evaporated fromtailings ponds. The Mining category also includes water used to irrigate new vegetative covers at former mine sites that have been reclaimed. It does not include the processing of raw materials, such as smelting ores, unless this activity occurs as an integral part of a mining operation and is included in an NMOSE permit." .

:Industrial%3AMineProduction-WY skos:definition "Annual employee hours and coal production data were downloaded from the Mine Safety and Health Administration (MSHA) web portal27. The MSHA is part of the United States Department of Labor." .

:MonthlyEffectivePrecipitation skos:definition """The portion of precipitation falling during the cropgrowing season that is available to meet the evapotranspiration requirements of
the crop.""" .

:Power-NMOSE skos:definition "The Power category includes all self-supplied power generating facilities and water used in conjunction with coal-mining operations that are directly associated with a power generating facility that owns and/or operates the coal mines. Section 5.6 describes some power generating facilities and their associated water use." .

:PublicWaterSupply-NMOSE skos:definition "The Public Water Supply category includes community water systems that rely on both surface water and groundwater diversions, and that consist of common collection, treatment, storage, and distribution facilities operated for the delivery of water to multiple service connections. For the purposes of this Report, these systems will be known as Public Water Suppliers (PWS) and this definition will include mutual domestic systems, mutual domestic water user associations, etc. Following are examples of multiple service connection systems: Municipalities that serve residential, commercial, and industrial water users, Prisons, Residential and mixed-use subdivisions, Mobile home parks. The Public Water Supply category also captures other water uses supplied by PWSs such as irrigation of golf courses, parks, athletic fields, or ponds/lakes. Wells permitted by the NMOSE under 72-12.1 New Mexico Statues Annotated (NMSA) 1978 are not included in this section." .

:MunicipalAndIndustrialDepeltion-UT skos:definition "Water Supplied for municipal and industrial uses, other than agriculture, provided through a municipal distribution system that is consumed and does not return to a natural water source or another body of water." .

:MunicipalAndIndustrialReturnFlow-UT skos:definition "Average flow for municipals areas" .

:ReturnFlow-CA skos:definition """Volume of applied water that is not consumptively used and flows to the
surface water system. It includes treated wastewater discharges to the
surface water system.""" .

:NMDiversionRecords skos:definition "Records available real-time for most diversions for 2011 through the current date. Diversions to Navajo Indian Irrigation Project measured." .

:OriginalHargreaves skos:definition "The original Hargreaves method (1975) is a daily grass-reference radiation method that uses mean air temperature, the differential between daily maximum and minimum air temperatures, and solar radiation to estimate ET." .

:NMIrrigationWithdrawals skos:definition """Where measured withdrawals are not available, the groundwater and surface water components must be estimated. Estimates are made by (1) examining historical water right diversion records,
(2) comparing recorded stream flows with the estimated demand, (3) contacting personnel in the County Extension Service, Natural Resources Conservation Service, or individual farmers with local familiarity, or (4) using component estimates from the previous Water Use by Categories report.""" .

:NMOSETechnicalReportNo.48 skos:definition "The most recent NMOSE indoor GPCD estimations are provided in NMOSEs Technical Report No. 48 (Wilson, 1996). Technical Report No. 48 includes conservation measures available during the early 1990s, and estimates an indoor GPCD of 58.9. It is well established that there have been significant advances in the efficiency of indoor plumbing fixtures since both the Brown and Caldwell study and Technical Report No. 48 were published. The values provided from Technical Report No. 48 are intended for planning or benchmarking purposes." .

:NativeVegetationConsumptiveUse-CO skos:definition "Amount of water that does not return to its source after it has been diverted and put to beneficial use by natural vegetation." .

:NaturalSystemUse-UT skos:definition "Volume of water lost through evapotranspiration from normal plants and surface waters. Non human consumptive use." .

:RiparianDepletions-UT skos:definition "Volume of water transpired from plants and evaporated along the riparian zone" .

:ProrationFactors skos:definition "Representing fraction of reach gain estimated to be tributary to a natural flow point" .

:Non-allocatedExtraction-AUS skos:definition "Extraction from the region's groundwater where no prior claim has been recognised" .

:OtherIncreases-AUS skos:definition "Groundwater Inflows not accounted in other components" .

:Outflow-AUS skos:definition "Volume of physical outflows fromsurface waterduring thereporting periodto outside theregionor to other stores" .

:PersonalOutreach skos:definition "When possible, these entities are identified through directories maintained by various business associations and/or regulatory agencies. The executive director or operator is then contacted by phone or mail to obtain an estimate of water use." .

:PopulationServedByPublicWaterSupply skos:definition "In noncensus years, the population must be estimated. Methodologies may range from a simple linear extrapolation to complex correlations based on the demographic characteristics of individual communities. An important step in determining the utilitys population served is to separate the population of self-supplied residents from the total population of the larger community served by the PWS. Populations for communities not identified in the census are obtained from the water system manager, city clerk, regulatory agency, or estimated by some other means. Many water utilities estimate, with reasonable accuracy, the population they serve based on the total number of connections and the average number of residents per connection." .

:Industrial%3AElectricalGeneration-WY skos:definition "Electrical generation is a major industrial water user in the Green, Northeast, and Platte River planning basins." .

:Precipitation-AUS skos:definition "All forms in which water falls on the region's surface water as rain, sleet, snow, hail, or drizzle" .

:PrecipitationOnLakes-CA skos:definition """Volume of water vapor that falls to the earth (land and surface water
systems) as rain, snow, hail, or is formed on the earth as dew, and frost.--Lakes Only""" .

:RechargeOfAppliedWater-CA skos:definition """Volume of applied water that travels vertically through
the soil/unsaturated zones and reaches the saturated zone of the aquifer
(groundwater system).""" .

:RechargeOfPrecipitation-CA skos:definition """Volume of  precipitation that travels vertically through
the soil/unsaturated zones and reaches the saturated zone of the aquifer
(groundwater system).""" .

:RecycledWaterExport-CA skos:definition """Volume of recycled water diverted from the land system within a water
budget zone for use outside the zone. Recycled Water: Volume of water which, as a result of treatment of waste, is suitable for a
direct beneficial use or a controlled use that would not otherwise occur
within the water budget zone. It includes wastewater that is treated,
stored, distributed, and reused or recirculated for beneficial uses.""" .

:RiverEvaporation-NM skos:definition "Volume of water evaporated from rivers into the atmosphere" .

:RiverUseByWetPasture-UT skos:definition "The volume of river water calculated to be used by wet pastures" .

:Runoff-AUS skos:definition "Runoff from landscape to the region's surface water due to rainfall or irrigation" .

:Runoff-CA skos:definition """Volume of water flowing into the surface water system within a water
budget zone from precipitation over the land surface.""" .

:Runoff-NM skos:definition "Runoff consists of water that goes from precipitation in a given MBAU into the surface water system in the same MBAU without moving through the groundwater system. Inflows from upstream MBAUs are counted as surface water inflows and not runoff" .

:Self-SuppliedDomestic-NMOSE skos:definition "The Self-Supplied Domestic category includes self-supplied residences that may be single family or multi-family dwellings with well permits issued by the NMOSE under 72-12-1.1 NMSA 1978. This category includes water used for domestic purposes as defined under 19.27.5.7.F New Mexico Administrative Code (NMAC)." .

:SelfSuppliedDomesticPopulation skos:definition "The self-supplied domestic population in a county is determined by subtracting the population served by PWSs from the total population in that county. When a county has two or more river basins, the total county population must be calculated by its basin components. The distribution of the population in each county by river basin is based upon ratios derived from 1990 census block and tract data that were overlaid with hydrologic cataloging units. The population served by PWSs in each basin is then subtracted from the total population of the respective basins to yield the self-supplied domestic population." .

:StoredWaterExtraction-CA skos:definition """Volume of groundwater pumped (extracted) from the underlying
aquifer(s) through a defined recharge and extraction program for use
within the water budget zone. For example, a water bank with dedicated
extraction wells can provide data for stored water extraction. It does not
include stored water export, groundwater extraction, and groundwater
export. Groundwater extraction and stored water extraction will be
combined if stored water extraction amounts are unknown or are not
separately measured. In such a case, the total volume of combined
extractions will be reported as groundwater extraction.""" .

:StreamEvaporation-CA skos:definition "Volume of water evaporated into the atmosphere from streams." .

:StreamGainFromGroundwater-CA skos:definition """Volume of water entering rivers and streams from the groundwater
system.""" .

:StreamLossToGroundwater-CA skos:definition """Volume of water entering the groundwater system from rivers and
streams.""" .

:SurfaceWaterDiversions-NM skos:definition "Volume of water diverted from surface water to human storage and distribution systems" .

:SurfaceWaterEvaporation-NM skos:definition "Surface water evaporation is calculated by multiplying river area by Hargreaves reference ET and an open water coefficient for the respective basin. In addition to the physically based estimate of river channel evaporation described above, the surface water evaporation term also includes the portion of surface water return flows that do not end up back in a gaged stream." .

:SurfaceWaterFlows-UT skos:definition "Volume of surface water flowing between different bodies of water within the budget zone" .

:SurfaceWaterGroundwaterInteractions-NM skos:definition "Groundwater and surface water interactions are determined as the closure term in surface water system. The groundwater-surface water interaction term is equal to the sum of surface water inflows minus the sum of surface water outflows." .

:SurfaceWaterInflows-NM skos:definition "As used in the NMDSWB, surface water inflows into a given MBAUconsist of flows which cross its boundary.Thus, MBAUs that occur at the headwaters of the river (for example the Pecos and Central Closed River Basins) do not have any surface water inflows." .

:SurfaceWaterOutflows-NM skos:definition "Surface water outflows are estimated based on USGS stream gage data as available. When a stream gage is available near the downstream border of a WPR, NMISC river basin, or County boundary it is used to represent the outflow." .

:SurfaceWaterReturns-NM skos:definition "Volume of water returned to surface water from human storage and distribution systems" .

:SurfaceWaterStock-NM skos:definition "The surface waterstock representsthe total amount ofwater in rivers and other natural water ways at any time.For the purposes of this mass balance we assume that any water in the surface water system can be diverted or impounded for human use. Available Water comes from stream flows across the boundaries of the mass balance accounting unit (MBAU) in question (State, County, or Water Planning Region), or runoff to streams and rivers from rainfall or groundwater discharge within the MBAU.Because the volume of water in surface water channels is relatively constant with respect to the states total water inventory, the actual storage of water in this stock will not be calculated, and storagechange through timewill be ignored.As a result of this simplifying assumptions, thefluxes into and out of this stock will be balancedat each timestep" .

:TotalLandReturnFlow-UT skos:definition "Total return flow from each land area" .

:TributaryInflow-UT skos:definition "Water that flows into major rivers in the budget zone from tributaries." .

:UngagedStreamGains-WY skos:definition "Stream gain from groundwater" .

:UrbanWaterSystemInflows-AUS skos:definition "Volume of physical inflows to the urban water system during the reporting period; from outside the region or from other stores" .

:WYDiversionRecords skos:definition "Major diversions and diversions on regulated tributaries recorded, ~150 continuously recorded, ~600 spot measured. Data available ~6 months after irrigation season.The State Engineers Office Board of Control Division is responsible for the administration and regulation of the waters of the state based on the Prior Appropriation System. The Division IV Superintendent, Hydrographers, and Water Commissioners are responsible for administering the water rights and permits in the Green River Basin and taking measurements of streamflow and diversions in their basin. The responsibility of recording diversions extends to both surface and ground water use, however there is very little ground water used for irrigation in the Green River Basin, therefore this discussion will focus on surface water diversions." .

:WYElectricalGenerationMethod skos:definition "The Green River Basin Plan reports consumptive electrical water use but does not state diversion/pumping or return flow rates. The Northeast River Basin reports average annual diversion/pumping volumes and return flows. From this data, Wenck determined consumptive water use for use in this index. The Platte River Basin Plan reports consumptive electrical water use. Electrical generation data were downloaded from the United States Energy Information Administration (USEIA) webpage25 for coal and natural gas fueled electrical generation facilities. The USEIA electrical generation dataset is updated monthly." .

:WYIndustrialProductionMethod skos:definition "Production data were downloaded from the WYOGCC data portal30 and compiled into annual production. This index assumes that a linear relationship exists between the volume produced and the net volume of water required. Therefore, the portion of industrial water use attributed to each sector is correlated to the produced volume." .

:WYMineProductionMethod skos:definition """Annual employee hours and coal production data were downloaded from the
Mine Safety and Health Administration (MSHA) web portal27. The MSHA is part of the United States Department of Labor. The MSHA publishes employee hours worked for all mine types and production quantities at coal mines data each quarter for all mines where the average quarterly employment is greater than zero.""" .

:WastewaterCollected-AUS skos:definition "Discharge of wastewater into the region's wastewater collection system. It includes discharge of wastewater by users into wastewater collection systems. It excludes wastewater collected by urban utilities outside the region and then transferred into the region" .

:WaterReleaseCausedByLandSubsidence-CA skos:definition """Volume of water released to an aquifer on a one-time basis as a result of
land subsidence, which is caused by the inelastic consolidation of porous
fine-grained material.""" .

:WaterUse-NM skos:definition "Water use is presented as withdrawals, depletions, and returns. Withdrawals are defined as the total amount of water taken from a source to be used elsewhere, depletions are defined as the quantity of water consumed, i.e. evaporated and no longer available for use elsewhere. Return flows are difference between withdrawals and depletions. The data is provided for each river basin and each county." .

:BrownAndCaldwell%2C1984 skos:definition """For the purpose of estimating withdrawals for the self-supplied domestic population, in most
counties, an area-wide average of 80 GPCD was used. This GPCD value was selected based upon
research completed by Brown and Caldwell (1984),""" .

:AllocatedDiversion%3AEnvironmentalPurposes-AUS skos:definition "Surface water diverted under a recognised commitment to deliver surface water for environmental purposes." .

:AllocatedDiversion%3AIndividualUsers-AUS skos:definition "Surface water diverted to users other than the urban water system, under water access entitlements for which an allocation has been recognised (see line item 32.3  surface water access entitlement for allocated diversions). It includes allocated diversions for: private users and irrigation schemes where those are not identified as a water asset of the water accounting region allocation holders located outside the region's boundary.It excludes allocated diversions for: irrigation schemes where those are identified as a water asset of the water accounting region (reported in line item 17.13  entitled diversion of allocated surface water to irrigation scheme)." .

:AllocatedDiversion%3AInter-region-AUS skos:definition "Surface water diverted outside of the region, under water access entitlements for which an allocation has been recognised" .

:AllocatedDiversion%3AIrrigation-AUS skos:definition "Diversion of surface water to the region's irrigation scheme to service a prior allocation announced on behalf of the irrigation scheme. It includes diversions under 32.3 Surface water access entitlement for allocation diversion." .

:AllocatedDiversion%3AIrrigationScheme-AUS skos:definition "Diversion of surface water to theregion'sirrigation schemeto service a prior allocation announced on behalf of theirrigation scheme. It includes diversions under32.3 Surface water access entitlement for allocation diversion" .

:AllocatedDiversion%3AUrbanSystem-AUS skos:definition "Surface water diverted to urban water system, under water access entitlements for which an allocation has been recognised (see account 2012-2017 line item 32.3  surface water access entitlement for allocation diversion). It includes allocated diversions for: allocation holders located outside the region's boundary." .

:AllocatedDiversions%3ASurfaceWater-AUS skos:definition "Diversion of surface water to theregion'surban water systemandirrigation scheme to service a priorallocation announcedon behalf of theurban water system. It includes diversions under32.3 Surface water access entitlement for allocation diversion." .

:AllocatedExtraction%3AEnvironmentalPurposes-AUS skos:definition "Groundwater extracted for environmental purposes, under water access entitlements for which an allocation has been recognised" .

:AllocatedExtraction%3AGroundwater-AUS skos:definition "Diversion ofgroundwaterto theregion'surban water systemto service a priorallocation announcedon behalf of theurban water system. It includes diversions under33.3 Groundwater access entitlement for allocation diversion." .

:AllocatedExtraction%3AIndividualUsers-AUS skos:definition "Groundwater extracted to users other than the urban water system, under water access entitlements for which an allocation has been recognised (see line item 33.3 Groundwater access entitlement for allocation extraction). It includes allocated extractions for:  private users and irrigation schemes where those are not identified as a water asset of the water accounting region allocation holders located outside the region's boundary.It excludes allocated extractions for: irrigation schemes where those are identified as a water asset of the water accounting region (reported in line item 18.13 Groundwater allocation diversion - irrigation scheme)." .

:AllocatedExtraction%3AIrrigation-AUS skos:definition "Diversion of groundwater to the external irrigation scheme to service a prior allocation announced on behalf of the irrigation scheme." .

:AllocatedExtraction%3AUrbanSystem-AUS skos:definition "Diversion of groundwater to the region's urban water system to service a prior allocation announced on behalf of the urban water system. It includes diversions under 33.3 Groundwater access entitlement for allocation diversion." .

:AppliedWaterReuse%2FRecycledWater-CA skos:definition """Volume of applied water contributing to (1) lateral flow below the land
surface that is influenced by impermeable layers and re-emerges as return
flow for reuse in the land system, (2) tailwater available for reuse in the
land system, or (3) a combination of both.""" .

:Commercial%3AGolfCourses-NMOSE skos:definition "Many golf course water supply systems in the state are metered and report their annual diversions to NMOSE. For the self-supplied courses that are not metered, withdrawals are estimated using the procedure outlined in Chapter 3, Irrigated Agriculture." .

:Commercial%3AUnmetered-NMOSE skos:definition "Some facilities are unmetered, and these can be difficult to identify if a declaration has never been filed with the NMOSE. Consequently, many of these facilities are not captured in the water use inventory. When possible, these entities are identified through directories maintained by various business associations and/or regulatory agencies. The executive director or operator is then contacted by phone or mail to obtain an estimate of water use." .

:Commercial%3AIncompleteMetered-NMOSE skos:definition "While most self-supplied facilities are required to be metered and to report their annual water use, many do not. When metered records for the water-use inventory year are incomplete, water use is estimated based on earlier records (as with other categories in this Report) or prorated based on similar operations." .

:Commercial%3AMetered-NMOSE skos:definition "Some facilities in the Self-Supplied Commercial, Industrial, Mining, and Power categories report their metered diversions to NMOSE, and those reports are identified in agency databases or through district office communications. NMOSE agency databases identify withdrawals by use, which are then used to separate the metered withdrawal categories in this chapter." .

:Commercial%3ASchools-NMOSE skos:definition "Water withdrawals for K-12 schools that are not metered, but are self supplied as identified by NMED, are computed by multiplying the student population by a per capita water requirement." .

:Delivery%3ADesalinatedWater-AUS skos:definition "Delivery of desalinated sea water to theregion'surban water systemwhere no prior claim has been recognised on behalf of theurban water system" .

:Delivery%3AInter-region-AUS skos:definition "Delivery of imported water to the region's surface water to service a prior claim recognised on behalf of the surface water. The prior claim may be an inter-basin agreement or an announced allocation held on a water resource located outside the region, but excludes water trade." .

:Delivery%3AInter-regionAgreement-AUS skos:definition "Delivery of imported water to the region's surface water to service a prior claim recognised on behalf of the surface water. The prior claim may be an inter-basin agreement or an announced allocation held on a water resource located outside the region, but excludes water trade." .

:Delivery%3AIrrigationScheme-AUS skos:definition "Water transferred out of the region or delivered to users from the irrigation scheme" .

:Discharge%3ALandscape-AUS skos:definition "Discharge from the groundwater or urban water system to the landscape, including soil, unconnected lakes and wetlands. It includes capillary rise and evaporation from the water table aquifer." .

:Discharge%3ASea-AUS skos:definition "Stormwater that discharges directly into the sea via a stormwater outflow drain located on the coastline." .

:Discharge%3ASurfaceWater-AUS skos:definition "Discharge of groundwater from the saturated zone or water from the urban system to streams, water storages, farm dams and natural surface water features." .

:Discharge%3AUrbanSupply-AUS skos:definition "Discharge from urban water systems to the region's surface water. It includes discharge of non-potable, potable, treated wastewater and recycled water. It includes pump back or transfer back of water to surface water for the purpose of storage and releases to meet environmental requirements. It excludes pump back or transfer of water to off-channel water storages considered part of the urban water system" .

:Discharge%3AUrbanSupplySystem-AUS skos:definition "Discharge from urban water systems to the region's surface water. It includes discharge of non-potable, potable, treated wastewater and recycled water. It includes pump back or transfer back of water to surface water for the purpose of storage and releases to meet environmental requirements. It excludes pump back or transfer of water to off-channel water storages considered part of the urban water system" .

:Discharge%3AWastewater-AUS skos:definition "Discharge of treated wastewater into the region. This definition includes discharge to sea and to other regions" .

:Diversions%3AStatutoryRights-AUS skos:definition "Surface water diverted under statutory rights" .

:Extraction%3AStatutoryRights-AUS skos:definition "Groundwater extracted under statutory rights" .

:Industrial%3ACoalbedMethandProduction-WY skos:definition "Monthly coalbed methane gas production and produced water data were downloaded from the WYOGCC data portal31. The WYOGCC compiles and publishes coalbed methane gas production according to the surface waterbody that receives produced water." .

:Industrial%3AMiscellaneous-WY skos:definition "USCB population data were used to index miscellaneous and road and bridge construction and maintenance industrial uses." .

:Industrial%3ANaturalGas-WY skos:definition "Natural gas processing is an industrial process to remove impurities from raw natural gas to create pipeline quality dry natural gas. Only the Bear River Basin accounted specifically consumptive water use at these facilities." .

:Industrial%3AOilAndGas-WY skos:definition "Annual employee hours and coal production data were downloaded from the Mine Safety and Health Administration (MSHA) web portal27. The MSHA is part of the United States Department of Labor." .

:Inter-regionInflow%3AGroundwater-AUS skos:definition "Groundwater transferred into the region from an external region" .

:Inter-regionInflow%3ASurfaceWater-AUS skos:definition "Surface water transferred into the region from an external region" .

:Inter-regionOutflow%3AGroundwater-AUS skos:definition "Groundwater transferred out of the region to an external region" .

:Leakage%3AGroundwater-AUS skos:definition "Leakage from urban system or surface water to the groundwater. It excludes pipe bursts, overflows or spills, which are classified as leakage to landscape." .

:Leakage%3ALandscape-AUS skos:definition "Leakage from thesurface water or irrigation scheme to the unsaturated zone of the soil profile and which does not infiltrate togroundwateras recharge" .

:Leakage%3AUrbanSystem-AUS skos:definition "Leakage fromurban water systemsto theregion'sgroundwater. It includes exfiltration from wastewater collection systems. It includes leakage from non-potable, potable and recycled water supply systems. It excludes pipe bursts, overflows or spills." .

:ManagedAquiferRecharge%3AIndividualUser-AUS skos:definition "Managed aquifer rechargeother than from theurban water systemto theregion'sgroundwater. It includes stormwater and industrial wastewater used formanaged aquifer rechargeand for amanaged aquifer rechargescheme" .

:Mining%3AUnreported-NMOSE skos:definition "Before opening any mining operation, the operator must register the mine, mill, smelter, or pit with the Mining and Minerals Division of the New Mexico Energy, Minerals, and Natural Resources Department. A directory of all of the mining facilities registered in the state is updated annually. This directory is used to identify the mines and mills that are not required to report their annual water withdrawals directly to the NMOSE. Those operations are then contacted by mail or phone to obtain withdrawal data." .

:MonthlyConsumptiveUseCoefficient%28k%29 skos:definition """k = (kt)(kc). The climatic coefficient (kt) equals 0.0173t-0.314, and kc is the crop growth
stage coefficient.""" .

:Non-AllocatedExtraction%3AIndividualUsers-AUS skos:definition "Extraction from the region's groundwater by individual users where no prior claim has been recognised for individual use" .

:Non-allocatedDiversion%3AEnvironmentalPurposes-AUS skos:definition "Surface water diverted without a recognised commitment to deliver surface water for environmental purposes." .

:Non-allocatedDiversion%3AIndividualUsers-AUS skos:definition """Surface water diverted to users other than the urban water system, under water access entitlements for which no allocation has been recognised (see line item 32.2 Surface water access entitlement for direct diversion). It includes non-allocated diversions for:
 private users and irrigation schemes where those are not identified as a water asset of the water accounting region
 allocation holders located outside the region's boundary.
It excludes non-allocated diversions for:
 irrigation schemes where those are identified as a water asset of the water accounting region""" .

:Non-allocatedDiversion%3AUrbanSystem-AUS skos:definition """Surface water diverted to an urban water system, under water access entitlements for which no allocation has been recognised. It includes non-allocated diversions for:
 allocation holders located outside the region's boundary.""" .

:PointReturn%3AIrrigation-AUS skos:definition "Point discharge from irrigation scheme to the region's surface water. It includes overflows from irrigation scheme water supply channels and discharge of used irrigation water from irrigation scheme collection systems" .

:Power%3AUnreported-NMOSE skos:definition "The New Mexico Public Regulation Commission maintains a directory of all power-generating facilities in the state. This directory is used to identify electric utility companies that are not required to report their annual withdrawals directly to NMOSE. As with other non-reporting entities, these facilities are contacted by mail and/or phone to obtain withdrawal data." .

:PublicWaterSupply%3AUnmetered-NMOSE skos:definition "For entities for which data were unavailable, information was either taken from NMEDs Water & Sewer Rate Surveys, or estimated based on population and the appropriate GPCD value for the Self-Supplied Domestic category." .

:Recharge%3AGroundwater-AUS skos:definition "Recharge from surface water to the region's groundwater. It includes the deliberate recharge of groundwater from surface water storages and rivers" .

:Recharge%3ALandscape-AUS skos:definition "Diffuse recharge from landscape to theregion'sgroundwaterdue to both natural and artificial processes. It includes irrigation induced recharge. It excludes urban infiltration basin recharge ormanaged aquifer recharge" .

:Recharge%3ASurfaceWater-AUS skos:definition "Recharge from surface water to the region's groundwater. It includes the deliberate recharge of groundwater from surface water storages and rivers." .

:RecycledWaterDelivery%3AUrbanUsers-AUS skos:definition "Delivery of recycled water from theregion'surban water systemto urban users for residential, commercial, industrial, municipal and individual irrigation use. It excludes delivery of water to theregion'sirrigation schemeswhere those are part of the w" .

:ReturnFlow%3AEnvironmentalPurposes-AUS skos:definition "The volume of returns of water from delivery service providers or water users to surface water assets for environmental use." .

:SupplySystemDelivery%3AInter-Region-AUS skos:definition "Delivery of physical water to theregion'surban water system through the supply system." .

:SupplySystemDelivery%3AUrbanUsers-AUS skos:definition "Delivery of water from theregion'surban water systemto urban users. It includes non-potable, potable and recycled water supplied from theregion'surban water systemfor residential, commercial, industrial, municipal and individual irrigation use. It e" .

:SupplySystemDischarge%3AReservoirs-AUS skos:definition "Discharge from the supply system to the regions reservoirs." .

:SupplySystemTransfer%3AInter-region-AUS skos:definition "Water transferred out of the region from the urban water system through the supply system" .

:WastewaterDischarge%3ALandscape-AUS skos:definition "The 'Discharge: landscape' volume is the metered treated wastewater discharge to landscape and/or infiltration ponds, where the primary purpose is disposal of the effluent rather than using the effluent for irrigation purposes. Also included in this volume is any other managed treated wastewater discharges not reported as discharges to surface water or sea." .

:AUS skos:definition "Australia" .

:AUSBureauOfMeteorology skos:definition "Rainfall and evaporation into/from storages and rivers were calculated using climate data from the Bureau of Meteorology interpolated to 0.05 degree (5 km) national grids (Jones et al. 2009). Calculations were done on a daily time step, with the annual totals summed from the daily values." .

:AWRA-LModel skos:definition "The AWRA-L model is a daily grid-based water balance model that is conceptualised as a small unimpaired catchment (Viney et al. 2015). It simulates the flow of water through the landscape from rainfall entering the grid cell through the vegetation and soil, and then out of the grid cell through evapotranspiration, runoff or deep drainage to the groundwater. Its inputs include gridded climate, soil, vegetation and topographic data. For more information see the Bureau of Meteorology's Australian Landscape Water Balance webpage." .

:AWRA-RModel skos:definition """AWRA-R is a river network model that represents key hydrological processes and diversions at a daily time step (Dutta et al. 2017; 2015). The model was used in the National Water Account to quantify river fluxes and stores along the river network.
The river system is conceptualised in AWRA-R as a node-link network comprising nodes connected by river reaches. Gauged streamflow data are used where available. For ungauged portions of catchment, the landscape runoff from the AWRA-L model is used (Viney et al. 2015).""" .

:AgriculturalAppliedWater-CA skos:definition """Volume of water applied on agricultural land from all sources of water to meet on-farm crop irrigation
requirements.""" .

:CAAgriculturalWaterManagementPlans skos:definition """The Water Conservation Act of 2009 (SB X7-7) requires
agricultural water suppliers serving more than 25,000 irrigated
acres (excluding recycled water deliveries) to adopt and submit
to DWR an Agricultural Water Management Plan (AWMP).
These plans had to include specific content, including reporting
on the implementation status of specific Efficient Water
Management Practices (EWMPs) that were required under SB
X7-7. In 2015, under the Drought Emergency Executive Order B-
29-15, agricultural water suppliers serving 10,000 to 25,000
irrigated acres were also required to prepare and submit an
AWMP to DWR. Additionally, all agricultural water suppliers had
to include more information in their AWMPs than required by
SB X7-7.""" .

:Cal-SIMETAWUnitValues skos:definition """The Cal-SIMETAW model was developed to compute soil water
balance to estimate crop evapotranspiration (ETc),
evapotranspiration of applied water (ETaw), and applied water
(AW) for California water resources planning. Computations are
made at a 4km resolution; output is compiled by DAUCO. Model
inputs include PRISM climate data, U.S. National Climate Data
Center climate stations, Spatial CIMIS, and SSURGO. This Cal-
SIMETAW Unit Values dataset contains cumulative monthly unit
values (per acre) of ETc, AW, and six other parameters for the
period 2000  2015. Unit values from the overlying DAUCO can
be multiplied by land use acreages to compute total ETc or AW
for a given study area. Along with ET estimates, DWR has
published the model assumptions for each DAUCO (LUCI files),
including growth periods and Kc values for each crop.""" .

:CaliforniaCentralValleySimulation%28C2VSim%29 skos:definition """DWR's C2VSim is an integrated numerical model that simulates water
movement through the linked land surface, groundwater and
surface water flow systems in Californias Central Valley using
the Integrated Water Flow Model (IWFM) modeling platform.
C2VSim contains monthly historical stream inflows, surface
water diversions, precipitation, and land use (including crop
acreage) from October 1921 through September 2009. C2VSim
dynamically calculates crop applied water, allocates
contributions from precipitation, soil moisture, and surface
water diversions, and calculates the groundwater extractions
required to meet the remaining demand. The model simulates
the historical response of the Central Valleys groundwater and
surface water flow system to historical stresses and can also be
used to simulate the response to projected future stresses.""" .

:CentralValleyHydrologicModel%28CVHM%29 skos:definition "Developed by USGS to develop monthly estimates of precipitation volume over model elements, which range in size from 0.6 to 1.5 square miles. The estimated monthly precipitation volumes are available for the periods of 1962 through 2003. Data from these numerical models can be used and the values by model elements can be aggregated to develop estimates for precipitation in the water budget zone. In addition, the pre-processing for the USGSs Basin Characterization Model includes precipitation from PRISM that have been downscaled to 270-meter spatial resolution and are available from 1900 through 2017." .

:Water-DutyBasedApproach skos:definition "In this approach, agricultural applied water is approximated based on water duty rates (also known as unit applied water) developed by local water purveyors and extrapolated to represent applied water for crops within the water budget zone. Local knowledge can be used to adjust water duty rates based on current water management practices (some areas may apply more or less than others)." .

:CropETRequirements skos:definition """Using crop data and reference ET information (ETo), calculate monthly
crop ET requirements (see Section 3.4) for all months of the growing season. Adjust crop ET based on deficit
irrigation practices within the water budget zone.""" .

:ETOfAppliedWater skos:definition """Subtract consumptive use of precipitation from the crop ET requirements
to determine consumptive use of applied water, also known as ETAW.""" .

:IrrigationEfficiency skos:definition "Obtain approximations of irrigation efficiencies from local knowledge or other sources." .

:PrecipitationVolumeForAgriculturalArea skos:definition """Obtain measured precipitation data, and
using methods described in Section 3.4., calculate monthly precipitation volume over the agricultural area during the
growing season.""" .

:RunoffVolume skos:definition "Using any of the methods described in Section 3.9, calculate monthly runoff volume over the agricultural area." .

:ApparentLosses skos:definition "The volume of apparent losses comprises two components: unauthorised consumption (e.g., water theft); and customer meter under-registration (e.g., meter inaccuracies)." .

:CADWRDemographicData skos:definition """DWR develops annual demography data for California Water
Plan Updates based on U.S. Census, American Community
Survey (ACS) and California Department of Finance (DOF) data.
The population data are computed at the various resolutions
for use by DWR in planning studies: Hydrologic Regions,
Planning Areas (PA), and Detailed Analysis Units (DAU)  a DAU
is the smallest study area. Each county consists of multiple
DAUs. The DAUs are often split by two or more counties.
DWR updates regional population data every year using GIS to
allocate census year block level population into DAU population
estimates for each of Californias 58 counties. For years that fall
between census years, DWR uses DOF's county and city total
numbers.""" .

:CADWRIrrigationMethodsSurvey skos:definition """Approximately every 10 years, a one-page irrigation survey
form is mailed out to California growers to update records on
irrigation system methods. A statewide survey of current
irrigation methods was conducted during 2011 to determine
which irrigation methods were used in California during 2010.
The 1991, 2001, and 2010 studies were conducted by mailing
questionnaires to growers who were randomly selected from a
list of growers. A list of approximately 58,000 growers in
California from the California Department of Food and
Agriculture (CDFA) was used to determine the mailing list. All
rice-only, non-irrigation, and livestock-only growers were
excluded from the list. Growers were asked to state the main
county in which they farmed and the acreages they had planted
during 2001 and 2010 to each of 20 possible crop categories by
irrigation method within that county.""" .

:CADWRLandUseViewer skos:definition """The Land Use Viewer allows groundwater sustainability
agencies (GSA) and the public to easily access both
statewide (2014 crop data) and county land use datasets (same
datasets as provided above in the DWR Land Use Survey Data)
that have been collected over the last 30 years. The Viewer also
includes a variety of tools that allow users to download and
analyze land use data. The Viewer provides consistent,
centralized land use data to improve coordination across the
State and help GSAs meet the requirements of SGMA and the
groundwater sustainability plans (GSPs) regulations.""" .

:CADWRSGMADataViewer skos:definition """The purpose of the SGMA Data Viewer is to compile and display
regional and statewide groundwater information so
groundwater sustainability agencies (GSAs) and related
stakeholders can efficiently access this information during
groundwater sustainability plan (GSP) development and
implementation.""" .

:CALSIM2 skos:definition "DWR numerical Model to develop monthly estimates of precipitation volume over model elements, which range in size from 0.6 to 1.5 square miles. The estimated monthly precipitation volumes are available for the periods of 1921 through 2015. CVHM. Data from these numerical models can be used and the values by model elements can be aggregated to develop estimates for precipitation in the water budget zone." .

:CAUrbanWaterManagementPlans skos:definition """Urban Water Management Plans (UWMPs) are prepared by
urban water suppliers every 5 years. These plans support the
suppliers long-term resource planning to ensure that adequate
water supplies are available to meet existing and future water
needs. Every urban water supplier that either provides over
3,000 acre-feet of water annually, or serves more than 3,000
urban connections is required to submit an UWMP.
Urban water includes the following uses:
 Drinking
 Toilets and showers
 Landscaping
 Car washing
 Businesses
 Industrial processes""" .

:CaliforniaAgriculturalLandAndWaterUseEstimates skos:definition """DWR estimates irrigated crop acreages, crop evapotranspiration
(ETc), evapotranspiration of applied water (ETAW), effective
precipitation (EP), and applied water (AW) for 20 crop
categories each year using the California Agricultural Water
Used Model (Ag Model). Inputs to the Ag Model include
evaporation pan data (Ep), planting and harvest dates, crop
development over time (crop coefficients), soil characteristics,
rooting depths, and precipitation. Applied water (AW) estimates
reflect irrigation efficiencies as well as the water required for
cultural practices such as the ponding of water in rice fields or
the leaching of accumulated salts from the soil.""" .

:CaliforniaDepartmentOfFinance skos:definition """The California Department of Finance provides population
estimates for historical years and future projections of
population in five-year increments through 2060. Population
estimates and projections are available at the city and county
level.""" .

:CaliforniaPesticideInformationPortal skos:definition """The California Pesticide Information Portal (CalPIP) provides
access to a collection of pesticide use information. At the heart
of CalPIP is a data warehouse that serves up pesticide data
produced, maintained, and used by a variety of programs within
DPR. The Pesticide Information Portal can be used to determine and
refine estimation of crop planting periods as well as spatial
coverage of different crop types by examining the distribution
of pesticide applications.""" .

:CaliforniaWaterPlanPortfolio skos:definition """DWRs California Water Plan team has a spreadsheet model, called the Water Portfolio, that provides an accounting of water budget components by DAUCO using collected data and analysis tools. This accounting occurs annually, and data are available for the period 2002 to 2015. The Water Portfolio incorporates data and analysis resulting in estimates of ET, ET of applied water, and applied water
by crop type by DAUCO.""" .

:DWRLandUseSurveys skos:definition """Since 1950 DWR has conducted over 250 land use surveys of all
or parts of California's 58 counties. Early land use surveys were
recorded on paper maps of USGS 7.5' quadrangles. In 1986,
DWR began to develop georeferenced digital maps of land use
survey data. The main emphasis of DWR's land use surveys is
the mapping of agricultural land. Over 70 different crops or crop
categories are included in the surveys. Irrigation methods and
water sources have also been mapped in some, but not all
surveys. Urban and native vegetation (undeveloped) areas are
mapped but not in the detail of agricultural land. DWR staff visit
and visually identify land uses on over 95 percent of the
developed agricultural areas within each survey area.""" .

:SWRCBWaterConservationPortal skos:definition """The State Water Resources Control Board has been collecting
water production information from urban water suppliers since
the July 2014 board action to adopt an emergency water
conservation regulation. In November 2017, the emergency
water conservation regulation expired, and monthly reporting is
now voluntary.""" .

:USDACropScape skos:definition """The United States Department of Agriculture has produced a
remotely sensed crop data layer (CropScape) that is publicly
available for California for 2007 through 2016. These data are a
gridded dataset with 30-meter by 30-meter pixels each with a
single crop identified.
CropScape can generally differentiate classifications of land
coverage (permanent crops vs. annual crops vs. urban).
However, it has difficulty accurately distinguishing between
native grassland and irrigated pasture as well as between
different types of orchards. Additionally, the individual land use
identified is often not consistent between years.""" .

:USDANaturalResourcesConservationServiceGeospatialWebSoilSurvey skos:definition """Web Soil Survey (WSS) provides soil data and information
produced by the National Cooperative Soil Survey. NRCS has soil
maps and data available online for more than 95 percent of the
nations counties and anticipates having 100 percent in the
future. The site is updated and maintained online as a single
authoritative source of soil survey information.""" .

:CAIntegratedWaterFlowModel%28IWFM%29 skos:definition """IWFM is a computer program used for water resources
management and planning within a basin. It calculates
groundwater flows, soil moisture movement in the topsoil,
stream flows, land surface flows, and flow exchange between
groundwater, streams, and land surface as generated by
precipitation, agricultural irrigation, and municipal and
industrial water use. IWFM also calculates agricultural applied
water based on crop types, crop acreages, soil types, irrigation
methods and rainfall rates, as well as the municipal and
industrial applied water based on population and per-capita
water use rates. IWFM can help water managers understand
the historical evolution of the surface and subsurface water
flows within their basin, and plan the use of groundwater and
surface water to meet future applied water needs.""" .

:CAIntegratedWaterFlowModel%28IWFM%29DemandCalculator skos:definition """IDC is the stand-alone executable version of the root zone
component of the Integrated Water Flow Model (IWFM). It
calculates agricultural, urban, managed wetlands, and native
vegetation water uses at a river-basin scale under user-specified
climatic, soil and land-use characteristics. It also routes
precipitation and irrigation water through the root zone, and
simulates land-surface and root zone flow processes. It can be
linked to finite-element as well as finite-difference type
integrated hydrologic models. IDC uses a computational grid to
represent spatial distribution of land use, climatic, soil and farm
management properties.""" .

:CaliforniaStateGroundwaterElevationMonitoring%28CASGEM%29 skos:definition """In accordance with the Water Code, DWR developed the
California Statewide Groundwater Elevation Monitoring
(CASGEM) program. The intent of the CASGEM program is to
establish a permanent, locally-managed program of regular and
systematic monitoring in all of California's alluvial groundwater
basins. The CASGEM program will rely and build on the many,
established local long-term groundwater monitoring and
management programs. DWR's role is to coordinate the
CASGEM program, to work cooperatively with local entities, and
to maintain the collected elevation data in a readily and widely
available public database. DWR will also continue its current
network of groundwater monitoring as funding allows.""" .

:MODFLOW-OWHM%3AOneWaterHydrologicFlowModel skos:definition """The One-Water Hydrologic Flow Model (MF-OWHM) is a
MODFLOW-based integrated hydrologic flow model. MFOWHM
allows the simulation, analysis, and management of
nearly all components of human and natural water movement
and its use in a physically-based supply-and-demand
framework. The supply-constrained and demand-driven
framework combined with the linkages between packages and
processes provides relations of water use and movement, and
helps to prevent mass loss to an open system thus facilitating
the accounting for all of the water everywhere and all of the
time.\"""" .

:NationalLandCoverDataBase%28NLCD%29 skos:definition """As with two previous NLCD land cover products, NLCD 2011
keeps the same 16-class land cover classification scheme that
has been applied consistently across the United States at a
spatial resolution of 30 meters. NLCD 2011 is based primarily on
a decision-tree classification of circa 2011 Landsat satellite data.""" .

:USDACountyAgCommissioner%27sDataListing skos:definition """This summary, which is published annually, is based on the
annual Crop Reports compiled by the California County
Agricultural Commissioners. These reports provide the most
detailed annual data available on agricultural production by
county. As of crop year 2011, the Summary and Data reports
are combined into one publication.""" .

:VegetationConditionExplorer%28VegScape%29 skos:definition """The vegetation condition refers to the density of vegetation,
which changes through a plants growth cycles.
Vegetation indices available:
 Normalized difference vegetation index (NDVI) products
- Current Vegetation Condition Explorer can provide
daily weekly and biweekly NDVI products from 2000 to
2013.
 Vegetation Condition Index (VCI) products - represents
the weather condition or the vegetation condition.
Currently Vegetation Condition Explorer can provide
weekly and biweekly VCI products from 2000 to 2013.
The Annual crop condition can be plotted from downloaded
data or using the interface.""" .

:WaterUseClassificationOfLandscapeSpecies%28WUCOLS%29 skos:definition """WUCOLS IV provides evaluations of the irrigation water needs
for over 3,500 taxa (taxonomic plant groups) used in California
landscapes. It is based on the observations and extensive field
experience of thirty-six landscape horticulturists and provides
guidance in the selection and care of landscape plants relative
to their water needs.""" .

:WesternMountLoftyRangesPrescribedWaterResourcesAreaWaterAllocationPlan skos:definition
    "Groundwater discharge to surface water in the Western Mount Lofty Ranges PWRA was summed from the annual baseflow figures detailed in the Western Mount Lofty Ranges PWRA Water Allocation Plan." .

:BaseflowSeparationTechniques skos:definition """Streamflow is fed by both surface runoff and by subsurface flow from riparian aquifers. The streamflow resulting from groundwater outflow is called baseflow. Similar to the mass balance approach discussed earlier, a separate but related approach is to use stream gaging stations immediately upstream and downstream of a water budget zone and perform a hydrograph analysis to determine the baseflow from the hydrograph. This allows the computation of groundwater contributions, even during stormwater events. There are numerous methods for baseflow separation. The USGS maintains the following software to calculate baseflow using streamflow timeseries data: HYSEP: Hydrograph Separation Program (http://water.usgs.gov/software/HYSEP/)
Purdue University maintains a similar program that utilizes USGS daily streamflow data to do a similar hydrograph
analysis. It is: WHAT: Web-based Hydrograph Analysis Tool (https://engineering.purdue.edu/~what/)""" .

:CACountyAgriculturalCommissionerCropReports skos:definition """California Department of Food and Agriculture provides links to
the various County Annual Crop Reports. Crop Reports can also
be accessed directly from the County Agricultural Commissioner
in your area of interest. As required by the California Food and
Agriculture Code, the County Agricultural Commissioner
compiles and records information in the annual crop and
livestock report regarding the gross production and value of the
countys commodities.""" .

:CALSIM3 skos:definition """CalSim 3 is the next generation of the CalSim 2 (C2VSim) model. Major
improvements and enhancements in CalSim 3 include:
 Finer model spatial resolution
 Better water supply and demand estimation
 Improved groundwater representation and simulation
 Enhanced model validation
 Extended model spatial and temporal domain
 Advanced model engine (WRIMS 2.0)
 Thorough model documentation
 Model supporting tools""" .

:CAValidatedWaterLossReporting skos:definition """Water loss audits evaluate real water losses (leaks) and
apparent water losses (e.g. data errors, water theft) occurring
in a potable water distribution system. Water loss audit
submissions are reviewed by validators. The reviews followed
the validation methodology detailed in Water Research
Foundation Project 4639: Level 1 Water Audit Validation. Level
1 water audit validation aims to:
1) Identify and, where possible, correct inaccuracies in
water audit data and application of methodology.
2) Evaluate and communicate the uncertainty inherent in
water audit data.""" .

:CSIROWavesModel skos:definition "The CSIRO WAVES model was used to calculate flows from some of the specific land use areas, such as agriculture, pine plantations, and native bushland (simpler models are used for general land use areas including residential, industrial, and parkland areas)." .

:CaliforniaNevadaRiverForecastCenter skos:definition """Contains current flow data for river and reservoir gauge
throughout California""" .

:ChangeInGroundwaterLevel skos:definition "The change in groundwater storage is calculated as the product of (1) the difference in groundwater elevation between two monitoring periods, (2) the area overlying the water budget zone, and (3) the average specific yield in an unconfined aquifer or storativity in a confined aquifer. Change in Groundwater Storage = (GWEt0  GWEt1) x Overlying Area x Specific Yield" .

:GroundwaterElevation skos:definition """The average groundwater elevation in an overlying area can be developed from point groundwater elevation measurements at wells at a given period of time using GIS interpolation function. Interpolating the point groundwater
elevations in GIS allows for spatial weighting and removes some of the uncertainty associated with using point measurements over a larger area. Caution should be taken when developing the average groundwater elevations from a monitoring network. Depending on the network of wells, areas with less data will likely result in higher uncertainty in groundwater elevation estimates.""" .

:SpecificYield skos:definition "Specific yield represents the water-yielding capacity of a material and is defined as the ratio of the volume of water that will drain by gravity from a saturated rock or soil compared to the total volume of rock or soil. Specific yield values can be determined in the field or laboratory using direct or indirect methods." .

:CADWRBulletin118%3AGroundwaterReport skos:definition """Bulletin 118 is Californias official compendium on the
occurrence and nature of groundwater statewide. Bulletin 118
defines the boundaries and describes the hydrologic
characteristics of Californias groundwater basins. Bulletin 118
also provides information on groundwater management and
recommendations for the future.
With the passage of SGMA in 2014, Bulletin 118 now serves an
additional role by providing groundwater sustainability agencies
with three critical pieces of information regarding groundwater
basins: Critical Conditions of Overdraft, Basin Boundaries, and
Basin Priority.""" .

:CaliforniaDataExchangeCenter%28CDEC%29 skos:definition """CDEC provides a centralized database to store, process, and
exchange real-time hydrologic information gathered by various
cooperators throughout the State. The data collected by CDEC
enable forecasters to prepare flood forecasts and water supply
forecasts; reservoir and hydroelectric operators to schedule
reservoir releases; and water suppliers to anticipate water
availability.
The two main entities that collect and manage data related to
flood forecasting and response for California are CDEC and the
NWS California-Nevada River Forecast Center (CNRFC).
Collection efforts by the CNRFC are centered on data necessary
to fulfill its mission of flood forecasting. CDECs original data
collection efforts revolved around supporting the State-Federal
Flood Operations Center (FOC), but since have grown into
managing hydrometeorological data statewide for a variety of
resource management uses.""" .

:GravityRecoveryAndClimateExperiment%28GRACE%29 skos:definition """Launched in March of 2002, the GRACE mission is to accurately
map variations in Earth's gravity field. GRACE consists of two
identical satellites that fly about 220 kilometers (137 miles)
apart in a polar orbit of 500 kilometers (310 miles) above Earth.
The Earth's gravity field is mapped by making accurate
measurements of the distance between the two satellites, using
GPS and a microwave ranging system. The results from this
mission are yielding crucial information about the distribution
and flow of mass within Earth and its surroundings.
The gravity variations studied by GRACE include: changes
caused by surface and deep currents in the ocean; runoff and
ground water storage on land masses; exchanges between ice
sheets or glaciers and the ocean; and variations of mass within
Earth. Another goal of the mission is to create a better profile of
Earth's atmosphere.""" .

:MassBalance skos:definition """Perform a mass balance on the conveyance facilities using available seepage and conveyance flows at the desired time step over the period of interest. If an estimate for conveyance seepage is not available, the mass balance approach will not work. 
Apply the following mass balance calculation to determine Conveyance Evaporation (Ec) for the period of interest at the desired time increment (e.g., monthly):
Ec =  Surface Water Diversions (Inflow) +  Imported Water (Inflow) -
 Surface Water Deliveries (Outflow) -  Conveyance Seepage (Outflow)  Operational Spills (Outflow)""" .

:WaterBalanceForUnsaturatedZoneStorage skos:definition """Estimating the change in unsaturated zone storage is often a difficult task that requires the use of modeling software
and the estimation of unsaturated zone properties. If conducting such an analysis is not feasible, then a simple water balance of using the other subcomponents can be used to make the initial estimates of change in unsaturated zone storage. If ponded water storage analysis and root zone soil moisture storage balances are computed, then the
unsaturated zone storage can be computed.""" .

:WaterUseModels skos:definition """crop and managed wetlands water use models that use soil moisture storage balances to
determine crop water use. That analysis should have a daily or monthly soil moisture storage for the root zone.""" .

:HYDRODatabase skos:definition "Storage volume at the start and end of the year was calculated using water level data (metres above Australian Height Datum) collected at each storage. Capacity tables established for each storage were used to convert the height measurement to a volume." .

:USBRCentralValleyProjectRefugeWaterDeliveryData skos:definition """Website contains operational reports for Central Valley Project
operations.""" .

:USGSSurface-WaterDataForCalifornia skos:definition """The USGSs National Water Information System (NWIS) is a
comprehensive and distributed application that supports the
acquisition, processing, and long-term storage of water data.
Water Data for the Nation serves as the publicly available
portal to a geographically seamless set of much of the water
data maintained within NWIS.
Nationally, USGS surface-water data includes more than
850,000 station years of time-series data that describe stream
water levels, streamflow (discharge), reservoir and lake levels,
surface-water quality, and precipitation. The data are collected
by automatic recorders and manual field measurements at
installations across the Nation. The data relayed through the
Geostationary Operational Environmental Satellite (GOES)
system are processed automatically in near real time, and in
many cases, current data are available online within minutes.
Once a complete day of readings are received from a site, daily
summary data are generated and made available online. USGS
finalizes data at individual sites on a continuous basis as
environmental conditions and hydrologic characteristics permit.""" .

:CenterForHydrometeorologyAndRemoteSensingDataPortal%28CHRS%29 skos:definition """CHRS Data Portal is an archive for global satellite precipitation
data and information produced by the PERSIANN, PERSIANNCCS,
and PERSIANN-CDR systems developed by CHRS and
directed by Dr. Soroosh Sorooshian at the UC Irvine.
CHRS Data Portal allows users to visualize and download
spatiotemporal statistics of global regular-interval satellite
precipitation from the PERSIANN, PERSIANN-CCS, and
PERSIANN-CDR systems.""" .

:CityWestWaterAnnualReport skos:definition "Water Utility" .

:ConstantPercentage skos:definition "A simpler method with lower accuracy for quantifying recharge of precipitation is to assume that a fixed percentage of precipitation is recharged to the groundwater system. This fixed percentage could be based on previous studies or existing models for areas that are similar to the water budget zone of interest. The percentage may vary from basin to basin and is dependent on land use conditions, hydrology, and soil type. The percentage of precipitation that is recharged into groundwater varies from 5 percent to 20 percent in the Central Valley of California (Brush et al., 2013)." .

:ConstantSeepagePercentage skos:definition """A simpler method with lower accuracy for quantifying the gains to the groundwater system from a stream is to
assume that a fixed percentage of total streamflow volume flows to the groundwater system as seepage over the
length of the stream (or a stream reach). The same assumption can be made for canals to estimate the conveyance facility seepage to the groundwater system in a water budget zone.""" .

:NOAANationalCentersForEnvironmentalInformation-ClimateDataOnline skos:definition
    """COOP stations data are collected from a variety of sources
including National Weather Service reporting stations,
volunteer cooperative observers, Federal Aviation
Administration (FAA), utility companies, etc.""" .

:NOAANationalCentersForEnvironmentalInformation-ClimatologicalDataPublications skos:definition
    """The climate data publications are a compilation of observations
from weather sites supervised by NOAA/National Weather
Service and received at the National Centers for Environmental
Information (NCEI). Monthly editions contain station daily
maximum and minimum temperatures and precipitation. Some
stations provide daily snowfall, snow depth, evaporation, and
soil temperature data. Each issue also contains monthly
summaries for heating and cooling degree days. The July issue
also contains monthly heating degree days and snow data for
the preceding July through June. The annual issue contains
monthly and annual averages of temperature, precipitation,
temperature extremes, freeze data, soil temperatures,
evaporation, and a recap of monthly cooling degree days.""" .

:NWSCLIMATEPREDICTIONCENTEREVAPORATION skos:definition """A series of maps showing current month and most recent 12
months average evaporation and anomalies; previous 12
months percentiles; evaporation climatology and 1- and 2-week
outlooks. This evaporation is computed from a soil moisture
balance model that uses precipitation and temperature as
inputs.""" .

:CADWRBulletin132%3AManagementOfTheCaliforniaStateWaterProject skos:definition """Bulletin 132 is an annual series of reports describing SWP
status, operations and water deliveries. Each report updates
project costs and financing, water supply planning, power
operations and significant events that affect SWP management.
Hydrologic information for the water year, capital construction
information for the fiscal year, and water delivery, operations,
maintenance and other activities for the calendar year are
included as well. The complete report series, beginning in 1963,
is available below in PDF format.""" .

:CaliforniaIrrigationManagementInformationSystem%28CIMIS%29 skos:definition """CIMIS includes over 145 weather stations used to assist
irrigators in managing their water resources more efficiently.
CIMIS station data include measured parameters such as solar radiation, air temperature, soil temperature, relative humidity,
wind speed, and wind direction, and derived parameters such
as vapor pressure, dew point temperature, and reference
evapotranspiration (ETo).""" .

:DWRBulletin73%3AEvaporationFromWaterSurfaceInCalifornia%281979%29 skos:definition
    """Bulletin 73-79 summarizes all readily available data on
evaporation pan measurements in California up to 1979. It
reports monthly total evaporation data from 478 stations,
dating back to the 1880s.""" .

:Evapotranspiration%28ET%29Rates skos:definition """Open water evaporation for shallow water bodies can be estimated by multiplying water surface area by a unit ET rate for shallow, open water. The unit ET rates can be either
Option 1  obtain DWR estimates of statewide regional unit ET rates
Option 2  compute from reference ET using either CIMIS station data or Spatial CIMIS and a representative
crop coefficient for shallow, open water.
Option 3  obtain ET data from alternative sources.""" .

:s.71WaterResourceReport skos:definition "(Section 71 of the Water Act 2007) data and water sharing plans" .

:EstimateConveyanceSeepageRateBasedOnCanalCharacteristics skos:definition "Conveyance Seepage can be estimated based on the lining of canals, soil characteristics, wetted perimeter, length of canal, and hydraulic conductivity of canal bed." .

:CropCoefficientApproach skos:definition """\"In this method, the volume of crop (or vegetation) ET is obtained by multiplying the crop acreage with the crop ET
rate (ETc).   (  ) =  ()   ()
Where, ETc is defined as
 =   \"""" .

:CAIrrigationTrainingAndResearchCenter%28ITRC%29EvapotranspirationData skos:definition
    """The Irrigation Training & Research Center (ITRC) provides
estimates of crop and soil unit (per acre) evapotranspiration
values for 1997  1999 for specific irrigation methods and
precipitation amount in different zones within California. ITRC
offers ET data for two purposes: water balance, and irrigation
scheduling and design. The monthly ET data for different land
cover (23 crop types) are provided for 13 of the 18 ETo zones.""" .

:SpatialCaliforniaIrrigationManagementInformationSystem%28CIMIS%29 skos:definition
    """Many areas of California are not sufficiently covered by the
network of CIMIS stations. Recognizing these spatial data gaps,
CIMIS, in cooperation with the UC Davis, developed a daily ETo
(reference evapotranspiration) map known as Spatial CIMIS.
The ETo maps are generated using complex sets of models. The
input parameters to these models are combinations of data
from satellites and ground measurements. Spatial CIMIS data
consists of ETo and solar radiation only. Daily reference
evapotranspiration (ETo) at a 2-km spatial resolution are
calculated statewide using the American Society of Civil
Engineers version of the Penman-Monteith equation (ASCEPM).
Daily solar radiation is generated from the visible band of
the National Oceanic and Atmospheric Administration's (NOAA)
Geostationary Operational Environmental Satellite (GOES) using
the Heliosat-II model.""" .

:CulturalPractices skos:definition """Cultural Practices (CP) = (Flood-up Volume + Circulation Water +Forage Irrigation) per acre
o Flood-up volume includes saturating soil pore space and depth of ponding.
o Circulation is the continuous flow rate needed for waterfowl disease management.
o Forage irrigation is the water applied to grow seed producing vegetation for waterfowl and
commonly consists of one or two applications of water about 3 inches in depth.""" .

:CumulativeWaterMeter skos:definition "The allocated abstraction of water for the urban water system during the licensed water year is based on measured data collected at the outlet of the water source using a cumulative water meter." .

:DailyWaterBalanceApproach skos:definition "The volume of water in the river channels at 30 June was estimated by using the daily water balance approach within the AWRA-R model. The water balance includes inflow at the upstream nodes and outflow at the downstream nodes; contributing catchment runoff, reservoir contribution, irrigation diversion and return; overbank flooding and floodplain return; loss to groundwater; anabranch flow; rainfall; and evaporation." .

:DepartmentOfWaterAndEnvironmentalRegulation skos:definition "The Department of Water and Environmental Regulation requires that all water meters, when tested under in situ conditions, must be within 5% accuracy across the full flow rate range (Department of Water 2009c )." .

:DrainageAreaOfSiteOfInterest skos:definition "Ay is the drainage area (square miles) of the site of interest" .

:DrainageAreaRatioMethod skos:definition "When stream inflows enter the water budget zone from unimpaired watersheds, the drainage-area ratio method can be used to estimate streamflows. The method is based on the assumption that streamflows for a site of interest can be approximated from gauged streamflow data at the nearby site by using the ratio of drainage area of the site of interest and drainage area of the nearby site" .

:DrainageAreaOfStreamflowGagingStation%28Ax%29 skos:definition "Ax is the drainage area (square miles) of the streamflow gaging station where measured data is available" .

:MeasureStreamflow%28Xij%29 skos:definition """Xij is the measured streamflow (cubic feet per second) for month i and year j for the streamflow gaging
station""" .

:EstimateAppliedWaterReuseAndRecycledWaterVolumes skos:definition """Recycled water and applied water reuse can be estimated for urban, agricultural, and managed wetlands systems using methods like those used in the California Water Plan. Recycled water data are generally measured and reflect internal reuse within the urban sector; however, unmeasured recycled water may include treated wastewater recycling, disposal through irrigation of landscape or other vegetation, or treated water percolated as managed aquifer recharge (including injection wells for seawater intrusion control). Recycled water data can be obtained from municipal water suppliers and waste water treatment plants, but where it is unavailable, it can be estimated based on the volumes of applied water. This method would calculate recycled water as: 
Recycled Water = Urban Applied Water  Surface Water Delivery  Groundwater Extraction
or
Applied Water Reuse (Ag, Urban, MW) = AW - SWdel - GWext for all applied water and all supplies""" .

:EstimationOfAbstraction skos:definition """For licences that expired and were renewed during the reporting year, the volume of abstraction is estimated to be the full licensed allocation.
For licences that expired during the reporting year (and were not renewed), the volume of abstraction is estimated to be the allocation remaining at the start of the year (1 July). That is, the allocation remaining at the start of the year is assumed to be abstracted before the licence expired.
For new licences that were created during the reporting year, the volume of abstraction is estimated to be the full allocation, multiplied by the ratio of the number of days from the licence issue date until the end of the year (30 June) and the number of days in the year.""" .

:Morton%27sShallowLakeFormulation skos:definition "Evaporation was estimated using Morton's shallow lake formulation (Morton 1983)." .

:EvaporationPanMethod skos:definition """If there are no evaporation estimates, but pan evaporation data are available, the following formula can be used to
estimate evaporation loss from a water body.
 =     """ .

:MeasuredPanEvaporationRate skos:definition "E pan = Measured pan evaporation rate" .

:PanCoefficient skos:definition """K p = Pan coefficient, a correction factor to the actual evaporation rate, with a range from 0.64 to 0.81 and
an average of 0.70 for the United States. This coefficient is specific for each water body and varies with the
geometry of the lake, water depth, lake surface conditions (turbidity, presence of vegetation), and local
weather conditions. Local or regional calibration or verification of the pan coefficients used is highly
recommended, and caution is needed to account for poor pan siting and handling.""" .

:USGSBasinCharacterizationModel skos:definition """The BCM can translate fine-scale maps of climate trends and
projections into the hydrologic consequences, to permit
evaluation of the impacts to water availability at regional,
watershed, and landscape scales, as caused by changes in
temperature and precipitation. The BCM was developed at a
270-m spatial resolution, using monthly data, and has been
supported by numerous federal, state, and local agencies, and
international organizations. The BCM uses historical climate
data from 1896-2010, and an ensemble of 18 future climate
projections that were used to develop hydrologic output such
as snowpack, recharge, runoff, and climatic water deficit. To
produce this dataset, digital maps of soils and geology for the
California hydrologic region were integrated with monthly maps
of climate and hydrology, to generate average water year and
30-year water year maps for the historical record (1951-1980
and 1981-2010) and future projections (2010-2039, 2040-2069,
and 2070-2099).""" .

:CADWRBulletin113%3ACropWaterUse skos:definition """Bulletin 113-4: Crop Water Use in California (April 1986) is the
fourth in a series of Department publications that provides the
basis for estimating per-acre ET of water and the quantities of
water applied by irrigation. The data presented was collected
during 1973 through 1983.
Bulletin 113-3: Vegetative Water Use in California, 1974 (April
1975) is the third in a series of DWR publications on the rate of
water use by crops. The report is based on field studies
conducted from 1954 to 1972, and expands the previously
published data. It summarizes growing season ET and ETAW
water for principal crops.""" .

:MOD16%3AMODISGlobalEvapotranspirationProject skos:definition """The MOD16 evapotranspiration (ET) datasets are estimated
using Mu et al.s improved ET algorithm (2011) over previous
Mu et al.s paper (2007a). The ET algorithm is based on the
Penman-Monteith equation (Monteith, 1965). Surface
resistance is an effective resistance to evaporation from land
surface and transpiration from the plant canopy. Terrestrial ET
includes evaporation from wet and moist soil, from rain water
intercepted by the canopy before it reaches the ground, and
the transpiration through stomata on plant leaves and stems.""" .

:NOAAOfficeOfSatelliteAndProductOperationsALEXI%3AAtmosphere-LandExchangeInverseModel
  skos:definition """GOES Evapotranspiration and Drought (GET-D) products are
derived from the Atmosphere-Land Exchange Inversion model
(ALEXI). ALEXI computes principle surface energy fluxes,
including Evapotranspiration (ET), which is a critical boundary
condition for weather and hydrologic modeling, and a quantity
required for regional water resource management. ALEXI ET
estimates have been rigorously evaluated in comparison with
ground-based data, and perform well over a range in climatic
and vegetation conditions.
The GET-D system is designed to generate ET and drought maps
operationally. ALEXI ET is retrieved over clear-sky pixels daily
and ALEXI drought product is generated over 1 to 6-month
compositing periods each day.""" .

:NorthAmericanLandDataAssimilationSystem%28NLDAS-2%29 skos:definition """The goal of the North American Land Data Assimilation System
(NLDAS) is to construct quality-controlled, and spatially and
temporally consistent, land-surface model (LSM) datasets from
the best available observations and model output to support
modeling activities. Specifically, this system is intended to
reduce the errors in the stores of soil moisture and energy
which are often present in numerical weather prediction
models, and which degrade the accuracy of forecasts. NLDAS is
currently running in near real-time on a 1/8th-degree grid over
central North America; retrospective NLDAS datasets and
simulations also extend back to January 1979. NLDAS constructs
a forcing dataset from gauge-based observed precipitation data
(temporally disaggregated using Stage II radar data), biascorrecting shortwave radiation, and surface meteorology reanalyses to drive several different LSMs to produce model
outputs of surface fluxes, soil moisture, and snow cover.
Phase 2 of NLDAS is referred to as NLDAS-2 and covers the
period 2-Jan-1979 to present.""" .

:OperationalSimplifiedSurfaceEnergyBalance%28SSEBop%29 skos:definition """Actual ET (ETa) is produced using the operational Simplified
Surface Energy Balance (SSEBop) model (Senay and others,
2013) for the period 2000 to 2015. The SSEBop setup is based
on the Simplified Surface Energy Balance (SSEB) approach
(Senay and others, 2007, 2011) with unique parameterization
for operational applications. It combines ET fractions generated
from remotely sensed MODIS thermal imagery, acquired every
8 days, with reference ET using a thermal index approach. The
unique feature of the SSEBop parameterization is that it uses
pre-defined, seasonally dynamic, boundary conditions that are
unique to each pixel for the hot/dry and cold/wet reference
points.""" .

:TOPS-SIMS%3ASatelliteIrrigationManagementSupport skos:definition """Different than other remote sensing ET models, Satellite
Irrigation Management Support (SIMS) is based on vegetation
indices, rather than the energy balance (e.g. METRIC-EEFLUX,
MOD16, etc.). SIMS captures vegetation growth (amount of
green biomass) but cannot capture changes in crop
temperature caused by stress because, unlike the energy
balance methods, SIMS does not use thermal information. SIMS
also doesnt account for evaporation from wet bare soil. The
advantage of SIMS is that it can use more satellites which
results in more frequent observations, at higher resolution.""" .

:FloodplainModule skos:definition "The AWRA-R floodplain module was used to model the volume of overbank flow from the river onto the floodplain, and the return flow from the floodplain back into the river. The module applies a simple storage-based floodplain model to each river reach. The floodplain modelling method is detailed in Dutta et al. (2013)." .

:FlowData skos:definition "the total river outflow was estimated using flow data collected at the most downstream gauging stations nearest to the outlet to the sea" .

:FlowNetAnalysis skos:definition """The flow net analysis is a graphical method for solving groundwater flow using the Darcys law as presented by
Cedergren (1997) and USGS (2008). The method involves drawing equipotential lines (lines of equal hydraulic head)
based on hydraulic head in the wells and flow lines (also called streamlines) based on stage in the surface-water
body. The flow lines are drawn perpendicular to both the no-flow boundaries and to the equipotential lines, which
assume the porous medium is homogeneous and isotropic. The number of flow lines to be drawn should result in
rectilinear shapes that approximate squares. The areas between the flow lines are called streamtubes, and the
intervals between equipotential lines are termed head drops. After constructing the flow net, Darcys law is used to
approximate flow to or from the surface-water body:
 =       /""" .

:GISGroundwaterModelling skos:definition """Regional and coastal groundwater flow into and out of the Adelaide region was calculated using a simple GIS approach based on Darcy's Law. A set of bores with current data was selected, including any bores within 20 km of the region's boundary.  Where no bores were present close to the boundary, the interpolated groundwater level surface was extended to the boundary and used to estimate groundwater flow across the boundary (this flow is small in magnitude).

Groundwater levels measured at monitoring bores were interpolated to a groundwater-level grid for each season during the 201718 year using the ArcGIS Topo-to-Raster tool. Seasonal groundwater-flow grids were then derived from these groundwater-level grids along with aquifer thickness and hydraulic conductivity data, using a modification of the ArcGIS Darcy velocity tool. Regional groundwater inflow/outflow was subsequently calculated across selected regional groundwater boundaries in the Adelaide Plains, using a simple GIS analysis. Coastal groundwater inflow/outflow was subsequently calculated across selected coastal boundaries in the Adelaide Plains and McLaren Vale PWAs using a simple GIS analysis.""" .

:Darcy%27sLaw skos:definition """Subsurface flows between two water budget zones depend on the groundwater level gradient between boundary of
the two zones. Darcys Law and groundwater elevation gradient data across the boundary can quantify the
subsurface inflows (and outflows) from adjacent groundwater basins using the following equation:
 =     
 =       
 =     """ .

:GippslandWaterAnnualReport skos:definition "Water Utility" .

:Peel-HarveyRegionalAquiferModelingSystem%28PHRAMS%29 skos:definition """The Department of Water and Environmental Regulation uses the Perth Regional Aquifer Modelling System (PRAMS) version 3.5 and PeelHarvey Regional Aquifer Modelling System (PHRAMS) to estimate the natural water movement to and from the groundwater store within the Perth region (Davidson and Yu 2008; URS 2009).
PHRAMS estimates groundwater movement for the PeelHarvey area south of Mandurah. The volumes reported in this account refer to the natural water movement that occurs within each model area within the Perth region boundary.""" .

:PerthRegionalAquiferModelingSystems%28PRAMS%29 skos:definition """The Department of Water and Environmental Regulation uses the Perth Regional Aquifer Modelling System (PRAMS) version 3.5 and PeelHarvey Regional Aquifer Modelling System (PHRAMS) to estimate the natural water movement to and from the groundwater store within the Perth region (Davidson and Yu 2008; URS 2009).
PRAMS estimates groundwater movement for the area north of Mandurah.he volumes reported in this account refer to the natural water movement that occurs within each model area within the Perth region boundary.""" .

:LandUseAndAppliedWaterEstimationMethod skos:definition "Groundwater exports from a water budget zone can be estimated by calculating the amount of applied groundwater at the place of use and adding the conveyance losses for transporting the groundwater to its place of use. Volumes of on-farm total applied water can be determined by estimating crop types, acreage, and irrigation practices at the place of use and using the estimates of applied water as calculated in Section 3.5.1  Agricultural Applied Water. Applied groundwater is calculated by subtracting the surface water deliveries and applied water reuse from the total applied water needed." .

:GroundwaterExtractionUnderStatutoryRightsEstimationMethod skos:definition """Groundwater extraction under other statutory rights is an estimate based on water allocation plans or spatial assessments. The assessments take into account variables such as number of properties, stock water requirements, and the distance stock must travel for water.

More information on water allocation plans in the region (Tindall Limestone and Oolloo Dolostone aquifers) can be found at the Department of Environment and Natural Resources website""" .

:GroundwaterModelling skos:definition """Inter-region inflow into the region' was estimated for the unconfined aquifer (Murray Group Limestone and Parilla Sands) and confined aquifer (Renmark Group) that underlie this boundary.

'Inter-region outflow from the region' refers to the lateral outflow from the aquifers into the Murray Limestone and Renmark Group aquifers near the Murray mouth.

The uncertainty in the field-measured data (e.g. groundwater levels, hydraulic conductivity) was not specified and is unknown, and hence the impacts of such uncertainty on the calculated groundwater flow were not estimated.""" .

:ExistingWaterRightInformationFromStateWaterResourcesControlBoard%28SWRCB%29 skos:definition
    """The Electronic Water Rights Information Management System
(eWRIMS) is a computer database developed by the State
Water Resources Control Board to track information on water
rights in California. eWRIMS contains information on
Statements of Water Diversion and Use that have been filed by
water diverters, as well as registrations, certificates, and water
right permits and licenses that have been issued by the State
Water Resources Control Board and its predecessors.""" .

:ManagedWetlandAppliedWater-CA skos:definition """Volume of water delivered from any source as either direct or incidental flows to a marsh or wetland for
wildlife areas. This would equal the volume of surface water delivery, groundwater water extraction, and reuse.""" .

:OrdIrrigationCooperative%3APacksaddleAndIvanhoePlains skos:definition "licence entitlements" .

:WaterCorporation%3AM1Channel skos:definition "licence entitlements" .

:MassTransferEquations skos:definition """The evaporation rate of streams and rivers can be estimated by calibrating mass transfer equations. The evaporation
rate is proportional to the vapor pressure deficit and wind speed, according to the equation""" .

:USGSPublications skos:definition """Many USGS reports on water resources are now being served
online. Most publications located at this site and other USGS
sites can be located by subject, author, date, USGS series or
publication series number by using the reports and thematic
maps.""" .

:MassCurve skos:definition "A mass curve is a plot of cumulative inflow into a reservoir overtime. Although usually used to determine reservoir capacity, outflows from a reservoir can be calculated from reservoir storage and demand" .

:ConsumptiveUseOfPrecipitation%28EP%29 skos:definition """The consumptive use of precipitation, also known as effective precipitation (EP), is that portion of the precipitation that is not runoff but is stored in the root zone and contributes to meeting the ET requirements during the growing season. It can be approximated as follows:
Consumptive Use of Precipitation (EP) = Minimum [(Precipitation (P)  Runoff (R)), Evapotranspiration (ET)]""" .

:LandscapeIrrigation skos:definition """Landscape irrigation includes golf courses and parks where the irrigated area and unit applied water values
can estimate supply.""" .

:LandscapeModelledRunoff skos:definition "The AWRA-L model is a daily grid-based water balance model that is conceptualised as a small unimpaired catchment (Viney et al. 2015). It simulates the flow of water through the landscape from rainfall entering the grid cell through the vegetation and soil, and then out of the grid cell through evapotranspiration, runoff or deep drainage to the groundwater. Its inputs include gridded climate, soil, vegetation and topographic data. For more information see the Bureau of Meteorology's Australian Landscape Water Balance webpage." .

:LyneAndHollickFilter skos:definition "The streamflow gauge for the North Para River at Yaldara (A5050502) was deemed the only streamflow site with a significant baseflow component outside the Western Mount Lofty Ranges PWRA. Baseflow was calculated for this site using a Lyne and Hollick filter (Grayson et al. 1996) with a filtering factor of 0.925 and daily flow records for 1 July 197530 June 2019." .

:ManagedWetlandsAppliedWaterEstimation skos:definition "Managed Wetlands AW = (Habitat Acreage x (Unit ETAW + CP)) by habitat type and management period" .

:UnitETOfAppliedWater skos:definition """Unit ETAW = ET of applied water per acre by habitat type and management. These values are generated
from crop/habitat spreadsheets, models, or soil moisture balance.""" .

:MelbourneWaterAnnualReport skos:definition "Water Utility" .

:SouthEastWaterAnnualReport skos:definition "Water Utility" .

:YarraValleyWaterAnnualReport skos:definition "Water Utility" .

:ModelledRunoff skos:definition "Runoff to surface water was estimated using the modelled runoff from the AWRA-R model. Runoff within AWRA-R is in turn derived from landscape runoff modelled in the AWRA-L model, with a scaling factor applied within AWRA-R during the calibration process." .

:MoretonAndLoganBasinResourceOperatingLicenses skos:definition "The Moreton and Logan Basin resource operating licences provide storage loss tables for Lake Wivenhoe, Lake Somerset and Lake Maroon, Cedar Grove Weir and Bromelton OffStream Storage, Lake Atkinson and Lake Moogerah." .

:NetworkRealLossesAndApparentLossesModelingSoftware skos:definition "modelling software of network real losses (leakages and busts) and apparent losses (unauthorised/authorised unbilled use); and/or" .

:OtherSupplySystemDecreases-AUS skos:definition "The 'Other supply system decreases' volume is the remaining non-revenue water from the urban water supply system (if not reported in leakage to landscape and groundwater respectively)." .

:RealLossesEquation skos:definition """The real losses is based on both avoidable and unavoidable losses (including pipe network background leaks, pipe leaks and bursts, tank and service reservoir leakage, and overflows) and is calculated using the following equation:

Real losses = Non-revenue water  (Apparent losses + Unmetered authorised consumption).""" .

:OtherWastewaterDecreases-AUS skos:definition """The 'Other wastewater decreases' volume represents the sum of the following components:
losses from wastewater treatment system not reported as evaporation
known losses from the wastewater collection system
known egress or exfiltration from the wastewater collection system occurring before metered inflow to wastewater treatment plants.""" .

:CentralValleySpatialDatabase-partOfTheCentralValleyHydrologicModel%5BCVHM%5DProject
  skos:definition """CVHM is a MODFLOW-FMP (Farm Process) application
developed by the USGS to simulate the historical hydrology of
Californias Central Valley. CVHM simultaneously accounts for
changing water supply and demand across the landscape, and
simulates surface water and groundwater flow across the entire
Central Valley. Hydraulic properties were assigned to the CVHM
grid based on a lithologic texture analysis of available drillers
logs (Faunt, Belitz, and Hanson 2009). It is built upon knowledge
from USGS and other federal, State, and local studies.""" .

:SpatialAveragingTechniques skos:definition """Precipitation into the water budget zone can be estimated using gauged data within or at the periphery of the water
budget zone and geographic information about the area. Gauges typically measure precipitation as depth. After
obtaining precipitation timeseries data for the gauges of interest, various established methods can be used to
estimate total precipitation volume. The methods include arithmetic mean method (precipitation gauges are weighted
equally) and Thiessen Polygon (precipitation gauges are weighted by area). Additional information regarding using
spatial averaging techniques to estimate precipitation can be found from the National Weather Service.""" .

:PropertyAreaEstimationMethodsForSurfaceWaterDiversions skos:definition """Surface water diversion for stock and domestic use is estimated based on property area around each of the major rivers within the Daly region and stock and domestic use factors.

The property area was assumed to equal the length of each river by an 8-km wide buffer. Total stock use was assumed to equal 0.2 ML/year/km2 for each river; this figure is based on best practice, stocking rates, and daily stock water needs, as recommended by the Department of Primary Industries and Fisheries. Total domestic use was assumed to equal 5.5 ML/year/km2 for each river, which is based on average metered water use by domestic water users in the region as part of a voluntary boremetering project conducted in 2008. Total volume of surface water diverted is calculated by multiplying the estimated property area by the stock and domestic use factors.""" .

:Rainfall-RunoffMethod skos:definition """Recharge of precipitation can be estimated by solving the mass balance equation for rainfall-runoff and consumptive use of precipitation:
Precipitation = Runoff (R) + Consumptive Use of Precipitation (EP) + Recharge of Precipitation (Dp)""" .

:RechargeAsPercentageOfRainfall skos:definition "Several models estimate recharge as a percentage of rainfall. The magnitude of recharge (as a percentage of rainfall) can be adjusted during the calibration of a groundwater model so that the observed groundwater levels are reproduced in model outputs as accurately as possible, typically for a period of around 20 years if data are available." .

:RechargeCreditBalance skos:definition "Managed aquifer recharge: individual users' volume was estimated by balancing recharge credit details for active licences as available with DEW." .

:WaterRecyclingSurvey%282015%29 skos:definition """The 2015 data set contains data from a SWRCB survey of
wastewater agencies and the 2015 Urban Water Management
Plans. The merging and validation of the data were conducted
jointly by both agencies and included follow-up email and direct
phone calls. Only treated municipal wastewater, originating in
whole or in part from a domestic source and directly used for
beneficial reuse was included. The data set includes direct
agricultural application and has been checked to remove
duplication from overlapping reporting by producers, wholesale
distributors, and users. In-plant process water use within a
wastewater treatment plant was considered part of treatment
plant operations and was not included as recycled water.
Discharges required by the treatment plant permit to maintain
habitat or instream flows or to complete treatment were
considered a permit requirement and not recycled water.
Groundwater recharge was only included in the data set if the
project is permitted by a regional water quality control board.
This data set is considered the most accurate and inclusive for
recycled water use in California.""" .

:ReturnFlowEstimationMethod skos:definition """Estimating return flow is an iterative process using either a simplified water balance of applied water (inflow versus outflow) or apportioning irrigation efficiencies. The simplified water balance of applied water is:
Applied Water (AW) = SW + GW + Applied Water Reuse = ETAW + Return Flow + Recharge
Return Flow = SW + GW + Applied Water Reuse  ETAW  Recharge""" .

:RiverAndGroundwaterInteractionModule skos:definition """The AWRA-R river and groundwater interaction module was used to model river losses. The module simulates seepage based on the potential infiltration rate from the river, the available storage in the underlying aquifer and the aquifer's discharge rate. The equations used in the module are based on Doble et al. (2014).

The AWRA-R output has been assumed to represent river losses to landscape, rather than groundwater, for the following reasons:
In the Perth Region, most river losses occur east of the Darling Escarpment outside of the coastal plain, where the aquifers are generally of low productivity or have non-potable water quality. In these areas, groundwater has not been recognised as an asset in the Perth Account.
On the coastal plain, where groundwater is recognised in the Perth Account, groundwater fluxes are estimated using the PRAMS and PHRAMS models. These models assume the river-aquifer flux is in the direction of groundwater discharge to rivers only and that all groundwater recharge is received via Recharge: landscape.""" .

:CaliforniaDepartmentOfTransportation%27sHighwayDesignManual skos:definition """This manual was prepared for the California Department of
Transportation (Department) by the Division of Design for use
on the California State highway system.
Tables 819.2A and 819.2B provide runoff coefficients for
different land use types.""" .

:RunoffCurveNumberMethod skos:definition """For drainage basins where no runoff has been measured, the Runoff Curve Number method can be used to estimate the depth of direct runoff from the rainfall depth. Direct runoff of precipitation from small watersheds can be estimated with the Natural Resources Conservation Service (NRCS) Runoff Curve Number method (NRCS was previously known as the Soil Conservation Service):
 = ((  0.2)^2)/ + 0.8
(   0.2)
where Qr is direct unit runoff in inches, P is precipitation (depth in inches), S is the potential maximum retention (inches). This equation allows the runoff depth to be estimated from rainfall depth, given the value of the potential
maximum retention, S. The potential maximum retention, S, is determined using the following equation:
 =(1000/CN)-10
To obtain total runoff volume (R), the direct runoff (Qr) calculated above may be multiplied by the watershed area: R = Qr * Watershed Area where CN is the curve number.""" .

:Precipitation-RunoffModelingSystem%28PRMS%29 skos:definition "This more detailed approach uses the USGSs Precipitation-Runoff Modeling System (PRMS) to simulate basin hydrology. Model documentation state that: PRMS is a modular-design, deterministic, distributed-parameter modeling system developed to evaluate the impacts of various combinations of precipitation, climate, and land use on streamflow, sediment yields, and general basin hydrology. Basin response to normal and extreme rainfall and snowmelt can be simulated to evaluate changes in water-balance relationships, flow regimes, flood peaks and volumes, soil-water relationships, sediment yields, and ground-water recharge. Parameter-optimization and sensitivity analysis capabilities are provided to fit selected model parameters and evaluate their individual and joint effects on model output. The modular design provides a flexible framework for continued model-system enhancement and hydrologic-modeling research and development." .

:SAWaterStorageVolumeRelationship skos:definition "Surface water storage volume was measured using gauged water level height(s) in metres with respect to the Australian height datum for individual storages. The height measurement was converted to a volume using the storagevolume relationship(s) provided by SA Water." .

:SpatialAssessments skos:definition """Non-allocated groundwater extraction for individual users is an estimate based on water allocation plans or spatial assessments. The assessments take into account variables such as number of properties, stock water requirements, and the distance stock must travel for water.

More information on water allocation plans in the region (Tindall Limestone and Oolloo Dolostone aquifers) can be found at the Department of Environment and Natural Resources website.""" .

:USGSDR3M skos:definition "rainfall-runoff model" .

:WaterResourceAssociatesHYSIM skos:definition "rainfall-runoff model" .

<http://purl.org/iow/WaterBudgetingFramework/UniversityOfWashington%E2%80%99sVariableInfiltrationCapacityModel%28VIC%29.>
  skos:definition "rainfall-runoff model" .

:Vieux%26Associates%27Vflo skos:definition "rainfall-runoff model" .

:SurplusIrrigationAssumption skos:definition "The volume of return flow from the Ord River Irrigation Area to the Ord River is an estimated volume based on the assumption that approximately 2 m3/s of surplus irrigation supply water and return flows contribute to the lower Ord River during the dry season (Department of Water 2012)." .

:VerticalFluxModel skos:definition "The Vertical Flux Model calculates recharge on a daily basis" .

:WaterAllocationPlans skos:definition """Non-allocated groundwater extraction for individual users is an estimate based on water allocation plans or spatial assessments. The assessments take into account variables such as number of properties, stock water requirements, and the distance stock must travel for water.

More information on water allocation plans in the region (Tindall Limestone and Oolloo Dolostone aquifers) can be found at the Department of Environment and Natural Resources website.""" .

:WaterSharingPlanForTheGreaterMetropolitanRegionUnregulatedRiverWaterSources skos:definition
    "The estimated annual water abstraction under riparian right for stock and domestic purposes and for cultural purposes was extracted from the Water Sharing Plan for the Greater Metropolitan Region Unregulated River Water Sources and the Water Sharing Plan for the Kangaroo River Water Source." .

:SupervisoryControlAndDataAcquisitions%28SCADA%29 skos:definition "Harvey Water maintains an Supervisory Control and Data Acquisition (SCADA) system that collects flow monitoring data within the irrigation scheme. Information from this system is provided to the Bureau of Meteorology under the Water Regulations 2008." .

:FiniteElementSubsurfaceFlowSystem%28FEFLOW%29 skos:definition """The Department of Environment and Natural Resources uses the Finite Element Subsurface Flow system (FEFLOW) to estimate the natural water movement to and from the groundwater store within the Daly region.

FEFLOW estimates groundwater movement for the entire extent of the Oolloo Dolostone Aquifer and the Tindall Limestone Aquifer, which extends beyond the Daly region boundary as shown in Figure N1. The volumes reported in this account refer to the natural water movement that occurs within these aquifers within the Daly region boundary.""" .

:Non-allocatedDiversion%3AUrbanWaterSystemEstimationMethod skos:definition "As metered data is not available at the inlet to each water treatment plant to distinguish between each water source, this volume is the total inflow to water treatment plants, less SA Water's total licensed diversion volume from the Western Mount Lofty Ranges PWRA as recorded in the WILMA licensing database" .

:RecycledWaterDelivery%3AIrrigation-AUS skos:definition "The 'Recycled water delivery: irrigation' volume is the metered volume of recycled water supplied for use in irrigation schemes." .

:SupplySystemDelivery%3AIrrigation-AUS skos:definition "The 'Supply system delivery: irrigation' volume is the metered volume of water supplied for use in irrigation schemes." .

:SupplySystemDischarge%3ASurfaceWater-AUS skos:definition "The supply system discharge; surface water volume is metered and includes return of excess water from the urban water supply system back to surface water / reservoirs." .

:WastewaterAndRecycledWaterDischarge%3ASurfaceWater-AUS skos:definition "The 'Wastewater and recycled water discharge: surface water' volume is metered and includes: disposal of treated wastewater to rivers and other surface water, discharge of recycled water for environmental purposes. Treated wastewater disposal to rivers and streams which are estuarine in nature, or subject to tidal impacts, are not reported in this volume, but reported as discharge outside the region (to sea)." .

:WastewaterDischarge%3ASurfaceWater-AUS skos:definition """The volume of wastewater and recycled water discharged to surface water is metered and includes:
disposal of treated wastewater to rivers and other surface water
discharge of recycled water for environmental purpose.
Treated wastewater disposal to rivers and streams that are estuarine in nature, or subject to tidal impacts, are not reported in this volume but instead reported as discharge to sea.""" .

skos:ConceptScheme skos:example "Thesauri, classification schemes, subject heading lists, taxonomies, 'folksonomies', and other types of controlled vocabulary are all examples of concept schemes. Concept schemes are also embedded in glossaries and terminologies."@en;
  skos:scopeNote "A concept scheme may be defined to include concepts from different sources."@en .

skos:Collection skos:scopeNote "Labelled collections can be used where you would like a set of concepts to be displayed under a 'node label' in the hierarchy."@en .

skos:OrderedCollection skos:scopeNote "Ordered collections can be used where you would like a set of concepts to be displayed in a specific order, and optionally under a 'node label'."@en .

skos:inScheme skos:scopeNote "A concept may be a member of more than one concept scheme."@en .

skos:notation skos:scopeNote "By convention, skos:notation is used with a typed literal in the object position of the triple."@en .

skos:note skos:scopeNote "This property may be used directly, or as a super-property for more specific note types."@en .

skos:semanticRelation skos:scopeNote "This property should not be used directly, but as a super-property for all properties denoting a relationship of meaning between concepts."@en .

skos:broader skos:scopeNote "By convention, skos:broader is only used to assert an immediate (i.e. direct) hierarchical link between two conceptual resources."@en .

skos:broaderTransitive skos:scopeNote "By convention, skos:broaderTransitive is not used to make assertions. Rather, the properties can be used to draw inferences about the transitive closure of the hierarchical relation, which is useful e.g. when implementing a simple query expansion algorithm in a search application."@en .

skos:narrower skos:scopeNote "By convention, skos:broader is only used to assert an immediate (i.e. direct) hierarchical link between two conceptual resources."@en .

skos:narrowerTransitive skos:scopeNote "By convention, skos:narrowerTransitive is not used to make assertions. Rather, the properties can be used to draw inferences about the transitive closure of the hierarchical relation, which is useful e.g. when implementing a simple query expansion algorithm in a search application."@en .

skos:altLabel skos:example "Acronyms, abbreviations, spelling variants, and irregular plural/singular forms may be included among the alternative labels for a concept. Mis-spelled terms are normally included as hidden labels (see skos:hiddenLabel)."@en .

:AgriculturalAndMunicipalDepletions-UT skos:prefLabel "Agricultural and Municipal Depletions" .

:CropConsumptiveUse-CO skos:prefLabel "Crop Consumptive use" .

:GroundwaterExtraction-CA skos:prefLabel "Groundwater Extraction" .

:LivestockConsumptiveUse-CO skos:prefLabel "Livestock Consumptive Use" .

:MunicipalAndIndustrialConsumptiveUse-CO skos:prefLabel "Municipal and Industrial Consumptive Use" .

:SurfaceWaterDiversions-CA skos:prefLabel "Surface Water Diversions" .

:AgriculturalAndMunicipalDiversions-UT skos:prefLabel "Agricultural and Municipal Diversions" .

:AppliedWater-CA skos:prefLabel "Applied Water" .

:Evapotranspiration-CA skos:prefLabel "Evapotranspiration" .

:AgriculturalDepletions-UT skos:prefLabel "Agricultural Depletions" .

:SurfaceDiversionToCropland-UT skos:prefLabel "Surface Diversion to Cropland" .

:AgriculturalPotentialConsumptiveUse-UT skos:prefLabel "Agricultural Potential Consumptive Use" .

:TotalLandSystemInflow-CA skos:prefLabel "Total Land System Inflow" .

:AreaOutflows skos:prefLabel "Area Outflows" .

:BasinOutflow-UT skos:prefLabel "Basin Outflow" .

:StreamOutfow-CA skos:prefLabel "Stream Outflow" .

:Exports-CO skos:prefLabel "Exports" .

:TotalSurfaceWaterOutflow-CA skos:prefLabel "Total Surface Water Outflow" .

:BasinInflow-UT skos:prefLabel "Basin Inflow" .

:RiverInflow-UT skos:prefLabel "River Inflow" .

:GagedSurfaceWaterInflow-CO skos:prefLabel "Gaged Surface Water Inflow" .

:UngagedSurfaceWaterInflow-CO skos:prefLabel "Ungaged Surface Water Inflow" .

:TotalSurfaceWaterInflow-CA skos:prefLabel "Total Surface Water Inflow" .

:StreamInflow-CA skos:prefLabel "Stream Inflow" .

:ChangeInGroundWaterStorage-CO skos:prefLabel "Change in Ground Water Storage" .

:ChangeInGroundwaterStorage-CA skos:prefLabel "Change in Groundwater Storage" .

:ChangeInTotalSystemStorage-CA skos:prefLabel "Change in Total System Storage" .

:ChangeInLandSystemStorage-CA skos:prefLabel "Change in Land System Storage" .

:ChangeInSurfaceWaterStorage-CA skos:prefLabel "Change in Surface Water Storage" .

:ChangeInSurfaceWaterStorage-CO skos:prefLabel "Change in Surface Water Storage" .

:Commercial-NMOSE skos:prefLabel "Commercial" .

:MunicipalAndIndustrialDiversions-UT skos:prefLabel "Municipal and Industrial Diversions" .

:ConveyanceEvaporation-CA skos:prefLabel "Conveyance Evaporation" .

:HumanConsumption-NM skos:prefLabel "Human Consumption" .

:ConveyanceLossesForAllocatedDiversions-AUS skos:prefLabel "Conveyance Losses for Allocated Diversions" .

:SurfaceWaterOutflows-AUS skos:prefLabel "Surface Water Outflows" .

:ConveyanceSeepage-CA skos:prefLabel "Conveyance Seepage" .

:TotalGroundwaterSystemInflow-CA skos:prefLabel "Total Groundwater System Inflow" .

:CoplandPrecipitation-UT skos:prefLabel "Cropland Precipitation" .

:Precipitation-CA skos:prefLabel "Precipitation on Land" .

:Precipitation-CO skos:prefLabel "Precipitation" .

:Precipitation-NM skos:prefLabel "Precipitation" .

:Precipitation-UT skos:prefLabel "Precipitation" .

:IrrigatedAgricultureDepletions-NMOSE skos:prefLabel "Irrigated Agriculture Depletions" .

:Evaporation-AUS skos:prefLabel "Evaporation" .

:Evaporation-NM skos:prefLabel "Evaporation" .

:TotalEvaporation-NM skos:prefLabel "Total Evaporation" .

:EvaporationFromReservoirs-NMOSE skos:prefLabel "Evaporation from Reservoirs" .

:LakeEvaporation-CA skos:prefLabel "Lake Evaporation" .

:ReservoirEvaporation-CO skos:prefLabel "Reservoir Evaporation" .

:ReservoirEvaporation-UT skos:prefLabel "Reservoir Evaporation" .

:TotalLandSystemOutflow-CA skos:prefLabel "Total Land System Outflow" .

:GroundwaterExport-CA skos:prefLabel "Groundwater Export" .

:StoredWaterExport-CA skos:prefLabel "Stored Water Export" .

:SurfaceWaterExports-CA skos:prefLabel "Surface Water Exports" .

:FloodReturn-AUS skos:prefLabel "Flood Return" .

:SurfaceWaterInflows-AUS skos:prefLabel "Surface Water Inflows" .

:TotalInflow-CA skos:prefLabel "Total Inflow" .

:TotalOutflow-CA skos:prefLabel "Total Outflow" .

:GagedSurfaceWaterOutflow-CO skos:prefLabel "Gaged Surface Water Outflow" .

:GroundWaterInflow-CO skos:prefLabel "Ground Water Inflow" .

:SubsurfaceInflow-CA skos:prefLabel "Subsurface Inflow" .

:GroundWaterOutflow-CO skos:prefLabel "Ground Water Outflow" .

:TotalGroundwaterSystemOutflow-CA skos:prefLabel "Total Groundwater System Outflow" .

:SubsurfaceOutflow-CA skos:prefLabel "Subsurface Outflow" .

:Discharge%3AGroundwater-AUS skos:prefLabel "Discharge Groundwater" .

:GroundwaterDiversions-NM skos:prefLabel "Groundwater Diversions" .

:GroundwaterET-NM skos:prefLabel "Groundwater ET" .

:RiparianConsumption-NM skos:prefLabel "Riparian Consumption" .

:LakeGainFromGroundwater-CA skos:prefLabel "Lake Gain from Groundwater" .

:GroundwaterInflows-AUS skos:prefLabel "Groundwater Inflows" .

:GroundwaterOutflows-AUS skos:prefLabel "Groundwater Outflows" .

:GroundwaterOutflows-NM skos:prefLabel "Groundwater Outflows" .

:GroundwaterReturn-NM skos:prefLabel "Groundwater Return" .

:GroundwaterStock-NM skos:prefLabel "Groundwater Stock" .

:GroundwaterUse-UT skos:prefLabel "Groundwater Use" .

:PumpedGroundwater-UT skos:prefLabel "Pumped Groundwater" .

:HumanReturns-NM skos:prefLabel "Human Returns" .

:HumanStorageAndDistributionSystemStock-NM skos:prefLabel "Human Storage and Distribution System Stock" .

:ImportedWater-CA skos:prefLabel "Imported Water" .

:Imports-CO skos:prefLabel "Imports" .

:Industrial-NMOSE skos:prefLabel "Industrial" .

:SurfaceWaterDelivery-CA skos:prefLabel "Surface Water Delivery" .

:IrrigatedAgriculture-NMOSE skos:prefLabel "Irrigated Agriculture" .

:IrrigatedAgricultureDiversions-NMOSE skos:prefLabel "Irrigated Agriculture Diversions" .

:IrrigationSchemeOutflows-AUS skos:prefLabel "Irrigation Scheme Outflows" .

:LakeLossToGroundwater-CA skos:prefLabel "Lake Loss to Groundwater" .

:Recharge-NM skos:prefLabel "Recharge" .

:LandSurfaceExapotranspiration-NM skos:prefLabel "Land Surface Evapotranspiration" .

:LandSurfaceStock-NM skos:prefLabel "Land Surface Stock" .

:ManagedAquiferRecharge-AUS skos:prefLabel "Managed Aquifer Recharge" .

:UrbanWaterSystemOutflows-AUS skos:prefLabel "Urban Water System Outflows" .

:ManagedAquiferRecharge-CA skos:prefLabel "Managed Aquifer Recharge" .

:Mining-NMOSE skos:prefLabel "Mining" .

:Power-NMOSE skos:prefLabel "Power" .

:PublicWaterSupply-NMOSE skos:prefLabel "Public Water Supply" .

:MunicipalAndIndustrialDepeltion-UT skos:prefLabel "Municipal and Industrial Depeltions" .

:MunicipalAndIndustrialReturnFlow-UT skos:prefLabel "Municipal and Industrial Return Flow" .

:ReturnFlow-CA skos:prefLabel "Return Flow" .

:NativeVegetationConsumptiveUse-CO skos:prefLabel "Native Vegetation Consumptive Use" .

:NaturalSystemUse-UT skos:prefLabel "Natural System Use" .

:RiparianDepletions-UT skos:prefLabel "Riparian Depletions" .

:Non-allocatedExtraction-AUS skos:prefLabel "Non-allocated Extraction" .

:Outflow-AUS skos:prefLabel "Outflow" .

:OverbankFlow-AUS skos:prefLabel "Overbank Flow" .

:Precipitation-AUS skos:prefLabel "Precipitation" .

:PrecipitationOnLakes-CA skos:prefLabel "Precipitation on Lakes" .

:RechargeOfAppliedWater-CA skos:prefLabel "Recharge of Applied Water" .

:RechargeOfPrecipitation-CA skos:prefLabel "Recharge of Precipitation" .

:RecycledWaterExport-CA skos:prefLabel "Recycled Water Export" .

:RiverEvaporation-NM skos:prefLabel "River Evaporation" .

:RiverUseByWetPasture-UT skos:prefLabel "River Use By Wet Pasture" .

:Runoff-AUS skos:prefLabel "Runoff" .

:Runoff-CA skos:prefLabel "Runoff" .

:Runoff-NM skos:prefLabel "Runoff" .

:StoredWaterExtraction-CA skos:prefLabel "Stored Water Extraction" .

:StreamEvaporation-CA skos:prefLabel "Stream Evaporation" .

:StreamGainFromGroundwater-CA skos:prefLabel "Stream Gain from Groundwater" .

:StreamLossToGroundwater-CA skos:prefLabel "Stream Loss to Groundwater" .

:SurfaceWaterDiversions-NM skos:prefLabel "Surface Water Diversions" .

:SurfaceWaterEvaporation-NM skos:prefLabel "Surface Water Evaporation" .

:SurfaceWaterFlows-UT skos:prefLabel "Surface Water Flows" .

:SurfaceWaterGroundwaterInteractions-NM skos:prefLabel "Surface Water Groundwater Interactions" .

:SurfaceWaterInflows-NM skos:prefLabel "Surface Water Inflows" .

:SurfaceWaterOutflows-NM skos:prefLabel "Surface Water Outflows" .

:SurfaceWaterReturns-NM skos:prefLabel "Surface Water Returns" .

:SurfaceWaterStock-NM skos:prefLabel "Surface Water Stock" .

:TotalLandReturnFlow-UT skos:prefLabel "Total Land Return Flow" .

:TributaryInflow-UT skos:prefLabel "Tributary Inflow" .

:UrbanWaterSystemInflows-AUS skos:prefLabel "Urban Water System Inflows" .

:WastewaterCollected-AUS skos:prefLabel "Wastewater Collected" .

:WaterReleaseCausedByLandSubsidence-CA skos:prefLabel "Water Release Caused by Land Subsidence" .

:WaterUse-NM skos:prefLabel "Water Use" .

:AllocatedDiversion%3AEnvironmentalPurposes-AUS skos:prefLabel "Allocated Diversion: Environmental Purposes" .

:AllocatedDiversion%3AIndividualUsers-AUS skos:prefLabel "Allocated Diversion: Individual Users" .

:AllocatedDiversion%3AInter-region-AUS skos:prefLabel "Allocated Diversion: Inter-region" .

:AllocatedDiversion%3AIrrigationScheme-AUS skos:prefLabel "Allocated Diversion: Irrigation Scheme" .

:AllocatedDiversion%3AUrbanSystem-AUS skos:prefLabel "Allocated Diversion: Urban System" .

:AllocatedDiversions%3ASurfaceWater-AUS skos:prefLabel "Allocated Diversions: Surface Water" .

:AllocatedExtraction%3AEnvironmentalPurposes-AUS skos:prefLabel "Allocated Extraction: Environmental Purposes" .

:AllocatedExtraction%3AGroundwater-AUS skos:prefLabel "Allocated Extraction: Groundwater" .

:AllocatedExtraction%3AIndividualUsers-AUS skos:prefLabel "Allocated Extraction: Individual Users" .

:AllocatedExtraction%3AUrbanSystem-AUS skos:prefLabel "Allocated Extraction: Urban System" .

:AppliedWaterReuse%2FRecycledWater-CA skos:prefLabel "Applied Water Reuse/Recycled Water" .

:Delivery%3ADesalinatedWater-AUS skos:prefLabel "Delivery: Desalinated Water" .

:Delivery%3AInter-regionAgreement-AUS skos:prefLabel "Delivery: Inter-region Agreement" .

:Delivery%3AIrrigationScheme-AUS skos:prefLabel "Delivery: Irrigation Scheme" .

:Discharge%3ALandscape-AUS skos:prefLabel "Discharge: Landscape" .

:Discharge%3ASea-AUS skos:prefLabel "Discharge: Sea" .

:Discharge%3ASurfaceWater-AUS skos:prefLabel "Discharge: Surface Water" .

:Discharge%3AUrbanSupply-AUS skos:prefLabel "Discharge: Urban Supply" .

:Discharge%3AUrbanSupplySystem-AUS skos:prefLabel "Discharge: Urban Supply System" .

:Discharge%3AWastewater-AUS skos:prefLabel "Discharge: Wastewater" .

:Diversions%3AStatutoryRights-AUS skos:prefLabel "Diversions: Statutory Rights" .

:Extraction%3AStatutoryRights-AUS skos:prefLabel "Extraction: Statutory Rights" .

:Inter-regionInflow%3AGroundwater-AUS skos:prefLabel "Inter-region Inflow: Groundwater" .

:Inter-regionInflow%3ASurfaceWater-AUS skos:prefLabel "Inter-region Inflow: Surface Water" .

:Inter-regionOutflow%3AGroundwater-AUS skos:prefLabel "Inter-region Outflow" .

:Leakage%3ALandscape-AUS skos:prefLabel "Leakage: Landscape" .

:Leakage%3AUrbanSystem-AUS skos:prefLabel "Leakage: Urban System" .

:ManagedAquiferRecharge%3AIndividualUser-AUS skos:prefLabel "Managed Aquifer Recharge: Individual User" .

:Non-allocatedDiversion%3AEnvironmentalPurposes-AUS skos:prefLabel "Non-allocated Diversion: Environmental Purposes" .

:Non-allocatedDiversion%3AIndividualUsers-AUS skos:prefLabel "Non-allocated Diversion: Individual Users" .

:Non-allocatedDiversion%3AUrbanSystem-AUS skos:prefLabel "Non-allocated Diversion: Urban System" .

:PointReturn%3AIrrigation-AUS skos:prefLabel "Point Return: Irrigation" .

:PublicWaterSupply%3AUnmetered-NMOSE skos:prefLabel "Public Water Supply: Unmetered" .

:Recharge%3AGroundwater-AUS skos:prefLabel "Recharge: Groundwater" .

:Recharge%3ALandscape-AUS skos:prefLabel "Recharge: Landscape" .

:Recharge%3ASurfaceWater-AUS skos:prefLabel "Recharge: Surface Water" .

:RecycledWaterDelivery%3AUrbanUsers-AUS skos:prefLabel "Recycled Water Delivery: Urban Users" .

:ReturnFlow%3AEnvironmentalPurposes-AUS skos:prefLabel "Return Flow: Environmental Purposes" .

:RiparianRelease%3AUrbanSupply-AUS skos:prefLabel "Riparian Release: Urban Supply" .

:SupplySystemDelivery%3AInter-Region-AUS skos:prefLabel "Supply System Delivery: Inter-Region-AUS" .

:SupplySystemDelivery%3AUrbanUsers-AUS skos:prefLabel "Supply System Delivery: Urban Users" .

:SupplySystemDischarge%3AReservoirs-AUS skos:prefLabel "Supply System Discharge: Reservoirs" .

:SupplySystemTransfer%3AInter-region-AUS skos:prefLabel "Supply System Transfer: Inter-region" .

:AgriculturalAndMunicipalDepletions-UT skos:note <https://www.westernstateswater.org/wp-content/uploads/2017/01/1-Water-Budget-Process.docx> .

:AgriculturalAndMunicipalDiversions-UT skos:note <https://www.westernstateswater.org/wp-content/uploads/2017/01/2-Water-Budget-Process.pptx> .

:UTDivisionOfWaterResourcesArea-AltitudeMethod skos:note "For flows estimated from either StreamStats or the Area-Altitude Method, monthly flows are calculated as a proportion of the flow of a base station." .

:AgriculturalDepletions-UT skos:note <https://www.westernstateswater.org/wp-content/uploads/2017/01/2-Water-Budget-Process.pptx> .

:SurfaceDiversionToCropland-UT skos:note <https://www.westernstateswater.org/wp-content/uploads/2017/01/3-Summary-Page-Documentation-cwm.docx> .

:AgriculturalPotentialConsumptiveUse-UT skos:note <https://www.westernstateswater.org/wp-content/uploads/2017/01/2-Water-Budget-Process.pptx> .

:PRISM skos:note "PRISM Climate Group, Oregon State University" .

:USUResearchReport145 skos:note "Blainey-Criddle crop coefficients from USU Research Report 145" .

:DailyPenman-Monteith skos:note "Project underway to use a modified analysis for the Upper Basin - USBR",
    "Used in CO where data are available, including areas of the Colorado River Basin",
    "Used in NM where data are available, not used in San Juan River Basin", "Used in UT where data available, not used in Colorado River Basin",
    "Used in WY where data is available, including areas of the Green River Basin since 2011",
    <http://opencdss.state.co.us/statecu/latest/doc-user/ModelDescription/31/#313-daily-penman-monteith-crop-et> .

:ModifiedBlaney-Criddle skos:note "Et (monthly) = kt  kc (T  p / 100)", "Most common statewide in CO, NM, WY, UT",
    """StateCU allows either the SCS TR-21 modified Blaney-Criddle or the original Blaney-Criddle procedure to estimate monthly evapotranspiration (ET). The empirical equation relates ET with mean air temperature and mean percentage daytime hours. The SCS TR-21 method was modified from the original Blaney-Criddle method to reasonably estimate short-period consumptive use. The modifications include the use of (1) climatic coefficients that are directly related to the mean air temperature for each of the consecutive short periods which constitutes the growing season and (2) coefficients which reflect the influence of the crop growth rates on consumptive use rates (SCS TR-21).

The basic relationship assumes that ET varies directly with the products of mean monthly air temperature and monthly percentage of annual daylight hours for an actively growing crop with adequate soil moisture. This is expressed mathematically as:
u=kf""",
    <http://opencdss.state.co.us/statecu/latest/doc-user/ModelDescription/31/#313-daily-penman-monteith-crop-et> .

:SolarRadiation skos:note <http://opencdss.state.co.us/statecu/latest/doc-user/ModelDescription/31/#313-daily-penman-monteith-crop-et> .

:VaporPressure skos:note <http://opencdss.state.co.us/statecu/latest/doc-user/ModelDescription/31/#313-daily-penman-monteith-crop-et> .

:WindRun skos:note <http://opencdss.state.co.us/statecu/latest/doc-user/ModelDescription/31/#313-daily-penman-monteith-crop-et> .

:ClimateCoefficient%28kt%29 skos:note <http://opencdss.state.co.us/statecu/latest/doc-user/ModelDescription/31/#3113-scs-tr-21-modified-or-original-blaney-criddle-method-with-et-elevation-adjustment> .

:CropGrowthStateCoefficient%28Kc%29 skos:note "The modified Blaney-Criddle crop coefficients are available from graphs in the SCS TR-21 publication for 25 crops, which were developed based on general climatic conditions representative of the Western U.S.",
    <http://opencdss.state.co.us/statecu/latest/doc-user/ModelDescription/31/#3111-scs-tr-21-modified-or-original-blaney-criddle-method> .

:MeanMonthlyAirTemperatures%28T%29 skos:note "Fahrenheit", <http://opencdss.state.co.us/statecu/latest/doc-user/ModelDescription/31/#3113-scs-tr-21-modified-or-original-blaney-criddle-method-with-et-elevation-adjustment> .

:MonthlyPercentageOfAnnualDaylightHours%28P%29 skos:note "based on latitude of the area under study",
    <http://opencdss.state.co.us/statecu/latest/doc-user/ModelDescription/31/#3113-scs-tr-21-modified-or-original-blaney-criddle-method-with-et-elevation-adjustment> .

:BasinOutflow-UT skos:note <https://www.westernstateswater.org/wp-content/uploads/2017/01/1-Water-Budget-Process.docx> .

:AverageUseRate skos:note "Source: CU and Losses Report 2001-2005 (Word Doc)" .

:MidwestPlanServiceStructuresAndEnvironmentalHandbook%2C1977 skos:note "Source: CU and Losses Report 2001-2005 (Word Doc)" .

:Baseflow skos:note """Baseflow estimation requires two steps in StateMod and one step in
TSTool: 1) StateMod adjusts USGS stream gage flows using historical records of operations to get baseflow time series at gaged points, for the gage period of record; 2) TSTool fills remaining
baseflow by regression; 3) StateMod distributes baseflow gains above and between gages to
user-specified, ungaged inflow nodes. These three steps are described below.""",
    "Natural Flow", <http://opencdss.state.co.us/statemod/latest/doc-user/input/04_input.pdf>,
    <https://dnrweblink.state.co.us/cwcb/0/doc/204368/Electronic.aspx?searchid=95b15b6f-2ace-4b3f-a0d5-134352e5d550> .

:BasinInflow-UT skos:note "Not sure if River inflow and Basin Inflow are exactly the same",
    <https://www.westernstateswater.org/wp-content/uploads/2017/01/1-Water-Budget-Process.docx> .

:RiverInflow-UT skos:note "Not sure if River inflow and Basin Inflow are exactly the same",
    <https://www.westernstateswater.org/utah-division-of-water-resources-water-budget-program-methods-description/>,
    <https://www.westernstateswater.org/wp-content/uploads/2017/01/2-Water-Budget-Process.pptx>,
    <https://www.westernstateswater.org/wp-content/uploads/2017/01/3-Summary-Page-Documentation-cwm.docx> .

:COAgriculturalMeteorologyNetworkStation skos:note "Managed by Colorado Climate Center at Colorado State University. Available through HydroBase or from CoAgMet website." .

:HydroBase skos:note "StateDMI is often used to extract data from HydroBase and put it into CU models" .

:CommunityCollaborativeRain%2CHailAndSnowNetwork%28CoCoRaHS%29 skos:note "Managed by Colorado Climate Center at Colorado State University" .

:COIrrigatedAcreageAssessment skos:note "updated every 5 years; available on the state website" .

:ModifiedBlaney-CriddleWithETElevationAdjustment skos:note <http://opencdss.state.co.us/statecu/latest/doc-user/ModelDescription/31/#3111-scs-tr-21-modified-or-original-blaney-criddle-method> .

:OriginalBlaney-Criddle skos:note """StateCU allows either the SCS TR-21 modified Blaney-Criddle or the original Blaney-Criddle procedure to estimate monthly evapotranspiration (ET). he SCS TR-21 method was modified from the original Blaney-Criddle method to reasonably estimate short-period consumptive use. The modifications include the use of (1) climatic coefficients that are directly related to the mean air temperature for each of the consecutive short periods which constitutes the growing season and (2) coefficients which reflect the influence of the crop growth rates on consumptive use rates (SCS TR-21).

The basic relationship assumes that ET varies directly with the products of mean monthly air temperature and monthly percentage of annual daylight hours for an actively growing crop with adequate soil moisture. This is expressed mathematically as:
u=kf""",
    <http://opencdss.state.co.us/statecu/latest/doc-user/ModelDescription/31/#3111-scs-tr-21-modified-or-original-blaney-criddle-method> .

:OriginalBlaney-CriddleWithETElevationAdjustment skos:note <http://opencdss.state.co.us/statecu/latest/doc-user/ModelDescription/31/#3111-scs-tr-21-modified-or-original-blaney-criddle-method> .

:EffectivePrecipitation skos:note "At this time, each of the states (with the exception of Utah) and Reclamation rely on the SCS monthly method outlined in Technical Release 21 in the Colorado River Basin. Utah estimates effective precipitation to be 80 percent of total precipitation during the irrigation season." .

:WaterSupply skos:note "Water supply data is based on diversion records and streamflow data" .

:COLivestockMethod skos:note "Source: CU and Losses Report 2001-2005 (Word Doc)" .

:StateAgriculturalStatistics skos:note "Source: CU and Losses Report 2001-2005 (Word Doc)" .

:LivestockCount skos:note "Source: CU and Losses Report 2001-2005 (Word Doc)" .

:COMunicipalAndIndustrialMethod skos:note "Source: CU and Losses Report 2001-2005 (Word Doc)" .

:ConsumptiveRatio skos:note "Source: CU and Losses Report 2001-2005 (Word Doc)" .

:GrossUsage skos:note "Source: CU and Losses Report 2001-2005 (Word Doc)" .

:Population skos:note "Source: CU and Losses Report 2001-2005 (Word Doc)" .

:CONativeVegetationMethod skos:note <http://s3-us-west-2.amazonaws.com/ucldc-nuxeo-ref-media/7ddb6359-e7b6-4713-93be-427286f81e4e> .

:ChangeInGroundwaterStorage-AUS skos:note "Adelaide", "Burdekin", "Canberra", "Daly",
    "Fitzroy", "Melbourne", "Murray Darling Basin", "Ord", "Perth", "South East Queensland",
    "Sydney" .

:ChangeInSurfaceWaterStorage-AUS skos:note "Adelaide", "Burdekin", "Canberra", "Daly",
    "Fitzroy", "Melbourne", "Murray Darling Basin", "Ord", "Perth", "South East Queensland",
    "Sydney" .

:ColoradoCensusBureau skos:note "Source: CU and Losses Report 2001-2005 (Word Doc)" .

:ColoradoStateMod skos:note <http://opencdss.state.co.us/tstool/13.02.00/doc-user/datastore-ref/CO-HydroBase/CO-HydroBase/#available-time-series-by-data-type-categories>,
    <https://www.colorado.gov/pacific/cdss/statedmi>, <https://www.colorado.gov/pacific/cdss/tstool> .

:InstreamFlowDemand-Annual skos:note <http://opencdss.state.co.us/statemod/latest/doc-user/input/04_input.pdf> .

:InstreamFlowDemand-Monthly skos:note <http://opencdss.state.co.us/statemod/latest/doc-user/input/04_input.pdf> .

:ReservoirTargets skos:note <http://opencdss.state.co.us/statemod/latest/doc-user/input/04_input.pdf> .

:MunicipalAndIndustrialDiversions-UT skos:note <https://www.westernstateswater.org/utah-division-of-water-resources-water-budget-program-methods-description/>,
    <https://www.westernstateswater.org/wp-content/uploads/2017/01/2-Water-Budget-Process.pptx> .

:ConveyanceLossesForAllocatedDiversions-AUS skos:note "Murray Darling Basin" .

:SurfaceWaterOutflows-AUS skos:note "Adelaide", "Burdekin", "Canberra", "Daly", "Fitzroy",
    "Melbourne", "Murray Darling Basin", "Ord", "Perth", "South East Queensland", "Sydney",
    <http://www.bom.gov.au/water/awid/search.shtml?q=Surface+Water+Outflows&p=> .

:CoplandPrecipitation-UT skos:note <https://www.westernstateswater.org/wp-content/uploads/2017/01/3-Summary-Page-Documentation-cwm.docx> .

:Precipitation-UT skos:note "PRISM Gridded Weather Data: The PRISM Climate Groups 30m grid-cell resolution PRISM data for temperature and precipitation are used to estimate precipitation inputs across the state and for the Colorado and Bear River Basins.",
    <https://www.westernstateswater.org/utah-division-of-water-resources-water-budget-program-methods-description/>,
    <https://www.westernstateswater.org/wp-content/uploads/2017/01/2-Water-Budget-Process.pptx> .

:MesoWestStations skos:note "From University of Utah" .

:SoilClimateAnalysisNetwork%28SCAN%29 skos:note "From Natural Resources Conservation Service" .

:DailyASCEStandardizedPenman-Monteith skos:note <http://opencdss.state.co.us/statecu/latest/doc-user/ModelDescription/31/#313-daily-penman-monteith-crop-et> .

:DailyEffectivePrecipitation skos:note "Daily effective precipitation (i.e. effective rainfall, Re) may be estimated in StateCU using three methods that can be selected by the user. Daily effective precipitation methods can only be used with daily consumptive use analyses.",
    <http://opencdss.state.co.us/statecu/latest/doc-user/ModelDescription/31/#316-daily-effective-precipitation> .

:DailyModifiedHargreaves skos:note <http://opencdss.state.co.us/statecu/latest/doc-user/ModelDescription/31/#315-daily-modified-hargreaves-crop-et> .

:EffectivePrecipitationFactor skos:note <https://coagmet.colostate.edu/ET_Workshop_2012/CDWR_StateCU.pdf> .

:Evaporation-AUS skos:note "Adelaide", "Burdekin", "Canberra", "Daly", "Fitzroy",
    "Melbourne", "Murray Darling Basin", "Ord", "Perth", "South East Queensland", "Sydney",
    <http://www.bom.gov.au/water/awid/search.shtml?q=Evaporation&p=> .

:ReservoirEvaporation-UT skos:note <https://www.westernstateswater.org/utah-division-of-water-resources-water-budget-program-methods-description/>,
    <https://www.westernstateswater.org/wp-content/uploads/2017/01/2-Water-Budget-Process.pptx> .

:FloodReturn-AUS skos:note "Adelaide", "Burdekin", "Canberra", "Daly", "Fitzroy",
    "Melbourne", "Murray Darling Basin", "Ord", "Perth", "Sydney", <http://www.bom.gov.au/water/awid/search.shtml?q=Flood+Return&p=> .

:SurfaceWaterInflows-AUS skos:note "Adelaide", "Burdekin", "Canberra", "Daly", "Fitzroy",
    "Melbourne", "Murray Darling Basin", "Ord", "Perth", "South East Queensland", "Sydney",
    <http://www.bom.gov.au/water/awid/search.shtml?q=Surface+Water+Inflows&p=> .

:GroundwaterDischarge-AUS skos:note "Perth", <http://www.bom.gov.au/water/awid/search.shtml?q=Groundwater+Discharge&p=> .

:Discharge%3AGroundwater-AUS skos:note "Adelaide", "Canberra", "Daly", "Melbourne",
    "Murray Darling Basin", <http://www.bom.gov.au/water/awid/search.shtml?q=Groundwater+Discharge&p=> .

:GroundwaterInflows-AUS skos:note "Adelaide", "Burdekin", "Canberra", "Daly", "Fitzroy",
    "Lateral flow of groundwater into the region's groundwater from inland groundwater aquifers that extend outside the region. It excludes lateral flow of groundwater from coastal aquifers",
    "Melbourne", "Murray Darling Basin", "Ord", "Perth", "South East Queensland", <http://www.bom.gov.au/water/awid/search.shtml?q=Groundwater+Inflow&p=> .

:GroundwaterOutflows-AUS skos:note "Adelaide", "Burdekin", "Canberra", "Daly", "Fitzroy",
    "Melbourne", "Murray Darling Basin", "Ord", "Perth", "South East Queensland", <http://www.bom.gov.au/water/awid/search.shtml?q=Groundwater&p=> .

:GroundwaterUse-UT skos:note <https://www.westernstateswater.org/utah-division-of-water-resources-water-budget-program-methods-description/>,
    <https://www.westernstateswater.org/wp-content/uploads/2017/01/2-Water-Budget-Process.pptx> .

:PumpedGroundwater-UT skos:note <https://www.westernstateswater.org/wp-content/uploads/2017/01/1-Water-Budget-Process.docx> .

:Imports-CO skos:note "Definition from CA" .

:Inter-regionCoastalInflow-AUS skos:note "Adelaide", "Melbourne", "Murray Darling Basin",
    "Perth" .

:Inter-regionCoastalOutflow-AUS skos:note "Adelaide", "Melbourne", "Murray Darling Basin",
    "Perth" .

:NMIrrigatedAcreageAssessment skos:note "updated annually; available by request" .

:UTIrrigatedAcreageAssessment skos:note "Each 5-year assessment includes field-verified estimates of acreage, crop type, and irrigation method. Water source (i.e. specific irrigating ditch) is not identified. Upon completion, data is filed in the State Geographic Information Database (SGID) and maintained by the State Automated Geographic Reference Center (AGRC). Once the data has been published on the AGRC website (http://gis.utah.gov/data/water-data-services/), the data becomes available to the public and is ready to be use in preparing water-related planning studies." .

:IrrigatedAgriculture-NMOSE skos:note "52% of Irrigated Agriculture is metered" .

:ConsumptiveIrrigationRequirement%28CIR%29 skos:note """CIR is computed using the
Blaney-Criddle Computer Program (BCCP) developed by NMOSE staff (Wilson, 1990).""" .

:IrrigationSchemeInflows-AUS skos:note "Adelaide", "Perth", <http://www.bom.gov.au/water/awid/search.shtml?q=Irrigation+Scheme+&p=> .

:IrrigationSchemeOutflows-AUS skos:note "Adelaide", "Perth" .

:ManagedAquiferRecharge-AUS skos:note "Adelaide", "Perth", <http://www.bom.gov.au/water/awid/search.shtml?q=Managed+Aquifer+Recharge&p=> .

:UrbanWaterSystemOutflows-AUS skos:note "Adelaide", "Canberra", "Melbourne", "Perth",
    "South East Queensland", "Sydney", <http://www.bom.gov.au/water/awid/search.shtml?q=Urban+Water+System+Outflows&p=> .

:SumOfMonthlyConsumptiveUseFactorsForGrowingSeason%28F%29 skos:note "F = (Temp)(DaylightHours)/100",
    <http://opencdss.state.co.us/statecu/latest/doc-user/ModelDescription/31/#3111-scs-tr-21-modified-or-original-blaney-criddle-method> .

:MonthlyEffectivePrecipitation skos:note "Effective precipitation (i.e. effective rainfall, Re) is the component of precipitation that is available to meet consumptive use. It does not include precipitation lost through runoff and deep percolation below the root zone. StateCU estimates the monthly effective precipitation using one of two methods.",
    <http://opencdss.state.co.us/statecu/latest/doc-user/ModelDescription/31/#312-monthly-effective-precipitation> .

:PublicWaterSupply-NMOSE skos:note "97% of Public Water Supply is metered" .

:MunicipalAndIndustrialDepeltion-UT skos:note <https://www.westernstateswater.org/utah-division-of-water-resources-water-budget-program-methods-description/>,
    <https://www.westernstateswater.org/wp-content/uploads/2017/01/2-Water-Budget-Process.pptx> .

:NMDiversionRecords skos:note "Diversions for most ditches in the San Juan River basin are routinely measured. Diversions to the NIIP are continuously recorded. The measured data is publically available from 2011 to the current date at http://meas.ose.state.nm.us/." .

:NMOSETechnicalReportNo.48 skos:note "Wilson, 1996" .

:RiparianDepletions-UT skos:note <https://www.westernstateswater.org/utah-division-of-water-resources-water-budget-program-methods-description/>,
    <https://www.westernstateswater.org/wp-content/uploads/2017/01/2-Water-Budget-Process.pptx> .

:NaturalFlowGainDistribution skos:note "Estimation method used for ungaged surface water inflow" .

:Non-allocatedExtraction-AUS skos:note "Burdekin", "Murray Darling Basin", <http://www.bom.gov.au/water/awid/search.shtml?q=Extraction&p=> .

:OtherIncreases-AUS skos:note "Burdekin", "Murray Darling Basin" .

:OtherStatutoryRights-AUS skos:note "Adelaide" .

:Outflow-AUS skos:note "Adelaide", "Burdekin", "Canberra", "Daly", "Fitzroy", "Melbourne",
    "Murray Darling Basin", "Ord", "Perth", "South East Queensland", "Sydney", <http://www.bom.gov.au/water/awid/search.shtml?q=Outflow&p=> .

:OverbankFloodSpilling-AUS skos:note "South East Queensland" .

:OverbankFlow-AUS skos:note "Adelaide", "Burdekin", "Canberra", "Daly", "Fitzroy",
    "Melbourne", "Murray Darling Basin", "Ord", "Perth", "South East Queensland", "Sydney" .

:PotentialEvapotranspiration skos:note "Monthly consumptive use", <https://coagmet.colostate.edu/ET_Workshop_2012/CDWR_StateCU.pdf> .

:Precipitation-AUS skos:note "Adelaide", "Burdekin", "Canberra", "Daly", "Fitzroy",
    "Melbourne", "Murray Darling Basin", "Ord", "Perth", "South East Queensland", "Sydney",
    <http://www.bom.gov.au/water/awid/search.shtml?q=Precipitation+&p=> .

:RiverAndFloodplainLosses-AUS skos:note "Canberra" .

:RiverUseByWetPasture-UT skos:note <https://www.westernstateswater.org/wp-content/uploads/2017/01/3-Summary-Page-Documentation-cwm.docx> .

:Runoff-AUS skos:note "Adelaide", "Burdekin", "Canberra", "Daly", "Fitzroy", "Melbourne",
    "Murray Darling Basin", "Ord", "Perth", "South East Queensland", "Sydney", <http://www.bom.gov.au/water/awid/search.shtml?q=Runoff&p=> .

:STATSGOSoilsData skos:note "Soil moisture capacity from crops and STATSGO soils data" .

:Self-SuppliedDomestic-NMOSE skos:note "0% of self supplied domestic is metered" .

:SurfaceWaterFlows-UT skos:note <https://www.westernstateswater.org/wp-content/uploads/2017/01/1-Water-Budget-Process.docx> .

:TotalLandReturnFlow-UT skos:note <https://www.westernstateswater.org/wp-content/uploads/2017/01/3-Summary-Page-Documentation-cwm.docx> .

:TributaryInflow-UT skos:note "https://www.westernstateswater.org/wp-content/uploads/2017/01/3-Summary-Page-Documentation-cwm.docx / Water Budget Process (PPT)",
    <https://www.westernstateswater.org/wp-content/uploads/2017/01/2-Water-Budget-Process.pptx> .

:UrbanWaterSystemInflows-AUS skos:note "Adelaide", "Canberra", "Melbourne", "Perth",
    "South East Queensland", "Sydney", <http://www.bom.gov.au/water/awid/search.shtml?q=Urban+Water+System+Inflows&p=> .

:WastewaterCollected-AUS skos:note "Adelaide", "Canberra", "Perth", "South East Queensland",
    "Sydney", <http://www.bom.gov.au/water/awid/search.shtml?q=Wastewater&p=> .

:AllocatedDiversion%3AEnvironmentalPurposes-AUS skos:note "Murray Darling Basin" .

:AllocatedDiversion%3AIndividualUsers-AUS skos:note "Adelaide", "Burdekin", "Canberra",
    "Daly", "Fitzroy", "Melbourne", "Murray Darling Basin", "Ord", "Perth", "South East Queensland",
    "Sydney", <http://www.bom.gov.au/water/awid/search.shtml?q=Allocated&p=> .

:AllocatedDiversion%3AInter-region-AUS skos:note "Burdekin" .

:AllocatedDiversion%3AIrrigation-AUS skos:note "Burdekin", "Fitzroy", "Ord", <http://www.bom.gov.au/water/awid/search.shtml?q=Irrigation&p=> .

:AllocatedDiversion%3AIrrigationScheme-AUS skos:note "Perth", <http://www.bom.gov.au/water/awid/search.shtml?q=diversion&p=> .

:AllocatedDiversion%3AUrbanSystem-AUS skos:note "Adelaide", "Burdekin", "Canberra",
    "Daly", "Fitzroy", "Melbourne", "Murray Darling Basin", "Ord", "Perth", "South East Queensland",
    "Sydney", <http://www.bom.gov.au/water/awid/search.shtml?q=Allocated&p=> .

:AllocatedDiversions%3ASurfaceWater-AUS skos:note "Adelaide", "Canberra", "Melbourne",
    "Perth", "South East Queensland", "Sydney", <http://www.bom.gov.au/water/awid/search.shtml?q=diversion&p=> .

:AllocatedExtraction%3AEnvironmentalPurposes-AUS skos:note "Murray Darling Basin" .

:AllocatedExtraction%3AGroundwater-AUS skos:note "Melbourne", "Perth", <http://www.bom.gov.au/water/awid/search.shtml?q=extraction+&p=> .

:AllocatedExtraction%3AIndividualUsers-AUS skos:note "Adelaide", "Burdekin", "Canberra",
    "Daly", "Fitzroy", "Melbourne", "Murray Darling Basin", "Ord", "Perth", "South East Queensland",
    <http://www.bom.gov.au/water/awid/search.shtml?q=Extraction&p=>, <http://www.bom.gov.au/water/awid/search.shtml?q=allocated&p=> .

:AllocatedExtraction%3AIrrigation-AUS skos:note "Burdekin", "Fitzroy", <http://www.bom.gov.au/water/awid/search.shtml?q=Extraction&p=> .

:AllocatedExtraction%3AUrbanSystem-AUS skos:note "Burdekin", "Daly", "Fitzroy", "Melbourne",
    "Murray Darling Basin", "Ord", "Perth", <http://www.bom.gov.au/water/awid/search.shtml?q=Extraction&p=> .

:AllocationExtraction%3ASalinityAndWaterTableManagement-AUS skos:note <http://www.bom.gov.au/water/awid/search.shtml?q=Extraction&p=> .

:Delivery%3ADesalinatedWater-AUS skos:note "Adelaide", "Melbourne", "Perth", "South East Queensland",
    "Sydney", <http://www.bom.gov.au/water/awid/search.shtml?q=delivery&p=> .

:Delivery%3AInter-region-AUS skos:note "Canberra", "Perth", "South East Queensland",
    <http://www.bom.gov.au/water/awid/search.shtml?q=Inter-region&p=> .

:Delivery%3AInter-regionAgreement-AUS skos:note "Adelaide", "Melbourne", "Murray Darling Basin",
    "Sydney", <http://www.bom.gov.au/water/awid/search.shtml?q=Inter-region&p=> .

:Delivery%3AIrrigationScheme-AUS skos:note "Adelaide", "Perth" .

:Delivery%3ARecycledWater-AUS skos:note "Adelaide" .

:Delivery%3AUrbanUsers-AUS skos:note "Melbourne" .

:Discharge%3ALandscape-AUS skos:note "Adelaide", "Canberra", "Daly", "Fitzroy", "Melbourne",
    "Murray Darling Basin", "Ord", "Perth", "South East Queensland", "Sydney", <http://www.bom.gov.au/water/awid/search.shtml?q=discharge&p=> .

:Discharge%3ASea-AUS skos:note "Adelaide", "Melbourne", "Perth", "South East Queensland",
    "Sydney", <http://www.bom.gov.au/water/awid/search.shtml?q=Discharge&p=> .

:Discharge%3ASurfaceWater-AUS skos:note "Adelaide", "Canberra", "Daly", "Melbourne",
    "Murray Darling Basin", "Perth", "South East Queensland", <http://www.bom.gov.au/water/awid/search.shtml?q=discharge&p=> .

:Discharge%3AUrbanSupply-AUS skos:note "Perth", <http://www.bom.gov.au/water/awid/search.shtml?q=Discharge&p=> .

:Discharge%3AUrbanSupplySystem-AUS skos:note "Canberra", "Melbourne", "Murray Darling Basin",
    <http://www.bom.gov.au/water/awid/search.shtml?q=Discharge&p=> .

:Discharge%3AUser-AUS skos:note "South East Queensland", "Sydney" .

:Discharge%3AWastewater-AUS skos:note "Adelaide", "Canberra", "Daly", "Melbourne",
    "Murray Darling Basin", "Ord", "South East Queensland", "Sydney", <http://www.bom.gov.au/water/awid/search.shtml?q=Wastewater+Discharge+&p=> .

:Diversions%3AStatutoryRights-AUS skos:note "Canberra", "Daly", "Murray Darling Basin",
    "South East Queensland", "Sydney", <http://www.bom.gov.au/water/awid/search.shtml?q=Diversions&p=> .

:Extraction%3AStatutoryRights-AUS skos:note "Adelaide", "Canberra", "Daly", "Fitzroy",
    "Murray Darling Basin", <http://www.bom.gov.au/water/awid/search.shtml?q=Extraction&p=> .

:Inter-regionInflow%3AGroundwater-AUS skos:note "Adelaide", "Canberra", "Daly", "Fitzroy",
    "Melbourne", "Murray Darling Basin", "Ord", "Perth" .

:Inter-regionInflow%3ASurfaceWater-AUS skos:note "Canberra", "Murray Darling Basin",
    "Perth" .

:Inter-regionOutflow%3AGroundwater-AUS skos:note "Adelaide", "Canberra", "Daly", "Fitzroy",
    "Melbourne", "Murray Darling Basin", "Ord", "Perth" .

:Leakage%3AFarmDams-AUS skos:note "Adelaide" .

:Leakage%3AGroundwater-AUS skos:note "Adelaide", "Canberra", "Melbourne", "Perth",
    "South East Queensland", "Sydney", <http://www.bom.gov.au/water/awid/search.shtml?q=leakage&p=> .

:Leakage%3ALandscape-AUS skos:note "Canberra", "Ord", "Perth", <http://www.bom.gov.au/water/awid/search.shtml?q=leakage&p=> .

:Leakage%3AUrbanSystem-AUS skos:note "Adelaide", "Canberra", "Melbourne", "Murray Darling Basin",
    "Perth", "South East Queensland", <http://www.bom.gov.au/water/awid/search.shtml?q=Leakage&p=> .

:Livestock%3AMetered-NMOSE skos:note "17% of livestock withdrawals are metered" .

:ManagedAquiferRecharge%3AIndividualUser-AUS skos:note "Adelaide", "Burdekin", "Murray Darling Basin",
    <http://www.bom.gov.au/water/awid/search.shtml?q=Aquifer+Recharge&p=> .

:ManagedAquiferRecharge%3AUrban-AUS skos:note "Adelaide" .

:Non-AllocatedDiversion%3ASurfaceWater-AUS skos:note "Adelaide", "South East Queensland" .

:Non-AllocatedExtraction%3AGroundwater-AUS skos:note "Adelaide", "South East Queensland" .

:Non-AllocatedExtraction%3AIndividualUsers-AUS skos:note "Canberra", "Daly", "Fitzroy",
    "Perth", "South East Queensland", <http://www.bom.gov.au/water/awid/search.shtml?q=extraction&p=> .

:Non-AllocatedExtraction%3AIrrigation-AUS skos:note "Adelaide" .

:Non-AllocatedExtraction%3AUrbanSystem-AUS skos:note "South East Queensland" .

:Non-allocatedDiversion%3AEnvironmentalPurposes-AUS skos:note "Murray Darling Basin" .

:Non-allocatedDiversion%3AIndividualUsers-AUS skos:note "Burdekin", "Canberra", "Fitzroy",
    "Melbourne", "Murray Darling Basin", "South East Queensland", <http://www.bom.gov.au/water/awid/search.shtml?q=Diversions&p=> .

:Non-allocatedDiversion%3AUrbanSystem-AUS skos:note "Adelaide", "Murray Darling Basin",
    "South East Queensland", <http://www.bom.gov.au/water/awid/search.shtml?q=Diversions&p=> .

:PointReturn%3AIrrigation-AUS skos:note "Melbourne", "Murray Darling Basin", "Ord",
    <http://www.bom.gov.au/water/awid/search.shtml?q=Point+Return&p=> .

:Recharge%3AGroundwater-AUS skos:note "Canberra", "Daly", "Melbourne", "Murray Darling Basin",
    <http://www.bom.gov.au/water/awid/search.shtml?q=REcharge&p=> .

:Recharge%3ALandscape-AUS skos:note "Adelaide", "Canberra", "Daly", "Fitzroy", "Melbourne",
    "Murray Darling Basin", "Ord", "Perth", <http://www.bom.gov.au/water/awid/search.shtml?q=recharge&p=> .

:Recharge%3ASurfaceWater-AUS skos:note "Canberra", "Daly", "Melbourne", "Murray Darling Basin",
    <http://www.bom.gov.au/water/awid/search.shtml?q=recharge&p=> .

:RecycledWaterDelivery%3AUrbanUsers-AUS skos:note "Adelaide", "Canberra", "Melbourne",
    "Perth", "South East Queensland", "Sydney", <http://www.bom.gov.au/water/awid/search.shtml?q=Delivery&p=> .

:ReturnFlow%3AEnvironmentalPurposes-AUS skos:note "Murray Darling Basin", <http://www.bom.gov.au/water/awid/search.shtml?q=Return+Flow&p=> .

:RiparianRelease%3AUrbanSupply-AUS skos:note "Perth" .

:SupplySystemDelivery%3AInter-Region-AUS skos:note "Perth" .

:SupplySystemDelivery%3AUrbanUsers-AUS skos:note "Adelaide", "Canberra", "Perth",
    "South East Queensland", "Sydney", <http://www.bom.gov.au/water/awid/search.shtml?q=Delivery&p=> .

:SupplySystemDischarge%3AReservoirs-AUS skos:note "Perth" .

:SupplySystemTransfer%3AInter-region-AUS skos:note "Adelaide", "Melbourne", "Perth" .

:Transfer%3AInter-region-AUS skos:note "Melbourne" .

:WastewaterDischarge%3ALandscape-AUS skos:note "Canberra" .

:CAAgriculturalWaterManagementPlans skos:note "Department of Water Resources (DWR)" .

:Cal-SIMETAWUnitValues skos:note "Monthly per acre precipitation", """The Hargreaves-Samani Equation for ET provides a method for estimating potential ET when climate data are limited for planning studies. This method relies on minimum and maximum temperatures and location (i.e., latitude) to predict ET (http://onlinecalc.sdsu.edu/onlinehargreaves.pdf). The Hargeaves-Samini equation is used in Cal-
SIMETAW.""" .

:CaliforniaCentralValleySimulation%28C2VSim%29 skos:note <https://www.water.ca.gov/Library/Modeling-and-Analysis/Central-Valley-models-andtools/C2VSim> .

:CentralValleyHydrologicModel%28CVHM%29 skos:note <https://ca.water.usgs.gov/projects/central-valley/central-valley-hydrologic-model.html> .

:Water-DutyBasedApproach skos:note """Applied water can be approximated by using water duty rates by crop (see Method 4 of Section 3.4) and extrapolating the rates to all areas of interest. Determine acreage by crop type, apply the representative water duty rate by crop, and then sum the results as follows:
Applied Water =  (Acreage by Crop Type * Water Duty Rate by Crop)
If crop acreage by water source (surface water, groundwater, applied water reuse) can be determined, then:
Applied Water by Water Source =  (Acreage by Crop by Water Source * Water Duty Rate by Crop by Water Source)""",
    "Crop ET = Crop Water Duty* Crop Acreage*Irrigation Efficiency" .

:CAUrbanWaterManagementPlans skos:note """California Department of Water Resources (DWR)
Source for Water Budget""" .

:CaliforniaDepartmentOfFinance skos:note "Data used to estimate populations" .

:SWRCBWaterConservationPortal skos:note "California State Water Resources Control Board" .

:USDACropScape skos:note """United States Department of Agriculture  National Agricultural
Statistics Service (NASS)""" .

:USDANaturalResourcesConservationServiceGeospatialWebSoilSurvey skos:note """United States Department of Agriculture  Natural Resources
Conservation Service (NRCS)""" .

:CAIntegratedWaterFlowModel%28IWFM%29 skos:note "California Department of Water Resources" .

:CAIntegratedWaterFlowModel%28IWFM%29DemandCalculator skos:note "California Department of Water Resources (DWR)" .

:CaliforniaStateGroundwaterElevationMonitoring%28CASGEM%29 skos:note "California Department of Water Resources (DWR)" .

:NationalLandCoverDataBase%28NLCD%29 skos:note "Multi-Resolution Land Characteristics (MRLC) Consortium" .

:USDACountyAgCommissioner%27sDataListing skos:note """U.S. Department of Agriculture (USDA)  National Agricultural
Statistics Service, California Field Office (Part of the Pacific
Regional Field Office)""" .

:VegetationConditionExplorer%28VegScape%29 skos:note """United States Department of Agriculture  National Agricultural
Statistics Service (NASS)""" .

:WaterUseClassificationOfLandscapeSpecies%28WUCOLS%29 skos:note """University of California Cooperative Extension, California
Department of Water Resources""" .

:CACountyAgriculturalCommissionerCropReports skos:note "California Agricultural Commissioners" .

:CAValidatedWaterLossReporting skos:note "California Department of Water Resources (DWR)" .

:WaterStorageProduct skos:note <http://www.bom.gov.au/water/dashboards/#/water-storages/summary/state> .

:CaliforniaDataExchangeCenter%28CDEC%29 skos:note "California Department of Water Resources" .

:GravityRecoveryAndClimateExperiment%28GRACE%29 skos:note """National Aeronautics and Space Administration  Earth System
Science Pathfinder Program""" .

:MassBalance skos:note "Change in Groundwater Storage = Inflow to Aquifer  Outflow from Aquifer",
    "Change in Lake/Reservoir Storage = Inflow to Lake  Outflow from Lake", """Evaporation from Stream = Stream Inflow  Stream Outflow + (Runoff + Return Flow + Loss to Stream
from Groundwater + Loss from Lake to Stream + Tributary Inflow to Stream + Precipitation [on Stream]) 
(Surface Water Diversions + Gain from Stream to Groundwater)""",
    """Groundwater Gain from /Loss to Lake = Inflow to Lake from streams  Outflow from Lake to streams 
Lake Evaporation + Precipitation + Change in Lake Storage""",
    "Lake-Stream Interaction = Stream Inflow to Lake (QL(in))  Stream Outflow from Lake (QL(out)) = Precipitation + Change in Lake/Reservoir Storage  Lake Evaporation  Lake to Groundwater Gain (+)/Loss (-)" .

:USGSCaliforniaWaterScienceCenter-GroundwaterModeling skos:note <https://ca.water.usgs.gov/sustainablegroundwater-management/california-groundwater-modeling.html> .

:WaterBalanceForUnsaturatedZoneStorage skos:note "Change in Unsaturated Zone Storage = Change in Land System Storage  Change in Root Zone Soil Moisture Storage  Change in Ponded Water Storage" .

:USBRCentralValleyProjectRefugeWaterDeliveryData skos:note "USBR" .

:NOAANationalCentersForEnvironmentalInformation-ClimateDataOnline skos:note """National Oceanic and Atmospheric Administration 
Cooperative Observe Program (COOP) Weather Stations""" .

:NOAANationalCentersForEnvironmentalInformation-ClimatologicalDataPublications skos:note
    """National Oceanic and Atmospheric Administration  National
Centers for Environmental Information""" .

:NWSCLIMATEPREDICTIONCENTEREVAPORATION skos:note "National Weather Service (NWS) Climate Prediction Center" .

:CaliforniaIrrigationManagementInformationSystem%28CIMIS%29 skos:note """The Penman-Monteith equation estimates ET using mean temperature, wind speed, relative humidity and solar
radiation. It is used in the calculation of ET for CIMIS.""" .

:Evapotranspiration%28ET%29Rates skos:note """ETc,shallow,open water = Kc,shallow,open water * ETo
where Kc,shallow,open water is the crop coefficient for shallow, open water, and
Kc,shallow,open water = 1.1""",
    "Stream Evap: Ec = Ac x ETc, shallow, open water" .

:DrainageAreaRatioMethod skos:note " = (/)  " .

:METRIC-EarthEngineEvapotranspirationFlux skos:note """University of Nebraska-Lincoln, University of Idaho, and Desert
Research Institute with funding support by Google""" .

:CADWRBulletin113%3ACropWaterUse skos:note "California Department of Water Resources (DWR)" .

:MOD16%3AMODISGlobalEvapotranspirationProject skos:note "National Aeronautics and Space Administration (NASA)" .

:NorthAmericanLandDataAssimilationSystem%28NLDAS-2%29 skos:note "National Aeronautics and Space Administration" .

:OperationalSimplifiedSurfaceEnergyBalance%28SSEBop%29 skos:note "USGS" .

:TOPS-SIMS%3ASatelliteIrrigationManagementSupport skos:note """National Atmospheric and Space Administration  Ames
Research Center, California Department of Water Resources,
California State University (Monterey Bay and Fresno), and US
Department of Agriculture  Agricultural Research Service""" .

:PortPhillipCatchmentManagementAuthorityGroundwaterModel skos:note <http://www.bom.gov.au/water/nwa/2019/melbourne/referenceinformation/references.shtml> .

:Darcy%27sLaw skos:note """Qb = Subsurface flow across the boundary
K = Hydraulic conductivity of the aquifer at the boundary
Ab = Cross-sectional area subject to boundary flow
i = Hydraulic gradient through the cross section = (hg  hb) / l
hg = Known groundwater elevation inside the boundary of water budget zone
hb = Known groundwater elevation outside the boundary of water budget zone
b = Depth of cross section
w = Width of cross section
l = Distance between two points with known head, hg and hb
T = Transmissivity of the aquifer at the boundary = K * b""",
    """() = (  )(   ) /   > 
>  """,
    """() = (  )(  ) /   > 
>  """,
    """() = (   +    )(   ) / 
  >  >  """,
    """() = (   +    )(   )/
  >  >  """ .

:Peel-HarveyRegionalAquiferModelingSystem%28PHRAMS%29 dc:source <http://www.bom.gov.au/water/nwa/2019/perth/referenceinformation/methods.shtml>;
  skos:note "This model uses the MODFLOW evaporation module to calculate evapotranspiration from the saturated zone open water wetland surfaces and near surface water table areas." .

:PerthRegionalAquiferModelingSystems%28PRAMS%29 dc:source <http://www.bom.gov.au/water/nwa/2019/perth/referenceinformation/methods.shtml>;
  skos:note "This model uses the MODFLOW evaporation module to calculate evapotranspiration from the saturated zone open water wetland surfaces and near surface water table areas." .

:LandUseAndAppliedWaterEstimationMethod skos:note "GWext = AW for Groundwater or GWext = AW  SWdel  RU",
    """Iw = Agricultural Applied Water / (1  CLF) + Urban Applied Water / (1  CLF) +
Managed Wetlands Applied Water / (1  CLF) + Operational Spill""",
    "Recharge of Applied Water (Di) = Applied Water (AW)  (Crop Evapotranspiration (ET)  Consumptive Use of Precipitation (EP))  Applied Water Reuse (Ru)  Return Flow (Rf)",
    "Recharge of Applied Water = Urban Applied Water  Landscape Evapotranspiration  Consumptive Use of Precipitation  Applied Water Reuse  Return Flow  Recycled Water  Recycled Water Export",
    "SWdel= Applied Water (AW) for Surface Water or SWdel = AW  GWext  RU", """SWdiv = Agricultural Applied Water / (1  CLF) + Urban Applied Water / (1  CLF) +
Managed Wetlands Applied Water / (1  CLF) + Operational Spill""",
    """SWx = Agricultural Applied Water / (1  CLF) + Urban Applied Water / (1  CLF) +
Managed Wetlands Applied Water / (1  CLF) + Operational Spill""" .

:CaliforniaStateWaterResourcesControlBoard%28SWRCB%29UrbanWaterSupplyStatistics skos:note
    "California State Water Resources Control Board" .

:ExistingWaterRightInformationFromStateWaterResourcesControlBoard%28SWRCB%29 skos:note
    "California State Water Resources Control Board" .

:MassTransferEquations skos:note """EL = Lake/reservoir evaporation in mm t-1
M = Mass transfer coefficient in mm t-1 s (kPa m)
es = Saturation vapor pressure at the surface water temperature (kPa)
ez = Saturation vapor pressure of the air at level z (kPa)
uz = Wind speed at level z (m/s)""",
    """Lake Evap: 
 = (  )  """, """ =   (/)
 =    ()
 =       ()
 =   ((/)/)""",
    " = (   )" .

:ReservoirOperationRuleCurve skos:note """In cases where lake and reservoir releases are not monitored and reported, it may be possible to estimate the reservoir operations using a rule curve. Rule curves for reservoirs govern the release of water to balance the demands of flood control, water supply, recreation, and other purposes. Most reservoirs have
a reservoir operation rule curve that can be used to predict the reservoir outflows, given knowledge of the reservoir elevation.""" .

:CentralValleySpatialDatabase-partOfTheCentralValleyHydrologicModel%5BCVHM%5DProject
  skos:note "USGS" .

:WaterRecyclingSurvey%282015%29 skos:note """California State Water Resources Control Board (SWRCB) in
collaboration with the Department of Water Resources (DWR)""" .

:PublicPolicyInstituteOfCalifornia%28PPIC%29Map skos:note "Source: http://www.ppic.org/map/californias-variable-climate/" .

:SWRCBElectronicAnnualReport skos:note "Public Water System" .

:LandSurfaceStock-NM skos:broader :ChangeInLandSystemStorage-CA .

:MunicipalConsumptiveUse-WY dc:source "WY-Agricultural, Municipal, Domestic, and Industrial Water Use Index PDF";
  :flowSink :Atmosphere .

:MunicipalTotalUse-WY dc:source "WY-Agricultural, Municipal, Domestic, and Industrial Water Use Index PDF";
  :flowSink :ZoneLandSystem .

:UTDiversionRecordsFromRiverCommissioners dc:source "Assessing Agricultural Consumptive Use in the Upper Colorado River Basin" .

:AgriculturalConsumptiveUse-WY dc:source "WY-Agricultural, Municipal, Domestic, and Industrial Water Use Index PDF";
  :flowSink :Atmosphere .

:COConsumptiveUseMethod dc:source "Assessing Agricultural Consumptive Use in the Upper Colorado River Basin" .

:CODiversionRecords dc:source "Assessing Agricultural Consumptive Use in the Upper Colorado River Basin" .

:HydroBase dc:source <https://www.colorado.gov/pacific/cdss/hydrobase> .

:CommunityCollaborativeRain%2CHailAndSnowNetwork%28CoCoRaHS%29 dc:source "Assessing Agricultural Consumptive Use in the Upper Colorado River Basin" .

:COIrrigatedAcreageAssessment dc:source "Assessing Agricultural Consumptive Use in the Upper Colorado River Basin" .

:METRIC dc:source "Assessing Agricultural Consumptive Use in the Upper Colorado River Basin" .

:NDVIstar dc:source "Assessing Agricultural Consumptive Use in the Upper Colorado River Basin" .

:RESET dc:source "Assessing Agricultural Consumptive Use in the Upper Colorado River Basin" .

:NationalWeatherServiceStations dc:source "Assessing Agricultural Consumptive Use in the Upper Colorado River Basin" .

:NewMexicoClimateCenterStations dc:source "Assessing Agricultural Consumptive Use in the Upper Colorado River Basin" .

:DaytimeHours dc:source <http://opencdss.state.co.us/statecu/latest/doc-user/ModelDescription/31/#3113-scs-tr-21-modified-or-original-blaney-criddle-method-with-et-elevation-adjustment> .

:DomesticTotalUse-WY dc:source "WY-Agricultural, Municipal, Domestic, and Industrial Water Use Index PDF";
  :flowSink :ZoneLandSystem .

:USGSGroundwaterReports dc:source "UT_1-Water-Budget-Process" .

:IndustrialConsumptiveUse-WY dc:source "WY-Agricultural, Municipal, Domestic, and Industrial Water Use Index PDF" .

:IndustrialTotalUse-WY dc:source "WY-Agricultural, Municipal, Domestic, and Industrial Water Use Index PDF" .

:UTIrrigatedAcreageAssessment dc:source "Assessing Agricultural Consumptive Use in the Upper Colorado River Basin" .

:OriginalHargreaves dc:source "Assessing Agricultural Consumptive Use in the Upper Colorado River Basin" .

:WYDiversionRecords dc:source "Assessing Agricultural Consumptive Use in the Upper Colorado River Basin" .

:AWRA-LModel dc:source <http://www.bom.gov.au/water/nwa/2019/mdb/referenceinformation/methods.shtml#Rivers> .

:AWRA-RModel dc:source <http://www.bom.gov.au/water/nwa/2019/mdb/referenceinformation/methods.shtml#Rivers> .

:AgriculturalAndMunicipalDepletions-UT :flowSink :Atmosphere .

:CropConsumptiveUse-CO :flowSink :Atmosphere .

:GroundwaterExtraction-CA :flowSink :ZoneLandSystem .

:LivestockConsumptiveUse-CO :flowSink :Atmosphere .

:MunicipalAndIndustrialConsumptiveUse-CO :flowSink :Atmosphere .

:SurfaceWaterDiversions-CA :flowSink :ZoneSurfaceWater .

:AgriculturalAndMunicipalDiversions-UT :flowSink :ZoneLandSystem .

:AppliedWater-CA :flowSink :ZoneLandSystem .

:Evapotranspiration-CA :flowSink :Atmosphere .

:IrrigationSurfaceWaterDiversions-WY :flowSink :ZoneLandSystem .

:TotalDiversions-WY :flowSink :ZoneLandSystem .

:AgriculturalDepletions-UT :flowSink :Atmosphere .

:SurfaceDiversionToCropland-UT :flowSink :ZoneLandSystem .

:AgriculturalPotentialConsumptiveUse-UT :flowSink :ZoneLandSystem .

:AreaOutflows :flowSink :ExternalSurfaceWater .

:BasinOutflow-UT :flowSink :ExternalSurfaceWater .

:GagedStreamOutflow-WY :flowSink :ZoneSurfaceWater .

:StreamOutfow-CA :flowSink :ExternalSurfaceWater .

:Exports-CO :flowSink :ExternalGroundwater, :ExternalSurfaceWater .

:BasinInflow-UT :flowSink :ZoneSurfaceWater .

:RiverInflow-UT :flowSink :ZoneSurfaceWater .

:GagedStreamInflow-WY :flowSink :ZoneSurfaceWater .

:GagedSurfaceWaterInflow-CO :flowSink :ZoneSurfaceWater .

:UngagedSurfaceWaterInflow-CO :flowSink :ZoneSurfaceWater .

:StreamInflow-CA :flowSink :ZoneSurfaceWater .

:Commercial-NMOSE :flowSink :ZoneLandSystem .

:MunicipalAndIndustrialDiversions-UT :flowSink :ZoneLandSystem .

:ConveyanceEvaporation-CA :flowSink :Atmosphere .

:HumanConsumption-NM :flowSink :Atmosphere .

:ConveyanceLossesForAllocatedDiversions-AUS :flowSink :ExternalSurfaceWater .

:SurfaceWaterOutflows-AUS :flowSink :Atmosphere, :ExternalGroundwater, :ExternalLandSystem,
    :ExternalSurfaceWater .

:ConveyanceSeepage-CA :flowSink :ZoneGroundwater .

:CoplandPrecipitation-UT :flowSink :ZoneLandSystem .

:Precipitation-CA :flowSink :ZoneLandSystem .

:Precipitation-CO :flowSink :ZoneLandSystem .

:Precipitation-NM :flowSink :ZoneLandSystem .

:Precipitation-UT :flowSink :ZoneLandSystem .

:Precipitation-WY :flowSink :ZoneSurfaceWater .

:IrrigatedAgricultureDepletions-NMOSE :flowSink :Atmosphere .

:Evaporation-AUS :flowSink :Atmosphere .

:Evaporation-NM :flowSink :Atmosphere .

:TotalEvaporation-NM :flowSink :Atmosphere .

:EvaporationFromReservoirs-NMOSE :flowSink :Atmosphere .

:LakeEvaporation-CA :flowSink :Atmosphere .

:ReservoirEvaporation-CO :flowSink :Atmosphere .

:ReservoirEvaporation-UT :flowSink :Atmosphere .

:GroundwaterExport-CA :flowSink :ExternalGroundwater .

:StoredWaterExport-CA :flowSink :ExternalGroundwater .

:SurfaceWaterExports-CA :flowSink :ExternalSurfaceWater .

:FloodReturn-AUS :flowSink :ZoneSurfaceWater .

:SurfaceWaterInflows-AUS :flowSink :ZoneSurfaceWater .

:GagedSurfaceWaterOutflow-CO :flowSink :ExternalSurfaceWater .

:GroundWaterInflow-CO :flowSink :ZoneGroundwater .

:SubsurfaceInflow-CA :flowSink :ZoneGroundwater .

:GroundWaterOutflow-CO :flowSink :ExternalGroundwater .

:SubsurfaceOutflow-CA :flowSink :ExternalGroundwater .

:GroundwaterDischarge-AUS :flowSink :ZoneSurfaceWater .

:Discharge%3AGroundwater-AUS :flowSink :ZoneSurfaceWater .

:GroundwaterDiversions-NM :flowSink :ZoneLandSystem .

:GroundwaterET-NM :flowSink :Atmosphere .

:RiparianConsumption-NM :flowSink :Atmosphere .

:LakeGainFromGroundwater-CA :flowSink :ZoneSurfaceWater .

:GroundwaterInflows-AUS :flowSink :ZoneGroundwater .

:GroundwaterInflows-NM :flowSink :ZoneGroundwater .

:GroundwaterOutflows-AUS :flowSink :ExternalGroundwater, :ExternalLandSystem, :ZoneSurfaceWater .

:GroundwaterOutflows-NM :flowSink :ExternalGroundwater .

:GroundwaterReturn-NM :flowSink :ZoneGroundwater .

:GroundwaterUse-UT :flowSink :ZoneLandSystem .

:PumpedGroundwater-UT :flowSink :ZoneLandSystem .

:ImportedWater-CA :flowSink :ZoneSurfaceWater .

:Imports-CO :flowSink :ZoneLandSystem .

:Industrial-NMOSE :flowSink :ZoneLandSystem .

:IndustrialConsumptiveUse-WY :flowSink :Atmosphere .

:IndustrialTotalUse-WY :flowSink :ZoneLandSystem .

:SurfaceWaterDelivery-CA :flowSink :ZoneLandSystem .

:Inter-regionCoastalInflow-AUS :flowSink :ZoneGroundwater .

:Inter-regionCoastalOutflow-AUS :flowSink :ExternalSurfaceWater .

:IrrigatedAgriculture-NMOSE :flowSink :Atmosphere, :ZoneLandSystem .

:IrrigatedAgricultureDiversions-NMOSE :flowSink :ZoneLandSystem .

:IrrigationSchemeInflows-AUS :flowSink :ZoneLandSystem .

:LakeLossToGroundwater-CA :flowSink :ZoneGroundwater .

:Recharge-NM :flowSink :ZoneGroundwater .

:LandSurfaceExapotranspiration-NM :flowSink :Atmosphere .

:Livestock-NMOSE :flowSink :ZoneLandSystem .

:LivestockConsumptiveUse-WY :flowSink :Atmosphere .

:ManagedAquiferRecharge-AUS :flowSink :ZoneGroundwater .

:UrbanWaterSystemOutflows-AUS :flowSink :ExternalLandSystem, :ExternalSurfaceWater,
    :ZoneGroundwater, :ZoneSurfaceWater .

:ManagedAquiferRecharge-CA :flowSink :ZoneGroundwater .

:Mining-NMOSE :flowSink :ZoneLandSystem .

:Industrial%3AMineProduction-WY :flowSink :ZoneLandSystem .

:Power-NMOSE :flowSink :ZoneLandSystem .

:PublicWaterSupply-NMOSE :flowSink :ZoneLandSystem .

:MunicipalAndIndustrialDepeltion-UT :flowSink :Atmosphere .

:MunicipalAndIndustrialReturnFlow-UT :flowSink :ZoneSurfaceWater .

:ReturnFlow-CA :flowSink :ZoneSurfaceWater .

:NativeVegetationConsumptiveUse-CO :flowSink :Atmosphere .

:NaturalSystemUse-UT :flowSink :Atmosphere .

:RiparianDepletions-UT :flowSink :Atmosphere .

:Non-allocatedExtraction-AUS :flowSink :ExternalLandSystem .

:Outflow-AUS :flowSink :ExternalSurfaceWater .

:OverbankFloodSpilling-AUS :flowSink :ExternalLandSystem .

:OverbankFlow-AUS :flowSink :ExternalLandSystem .

:Industrial%3AElectricalGeneration-WY :flowSink :ZoneLandSystem .

:Precipitation-AUS :flowSink :ZoneSurfaceWater .

:PrecipitationOnLakes-CA :flowSink :ZoneSurfaceWater .

:RechargeOfAppliedWater-CA :flowSink :ZoneGroundwater .

:RechargeOfPrecipitation-CA :flowSink :ZoneGroundwater .

:RecycledWaterExport-CA :flowSink :ExternalLandSystem .

:ReservoirEvaporation-WY :flowSink :Atmosphere .

:RiverAndFloodplainLosses-AUS :flowSink :Atmosphere .

:RiverEvaporation-NM :flowSink :Atmosphere .

:RiverUseByWetPasture-UT :flowSink :ZoneLandSystem .

:Runoff-AUS :flowSink :ZoneLandSystem .

:Runoff-CA :flowSink :ZoneSurfaceWater .

:Runoff-NM :flowSink :ZoneSurfaceWater .

:Self-SuppliedDomestic-NMOSE :flowSink :ZoneLandSystem .

:StoredWaterExtraction-CA :flowSink :ZoneLandSystem .

:StreamEvaporation-CA :flowSink :Atmosphere .

:StreamGainFromGroundwater-CA :flowSink :ZoneSurfaceWater .

:StreamLossToGroundwater-CA :flowSink :ZoneGroundwater .

:SurfaceWaterDiversions-NM :flowSink :ZoneLandSystem .

:SurfaceWaterEvaporation-NM :flowSink :Atmosphere .

:SurfaceWaterFlows-UT :flowSink :ZoneSurfaceWater .

:SurfaceWaterGroundwaterInteractions-NM :flowSink :ZoneGroundwater, :ZoneSurfaceWater .

:SurfaceWaterInflows-NM :flowSink :ZoneSurfaceWater .

:SurfaceWaterOutflows-NM :flowSink :ExternalSurfaceWater .

:SurfaceWaterReturns-NM :flowSink :ZoneSurfaceWater .

:TotalLandReturnFlow-UT :flowSink :ZoneSurfaceWater .

:TributaryInflow-UT :flowSink :ZoneSurfaceWater .

:UngagedStreamGains-WY :flowSink :ZoneSurfaceWater .

:UngagedStreamLosses-WY :flowSink :ExternalGroundwater .

:UrbanWaterSystemInflows-AUS :flowSink :ZoneLandSystem .

:WastewaterCollected-AUS :flowSink :ZoneLandSystem .

:WaterReleaseCausedByLandSubsidence-CA :flowSink :ZoneGroundwater .

:WaterUse-NM :flowSink :ExternalLandSystem, :ExternalSurfaceWater .

:AllocatedDiversion%3AEnvironmentalPurposes-AUS :flowSink :ExternalLandSystem .

:AllocatedDiversion%3AIndividualUsers-AUS :flowSink :ExternalLandSystem .

:AllocatedDiversion%3AInter-region-AUS :flowSink :ExternalSurfaceWater .

:AllocatedDiversion%3AIrrigation-AUS :flowSink :ExternalLandSystem .

:AllocatedDiversion%3AIrrigationScheme-AUS :flowSink :ZoneLandSystem .

:AllocatedDiversion%3AUrbanSystem-AUS :flowSink :ExternalLandSystem .

:AllocatedDiversions%3ASurfaceWater-AUS :flowSink :ZoneLandSystem .

:AllocatedExtraction%3AEnvironmentalPurposes-AUS :flowSink :ExternalLandSystem .

:AllocatedExtraction%3AGroundwater-AUS :flowSink :ZoneLandSystem .

:AllocatedExtraction%3AIndividualUsers-AUS :flowSink :ExternalLandSystem .

:AllocatedExtraction%3AIrrigation-AUS :flowSink :ExternalLandSystem .

:AllocatedExtraction%3AUrbanSystem-AUS :flowSink :ExternalLandSystem .

:AllocationExtraction%3ASalinityAndWaterTableManagement-AUS :flowSink :ExternalLandSystem,
    :ExternalSurfaceWater .

:AppliedWaterReuse%2FRecycledWater-CA :flowSink :ZoneLandSystem .

:Delivery%3ADesalinatedWater-AUS :flowSink :ZoneLandSystem .

:Delivery%3AInter-region-AUS :flowSink :ZoneLandSystem, :ZoneSurfaceWater .

:Delivery%3AInter-regionAgreement-AUS :flowSink :ZoneSurfaceWater .

:Delivery%3AIrrigationScheme-AUS :flowSink :ExternalLandSystem .

:Discharge%3ALandscape-AUS :flowSink :ExternalLandSystem .

:Discharge%3ASea-AUS :flowSink :ExternalSurfaceWater .

:Discharge%3ASurfaceWater-AUS :flowSink :ZoneSurfaceWater .

:Discharge%3AUrbanSupply-AUS :flowSink :ZoneSurfaceWater .

:Discharge%3AUrbanSupplySystem-AUS :flowSink :ZoneSurfaceWater .

:Discharge%3AUser-AUS :flowSink :ZoneSurfaceWater .

:Discharge%3AWastewater-AUS :flowSink :ZoneSurfaceWater .

:Diversions%3AStatutoryRights-AUS :flowSink :ExternalLandSystem .

:Extraction%3AStatutoryRights-AUS :flowSink :ExternalLandSystem .

:Industrial%3ACoalbedMethandProduction-WY :flowSink :ZoneLandSystem .

:Industrial%3AMiscellaneous-WY :flowSink :ZoneLandSystem .

:Industrial%3ANaturalGas-WY :flowSink :Atmosphere .

:Industrial%3AOilAndGas-WY :flowSink :ZoneLandSystem .

:Inter-regionInflow%3AGroundwater-AUS :flowSink :ZoneGroundwater .

:Inter-regionInflow%3ASurfaceWater-AUS :flowSink :ZoneSurfaceWater .

:Inter-regionOutflow%3AGroundwater-AUS :flowSink :ExternalGroundwater .

:IrrigationWaterSupplyLimitedConsumptiveUse%28Depletions%29-WY :flowSink :Atmosphere .

:Leakage%3AFarmDams-AUS :flowSink :ZoneGroundwater .

:Leakage%3AGroundwater-AUS :flowSink :ExternalGroundwater, :ZoneGroundwater .

:Leakage%3ALandscape-AUS :flowSink :ZoneLandSystem .

:Leakage%3AUrbanSystem-AUS :flowSink :ZoneGroundwater .

:ManagedAquiferRecharge%3AIndividualUser-AUS :flowSink :ZoneGroundwater .

:Non-AllocatedExtraction%3AIndividualUsers-AUS :flowSink :ExternalLandSystem .

:Non-allocatedDiversion%3AEnvironmentalPurposes-AUS :flowSink :ExternalLandSystem .

:Non-allocatedDiversion%3AIndividualUsers-AUS :flowSink :ExternalLandSystem .

:Non-allocatedDiversion%3AUrbanSystem-AUS :flowSink :ExternalLandSystem .

:PointReturn%3AIrrigation-AUS :flowSink :ZoneLandSystem .

:Recharge%3AGroundwater-AUS :flowSink :ZoneGroundwater .

:Recharge%3ALandscape-AUS :flowSink :ZoneGroundwater .

:Recharge%3ASurfaceWater-AUS :flowSink :ZoneGroundwater .

:RecycledWaterDelivery%3AUrbanUsers-AUS :flowSink :ExternalLandSystem .

:ReturnFlow%3AEnvironmentalPurposes-AUS :flowSink :ZoneSurfaceWater .

:RiparianRelease%3AUrbanSupply-AUS :flowSink :ZoneSurfaceWater .

:SupplySystemDelivery%3AInter-Region-AUS :flowSink :ZoneLandSystem .

:SupplySystemDelivery%3AUrbanUsers-AUS :flowSink :ExternalLandSystem .

:SupplySystemDischarge%3AReservoirs-AUS :flowSink :ZoneSurfaceWater .

:SupplySystemTransfer%3AInter-region-AUS :flowSink :ExternalLandSystem .

:OtherSupplySystemDecreases-AUS :flowSink :ExternalGroundwater, :ExternalLandSystem,
    :ExternalSurfaceWater .

:OtherWastewaterDecreases-AUS :flowSink :ExternalLandSystem .

:RiverLosses-AUS :flowSink :ExternalGroundwater, :ExternalLandSystem .

:Losses%3AManagementOfTreatedWater-AUS :flowSink :ExternalSurfaceWater .

:Losses%3AWastewaterTreatmentSystem-AUS :flowSink :ExternalSurfaceWater .

:RecycledWaterDelivery%3AIrrigation-AUS :flowSink :ExternalLandSystem .

:SupplySystemDelivery%3AIrrigation-AUS :flowSink :ExternalLandSystem .

:SupplySystemDischarge%3ASurfaceWater-AUS :flowSink :ZoneSurfaceWater .

:WastewaterAndRecycledWaterDischarge%3ASurfaceWater-AUS :flowSink :ZoneSurfaceWater .

:WastewaterDischarge%3ASurfaceWater-AUS :flowSink :ZoneSurfaceWater .

:AgriculturalAndMunicipalDepletions-UT :flowSource :ZoneGroundwater, :ZoneSurfaceWater .

:CropConsumptiveUse-CO :flowSource :ZoneLandSystem .

:GroundwaterExtraction-CA :flowSource :ZoneGroundwater .

:LivestockConsumptiveUse-CO :flowSource :ZoneGroundwater, :ZoneSurfaceWater .

:MunicipalAndIndustrialConsumptiveUse-CO :flowSource :ZoneGroundwater, :ZoneSurfaceWater .

:MunicipalConsumptiveUse-WY :flowSource :ZoneGroundwater, :ZoneSurfaceWater .

:MunicipalTotalUse-WY :flowSource :ZoneGroundwater, :ZoneSurfaceWater .

:SurfaceWaterDiversions-CA :flowSource :ZoneSurfaceWater .

:AgriculturalAndMunicipalDiversions-UT :flowSource :ZoneGroundwater, :ZoneSurfaceWater .

:AppliedWater-CA :flowSource :ZoneLandSystem .

:AgriculturalConsumptiveUse-WY :flowSource :ZoneGroundwater, :ZoneSurfaceWater .

:Evapotranspiration-CA :flowSource :ZoneLandSystem .

:IrrigationSurfaceWaterDiversions-WY :flowSource :ZoneSurfaceWater .

:TotalDiversions-WY :flowSource :ZoneSurfaceWater .

:AgriculturalDepletions-UT :flowSource :ZoneGroundwater, :ZoneLandSystem .

:SurfaceDiversionToCropland-UT :flowSource :ZoneSurfaceWater .

:AgriculturalPotentialConsumptiveUse-UT :flowSource :ZoneGroundwater, :ZoneSurfaceWater .

:AreaOutflows :flowSource :ZoneLandSystem, :ZoneSurfaceWater .

:BasinOutflow-UT :flowSource :ZoneSurfaceWater .

:GagedStreamOutflow-WY :flowSource :ZoneSurfaceWater .

:StreamOutfow-CA :flowSource :ZoneSurfaceWater .

:Exports-CO :flowSource :ZoneGroundwater, :ZoneSurfaceWater .

:BasinInflow-UT :flowSource :ExternalSurfaceWater .

:RiverInflow-UT :flowSource :ExternalSurfaceWater .

:GagedStreamInflow-WY :flowSource :ExternalSurfaceWater .

:GagedSurfaceWaterInflow-CO :flowSource :ExternalSurfaceWater .

:UngagedSurfaceWaterInflow-CO :flowSource :ExternalSurfaceWater .

:StreamInflow-CA :flowSource :ExternalSurfaceWater .

:Commercial-NMOSE :flowSource :ZoneGroundwater, :ZoneSurfaceWater .

:MunicipalAndIndustrialDiversions-UT :flowSource :ZoneGroundwater, :ZoneSurfaceWater .

:ConveyanceEvaporation-CA :flowSource :ZoneSurfaceWater .

:HumanConsumption-NM :flowSource :ZoneLandSystem .

:ConveyanceLossesForAllocatedDiversions-AUS :flowSource :ZoneSurfaceWater .

:SurfaceWaterOutflows-AUS :flowSource :ZoneSurfaceWater .

:ConveyanceSeepage-CA :flowSource :ZoneSurfaceWater .

:CoplandPrecipitation-UT :flowSource :Atmosphere .

:Precipitation-CA :flowSource :Atmosphere .

:Precipitation-CO :flowSource :Atmosphere .

:Precipitation-NM :flowSource :Atmosphere .

:Precipitation-UT :flowSource :Atmosphere .

:Precipitation-WY :flowSource :Atmosphere .

:IrrigatedAgricultureDepletions-NMOSE :flowSource :ZoneLandSystem .

:DomesticTotalUse-WY :flowSource :ZoneGroundwater .

:Evaporation-AUS :flowSource :ZoneSurfaceWater .

:Evaporation-NM :flowSource :ZoneLandSystem .

:TotalEvaporation-NM :flowSource :ZoneGroundwater, :ZoneLandSystem, :ZoneSurfaceWater .

:EvaporationFromReservoirs-NMOSE :flowSource :ZoneSurfaceWater .

:LakeEvaporation-CA :flowSource :ZoneSurfaceWater .

:ReservoirEvaporation-CO :flowSource :ZoneSurfaceWater .

:ReservoirEvaporation-UT :flowSource :ZoneSurfaceWater .

:GroundwaterExport-CA :flowSource :ZoneGroundwater .

:StoredWaterExport-CA :flowSource :ZoneGroundwater .

:SurfaceWaterExports-CA :flowSource :ZoneSurfaceWater .

:FloodReturn-AUS :flowSource :ExternalLandSystem .

:SurfaceWaterInflows-AUS :flowSource :Atmosphere, :ExternalLandSystem, :ExternalSurfaceWater,
    :ZoneGroundwater .

:GagedSurfaceWaterOutflow-CO :flowSource :ZoneSurfaceWater .

:GroundWaterInflow-CO :flowSource :ExternalGroundwater .

:SubsurfaceInflow-CA :flowSource :ExternalGroundwater .

:GroundWaterOutflow-CO :flowSource :ZoneGroundwater .

:SubsurfaceOutflow-CA :flowSource :ZoneGroundwater .

:GroundwaterDischarge-AUS :flowSource :ZoneGroundwater .

:Discharge%3AGroundwater-AUS :flowSource :ZoneGroundwater .

:GroundwaterDiversions-NM :flowSource :ZoneGroundwater .

:GroundwaterET-NM :flowSource :ZoneGroundwater .

:RiparianConsumption-NM :flowSource :ZoneGroundwater .

:LakeGainFromGroundwater-CA :flowSource :ZoneGroundwater .

:GroundwaterInflows-AUS :flowSource :ExternalGroundwater, :ExternalLandSystem, :ExternalSurfaceWater,
    :ZoneLandSystem, :ZoneSurfaceWater .

:GroundwaterInflows-NM :flowSource :ExternalGroundwater .

:GroundwaterOutflows-AUS :flowSource :ZoneGroundwater .

:GroundwaterOutflows-NM :flowSource :ZoneGroundwater .

:GroundwaterReturn-NM :flowSource :ZoneLandSystem .

:GroundwaterUse-UT :flowSource :ZoneGroundwater .

:PumpedGroundwater-UT :flowSource :ZoneGroundwater .

:ImportedWater-CA :flowSource :ExternalSurfaceWater .

:Imports-CO :flowSource :ExternalGroundwater, :ExternalSurfaceWater .

:Industrial-NMOSE :flowSource :ZoneGroundwater .

:IndustrialConsumptiveUse-WY :flowSource :ZoneGroundwater, :ZoneSurfaceWater .

:IndustrialTotalUse-WY :flowSource :ZoneGroundwater, :ZoneSurfaceWater .

:SurfaceWaterDelivery-CA :flowSource :ZoneSurfaceWater .

:Inter-regionCoastalInflow-AUS :flowSource :ExternalSurfaceWater .

:Inter-regionCoastalOutflow-AUS :flowSource :ZoneGroundwater .

:IrrigatedAgriculture-NMOSE :flowSource :ZoneGroundwater, :ZoneSurfaceWater .

:IrrigatedAgricultureDiversions-NMOSE :flowSource :ZoneGroundwater, :ZoneSurfaceWater .

:IrrigationSchemeOutflows-AUS :flowSource :ZoneLandSystem .

:LakeLossToGroundwater-CA :flowSource :ZoneSurfaceWater .

:Recharge-NM :flowSource :ZoneLandSystem .

:LandSurfaceExapotranspiration-NM :flowSource :ZoneLandSystem .

:Livestock-NMOSE :flowSource :ZoneGroundwater, :ZoneSurfaceWater .

:LivestockConsumptiveUse-WY :flowSource :ZoneSurfaceWater .

:ManagedAquiferRecharge-AUS :flowSource :ZoneLandSystem, :ZoneSurfaceWater .

:UrbanWaterSystemOutflows-AUS :flowSource :ZoneLandSystem .

:ManagedAquiferRecharge-CA :flowSource :ZoneLandSystem .

:Mining-NMOSE :flowSource :ZoneGroundwater, :ZoneSurfaceWater .

:Industrial%3AMineProduction-WY :flowSource :ZoneGroundwater, :ZoneSurfaceWater .

:Power-NMOSE :flowSource :ZoneGroundwater, :ZoneSurfaceWater .

:PublicWaterSupply-NMOSE :flowSource :ZoneGroundwater, :ZoneSurfaceWater .

:MunicipalAndIndustrialDepeltion-UT :flowSource :ZoneGroundwater, :ZoneSurfaceWater .

:MunicipalAndIndustrialReturnFlow-UT :flowSource :ZoneLandSystem .

:ReturnFlow-CA :flowSource :ZoneLandSystem .

:NativeVegetationConsumptiveUse-CO :flowSource :ZoneGroundwater, :ZoneSurfaceWater .

:NaturalSystemUse-UT :flowSource :ZoneLandSystem, :ZoneSurfaceWater .

:RiparianDepletions-UT :flowSource :ZoneLandSystem .

:Non-allocatedExtraction-AUS :flowSource :ZoneGroundwater .

:Outflow-AUS :flowSource :AUSBureauOfMeteorology, :ZoneSurfaceWater .

:OverbankFloodSpilling-AUS :flowSource :ZoneSurfaceWater .

:OverbankFlow-AUS :flowSource :ZoneSurfaceWater .

:Industrial%3AElectricalGeneration-WY :flowSource :ZoneGroundwater .

:Precipitation-AUS :flowSource :Atmosphere .

:PrecipitationOnLakes-CA :flowSource :Atmosphere .

:RechargeOfAppliedWater-CA :flowSource :ZoneLandSystem .

:RechargeOfPrecipitation-CA :flowSource :ZoneLandSystem .

:RecycledWaterExport-CA :flowSource :ZoneLandSystem .

:ReservoirEvaporation-WY :flowSource :ZoneSurfaceWater .

:RiverAndFloodplainLosses-AUS :flowSource :ZoneLandSystem, :ZoneSurfaceWater .

:RiverEvaporation-NM :flowSource :ZoneSurfaceWater .

:RiverUseByWetPasture-UT :flowSource :ZoneSurfaceWater .

:Runoff-AUS :flowSource :ExternalLandSystem .

:Runoff-CA :flowSource :ZoneLandSystem .

:Runoff-NM :flowSource :ZoneLandSystem .

:Self-SuppliedDomestic-NMOSE :flowSource :ZoneGroundwater .

:StoredWaterExtraction-CA :flowSource :ZoneGroundwater .

:StreamEvaporation-CA :flowSource :ZoneSurfaceWater .

:StreamGainFromGroundwater-CA :flowSource :ZoneGroundwater .

:StreamLossToGroundwater-CA :flowSource :ZoneSurfaceWater .

:SurfaceWaterDiversions-NM :flowSource :ZoneSurfaceWater .

:SurfaceWaterEvaporation-NM :flowSource :ZoneSurfaceWater .

:SurfaceWaterFlows-UT :flowSource :ZoneSurfaceWater .

:SurfaceWaterGroundwaterInteractions-NM :flowSource :ZoneGroundwater, :ZoneSurfaceWater .

:SurfaceWaterInflows-NM :flowSource :ExternalSurfaceWater .

:SurfaceWaterOutflows-NM :flowSource :ZoneSurfaceWater .

:SurfaceWaterReturns-NM :flowSource :ZoneLandSystem .

:TotalLandReturnFlow-UT :flowSource :ZoneLandSystem .

:TributaryInflow-UT :flowSource :ExternalSurfaceWater .

:UngagedStreamGains-WY :flowSource :ExternalGroundwater .

:UngagedStreamLosses-WY :flowSource :ZoneSurfaceWater .

:WastewaterCollected-AUS :flowSource :ExternalLandSystem .

:WaterUse-NM :flowSource :ZoneGroundwater, :ZoneSurfaceWater .

:AllocatedDiversion%3AEnvironmentalPurposes-AUS :flowSource :ZoneSurfaceWater .

:AllocatedDiversion%3AIndividualUsers-AUS :flowSource :ZoneSurfaceWater .

:AllocatedDiversion%3AInter-region-AUS :flowSource :ZoneSurfaceWater .

:AllocatedDiversion%3AIrrigation-AUS :flowSource :ZoneSurfaceWater .

:AllocatedDiversion%3AIrrigationScheme-AUS :flowSource :ZoneSurfaceWater .

:AllocatedDiversion%3AUrbanSystem-AUS :flowSource :ZoneSurfaceWater .

:AllocatedDiversions%3ASurfaceWater-AUS :flowSource :ZoneSurfaceWater .

:AllocatedExtraction%3AEnvironmentalPurposes-AUS :flowSource :ZoneGroundwater .

:AllocatedExtraction%3AGroundwater-AUS :flowSource :ZoneGroundwater .

:AllocatedExtraction%3AIndividualUsers-AUS :flowSource :ZoneGroundwater .

:AllocatedExtraction%3AIrrigation-AUS :flowSource :ZoneGroundwater .

:AllocatedExtraction%3AUrbanSystem-AUS :flowSource :ZoneGroundwater .

:AllocationExtraction%3ASalinityAndWaterTableManagement-AUS :flowSource :ZoneGroundwater .

:AppliedWaterReuse%2FRecycledWater-CA :flowSource :ZoneLandSystem .

:Delivery%3ADesalinatedWater-AUS :flowSource :ExternalSurfaceWater .

:Delivery%3AInter-region-AUS :flowSource :ExternalSurfaceWater .

:Delivery%3AInter-regionAgreement-AUS :flowSource :ExternalSurfaceWater .

:Delivery%3AIrrigationScheme-AUS :flowSource :ZoneLandSystem .

:Discharge%3ALandscape-AUS :flowSource :ZoneGroundwater, :ZoneLandSystem .

:Discharge%3ASea-AUS :flowSource :ZoneLandSystem .

:Discharge%3ASurfaceWater-AUS :flowSource :ZoneGroundwater, :ZoneLandSystem .

:Discharge%3AUrbanSupply-AUS :flowSource :ZoneLandSystem .

:Discharge%3AUrbanSupplySystem-AUS :flowSource :ExternalLandSystem .

:Discharge%3AUser-AUS :flowSource :ExternalLandSystem .

:Discharge%3AWastewater-AUS :flowSource :ExternalLandSystem .

:Diversions%3AStatutoryRights-AUS :flowSource :ZoneSurfaceWater .

:Extraction%3AStatutoryRights-AUS :flowSource :ZoneGroundwater .

:Industrial%3ACoalbedMethandProduction-WY :flowSource :ZoneGroundwater, :ZoneSurfaceWater .

:Industrial%3AMiscellaneous-WY :flowSource :ZoneGroundwater, :ZoneSurfaceWater .

:Industrial%3ANaturalGas-WY :flowSource :ZoneGroundwater, :ZoneSurfaceWater .

:Industrial%3AOilAndGas-WY :flowSource :ZoneGroundwater, :ZoneSurfaceWater .

:Inter-regionInflow%3AGroundwater-AUS :flowSource :ExternalGroundwater .

:Inter-regionInflow%3ASurfaceWater-AUS :flowSource :ExternalSurfaceWater .

:Inter-regionOutflow%3AGroundwater-AUS :flowSource :ZoneGroundwater .

:IrrigationWaterSupplyLimitedConsumptiveUse%28Depletions%29-WY :flowSource :ZoneSurfaceWater .

:Leakage%3AFarmDams-AUS :flowSource :ExternalLandSystem .

:Leakage%3AGroundwater-AUS :flowSource :ZoneLandSystem .

:Leakage%3ALandscape-AUS :flowSource :ZoneSurfaceWater .

:Leakage%3AUrbanSystem-AUS :flowSource :ExternalLandSystem, :ZoneLandSystem .

:ManagedAquiferRecharge%3AIndividualUser-AUS :flowSource :ExternalLandSystem .

:Non-AllocatedExtraction%3AIndividualUsers-AUS :flowSource :ZoneGroundwater .

:Non-allocatedDiversion%3AEnvironmentalPurposes-AUS :flowSource :ZoneSurfaceWater .

:Non-allocatedDiversion%3AIndividualUsers-AUS :flowSource :ZoneSurfaceWater .

:Non-allocatedDiversion%3AUrbanSystem-AUS :flowSource :ZoneSurfaceWater .

:PointReturn%3AIrrigation-AUS :flowSource :ExternalLandSystem .

:Recharge%3AGroundwater-AUS :flowSource :ZoneSurfaceWater .

:Recharge%3ALandscape-AUS :flowSource :ExternalLandSystem .

:Recharge%3ASurfaceWater-AUS :flowSource :ZoneSurfaceWater .

:RecycledWaterDelivery%3AUrbanUsers-AUS :flowSource :ZoneLandSystem .

:ReturnFlow%3AEnvironmentalPurposes-AUS :flowSource :ExternalLandSystem .

:RiparianRelease%3AUrbanSupply-AUS :flowSource :ZoneLandSystem .

:SupplySystemDelivery%3AInter-Region-AUS :flowSource :ExternalLandSystem .

:SupplySystemDelivery%3AUrbanUsers-AUS :flowSource :ZoneLandSystem .

:SupplySystemDischarge%3AReservoirs-AUS :flowSource :ZoneLandSystem .

:SupplySystemTransfer%3AInter-region-AUS :flowSource :ZoneLandSystem .

:FlowData :flowSource :AUSBureauOfMeteorology .

:OtherSupplySystemDecreases-AUS :flowSource :ZoneLandSystem .

:OtherWastewaterDecreases-AUS :flowSource :ZoneLandSystem .

:RiverLosses-AUS :flowSource :ZoneSurfaceWater .

:Losses%3AManagementOfTreatedWater-AUS :flowSource :ZoneLandSystem .

:Losses%3AWastewaterTreatmentSystem-AUS :flowSource :ZoneLandSystem .

:RecycledWaterDelivery%3AIrrigation-AUS :flowSource :ZoneLandSystem .

:SupplySystemDelivery%3AIrrigation-AUS :flowSource :ZoneLandSystem .

:SupplySystemDischarge%3ASurfaceWater-AUS :flowSource :ZoneLandSystem .

:WastewaterAndRecycledWaterDischarge%3ASurfaceWater-AUS :flowSource :ZoneLandSystem .

:WastewaterDischarge%3ASurfaceWater-AUS :flowSource :ZoneLandSystem .

:GroundwaterExtraction-CA :hasDataSource :CAIntegratedWaterFlowModel%28IWFM%29, :CALSIM2,
    :CAPreviousReports, :Cal-SIMETAWUnitValues, :CaliforniaAgriculturalLandAndWaterUseEstimates,
    :CaliforniaCentralValleySimulation%28C2VSim%29, :CaliforniaDepartmentOfWaterResources%28DWR%29UrbanWaterSupplyStatistics,
    :CaliforniaStateWaterResourcesControlBoard%28SWRCB%29UrbanWaterSupplyStatistics, :CaliforniaWaterPlanPortfolio,
    :CaliforniaWaterPlanUpdateData, :CentralValleyHydrologicModel%28CVHM%29, :DWRLandUseSurveys,
    :LocalAgencyRecords, :MODFLOW-OWHM%3AOneWaterHydrologicFlowModel, :SWRCBWaterConservationPortal .

:LivestockConsumptiveUse-CO :hasDataSource :StateAgriculturalStatistics .

:MunicipalAndIndustrialConsumptiveUse-CO :hasDataSource :ColoradoCensusBureau .

:MunicipalConsumptiveUse-WY :hasDataSource :USCensusBureau .

:MunicipalTotalUse-WY :hasDataSource :USCensusBureau .

:SurfaceWaterDiversions-CA :hasDataSource :CADWRBulletin132%3AManagementOfTheCaliforniaStateWaterProject,
    :CADWRSGMADataViewer, :CAIntegratedWaterFlowModel%28IWFM%29, :CALSIM2, :CALSIM3, :Cal-SIMETAWUnitValues,
    :CaliforniaAgriculturalLandAndWaterUseEstimates, :CaliforniaCentralValleySimulation%28C2VSim%29,
    :CaliforniaWaterPlanPortfolio, :DWRWaterDataLibrary%3ASurfaceWaterAndGroundwaterData,
    :ExistingWaterRightInformationFromStateWaterResourcesControlBoard%28SWRCB%29, :MODFLOW-OWHM%3AOneWaterHydrologicFlowModel,
    :USBRCentralValleyProjectRefugeWaterDeliveryData, :USGSPublications, :USGSSurface-WaterDataForCalifornia .

:AgriculturalAndMunicipalDiversions-UT :hasDataSource :USGSStreamGages, :UTDiversionRecordsFromRiverCommissioners,
    :UTMunicipalPotableAndSecondaryDiversionRecords, :UTOtherIrrigationCompanyRecords,
    :UTReservoirStorageAndReleaseRecords, :UTWaterRights .

:AppliedWater-CA :hasDataSource :CAAgriculturalWaterManagementPlans, :CADWRDemographicData,
    :CADWRIrrigationMethodsSurvey, :CADWRLandUseViewer, :CADWRSGMADataViewer, :CAIntegratedWaterFlowModel%28IWFM%29,
    :CAIntegratedWaterFlowModel%28IWFM%29DemandCalculator, :CALSIM2, :CAUrbanWaterManagementPlans,
    :Cal-SIMETAWUnitValues, :CaliforniaAgriculturalLandAndWaterUseEstimates, :CaliforniaCentralValleySimulation%28C2VSim%29,
    :CaliforniaDepartmentOfFinance, :CaliforniaPesticideInformationPortal, :CaliforniaStateGroundwaterElevationMonitoring%28CASGEM%29,
    :CaliforniaWaterPlanPortfolio, :CentralValleyHydrologicModel%28CVHM%29, :DWRLandUseSurveys,
    :MODFLOW-OWHM%3AOneWaterHydrologicFlowModel, :NationalLandCoverDataBase%28NLCD%29,
    :SWRCBWaterConservationPortal, :USCensusBureau, :USDACountyAgCommissioner%27sDataListing,
    :USDACropScape, :USDANaturalResourcesConservationServiceGeospatialWebSoilSurvey, :VegetationConditionExplorer%28VegScape%29,
    :WaterUseClassificationOfLandscapeSpecies%28WUCOLS%29 .

:USGSStreamStats :hasDataSource :USGSStreamGages .

:WYConsumptiveUseMethod :hasDataSource :NationalClimaticDataCenter%27sClimatographyOfTheUnitedStatesNo.81,
    :NationalOceanicAndAtmosphericAdministrationStations, :NationalWeatherServiceStations,
    :NaturalResourcesConservationServiceStations%28NRCS%29, :PRISM, :RemoteAutomatedWeatherStations%28RAWS%29,
    :SCSTR21, :SatelliteAndAerialPhotos, :SnotelNetworkOfWeatherStations, :USBureauOfLandManagement%28BLM%29,
    :USGSStreamGages, :USGeologicalSurvey%28USGS%29, :WYDepartmentOfEnvironmentalQuality%28DEQ%29,
    :WYDiversionRecords, :WyomingStateEngineer%27sOfficeStations, :WyomingWaterResourcesDataSystem%28WRDS%29 .

:Evapotranspiration-CA :hasDataSource :CAAgriculturalWaterManagementPlans, :CACountyAgriculturalCommissionerCropReports,
    :CADWRBulletin113%3ACropWaterUse, :CADWRLandUseViewer, :CADWRSGMADataViewer, :CAIntegratedWaterFlowModel%28IWFM%29,
    :CAIntegratedWaterFlowModel%28IWFM%29DemandCalculator, :CAIrrigationTrainingAndResearchCenter%28ITRC%29EvapotranspirationData,
    :CALSIM2, :Cal-SIMETAWUnitValues, :CaliforniaAgriculturalLandAndWaterUseEstimates,
    :CaliforniaCentralValleySimulation%28C2VSim%29, :CaliforniaPesticideInformationPortal,
    :CaliforniaStateGroundwaterElevationMonitoring%28CASGEM%29, :CaliforniaWaterPlanPortfolio,
    :CentralValleyHydrologicModel%28CVHM%29, :DWRLandUseSurveys, :FAO56Chapter6SingleCropCoefficients%28Kc%29,
    :METRIC-EarthEngineEvapotranspirationFlux, :MOD16%3AMODISGlobalEvapotranspirationProject,
    :MODFLOW-OWHM%3AOneWaterHydrologicFlowModel, :NOAANationalCentersForEnvironmentalInformation-ClimateDataOnline,
    :NOAANationalCentersForEnvironmentalInformation-ClimatologicalDataPublications, :NOAAOfficeOfSatelliteAndProductOperationsALEXI%3AAtmosphere-LandExchangeInverseModel,
    :NWSCLIMATEPREDICTIONCENTEREVAPORATION, :NationalLandCoverDataBase%28NLCD%29, :NorthAmericanLandDataAssimilationSystem%28NLDAS-2%29,
    :OperationalSimplifiedSurfaceEnergyBalance%28SSEBop%29, :SpatialCaliforniaIrrigationManagementInformationSystem%28CIMIS%29,
    :TOPS-SIMS%3ASatelliteIrrigationManagementSupport, :USDACountyAgCommissioner%27sDataListing,
    :USDACropScape, :USGSBasinCharacterizationModel, :VegetationConditionExplorer%28VegScape%29,
    :WaterUseClassificationOfLandscapeSpecies%28WUCOLS%29 .

:IrrigationSurfaceWaterDiversions-WY :hasDataSource :WYDiversionDataFromWaterUsers,
    :WYOfficeOfTheStateEngineer .

:TotalDiversions-WY :hasDataSource :WYDiversionDataFromWaterUsers, :WYOfficeOfTheStateEngineer .

:UTConsumptiveUseMethod :hasDataSource :EmeryWaterConservancyDistrictStations, :FruitGrowersNetworkStations%28FGNET%29,
    :GroundSurvey, :MesoWestStations, :NationalOceanicAndAtmosphericAdministrationStations,
    :PRISM, :SatelliteAndAerialPhotos, :SoilClimateAnalysisNetwork%28SCAN%29, :USBureauOfReclamationAgriMetStations,
    :USGSStreamGages, :UTDiversionRecordsFromRiverCommissioners .

:SurfaceDiversionToCropland-UT :hasDataSource :USGSStreamGages, :UTDiversionRecordsFromRiverCommissioners,
    :UTMunicipalPotableAndSecondaryDiversionRecords, :UTOtherIrrigationCompanyRecords,
    :UTReservoirStorageAndReleaseRecords, :UTWaterRights .

:AgriculturalPotentialConsumptiveUse-UT :hasDataSource :NationalOceanicAndAtmosphericAdministrationStations,
    :PRISM, :USBureauOfReclamationAgriMetStations, :USUResearchReport145 .

:DailyPenman-Monteith :hasDataSource :COAgriculturalMeteorologyNetworkStation, :CooperativeObserverNetwork%28COOP%29,
    :EmeryWaterConservancyDistrictStations, :FruitGrowersNetworkStations%28FGNET%29, :MesoWestStations,
    :NationalClimaticDataCenter%27sClimatographyOfTheUnitedStatesNo.81, :NationalOceanicAndAtmosphericAdministrationStations,
    :NationalWeatherServiceStations, :NaturalResourcesConservationServiceStations%28NRCS%29,
    :NewMexicoClimateCenterStations, :PRISM, :SoilClimateAnalysisNetwork%28SCAN%29, :USBureauOfReclamationAgriMetStations,
    :WeatherStations, :WesternRegionalClimateCenter%28WRCC%29Stations .

:ModifiedBlaney-Criddle :hasDataSource :COAgriculturalMeteorologyNetworkStation, :CommunityCollaborativeRain%2CHailAndSnowNetwork%28CoCoRaHS%29,
    :CooperativeObserverNetwork%28COOP%29, :EmeryWaterConservancyDistrictStations, :FruitGrowersNetworkStations%28FGNET%29,
    :MesoWestStations, :NationalClimaticDataCenter%27sClimatographyOfTheUnitedStatesNo.81,
    :NationalOceanicAndAtmosphericAdministrationStations, :NationalWeatherServiceStations,
    :NaturalResourcesConservationServiceStations%28NRCS%29, :NewMexicoClimateCenterStations,
    :PRISM, :RemoteAutomatedWeatherStations%28RAWS%29, :SCSTR21, :SnotelNetworkOfWeatherStations,
    :SoilClimateAnalysisNetwork%28SCAN%29, :USBureauOfReclamationAgriMetStations, :WeatherStations,
    :WesternRegionalClimateCenter%28WRCC%29Stations .

:SolarRadiation :hasDataSource :COAgriculturalMeteorologyNetworkStation, :CommunityCollaborativeRain%2CHailAndSnowNetwork%28CoCoRaHS%29,
    :CooperativeObserverNetwork%28COOP%29, :EmeryWaterConservancyDistrictStations, :FruitGrowersNetworkStations%28FGNET%29,
    :MesoWestStations, :NationalClimaticDataCenter%27sClimatographyOfTheUnitedStatesNo.81,
    :NationalOceanicAndAtmosphericAdministrationStations, :NationalWeatherServiceStations,
    :NaturalResourcesConservationServiceStations%28NRCS%29, :NewMexicoClimateCenterStations,
    :PRISM, :RemoteAutomatedWeatherStations%28RAWS%29, :SnotelNetworkOfWeatherStations,
    :SoilClimateAnalysisNetwork%28SCAN%29, :USBureauOfLandManagement%28BLM%29, :USBureauOfReclamationAgriMetStations,
    :USGeologicalSurvey%28USGS%29, :WYDepartmentOfEnvironmentalQuality%28DEQ%29, :WeatherStations,
    :WesternRegionalClimateCenter%28WRCC%29Stations, :WyomingStateEngineer%27sOfficeStations .

:Temperature :hasDataSource :COAgriculturalMeteorologyNetworkStation, :CommunityCollaborativeRain%2CHailAndSnowNetwork%28CoCoRaHS%29,
    :CooperativeObserverNetwork%28COOP%29, :EmeryWaterConservancyDistrictStations, :FruitGrowersNetworkStations%28FGNET%29,
    :MesoWestStations, :NationalClimaticDataCenter%27sClimatographyOfTheUnitedStatesNo.81,
    :NationalOceanicAndAtmosphericAdministrationStations, :RemoteAutomatedWeatherStations%28RAWS%29,
    :SnotelNetworkOfWeatherStations, :SoilClimateAnalysisNetwork%28SCAN%29, :USBureauOfLandManagement%28BLM%29,
    :USBureauOfReclamationAgriMetStations, :USGeologicalSurvey%28USGS%29, :WYDepartmentOfEnvironmentalQuality%28DEQ%29,
    :WyomingStateEngineer%27sOfficeStations .

:VaporPressure :hasDataSource :COAgriculturalMeteorologyNetworkStation, :CommunityCollaborativeRain%2CHailAndSnowNetwork%28CoCoRaHS%29,
    :CooperativeObserverNetwork%28COOP%29, :EmeryWaterConservancyDistrictStations, :FruitGrowersNetworkStations%28FGNET%29,
    :MesoWestStations, :NationalClimaticDataCenter%27sClimatographyOfTheUnitedStatesNo.81,
    :NationalOceanicAndAtmosphericAdministrationStations, :NationalWeatherServiceStations,
    :NaturalResourcesConservationServiceStations%28NRCS%29, :NewMexicoClimateCenterStations,
    :RemoteAutomatedWeatherStations%28RAWS%29, :SnotelNetworkOfWeatherStations, :SoilClimateAnalysisNetwork%28SCAN%29,
    :USBureauOfLandManagement%28BLM%29, :USBureauOfReclamationAgriMetStations, :USGeologicalSurvey%28USGS%29,
    :WYDepartmentOfEnvironmentalQuality%28DEQ%29, :WesternRegionalClimateCenter%28WRCC%29Stations,
    :WyomingStateEngineer%27sOfficeStations .

:WindRun :hasDataSource :COAgriculturalMeteorologyNetworkStation, :CommunityCollaborativeRain%2CHailAndSnowNetwork%28CoCoRaHS%29,
    :CooperativeObserverNetwork%28COOP%29, :EmeryWaterConservancyDistrictStations, :FruitGrowersNetworkStations%28FGNET%29,
    :MesoWestStations, :NationalClimaticDataCenter%27sClimatographyOfTheUnitedStatesNo.81,
    :NationalOceanicAndAtmosphericAdministrationStations, :NaturalResourcesConservationServiceStations%28NRCS%29,
    :NewMexicoClimateCenterStations, :PRISM, :RemoteAutomatedWeatherStations%28RAWS%29,
    :SnotelNetworkOfWeatherStations, :SoilClimateAnalysisNetwork%28SCAN%29, :USBureauOfLandManagement%28BLM%29,
    :USBureauOfReclamationAgriMetStations, :USGeologicalSurvey%28USGS%29, :WYDepartmentOfEnvironmentalQuality%28DEQ%29,
    :WeatherStations, :WesternRegionalClimateCenter%28WRCC%29Stations, :WyomingStateEngineer%27sOfficeStations .

:ClimateCoefficient%28kt%29 :hasDataSource :COAgriculturalMeteorologyNetworkStation,
    :NationalClimaticDataCenter%27sClimatographyOfTheUnitedStatesNo.81, :NationalOceanicAndAtmosphericAdministrationStations,
    :PRISM, :USBureauOfReclamationAgriMetStations .

:CropGrowthStateCoefficient%28Kc%29 :hasDataSource :FAO56Chapter6SingleCropCoefficients%28Kc%29,
    :SCSTR21, :USUResearchReport145 .

:MeanMonthlyAirTemperatures%28T%29 :hasDataSource :COAgriculturalMeteorologyNetworkStation,
    :CooperativeObserverNetwork%28COOP%29, :EmeryWaterConservancyDistrictStations, :FruitGrowersNetworkStations%28FGNET%29,
    :MesoWestStations, :NationalClimaticDataCenter%27sClimatographyOfTheUnitedStatesNo.81,
    :NationalOceanicAndAtmosphericAdministrationStations, :NationalWeatherServiceStations,
    :NaturalResourcesConservationServiceStations%28NRCS%29, :NewMexicoClimateCenterStations,
    :PRISM, :SoilClimateAnalysisNetwork%28SCAN%29, :USBureauOfLandManagement%28BLM%29,
    :USBureauOfReclamationAgriMetStations, :USGeologicalSurvey%28USGS%29, :WYDepartmentOfEnvironmentalQuality%28DEQ%29,
    :WeatherStations, :WesternRegionalClimateCenter%28WRCC%29Stations, :WyomingStateEngineer%27sOfficeStations .

:AnnualEmployeeHours :hasDataSource :MineSafetyAndHealthAdministration%28MSHA%29 .

:AnnualEvaporation :hasDataSource :MonthlyEvaporation .

:MonthlyEvaporation :hasDataSource :NationalOceanicAndAtmosphericAdministrationStations,
    :USBureauOfReclamationStations .

:AnnualSodaAshProduction :hasDataSource :USGeologicalSurvey%28USGS%29 .

:AreaOutflows :hasDataSource :USGSStreamGages, :UTDiversionRecordsFromRiverCommissioners,
    :UTMunicipalPotableAndSecondaryDiversionRecords, :UTOtherIrrigationCompanyRecords,
    :UTReservoirStorageAndReleaseRecords, :UTWaterRights .

:BasinOutflow-UT :hasDataSource :USGSStreamGages, :UTDiversionRecordsFromRiverCommissioners,
    :UTMunicipalPotableAndSecondaryDiversionRecords, :UTOtherIrrigationCompanyRecords,
    :UTReservoirStorageAndReleaseRecords, :UTWaterRights .

:GagedStreamOutflow-WY :hasDataSource :USGSStreamGages, :WyomingWaterResourcesDataSystem%28WRDS%29 .

:StreamOutfow-CA :hasDataSource :CADWRSGMADataViewer, :CAIntegratedWaterFlowModel%28IWFM%29,
    :CALSIM2, :CALSIM3, :Cal-SIMETAWUnitValues, :CaliforniaAgriculturalLandAndWaterUseEstimates,
    :CaliforniaCentralValleySimulation%28C2VSim%29, :CaliforniaDepartmentOfTransportation%27sHighwayDesignManual,
    :CaliforniaNevadaRiverForecastCenter, :CaliforniaWaterPlanPortfolio, :CenterForHydrometeorologyAndRemoteSensingDataPortal%28CHRS%29,
    :DWRWaterDataLibrary%3ASurfaceWaterAndGroundwaterData, :MODFLOW-OWHM%3AOneWaterHydrologicFlowModel,
    :USGSPublications, :USGSSurface-WaterDataForCalifornia .

:Exports-CO :hasDataSource :HistoricalDiversionsFile .

:AverageMonthlyReservoirGageHeight :hasDataSource :IrrigationDistricts, :NationalOceanicAndAtmosphericAdministrationStations,
    :NewMexicoInterstateStreamCommission%28NMISC%29, :USArmyCorpsOfEngineers, :USBureauOfReclamationStations,
    :USGSStreamGages .

:AverageUseRate :hasDataSource :MidwestPlanServiceStructuresAndEnvironmentalHandbook%2C1977 .

:Baseflow :hasDataSource :HistoricalData, :USGSStreamGages, :WesternMountLoftyRangesPrescribedWaterResourcesAreaWaterAllocationPlan .

:HistoricalData :hasDataSource :FederalArchives, :HistoricalDiversionsFile, :UTOtherIrrigationCompanyRecords,
    :UTStateArchives .

:BasinInflow-UT :hasDataSource :USGSStreamGages, :UTDiversionRecordsFromRiverCommissioners,
    :UTMunicipalPotableAndSecondaryDiversionRecords, :UTOtherIrrigationCompanyRecords,
    :UTReservoirStorageAndReleaseRecords, :UTWaterRights .

:RiverInflow-UT :hasDataSource :USGSStreamGages, :UTDiversionRecordsFromRiverCommissioners,
    :UTMunicipalPotableAndSecondaryDiversionRecords, :UTOtherIrrigationCompanyRecords,
    :UTReservoirStorageAndReleaseRecords, :UTWaterRights .

:GagedStreamInflow-WY :hasDataSource :USGSStreamGages, :WyomingWaterResourcesDataSystem%28WRDS%29 .

:GagedSurfaceWaterInflow-CO :hasDataSource :CODivisionOfWaterResourcesGages, :USGSStreamGages .

:UngagedSurfaceWaterInflow-CO :hasDataSource :CODivisionOfWaterResourcesGages, :USGSStreamGages .

:StreamInflow-CA :hasDataSource :CADWRSGMADataViewer, :CAIntegratedWaterFlowModel%28IWFM%29,
    :CALSIM2, :CALSIM3, :Cal-SIMETAWUnitValues, :CaliforniaAgriculturalLandAndWaterUseEstimates,
    :CaliforniaCentralValleySimulation%28C2VSim%29, :CaliforniaDepartmentOfTransportation%27sHighwayDesignManual,
    :CaliforniaNevadaRiverForecastCenter, :CaliforniaWaterPlanPortfolio, :CenterForHydrometeorologyAndRemoteSensingDataPortal%28CHRS%29,
    :DWRWaterDataLibrary%3ASurfaceWaterAndGroundwaterData, :MODFLOW-OWHM%3AOneWaterHydrologicFlowModel,
    :USGSPublications, :USGSSurface-WaterDataForCalifornia .

:COConsumptiveUseMethod :hasDataSource :COAgriculturalMeteorologyNetworkStation, :CODiversionRecords,
    :CODivisionOfWaterResourcesGages, :CommunityCollaborativeRain%2CHailAndSnowNetwork%28CoCoRaHS%29,
    :HydroBase, :NationalAgriculturalStatisticsService%28NASS%29CroplandDataLayer, :NationalOceanicAndAtmosphericAdministrationStations,
    :RemoteAutomatedWeatherStations%28RAWS%29, :SCSTR21, :SatelliteAndAerialPhotos, :SnotelNetworkOfWeatherStations,
    :USGSStreamGages, :WeatherStations .

:SCSTR21 :hasDataSource :COAgriculturalMeteorologyNetworkStation, :CommunityCollaborativeRain%2CHailAndSnowNetwork%28CoCoRaHS%29,
    :CooperativeObserverNetwork%28COOP%29, :NationalClimaticDataCenter%27sClimatographyOfTheUnitedStatesNo.81,
    :NationalOceanicAndAtmosphericAdministrationStations, :NationalWeatherServiceStations,
    :NaturalResourcesConservationServiceStations%28NRCS%29, :NewMexicoClimateCenterStations,
    :PRISM, :RemoteAutomatedWeatherStations%28RAWS%29, :SnotelNetworkOfWeatherStations,
    :USBureauOfLandManagement%28BLM%29, :USGeologicalSurvey%28USGS%29, :WYDepartmentOfEnvironmentalQuality%28DEQ%29,
    :WeatherStations, :WesternRegionalClimateCenter%28WRCC%29Stations, :WyomingStateEngineer%27sOfficeStations .

:COIrrigatedAcreageAssessment :hasDataSource :HydroBase, :NationalAgriculturalStatisticsService%28NASS%29CroplandDataLayer,
    :SatelliteAndAerialPhotos .

:CropIrrigationRequirementEstimationMethod :hasDataSource :COAgriculturalMeteorologyNetworkStation,
    :CommunityCollaborativeRain%2CHailAndSnowNetwork%28CoCoRaHS%29, :CooperativeObserverNetwork%28COOP%29,
    :EmeryWaterConservancyDistrictStations, :FruitGrowersNetworkStations%28FGNET%29, :MesoWestStations,
    :NationalClimaticDataCenter%27sClimatographyOfTheUnitedStatesNo.81, :NationalOceanicAndAtmosphericAdministrationStations,
    :NationalWeatherServiceStations, :NaturalResourcesConservationServiceStations%28NRCS%29,
    :NewMexicoClimateCenterStations, :RemoteAutomatedWeatherStations%28RAWS%29, :SCSTR21,
    :SnotelNetworkOfWeatherStations, :SoilClimateAnalysisNetwork%28SCAN%29, :USBureauOfLandManagement%28BLM%29,
    :USBureauOfReclamationAgriMetStations, :USGeologicalSurvey%28USGS%29, :WYDepartmentOfEnvironmentalQuality%28DEQ%29,
    :WeatherStations, :WesternRegionalClimateCenter%28WRCC%29Stations, :WyomingStateEngineer%27sOfficeStations .

:ModifiedBlaney-CriddleWithETElevationAdjustment :hasDataSource :COAgriculturalMeteorologyNetworkStation,
    :CommunityCollaborativeRain%2CHailAndSnowNetwork%28CoCoRaHS%29, :NationalOceanicAndAtmosphericAdministrationStations,
    :RemoteAutomatedWeatherStations%28RAWS%29, :SCSTR21, :SnotelNetworkOfWeatherStations .

:On-FarmWaterBalance :hasDataSource :COAgriculturalMeteorologyNetworkStation, :CODiversionRecords,
    :NationalOceanicAndAtmosphericAdministrationStations, :SCSTR21, :USGSStreamGages,
    :WeatherStations .

:OriginalBlaney-Criddle :hasDataSource :COAgriculturalMeteorologyNetworkStation, :NationalOceanicAndAtmosphericAdministrationStations,
    :SCSTR21 .

:OriginalBlaney-CriddleWithETElevationAdjustment :hasDataSource :COAgriculturalMeteorologyNetworkStation,
    :CommunityCollaborativeRain%2CHailAndSnowNetwork%28CoCoRaHS%29, :NationalOceanicAndAtmosphericAdministrationStations,
    :RemoteAutomatedWeatherStations%28RAWS%29, :SCSTR21, :SnotelNetworkOfWeatherStations .

:StateCU :hasDataSource :WYOfficeOfTheStateEngineer .

:CropIrrigationRequirement :hasDataSource :COAgriculturalMeteorologyNetworkStation,
    :CommunityCollaborativeRain%2CHailAndSnowNetwork%28CoCoRaHS%29, :CooperativeObserverNetwork%28COOP%29,
    :EmeryWaterConservancyDistrictStations, :FruitGrowersNetworkStations%28FGNET%29, :MesoWestStations,
    :NationalClimaticDataCenter%27sClimatographyOfTheUnitedStatesNo.81, :NationalOceanicAndAtmosphericAdministrationStations,
    :NationalWeatherServiceStations, :NaturalResourcesConservationServiceStations%28NRCS%29,
    :NewMexicoClimateCenterStations, :PRISM, :RemoteAutomatedWeatherStations%28RAWS%29,
    :SCSTR21, :SnotelNetworkOfWeatherStations, :SoilClimateAnalysisNetwork%28SCAN%29,
    :USBureauOfLandManagement%28BLM%29, :USBureauOfReclamationAgriMetStations, :USGeologicalSurvey%28USGS%29,
    :WYDepartmentOfEnvironmentalQuality%28DEQ%29, :WeatherStations, :WesternRegionalClimateCenter%28WRCC%29Stations,
    :WyomingStateEngineer%27sOfficeStations .

:CropType :hasDataSource :CropTypeStateAssessments, :FieldSurvey, :GroundSurvey, :NationalAgriculturalStatisticsService%28NASS%29CroplandDataLayer,
    :SatelliteAndAerialPhotos, :USDACroplandDataLayer%28CDL%29 .

:EffectivePrecipitation :hasDataSource :COAgriculturalMeteorologyNetworkStation, :CommunityCollaborativeRain%2CHailAndSnowNetwork%28CoCoRaHS%29,
    :CooperativeObserverNetwork%28COOP%29, :EmeryWaterConservancyDistrictStations, :FruitGrowersNetworkStations%28FGNET%29,
    :MesoWestStations, :NationalClimaticDataCenter%27sClimatographyOfTheUnitedStatesNo.81,
    :NationalOceanicAndAtmosphericAdministrationStations, :NationalWeatherServiceStations,
    :NaturalResourcesConservationServiceStations%28NRCS%29, :NewMexicoClimateCenterStations,
    :PRISM, :RemoteAutomatedWeatherStations%28RAWS%29, :SnotelNetworkOfWeatherStations,
    :SoilClimateAnalysisNetwork%28SCAN%29, :USBureauOfLandManagement%28BLM%29, :USBureauOfReclamationAgriMetStations,
    :USGeologicalSurvey%28USGS%29, :WYDepartmentOfEnvironmentalQuality%28DEQ%29, :WeatherStations,
    :WesternRegionalClimateCenter%28WRCC%29Stations, :WyomingStateEngineer%27sOfficeStations .

:IrrigatedAcreage :hasDataSource :CropTypeStateAssessments, :GroundSurvey, :HistoricalData,
    :HydroBase, :NationalAgriculturalStatisticsService%28NASS%29CroplandDataLayer, :SatelliteAndAerialPhotos,
    :Unknown .

:IrrigationMethod :hasDataSource :HydroBase, :Unknown .

:PotentialConsumptiveUse :hasDataSource :COAgriculturalMeteorologyNetworkStation,
    :CommunityCollaborativeRain%2CHailAndSnowNetwork%28CoCoRaHS%29, :CooperativeObserverNetwork%28COOP%29,
    :NationalClimaticDataCenter%27sClimatographyOfTheUnitedStatesNo.81, :NationalOceanicAndAtmosphericAdministrationStations,
    :NationalWeatherServiceStations, :NaturalResourcesConservationServiceStations%28NRCS%29,
    :NewMexicoClimateCenterStations, :PRISM, :RemoteAutomatedWeatherStations%28RAWS%29,
    :SnotelNetworkOfWeatherStations, :USBureauOfLandManagement%28BLM%29, :USGeologicalSurvey%28USGS%29,
    :WYDepartmentOfEnvironmentalQuality%28DEQ%29, :WeatherStations, :WesternRegionalClimateCenter%28WRCC%29Stations,
    :WyomingStateEngineer%27sOfficeStations .

:Precipitation :hasDataSource :COAgriculturalMeteorologyNetworkStation, :CommunityCollaborativeRain%2CHailAndSnowNetwork%28CoCoRaHS%29,
    :CooperativeObserverNetwork%28COOP%29, :EmeryWaterConservancyDistrictStations, :FruitGrowersNetworkStations%28FGNET%29,
    :MesoWestStations, :NationalOceanicAndAtmosphericAdministrationStations, :NationalWeatherServiceStations,
    :NaturalResourcesConservationServiceStations%28NRCS%29, :NewMexicoClimateCenterStations,
    :PRISM, :RemoteAutomatedWeatherStations%28RAWS%29, :SnotelNetworkOfWeatherStations,
    :SoilClimateAnalysisNetwork%28SCAN%29, :USBureauOfLandManagement%28BLM%29, :USBureauOfReclamationAgriMetStations,
    :USGeologicalSurvey%28USGS%29, :WYDepartmentOfEnvironmentalQuality%28DEQ%29, :WeatherStations,
    :WesternRegionalClimateCenter%28WRCC%29Stations, :WyomingStateEngineer%27sOfficeStations,
    :WyomingWaterResourcesDataSystemsWaterAndClimateMapServer .

:SupplySource :hasDataSource :HydroBase, :Unknown .

:SupplyType :hasDataSource :HydroBase, :Unknown .

:WaterSupply :hasDataSource :CODiversionRecords, :CODivisionOfWaterResourcesGages,
    :NMDiversionRecords, :StateData, :USGSStreamGages, :UTDiversionRecordsFromRiverCommissioners,
    :WYDiversionRecords, :WyomingWaterResourcesDataSystem%28WRDS%29 .

:COLivestockMethod :hasDataSource :StateAgriculturalStatistics .

:LivestockCount :hasDataSource :StateAgriculturalStatistics .

:Population :hasDataSource :CaliforniaDepartmentOfFinance, :ColoradoCensusBureau,
    :USCensusBureau .

:CONativeVegetationMethod :hasDataSource :HistoricalDiversionsFile, :Unknown .

:Diversions :hasDataSource :ColoradoWaterConservationBoard%28CWCB%29, :HistoricalDiversionsFile,
    :WYDiversionDataFromWaterUsers, :WYOfficeOfTheStateEngineer .

:NativeVegetationCoefficient :hasDataSource :Unknown .

:ChangeInGroundwaterStorage-CA :hasDataSource :CADWRBulletin118%3AGroundwaterReport,
    :CADWRSGMADataViewer, :CAIntegratedWaterFlowModel%28IWFM%29, :CALSIM2, :CaliforniaAgriculturalLandAndWaterUseEstimates,
    :CaliforniaCentralValleySimulation%28C2VSim%29, :CaliforniaDataExchangeCenter%28CDEC%29,
    :CaliforniaWaterPlanPortfolio, :DWRWaterDataLibrary%3ASurfaceWaterAndGroundwaterData,
    :GravityRecoveryAndClimateExperiment%28GRACE%29, :MODFLOW-OWHM%3AOneWaterHydrologicFlowModel .

:ChangeInGroundwaterStorage-AUS :hasDataSource :AUSBureauOfMeteorology .

:ChangeInSurfaceWaterStorage-AUS :hasDataSource :AWRA-LModel, :AWRA-RModel, :HYDRODatabase .

:ChangeInSurfaceWaterStorage-CA :hasDataSource :CAIntegratedWaterFlowModel%28IWFM%29,
    :CenterForHydrometeorologyAndRemoteSensingDataPortal%28CHRS%29, :MODFLOW-OWHM%3AOneWaterHydrologicFlowModel,
    :USBRCentralValleyProjectRefugeWaterDeliveryData, :USGSSurface-WaterDataForCalifornia .

:ChangeInSurfaceWaterStorage-CO :hasDataSource :CODivisionOfWaterResources, :USBureauOfReclamationStations .

:ClassAPanEvaporationData :hasDataSource :NationalOceanicAndAtmosphericAdministrationStations,
    :WeatherStations .

:CoalProductionQuantities :hasDataSource :MineSafetyAndHealthAdministration%28MSHA%29 .

:ColoradoStateMod :hasDataSource :COAgriculturalMeteorologyNetworkStation, :CODivisionOfWaterResources,
    :CODivisionOfWaterResourcesGages, :ColoradoWaterConservationBoard%28CWCB%29, :NationalOceanicAndAtmosphericAdministrationStations,
    :USBureauOfReclamationStations, :USGSStreamGages .

:DirectFlowDemand-Annual :hasDataSource :CODivisionOfWaterResources .

:DirectFlowDemand-Monthly :hasDataSource :CODivisionOfWaterResources .

:Evaporation :hasDataSource :COAgriculturalMeteorologyNetworkStation, :NationalOceanicAndAtmosphericAdministrationStations,
    :PRISM, :USUResearchReport145 .

:InstreamFlowDemand-Annual :hasDataSource :CODivisionOfWaterResources, :ColoradoWaterConservationBoard%28CWCB%29 .

:InstreamFlowDemand-Monthly :hasDataSource :CODivisionOfWaterResources, :ColoradoWaterConservationBoard%28CWCB%29 .

:ReservoirTargets :hasDataSource :CODivisionOfWaterResources, :USBureauOfReclamationStations .

:Streamflow :hasDataSource :CODivisionOfWaterResourcesGages, :USGSStreamGages .

:MunicipalAndIndustrialDiversions-UT :hasDataSource :USGSStreamGages, :UTMunicipalPotableAndSecondaryDiversionRecords,
    :UTOtherIrrigationCompanyRecords, :UTReservoirStorageAndReleaseRecords, :UTWaterRights .

:ConveyanceEvaporation-CA :hasDataSource :CACountyAgriculturalCommissionerCropReports,
    :CADWRBulletin132%3AManagementOfTheCaliforniaStateWaterProject, :CAIntegratedWaterFlowModel%28IWFM%29,
    :CALSIM2, :Cal-SIMETAWUnitValues, :CaliforniaAgriculturalLandAndWaterUseEstimates,
    :CaliforniaCentralValleySimulation%28C2VSim%29, :CaliforniaIrrigationManagementInformationSystem%28CIMIS%29,
    :CaliforniaStateGroundwaterElevationMonitoring%28CASGEM%29, :CaliforniaWaterPlanPortfolio,
    :DWRBulletin73%3AEvaporationFromWaterSurfaceInCalifornia%281979%29, :MODFLOW-OWHM%3AOneWaterHydrologicFlowModel,
    :NOAANationalCentersForEnvironmentalInformation-ClimateDataOnline, :NOAANationalCentersForEnvironmentalInformation-ClimatologicalDataPublications,
    :NWSCLIMATEPREDICTIONCENTEREVAPORATION, :USBRCentralValleyProjectRefugeWaterDeliveryData .

:ConveyanceLossesForAllocatedDiversions-AUS :hasDataSource :s.71WaterResourceReport .

:SurfaceWaterOutflows-AUS :hasDataSource :AWRA-LModel, :AWRA-RModel .

:ConveyanceSeepage-CA :hasDataSource :CADWRBulletin132%3AManagementOfTheCaliforniaStateWaterProject,
    :CAIntegratedWaterFlowModel%28IWFM%29, :CALSIM2, :CAValidatedWaterLossReporting, :Cal-SIMETAWUnitValues,
    :CaliforniaAgriculturalLandAndWaterUseEstimates, :CaliforniaCentralValleySimulation%28C2VSim%29,
    :CaliforniaWaterPlanPortfolio, :MODFLOW-OWHM%3AOneWaterHydrologicFlowModel, :USBRCentralValleyProjectRefugeWaterDeliveryData .

:CoplandPrecipitation-UT :hasDataSource :PRISM, :USBureauOfReclamationAgriMetStations .

:Precipitation-CA :hasDataSource :CAAgriculturalWaterManagementPlans, :CADWRSGMADataViewer,
    :CAIntegratedWaterFlowModel%28IWFM%29, :CAPreviousReports, :Cal-SIMETAWUnitValues,
    :CaliforniaAgriculturalLandAndWaterUseEstimates, :CaliforniaCentralValleySimulation%28C2VSim%29,
    :CaliforniaDataExchangeCenter%28CDEC%29, :CaliforniaIrrigationManagementInformationSystem%28CIMIS%29,
    :CaliforniaNevadaRiverForecastCenter, :CaliforniaStateGroundwaterElevationMonitoring%28CASGEM%29,
    :CaliforniaWaterPlanPortfolio, :CentralValleySpatialDatabase-partOfTheCentralValleyHydrologicModel%5BCVHM%5DProject,
    :MODFLOW-OWHM%3AOneWaterHydrologicFlowModel, :NOAANationalCentersForEnvironmentalInformation-ClimateDataOnline,
    :NOAANationalCentersForEnvironmentalInformation-ClimatologicalDataPublications, :NationalOceanicAndAtmosphericAdministrationStations,
    :PRISM, :SpatialCaliforniaIrrigationManagementInformationSystem%28CIMIS%29, :USGSBasinCharacterizationModel .

:Precipitation-CO :hasDataSource :COAgriculturalMeteorologyNetworkStation, :NationalOceanicAndAtmosphericAdministrationStations .

:Precipitation-UT :hasDataSource :PRISM, :USBureauOfReclamationAgriMetStations .

:Precipitation-WY :hasDataSource :NationalClimaticDataCenter%27sClimatographyOfTheUnitedStatesNo.81 .

:DailyASCEStandardizedPenman-Monteith :hasDataSource :COAgriculturalMeteorologyNetworkStation,
    :NationalOceanicAndAtmosphericAdministrationStations .

:DailyEffectivePrecipitation :hasDataSource :COAgriculturalMeteorologyNetworkStation,
    :NationalOceanicAndAtmosphericAdministrationStations .

:DailyModifiedHargreaves :hasDataSource :COAgriculturalMeteorologyNetworkStation,
    :CommunityCollaborativeRain%2CHailAndSnowNetwork%28CoCoRaHS%29, :NationalOceanicAndAtmosphericAdministrationStations,
    :RemoteAutomatedWeatherStations%28RAWS%29, :SnotelNetworkOfWeatherStations .

:DaytimeHours :hasDataSource :COAgriculturalMeteorologyNetworkStation, :NationalOceanicAndAtmosphericAdministrationStations .

:DirectCommunication :hasDataSource :WyomingWaterDevelopmentCommission%28WWDC%292002WaterSystemSurveyReport .

:DomesticTotalUse-WY :hasDataSource :USCensusBureau .

:WithdrawalMethod :hasDataSource :BrownAndCaldwell%2C1984, :NMOfficeOfTheStateEngineer%28NMOSE%29,
    :NewMexicoDepartmentOfAgriculture, :NewMexicoEnvironmentDepartment%28NMED%29, :USCensusBureau,
    :UniversityOfNewMexicoGeospatialAndPopulationStudies%28UNMGPS%29 .

:GallonsPerCapitaPerDay%28GPCD%29 :hasDataSource :BrownAndCaldwell%2C1984, :MunicipalWaterUseRecords,
    :NMOSETechnicalReportNo.48, :NMOfficeOfTheStateEngineer%28NMOSE%29 .

:DownstreamFlow :hasDataSource :USGSStreamGages, :WyomingWaterResourcesDataSystem%28WRDS%29 .

:UTEffectivePrecipitationMethod :hasDataSource :EmeryWaterConservancyDistrictStations,
    :FruitGrowersNetworkStations%28FGNET%29, :MesoWestStations, :NationalOceanicAndAtmosphericAdministrationStations,
    :NationalWeatherServiceStations, :PRISM, :SoilClimateAnalysisNetwork%28SCAN%29, :USBureauOfReclamationAgriMetStations .

:EffectivePrecipitationFactor :hasDataSource :SCSTR21 .

:ElectricalGenerationData :hasDataSource :USEnergyInformationAdministration%28USEIA%29 .

:Elevation-Area-CapacityTables :hasDataSource :USBureauOfReclamation, :UTStateEngineerData,
    :WaterResourcesStudies .

:MonthlyPrecipitationVolume :hasDataSource :PRISM, :WeatherStations .

:Rainfall :hasDataSource :NationalOceanicAndAtmosphericAdministrationStations, :PRISM,
    :USUResearchReport145 .

:ReservoirSurfaceArea :hasDataSource :IrrigationDistricts, :NationalOceanicAndAtmosphericAdministrationStations,
    :NewMexicoInterstateStreamCommission%28NMISC%29, :USArmyCorpsOfEngineers, :USBureauOfReclamationStations,
    :USGSStreamGages .

:Evaporation-AUS :hasDataSource :AUSBureauOfMeteorology, :AWRA-RModel .

:EvaporationFromReservoirs-NMOSE :hasDataSource :IrrigationDistricts, :NationalOceanicAndAtmosphericAdministrationStations,
    :NewMexicoInterstateStreamCommission%28NMISC%29, :USArmyCorpsOfEngineers, :USBureauOfReclamationStations,
    :USGSStreamGages .

:PanApproach :hasDataSource :IrrigationDistricts, :NationalOceanicAndAtmosphericAdministrationStations,
    :NewMexicoInterstateStreamCommission%28NMISC%29, :USArmyCorpsOfEngineers, :USBureauOfReclamationStations,
    :USGSStreamGages .

:MonthlyGrossEvaporationRate :hasDataSource :USBureauOfReclamationStations .

:WinterIceSurfaceArea :hasDataSource :HistoricalData .

:LakeEvaporation-CA :hasDataSource :CACountyAgriculturalCommissionerCropReports, :CAIntegratedWaterFlowModel%28IWFM%29,
    :CALSIM2, :CaliforniaWaterPlanPortfolio, :MODFLOW-OWHM%3AOneWaterHydrologicFlowModel,
    :NOAANationalCentersForEnvironmentalInformation-ClimateDataOnline, :NOAANationalCentersForEnvironmentalInformation-ClimatologicalDataPublications,
    :NWSCLIMATEPREDICTIONCENTEREVAPORATION, :SpatialCaliforniaIrrigationManagementInformationSystem%28CIMIS%29 .

:ReservoirEvaporation-CO :hasDataSource :COGISExercise, :NOAATechnicalReportNWS33,
    :NationalOceanicAndAtmosphericAdministrationStations .

:ReservoirEvaporation-UT :hasDataSource :FederalArchives, :PRISM, :USBureauOfReclamation,
    :USUResearchReport145, :UTOtherIrrigationCompanyRecords, :UTStateArchives, :UTStateEngineerData,
    :WaterResourcesStudies .

:GroundwaterExport-CA :hasDataSource :CAIntegratedWaterFlowModel%28IWFM%29, :CALSIM2,
    :Cal-SIMETAWUnitValues, :CaliforniaAgriculturalLandAndWaterUseEstimates, :CaliforniaCentralValleySimulation%28C2VSim%29,
    :CaliforniaWaterPlanPortfolio, :MODFLOW-OWHM%3AOneWaterHydrologicFlowModel .

:StoredWaterExport-CA :hasDataSource :CAIntegratedWaterFlowModel%28IWFM%29, :CALSIM2,
    :MODFLOW-OWHM%3AOneWaterHydrologicFlowModel .

:SurfaceWaterExports-CA :hasDataSource :CADWRBulletin132%3AManagementOfTheCaliforniaStateWaterProject,
    :CAIntegratedWaterFlowModel%28IWFM%29, :CALSIM2, :CALSIM3, :Cal-SIMETAWUnitValues,
    :CaliforniaAgriculturalLandAndWaterUseEstimates, :CaliforniaCentralValleySimulation%28C2VSim%29,
    :CaliforniaWaterPlanPortfolio, :ExistingWaterRightInformationFromStateWaterResourcesControlBoard%28SWRCB%29,
    :MODFLOW-OWHM%3AOneWaterHydrologicFlowModel, :USBRCentralValleyProjectRefugeWaterDeliveryData,
    :USGSSurface-WaterDataForCalifornia .

:FloodReturn-AUS :hasDataSource :AWRA-RModel .

:SurfaceWaterInflows-AUS :hasDataSource :AWRA-LModel, :AWRA-RModel .

:GageHeight :hasDataSource :CODivisionOfWaterResourcesGages, :USGSStreamGages .

:GagedSurfaceWaterOutflow-CO :hasDataSource :CODivisionOfWaterResourcesGages, :USGSStreamGages .

:GrossActivelyIrrigatedAcreage :hasDataSource :ConservancyDistricts, :NMOfficeOfTheStateEngineer%28NMOSE%29,
    :NationalAgriculturalStatisticsService, :NewMexicoInterstateStreamCommission%28NMISC%29,
    :USBureauOfReclamation, :USDACroplandDataLayer%28CDL%29, :USDAFarmServiceAgency .

:GrossMonthlyFreeWaterSurfaceEvaporation :hasDataSource :NOAATechnicalReportNWS33 .

:SubsurfaceInflow-CA :hasDataSource :CADWRBulletin118%3AGroundwaterReport, :CAIntegratedWaterFlowModel%28IWFM%29,
    :CaliforniaAgriculturalLandAndWaterUseEstimates, :CaliforniaCentralValleySimulation%28C2VSim%29,
    :CaliforniaDataExchangeCenter%28CDEC%29, :DWRWaterDataLibrary%3ASurfaceWaterAndGroundwaterData,
    :MODFLOW-OWHM%3AOneWaterHydrologicFlowModel, :USGSPublications .

:SubsurfaceOutflow-CA :hasDataSource :CADWRBulletin118%3AGroundwaterReport, :CAIntegratedWaterFlowModel%28IWFM%29,
    :CaliforniaAgriculturalLandAndWaterUseEstimates, :CaliforniaCentralValleySimulation%28C2VSim%29,
    :CaliforniaDataExchangeCenter%28CDEC%29, :DWRWaterDataLibrary%3ASurfaceWaterAndGroundwaterData,
    :MODFLOW-OWHM%3AOneWaterHydrologicFlowModel, :USGSPublications .

:GroundwaterDischarge-AUS :hasDataSource :DepartmentOfWaterAndEnvironmentalRegulation .

:Discharge%3AGroundwater-AUS :hasDataSource :AUSDepartmentOfEnvironment%2CLand%2CWaterAndPlanning .

:LakeGainFromGroundwater-CA :hasDataSource :CAIntegratedWaterFlowModel%28IWFM%29,
    :MODFLOW-OWHM%3AOneWaterHydrologicFlowModel .

:GroundwaterUse :hasDataSource :MunicipalAndIndustrialDiversionReports, :USGSEstimatesOfBasinGroundwaterFlows,
    :USGSGroundwaterReports, :UTWaterRights .

:GroundwaterUse-UT :hasDataSource :MunicipalAndIndustrialDiversionReports, :USGSEstimatesOfBasinGroundwaterFlows,
    :USGSGroundwaterReports, :UTWaterRights .

:ImportedWater-CA :hasDataSource :CADWRBulletin132%3AManagementOfTheCaliforniaStateWaterProject,
    :CAIntegratedWaterFlowModel%28IWFM%29, :CALSIM2, :CALSIM3, :Cal-SIMETAWUnitValues,
    :CaliforniaCentralValleySimulation%28C2VSim%29, :CaliforniaWaterPlanPortfolio, :ExistingWaterRightInformationFromStateWaterResourcesControlBoard%28SWRCB%29,
    :MODFLOW-OWHM%3AOneWaterHydrologicFlowModel, :USBRCentralValleyProjectRefugeWaterDeliveryData,
    :USGSSurface-WaterDataForCalifornia, :WaterUseEstimate .

:Imports-CO :hasDataSource :HistoricalDiversionsFile .

:IndicatorGageApproach :hasDataSource :USGSStreamGages .

:Industrial-NMOSE :hasDataSource :NMOfficeOfTheStateEngineer%28NMOSE%29 .

:Metered :hasDataSource :NMOfficeOfTheStateEngineer%28NMOSE%29 .

:IndustrialConsumptiveUse-WY :hasDataSource :MineSafetyAndHealthAdministration%28MSHA%29,
    :USCensusBureau, :USEnergyInformationAdministration%28USEIA%29, :USGeologicalSurvey%28USGS%29,
    :WyomingOilAndGasConservationCommission%28WYOGCC%29 .

:IndustrialTotalUse-WY :hasDataSource :MineSafetyAndHealthAdministration%28MSHA%29,
    :USCensusBureau, :USEnergyInformationAdministration%28USEIA%29, :USGeologicalSurvey%28USGS%29,
    :WyomingOilAndGasConservationCommission%28WYOGCC%29 .

:MonthlyCoalbedMethaneGasProductionAndProducedWater :hasDataSource :WyomingOilAndGasConservationCommission%28WYOGCC%29 .

:NaturalGasProcessingVolumes :hasDataSource :WyomingOilAndGasConservationCommission%28WYOGCC%29 .

:MonthlyOil%2CGas%2CAndProducedWater :hasDataSource :WyomingOilAndGasConservationCommission%28WYOGCC%29 .

:SurfaceWaterDelivery-CA :hasDataSource :CADWRBulletin132%3AManagementOfTheCaliforniaStateWaterProject,
    :CAIntegratedWaterFlowModel%28IWFM%29, :CALSIM2, :CAUrbanWaterManagementPlans, :Cal-SIMETAWUnitValues,
    :CaliforniaAgriculturalLandAndWaterUseEstimates, :CaliforniaCentralValleySimulation%28C2VSim%29,
    :CaliforniaWaterPlanPortfolio, :DWRLandUseSurveys, :LocalAgencyRecords, :MODFLOW-OWHM%3AOneWaterHydrologicFlowModel,
    :SWRCBWaterConservationPortal, :USBRCentralValleyProjectRefugeWaterDeliveryData .

:Inter-regionCoastalInflow-AUS :hasDataSource :AUSDepartmentOfEnvironment%2CLand%2CWaterAndPlanning,
    :DepartmentOfWaterAndEnvironmentalRegulation, :PortPhillipCatchmentManagementAuthority .

:Inter-regionCoastalOutflow-AUS :hasDataSource :AUSDepartmentOfEnvironment%2CLand%2CWaterAndPlanning,
    :DepartmentOfWaterAndEnvironmentalRegulation, :PortPhillipCatchmentManagementAuthority .

:InterpolationFromOtherRecords :hasDataSource :NMOfficeOfTheStateEngineer%28NMOSE%29 .

:NMIrrigatedAcreageAssessment :hasDataSource :FieldSurvey, :NMOfficeOfTheStateEngineer%28NMOSE%29,
    :NationalAgriculturalStatisticsService, :NewMexicoInterstateStreamCommission%28NMISC%29,
    :USBureauOfReclamation, :USDACroplandDataLayer%28CDL%29 .

:USBRIrrigatedAcreageAssessment :hasDataSource :CropTypeStateAssessments, :NationalAgriculturalStatisticsService%28NASS%29CroplandDataLayer,
    :SatelliteAndAerialPhotos .

:UTIrrigatedAcreageAssessment :hasDataSource :GroundSurvey, :SatelliteAndAerialPhotos,
    :Unknown .

:WYIrrigatedAcreageAssessment :hasDataSource :HistoricalData, :SatelliteAndAerialPhotos .

:SupplyStructure :hasDataSource :Unknown .

:NMConsumptiveUseMethod :hasDataSource :FieldSurvey, :NMDiversionRecords, :NMOfficeOfTheStateEngineer%28NMOSE%29,
    :NationalAgriculturalStatisticsService, :NationalOceanicAndAtmosphericAdministrationStations,
    :NationalWeatherServiceStations, :NaturalResourcesConservationServiceStations%28NRCS%29,
    :NewMexicoClimateCenterStations, :NewMexicoInterstateStreamCommission%28NMISC%29,
    :PRISM, :USBureauOfReclamation, :USDACroplandDataLayer%28CDL%29, :USGSStreamGages,
    :WeatherStations, :WesternRegionalClimateCenter%28WRCC%29Stations .

:IrrigatedAgricultureDiversions-NMOSE :hasDataSource :ConservancyDistricts, :IrrigationDistricts,
    :NMOSECropAcreageFile, :NMOSEGrowingSeasonFile, :NMOSETemperatureAndPrecipitationFile,
    :NMOfficeOfTheStateEngineer%28NMOSE%29, :NationalAgriculturalStatisticsService, :NewMexicoInterstateStreamCommission%28NMISC%29,
    :PRISM, :USBureauOfReclamation, :USDACroplandDataLayer%28CDL%29, :USDAFarmServiceAgency,
    :WeatherStations .

:ConsumptiveIrrigationRequirement%28CIR%29 :hasDataSource :NMOSECropAcreageFile, :NMOSEGrowingSeasonFile,
    :NMOSETemperatureAndPrecipitationFile, :NMOfficeOfTheStateEngineer%28NMOSE%29 .

:LakeLossToGroundwater-CA :hasDataSource :CAIntegratedWaterFlowModel%28IWFM%29, :MODFLOW-OWHM%3AOneWaterHydrologicFlowModel .

:LivestockPopulation :hasDataSource :NewMexicoDepartmentOfAgriculture .

:ManagedAquiferRecharge-AUS :hasDataSource :AUSDepartmentOfEnvironmentAndNaturalResources,
    :DepartmentOfWaterAndEnvironmentalRegulation .

:ManagedAquiferRecharge-CA :hasDataSource :CAIntegratedWaterFlowModel%28IWFM%29, :CALSIM2,
    :Cal-SIMETAWUnitValues, :CaliforniaAgriculturalLandAndWaterUseEstimates, :CaliforniaCentralValleySimulation%28C2VSim%29,
    :CaliforniaWaterPlanPortfolio, :MODFLOW-OWHM%3AOneWaterHydrologicFlowModel .

:Industrial%3AMineProduction-WY :hasDataSource :MineSafetyAndHealthAdministration%28MSHA%29 .

:SumOfMonthlyConsumptiveUseFactorsForGrowingSeason%28F%29 :hasDataSource :COAgriculturalMeteorologyNetworkStation,
    :NationalOceanicAndAtmosphericAdministrationStations .

:MonthlyEffectivePrecipitation :hasDataSource :COAgriculturalMeteorologyNetworkStation,
    :NationalOceanicAndAtmosphericAdministrationStations .

:ReturnFlow-CA :hasDataSource :CAIntegratedWaterFlowModel%28IWFM%29, :CAIntegratedWaterFlowModel%28IWFM%29DemandCalculator,
    :CALSIM2, :Cal-SIMETAWUnitValues, :CaliforniaAgriculturalLandAndWaterUseEstimates,
    :CaliforniaCentralValleySimulation%28C2VSim%29, :CaliforniaWaterPlanPortfolio, :IrrigationMethod,
    :MODFLOW-OWHM%3AOneWaterHydrologicFlowModel, :USDANaturalResourcesConservationServiceGeospatialWebSoilSurvey,
    :USGSPublications, :USGSSurface-WaterDataForCalifornia .

:OriginalHargreaves :hasDataSource :COAgriculturalMeteorologyNetworkStation, :CommunityCollaborativeRain%2CHailAndSnowNetwork%28CoCoRaHS%29,
    :NationalOceanicAndAtmosphericAdministrationStations, :NationalWeatherServiceStations,
    :NaturalResourcesConservationServiceStations%28NRCS%29, :NewMexicoClimateCenterStations,
    :RemoteAutomatedWeatherStations%28RAWS%29, :SnotelNetworkOfWeatherStations, :WesternRegionalClimateCenter%28WRCC%29Stations .

:NMIrrigationWithdrawals :hasDataSource :ConservancyDistricts, :IrrigationDistricts,
    :NMOSEWaterRightsDatabase, :NMOfficeOfTheStateEngineer%28NMOSE%29, :NationalAgriculturalStatisticsService,
    :NewMexicoInterstateStreamCommission%28NMISC%29, :PRISM, :USBureauOfReclamation, :USDACroplandDataLayer%28CDL%29,
    :USDAFarmServiceAgency, :WeatherStations .

:NativeVegetationConsumptiveUse-CO :hasDataSource :HistoricalDiversionsFile, :Unknown .

:NaturalFlowGainDistribution :hasDataSource :CODivisionOfWaterResourcesGages, :USGSStreamGages .

:ProrationFactors :hasDataSource :Unknown .

:OtherIncreases-AUS :hasDataSource :AUSBureauOfMeteorology, :s.71WaterResourceReport .

:Outflow-AUS :hasDataSource :StreamGages .

:OverbankFloodSpilling-AUS :hasDataSource :AWRA-RModel .

:OverbankFlow-AUS :hasDataSource :AWRA-RModel .

:PersonalOutreach :hasDataSource :FacilityDirectorOrOperator .

:WaterUseEstimate :hasDataSource :FacilityDirectorOrOperator .

:PopulationServedByPublicWaterSupply :hasDataSource :GPSPopulationData, :MilitaryBasePopulationData,
    :NewMexicoEnvironmentDepartment%28NMED%29, :USCensusBureau, :UniversityOfNewMexicoGeospatialAndPopulationStudies%28UNMGPS%29 .

:Industrial%3AElectricalGeneration-WY :hasDataSource :USEnergyInformationAdministration%28USEIA%29 .

:Precipitation-AUS :hasDataSource :AUSBureauOfMeteorology, :AWRA-RModel .

:RechargeOfAppliedWater-CA :hasDataSource :CAAgriculturalWaterManagementPlans, :CADWRIrrigationMethodsSurvey,
    :CAIntegratedWaterFlowModel%28IWFM%29, :CAIntegratedWaterFlowModel%28IWFM%29DemandCalculator,
    :CALSIM2, :CAValidatedWaterLossReporting, :Cal-SIMETAWUnitValues, :CaliforniaAgriculturalLandAndWaterUseEstimates,
    :CaliforniaCentralValleySimulation%28C2VSim%29, :CaliforniaWaterPlanPortfolio, :MODFLOW-OWHM%3AOneWaterHydrologicFlowModel,
    :NOAANationalCentersForEnvironmentalInformation-ClimateDataOnline, :NOAANationalCentersForEnvironmentalInformation-ClimatologicalDataPublications,
    :USDANaturalResourcesConservationServiceGeospatialWebSoilSurvey, :USGSBasinCharacterizationModel .

:RecycledWaterExport-CA :hasDataSource :CAAgriculturalWaterManagementPlans, :CALSIM2,
    :CAUrbanWaterManagementPlans, :Cal-SIMETAWUnitValues, :CaliforniaWaterPlanPortfolio,
    :WaterRecyclingSurvey%282015%29 .

:ReservoirEstimationMethod :hasDataSource :COGISExercise, :NOAATechnicalReportNWS33,
    :NationalOceanicAndAtmosphericAdministrationStations .

:SurfaceAreaOfReservoir :hasDataSource :COGISExercise .

:ReservoirEvaporation-WY :hasDataSource :HighPlainsClimateCenter-UniversityOfNebraska,
    :WyomingWaterResourcesDataSystemsWaterAndClimateMapServer .

:PanMethod%28NetEvaporation%29 :hasDataSource :HighPlainsClimateCenter-UniversityOfNebraska,
    :WyomingWaterResourcesDataSystemsWaterAndClimateMapServer .

:GrossPanEvaportation%28inches%29 :hasDataSource :HighPlainsClimateCenter-UniversityOfNebraska .

:RiverAndFloodplainLosses-AUS :hasDataSource :AWRA-LModel, :AWRA-RModel .

:Runoff-AUS :hasDataSource :AWRA-LModel, :AWRA-RModel .

:Runoff-CA :hasDataSource :CAIntegratedWaterFlowModel%28IWFM%29, :CAIntegratedWaterFlowModel%28IWFM%29DemandCalculator,
    :Cal-SIMETAWUnitValues, :CaliforniaAgriculturalLandAndWaterUseEstimates, :CaliforniaCentralValleySimulation%28C2VSim%29,
    :CaliforniaDepartmentOfTransportation%27sHighwayDesignManual, :MODFLOW-OWHM%3AOneWaterHydrologicFlowModel,
    :USGSBasinCharacterizationModel, :USGSPublications, :USGSSurface-WaterDataForCalifornia .

:Self-SuppliedDomestic-NMOSE :hasDataSource :GPSPopulationData, :MilitaryBasePopulationData,
    :NMOSETechnicalReportNo.48, :NewMexicoEnvironmentDepartment%28NMED%29, :PopulationServedByPublicWaterSupply,
    :USCensusBureau, :UniversityOfNewMexicoGeospatialAndPopulationStudies%28UNMGPS%29 .

:SelfSuppliedDomesticPopulation :hasDataSource :GPSPopulationData, :MilitaryBasePopulationData,
    :NewMexicoEnvironmentDepartment%28NMED%29, :PopulationServedByPublicWaterSupply, :USCensusBureau,
    :UniversityOfNewMexicoGeospatialAndPopulationStudies%28UNMGPS%29 .

:SoilMoistureHoldingCapacity :hasDataSource :STATSGOSoilsData, :WaterResourcesIrrigatedLandUseDatabase .

:StoredWaterExtraction-CA :hasDataSource :CAIntegratedWaterFlowModel%28IWFM%29, :CALSIM2,
    :Cal-SIMETAWUnitValues, :CaliforniaAgriculturalLandAndWaterUseEstimates, :CaliforniaCentralValleySimulation%28C2VSim%29,
    :CaliforniaWaterPlanPortfolio, :MODFLOW-OWHM%3AOneWaterHydrologicFlowModel .

:StreamEvaporation-CA :hasDataSource :CACountyAgriculturalCommissionerCropReports,
    :Cal-SIMETAWUnitValues, :CaliforniaStateGroundwaterElevationMonitoring%28CASGEM%29,
    :CaliforniaWaterPlanPortfolio, :DWRBulletin73%3AEvaporationFromWaterSurfaceInCalifornia%281979%29,
    :NOAANationalCentersForEnvironmentalInformation-ClimateDataOnline, :NOAANationalCentersForEnvironmentalInformation-ClimatologicalDataPublications,
    :NWSCLIMATEPREDICTIONCENTEREVAPORATION, :SpatialCaliforniaIrrigationManagementInformationSystem%28CIMIS%29 .

:StreamGainFromGroundwater-CA :hasDataSource :CADWRSGMADataViewer, :CAIntegratedWaterFlowModel%28IWFM%29,
    :CaliforniaAgriculturalLandAndWaterUseEstimates, :CaliforniaCentralValleySimulation%28C2VSim%29,
    :MODFLOW-OWHM%3AOneWaterHydrologicFlowModel, :USDANaturalResourcesConservationServiceGeospatialWebSoilSurvey,
    :USGSBasinCharacterizationModel .

:StreamLossToGroundwater-CA :hasDataSource :CADWRSGMADataViewer, :CAIntegratedWaterFlowModel%28IWFM%29,
    :CaliforniaAgriculturalLandAndWaterUseEstimates, :CaliforniaCentralValleySimulation%28C2VSim%29,
    :MODFLOW-OWHM%3AOneWaterHydrologicFlowModel, :USDANaturalResourcesConservationServiceGeospatialWebSoilSurvey,
    :USGSBasinCharacterizationModel .

:SurfaceWaterFlows-UT :hasDataSource :USGSStreamGages, :UTDiversionRecordsFromRiverCommissioners,
    :UTMunicipalPotableAndSecondaryDiversionRecords, :UTOtherIrrigationCompanyRecords,
    :UTReservoirStorageAndReleaseRecords, :UTWaterRights .

:TributaryInflow-UT :hasDataSource :USGSStreamGages, :UTDiversionRecordsFromRiverCommissioners,
    :UTMunicipalPotableAndSecondaryDiversionRecords, :UTOtherIrrigationCompanyRecords,
    :UTReservoirStorageAndReleaseRecords, :UTWaterRights .

:USBRConsumptiveUseMethod :hasDataSource :CooperativeObserverNetwork%28COOP%29, :CropTypeStateAssessments,
    :NationalAgriculturalStatisticsService%28NASS%29CroplandDataLayer, :PRISM, :SatelliteAndAerialPhotos,
    :StateData, :USGSStreamGages .

:UngagedStreamGains-WY :hasDataSource :USGSStreamGages, :WyomingWaterResourcesDataSystem%28WRDS%29 .

:WyomingGain%2FLossEstimationMethod :hasDataSource :USGSStreamGages, :WyomingWaterResourcesDataSystem%28WRDS%29 .

:UpstreamFlow :hasDataSource :USGSStreamGages, :WyomingWaterResourcesDataSystem%28WRDS%29 .

:UngagedStreamLosses-WY :hasDataSource :USGSStreamGages, :WyomingWaterResourcesDataSystem%28WRDS%29 .

:WYAgricultureConsumptiveUseEstimationMethod :hasDataSource :HistoricalData .

:WYElectricalGenerationMethod :hasDataSource :USEnergyInformationAdministration%28USEIA%29 .

:WYIndustrialProductionMethod :hasDataSource :WyomingOilAndGasConservationCommission%28WYOGCC%29 .

:WYIrrigatedAcreageConsumptiveUseModel :hasDataSource :HistoricalData .

:WYMineProductionMethod :hasDataSource :MineSafetyAndHealthAdministration%28MSHA%29 .

:WastewaterCollected-AUS :hasDataSource :DepartmentOfWaterAndEnvironmentalRegulation .

:WaterReleaseCausedByLandSubsidence-CA :hasDataSource :CADWRExtensometer, :CAIntegratedWaterFlowModel%28IWFM%29,
    :CaliforniaAgriculturalLandAndWaterUseEstimates, :CaliforniaCentralValleySimulation%28C2VSim%29,
    :CentralValleyHydrologicModel%28CVHM%29, :GravityRecoveryAndClimateExperiment%28GRACE%29,
    :MODFLOW-OWHM%3AOneWaterHydrologicFlowModel, :USGSExtensometer .

:AllocatedDiversion%3AIndividualUsers-AUS :hasDataSource :AUSDepartmentForEnvironmentAndWater%28DEW%29,
    :AUSDepartmentOfIndustry, :DepartmentOfWaterAndEnvironmentalRegulation, :EntitlementVolume,
    :IndividualUserLicenses, :Seqwater, :WaterIndustryLicensingManagementDatabase%28WILMA%29 .

:AllocatedDiversion%3AInter-region-AUS :hasDataSource :GippslandWaterAnnualReport .

:AllocatedDiversion%3AIrrigation-AUS :hasDataSource :DepartmentOfWaterAndEnvironmentalRegulation,
    :KimberelyAgriculturalInvestment%3AGoomingFarmlands, :OrdIrrigationCooperative%3APacksaddleAndIvanhoePlains,
    :SupervisoryControlAndDataAcquisitions%28SCADA%29, :WaterCorporation%3AM1Channel .

:AllocatedDiversion%3AUrbanSystem-AUS :hasDataSource :CumulativeWaterMeter, :DepartmentOfWaterAndEnvironmentalRegulation,
    :EntitlementVolume, :IndividualUserLicenses, :WaterIndustryLicensingManagementDatabase%28WILMA%29 .

:AllocatedDiversions%3ASurfaceWater-AUS :hasDataSource :AWRA-RModel, :WaterIndustryLicensingManagementDatabase%28WILMA%29 .

:AllocatedExtraction%3AIndividualUsers-AUS :hasDataSource :AUSDepartmentForEnvironmentAndWater%28DEW%29,
    :DepartmentOfWaterAndEnvironmentalRegulation, :EntitlementVolume, :IndividualUserLicenses,
    :WaterIndustryLicensingManagementDatabase%28WILMA%29 .

:AllocatedExtraction%3AIrrigation-AUS :hasDataSource :ReportFromBowenBrokenAndBurdekinHaughtonWaterSupplySchemes .

:AllocatedExtraction%3AUrbanSystem-AUS :hasDataSource :CumulativeWaterMeter, :DepartmentOfWaterAndEnvironmentalRegulation,
    :EntitlementVolume, :IndividualUserLicenses .

:AppliedWaterReuse%2FRecycledWater-CA :hasDataSource :CAAgriculturalWaterManagementPlans,
    :CADWRIrrigationMethodsSurvey, :CAIntegratedWaterFlowModel%28IWFM%29, :CAIntegratedWaterFlowModel%28IWFM%29DemandCalculator,
    :CALSIM2, :CARecycledWaterDataFromIndustrialUsers, :CARecycledWaterDataFromLocal%2FMunicipalWaterSuppliers,
    :CAUrbanWaterManagementPlans, :CAWastewaterDataAndDispositionOfTheWater, :Cal-SIMETAWUnitValues,
    :CaliforniaAgriculturalLandAndWaterUseEstimates, :CaliforniaCentralValleySimulation%28C2VSim%29,
    :CaliforniaStateWaterResourcesControlBoard%28SWRCB%29UrbanWaterSupplyStatistics, :CaliforniaWaterPlanPortfolio,
    :CaliforniaWaterPlanUpdateData, :DWRLandUseSurveys, :ExistingWaterRightInformationFromStateWaterResourcesControlBoard%28SWRCB%29,
    :MODFLOW-OWHM%3AOneWaterHydrologicFlowModel, :SWRCBWaterConservationPortal .

:Commercial%3AGolfCourses-NMOSE :hasDataSource :HistoricalDiversionsFile, :NMOSECropAcreageFile,
    :NMOSEGrowingSeasonFile, :NMOfficeOfTheStateEngineer%28NMOSE%29, :NationalAgriculturalStatisticsService,
    :NewMexicoInterstateStreamCommission%28NMISC%29, :PRISM, :USBureauOfReclamationStations,
    :USDACroplandDataLayer%28CDL%29, :USDAFarmServiceAgency, :WeatherStations .

:Commercial%3AUnmetered-NMOSE :hasDataSource :FacilityDirectorOrOperator .

:Commercial%3AIncompleteMetered-NMOSE :hasDataSource :NMOfficeOfTheStateEngineer%28NMOSE%29 .

:Commercial%3AMetered-NMOSE :hasDataSource :NMOfficeOfTheStateEngineer%28NMOSE%29 .

:Commercial%3ASchools-NMOSE :hasDataSource :NMOfficeOfTheStateEngineer%28NMOSE%29 .

:Delivery%3ADesalinatedWater-AUS :hasDataSource :CityWestWaterAnnualReport, :DepartmentOfWaterAndEnvironmentalRegulation,
    :SouthEastWaterAnnualReport, :YarraValleyWaterAnnualReport, :s.71WaterResourceReport .

:Delivery%3AInter-regionAgreement-AUS :hasDataSource :AUSDepartmentOfIndustry .

:Delivery%3AIrrigationScheme-AUS :hasDataSource :BarossaInfrastructureLimited%28BIL%29AnnualReport,
    :CustomerMeters, :SupervisoryControlAndDataAcquisitions%28SCADA%29, :VirginiaPipelineSchemePumpStation,
    :WillungaBasinWaterCompany .

:Delivery%3ARecycledWater-AUS :hasDataSource :BarossaInfrastructureLimited%28BIL%29AnnualReport,
    :WillungaBasinWaterCompany .

:Discharge%3ALandscape-AUS :hasDataSource :MODFLOW-OWHM%3AOneWaterHydrologicFlowModel,
    :WaterTableFluctuationModelling .

:Discharge%3ASurfaceWater-AUS :hasDataSource :DepartmentOfWaterAndEnvironmentalRegulation,
    :MODFLOW-OWHM%3AOneWaterHydrologicFlowModel, :WaterTableFluctuationModelling, :WesternMountLoftyRangesPrescribedWaterResourcesAreaWaterAllocationPlan .

:Discharge%3AUser-AUS :hasDataSource :UltrasonicFlowMeters, :WaterTrackingAndElectronicReportingSystem%28WaTERS%29 .

:Diversions%3AStatutoryRights-AUS :hasDataSource :AUSDepartmentOfEnvironmentAndNaturalResources,
    :NewSouthWalesDepartmentOfWater, :WaterSharingPlanForTheGreaterMetropolitanRegionUnregulatedRiverWaterSources,
    :WaterSharingPlanForTheKangarooRiverWaterSource, :s.71WaterResourceReport .

:Extraction%3AStatutoryRights-AUS :hasDataSource :AUSDepartmentOfEnvironmentAndNaturalResources,
    :NewSouthWalesDepartmentOfWater, :WaterIndustryLicensingManagementDatabase%28WILMA%29,
    :s.71WaterResourceReport .

:Industrial%3ACoalbedMethandProduction-WY :hasDataSource :WyomingOilAndGasConservationCommission%28WYOGCC%29 .

:Industrial%3AMiscellaneous-WY :hasDataSource :USCensusBureau .

:Industrial%3ANaturalGas-WY :hasDataSource :WyomingOilAndGasConservationCommission%28WYOGCC%29 .

:Industrial%3AOilAndGas-WY :hasDataSource :WyomingOilAndGasConservationCommission%28WYOGCC%29 .

:Inter-regionInflow%3AGroundwater-AUS :hasDataSource :AUSDepartmentOfEnvironment%2CLand%2CWaterAndPlanning,
    :DepartmentOfWaterAndEnvironmentalRegulation, :PortPhillipCatchmentManagementAuthority .

:Inter-regionInflow%3ASurfaceWater-AUS :hasDataSource :SnowyHydro, :StreamGages .

:Inter-regionOutflow%3AGroundwater-AUS :hasDataSource :AUSDepartmentOfEnvironment%2CLand%2CWaterAndPlanning,
    :DepartmentOfWaterAndEnvironmentalRegulation, :PortPhillipCatchmentManagementAuthority .

:Leakage%3AGroundwater-AUS :hasDataSource :EstimatedNon-revenueWaterVolumes .

:Leakage%3ALandscape-AUS :hasDataSource :MoretonAndLoganBasinResourceOperatingLicenses,
    :ResourceOperatingLicenseTables, :SupervisoryControlAndDataAcquisitions%28SCADA%29 .

:Livestock%3AMetered-NMOSE :hasDataSource :NMOfficeOfTheStateEngineer%28NMOSE%29 .

:Livestock%3AUnmetered-NMOSE :hasDataSource :NewMexicoDepartmentOfAgriculture .

:ManagedAquiferRecharge%3AIndividualUser-AUS :hasDataSource :AUSDepartmentForEnvironmentAndWater%28DEW%29,
    :IndividualUserLicenses .

:Mining%3AUnreported-NMOSE :hasDataSource :FacilityDirectorOrOperator .

:Non-AllocatedExtraction%3AIndividualUsers-AUS :hasDataSource :AustralianBureauOfStatisticsSurveys,
    :WaterCorporationSurveys .

:Non-allocatedDiversion%3AIndividualUsers-AUS :hasDataSource :EntitlementVolume, :IndividualUserLicenses .

:Power%3AUnreported-NMOSE :hasDataSource :FacilityDirectorOrOperator .

:PublicWaterSupply%3AMetered-NMOSE :hasDataSource :NMOSE%E2%80%99sWaterUseAndConservationBureau%28WUCB%29Survey,
    :NMOfficeOfTheStateEngineer%28NMOSE%29 .

:PublicWaterSupply%3AUnmetered-NMOSE :hasDataSource :GPSPopulationData, :MilitaryBasePopulationData,
    :NMOSETechnicalReportNo.48, :NMOfficeOfTheStateEngineer%28NMOSE%29, :NewMexicoEnvironmentDepartment%28NMED%29,
    :USCensusBureau, :UniversityOfNewMexicoGeospatialAndPopulationStudies%28UNMGPS%29 .

:Recharge%3AGroundwater-AUS :hasDataSource :AWRA-RModel, :MODFLOW-OWHM%3AOneWaterHydrologicFlowModel,
    :WaterTableFluctuationModelling .

:Recharge%3ALandscape-AUS :hasDataSource :DepartmentOfWaterAndEnvironmentalRegulation,
    :MODFLOW-OWHM%3AOneWaterHydrologicFlowModel, :WaterTableFluctuationModelling .

:Recharge%3ASurfaceWater-AUS :hasDataSource :DepartmentOfWaterAndEnvironmentalRegulation,
    :MODFLOW-OWHM%3AOneWaterHydrologicFlowModel, :WaterTableFluctuationModelling .

:RecycledWaterDelivery%3AUrbanUsers-AUS :hasDataSource :BillingMeters, :CustomerMeters,
    :OnsiteRe-useMeters .

:ReturnFlow%3AEnvironmentalPurposes-AUS :hasDataSource :s.71WaterResourceReport .

:SupplySystemDelivery%3AInter-Region-AUS :hasDataSource :DepartmentOfWaterAndEnvironmentalRegulation .

:SupplySystemDelivery%3AUrbanUsers-AUS :hasDataSource :BillingMeters, :CustomerMeters,
    :DepartmentOfWaterAndEnvironmentalRegulation, :EstimatedNon-revenueWaterVolumes .

:SupplySystemDischarge%3AReservoirs-AUS :hasDataSource :DepartmentOfWaterAndEnvironmentalRegulation .

:SupplySystemTransfer%3AInter-region-AUS :hasDataSource :DepartmentOfWaterAndEnvironmentalRegulation .

:Transfer%3AInter-region-AUS :hasDataSource :GippslandWaterAnnualReport, :MelbourneWaterAnnualReport .

:AgriculturalAppliedWater-CA :hasDataSource :CAAgriculturalWaterManagementPlans, :CALocalAgencyWaterDeliveryRecords,
    :CAPreviousReports, :Cal-SIMETAWUnitValues, :CaliforniaCentralValleySimulation%28C2VSim%29,
    :CentralValleyHydrologicModel%28CVHM%29, :ExistingCaliforniaWaterPlan, :On-farmWaterUseData,
    :UniversityOfCaliforniaCooperativeExtensionFarmAdvisors .

:CaliforniaCentralValleySimulation%28C2VSim%29 :hasDataSource :PRISM .

:Cal-SIMETAWModel :hasDataSource :Cal-SIMETAWUnitValues .

:Water-DutyBasedApproach :hasDataSource :CADWRIrrigationMethodsSurvey, :CAIrrigationTrainingAndResearchCenter%28ITRC%29EvapotranspirationData,
    :Cal-SIMETAWUnitValues, :CaliforniaWaterPlanPortfolio, :FAO56Chapter6SingleCropCoefficients%28Kc%29,
    :UniversityOfCaliforniaCooperativeExtensionFarmAdvisors .

:AquiferAttribution :hasDataSource :AUSDepartmentOfEnvironment%2CLand%2CWaterAndPlanning .

:AquiferThickness :hasDataSource :PortPhillipCatchmentManagementAuthority .

:BoreLocation :hasDataSource :AUSDepartmentOfEnvironment%2CLand%2CWaterAndPlanning .

:ChangeInGroundwaterLevel :hasDataSource :CaliforniaCentralValleySimulation%28C2VSim%29,
    :CentralValleyHydrologicModel%28CVHM%29 .

:SpecificYield :hasDataSource :CaliforniaCentralValleySimulation%28C2VSim%29, :CentralValleyHydrologicModel%28CVHM%29 .

:WaterStorageProduct :hasDataSource :AUSBureauOfMeteorology .

:LakeInflowFromStreams-CA :hasDataSource :CAIntegratedWaterFlowModel%28IWFM%29, :CaliforniaDataExchangeCenter%28CDEC%29,
    :CenterForHydrometeorologyAndRemoteSensingDataPortal%28CHRS%29, :DWRBulletin73%3AEvaporationFromWaterSurfaceInCalifornia%281979%29,
    :MODFLOW-OWHM%3AOneWaterHydrologicFlowModel, :USGSPublications, :USGSSurface-WaterDataForCalifornia .

:LakeOutflowToStreams-CA :hasDataSource :CAIntegratedWaterFlowModel%28IWFM%29, :CaliforniaDataExchangeCenter%28CDEC%29,
    :CenterForHydrometeorologyAndRemoteSensingDataPortal%28CHRS%29, :DWRBulletin73%3AEvaporationFromWaterSurfaceInCalifornia%281979%29,
    :MODFLOW-OWHM%3AOneWaterHydrologicFlowModel, :USGSPublications, :USGSSurface-WaterDataForCalifornia .

:Evapotranspiration%28ET%29Rates :hasDataSource :Cal-SIMETAWUnitValues, :CaliforniaIrrigationManagementInformationSystem%28CIMIS%29,
    :DWRBulletin73%3AEvaporationFromWaterSurfaceInCalifornia%281979%29, :SpatialCaliforniaIrrigationManagementInformationSystem%28CIMIS%29 .

:EstimateConveyanceSeepageRateBasedOnCanalCharacteristics :hasDataSource :CaliforniaCentralValleySimulation%28C2VSim%29,
    :CentralValleyHydrologicModel%28CVHM%29 .

:CropCoefficientApproach :hasDataSource :CAIrrigationTrainingAndResearchCenter%28ITRC%29EvapotranspirationData,
    :Cal-SIMETAWUnitValues, :CaliforniaIrrigationManagementInformationSystem%28CIMIS%29,
    :CaliforniaWaterPlanPortfolio, :FAO56Chapter6SingleCropCoefficients%28Kc%29, :SpatialCaliforniaIrrigationManagementInformationSystem%28CIMIS%29 .

:ReferenceCropET%28ETo%29 :hasDataSource :CAIrrigationTrainingAndResearchCenter%28ITRC%29EvapotranspirationData,
    :Cal-SIMETAWUnitValues, :CaliforniaIrrigationManagementInformationSystem%28CIMIS%29 .

:CulturalPractices :hasDataSource :CaliforniaDepartmentOfFishAndWildlife%28CDFW%29,
    :CaliforniaWaterPlanPortfolio, :DWRLandUseSurveys, :DataFromPrivateWetlandsOrDuckClubs,
    :USFishAndWildlifeServices .

:CustomerMeters :hasDataSource :SAWaterGISDatabase .

:DailyMaxAndMinAirTemperature :hasDataSource :CaliforniaDataExchangeCenter%28CDEC%29,
    :CaliforniaIrrigationManagementInformationSystem%28CIMIS%29 .

:DailyPrecipitation :hasDataSource :CaliforniaDataExchangeCenter%28CDEC%29, :CaliforniaIrrigationManagementInformationSystem%28CIMIS%29 .

:DailyShort-WaveSolarRadiation :hasDataSource :CaliforniaDataExchangeCenter%28CDEC%29,
    :CaliforniaIrrigationManagementInformationSystem%28CIMIS%29 .

:DailyWaterBalanceApproach :hasDataSource :AWRA-RModel .

:FloodplainModule :hasDataSource :AWRA-RModel .

:GISGroundwaterModelling :hasDataSource :AUSDepartmentOfEnvironment%2CLand%2CWaterAndPlanning,
    :PortPhillipCatchmentManagementAuthority .

:GroundwaterLevel :hasDataSource :AUSDepartmentOfEnvironment%2CLand%2CWaterAndPlanning .

:HydraulicConductivity :hasDataSource :PortPhillipCatchmentManagementAuthority .

:Peel-HarveyRegionalAquiferModelingSystem%28PHRAMS%29 :hasDataSource :DepartmentOfWaterAndEnvironmentalRegulation .

:PerthRegionalAquiferModelingSystems%28PRAMS%29 :hasDataSource :DepartmentOfWaterAndEnvironmentalRegulation .

:GroundwaterExtractionUnderStatutoryRightsEstimationMethod :hasDataSource :AUSDepartmentOfEnvironmentAndNaturalResources .

:HabitatAcreage :hasDataSource :CaliforniaDepartmentOfFishAndWildlife%28CDFW%29, :CaliforniaWaterPlanPortfolio,
    :DWRLandUseSurveys, :DataFromPrivateWetlandsOrDuckClubs, :USFishAndWildlifeServices .

:ManagedWetlandAppliedWater-CA :hasDataSource :CAPreviousReports, :Cal-SIMETAWUnitValues,
    :CaliforniaCentralValleySimulation%28C2VSim%29, :CaliforniaDepartmentOfFishAndWildlife%28CDFW%29,
    :CaliforniaWaterPlanPortfolio, :CaliforniaWaterPlanWaterPortfolioManagedWetlandsWaterUseData,
    :CentralValleyHydrologicModel%28CVHM%29, :DWRLandUseSurveys, :DataFromPrivateWetlandsOrDuckClubs,
    :LocalAgencyRecords, :USBRCentralValleyProjectRefugeWaterDeliveryData, :USFWSAndCDFWRefugeWaterManagementPlans,
    :USFishAndWildlifeServices .

:UrbanAppliedWater-CA :hasDataSource :CAPreviousReports, :CAUrbanWaterManagementPlans,
    :CaliforniaCentralValleySimulation%28C2VSim%29, :CaliforniaDepartmentOfFinance, :CaliforniaWaterPlanPortfolio,
    :CentralValleyHydrologicModel%28CVHM%29, :DWRPublicWaterSupplyStatisticsData-Historical,
    :LocalAgencyRecords, :MunicipalWaterUseRecords, :SWRCBElectronicAnnualReport, :SWRCBMonthlyUrbanWaterProductionReporting,
    :USCensusBureau, :UrbanAppliedWater-CA, :WaterUseSurveys .

:IndividualUserLicenses :hasDataSource :KimberelyAgriculturalInvestment%3AGoomingFarmlands,
    :OrdIrrigationCooperative%3APacksaddleAndIvanhoePlains, :WaterCorporation%3AM1Channel .

:IndustrialWaterUse :hasDataSource :WaterUseSurveys .

:LandscapeModelledRunoff :hasDataSource :AWRA-LModel .

:MeteredWaterData :hasDataSource :AUSDepartmentOfIndustry, :BillingMeters, :CityWestWaterAnnualReport,
    :CumulativeWaterMeter, :CustomerMeters, :DepartmentOfWaterAndEnvironmentalRegulation,
    :SnowyHydro, :SouthEastWaterAnnualReport, :UltrasonicFlowMeters, :YarraValleyWaterAnnualReport .

:ManagedWetlandsAppliedWaterEstimation :hasDataSource :CaliforniaDepartmentOfFishAndWildlife%28CDFW%29,
    :CaliforniaWaterPlanPortfolio, :DWRLandUseSurveys, :DataFromPrivateWetlandsOrDuckClubs,
    :USFishAndWildlifeServices .

:UnitETOfAppliedWater :hasDataSource :CaliforniaWaterPlanPortfolio .

:ModelledRunoff :hasDataSource :AWRA-RModel .

:OtherSupplySystemDecreases-AUS :hasDataSource :DepartmentOfWaterAndEnvironmentalRegulation,
    :EstimatedNon-revenueWaterVolumes .

:PopulationAndPer-CapitaWaterUse :hasDataSource :CaliforniaDepartmentOfFinance, :MunicipalWaterUseRecords,
    :USCensusBureau, :WaterUseSurveys .

:PropertyAreaEstimationMethodsForSurfaceWaterDiversions :hasDataSource :AUSDepartmentOfEnvironmentAndNaturalResources .

:RechargeCreditBalance :hasDataSource :AUSDepartmentForEnvironmentAndWater%28DEW%29,
    :IndividualUserLicenses .

:RiverAndGroundwaterInteractionModule :hasDataSource :AWRA-RModel .

:RiverLosses-AUS :hasDataSource :AWRA-RModel .

:Precipitation-RunoffModelingSystem%28PRMS%29 :hasDataSource :CaliforniaDataExchangeCenter%28CDEC%29,
    :CaliforniaIrrigationManagementInformationSystem%28CIMIS%29, :STATSGOSoilsData, :USDANaturalResourcesConservationServiceGeospatialWebSoilSurvey .

:PublicPolicyInstituteOfCalifornia%28PPIC%29Map :hasDataSource :CaliforniaIrrigationManagementInformationSystem%28CIMIS%29,
    :PRISM, :U.C.DavisSoilResourceLab .

:DescriptiveDataOfTopography%2CSoils%2CAndVegetation :hasDataSource :STATSGOSoilsData,
    :USDANaturalResourcesConservationServiceGeospatialWebSoilSurvey .

:FiniteElementSubsurfaceFlowSystem%28FEFLOW%29 :hasDataSource :AUSDepartmentOfEnvironmentAndNaturalResources .

:Non-allocatedDiversion%3AUrbanWaterSystemEstimationMethod :hasDataSource :WaterIndustryLicensingManagementDatabase%28WILMA%29 .

:CropConsumptiveUse-CO :hasEstimationMethod :COConsumptiveUseMethod .

:GroundwaterExtraction-CA :hasEstimationMethod :CaliforniaCentralValleySimulation%28C2VSim%29,
    :CentralValleyHydrologicModel%28CVHM%29, :LandUseAndAppliedWaterEstimationMethod .

:LivestockConsumptiveUse-CO :hasEstimationMethod :COLivestockMethod .

:MunicipalAndIndustrialConsumptiveUse-CO :hasEstimationMethod :COMunicipalAndIndustrialMethod .

:MunicipalConsumptiveUse-WY :hasEstimationMethod :WithdrawalMethod .

:MunicipalTotalUse-WY :hasEstimationMethod :WithdrawalMethod .

:SurfaceWaterDiversions-CA :hasEstimationMethod :LandUseAndAppliedWaterEstimationMethod .

:AgriculturalAndMunicipalDiversions-UT :hasEstimationMethod :USGSStreamStats, :UTDivisionOfWaterResourcesArea-AltitudeMethod .

:AgriculturalConsumptiveUse-WY :hasEstimationMethod :WYConsumptiveUseMethod .

:WYConsumptiveUseMethod :hasEstimationMethod :CropIrrigationRequirement, :DailyPenman-Monteith,
    :EnergyBalanceRemoteSensing, :METRIC, :ModifiedBlaney-Criddle, :ModifiedBlaney-CriddleWithETElevationAdjustment,
    :On-FarmWaterBalance, :OriginalHargreaves, :SCSTR21, :StateCU, :WYIrrigatedAcreageAssessment .

:Evapotranspiration-CA :hasEstimationMethod :Cal-SIMETAWModel, :CaliforniaCentralValleySimulation%28C2VSim%29,
    :CaliforniaWaterPlanPortfolio, :CropCoefficientApproach, :METRIC, :Water-DutyBasedApproach .

:AgriculturalDepletions-UT :hasEstimationMethod :UTConsumptiveUseMethod .

:UTConsumptiveUseMethod :hasEstimationMethod :CropIrrigationRequirementEstimationMethod,
    :DailyPenman-Monteith, :EnergyBalanceRemoteSensing, :Inflow-OutflowApproach, :METRIC,
    :ModifiedBlaney-Criddle, :UTEffectivePrecipitationMethod, :UTIrrigatedAcreageAssessment .

:SurfaceDiversionToCropland-UT :hasEstimationMethod :USGSStreamStats, :UTDivisionOfWaterResourcesArea-AltitudeMethod .

:AgriculturalPotentialConsumptiveUse-UT :hasEstimationMethod :DailyPenman-Monteith,
    :ModifiedBlaney-Criddle .

:AreaOutflows :hasEstimationMethod :USGSStreamStats, :UTDivisionOfWaterResourcesArea-AltitudeMethod .

:BasinOutflow-UT :hasEstimationMethod :USGSStreamStats, :UTDivisionOfWaterResourcesArea-AltitudeMethod .

:StreamOutfow-CA :hasEstimationMethod :DrainageAreaRatioMethod, :Precipitation-RunoffModelingSystem%28PRMS%29,
    :USGSDR3M, <http://purl.org/iow/WaterBudgetingFramework/UniversityOfWashington%E2%80%99sVariableInfiltrationCapacityModel%28VIC%29.>,
    :Vieux%26Associates%27Vflo, :WaterResourceAssociatesHYSIM .

:Exports-CO :hasEstimationMethod :HistoricalData .

:BasinInflow-UT :hasEstimationMethod :USGSStreamStats, :UTDivisionOfWaterResourcesArea-AltitudeMethod .

:RiverInflow-UT :hasEstimationMethod :USGSStreamStats, :UTDivisionOfWaterResourcesArea-AltitudeMethod .

:UngagedSurfaceWaterInflow-CO :hasEstimationMethod :NaturalFlowGainDistribution .

:StreamInflow-CA :hasEstimationMethod :DrainageAreaRatioMethod, :Precipitation-RunoffModelingSystem%28PRMS%29,
    :USGSDR3M, <http://purl.org/iow/WaterBudgetingFramework/UniversityOfWashington%E2%80%99sVariableInfiltrationCapacityModel%28VIC%29.>,
    :Vieux%26Associates%27Vflo, :WaterResourceAssociatesHYSIM .

:COConsumptiveUseMethod :hasEstimationMethod :COIrrigatedAcreageAssessment, :CropIrrigationRequirementEstimationMethod,
    :DailyPenman-Monteith, :EnergyBalanceRemoteSensing, :METRIC, :ModifiedBlaney-Criddle,
    :ModifiedBlaney-CriddleWithETElevationAdjustment, :NDVIRemoteSensing, :NDVIstar, :On-FarmWaterBalance,
    :OriginalBlaney-Criddle, :OriginalBlaney-CriddleWithETElevationAdjustment, :RESET,
    :SCSTR21, :StateCU .

:StateCU :hasEstimationMethod :ModifiedBlaney-Criddle, :OriginalBlaney-Criddle .

:CropIrrigationRequirement :hasEstimationMethod :CropIrrigationRequirementEstimationMethod .

:EffectivePrecipitation :hasEstimationMethod :SCSTR21, :UTEffectivePrecipitationMethod .

:IrrigatedAcreage :hasEstimationMethod :COIrrigatedAcreageAssessment, :NMIrrigatedAcreageAssessment,
    :USBRIrrigatedAcreageAssessment, :UTIrrigatedAcreageAssessment, :WYIrrigatedAcreageAssessment .

:PotentialConsumptiveUse :hasEstimationMethod :DailyPenman-Monteith, :ModifiedBlaney-Criddle,
    :ModifiedBlaney-CriddleWithETElevationAdjustment, :OriginalBlaney-Criddle, :OriginalBlaney-CriddleWithETElevationAdjustment .

:ChangeInGroundwaterStorage-CA :hasEstimationMethod :CaliforniaCentralValleySimulation%28C2VSim%29,
    :CentralValleyHydrologicModel%28CVHM%29, :ChangeInGroundwaterLevel, :MassBalance,
    :USGSCaliforniaWaterScienceCenter-GroundwaterModeling .

:ChangeInGroundwaterStorage-AUS :hasEstimationMethod :WaterStorageProduct .

:ChangeInLandSystemStorage-CA :hasEstimationMethod :CALSIM3, :Cal-SIMETAWModel, :CaliforniaCentralValleySimulation%28C2VSim%29,
    :CentralValleyHydrologicModel%28CVHM%29, :WaterBalanceForUnsaturatedZoneStorage, :WaterUseModels .

:ChangeInSurfaceWaterStorage-AUS :hasEstimationMethod :Elevation-Area-CapacityTables,
    :WaterStorageProduct .

:ChangeInSurfaceWaterStorage-CA :hasEstimationMethod :CALSIM2, :CALSIM3, :CaliforniaCentralValleySimulation%28C2VSim%29,
    :CaliforniaDataExchangeCenter%28CDEC%29, :CentralValleyHydrologicModel%28CVHM%29,
    :MassBalance .

:MunicipalAndIndustrialDiversions-UT :hasEstimationMethod :USGSStreamStats, :UTDivisionOfWaterResourcesArea-AltitudeMethod .

:ConveyanceEvaporation-CA :hasEstimationMethod :Evapotranspiration%28ET%29Rates, :MassBalance .

:ConveyanceSeepage-CA :hasEstimationMethod :EstimateConveyanceSeepageRateBasedOnCanalCharacteristics,
    :MassBalance .

:Precipitation-CA :hasEstimationMethod :CaliforniaCentralValleySimulation%28C2VSim%29,
    :CentralValleyHydrologicModel%28CVHM%29, :SpatialAveragingTechniques .

:Precipitation-NM :hasEstimationMethod :MonthlyPrecipitationVolume .

:IrrigatedAgricultureDepletions-NMOSE :hasEstimationMethod :NMConsumptiveUseMethod .

:DomesticTotalUse-WY :hasEstimationMethod :WithdrawalMethod .

:Evaporation-AUS :hasEstimationMethod :Morton%27sShallowLakeFormulation .

:EvaporationFromReservoirs-NMOSE :hasEstimationMethod :EmpiricalDataForSmallReservoirs,
    :PanApproach .

:LakeEvaporation-CA :hasEstimationMethod :EvaporationPanMethod, :MassTransferEquations .

:ReservoirEvaporation-CO :hasEstimationMethod :ReservoirEstimationMethod .

:ReservoirEvaporation-UT :hasEstimationMethod :Elevation-Area-CapacityTables, :Evaporation,
    :HistoricalData, :Rainfall .

:GroundwaterExport-CA :hasEstimationMethod :LandUseAndAppliedWaterEstimationMethod .

:SurfaceWaterExports-CA :hasEstimationMethod :CALSIM2, :CaliforniaCentralValleySimulation%28C2VSim%29,
    :CentralValleyHydrologicModel%28CVHM%29, :LandUseAndAppliedWaterEstimationMethod .

:FloodReturn-AUS :hasEstimationMethod :FloodplainModule .

:SubsurfaceInflow-CA :hasEstimationMethod :CaliforniaCentralValleySimulation%28C2VSim%29,
    :CentralValleyHydrologicModel%28CVHM%29, :Darcy%27sLaw, :USGSCaliforniaWaterScienceCenter-GroundwaterModeling .

:SubsurfaceOutflow-CA :hasEstimationMethod :CaliforniaCentralValleySimulation%28C2VSim%29,
    :CentralValleyHydrologicModel%28CVHM%29, :Darcy%27sLaw, :USGSCaliforniaWaterScienceCenter-GroundwaterModeling .

:GroundwaterDischarge-AUS :hasEstimationMethod :MODFLOW-OWHM%3AOneWaterHydrologicFlowModel,
    :Peel-HarveyRegionalAquiferModelingSystem%28PHRAMS%29, :PerthRegionalAquiferModelingSystems%28PRAMS%29 .

:Discharge%3AGroundwater-AUS :hasEstimationMethod :MODFLOW-OWHM%3AOneWaterHydrologicFlowModel .

:LakeGainFromGroundwater-CA :hasEstimationMethod :Darcy%27sLaw, :EffectiveThicknessOfTheAquifer%28b%29,
    :FlowNetAnalysis, :MassBalance .

:ImportedWater-CA :hasEstimationMethod :CALSIM2, :CaliforniaCentralValleySimulation%28C2VSim%29,
    :CentralValleyHydrologicModel%28CVHM%29, :LandUseAndAppliedWaterEstimationMethod .

:Industrial-NMOSE :hasEstimationMethod :Metered .

:SurfaceWaterDelivery-CA :hasEstimationMethod :LandUseAndAppliedWaterEstimationMethod .

:Inter-regionCoastalInflow-AUS :hasEstimationMethod :Darcy%27sLaw, :GISGroundwaterModelling,
    :GeographicInformationSystem%28GIS%29, :Peel-HarveyRegionalAquiferModelingSystem%28PHRAMS%29,
    :PerthRegionalAquiferModelingSystems%28PRAMS%29, :PortPhillipCatchmentManagementAuthorityGroundwaterModel .

:Inter-regionCoastalOutflow-AUS :hasEstimationMethod :Adelaide, :Darcy%27sLaw, :GeographicInformationSystem%28GIS%29,
    :Peel-HarveyRegionalAquiferModelingSystem%28PHRAMS%29, :PerthRegionalAquiferModelingSystems%28PRAMS%29,
    :PortPhillipCatchmentManagementAuthorityGroundwaterModel .

:NMConsumptiveUseMethod :hasEstimationMethod :DailyPenman-Monteith, :EnergyBalanceRemoteSensing,
    :IndicatorGageApproach, :METRIC, :ModifiedBlaney-Criddle, :NMIrrigatedAcreageAssessment,
    :NMSpreadsheet-BasedConsumptiveUseModel, :OriginalHargreaves, :SCSTR21 .

:ConsumptiveIrrigationRequirement%28CIR%29 :hasEstimationMethod :OriginalBlaney-Criddle .

:LakeLossToGroundwater-CA :hasEstimationMethod :Darcy%27sLaw, :FlowNetAnalysis, :MassBalance .

:ManagedAquiferRecharge-AUS :hasEstimationMethod :MeteredWaterData .

:ManagedAquiferRecharge-CA :hasEstimationMethod :LandUseAndAppliedWaterEstimationMethod .

:Industrial%3AMineProduction-WY :hasEstimationMethod :WYMineProductionMethod .

:ReturnFlow-CA :hasEstimationMethod :ReturnFlowEstimationMethod .

:NativeVegetationConsumptiveUse-CO :hasEstimationMethod :CONativeVegetationMethod .

:Outflow-AUS :hasEstimationMethod :AWRA-LModel, :AWRA-RModel .

:OverbankFloodSpilling-AUS :hasEstimationMethod :FloodplainModule .

:OverbankFlow-AUS :hasEstimationMethod :FloodplainModule .

:RechargeOfAppliedWater-CA :hasEstimationMethod :CaliforniaCentralValleySimulation%28C2VSim%29,
    :CaliforniaWaterPlanPortfolio, :CentralValleyHydrologicModel%28CVHM%29, :LandUseAndAppliedWaterEstimationMethod .

:RechargeOfPrecipitation-CA :hasEstimationMethod :CaliforniaCentralValleySimulation%28C2VSim%29,
    :CentralValleyHydrologicModel%28CVHM%29, :ConstantPercentage, :Rainfall-RunoffMethod .

:ReservoirEvaporation-WY :hasEstimationMethod :PanMethod%28NetEvaporation%29 .

:Runoff-AUS :hasEstimationMethod :LandscapeModelledRunoff, :ModelledRunoff .

:Runoff-CA :hasEstimationMethod :Precipitation-RunoffModelingSystem%28PRMS%29, :PublicPolicyInstituteOfCalifornia%28PPIC%29Map,
    :RunoffCurveNumberMethod, :U.C.DavisSoilResourceLab, :USGSBasinCharacterizationModel .

:Self-SuppliedDomestic-NMOSE :hasEstimationMethod :WithdrawalMethod .

:StreamEvaporation-CA :hasEstimationMethod :Evapotranspiration%28ET%29Rates, :MassBalance,
    :MassTransferEquations .

:StreamGainFromGroundwater-CA :hasEstimationMethod :BaseflowSeparationTechniques,
    :CaliforniaCentralValleySimulation%28C2VSim%29, :CentralValleyHydrologicModel%28CVHM%29,
    :ConstantSeepagePercentage, :Darcy%27sLaw, :FlowNetAnalysis, :MassBalance .

:StreamLossToGroundwater-CA :hasEstimationMethod :BaseflowSeparationTechniques, :CaliforniaCentralValleySimulation%28C2VSim%29,
    :CentralValleyHydrologicModel%28CVHM%29, :ConstantSeepagePercentage, :FlowNetAnalysis,
    :MassBalance .

:SurfaceWaterFlows-UT :hasEstimationMethod :USGSStreamStats, :UTDivisionOfWaterResourcesArea-AltitudeMethod .

:SurfaceWaterInflows-NM :hasEstimationMethod :Streamflow .

:TributaryInflow-UT :hasEstimationMethod :USGSStreamStats, :UTDivisionOfWaterResourcesArea-AltitudeMethod .

:USBRConsumptiveUseMethod :hasEstimationMethod :DailyPenman-Monteith, :EnergyBalanceRemoteSensing,
    :IndicatorGageApproach, :METRIC, :ModifiedBlaney-Criddle, :RESET, :SCSTR21, :USBRIrrigatedAcreageAssessment,
    :XCONS .

:UngagedStreamGains-WY :hasEstimationMethod :WyomingGain%2FLossEstimationMethod .

:UngagedStreamLosses-WY :hasEstimationMethod :WyomingGain%2FLossEstimationMethod .

:WYAgricultureConsumptiveUseEstimationMethod :hasEstimationMethod :StateCU .

:WastewaterCollected-AUS :hasEstimationMethod :MeteredWaterData .

:WaterReleaseCausedByLandSubsidence-CA :hasEstimationMethod :CaliforniaCentralValleySimulation%28C2VSim%29,
    :CentralValleyHydrologicModel%28CVHM%29, :MODFLOW-OWHM%3AOneWaterHydrologicFlowModel .

:AllocatedDiversion%3AEnvironmentalPurposes-AUS :hasEstimationMethod :MeteredWaterData .

:AllocatedDiversion%3AIndividualUsers-AUS :hasEstimationMethod :EstimationOfAbstraction,
    :MeteredWaterData .

:AllocatedDiversion%3AIrrigation-AUS :hasEstimationMethod :IndividualUserLicenses,
    :MeteredWaterData, :ReportFromBowenBrokenAndBurdekinHaughtonWaterSupplySchemes .

:AllocatedDiversion%3AIrrigationScheme-AUS :hasEstimationMethod :MeteredWaterData .

:AllocatedDiversion%3AUrbanSystem-AUS :hasEstimationMethod :MeteredWaterData .

:AllocatedDiversions%3ASurfaceWater-AUS :hasEstimationMethod :MeteredWaterData .

:AllocatedExtraction%3AEnvironmentalPurposes-AUS :hasEstimationMethod :MeteredWaterData .

:AllocatedExtraction%3AIndividualUsers-AUS :hasEstimationMethod :EstimationOfAbstraction,
    :MeteredWaterData .

:AllocatedExtraction%3AIrrigation-AUS :hasEstimationMethod :MeteredWaterData .

:AllocatedExtraction%3AUrbanSystem-AUS :hasEstimationMethod :MeteredWaterData .

:AllocationExtraction%3ASalinityAndWaterTableManagement-AUS :hasEstimationMethod :Metered .

:AppliedWaterReuse%2FRecycledWater-CA :hasEstimationMethod :EstimateAppliedWaterReuseAndRecycledWaterVolumes .

:Commercial%3AGolfCourses-NMOSE :hasEstimationMethod :NMIrrigationWithdrawals .

:Commercial%3AUnmetered-NMOSE :hasEstimationMethod :PersonalOutreach .

:Commercial%3AIncompleteMetered-NMOSE :hasEstimationMethod :InterpolationFromOtherRecords .

:Commercial%3AMetered-NMOSE :hasEstimationMethod :Metered .

:Commercial%3ASchools-NMOSE :hasEstimationMethod :WithdrawalMethod .

:Delivery%3ADesalinatedWater-AUS :hasEstimationMethod :MeteredWaterData .

:Delivery%3AInter-regionAgreement-AUS :hasEstimationMethod :MeteredWaterData .

:Delivery%3AIrrigationScheme-AUS :hasEstimationMethod :MeteredWaterData .

:Discharge%3ALandscape-AUS :hasEstimationMethod :FiniteElementSubsurfaceFlowSystem%28FEFLOW%29,
    :MODFLOW-OWHM%3AOneWaterHydrologicFlowModel, :MeteredWaterData, :Peel-HarveyRegionalAquiferModelingSystem%28PHRAMS%29,
    :PerthRegionalAquiferModelingSystems%28PRAMS%29 .

:Discharge%3ASea-AUS :hasEstimationMethod :MeteredWaterData .

:Discharge%3ASurfaceWater-AUS :hasEstimationMethod :FiniteElementSubsurfaceFlowSystem%28FEFLOW%29,
    :LyneAndHollickFilter, :MIKE11, :MODFLOW-OWHM%3AOneWaterHydrologicFlowModel, :MeteredWaterData,
    :Peel-HarveyRegionalAquiferModelingSystem%28PHRAMS%29, :PerthRegionalAquiferModelingSystems%28PRAMS%29 .

:Discharge%3AUrbanSupply-AUS :hasEstimationMethod :MeteredWaterData .

:Discharge%3AUrbanSupplySystem-AUS :hasEstimationMethod :MeteredWaterData .

:Discharge%3AUser-AUS :hasEstimationMethod :MeteredWaterData .

:Discharge%3AWastewater-AUS :hasEstimationMethod :MeteredWaterData .

:Diversions%3AStatutoryRights-AUS :hasEstimationMethod :PropertyAreaEstimationMethodsForSurfaceWaterDiversions .

:Extraction%3AStatutoryRights-AUS :hasEstimationMethod :GroundwaterExtractionUnderStatutoryRightsEstimationMethod .

:Industrial%3ACoalbedMethandProduction-WY :hasEstimationMethod :WYIndustrialProductionMethod .

:Industrial%3ANaturalGas-WY :hasEstimationMethod :WYIndustrialProductionMethod .

:Industrial%3AOilAndGas-WY :hasEstimationMethod :WYIndustrialProductionMethod .

:Inter-regionInflow%3AGroundwater-AUS :hasEstimationMethod :FiniteElementSubsurfaceFlowSystem%28FEFLOW%29,
    :GISGroundwaterModelling, :GroundwaterModelling, :Peel-HarveyRegionalAquiferModelingSystem%28PHRAMS%29,
    :PerthRegionalAquiferModelingSystems%28PRAMS%29, :PortPhillipCatchmentManagementAuthorityGroundwaterModel .

:Inter-regionInflow%3ASurfaceWater-AUS :hasEstimationMethod :AWRA-RModel, :MeteredWaterData .

:Inter-regionOutflow%3AGroundwater-AUS :hasEstimationMethod :GISGroundwaterModelling,
    :GroundwaterModelling, :Peel-HarveyRegionalAquiferModelingSystem%28PHRAMS%29, :PerthRegionalAquiferModelingSystems%28PRAMS%29,
    :PortPhillipCatchmentManagementAuthorityGroundwaterModel .

:Leakage%3AFarmDams-AUS :hasEstimationMethod :NetworkRealLossesAndApparentLossesModelingSoftware .

:Leakage%3AGroundwater-AUS :hasEstimationMethod :MeteredWaterData, :NetworkRealLossesAndApparentLossesModelingSoftware,
    :RealLossesEquation .

:Leakage%3ALandscape-AUS :hasEstimationMethod :MeteredWaterData .

:Leakage%3AUrbanSystem-AUS :hasEstimationMethod :MeteredWaterData, :NetworkRealLossesAndApparentLossesModelingSoftware,
    :RealLossesEquation .

:Livestock%3AMetered-NMOSE :hasEstimationMethod :Metered .

:Livestock%3AUnmetered-NMOSE :hasEstimationMethod :WithdrawalMethod .

:ManagedAquiferRecharge%3AIndividualUser-AUS :hasEstimationMethod :RechargeCreditBalance .

:ManagedAquiferRecharge%3AUrban-AUS :hasEstimationMethod :MeteredWaterData .

:Mining%3AUnreported-NMOSE :hasEstimationMethod :PersonalOutreach .

:Non-AllocatedDiversion%3ASurfaceWater-AUS :hasEstimationMethod :AWRA-RModel, :MeteredWaterData .

:Non-AllocatedExtraction%3AGroundwater-AUS :hasEstimationMethod :MeteredWaterData .

:Non-AllocatedExtraction%3AIndividualUsers-AUS :hasEstimationMethod :IndividualUserLicenses,
    :MeteredWaterData, :SpatialAssessments, :WaterAllocationPlans, :WaterUseSurveys .

:Non-allocatedDiversion%3AEnvironmentalPurposes-AUS :hasEstimationMethod :HistoricalData,
    :MeteredWaterData .

:Non-allocatedDiversion%3AIndividualUsers-AUS :hasEstimationMethod :HistoricalData,
    :MeteredWaterData .

:Non-allocatedDiversion%3AUrbanSystem-AUS :hasEstimationMethod :HistoricalData, :MeteredWaterData,
    :Non-allocatedDiversion%3AUrbanWaterSystemEstimationMethod .

:PointReturn%3AIrrigation-AUS :hasEstimationMethod :MeteredWaterData, :SurplusIrrigationAssumption .

:Power%3AUnreported-NMOSE :hasEstimationMethod :PersonalOutreach .

:PublicWaterSupply%3AMetered-NMOSE :hasEstimationMethod :Metered .

:PublicWaterSupply%3AUnmetered-NMOSE :hasEstimationMethod :WithdrawalMethod .

:Recharge%3AGroundwater-AUS :hasEstimationMethod :RechargeAsPercentageOfRainfall,
    :RiverAndGroundwaterInteractionModule .

:Recharge%3ALandscape-AUS :hasEstimationMethod :AWRA-LModel, :CSIROWavesModel, :FiniteElementSubsurfaceFlowSystem%28FEFLOW%29,
    :MODFLOW-OWHM%3AOneWaterHydrologicFlowModel, :Peel-HarveyRegionalAquiferModelingSystem%28PHRAMS%29,
    :PerthRegionalAquiferModelingSystems%28PRAMS%29, :RechargeAsPercentageOfRainfall,
    :VerticalFluxModel .

:Recharge%3ASurfaceWater-AUS :hasEstimationMethod :FiniteElementSubsurfaceFlowSystem%28FEFLOW%29,
    :MIKE11, :MODFLOW-OWHM%3AOneWaterHydrologicFlowModel, :Peel-HarveyRegionalAquiferModelingSystem%28PHRAMS%29,
    :PerthRegionalAquiferModelingSystems%28PRAMS%29, :RechargeAsPercentageOfRainfall .

:RecycledWaterDelivery%3AUrbanUsers-AUS :hasEstimationMethod :MeteredWaterData .

:RiparianRelease%3AUrbanSupply-AUS :hasEstimationMethod :MeteredWaterData .

:SupplySystemDelivery%3AInter-Region-AUS :hasEstimationMethod :MeteredWaterData .

:SupplySystemDelivery%3AUrbanUsers-AUS :hasEstimationMethod :MeteredWaterData .

:SupplySystemDischarge%3AReservoirs-AUS :hasEstimationMethod :MeteredWaterData .

:SupplySystemTransfer%3AInter-region-AUS :hasEstimationMethod :MeteredWaterData .

:WastewaterDischarge%3ALandscape-AUS :hasEstimationMethod :MeteredWaterData .

:AgriculturalAppliedWater-CA :hasEstimationMethod :Cal-SIMETAWModel, :CaliforniaCentralValleySimulation%28C2VSim%29,
    :CentralValleyHydrologicModel%28CVHM%29, :CropETApproach, :Water-DutyBasedApproach .

:LakeInflowFromStreams-CA :hasEstimationMethod :MassBalance, :MassCurve, :ReservoirOperationRuleCurve .

:LakeOutflowToStreams-CA :hasEstimationMethod :MassBalance, :MassCurve, :ReservoirOperationRuleCurve .

:GISGroundwaterModelling :hasEstimationMethod :PortPhillipCatchmentManagementAuthorityGroundwaterModel .

:ManagedWetlandAppliedWater-CA :hasEstimationMethod :ManagedWetlandsAppliedWaterEstimation .

:UrbanAppliedWater-CA :hasEstimationMethod :CaliforniaCentralValleySimulation%28C2VSim%29,
    :CaliforniaWaterPlanPortfolio, :CentralValleyHydrologicModel%28CVHM%29, :PopulationAndPer-CapitaWaterUse .

:ManagedWetlandsAppliedWaterEstimation :hasEstimationMethod :Cal-SIMETAWModel, :CaliforniaCentralValleySimulation%28C2VSim%29,
    :CaliforniaWaterPlanPortfolio, :CentralValleyHydrologicModel%28CVHM%29, :ManagedWetlandsAppliedWaterEstimation .

:OtherSupplySystemDecreases-AUS :hasEstimationMethod :MeteredWaterData, :NetworkRealLossesAndApparentLossesModelingSoftware,
    :Observation, :RealLossesEquation .

:OtherWastewaterDecreases-AUS :hasEstimationMethod :MeteredWaterData, :Observation .

:RiverLosses-AUS :hasEstimationMethod :RiverAndGroundwaterInteractionModule .

:Losses%3AManagementOfTreatedWater-AUS :hasEstimationMethod :MeteredWaterData .

:Losses%3AWastewaterTreatmentSystem-AUS :hasEstimationMethod :MeteredWaterData .

:RecycledWaterDelivery%3AIrrigation-AUS :hasEstimationMethod :MeteredWaterData .

:SupplySystemDelivery%3AIrrigation-AUS :hasEstimationMethod :MeteredWaterData .

:SupplySystemDischarge%3ASurfaceWater-AUS :hasEstimationMethod :MeteredWaterData .

:WastewaterAndRecycledWaterDischarge%3ASurfaceWater-AUS :hasEstimationMethod :MeteredWaterData .

:WastewaterDischarge%3ASurfaceWater-AUS :hasEstimationMethod :MeteredWaterData .

:GroundwaterExtraction-CA :hasParameter :AppliedWater-CA, :AppliedWaterReuse%2FRecycledWater-CA,
    :SurfaceWaterDelivery-CA .

:MunicipalConsumptiveUse-WY :hasParameter :GallonsPerCapitaPerDay%28GPCD%29, :Population .

:MunicipalTotalUse-WY :hasParameter :GallonsPerCapitaPerDay%28GPCD%29, :Population .

:SurfaceWaterDiversions-CA :hasParameter :AgriculturalAppliedWater-CA, :ConveyanceEvaporation-CA,
    :ManagedWetlandAppliedWater-CA, :OperationalSpill, :UrbanAppliedWater-CA .

:AgriculturalAndMunicipalDiversions-UT :hasParameter :USGSMeanAnnualReachEstimates .

:WYConsumptiveUseMethod :hasParameter :ClimateCoefficient%28kt%29, :CropGrowthStateCoefficient%28Kc%29,
    :CropIrrigationRequirement, :CropType, :EffectivePrecipitation, :IrrigatedAcreage,
    :IrrigationMethod, :MeanMonthlyAirTemperatures%28T%29, :MonthlyPercentageOfAnnualDaylightHours%28P%29,
    :PotentialConsumptiveUse, :SolarRadiation, :SupplySource, :SupplyStructure, :Temperature,
    :VaporPressure, :WaterSupply, :WindRun .

:Evapotranspiration-CA :hasParameter :AcreageByCropType, :CropGrowthStateCoefficient%28Kc%29,
    :IrrigationEfficiency, :ReferenceCropET%28ETo%29, :WaterDutyRateByCrop .

:IrrigationSurfaceWaterDiversions-WY :hasParameter :Diversions .

:TotalDiversions-WY :hasParameter :Diversions, :DivertibleFlow-WY .

:UTConsumptiveUseMethod :hasParameter :AgriculturalPotentialConsumptiveUse-UT, :ClimateCoefficient%28kt%29,
    :CropGrowthStateCoefficient%28Kc%29, :CropIrrigationRequirement, :CropType, :EffectivePrecipitation,
    :IrrigatedAcreage, :IrrigationMethod, :MeanMonthlyAirTemperatures%28T%29, :MonthlyPercentageOfAnnualDaylightHours%28P%29,
    :SolarRadiation, :Temperature, :VaporPressure, :WaterSupply, :WindRun .

:SurfaceDiversionToCropland-UT :hasParameter :USGSMeanAnnualReachEstimates .

:AgriculturalPotentialConsumptiveUse-UT :hasParameter :ClimateCoefficient%28kt%29,
    :CropGrowthStateCoefficient%28Kc%29, :MeanMonthlyAirTemperatures%28T%29, :MonthlyPercentageOfAnnualDaylightHours%28P%29,
    :SolarRadiation, :Temperature, :VaporPressure, :WindRun .

:DailyPenman-Monteith :hasParameter :SolarRadiation, :Temperature, :VaporPressure,
    :WindRun .

:ModifiedBlaney-Criddle :hasParameter :ClimateCoefficient%28kt%29, :CropGrowthStateCoefficient%28Kc%29,
    :MeanMonthlyAirTemperatures%28T%29, :MonthlyPercentageOfAnnualDaylightHours%28P%29 .

:AreaOutflows :hasParameter :USGSMeanAnnualReachEstimates .

:BasinOutflow-UT :hasParameter :USGSMeanAnnualReachEstimates .

:StreamOutfow-CA :hasParameter :DailyMaxAndMinAirTemperature, :DailyPrecipitation,
    :DailyShort-WaveSolarRadiation, :DescriptiveDataOfTopography%2CSoils%2CAndVegetation,
    :DrainageAreaOfSiteOfInterest, :DrainageAreaOfStreamflowGagingStation%28Ax%29, :MeasureStreamflow%28Xij%29 .

:HistoricalData :hasParameter :Diversions .

:BasinInflow-UT :hasParameter :USGSMeanAnnualReachEstimates .

:RiverInflow-UT :hasParameter :USGSMeanAnnualReachEstimates .

:StreamInflow-CA :hasParameter :DailyMaxAndMinAirTemperature, :DailyPrecipitation,
    :DailyShort-WaveSolarRadiation, :DescriptiveDataOfTopography%2CSoils%2CAndVegetation,
    :DrainageAreaOfSiteOfInterest, :DrainageAreaOfStreamflowGagingStation%28Ax%29, :MeasureStreamflow%28Xij%29 .

:COConsumptiveUseMethod :hasParameter :ClimateCoefficient%28kt%29, :CropGrowthStateCoefficient%28Kc%29,
    :CropIrrigationRequirement, :CropType, :EffectivePrecipitation, :IrrigatedAcreage,
    :IrrigationMethod, :MeanMonthlyAirTemperatures%28T%29, :MonthlyPercentageOfAnnualDaylightHours%28P%29,
    :PotentialConsumptiveUse, :Precipitation, :SolarRadiation, :SupplySource, :SupplyType,
    :Temperature, :WaterSupply, :WindRun .

:COIrrigatedAcreageAssessment :hasParameter :CropType, :IrrigationMethod, :SupplySource,
    :SupplyType .

:CropIrrigationRequirementEstimationMethod :hasParameter :AgriculturalPotentialConsumptiveUse-UT,
    :EffectivePrecipitation, :PotentialConsumptiveUse .

:ModifiedBlaney-CriddleWithETElevationAdjustment :hasParameter :CropGrowthStateCoefficient%28Kc%29,
    :SumOfMonthlyConsumptiveUseFactorsForGrowingSeason%28F%29 .

:On-FarmWaterBalance :hasParameter :CropIrrigationRequirement, :WaterSupply .

:OriginalBlaney-Criddle :hasParameter :MeanMonthlyAirTemperatures%28T%29, :MonthlyPercentageOfAnnualDaylightHours%28P%29 .

:OriginalBlaney-CriddleWithETElevationAdjustment :hasParameter :CropGrowthStateCoefficient%28Kc%29,
    :SumOfMonthlyConsumptiveUseFactorsForGrowingSeason%28F%29 .

:StateCU :hasParameter :CropType, :Diversions, :IrrigatedAcreage .

:CropIrrigationRequirement :hasParameter :AgriculturalPotentialConsumptiveUse-UT,
    :EffectivePrecipitation, :PotentialConsumptiveUse .

:EffectivePrecipitation :hasParameter :EffectivePrecipitationFactor, :Precipitation .

:IrrigatedAcreage :hasParameter :CropType, :IrrigationMethod, :SupplySource, :SupplyStructure,
    :SupplyType .

:PotentialConsumptiveUse :hasParameter :ClimateCoefficient%28kt%29, :CropGrowthStateCoefficient%28Kc%29,
    :MeanMonthlyAirTemperatures%28T%29, :MonthlyPercentageOfAnnualDaylightHours%28P%29,
    :SolarRadiation, :Temperature, :VaporPressure, :WindRun .

:COLivestockMethod :hasParameter :AverageUseRate, :LivestockCount .

:COMunicipalAndIndustrialMethod :hasParameter :ConsumptiveRatio, :GrossUsage, :Population .

:CONativeVegetationMethod :hasParameter :Diversions, :NativeVegetationCoefficient,
    :ReturnFlow .

:ChangeInGroundwaterStorage-CA :hasParameter :BudgetZoneArea, :ConveyanceSeepage-CA,
    :GroundwaterElevation, :GroundwaterExport-CA, :GroundwaterExtraction-CA, :LakeGainFromGroundwater-CA,
    :LakeLossToGroundwater-CA, :ManagedAquiferRecharge-CA, :RechargeOfAppliedWater-CA,
    :RechargeOfPrecipitation-CA, :SpecificYield, :StoredWaterExtraction-CA, :StreamGainFromGroundwater-CA,
    :StreamLossToGroundwater-CA, :SubsurfaceInflow-CA, :SubsurfaceOutflow-CA, :TotalGroundwaterSystemInflow-CA,
    :TotalGroundwaterSystemOutflow-CA .

:ChangeInLandSystemStorage-CA :hasParameter :ChangeInPondedWaterStorage, :ChangeInRootZoneSoilMoisture,
    :ChangeInSoilMoisture, :ChangeInUnsaturatedZoneStorage, :TotalLandSystemInflow-CA,
    :TotalLandSystemOutflow-CA .

:ChangeInSurfaceWaterStorage-AUS :hasParameter :WaterLevel .

:ChangeInSurfaceWaterStorage-CA :hasParameter :LakeGainFromGroundwater-CA, :LakeInflowFromStreams-CA,
    :LakeLossToGroundwater-CA, :LakeOutflowToStreams-CA, :Precipitation-CA .

:ColoradoStateMod :hasParameter :Baseflow, :DirectFlowDemand-Annual, :DirectFlowDemand-Monthly,
    :Evaporation, :InstreamFlowDemand-Annual, :InstreamFlowDemand-Monthly, :Precipitation,
    :ReservoirTargets, :Streamflow, :WellDemand-Monthly .

:MunicipalAndIndustrialDiversions-UT :hasParameter :USGSMeanAnnualReachEstimates .

:ConveyanceEvaporation-CA :hasParameter :ConveyanceSeepage-CA, :Evapotranspiration-CA,
    :ImportedWater-CA, :SurfaceWaterDelivery-CA, :SurfaceWaterDiversions-CA .

:ConveyanceSeepage-CA :hasParameter :ConveyanceEvaporation-CA, :ImportedWater-CA,
    :SurfaceWaterDelivery-CA, :SurfaceWaterDiversions-CA .

:DailyASCEStandardizedPenman-Monteith :hasParameter :SolarRadiation, :Temperature,
    :VaporPressure, :WindRun .

:DailyModifiedHargreaves :hasParameter :SolarRadiation, :Temperature, :WindRun .

:DomesticTotalUse-WY :hasParameter :GallonsPerCapitaPerDay%28GPCD%29, :Population .

:WithdrawalMethod :hasParameter :GallonsPerCapitaPerDay%28GPCD%29, :LivestockPopulation,
    :Population, :PopulationServedByPublicWaterSupply, :SelfSuppliedDomesticPopulation,
    :StudentPopulation .

:UTEffectivePrecipitationMethod :hasParameter :Precipitation .

:Elevation-Area-CapacityTables :hasParameter :WaterLevel .

:EmpiricalDataForSmallReservoirs :hasParameter :AnnualEvaporation, :MonthlyPrecipitationVolume,
    :Rainfall, :ReservoirSurfaceArea .

:EvaporationFromReservoirs-NMOSE :hasParameter :AnnualEvaporation, :AverageMonthlyReservoirGageHeight,
    :ClassAPanEvaporationData, :MonthlyEvaporation, :MonthlyGrossEvaporationRate, :MonthlyPrecipitationVolume,
    :Rainfall, :ReservoirSurfaceArea, :WinterIceSurfaceArea .

:PanApproach :hasParameter :AnnualEvaporation, :AverageMonthlyReservoirGageHeight,
    :ClassAPanEvaporationData, :MonthlyEvaporation, :MonthlyGrossEvaporationRate, :Rainfall,
    :ReservoirSurfaceArea, :WinterIceSurfaceArea .

:LakeEvaporation-CA :hasParameter :MassTransferCoefficient, :MeasuredPanEvaporationRate,
    :PanCoefficient, :SaturationVaporPressure, :SurfaceAreaOfWaterBody, :VaporPressure,
    :WindFunction .

:GroundwaterExport-CA :hasParameter :AppliedWater-CA, :AppliedWaterReuse%2FRecycledWater-CA,
    :ConveyanceEvaporation-CA, :SurfaceWaterDelivery-CA .

:SurfaceWaterExports-CA :hasParameter :AgriculturalAppliedWater-CA, :ManagedWetlandAppliedWater-CA,
    :UrbanAppliedWater-CA .

:SubsurfaceInflow-CA :hasParameter :Cross-sectionalAreaSubjectToBoundaryFlow%28Ab%29,
    :DepthOfCrossSection%28b%29, :DistanceBetweenTwoPointsWithKnownHead%28I%29, :HydraulicConductivityOfTheAquiferBoundary%28K%29,
    :HydraulicGradientThroughTheCrossSection%28i%29, :KnownGroundwaterElevationInsideTheBoundary%28hg%29,
    :KnownGroundwaterElevationOutsideTheBoundary%28hb%29, :SubsurfaceFlowAcrossTheBoundary%28Qb%29,
    :TransmissivityOfTheAquiferAtTheBoundary%28T%29, :WidthOfCrossSection%28w%29 .

:SubsurfaceOutflow-CA :hasParameter :Cross-sectionalAreaSubjectToBoundaryFlow%28Ab%29,
    :DepthOfCrossSection%28b%29, :DistanceBetweenTwoPointsWithKnownHead%28I%29, :HydraulicConductivityOfTheAquiferBoundary%28K%29,
    :HydraulicGradientThroughTheCrossSection%28i%29, :KnownGroundwaterElevationInsideTheBoundary%28hg%29,
    :KnownGroundwaterElevationOutsideTheBoundary%28hb%29, :SubsurfaceFlowAcrossTheBoundary%28Qb%29,
    :TransmissivityOfTheAquiferAtTheBoundary%28T%29, :WidthOfCrossSection%28w%29 .

:LakeGainFromGroundwater-CA :hasParameter :BottomElevationOfTheLakebedSediments%28HlakebedBottom%29,
    :ChangeInLakeStorage, :DistanceBetweenTwoPointsWithKnownHead%28I%29, :FlowThroughAVerticalPlaneThatExtendsBeneathTheShorelineOfASurfaceWaterBody%28Q%29,
    :GroundwaterLevel%28Haquifer%29, :HorizonalHydraulicConductivityOfTheAquiferAtTheBoundary%28K%29,
    :LakeEvaporation-CA, :LakeInflowFromStreams-CA, :LakeOutflowToStreams-CA, :NumberOfEquipotentialHeadDropsOverTheAreaOfInterest%28n%29,
    :NumberOfStreamtubesAcrossAFlowNet%28M%29, :PrecipitationOnLakes-CA, :SurfaceAreaOfLake%28Al%29,
    :TotalHeadDropAcrossTheAreaOfInterest%28H%29, :VerticalHydraulicConductivityOfTheSurroundingAquifer%28Kv%29,
    :WaterLevelInLake%28Hlake%29, :WettedPerimeterOfLakeMultipliedByTheAverageSaturatedThicknessOfAquiferAroundTheLake%28Awpl%29 .

:GroundwaterUse-UT :hasParameter :GroundwaterUse .

:ImportedWater-CA :hasParameter :AgriculturalAppliedWater-CA, :ManagedWetlandAppliedWater-CA,
    :OperationalSpill, :UrbanAppliedWater-CA .

:IndicatorGageApproach :hasParameter :Streamflow .

:Industrial-NMOSE :hasParameter :Flow .

:Metered :hasParameter :Flow .

:IndustrialConsumptiveUse-WY :hasParameter :AnnualEmployeeHours, :AnnualSodaAshProduction,
    :CoalProductionQuantities, :ElectricalGenerationData, :MonthlyCoalbedMethaneGasProductionAndProducedWater,
    :MonthlyOil%2CGas%2CAndProducedWater, :NaturalGasProcessingVolumes, :Population .

:IndustrialTotalUse-WY :hasParameter :AnnualEmployeeHours, :AnnualSodaAshProduction,
    :CoalProductionQuantities, :ElectricalGenerationData, :MonthlyCoalbedMethaneGasProductionAndProducedWater,
    :MonthlyOil%2CGas%2CAndProducedWater, :NaturalGasProcessingVolumes, :Population .

:SurfaceWaterDelivery-CA :hasParameter :AppliedWaterReuse%2FRecycledWater-CA, :GroundwaterExtraction-CA .

:Inter-regionCoastalInflow-AUS :hasParameter :AquiferAttribution, :AquiferThickness,
    :BoreLocation, :GroundwaterLevel, :HydraulicConductivity .

:Inter-regionCoastalOutflow-AUS :hasParameter :AquiferAttribution, :AquiferThickness,
    :BoreLocation, :GroundwaterLevel, :HydraulicConductivity .

:NMIrrigatedAcreageAssessment :hasParameter :CropType, :IrrigationMethod, :SupplyStructure .

:USBRIrrigatedAcreageAssessment :hasParameter :CropType .

:UTIrrigatedAcreageAssessment :hasParameter :CropType, :IrrigationMethod .

:WYIrrigatedAcreageAssessment :hasParameter :CropType, :IrrigationMethod, :SupplySource,
    :SupplyStructure .

:NMConsumptiveUseMethod :hasParameter :ClimateCoefficient%28kt%29, :CropGrowthStateCoefficient%28Kc%29,
    :CropIrrigationRequirement, :CropType, :EffectivePrecipitation, :IrrigatedAcreage,
    :IrrigationMethod, :MeanMonthlyAirTemperatures%28T%29, :MonthlyPercentageOfAnnualDaylightHours%28P%29,
    :PotentialConsumptiveUse, :Precipitation, :SolarRadiation, :Streamflow, :SupplyStructure,
    :Temperature, :WaterSupply, :WindRun .

:IrrigatedAgricultureDiversions-NMOSE :hasParameter :ConsumptiveIrrigationRequirement%28CIR%29,
    :GrossActivelyIrrigatedAcreage, :MeanMonthlyAirTemperatures%28T%29, :MonthlyPrecipitationVolume .

:LakeLossToGroundwater-CA :hasParameter :BottomElevationOfTheLakebedSediments%28HlakebedBottom%29,
    :ChangeInLakeStorage, :DistanceBetweenTwoPointsWithKnownHead%28I%29, :EffectiveThicknessOfTheAquifer%28b%29,
    :FlowThroughAVerticalPlaneThatExtendsBeneathTheShorelineOfASurfaceWaterBody%28Q%29,
    :GroundwaterLevel%28Haquifer%29, :HorizonalHydraulicConductivityOfTheAquiferAtTheBoundary%28K%29,
    :LakeEvaporation-CA, :LakeInflowFromStreams-CA, :LakeOutflowToStreams-CA, :NumberOfEquipotentialHeadDropsOverTheAreaOfInterest%28n%29,
    :NumberOfStreamtubesAcrossAFlowNet%28M%29, :PrecipitationOnLakes-CA, :SurfaceAreaOfLake%28Al%29,
    :TotalHeadDropAcrossTheAreaOfInterest%28H%29, :VerticalHydraulicConductivityOfTheSurroundingAquifer%28Kv%29,
    :WaterLevelInLake%28Hlake%29, :WettedPerimeterOfLakeMultipliedByTheAverageSaturatedThicknessOfAquiferAroundTheLake%28Awpl%29 .

:Industrial%3AMineProduction-WY :hasParameter :AnnualEmployeeHours, :CoalProductionQuantities .

:ReturnFlow-CA :hasParameter :AppliedWaterReuse%2FRecycledWater-CA, :Evapotranspiration-CA,
    :StreamLossToGroundwater-CA, :TotalGroundwaterSystemInflow-CA, :TotalSurfaceWaterInflow-CA .

:OriginalHargreaves :hasParameter :SolarRadiation, :Temperature .

:NMIrrigationWithdrawals :hasParameter :ConsumptiveIrrigationRequirement%28CIR%29,
    :GrossActivelyIrrigatedAcreage, :MeanMonthlyAirTemperatures%28T%29, :MonthlyPrecipitationVolume .

:NaturalFlowGainDistribution :hasParameter :GageHeight, :ProrationFactors .

:Outflow-AUS :hasParameter :FlowData .

:PersonalOutreach :hasParameter :WaterUseEstimate .

:Industrial%3AElectricalGeneration-WY :hasParameter :ElectricalGenerationData .

:RechargeOfAppliedWater-CA :hasParameter :AppliedWater-CA, :AppliedWaterReuse%2FRecycledWater-CA,
    :ConsumptiveUseOfPrecipitation%28EP%29, :Evapotranspiration-CA, :RecycledWaterExport-CA,
    :ReturnFlow-CA, :UrbanAppliedWater-CA .

:RechargeOfPrecipitation-CA :hasParameter :ConsumptiveUseOfPrecipitation%28EP%29,
    :Precipitation-CA, :Runoff-CA .

:ReservoirEstimationMethod :hasParameter :GrossMonthlyFreeWaterSurfaceEvaporation,
    :MonthlyEffectivePrecipitation, :SurfaceAreaOfReservoir .

:ReservoirEvaporation-WY :hasParameter :GrossPanEvaportation%28inches%29, :Precipitation .

:PanMethod%28NetEvaporation%29 :hasParameter :GrossPanEvaportation%28inches%29, :Precipitation .

:Runoff-CA :hasParameter :Precipitation .

:Self-SuppliedDomestic-NMOSE :hasParameter :GallonsPerCapitaPerDay%28GPCD%29, :SelfSuppliedDomesticPopulation .

:StreamEvaporation-CA :hasParameter :SaturationVaporPressure, :StreamInflow-CA, :StreamOutfow-CA,
    :VaporPressure, :WindFunction .

:StreamGainFromGroundwater-CA :hasParameter :AverageThicknessOfStreambed%28Bstream%29,
    :BottomElevationOfStreambedSediments%28HstreambedBottom%29, :EffectiveAreaOfFlowExchange%28Awps%29,
    :EffectiveThicknessOfTheAquifer%28b%29, :FlowThroughAVerticalPlaneThatExtendsBeneathTheShorelineOfASurfaceWaterBody%28Q%29,
    :GroundwaterLevel%28Haquifer%29, :HorizonalHydraulicConductivityOfTheAquiferAtTheBoundary%28K%29,
    :HydraulicConductivityOfTheStreambedMaterial%28Ks%29, :InflowFromContributingOrTributaryStreams,
    :NumberOfEquipotentialHeadDropsOverTheAreaOfInterest%28n%29, :NumberOfStreamtubesAcrossAFlowNet%28M%29,
    :ReturnFlow-CA, :Runoff-CA, :StreamEvaporation-CA, :StreamflowAtDownstreamGauge, :StreamflowAtUpstreamGauge,
    :SurfaceWaterDiversions-CA, :TotalHeadDropAcrossTheAreaOfInterest%28H%29, :WaterStageInStream%28Hstream%29 .

:StreamLossToGroundwater-CA :hasParameter :AverageThicknessOfStreambed%28Bstream%29,
    :BottomElevationOfStreambedSediments%28HstreambedBottom%29, :EffectiveAreaOfFlowExchange%28Awps%29,
    :EffectiveThicknessOfTheAquifer%28b%29, :FlowThroughAVerticalPlaneThatExtendsBeneathTheShorelineOfASurfaceWaterBody%28Q%29,
    :GroundwaterLevel%28Haquifer%29, :HorizonalHydraulicConductivityOfTheAquiferAtTheBoundary%28K%29,
    :HydraulicConductivityOfTheStreambedMaterial%28Ks%29, :InflowFromContributingOrTributaryStreams,
    :NumberOfEquipotentialHeadDropsOverTheAreaOfInterest%28n%29, :NumberOfStreamtubesAcrossAFlowNet%28M%29,
    :ReturnFlow-CA, :Runoff-CA, :StreamEvaporation-CA, :StreamflowAtDownstreamGauge, :StreamflowAtUpstreamGauge,
    :SurfaceWaterDiversions-CA, :TotalHeadDropAcrossTheAreaOfInterest%28H%29, :WaterStageInStream%28Hstream%29 .

:SurfaceWaterFlows-UT :hasParameter :USGSMeanAnnualReachEstimates .

:TributaryInflow-UT :hasParameter :USGSMeanAnnualReachEstimates .

:USBRConsumptiveUseMethod :hasParameter :ClimateCoefficient%28kt%29, :CropGrowthStateCoefficient%28Kc%29,
    :CropIrrigationRequirement, :CropType, :EffectivePrecipitation, :IrrigatedAcreage,
    :MeanMonthlyAirTemperatures%28T%29, :MonthlyPercentageOfAnnualDaylightHours%28P%29,
    :PotentialConsumptiveUse, :SolarRadiation, :Temperature, :VaporPressure, :WaterSupply,
    :WindRun .

:UngagedStreamGains-WY :hasParameter :DownstreamFlow, :UpstreamFlow .

:WyomingGain%2FLossEstimationMethod :hasParameter :DownstreamFlow, :UpstreamFlow .

:UngagedStreamLosses-WY :hasParameter :DownstreamFlow, :UpstreamFlow .

:WYAgricultureConsumptiveUseEstimationMethod :hasParameter :IrrigatedAcreage, :NDVI,
    :StateCUOutput .

:WYElectricalGenerationMethod :hasParameter :ElectricalGenerationData .

:WYIndustrialProductionMethod :hasParameter :MonthlyCoalbedMethaneGasProductionAndProducedWater,
    :MonthlyOil%2CGas%2CAndProducedWater, :NaturalGasProcessingVolumes .

:WYIrrigatedAcreageConsumptiveUseModel :hasParameter :NDVI .

:WYMineProductionMethod :hasParameter :AnnualEmployeeHours, :CoalProductionQuantities .

:AllocatedDiversion%3AIndividualUsers-AUS :hasParameter :EntitlementVolume, :MeteredWaterData .

:Commercial%3AGolfCourses-NMOSE :hasParameter :ConsumptiveIrrigationRequirement%28CIR%29,
    :GrossActivelyIrrigatedAcreage, :MeanMonthlyAirTemperatures%28T%29, :MonthlyPrecipitationVolume .

:Commercial%3AUnmetered-NMOSE :hasParameter :WaterUseEstimate .

:Commercial%3AMetered-NMOSE :hasParameter :Flow .

:Commercial%3ASchools-NMOSE :hasParameter :GallonsPerCapitaPerDay%28GPCD%29, :StudentPopulation .

:Discharge%3ASurfaceWater-AUS :hasParameter :Baseflow .

:Diversions%3AStatutoryRights-AUS :hasParameter :AssumedDiversionRate, :RiparianWaterAuthorisations .

:Industrial%3ACoalbedMethandProduction-WY :hasParameter :MonthlyCoalbedMethaneGasProductionAndProducedWater .

:Industrial%3AMiscellaneous-WY :hasParameter :Population .

:Industrial%3ANaturalGas-WY :hasParameter :NaturalGasProcessingVolumes .

:Industrial%3AOilAndGas-WY :hasParameter :MonthlyOil%2CGas%2CAndProducedWater .

:Inter-regionInflow%3AGroundwater-AUS :hasParameter :AquiferAttribution, :AquiferThickness,
    :BoreLocation, :GroundwaterLevel, :HydraulicConductivity .

:Inter-regionOutflow%3AGroundwater-AUS :hasParameter :AquiferAttribution, :AquiferThickness,
    :BoreLocation, :GroundwaterLevel, :HydraulicConductivity .

:Leakage%3AGroundwater-AUS :hasParameter :ApparentLosses, :UnmeteredAuthorisedConsumption .

:Leakage%3AUrbanSystem-AUS :hasParameter :ApparentLosses, :EstimatedNon-revenueWaterVolumes,
    :UnmeteredAuthorisedConsumption .

:Livestock%3AMetered-NMOSE :hasParameter :Flow .

:Livestock%3AUnmetered-NMOSE :hasParameter :GallonsPerCapitaPerDay%28GPCD%29, :LivestockPopulation .

:Mining%3AUnreported-NMOSE :hasParameter :WaterUseEstimate .

:Non-allocatedDiversion%3AUrbanSystem-AUS :hasParameter :InflowToWaterTreatmentPlants,
    :SAWater%27sTotalLicensedDiversionVolumeFromWesternMountLoftyRangesPWRA .

:Power%3AUnreported-NMOSE :hasParameter :WaterUseEstimate .

:PublicWaterSupply%3AMetered-NMOSE :hasParameter :Flow .

:PublicWaterSupply%3AUnmetered-NMOSE :hasParameter :GallonsPerCapitaPerDay%28GPCD%29,
    :PopulationServedByPublicWaterSupply .

:AgriculturalAppliedWater-CA :hasParameter :AcreageByCropType, :AppliedWater-CA, :AppliedWaterReuse%2FRecycledWater-CA,
    :CropETRequirements, :ETOfAppliedWater, :GroundwaterExtraction-CA, :IrrigationEfficiency,
    :IrrigationRecharge, :PrecipitationVolumeForAgriculturalArea, :ReturnFlow-CA, :RunoffVolume,
    :SurfaceWaterDelivery-CA, :WaterDutyRateByCrop .

:CropETApproach :hasParameter :AppliedWater-CA, :AppliedWaterReuse%2FRecycledWater-CA,
    :CropETRequirements, :ETOfAppliedWater, :GroundwaterExtraction-CA, :IrrigationEfficiency,
    :IrrigationRecharge, :PrecipitationVolumeForAgriculturalArea, :ReturnFlow-CA, :RunoffVolume,
    :SurfaceWaterDelivery-CA .

:Water-DutyBasedApproach :hasParameter :AcreageByCropType, :IrrigationEfficiency,
    :WaterDutyRateByCrop .

:ChangeInGroundwaterLevel :hasParameter :BudgetZoneArea, :GroundwaterElevation, :SpecificYield .

:MassBalance :hasParameter :ChangeInLakeStorage, :ConveyanceSeepage-CA, :GroundwaterExport-CA,
    :GroundwaterExtraction-CA, :ImportedWater-CA, :InflowFromContributingOrTributaryStreams,
    :LakeEvaporation-CA, :LakeGainFromGroundwater-CA, :LakeInflowFromStreams-CA, :LakeLossToGroundwater-CA,
    :LakeOutflowToStreams-CA, :ManagedAquiferRecharge-CA, :PrecipitationOnLakes-CA, :RechargeOfAppliedWater-CA,
    :RechargeOfPrecipitation-CA, :ReturnFlow-CA, :Runoff-CA, :StoredWaterExtraction-CA,
    :StreamEvaporation-CA, :StreamGainFromGroundwater-CA, :StreamInflow-CA, :StreamLossToGroundwater-CA,
    :StreamOutfow-CA, :StreamflowAtDownstreamGauge, :StreamflowAtUpstreamGauge, :SubsurfaceInflow-CA,
    :SubsurfaceOutflow-CA, :SurfaceWaterDelivery-CA, :SurfaceWaterDiversions-CA, :TotalGroundwaterSystemInflow-CA,
    :TotalGroundwaterSystemOutflow-CA .

:WaterBalanceForUnsaturatedZoneStorage :hasParameter :ChangeInPondedWaterStorage,
    :ChangeInRootZoneSoilMoisture, :ChangeInUnsaturatedZoneStorage .

:WaterUseModels :hasParameter :ChangeInSoilMoisture .

:LakeInflowFromStreams-CA :hasParameter :ChangeInSurfaceWaterStorage-CA, :LakeEvaporation-CA,
    :LakeGainFromGroundwater-CA, :LakeLossToGroundwater-CA, :Precipitation-CA .

:LakeOutflowToStreams-CA :hasParameter :ChangeInSurfaceWaterStorage-CA, :LakeEvaporation-CA,
    :LakeGainFromGroundwater-CA, :LakeLossToGroundwater-CA, :Precipitation-CA .

:Evapotranspiration%28ET%29Rates :hasParameter :Evapotranspiration-CA .

:CropCoefficientApproach :hasParameter :AcreageByCropType, :CropGrowthStateCoefficient%28Kc%29,
    :ReferenceCropET%28ETo%29 .

:DrainageAreaRatioMethod :hasParameter :DrainageAreaOfSiteOfInterest, :DrainageAreaOfStreamflowGagingStation%28Ax%29,
    :MeasureStreamflow%28Xij%29 .

:EstimateAppliedWaterReuseAndRecycledWaterVolumes :hasParameter :AppliedWater-CA,
    :GroundwaterExtraction-CA, :SurfaceWaterDelivery-CA .

:EvaporationPanMethod :hasParameter :MeasuredPanEvaporationRate, :PanCoefficient,
    :SurfaceAreaOfWaterBody .

:FlowNetAnalysis :hasParameter :EffectiveThicknessOfTheAquifer%28b%29, :FlowThroughAVerticalPlaneThatExtendsBeneathTheShorelineOfASurfaceWaterBody%28Q%29,
    :HorizonalHydraulicConductivityOfTheAquiferAtTheBoundary%28K%29, :NumberOfEquipotentialHeadDropsOverTheAreaOfInterest%28n%29,
    :NumberOfStreamtubesAcrossAFlowNet%28M%29, :TotalHeadDropAcrossTheAreaOfInterest%28H%29 .

:GISGroundwaterModelling :hasParameter :AquiferAttribution, :AquiferThickness, :BoreLocation,
    :Darcy%27sLaw, :GroundwaterLevel, :HydraulicConductivity .

:PortPhillipCatchmentManagementAuthorityGroundwaterModel :hasParameter :AquiferAttribution,
    :AquiferThickness, :BoreLocation, :GroundwaterLevel, :HydraulicConductivity .

:Darcy%27sLaw :hasParameter :AverageThicknessOfStreambed%28Bstream%29, :BottomElevationOfStreambedSediments%28HstreambedBottom%29,
    :BottomElevationOfTheLakebedSediments%28HlakebedBottom%29, :Cross-sectionalAreaSubjectToBoundaryFlow%28Ab%29,
    :DepthOfCrossSection%28b%29, :DistanceBetweenTwoPointsWithKnownHead%28I%29, :EffectiveAreaOfFlowExchange%28Awps%29,
    :GroundwaterLevel%28Haquifer%29, :HydraulicConductivityOfTheAquiferBoundary%28K%29,
    :HydraulicConductivityOfTheStreambedMaterial%28Ks%29, :HydraulicGradientThroughTheCrossSection%28i%29,
    :KnownGroundwaterElevationInsideTheBoundary%28hg%29, :KnownGroundwaterElevationOutsideTheBoundary%28hb%29,
    :SubsurfaceFlowAcrossTheBoundary%28Qb%29, :SurfaceAreaOfLake%28Al%29, :TransmissivityOfTheAquiferAtTheBoundary%28T%29,
    :VerticalHydraulicConductivityOfTheSurroundingAquifer%28Kv%29, :WaterLevelInLake%28Hlake%29,
    :WaterStageInStream%28Hstream%29, :WettedPerimeterOfLakeMultipliedByTheAverageSaturatedThicknessOfAquiferAroundTheLake%28Awpl%29,
    :WidthOfCrossSection%28w%29 .

:LandUseAndAppliedWaterEstimationMethod :hasParameter :AgriculturalAppliedWater-CA,
    :AppliedWater-CA, :AppliedWaterReuse%2FRecycledWater-CA, :ConsumptiveUseOfPrecipitation%28EP%29,
    :ConveyanceEvaporation-CA, :Evapotranspiration-CA, :GroundwaterExtraction-CA, :ManagedWetlandAppliedWater-CA,
    :OperationalSpill, :RecycledWaterExport-CA, :ReturnFlow-CA, :SurfaceWaterDelivery-CA,
    :UrbanAppliedWater-CA .

:ManagedWetlandAppliedWater-CA :hasParameter :CulturalPractices, :HabitatAcreage,
    :UnitETOfAppliedWater .

:UrbanAppliedWater-CA :hasParameter :GallonsPerCapitaPerDay%28GPCD%29, :IndustrialWaterUse,
    :LandscapeIrrigation, :Population .

:MassTransferEquations :hasParameter :MassTransferCoefficient, :SaturationVaporPressure,
    :VaporPressure, :WindFunction .

:LyneAndHollickFilter :hasParameter :Baseflow .

:ManagedWetlandsAppliedWaterEstimation :hasParameter :CulturalPractices, :HabitatAcreage,
    :UnitETOfAppliedWater .

:RealLossesEquation :hasParameter :ApparentLosses, :EstimatedNon-revenueWaterVolumes,
    :UnmeteredAuthorisedConsumption .

:PopulationAndPer-CapitaWaterUse :hasParameter :GallonsPerCapitaPerDay%28GPCD%29,
    :IndustrialWaterUse, :LandscapeIrrigation, :Population .

:Rainfall-RunoffMethod :hasParameter :ConsumptiveUseOfPrecipitation%28EP%29, :Precipitation-CA,
    :Runoff-CA .

:ReturnFlowEstimationMethod :hasParameter :AppliedWaterReuse%2FRecycledWater-CA, :Evapotranspiration-CA,
    :StreamLossToGroundwater-CA, :TotalGroundwaterSystemInflow-CA, :TotalSurfaceWaterInflow-CA .

:RunoffCurveNumberMethod :hasParameter :Precipitation .

:Precipitation-RunoffModelingSystem%28PRMS%29 :hasParameter :DailyMaxAndMinAirTemperature,
    :DailyPrecipitation, :DailyShort-WaveSolarRadiation, :DescriptiveDataOfTopography%2CSoils%2CAndVegetation .

:SAWaterStorageVolumeRelationship :hasParameter :WaterLevel .

:Non-allocatedDiversion%3AUrbanWaterSystemEstimationMethod :hasParameter :InflowToWaterTreatmentPlants,
    :SAWater%27sTotalLicensedDiversionVolumeFromWesternMountLoftyRangesPWRA .

:AgriculturalAndMunicipalDepletions-UT :isFlowType :Outflow .

:CropConsumptiveUse-CO :isFlowType :Outflow .

:GroundwaterExtraction-CA :isFlowType :InternalTransfer .

:LivestockConsumptiveUse-CO :isFlowType :Outflow .

:MunicipalAndIndustrialConsumptiveUse-CO :isFlowType :Outflow .

:SurfaceWaterDiversions-CA :isFlowType :InternalTransfer .

:AgriculturalAndMunicipalDiversions-UT :isFlowType :InternalTransfer .

:AppliedWater-CA :isFlowType :InternalTransfer .

:Evapotranspiration-CA :isFlowType :Outflow .

:IrrigationSurfaceWaterDiversions-WY :isFlowType :InternalTransfer .

:TotalDiversions-WY :isFlowType :InternalTransfer .

:AgriculturalDepletions-UT :isFlowType :Outflow .

:SurfaceDiversionToCropland-UT :isFlowType :InternalTransfer .

:AgriculturalPotentialConsumptiveUse-UT :isFlowType :InternalTransfer .

:AreaOutflows :isFlowType :Outflow .

:BasinOutflow-UT :isFlowType :Outflow .

:GagedStreamOutflow-WY :isFlowType :Outflow .

:StreamOutfow-CA :isFlowType :Outflow .

:Exports-CO :isFlowType :Outflow .

:BasinInflow-UT :isFlowType :Inflow .

:RiverInflow-UT :isFlowType :Inflow .

:GagedStreamInflow-WY :isFlowType :Inflow .

:UngagedSurfaceWaterInflow-CO :isFlowType :Inflow .

:StreamInflow-CA :isFlowType :Inflow .

:ChangeInGroundWaterStorage-CO :isFlowType :StorageChange .

:ChangeInGroundwaterStorage-CA :isFlowType :StorageChange .

:ChangeInGroundwaterStorage-AUS :isFlowType :StorageChange .

:ChangeInTotalSystemStorage-CA :isFlowType :StorageChange .

:ChangeInLandSystemStorage-CA :isFlowType :StorageChange .

:ChangeInSurfaceWaterStorage-AUS :isFlowType :StorageChange .

:ChangeInSurfaceWaterStorage-CA :isFlowType :StorageChange .

:ChangeInSurfaceWaterStorage-CO :isFlowType :StorageChange .

:Commercial-NMOSE :isFlowType :InternalTransfer .

:MunicipalAndIndustrialDiversions-UT :isFlowType :InternalTransfer .

:ConveyanceEvaporation-CA :isFlowType :Outflow .

:HumanConsumption-NM :isFlowType :Outflow .

:ConveyanceLossesForAllocatedDiversions-AUS :isFlowType :Outflow .

:SurfaceWaterOutflows-AUS :isFlowType :Outflow .

:ConveyanceSeepage-CA :isFlowType :InternalTransfer .

:TotalGroundwaterSystemInflow-CA :isFlowType :Inflow .

:CoplandPrecipitation-UT :isFlowType :Inflow .

:Precipitation-CA :isFlowType :Inflow .

:Precipitation-CO :isFlowType :Inflow .

:Precipitation-NM :isFlowType :Inflow .

:Precipitation-UT :isFlowType :Inflow .

:Precipitation-WY :isFlowType :Inflow .

:IrrigatedAgricultureDepletions-NMOSE :isFlowType :Outflow .

:Evaporation-AUS :isFlowType :Outflow .

:Evaporation-NM :isFlowType :Outflow .

:TotalEvaporation-NM :isFlowType :Outflow .

:EvaporationFromReservoirs-NMOSE :isFlowType :Outflow .

:LakeEvaporation-CA :isFlowType :Outflow .

:ReservoirEvaporation-CO :isFlowType :Outflow .

:ReservoirEvaporation-UT :isFlowType :Outflow .

:GroundwaterExport-CA :isFlowType :Outflow .

:StoredWaterExport-CA :isFlowType :Outflow .

:SurfaceWaterExports-CA :isFlowType :Outflow .

:FloodReturn-AUS :isFlowType :Inflow .

:SurfaceWaterInflows-AUS :isFlowType :Inflow, :InternalTransfer .

:GagedSurfaceWaterOutflow-CO :isFlowType :Outflow .

:GroundWaterInflow-CO :isFlowType :Inflow .

:SubsurfaceInflow-CA :isFlowType :Inflow .

:GroundWaterOutflow-CO :isFlowType :Outflow .

:TotalGroundwaterSystemOutflow-CA :isFlowType :Outflow .

:SubsurfaceOutflow-CA :isFlowType :Outflow .

:GroundwaterDischarge-AUS :isFlowType :Inflow .

:Discharge%3AGroundwater-AUS :isFlowType :InternalTransfer .

:GroundwaterDiversions-NM :isFlowType :InternalTransfer .

:GroundwaterET-NM :isFlowType :Outflow .

:RiparianConsumption-NM :isFlowType :Outflow .

:LakeGainFromGroundwater-CA :isFlowType :InternalTransfer .

:GroundwaterInflows-AUS :isFlowType :Inflow, :InternalTransfer .

:GroundwaterInflows-NM :isFlowType :Inflow .

:GroundwaterOutflows-AUS :isFlowType :Outflow .

:GroundwaterOutflows-NM :isFlowType :Outflow .

:GroundwaterReturn-NM :isFlowType :InternalTransfer .

:GroundwaterUse-UT :isFlowType :InternalTransfer .

:PumpedGroundwater-UT :isFlowType :InternalTransfer .

:ImportedWater-CA :isFlowType :Inflow .

:Imports-CO :isFlowType :Inflow .

:Industrial-NMOSE :isFlowType :InternalTransfer .

:IndustrialConsumptiveUse-WY :isFlowType :Outflow .

:IndustrialTotalUse-WY :isFlowType :InternalTransfer .

:SurfaceWaterDelivery-CA :isFlowType :InternalTransfer .

:Inter-regionCoastalInflow-AUS :isFlowType :Inflow .

:Inter-regionCoastalOutflow-AUS :isFlowType :Outflow .

:IrrigatedAgriculture-NMOSE :isFlowType :InternalTransfer, :Outflow .

:IrrigatedAgricultureDiversions-NMOSE :isFlowType :InternalTransfer .

:IrrigationSchemeInflows-AUS :isFlowType :Inflow .

:IrrigationSchemeOutflows-AUS :isFlowType :Outflow .

:LakeLossToGroundwater-CA :isFlowType :InternalTransfer .

:Recharge-NM :isFlowType :InternalTransfer .

:LandSurfaceExapotranspiration-NM :isFlowType :Outflow .

:Livestock-NMOSE :isFlowType :InternalTransfer .

:LivestockConsumptiveUse-WY :isFlowType :Outflow .

:ManagedAquiferRecharge-AUS :isFlowType :InternalTransfer .

:UrbanWaterSystemOutflows-AUS :isFlowType :Outflow .

:ManagedAquiferRecharge-CA :isFlowType :InternalTransfer .

:Mining-NMOSE :isFlowType :InternalTransfer .

:Industrial%3AMineProduction-WY :isFlowType :InternalTransfer .

:Power-NMOSE :isFlowType :InternalTransfer .

:PublicWaterSupply-NMOSE :isFlowType :InternalTransfer .

:MunicipalAndIndustrialDepeltion-UT :isFlowType :Outflow .

:MunicipalAndIndustrialReturnFlow-UT :isFlowType :InternalTransfer .

:ReturnFlow-CA :isFlowType :InternalTransfer .

:NativeVegetationConsumptiveUse-CO :isFlowType :Outflow .

:NaturalSystemUse-UT :isFlowType :Outflow .

:RiparianDepletions-UT :isFlowType :Outflow .

:Non-allocatedExtraction-AUS :isFlowType :Outflow .

:OtherStatutoryRights-AUS :isFlowType :Outflow .

:Outflow-AUS :isFlowType :Outflow .

:OverbankFloodSpilling-AUS :isFlowType :Outflow .

:OverbankFlow-AUS :isFlowType :Outflow .

:Precipitation-AUS :isFlowType :Inflow .

:PrecipitationOnLakes-CA :isFlowType :Inflow .

:RechargeOfAppliedWater-CA :isFlowType :InternalTransfer .

:RechargeOfPrecipitation-CA :isFlowType :InternalTransfer .

:RecycledWaterExport-CA :isFlowType :Outflow .

:ReservoirEvaporation-WY :isFlowType :Outflow .

:RiverAndFloodplainLosses-AUS :isFlowType :Outflow .

:RiverEvaporation-NM :isFlowType :Outflow .

:RiverUseByWetPasture-UT :isFlowType :InternalTransfer .

:Runoff-AUS :isFlowType :Inflow .

:Runoff-CA :isFlowType :InternalTransfer .

:Runoff-NM :isFlowType :InternalTransfer .

:Self-SuppliedDomestic-NMOSE :isFlowType :InternalTransfer .

:StoredWaterExtraction-CA :isFlowType :InternalTransfer .

:StreamEvaporation-CA :isFlowType :Outflow .

:StreamGainFromGroundwater-CA :isFlowType :InternalTransfer .

:StreamLossToGroundwater-CA :isFlowType :InternalTransfer .

:SurfaceWaterDiversions-NM :isFlowType :InternalTransfer .

:SurfaceWaterEvaporation-NM :isFlowType :Outflow .

:SurfaceWaterFlows-UT :isFlowType :InternalTransfer .

:SurfaceWaterGroundwaterInteractions-NM :isFlowType :InternalTransfer .

:SurfaceWaterInflows-NM :isFlowType :Inflow .

:SurfaceWaterOutflows-NM :isFlowType :Outflow .

:SurfaceWaterReturns-NM :isFlowType :InternalTransfer .

:TotalLandReturnFlow-UT :isFlowType :InternalTransfer .

:TributaryInflow-UT :isFlowType :Inflow .

:UngagedStreamGains-WY :isFlowType :Inflow .

:UngagedStreamLosses-WY :isFlowType :Outflow .

:UrbanWaterSystemInflows-AUS :isFlowType :Inflow .

:WastewaterCollected-AUS :isFlowType :Inflow .

:WaterReleaseCausedByLandSubsidence-CA :isFlowType :Inflow .

:WaterUse-NM :isFlowType :Outflow .

:AllocatedDiversion%3AEnvironmentalPurposes-AUS :isFlowType :Outflow .

:AllocatedDiversion%3AIndividualUsers-AUS :isFlowType :Outflow .

:AllocatedDiversion%3AInter-region-AUS :isFlowType :Outflow .

:AllocatedDiversion%3AIrrigation-AUS :isFlowType :Outflow .

:AllocatedDiversion%3AIrrigationScheme-AUS :isFlowType :Outflow .

:AllocatedDiversion%3AUrbanSystem-AUS :isFlowType :Outflow .

:AllocatedDiversions%3ASurfaceWater-AUS :isFlowType :Inflow, :InternalTransfer .

:AllocatedExtraction%3AEnvironmentalPurposes-AUS :isFlowType :Outflow .

:AllocatedExtraction%3AGroundwater-AUS :isFlowType :InternalTransfer .

:AllocatedExtraction%3AIndividualUsers-AUS :isFlowType :Outflow .

:AllocatedExtraction%3AIrrigation-AUS :isFlowType :Outflow .

:AllocatedExtraction%3AUrbanSystem-AUS :isFlowType :Outflow .

:AllocationExtraction%3ASalinityAndWaterTableManagement-AUS :isFlowType :Outflow .

:AppliedWaterReuse%2FRecycledWater-CA :isFlowType :InternalTransfer .

:Delivery%3ADesalinatedWater-AUS :isFlowType :Inflow .

:Delivery%3AInter-region-AUS :isFlowType :Inflow .

:Delivery%3AInter-regionAgreement-AUS :isFlowType :Inflow .

:Delivery%3AIrrigationScheme-AUS :isFlowType :Outflow .

:Delivery%3AUrbanUsers-AUS :isFlowType :Outflow .

:Discharge%3ALandscape-AUS :isFlowType :Outflow .

:Discharge%3ASea-AUS :isFlowType :Outflow .

:Discharge%3ASurfaceWater-AUS :isFlowType :InternalTransfer .

:Discharge%3AUrbanSupply-AUS :isFlowType :InternalTransfer .

:Discharge%3AUrbanSupplySystem-AUS :isFlowType :Inflow .

:Discharge%3AUser-AUS :isFlowType :Inflow .

:Discharge%3AWastewater-AUS :isFlowType :Inflow .

:Diversions%3AStatutoryRights-AUS :isFlowType :Outflow .

:Extraction%3AStatutoryRights-AUS :isFlowType :Outflow .

:Industrial%3ACoalbedMethandProduction-WY :isFlowType :InternalTransfer .

:Industrial%3AMiscellaneous-WY :isFlowType :InternalTransfer .

:Industrial%3AOilAndGas-WY :isFlowType :InternalTransfer .

:Inter-regionInflow%3AGroundwater-AUS :isFlowType :Inflow .

:Inter-regionInflow%3ASurfaceWater-AUS :isFlowType :Inflow .

:Inter-regionOutflow%3AGroundwater-AUS :isFlowType :Outflow .

:IrrigationWaterSupplyLimitedConsumptiveUse%28Depletions%29-WY :isFlowType :Outflow .

:Leakage%3AFarmDams-AUS :isFlowType :Inflow .

:Leakage%3AGroundwater-AUS :isFlowType :InternalTransfer, :Outflow .

:Leakage%3ALandscape-AUS :isFlowType :Outflow .

:Leakage%3AUrbanSystem-AUS :isFlowType :Inflow, :InternalTransfer .

:ManagedAquiferRecharge%3AIndividualUser-AUS :isFlowType :Inflow .

:Non-AllocatedExtraction%3AGroundwater-AUS :isFlowType :Inflow .

:Non-AllocatedExtraction%3AIndividualUsers-AUS :isFlowType :Outflow .

:Non-AllocatedExtraction%3AUrbanSystem-AUS :isFlowType :InternalTransfer .

:Non-allocatedDiversion%3AEnvironmentalPurposes-AUS :isFlowType :Outflow .

:Non-allocatedDiversion%3AIndividualUsers-AUS :isFlowType :Outflow .

:Non-allocatedDiversion%3AUrbanSystem-AUS :isFlowType :Outflow .

:PointReturn%3AIrrigation-AUS :isFlowType :Inflow .

:Recharge%3AGroundwater-AUS :isFlowType :InternalTransfer .

:Recharge%3ALandscape-AUS :isFlowType :Inflow .

:Recharge%3ASurfaceWater-AUS :isFlowType :InternalTransfer .

:RecycledWaterDelivery%3AUrbanUsers-AUS :isFlowType :Outflow .

:ReturnFlow%3AEnvironmentalPurposes-AUS :isFlowType :Inflow .

:RiparianRelease%3AUrbanSupply-AUS :isFlowType :InternalTransfer .

:SupplySystemDelivery%3AInter-Region-AUS :isFlowType :Inflow .

:SupplySystemDelivery%3AUrbanUsers-AUS :isFlowType :Outflow .

:SupplySystemDischarge%3AReservoirs-AUS :isFlowType :InternalTransfer .

:SupplySystemTransfer%3AInter-region-AUS :isFlowType :Outflow .

:Transfer%3AInter-region-AUS :isFlowType :Outflow .

:WastewaterDischarge%3ALandscape-AUS :isFlowType :Outflow .

:OtherSupplySystemDecreases-AUS :isFlowType :Outflow .

:OtherWastewaterDecreases-AUS :isFlowType :Outflow .

:RiverLosses-AUS :isFlowType :Outflow .

:Losses%3AManagementOfTreatedWater-AUS :isFlowType :Outflow .

:Losses%3AWastewaterTreatmentSystem-AUS :isFlowType :Outflow .

:RecycledWaterDelivery%3AIrrigation-AUS :isFlowType :Outflow .

:SupplySystemDelivery%3AIrrigation-AUS :isFlowType :Outflow .

:SupplySystemDischarge%3ASurfaceWater-AUS :isFlowType :InternalTransfer .

:WastewaterAndRecycledWaterDischarge%3ASurfaceWater-AUS :isFlowType :InternalTransfer .

:WastewaterDischarge%3ASurfaceWater-AUS :isFlowType :InternalTransfer .

:AgriculturalAndMunicipalDepletions-UT :isPartialSubComponentOf :CropConsumptiveUse-CO,
    :GroundwaterExtraction-CA, :LivestockConsumptiveUse-CO, :MunicipalAndIndustrialConsumptiveUse-CO,
    :MunicipalConsumptiveUse-WY, :MunicipalTotalUse-WY, :SurfaceWaterDiversions-CA .

:LivestockConsumptiveUse-CO :isPartialSubComponentOf :AgriculturalAndMunicipalDepletions-UT,
    :AgriculturalDepletions-UT, :AppliedWater-CA, :GroundwaterExtraction-CA, :SurfaceWaterDiversions-CA .

:MunicipalAndIndustrialConsumptiveUse-CO :isPartialSubComponentOf :AppliedWater-CA,
    :Commercial-NMOSE, :GroundwaterExtraction-CA, :Industrial-NMOSE, :Mining-NMOSE, :Power-NMOSE,
    :PublicWaterSupply-NMOSE, :SurfaceWaterDiversions-CA .

:MunicipalTotalUse-WY :isPartialSubComponentOf :GroundwaterExtraction-CA, :MunicipalAndIndustrialConsumptiveUse-CO,
    :SurfaceWaterDiversions-CA .

:AgriculturalAndMunicipalDiversions-UT :isPartialSubComponentOf :GroundwaterExtraction-CA,
    :SurfaceWaterDiversions-CA .

:AgriculturalConsumptiveUse-WY :isPartialSubComponentOf :AppliedWater-CA .

:AgriculturalDepletions-UT :isPartialSubComponentOf :AppliedWater-CA, :SurfaceDiversionToCropland-UT .

:AreaOutflows :isPartialSubComponentOf :GagedStreamOutflow-WY, :StreamOutfow-CA .

:BasinOutflow-UT :isPartialSubComponentOf :GagedStreamOutflow-WY .

:Exports-CO :isPartialSubComponentOf :GroundwaterExport-CA, :StoredWaterExport-CA,
    :SurfaceWaterExports-CA .

:BasinInflow-UT :isPartialSubComponentOf :GagedStreamInflow-WY, :GagedSurfaceWaterInflow-CO,
    :UngagedSurfaceWaterInflow-CO .

:RiverInflow-UT :isPartialSubComponentOf :GagedStreamInflow-WY, :GagedSurfaceWaterInflow-CO,
    :UngagedSurfaceWaterInflow-CO .

:GagedSurfaceWaterInflow-CO :isPartialSubComponentOf :StreamInflow-CA .

:UngagedSurfaceWaterInflow-CO :isPartialSubComponentOf :StreamInflow-CA .

:Commercial-NMOSE :isPartialSubComponentOf :AppliedWater-CA .

:MunicipalAndIndustrialDiversions-UT :isPartialSubComponentOf :AppliedWater-CA, :GroundwaterExtraction-CA,
    :IndustrialConsumptiveUse-WY, :IndustrialTotalUse-WY, :MunicipalConsumptiveUse-WY,
    :MunicipalTotalUse-WY, :SurfaceWaterDiversions-CA .

:Precipitation-CO :isPartialSubComponentOf :PrecipitationOnLakes-CA .

:Precipitation-UT :isPartialSubComponentOf :PrecipitationOnLakes-CA .

:Precipitation-WY :isPartialSubComponentOf :PrecipitationOnLakes-CA .

:IrrigatedAgricultureDepletions-NMOSE :isPartialSubComponentOf :AgriculturalAndMunicipalDepletions-UT,
    :AppliedWater-CA .

:EvaporationFromReservoirs-NMOSE :isPartialSubComponentOf :LakeEvaporation-CA .

:GagedSurfaceWaterOutflow-CO :isPartialSubComponentOf :StreamOutfow-CA .

:Industrial-NMOSE :isPartialSubComponentOf :AppliedWater-CA, :IndustrialConsumptiveUse-WY,
    :IndustrialTotalUse-WY .

:IndustrialConsumptiveUse-WY :isPartialSubComponentOf :GroundwaterExtraction-CA, :SurfaceWaterDiversions-CA .

:IndustrialTotalUse-WY :isPartialSubComponentOf :GroundwaterExtraction-CA, :MunicipalAndIndustrialConsumptiveUse-CO,
    :SurfaceWaterDelivery-CA .

:IrrigatedAgricultureDiversions-NMOSE :isPartialSubComponentOf :GroundwaterExtraction-CA,
    :IrrigationSurfaceWaterDiversions-WY, :SurfaceWaterDiversions-CA .

:Livestock-NMOSE :isPartialSubComponentOf :AppliedWater-CA, :GroundwaterExtraction-CA,
    :SurfaceWaterDiversions-CA .

:Mining-NMOSE :isPartialSubComponentOf :AppliedWater-CA, :GroundwaterExtraction-CA,
    :IndustrialConsumptiveUse-WY, :IndustrialTotalUse-WY, :SurfaceWaterDiversions-CA .

:Industrial%3AMineProduction-WY :isPartialSubComponentOf :IndustrialConsumptiveUse-WY,
    :IndustrialTotalUse-WY .

:Power-NMOSE :isPartialSubComponentOf :AppliedWater-CA, :GroundwaterExtraction-CA,
    :IndustrialConsumptiveUse-WY, :IndustrialTotalUse-WY, :SurfaceWaterDiversions-CA .

:PublicWaterSupply-NMOSE :isPartialSubComponentOf :AgriculturalAndMunicipalDiversions-UT,
    :DomesticTotalUse-WY, :GroundwaterExtraction-CA, :MunicipalAndIndustrialDiversions-UT,
    :MunicipalConsumptiveUse-WY, :MunicipalTotalUse-WY, :SurfaceWaterDiversions-CA .

:MunicipalAndIndustrialDepeltion-UT :isPartialSubComponentOf :AppliedWater-CA, :GroundwaterExtraction-CA,
    :IndustrialConsumptiveUse-WY, :IndustrialTotalUse-WY, :MunicipalConsumptiveUse-WY,
    :MunicipalTotalUse-WY, :SurfaceWaterDiversions-CA .

:MunicipalAndIndustrialReturnFlow-UT :isPartialSubComponentOf :IndustrialTotalUse-WY,
    :MunicipalTotalUse-WY .

:NativeVegetationConsumptiveUse-CO :isPartialSubComponentOf :NaturalSystemUse-UT,
    :RiparianDepletions-UT .

:Industrial%3AElectricalGeneration-WY :isPartialSubComponentOf :IndustrialConsumptiveUse-WY,
    :IndustrialTotalUse-WY .

:Self-SuppliedDomestic-NMOSE :isPartialSubComponentOf :GroundwaterExtraction-CA, :SurfaceWaterDiversions-CA .

:SurfaceWaterFlows-UT :isPartialSubComponentOf :SurfaceWaterDiversions-CA .

:TributaryInflow-UT :isPartialSubComponentOf :GagedStreamInflow-WY, :GagedSurfaceWaterInflow-CO,
    :UngagedSurfaceWaterInflow-CO .

:Industrial%3ACoalbedMethandProduction-WY :isPartialSubComponentOf :IndustrialConsumptiveUse-WY,
    :IndustrialTotalUse-WY .

:Industrial%3AMiscellaneous-WY :isPartialSubComponentOf :IndustrialConsumptiveUse-WY,
    :IndustrialTotalUse-WY .

:Industrial%3ANaturalGas-WY :isPartialSubComponentOf :IndustrialConsumptiveUse-WY .

:Industrial%3AOilAndGas-WY :isPartialSubComponentOf :IndustrialConsumptiveUse-WY,
    :IndustrialTotalUse-WY .

:SupplySystemDischarge%3ASurfaceWater-AUS :isPartialSubComponentOf :SupplySystemDischarge%3AReservoirs-AUS .

:AgriculturalAndMunicipalDepletions-UT :isSubComponentOf :AgriculturalAndMunicipalDiversions-UT,
    :AppliedWater-CA .

:CropConsumptiveUse-CO :isSubComponentOf :AppliedWater-CA, :Evapotranspiration-CA,
    :SurfaceWaterDiversions-CA .

:GroundwaterExtraction-CA :isSubComponentOf :TotalGroundwaterSystemOutflow-CA, :TotalLandSystemInflow-CA .

:LivestockConsumptiveUse-CO :isSubComponentOf :Livestock-NMOSE .

:MunicipalConsumptiveUse-WY :isSubComponentOf :AppliedWater-CA, :MunicipalAndIndustrialConsumptiveUse-CO .

:MunicipalTotalUse-WY :isSubComponentOf :AppliedWater-CA .

:SurfaceWaterDiversions-CA :isSubComponentOf :TotalSurfaceWaterInflow-CA, :TotalSurfaceWaterOutflow-CA .

:AgriculturalAndMunicipalDiversions-UT :isSubComponentOf :AppliedWater-CA .

:AppliedWater-CA :isSubComponentOf :TotalLandSystemInflow-CA .

:AgriculturalConsumptiveUse-WY :isSubComponentOf :Evapotranspiration-CA, :IrrigationSurfaceWaterDiversions-WY,
    :SurfaceWaterDiversions-CA, :TotalDiversions-WY .

:Evapotranspiration-CA :isSubComponentOf :TotalLandSystemOutflow-CA .

:AgriculturalDepletions-UT :isSubComponentOf :AgriculturalPotentialConsumptiveUse-UT,
    :Evapotranspiration-CA, :SurfaceWaterDiversions-CA .

:SurfaceDiversionToCropland-UT :isSubComponentOf :SurfaceWaterDiversions-CA .

:AreaOutflows :isSubComponentOf :Exports-CO .

:BasinOutflow-UT :isSubComponentOf :Exports-CO, :TotalSurfaceWaterOutflow-CA .

:GagedStreamOutflow-WY :isSubComponentOf :StreamOutfow-CA, :TotalOutflow-CA, :TotalSurfaceWaterOutflow-CA .

:StreamOutfow-CA :isSubComponentOf :TotalSurfaceWaterOutflow-CA .

:BasinInflow-UT :isSubComponentOf :TotalSurfaceWaterInflow-CA .

:RiverInflow-UT :isSubComponentOf :TotalSurfaceWaterInflow-CA .

:GagedStreamInflow-WY :isSubComponentOf :StreamInflow-CA, :TotalInflow-CA, :TotalSurfaceWaterInflow-CA .

:GagedSurfaceWaterInflow-CO :isSubComponentOf :BasinInflow-UT, :RiverInflow-UT, :TotalInflow-CA,
    :TotalSurfaceWaterInflow-CA .

:UngagedSurfaceWaterInflow-CO :isSubComponentOf :RiverInflow-UT, :TotalInflow-CA,
    :TotalSurfaceWaterInflow-CA .

:StreamInflow-CA :isSubComponentOf :TotalSurfaceWaterInflow-CA .

:ChangeInGroundwaterStorage-CA :isSubComponentOf :ChangeInTotalSystemStorage-CA .

:ChangeInLandSystemStorage-CA :isSubComponentOf :ChangeInTotalSystemStorage-CA .

:ChangeInSurfaceWaterStorage-CA :isSubComponentOf :ChangeInTotalSystemStorage-CA .

:Commercial-NMOSE :isSubComponentOf :MunicipalAndIndustrialDiversions-UT .

:ConveyanceEvaporation-CA :isSubComponentOf :HumanConsumption-NM, :TotalSurfaceWaterOutflow-CA .

:ConveyanceLossesForAllocatedDiversions-AUS :isSubComponentOf :SurfaceWaterOutflows-AUS .

:ConveyanceSeepage-CA :isSubComponentOf :TotalGroundwaterSystemInflow-CA, :TotalSurfaceWaterOutflow-CA .

:CoplandPrecipitation-UT :isSubComponentOf :Precipitation-CA, :Precipitation-CO, :Precipitation-NM,
    :Precipitation-UT, :Precipitation-WY .

:Precipitation-CA :isSubComponentOf :Precipitation-NM, :TotalLandSystemInflow-CA .

:IrrigatedAgricultureDepletions-NMOSE :isSubComponentOf :Evapotranspiration-CA, :IrrigatedAgriculture-NMOSE,
    :IrrigatedAgricultureDiversions-NMOSE, :SurfaceWaterDiversions-CA .

:DomesticTotalUse-WY :isSubComponentOf :AppliedWater-CA .

:Evaporation-AUS :isSubComponentOf :SurfaceWaterOutflows-AUS .

:Evaporation-NM :isSubComponentOf :TotalEvaporation-NM .

:LakeEvaporation-CA :isSubComponentOf :TotalSurfaceWaterOutflow-CA .

:ReservoirEvaporation-CO :isSubComponentOf :LakeEvaporation-CA .

:ReservoirEvaporation-UT :isSubComponentOf :LakeEvaporation-CA .

:GroundwaterExport-CA :isSubComponentOf :TotalGroundwaterSystemOutflow-CA .

:StoredWaterExport-CA :isSubComponentOf :TotalGroundwaterSystemOutflow-CA .

:SurfaceWaterExports-CA :isSubComponentOf :TotalSurfaceWaterOutflow-CA .

:FloodReturn-AUS :isSubComponentOf :SurfaceWaterInflows-AUS .

:GagedSurfaceWaterOutflow-CO :isSubComponentOf :BasinOutflow-UT, :TotalSurfaceWaterOutflow-CA .

:GroundWaterInflow-CO :isSubComponentOf :TotalGroundwaterSystemInflow-CA, :TotalInflow-CA .

:SubsurfaceInflow-CA :isSubComponentOf :TotalGroundwaterSystemInflow-CA .

:GroundWaterOutflow-CO :isSubComponentOf :TotalGroundwaterSystemOutflow-CA .

:SubsurfaceOutflow-CA :isSubComponentOf :TotalGroundwaterSystemOutflow-CA .

:GroundwaterDischarge-AUS :isSubComponentOf :SurfaceWaterInflows-AUS .

:Discharge%3AGroundwater-AUS :isSubComponentOf :Discharge%3ASurfaceWater-AUS, :SurfaceWaterInflows-AUS .

:GroundwaterET-NM :isSubComponentOf :Evapotranspiration-CA, :TotalEvaporation-NM .

:LakeGainFromGroundwater-CA :isSubComponentOf :TotalGroundwaterSystemOutflow-CA, :TotalSurfaceWaterInflow-CA .

:GroundwaterOutflows-AUS :isSubComponentOf :GroundwaterOutflows-AUS .

:HumanStorageAndDistributionSystemStock-NM :isSubComponentOf :ChangeInSurfaceWaterStorage-CA .

:ImportedWater-CA :isSubComponentOf :TotalSurfaceWaterInflow-CA .

:Industrial-NMOSE :isSubComponentOf :MunicipalAndIndustrialDiversions-UT .

:IndustrialConsumptiveUse-WY :isSubComponentOf :AppliedWater-CA, :MunicipalAndIndustrialConsumptiveUse-CO .

:IndustrialTotalUse-WY :isSubComponentOf :AppliedWater-CA .

:SurfaceWaterDelivery-CA :isSubComponentOf :TotalLandSystemInflow-CA, :TotalSurfaceWaterOutflow-CA .

:Inter-regionCoastalInflow-AUS :isSubComponentOf :GroundwaterInflows-AUS .

:Inter-regionCoastalOutflow-AUS :isSubComponentOf :GroundwaterOutflows-AUS .

:IrrigatedAgricultureDiversions-NMOSE :isSubComponentOf :AgriculturalAndMunicipalDiversions-UT,
    :IrrigatedAgriculture-NMOSE .

:LakeLossToGroundwater-CA :isSubComponentOf :Recharge-NM, :TotalGroundwaterSystemInflow-CA,
    :TotalSurfaceWaterOutflow-CA .

:Livestock-NMOSE :isSubComponentOf :AgriculturalAndMunicipalDiversions-UT .

:LivestockConsumptiveUse-WY :isSubComponentOf :AppliedWater-CA .

:ManagedAquiferRecharge-AUS :isSubComponentOf :GroundwaterInflows-AUS, :UrbanWaterSystemOutflows-AUS .

:ManagedAquiferRecharge-CA :isSubComponentOf :Recharge-NM, :TotalGroundwaterSystemInflow-CA,
    :TotalLandSystemOutflow-CA .

:Mining-NMOSE :isSubComponentOf :MunicipalAndIndustrialDiversions-UT .

:Power-NMOSE :isSubComponentOf :MunicipalAndIndustrialDiversions-UT .

:PublicWaterSupply-NMOSE :isSubComponentOf :AppliedWater-CA .

:MunicipalAndIndustrialDepeltion-UT :isSubComponentOf :MunicipalAndIndustrialConsumptiveUse-CO,
    :MunicipalAndIndustrialDiversions-UT .

:MunicipalAndIndustrialReturnFlow-UT :isSubComponentOf :AppliedWater-CA, :MunicipalAndIndustrialDiversions-UT,
    :ReturnFlow-CA .

:ReturnFlow-CA :isSubComponentOf :TotalLandSystemOutflow-CA, :TotalSurfaceWaterInflow-CA .

:NativeVegetationConsumptiveUse-CO :isSubComponentOf :Evapotranspiration-CA .

:RiparianDepletions-UT :isSubComponentOf :Evapotranspiration-CA, :NativeVegetationConsumptiveUse-CO,
    :NaturalSystemUse-UT .

:Non-allocatedExtraction-AUS :isSubComponentOf :GroundwaterOutflows-AUS .

:OtherStatutoryRights-AUS :isSubComponentOf :SurfaceWaterOutflows-AUS .

:Outflow-AUS :isSubComponentOf :SurfaceWaterOutflows-AUS .

:OverbankFloodSpilling-AUS :isSubComponentOf :SurfaceWaterOutflows-AUS .

:OverbankFlow-AUS :isSubComponentOf :SurfaceWaterOutflows-AUS .

:Precipitation-AUS :isSubComponentOf :SurfaceWaterInflows-AUS .

:PrecipitationOnLakes-CA :isSubComponentOf :Precipitation-CA, :Precipitation-NM, :TotalSurfaceWaterInflow-CA .

:RechargeOfAppliedWater-CA :isSubComponentOf :Recharge-NM, :TotalGroundwaterSystemInflow-CA,
    :TotalLandSystemOutflow-CA .

:RechargeOfPrecipitation-CA :isSubComponentOf :Recharge-NM, :TotalGroundwaterSystemInflow-CA,
    :TotalLandSystemOutflow-CA .

:RecycledWaterExport-CA :isSubComponentOf :TotalLandSystemOutflow-CA .

:ReservoirEvaporation-WY :isSubComponentOf :LakeEvaporation-CA .

:RiverAndFloodplainLosses-AUS :isSubComponentOf :SurfaceWaterOutflows-AUS .

:RiverEvaporation-NM :isSubComponentOf :TotalEvaporation-NM .

:RiverUseByWetPasture-UT :isSubComponentOf :AgriculturalDepletions-UT, :CropConsumptiveUse-CO .

:Runoff-AUS :isSubComponentOf :SurfaceWaterInflows-AUS .

:Runoff-CA :isSubComponentOf :TotalLandSystemOutflow-CA, :TotalSurfaceWaterInflow-CA .

:StoredWaterExtraction-CA :isSubComponentOf :TotalGroundwaterSystemOutflow-CA, :TotalLandSystemInflow-CA .

:StreamEvaporation-CA :isSubComponentOf :TotalSurfaceWaterOutflow-CA .

:StreamGainFromGroundwater-CA :isSubComponentOf :TotalGroundwaterSystemOutflow-CA,
    :TotalSurfaceWaterInflow-CA .

:StreamLossToGroundwater-CA :isSubComponentOf :Recharge-NM, :TotalGroundwaterSystemInflow-CA,
    :TotalSurfaceWaterInflow-CA .

:SurfaceWaterEvaporation-NM :isSubComponentOf :TotalEvaporation-NM .

:SurfaceWaterGroundwaterInteractions-NM :isSubComponentOf :Recharge-NM .

:TributaryInflow-UT :isSubComponentOf :StreamInflow-CA, :TotalInflow-CA, :TotalSurfaceWaterInflow-CA .

:UngagedStreamGains-WY :isSubComponentOf :StreamGainFromGroundwater-CA .

:UngagedStreamLosses-WY :isSubComponentOf :StreamLossToGroundwater-CA .

:WastewaterCollected-AUS :isSubComponentOf :UrbanWaterSystemInflows-AUS .

:WaterReleaseCausedByLandSubsidence-CA :isSubComponentOf :TotalGroundwaterSystemInflow-CA .

:AllocatedDiversion%3AEnvironmentalPurposes-AUS :isSubComponentOf :SurfaceWaterOutflows-AUS .

:AllocatedDiversion%3AIndividualUsers-AUS :isSubComponentOf :SurfaceWaterOutflows-AUS .

:AllocatedDiversion%3AInter-region-AUS :isSubComponentOf :SurfaceWaterOutflows-AUS .

:AllocatedDiversion%3AIrrigation-AUS :isSubComponentOf :AllocatedDiversions%3ASurfaceWater-AUS,
    :SurfaceWaterOutflows-AUS .

:AllocatedDiversion%3AIrrigationScheme-AUS :isSubComponentOf :SurfaceWaterOutflows-AUS .

:AllocatedDiversion%3AUrbanSystem-AUS :isSubComponentOf :AllocatedDiversions%3ASurfaceWater-AUS,
    :SurfaceWaterOutflows-AUS .

:AllocatedDiversions%3ASurfaceWater-AUS :isSubComponentOf :IrrigationSchemeInflows-AUS,
    :UrbanWaterSystemInflows-AUS .

:AllocatedExtraction%3AEnvironmentalPurposes-AUS :isSubComponentOf :GroundwaterOutflows-AUS .

:AllocatedExtraction%3AGroundwater-AUS :isSubComponentOf :UrbanWaterSystemInflows-AUS .

:AllocatedExtraction%3AIndividualUsers-AUS :isSubComponentOf :GroundwaterOutflows-AUS .

:AllocatedExtraction%3AIrrigation-AUS :isSubComponentOf :GroundwaterOutflows-AUS .

:AllocatedExtraction%3AUrbanSystem-AUS :isSubComponentOf :GroundwaterOutflows-AUS .

:AppliedWaterReuse%2FRecycledWater-CA :isSubComponentOf :AppliedWater-CA, :TotalLandSystemInflow-CA .

:Commercial%3AGolfCourses-NMOSE :isSubComponentOf :Commercial%3AUnmetered-NMOSE .

:Commercial%3AUnmetered-NMOSE :isSubComponentOf :Commercial-NMOSE .

:Commercial%3AIncompleteMetered-NMOSE :isSubComponentOf :Commercial-NMOSE .

:Commercial%3AMetered-NMOSE :isSubComponentOf :Commercial-NMOSE .

:Commercial%3ASchools-NMOSE :isSubComponentOf :Commercial%3AUnmetered-NMOSE .

:Delivery%3ADesalinatedWater-AUS :isSubComponentOf :UrbanWaterSystemInflows-AUS .

:Delivery%3AInter-region-AUS :isSubComponentOf :SurfaceWaterInflows-AUS, :UrbanWaterSystemInflows-AUS .

:Delivery%3AInter-regionAgreement-AUS :isSubComponentOf :IrrigationSchemeInflows-AUS,
    :SurfaceWaterInflows-AUS, :UrbanWaterSystemInflows-AUS .

:Delivery%3AIrrigationScheme-AUS :isSubComponentOf :IrrigationSchemeOutflows-AUS .

:Delivery%3ARecycledWater-AUS :isSubComponentOf :IrrigationSchemeInflows-AUS .

:Delivery%3AUrbanUsers-AUS :isSubComponentOf :UrbanWaterSystemOutflows-AUS .

:Discharge%3ALandscape-AUS :isSubComponentOf :Discharge%3AGroundwater-AUS, :GroundwaterOutflows-AUS,
    :UrbanWaterSystemOutflows-AUS .

:Discharge%3ASea-AUS :isSubComponentOf :UrbanWaterSystemOutflows-AUS .

:Discharge%3ASurfaceWater-AUS :isSubComponentOf :Discharge%3AGroundwater-AUS, :GroundwaterOutflows-AUS,
    :UrbanWaterSystemOutflows-AUS .

:Discharge%3AUrbanSupply-AUS :isSubComponentOf :SurfaceWaterInflows-AUS .

:Discharge%3AUrbanSupplySystem-AUS :isSubComponentOf :SurfaceWaterInflows-AUS .

:Discharge%3AUser-AUS :isSubComponentOf :SurfaceWaterInflows-AUS .

:Discharge%3AWastewater-AUS :isSubComponentOf :SurfaceWaterInflows-AUS .

:Diversions%3AStatutoryRights-AUS :isSubComponentOf :SurfaceWaterOutflows-AUS .

:Extraction%3AStatutoryRights-AUS :isSubComponentOf :GroundwaterOutflows-AUS .

:Inter-regionInflow%3AGroundwater-AUS :isSubComponentOf :GroundwaterInflows-AUS .

:Inter-regionInflow%3ASurfaceWater-AUS :isSubComponentOf :SurfaceWaterInflows-AUS .

:Inter-regionOutflow%3AGroundwater-AUS :isSubComponentOf :GroundwaterOutflows-AUS .

:Leakage%3AGroundwater-AUS :isSubComponentOf :SurfaceWaterOutflows-AUS, :UrbanWaterSystemOutflows-AUS .

:Leakage%3ALandscape-AUS :isSubComponentOf :IrrigationSchemeOutflows-AUS, :SurfaceWaterOutflows-AUS .

:Leakage%3AUrbanSystem-AUS :isSubComponentOf :GroundwaterInflows-AUS .

:ManagedAquiferRecharge%3AIndividualUser-AUS :isSubComponentOf :GroundwaterInflows-AUS .

:Mining%3AReported-NMOSE :isSubComponentOf :Mining-NMOSE .

:Mining%3AUnreported-NMOSE :isSubComponentOf :Mining-NMOSE .

:Non-AllocatedDiversion%3ASurfaceWater-AUS :isSubComponentOf :UrbanWaterSystemInflows-AUS .

:Non-AllocatedExtraction%3AGroundwater-AUS :isSubComponentOf :IrrigationSchemeInflows-AUS,
    :UrbanWaterSystemInflows-AUS .

:Non-AllocatedExtraction%3AIndividualUsers-AUS :isSubComponentOf :GroundwaterOutflows-AUS .

:Non-AllocatedExtraction%3AUrbanSystem-AUS :isSubComponentOf :GroundwaterOutflows-AUS .

:Non-allocatedDiversion%3AEnvironmentalPurposes-AUS :isSubComponentOf :SurfaceWaterOutflows-AUS .

:Non-allocatedDiversion%3AIndividualUsers-AUS :isSubComponentOf :SurfaceWaterOutflows-AUS .

:Non-allocatedDiversion%3AUrbanSystem-AUS :isSubComponentOf :SurfaceWaterOutflows-AUS .

:PointReturn%3AIrrigation-AUS :isSubComponentOf :SurfaceWaterInflows-AUS .

:Power%3AReported-NMOSE :isSubComponentOf :Power-NMOSE .

:Power%3AUnreported-NMOSE :isSubComponentOf :Power-NMOSE .

:PublicWaterSupply%3AMetered-NMOSE :isSubComponentOf :PublicWaterSupply-NMOSE .

:PublicWaterSupply%3AUnmetered-NMOSE :isSubComponentOf :PublicWaterSupply-NMOSE .

:Recharge%3AGroundwater-AUS :isSubComponentOf :SurfaceWaterOutflows-AUS .

:Recharge%3ALandscape-AUS :isSubComponentOf :GroundwaterInflows-AUS, :Recharge%3AGroundwater-AUS .

:Recharge%3ASurfaceWater-AUS :isSubComponentOf :GroundwaterInflows-AUS, :Recharge%3AGroundwater-AUS .

:RecycledWaterDelivery%3AUrbanUsers-AUS :isSubComponentOf :UrbanWaterSystemOutflows-AUS .

:ReturnFlow%3AEnvironmentalPurposes-AUS :isSubComponentOf :SurfaceWaterInflows-AUS .

:RiparianRelease%3AUrbanSupply-AUS :isSubComponentOf :SurfaceWaterInflows-AUS .

:SupplySystemDelivery%3AInter-Region-AUS :isSubComponentOf :UrbanWaterSystemInflows-AUS .

:SupplySystemDelivery%3AUrbanUsers-AUS :isSubComponentOf :UrbanWaterSystemOutflows-AUS .

:SupplySystemDischarge%3AReservoirs-AUS :isSubComponentOf :UrbanWaterSystemOutflows-AUS .

:SupplySystemTransfer%3AInter-region-AUS :isSubComponentOf :UrbanWaterSystemOutflows-AUS .

:Transfer%3AInter-region-AUS :isSubComponentOf :SurfaceWaterOutflows-AUS .

:WastewaterDischarge%3ALandscape-AUS :isSubComponentOf :UrbanWaterSystemOutflows-AUS .

:AgriculturalAppliedWater-CA :isSubComponentOf :AppliedWater-CA .

:ManagedWetlandAppliedWater-CA :isSubComponentOf :AppliedWater-CA .

:UrbanAppliedWater-CA :isSubComponentOf :AppliedWater-CA .

:OtherWastewaterDecreases-AUS :isSubComponentOf :UrbanWaterSystemOutflows-AUS .

:Losses%3AManagementOfTreatedWater-AUS :isSubComponentOf :UrbanWaterSystemOutflows-AUS .

:Losses%3AWastewaterTreatmentSystem-AUS :isSubComponentOf :UrbanWaterSystemOutflows-AUS .

:RecycledWaterDelivery%3AIrrigation-AUS :isSubComponentOf :UrbanWaterSystemOutflows-AUS .

:SupplySystemDelivery%3AIrrigation-AUS :isSubComponentOf :UrbanWaterSystemOutflows-AUS .

:WastewaterAndRecycledWaterDischarge%3ASurfaceWater-AUS :isSubComponentOf :UrbanWaterSystemOutflows-AUS .

:WastewaterDischarge%3ASurfaceWater-AUS :isSubComponentOf :UrbanWaterSystemOutflows-AUS .

:GagedSurfaceWaterInflow-CO :type :Inflow .

:AgriculturalAndMunicipalDepletions-UT :usedBy :UT .

:CropConsumptiveUse-CO :usedBy :CO .

:GroundwaterExtraction-CA :usedBy :CA .

:LivestockConsumptiveUse-CO :usedBy :CO .

:MunicipalAndIndustrialConsumptiveUse-CO :usedBy :CO .

:MunicipalConsumptiveUse-WY :usedBy :BearRiver, :GreenRiver, :NortheastRiver, :PlatteRiver,
    :Powder-TongueRiver, :WY .

:MunicipalTotalUse-WY :usedBy :Salt-SnakeRiver, :WY, :Wind-BighornRiver .

:SurfaceWaterDiversions-CA :usedBy :CA .

:AgriculturalAndMunicipalDiversions-UT :usedBy :UT .

:AppliedWater-CA :usedBy :CA .

:USGSStreamGages :usedBy :CO, :NM, :USBR, :UT, :WY .

:UTDiversionRecordsFromRiverCommissioners :usedBy :UT .

:UTMunicipalPotableAndSecondaryDiversionRecords :usedBy :UT .

:UTOtherIrrigationCompanyRecords :usedBy :UT .

:UTReservoirStorageAndReleaseRecords :usedBy :UT .

:UTWaterRights :usedBy :UT .

:USGSStreamStats :usedBy :UT .

:UTDivisionOfWaterResourcesArea-AltitudeMethod :usedBy :UT .

:USGSMeanAnnualReachEstimates :usedBy :UT .

:AgriculturalConsumptiveUse-WY :usedBy :BearRiver, :GreenRiver, :NortheastRiver, :PlatteRiver,
    :Powder-TongueRiver, :Salt-SnakeRiver, :WY, :Wind-BighornRiver .

:WYConsumptiveUseMethod :usedBy :WY .

:Evapotranspiration-CA :usedBy :CA .

:IrrigationSurfaceWaterDiversions-WY :usedBy :WY .

:TotalDiversions-WY :usedBy :WY .

:BearRiver :usedBy :WY .

:GreenRiver :usedBy :WY .

:NortheastRiver :usedBy :WY .

:PlatteRiver :usedBy :WY .

:Powder-TongueRiver :usedBy :WY .

:Salt-SnakeRiver :usedBy :WY .

:Wind-BighornRiver :usedBy :WY .

:AgriculturalDepletions-UT :usedBy :UT .

:UTConsumptiveUseMethod :usedBy :UT .

:SurfaceDiversionToCropland-UT :usedBy :UT .

:AgriculturalPotentialConsumptiveUse-UT :usedBy :UT .

:NationalOceanicAndAtmosphericAdministrationStations :usedBy :CO, :NM, :UT, :WY .

:PRISM :usedBy :CA, :CO, :NM, :USBR, :UT, :WY .

:USBureauOfReclamationAgriMetStations :usedBy :UT .

:USUResearchReport145 :usedBy :UT .

:DailyPenman-Monteith :usedBy :CO, :NM, :UT, :WY .

:ModifiedBlaney-Criddle :usedBy :CO, :NM, :UT, :WY .

:SolarRadiation :usedBy :CO, :NM, :USBR, :UT, :WY .

:Temperature :usedBy :CO, :NM, :USBR, :UT, :WY .

:VaporPressure :usedBy :CA, :CO, :NM, :USBR, :UT, :WY .

:WindRun :usedBy :CO, :NM, :USBR, :UT, :WY .

:ClimateCoefficient%28kt%29 :usedBy :CO, :NM, :USBR, :UT, :WY .

:CropGrowthStateCoefficient%28Kc%29 :usedBy :CA, :CO, :NM, :USBR, :UT, :WY .

:MeanMonthlyAirTemperatures%28T%29 :usedBy :CO, :NM, :USBR, :UT, :WY .

:MonthlyPercentageOfAnnualDaylightHours%28P%29 :usedBy :CO, :NM, :USBR, :UT, :WY .

:AnnualEmployeeHours :usedBy :WY .

:MineSafetyAndHealthAdministration%28MSHA%29 :usedBy :WY .

:AnnualEvaporation :usedBy :NM .

:MonthlyEvaporation :usedBy :NM .

:AnnualSodaAshProduction :usedBy :WY .

:USGeologicalSurvey%28USGS%29 :usedBy :WY .

:TotalLandSystemInflow-CA :usedBy :CA .

:AreaOutflows :usedBy :UT .

:BasinOutflow-UT :usedBy :UT .

:GagedStreamOutflow-WY :usedBy :WY .

:StreamOutfow-CA :usedBy :CA .

:Exports-CO :usedBy :CO .

:TotalSurfaceWaterOutflow-CA :usedBy :CA .

:AverageMonthlyReservoirGageHeight :usedBy :NM .

:IrrigationDistricts :usedBy :NM .

:USArmyCorpsOfEngineers :usedBy :NM .

:USBureauOfReclamationStations :usedBy :CO, :NM .

:NewMexicoInterstateStreamCommission%28NMISC%29 :usedBy :NM .

:AverageUseRate :usedBy :CO .

:MidwestPlanServiceStructuresAndEnvironmentalHandbook%2C1977 :usedBy :CO .

:Baseflow :usedBy :AUS, :Adelaide, :CO .

:HistoricalData :usedBy :AUS, :CO, :UT .

:BasinInflow-UT :usedBy :UT .

:RiverInflow-UT :usedBy :UT .

:GagedStreamInflow-WY :usedBy :WY .

:GagedSurfaceWaterInflow-CO :usedBy :CO .

:UngagedSurfaceWaterInflow-CO :usedBy :CO .

:TotalSurfaceWaterInflow-CA :usedBy :CA .

:StreamInflow-CA :usedBy :CA .

:COAgriculturalMeteorologyNetworkStation :usedBy :CO .

:CODiversionRecords :usedBy :CO .

:CODivisionOfWaterResourcesGages :usedBy :CO .

:HydroBase :usedBy :CO .

:SCSTR21 :usedBy :CO, :NM, :USBR, :WY .

:SatelliteAndAerialPhotos :usedBy :CO, :USBR, :UT, :WY .

:SnotelNetworkOfWeatherStations :usedBy :CO, :WY .

:WeatherStations :usedBy :CO, :NM, :UT, :WY .

:CommunityCollaborativeRain%2CHailAndSnowNetwork%28CoCoRaHS%29 :usedBy :CO .

:NationalAgriculturalStatisticsService%28NASS%29CroplandDataLayer :usedBy :CO, :USBR .

:RemoteAutomatedWeatherStations%28RAWS%29 :usedBy :CO, :WY .

:COIrrigatedAcreageAssessment :usedBy :CO .

:CropIrrigationRequirementEstimationMethod :usedBy :CO, :NM, :USBR, :UT, :WY .

:EnergyBalanceRemoteSensing :usedBy :CO, :NM, :USBR, :UT, :WY .

:METRIC :usedBy :CO, :NM, :USBR, :UT, :WY .

:ModifiedBlaney-CriddleWithETElevationAdjustment :usedBy :CO, :UT, :WY .

:NDVIRemoteSensing :usedBy :CO .

:NDVIstar :usedBy :CO .

:On-FarmWaterBalance :usedBy :CO, :WY .

:OriginalBlaney-Criddle :usedBy :CO, :NM, :UT .

:OriginalBlaney-CriddleWithETElevationAdjustment :usedBy :CO .

:RESET :usedBy :CO, :USBR .

:StateCU :usedBy :CO, :WY .

:CropIrrigationRequirement :usedBy :CO, :NM, :USBR, :UT, :WY .

:CropType :usedBy :CO, :NM, :UT, :WY .

:EffectivePrecipitation :usedBy :CO, :NM, :USBR, :UT, :WY .

:IrrigatedAcreage :usedBy :CO, :NM, :USBR, :WY .

:IrrigationMethod :usedBy :CO, :NM, :UT, :WY .

:PotentialConsumptiveUse :usedBy :CO, :NM, :USBR, :WY .

:Precipitation :usedBy :CO, :NM, :UT, :WY .

:SupplySource :usedBy :CO, :WY .

:SupplyType :usedBy :CO .

:WaterSupply :usedBy :CO, :NM, :USBR, :UT, :WY .

:COGISExercise :usedBy :CO .

:COLivestockMethod :usedBy :CO .

:StateAgriculturalStatistics :usedBy :CO .

:LivestockCount :usedBy :CO .

:ConsumptiveRatio :usedBy :CO .

:GrossUsage :usedBy :CO .

:Population :usedBy :CA, :CO, :WY .

:CONativeVegetationMethod :usedBy :CO .

:HistoricalDiversionsFile :usedBy :CO .

:Diversions :usedBy :CO, :WY .

:NativeVegetationCoefficient :usedBy :CO .

:ReturnFlow :usedBy :CO, :WY .

:ChangeInGroundWaterStorage-CO :usedBy :CO .

:ChangeInGroundwaterStorage-CA :usedBy :CA .

:ChangeInGroundwaterStorage-AUS :usedBy :AUS, :Adelaide, :Burdekin, :Canberra, :Daly,
    :Fitzroy, :Melbourne, :MurrayDarling, :Ord, :Perth, :SouthEastQueensland, :Sydney .

:ChangeInTotalSystemStorage-CA :usedBy :CA .

:ChangeInLandSystemStorage-CA :usedBy :CA .

:ChangeInSurfaceWaterStorage-AUS :usedBy :AUS, :Adelaide, :Burdekin, :Canberra, :Daly,
    :Fitzroy, :Melbourne, :MurrayDarling, :Ord, :Perth, :SouthEastQueensland, :Sydney .

:ChangeInSurfaceWaterStorage-CA :usedBy :CA .

:ChangeInSurfaceWaterStorage-CO :usedBy :CO .

:ClassAPanEvaporationData :usedBy :NM .

:CoalProductionQuantities :usedBy :WY .

:ColoradoCensusBureau :usedBy :CO .

:ColoradoStateMod :usedBy :CO .

:ColoradoWaterConservationBoard%28CWCB%29 :usedBy :CO .

:DirectFlowDemand-Annual :usedBy :CO .

:DirectFlowDemand-Monthly :usedBy :CO .

:Evaporation :usedBy :CO, :UT .

:InstreamFlowDemand-Annual :usedBy :CO .

:InstreamFlowDemand-Monthly :usedBy :CO .

:ReservoirTargets :usedBy :CO .

:Streamflow :usedBy :CO, :NM .

:Commercial-NMOSE :usedBy :NM .

:MunicipalAndIndustrialDiversions-UT :usedBy :UT .

:ConservancyDistricts :usedBy :NM .

:ConveyanceEvaporation-CA :usedBy :CA .

:ConveyanceLossesForAllocatedDiversions-AUS :usedBy :AUS, :MurrayDarling .

:SurfaceWaterOutflows-AUS :usedBy :AUS, :Adelaide, :Burdekin, :Canberra, :Daly, :Fitzroy,
    :Melbourne, :MurrayDarling, :Ord, :Perth, :SouthEastQueensland, :Sydney .

:ConveyanceSeepage-CA :usedBy :CA .

:TotalGroundwaterSystemInflow-CA :usedBy :CA .

:CoplandPrecipitation-UT :usedBy :UT .

:Precipitation-CA :usedBy :CA .

:Precipitation-CO :usedBy :CO .

:Precipitation-NM :usedBy :NM .

:Precipitation-UT :usedBy :UT .

:Precipitation-WY :usedBy :WY .

:IrrigatedAgricultureDepletions-NMOSE :usedBy :NM .

:EmeryWaterConservancyDistrictStations :usedBy :UT .

:MesoWestStations :usedBy :UT .

:NationalWeatherServiceStations :usedBy :NM, :WY .

:NewMexicoClimateCenterStations :usedBy :NM .

:CooperativeObserverNetwork%28COOP%29 :usedBy :USBR .

:FruitGrowersNetworkStations%28FGNET%29 :usedBy :UT .

:NationalClimaticDataCenter%27sClimatographyOfTheUnitedStatesNo.81 :usedBy :WY .

:NaturalResourcesConservationServiceStations%28NRCS%29 :usedBy :NM, :WY .

:SoilClimateAnalysisNetwork%28SCAN%29 :usedBy :UT .

:USBureauOfLandManagement%28BLM%29 :usedBy :NM, :WY .

:WYDepartmentOfEnvironmentalQuality%28DEQ%29 :usedBy :WY .

:WesternRegionalClimateCenter%28WRCC%29Stations :usedBy :NM .

:WyomingStateEngineer%27sOfficeStations :usedBy :WY .

:CropTypeStateAssessments :usedBy :USBR .

:FieldSurvey :usedBy :NM .

:GroundSurvey :usedBy :UT .

:USDACroplandDataLayer%28CDL%29 :usedBy :NM .

:DailyASCEStandardizedPenman-Monteith :usedBy :CO, :WY .

:DailyEffectivePrecipitation :usedBy :CO .

:DailyModifiedHargreaves :usedBy :CO .

:DaytimeHours :usedBy :CO .

:DirectCommunication :usedBy :WY .

:WyomingWaterDevelopmentCommission%28WWDC%292002WaterSystemSurveyReport :usedBy :WY .

:WYDiversionDataFromWaterUsers :usedBy :WY .

:WYOfficeOfTheStateEngineer :usedBy :WY .

:DivertibleFlow-WY :usedBy :WY .

:DomesticTotalUse-WY :usedBy :BearRiver, :GreenRiver, :NortheastRiver, :PlatteRiver,
    :Powder-TongueRiver, :Salt-SnakeRiver, :WY, :Wind-BighornRiver .

:USCensusBureau :usedBy :CA, :NM, :WY .

:WithdrawalMethod :usedBy :NM, :WY .

:GallonsPerCapitaPerDay%28GPCD%29 :usedBy :CA, :NM .

:DownstreamFlow :usedBy :WY .

:WyomingWaterResourcesDataSystem%28WRDS%29 :usedBy :WY .

:EffectivePrecipitationFactor :usedBy :CO, :NM, :WY .

:ElectricalGenerationData :usedBy :WY .

:USEnergyInformationAdministration%28USEIA%29 :usedBy :WY .

:Elevation-Area-CapacityTables :usedBy :AUS, :Burdekin, :Fitzroy, :Melbourne, :Ord,
    :SouthEastQueensland, :Sydney, :UT .

:USBureauOfReclamation :usedBy :NM .

:UTStateEngineerData :usedBy :UT .

:WaterResourcesStudies :usedBy :UT .

:EmpiricalDataForSmallReservoirs :usedBy :NM .

:MonthlyPrecipitationVolume :usedBy :NM, :UT .

:Rainfall :usedBy :NM, :UT .

:ReservoirSurfaceArea :usedBy :NM .

:Evaporation-AUS :usedBy :AUS, :Adelaide, :Burdekin, :Canberra, :Daly, :Fitzroy, :Melbourne,
    :MurrayDarling, :Ord, :Perth, :SouthEastQueensland, :Sydney .

:Evaporation-NM :usedBy :NM .

:EvaporationFromReservoirs-NMOSE :usedBy :NM .

:PanApproach :usedBy :NM .

:MonthlyGrossEvaporationRate :usedBy :NM .

:WinterIceSurfaceArea :usedBy :NM .

:LakeEvaporation-CA :usedBy :CA .

:ReservoirEvaporation-CO :usedBy :CO .

:ReservoirEvaporation-UT :usedBy :UT .

:TotalLandSystemOutflow-CA :usedBy :CA .

:GroundwaterExport-CA :usedBy :CA .

:StoredWaterExport-CA :usedBy :CA .

:SurfaceWaterExports-CA :usedBy :CA .

:FacilityDirectorOrOperator :usedBy :NM .

:FederalArchives :usedBy :UT .

:FloodReturn-AUS :usedBy :AUS, :Adelaide, :Burdekin, :Canberra, :Daly, :Fitzroy, :Melbourne,
    :MurrayDarling, :Ord, :Perth, :Sydney .

:SurfaceWaterInflows-AUS :usedBy :AUS, :Adelaide, :Burdekin, :Canberra, :Daly, :Fitzroy,
    :Melbourne, :MurrayDarling, :Ord, :Perth, :SouthEastQueensland, :Sydney .

:GPSPopulationData :usedBy :NM .

:GageHeight :usedBy :CO .

:TotalInflow-CA :usedBy :CA .

:TotalOutflow-CA :usedBy :CA .

:GagedSurfaceWaterOutflow-CO :usedBy :CO .

:NationalAgriculturalStatisticsService :usedBy :NM .

:USDAFarmServiceAgency :usedBy :NM .

:GrossMonthlyFreeWaterSurfaceEvaporation :usedBy :CO .

:NOAATechnicalReportNWS33 :usedBy :CO .

:GroundWaterInflow-CO :usedBy :CO .

:SubsurfaceInflow-CA :usedBy :CA .

:GroundWaterOutflow-CO :usedBy :CO .

:TotalGroundwaterSystemOutflow-CA :usedBy :CA .

:SubsurfaceOutflow-CA :usedBy :CA .

:GroundwaterDischarge-AUS :usedBy :AUS, :Perth .

:Discharge%3AGroundwater-AUS :usedBy :AUS, :Adelaide, :Canberra, :Daly, :Melbourne .

:GroundwaterDiversions-NM :usedBy :NM .

:GroundwaterET-NM :usedBy :NM .

:RiparianConsumption-NM :usedBy :NM .

:LakeGainFromGroundwater-CA :usedBy :CA .

:GroundwaterInflows-AUS :usedBy :AUS, :Adelaide, :Burdekin, :Canberra, :Daly, :Fitzroy,
    :Melbourne, :Ord, :Perth, :SouthEastQueensland .

:GroundwaterInflows-NM :usedBy :NM .

:GroundwaterOutflows-AUS :usedBy :AUS, :Adelaide, :Burdekin, :Canberra, :Daly, :Fitzroy,
    :Melbourne, :MurrayDarling, :Ord, :Perth, :SouthEastQueensland .

:GroundwaterOutflows-NM :usedBy :NM .

:GroundwaterReturn-NM :usedBy :NM .

:GroundwaterStock-NM :usedBy :NM .

:GroundwaterUse :usedBy :UT .

:MunicipalAndIndustrialDiversionReports :usedBy :UT .

:USGSEstimatesOfBasinGroundwaterFlows :usedBy :UT .

:USGSGroundwaterReports :usedBy :UT .

:GroundwaterUse-UT :usedBy :UT .

:PumpedGroundwater-UT :usedBy :UT .

:HighPlainsClimateCenter-UniversityOfNebraska :usedBy :WY .

:UTStateArchives :usedBy :UT .

:HumanStorageAndDistributionSystemStock-NM :usedBy :NM .

:ImportedWater-CA :usedBy :CA .

:Imports-CO :usedBy :CO .

:IndicatorGageApproach :usedBy :NM, :USBR .

:Industrial-NMOSE :usedBy :NM .

:IndustrialConsumptiveUse-WY :usedBy :GreenRiver, :NortheastRiver, :PlatteRiver, :Salt-SnakeRiver,
    :WY, :Wind-BighornRiver .

:IndustrialTotalUse-WY :usedBy :BearRiver, :GreenRiver, :PlatteRiver, :Powder-TongueRiver,
    :WY .

:WyomingOilAndGasConservationCommission%28WYOGCC%29 :usedBy :WY .

:MonthlyCoalbedMethaneGasProductionAndProducedWater :usedBy :WY .

:NaturalGasProcessingVolumes :usedBy :WY .

:MonthlyOil%2CGas%2CAndProducedWater :usedBy :WY .

:SurfaceWaterDelivery-CA :usedBy :CA .

:Inflow-OutflowApproach :usedBy :UT .

:Inter-regionCoastalInflow-AUS :usedBy :AUS, :Adelaide, :Melbourne, :MurrayDarling,
    :Perth .

:Inter-regionCoastalOutflow-AUS :usedBy :AUS, :Adelaide, :Melbourne, :MurrayDarling,
    :Perth .

:InterpolationFromOtherRecords :usedBy :NM .

:NMIrrigatedAcreageAssessment :usedBy :NM .

:USBRIrrigatedAcreageAssessment :usedBy :USBR .

:UTIrrigatedAcreageAssessment :usedBy :UT .

:WYIrrigatedAcreageAssessment :usedBy :WY .

:SupplyStructure :usedBy :NM, :WY .

:IrrigatedAgriculture-NMOSE :usedBy :NM .

:NMConsumptiveUseMethod :usedBy :NM .

:IrrigatedAgricultureDiversions-NMOSE :usedBy :NM .

:NMOSECropAcreageFile :usedBy :NM .

:NMOSEGrowingSeasonFile :usedBy :NM .

:NMOSETemperatureAndPrecipitationFile :usedBy :NM .

:ConsumptiveIrrigationRequirement%28CIR%29 :usedBy :NM .

:IrrigationSchemeInflows-AUS :usedBy :AUS, :Adelaide, :Perth .

:IrrigationSchemeOutflows-AUS :usedBy :AUS, :Adelaide, :Perth .

:LakeLossToGroundwater-CA :usedBy :CA .

:Recharge-NM :usedBy :NM .

:LandSurfaceExapotranspiration-NM :usedBy :NM .

:LandSurfaceStock-NM :usedBy :NM .

:Livestock-NMOSE :usedBy :NM .

:LivestockConsumptiveUse-WY :usedBy :WY .

:LivestockPopulation :usedBy :NM .

:ManagedAquiferRecharge-AUS :usedBy :AUS, :Adelaide, :Perth .

:UrbanWaterSystemOutflows-AUS :usedBy :AUS, :Adelaide, :Canberra, :Melbourne, :Perth,
    :SouthEastQueensland, :Sydney .

:ManagedAquiferRecharge-CA :usedBy :CA .

:MilitaryBasePopulationData :usedBy :NM .

:Mining-NMOSE :usedBy :NM .

:Industrial%3AMineProduction-WY :usedBy :WY .

:SumOfMonthlyConsumptiveUseFactorsForGrowingSeason%28F%29 :usedBy :CO .

:MonthlyEffectivePrecipitation :usedBy :CO .

:Power-NMOSE :usedBy :NM .

:PublicWaterSupply-NMOSE :usedBy :NM .

:MunicipalAndIndustrialDepeltion-UT :usedBy :UT .

:MunicipalAndIndustrialReturnFlow-UT :usedBy :UT .

:ReturnFlow-CA :usedBy :CA .

:NDVI :usedBy :WY .

:NMDiversionRecords :usedBy :NM .

:NMSpreadsheet-BasedConsumptiveUseModel :usedBy :NM .

:OriginalHargreaves :usedBy :CO, :NM, :WY .

:NMIrrigationWithdrawals :usedBy :NM .

:NMOSEWaterRightsDatabase :usedBy :NM .

:NMOSETechnicalReportNo.48 :usedBy :NM .

:NativeVegetationConsumptiveUse-CO :usedBy :CO .

:NaturalSystemUse-UT :usedBy :UT .

:RiparianDepletions-UT :usedBy :UT .

:NaturalFlowGainDistribution :usedBy :CO .

:ProrationFactors :usedBy :CO .

:Non-allocatedExtraction-AUS :usedBy :AUS, :Burdekin, :MurrayDarling .

:OtherIncreases-AUS :usedBy :AUS, :Burdekin, :MurrayDarling .

:OtherStatutoryRights-AUS :usedBy :AUS, :Adelaide .

:Outflow-AUS :usedBy :AUS, :Adelaide, :Burdekin, :Canberra, :Daly, :Fitzroy, :Melbourne,
    :MurrayDarling, :Ord, :Perth, :SouthEastQueensland, :Sydney .

:OverbankFloodSpilling-AUS :usedBy :AUS, :SouthEastQueensland .

:OverbankFlow-AUS :usedBy :AUS, :Adelaide, :Burdekin, :Canberra, :Daly, :Fitzroy,
    :Melbourne, :MurrayDarling, :Ord, :Perth, :SouthEastQueensland, :Sydney .

:PersonalOutreach :usedBy :NM .

:WaterUseEstimate :usedBy :NM .

:PopulationServedByPublicWaterSupply :usedBy :NM .

:NewMexicoEnvironmentDepartment%28NMED%29 :usedBy :NM .

:UniversityOfNewMexicoGeospatialAndPopulationStudies%28UNMGPS%29 :usedBy :NM .

:PotentialEvapotranspiration :usedBy :CO, :UT .

:Industrial%3AElectricalGeneration-WY :usedBy :WY .

:WyomingWaterResourcesDataSystemsWaterAndClimateMapServer :usedBy :WY .

:Precipitation-AUS :usedBy :AUS, :Adelaide, :Burdekin, :Canberra, :Daly, :Fitzroy,
    :Melbourne, :MurrayDarling, :Ord, :Perth, :SouthEastQueensland, :Sydney .

:PrecipitationOnLakes-CA :usedBy :CA .

:RechargeOfAppliedWater-CA :usedBy :CA .

:RechargeOfPrecipitation-CA :usedBy :CA .

:RecycledWaterExport-CA :usedBy :CA .

:ReservoirEstimationMethod :usedBy :CO .

:ReservoirEvaporation-WY :usedBy :WY .

:PanMethod%28NetEvaporation%29 :usedBy :WY .

:GrossPanEvaportation%28inches%29 :usedBy :WY .

:RiverAndFloodplainLosses-AUS :usedBy :AUS, :Canberra .

:RiverEvaporation-NM :usedBy :NM .

:RiverUseByWetPasture-UT :usedBy :UT .

:Runoff-AUS :usedBy :AUS, :Adelaide, :Burdekin, :Canberra, :Daly, :Fitzroy, :Melbourne,
    :MurrayDarling, :Ord, :Perth, :SouthEastQueensland, :Sydney .

:Runoff-CA :usedBy :CA .

:Runoff-NM :usedBy :NM .

:STATSGOSoilsData :usedBy :UT .

:Self-SuppliedDomestic-NMOSE :usedBy :NM .

:SelfSuppliedDomesticPopulation :usedBy :NM .

:SoilMoistureHoldingCapacity :usedBy :UT .

:WaterResourcesIrrigatedLandUseDatabase :usedBy :UT .

:StateCUOutput :usedBy :WY .

:StateData :usedBy :USBR .

:StoredWaterExtraction-CA :usedBy :CA .

:StreamEvaporation-CA :usedBy :CA .

:StreamGainFromGroundwater-CA :usedBy :CA .

:StreamLossToGroundwater-CA :usedBy :CA .

:StudentPopulation :usedBy :NM .

:SurfaceWaterDiversions-NM :usedBy :NM .

:SurfaceWaterFlows-UT :usedBy :UT .

:SurfaceWaterInflows-NM :usedBy :NM .

:SurfaceWaterOutflows-NM :usedBy :NM .

:SurfaceWaterReturns-NM :usedBy :NM .

:SurfaceWaterStock-NM :usedBy :NM .

:TotalLandReturnFlow-UT :usedBy :UT .

:TributaryInflow-UT :usedBy :UT .

:USBRConsumptiveUseMethod :usedBy :USBR .

:XCONS :usedBy :USBR .

:UngagedStreamGains-WY :usedBy :WY .

:WyomingGain%2FLossEstimationMethod :usedBy :WY .

:UpstreamFlow :usedBy :WY .

:UngagedStreamLosses-WY :usedBy :WY .

:UniversityOfNewMexico :usedBy :NM .

:UrbanWaterSystemInflows-AUS :usedBy :AUS, :Adelaide, :Canberra, :Melbourne, :Perth,
    :SouthEastQueensland, :Sydney .

:WYDiversionRecords :usedBy :WY .

:WYElectricalGenerationMethod :usedBy :WY .

:WYIndustrialProductionMethod :usedBy :WY .

:WYMineProductionMethod :usedBy :WY .

:WYVariousWaterSupplyReports :usedBy :WY .

:WastewaterCollected-AUS :usedBy :AUS, :Adelaide, :Canberra, :Melbourne, :Perth, :SouthEastQueensland,
    :Sydney .

:WaterReleaseCausedByLandSubsidence-CA :usedBy :CA .

:BrownAndCaldwell%2C1984 :usedBy :NM .

:AllocatedDiversion%3AEnvironmentalPurposes-AUS :usedBy :AUS, :MurrayDarling .

:AllocatedDiversion%3AIndividualUsers-AUS :usedBy :AUS, :Adelaide, :Burdekin, :Canberra,
    :Daly, :Fitzroy, :Melbourne, :Ord, :Perth, :SouthEastQueensland, :Sydney .

:AllocatedDiversion%3AInter-region-AUS :usedBy :AUS, :Burdekin, :Melbourne .

:AllocatedDiversion%3AIrrigation-AUS :usedBy :AUS, :Burdekin, :Fitzroy, :Ord .

:AllocatedDiversion%3AIrrigationScheme-AUS :usedBy :AUS, :Perth .

:AllocatedDiversion%3AUrbanSystem-AUS :usedBy :AUS, :Adelaide, :Burdekin, :Canberra,
    :Daly, :Fitzroy, :Melbourne, :MurrayDarling, :Ord, :Perth, :SouthEastQueensland, :Sydney .

:AllocatedDiversions%3ASurfaceWater-AUS :usedBy :AUS, :Adelaide, :Canberra, :Melbourne,
    :SouthEastQueensland, :Sydney .

:AllocatedExtraction%3AEnvironmentalPurposes-AUS :usedBy :AUS, :MurrayDarling .

:AllocatedExtraction%3AGroundwater-AUS :usedBy :AUS, :Melbourne, :Perth .

:AllocatedExtraction%3AIndividualUsers-AUS :usedBy :AUS, :Adelaide, :Burdekin, :Canberra,
    :Daly, :Fitzroy, :Melbourne, :MurrayDarling, :Ord, :Perth, :SouthEastQueensland .

:AllocatedExtraction%3AIrrigation-AUS :usedBy :AUS, :Burdekin, :Fitzroy .

:AllocatedExtraction%3AUrbanSystem-AUS :usedBy :AUS, :Burdekin, :Daly, :Fitzroy, :Melbourne,
    :MurrayDarling, :Ord, :Perth .

:AllocationExtraction%3ASalinityAndWaterTableManagement-AUS :usedBy :AUS, :MurrayDarling .

:AppliedWaterReuse%2FRecycledWater-CA :usedBy :CA .

:Commercial%3AUnmetered-NMOSE :usedBy :NM .

:Commercial%3AIncompleteMetered-NMOSE :usedBy :NM .

:Commercial%3AMetered-NMOSE :usedBy :NM .

:Commercial%3ASchools-NMOSE :usedBy :NM .

:Delivery%3ADesalinatedWater-AUS :usedBy :AUS, :Adelaide, :Melbourne, :MurrayDarling,
    :Perth, :SouthEastQueensland, :Sydney .

:Delivery%3AInter-region-AUS :usedBy :AUS, :Canberra, :Perth, :SouthEastQueensland .

:Delivery%3AInter-regionAgreement-AUS :usedBy :AUS, :Adelaide, :Melbourne, :Sydney .

:Delivery%3AIrrigationScheme-AUS :usedBy :AUS, :Adelaide, :Perth .

:Delivery%3ARecycledWater-AUS :usedBy :AUS, :Adelaide .

:Delivery%3AUrbanUsers-AUS :usedBy :AUS, :Melbourne .

:Discharge%3ALandscape-AUS :usedBy :AUS, :Adelaide, :Canberra, :Daly, :Fitzroy, :Melbourne,
    :MurrayDarling, :Ord, :Perth, :SouthEastQueensland, :Sydney .

:Discharge%3ASea-AUS :usedBy :AUS, :Adelaide, :Melbourne, :Perth, :SouthEastQueensland,
    :Sydney .

:Discharge%3ASurfaceWater-AUS :usedBy :AUS, :Adelaide, :Canberra, :Daly, :Melbourne,
    :MurrayDarling, :Perth, :SouthEastQueensland .

:Discharge%3AUrbanSupply-AUS :usedBy :AUS, :Perth .

:Discharge%3AUrbanSupplySystem-AUS :usedBy :AUS, :Canberra, :Melbourne, :MurrayDarling .

:Discharge%3AUser-AUS :usedBy :AUS, :SouthEastQueensland, :Sydney .

:Discharge%3AWastewater-AUS :usedBy :AUS, :Adelaide, :Canberra, :Daly, :Melbourne,
    :MurrayDarling, :Ord, :SouthEastQueensland, :Sydney .

:Diversions%3AStatutoryRights-AUS :usedBy :AUS, :Canberra, :Daly, :SouthEastQueensland,
    :Sydney .

:Extraction%3AStatutoryRights-AUS :usedBy :AUS, :Adelaide, :Canberra, :Daly, :Fitzroy,
    :MurrayDarling .

:Industrial%3ACoalbedMethandProduction-WY :usedBy :WY .

:Industrial%3AMiscellaneous-WY :usedBy :WY .

:Industrial%3ANaturalGas-WY :usedBy :BearRiver, :WY .

:Industrial%3AOilAndGas-WY :usedBy :WY .

:Inter-regionInflow%3AGroundwater-AUS :usedBy :AUS, :Adelaide, :Canberra, :Daly, :Fitzroy,
    :Melbourne, :MurrayDarling, :Ord, :Perth .

:Inter-regionInflow%3ASurfaceWater-AUS :usedBy :AUS, :Canberra, :MurrayDarling, :Perth .

:Inter-regionOutflow%3AGroundwater-AUS :usedBy :AUS, :Adelaide, :Canberra, :Daly,
    :Fitzroy, :Melbourne, :MurrayDarling, :Ord, :Perth .

:Leakage%3AFarmDams-AUS :usedBy :AUS, :Adelaide .

:Leakage%3AGroundwater-AUS :usedBy :AUS, :Adelaide, :Canberra, :Melbourne, :Perth,
    :SouthEastQueensland, :Sydney .

:Leakage%3ALandscape-AUS :usedBy :AUS, :Canberra, :Ord, :Perth .

:Leakage%3AUrbanSystem-AUS :usedBy :AUS, :Adelaide, :Canberra, :Melbourne, :MurrayDarling,
    :Perth, :SouthEastQueensland .

:Livestock%3AMetered-NMOSE :usedBy :NM .

:Livestock%3AUnmetered-NMOSE :usedBy :NM .

:ManagedAquiferRecharge%3AIndividualUser-AUS :usedBy :AUS, :Adelaide, :Burdekin, :MurrayDarling .

:ManagedAquiferRecharge%3AUrban-AUS :usedBy :AUS, :Adelaide .

:MonthlyConsumptiveUseCoefficient%28k%29 :usedBy :NM .

:NMOSE%E2%80%99sWaterUseAndConservationBureau%28WUCB%29Survey :usedBy :NM .

:Non-AllocatedDiversion%3ASurfaceWater-AUS :usedBy :AUS, :Adelaide, :SouthEastQueensland .

:Non-AllocatedExtraction%3AGroundwater-AUS :usedBy :AUS, :Adelaide, :SouthEastQueensland .

:Non-AllocatedExtraction%3AIndividualUsers-AUS :usedBy :AUS, :Canberra, :Daly, :Fitzroy,
    :Perth, :SouthEastQueensland .

:Non-AllocatedExtraction%3AIrrigation-AUS :usedBy :AUS, :Adelaide .

:Non-AllocatedExtraction%3AUrbanSystem-AUS :usedBy :AUS, :SouthEastQueensland .

:Non-allocatedDiversion%3AEnvironmentalPurposes-AUS :usedBy :AUS, :MurrayDarling .

:Non-allocatedDiversion%3AIndividualUsers-AUS :usedBy :AUS, :Burdekin, :Canberra,
    :Fitzroy, :Melbourne, :MurrayDarling, :SouthEastQueensland .

:Non-allocatedDiversion%3AUrbanSystem-AUS :usedBy :AUS, :Adelaide, :MurrayDarling,
    :SouthEastQueensland .

:PointReturn%3AIrrigation-AUS :usedBy :AUS, :Melbourne, :MurrayDarling, :Ord .

:Power%3AUnreported-NMOSE :usedBy :NM .

:PublicWaterSupply%3AMetered-NMOSE :usedBy :NM .

:PublicWaterSupply%3AUnmetered-NMOSE :usedBy :NM .

:Recharge%3AGroundwater-AUS :usedBy :AUS, :Canberra, :Daly, :Melbourne, :MurrayDarling,
    :Sydney .

:Recharge%3ALandscape-AUS :usedBy :AUS, :Adelaide, :Canberra, :Daly, :Fitzroy, :Melbourne,
    :MurrayDarling, :Ord, :Perth .

:Recharge%3ASurfaceWater-AUS :usedBy :AUS, :Canberra, :Daly, :Melbourne, :MurrayDarling,
    :Perth .

:RecycledWaterDelivery%3AUrbanUsers-AUS :usedBy :AUS, :Adelaide, :Canberra, :Melbourne,
    :Perth, :SouthEastQueensland, :Sydney .

:ReturnFlow%3AEnvironmentalPurposes-AUS :usedBy :AUS, :MurrayDarling .

:RiparianRelease%3AUrbanSupply-AUS :usedBy :AUS, :Perth .

:SeasonalConsumptiveUseCoefficients%28K%29 :usedBy :CO, :NM .

:SupplySystemDelivery%3AInter-Region-AUS :usedBy :AUS, :Melbourne, :Perth .

:SupplySystemDelivery%3AUrbanUsers-AUS :usedBy :AUS, :Adelaide, :Canberra, :Melbourne,
    :Perth, :SouthEastQueensland, :Sydney .

:SupplySystemDischarge%3AReservoirs-AUS :usedBy :AUS, :Perth .

:SupplySystemTransfer%3AInter-region-AUS :usedBy :AUS, :Adelaide, :Melbourne, :Perth .

:Transfer%3AInter-region-AUS :usedBy :AUS, :Melbourne .

:USCensusBureau%22CityAndTown%28IncorporatedPlacesAndMinorCivilDivisions%29%22DataSet
  :usedBy :WY .

:WastewaterDischarge%3ALandscape-AUS :usedBy :AUS, :Canberra, :Melbourne .

:WyomingDepartmentOfEnvironmentalQuality%28WYDEQ%29 :usedBy :WY .

:CaliforniaStateWaterResourcesControlBoardUrbanWaterSupplyStatistics :usedBy :CA .

:AUSBureauOfMeteorology :usedBy :AUS, :Adelaide, :Burdekin, :Canberra, :Daly, :Fitzroy,
    :Melbourne, :MurrayDarling, :Ord, :Perth, :SouthEastQueensland, :Sydney .

:Adelaide :usedBy :AUS .

:Burdekin :usedBy :AUS .

:Canberra :usedBy :AUS .

:Daly :usedBy :AUS .

:Fitzroy :usedBy :AUS .

:Melbourne :usedBy :AUS .

:MurrayDarling :usedBy :AUS .

:Ord :usedBy :AUS .

:Perth :usedBy :AUS .

:SouthEastQueensland :usedBy :AUS .

:Sydney :usedBy :AUS .

:AUSDepartmentOfEnvironmentAndNaturalResources :usedBy :AUS, :Daly .

:AUSDepartmentOfIndustry :usedBy :AUS, :Sydney .

:AWRA-LModel :usedBy :AUS, :Adelaide, :Burdekin, :Canberra, :Daly, :Fitzroy, :Melbourne,
    :MurrayDarling, :Ord, :Perth, :SouthEastQueensland, :Sydney .

:AWRA-RModel :usedBy :AUS, :Adelaide, :Burdekin, :Daly, :Fitzroy, :Melbourne, :MurrayDarling,
    :Ord, :Perth, :SouthEastQueensland, :Sydney .

:AcreageByCropType :usedBy :CA .

:AgriculturalAppliedWater-CA :usedBy :CA .

:CAAgriculturalWaterManagementPlans :usedBy :CA .

:CALocalAgencyWaterDeliveryRecords :usedBy :CA .

:CAPreviousReports :usedBy :CA .

:ExistingCaliforniaWaterPlan :usedBy :CA .

:On-farmWaterUseData :usedBy :CA .

:UniversityOfCaliforniaCooperativeExtensionFarmAdvisors :usedBy :CA .

:CentralValleyHydrologicModel%28CVHM%29 :usedBy :CA .

:Cal-SIMETAWModel :usedBy :CA .

:CropETApproach :usedBy :CA .

:Water-DutyBasedApproach :usedBy :CA .

:CropETRequirements :usedBy :CA .

:ETOfAppliedWater :usedBy :CA .

:IrrigationEfficiency :usedBy :CA .

:IrrigationRecharge :usedBy :CA .

:PrecipitationVolumeForAgriculturalArea :usedBy :CA .

:RunoffVolume :usedBy :CA .

:WaterDutyRateByCrop :usedBy :CA .

:ApparentLosses :usedBy :AUS, :Canberra, :Melbourne, :Sydney .

:CADWRDemographicData :usedBy :CA .

:CADWRIrrigationMethodsSurvey :usedBy :CA .

:CADWRLandUseViewer :usedBy :CA .

:CADWRSGMADataViewer :usedBy :CA .

:CALSIM2 :usedBy :CA .

:CAUrbanWaterManagementPlans :usedBy :CA .

:CaliforniaAgriculturalLandAndWaterUseEstimates :usedBy :CA .

:CaliforniaDepartmentOfFinance :usedBy :CA .

:CaliforniaPesticideInformationPortal :usedBy :CA .

:CaliforniaWaterPlanPortfolio :usedBy :CA .

:DWRLandUseSurveys :usedBy :CA .

:SWRCBWaterConservationPortal :usedBy :CA .

:USDACropScape :usedBy :CA .

:USDANaturalResourcesConservationServiceGeospatialWebSoilSurvey :usedBy :CA .

:CAIntegratedWaterFlowModel%28IWFM%29 :usedBy :CA .

:CAIntegratedWaterFlowModel%28IWFM%29DemandCalculator :usedBy :CA .

:CaliforniaStateGroundwaterElevationMonitoring%28CASGEM%29 :usedBy :CA .

:MODFLOW-OWHM%3AOneWaterHydrologicFlowModel :usedBy :AUS, :CA, :MurrayDarling .

:NationalLandCoverDataBase%28NLCD%29 :usedBy :CA .

:USDACountyAgCommissioner%27sDataListing :usedBy :CA .

:VegetationConditionExplorer%28VegScape%29 :usedBy :CA .

:WaterUseClassificationOfLandscapeSpecies%28WUCOLS%29 :usedBy :CA .

:AquiferAttribution :usedBy :AUS, :Melbourne .

:AUSDepartmentOfEnvironment%2CLand%2CWaterAndPlanning :usedBy :AUS, :Melbourne .

:AquiferThickness :usedBy :AUS, :Melbourne .

:PortPhillipCatchmentManagementAuthority :usedBy :AUS, :Melbourne .

:AssumedDiversionRate :usedBy :AUS, :SouthEastQueensland .

:AustralianBureauOfStatisticsSurveys :usedBy :AUS, :Perth .

:WesternMountLoftyRangesPrescribedWaterResourcesAreaWaterAllocationPlan :usedBy :AUS,
    :Adelaide .

:BaseflowSeparationTechniques :usedBy :CA .

:BillingMeters :usedBy :AUS, :Adelaide, :Canberra, :Melbourne, :Perth, :SouthEastQueensland,
    :Sydney .

:BoreLocation :usedBy :AUS, :Melbourne .

:BudgetZoneArea :usedBy :CA .

:CACountyAgriculturalCommissionerCropReports :usedBy :CA .

:CADWRExtensometer :usedBy :CA .

:CALSIM3 :usedBy :CA .

:CARecycledWaterDataFromIndustrialUsers :usedBy :CA .

:CAValidatedWaterLossReporting :usedBy :CA .

:CAWastewaterDataAndDispositionOfTheWater :usedBy :CA .

:CSIROWavesModel :usedBy :AUS, :Perth .

:CaliforniaNevadaRiverForecastCenter :usedBy :CA .

:CaliforniaWaterPlanUpdateData :usedBy :CA .

:CaliforniaWaterPlanWaterPortfolioManagedWetlandsWaterUseData :usedBy :CA .

:ChangeInGroundwaterLevel :usedBy :CA .

:GroundwaterElevation :usedBy :CA .

:SpecificYield :usedBy :CA .

:WaterStorageProduct :usedBy :AUS, :Melbourne, :Perth, :SouthEastQueensland .

:CADWRBulletin118%3AGroundwaterReport :usedBy :CA .

:CaliforniaDataExchangeCenter%28CDEC%29 :usedBy :CA .

:DWRWaterDataLibrary%3ASurfaceWaterAndGroundwaterData :usedBy :CA .

:GravityRecoveryAndClimateExperiment%28GRACE%29 :usedBy :CA .

:MassBalance :usedBy :CA .

:USGSCaliforniaWaterScienceCenter-GroundwaterModeling :usedBy :CA .

:ChangeInLakeStorage :usedBy :CA .

:WaterUseModels :usedBy :CA .

:ChangeInPondedWaterStorage :usedBy :CA .

:ChangeInRootZoneSoilMoisture :usedBy :CA .

:ChangeInSoilMoisture :usedBy :CA .

:ChangeInUnsaturatedZoneStorage :usedBy :CA .

:HYDRODatabase :usedBy :AUS, :MurrayDarling .

:WaterLevel :usedBy :AUS, :Adelaide, :Burdekin, :Fitzroy, :Melbourne, :Ord, :SouthEastQueensland,
    :Sydney .

:USBRCentralValleyProjectRefugeWaterDeliveryData :usedBy :CA .

:USGSSurface-WaterDataForCalifornia :usedBy :CA .

:CenterForHydrometeorologyAndRemoteSensingDataPortal%28CHRS%29 :usedBy :CA .

:LakeInflowFromStreams-CA :usedBy :CA .

:LakeOutflowToStreams-CA :usedBy :CA .

:CityWestWaterAnnualReport :usedBy :AUS, :MurrayDarling .

:ConstantPercentage :usedBy :CA .

:ConstantSeepagePercentage :usedBy :CA .

:NOAANationalCentersForEnvironmentalInformation-ClimateDataOnline :usedBy :CA .

:NOAANationalCentersForEnvironmentalInformation-ClimatologicalDataPublications :usedBy
    :CA .

:NWSCLIMATEPREDICTIONCENTEREVAPORATION :usedBy :CA .

:CADWRBulletin132%3AManagementOfTheCaliforniaStateWaterProject :usedBy :CA .

:CaliforniaIrrigationManagementInformationSystem%28CIMIS%29 :usedBy :CA .

:DWRBulletin73%3AEvaporationFromWaterSurfaceInCalifornia%281979%29 :usedBy :CA .

:Evapotranspiration%28ET%29Rates :usedBy :CA .

:s.71WaterResourceReport :usedBy :AUS, :MurrayDarling .

:EstimateConveyanceSeepageRateBasedOnCanalCharacteristics :usedBy :CA .

:CropCoefficientApproach :usedBy :CA .

:CAIrrigationTrainingAndResearchCenter%28ITRC%29EvapotranspirationData :usedBy :CA .

:FAO56Chapter6SingleCropCoefficients%28Kc%29 :usedBy :CA .

:SpatialCaliforniaIrrigationManagementInformationSystem%28CIMIS%29 :usedBy :CA .

:ReferenceCropET%28ETo%29 :usedBy :CA .

:CulturalPractices :usedBy :CA .

:DataFromPrivateWetlandsOrDuckClubs :usedBy :CA .

:USFishAndWildlifeServices :usedBy :CA .

:CaliforniaDepartmentOfFishAndWildlife%28CDFW%29 :usedBy :CA .

:CumulativeWaterMeter :usedBy :AUS, :Fitzroy .

:CustomerMeters :usedBy :AUS, :Adelaide, :Canberra, :Melbourne, :Perth, :SouthEastQueensland,
    :Sydney .

:SAWaterGISDatabase :usedBy :AUS, :Adelaide .

:DWRGuideToEstimatingIrrigationWaterNeedsOfLandscapePlantingsInCalifornia1 :usedBy
    :CA .

:DWRPublicWaterSupplyStatisticsData-Historical :usedBy :CA .

:DailyMaxAndMinAirTemperature :usedBy :CA .

:DailyPrecipitation :usedBy :CA .

:DailyShort-WaveSolarRadiation :usedBy :CA .

:DailyWaterBalanceApproach :usedBy :AUS, :MurrayDarling .

:DepartmentOfWaterAndEnvironmentalRegulation :usedBy :AUS, :Daly, :Perth .

:DrainageAreaOfSiteOfInterest :usedBy :CA .

:DrainageAreaRatioMethod :usedBy :CA .

:DrainageAreaOfStreamflowGagingStation%28Ax%29 :usedBy :CA .

:MeasureStreamflow%28Xij%29 :usedBy :CA .

:EntitlementVolume :usedBy :AUS, :Canberra, :Melbourne .

:EstimateAppliedWaterReuseAndRecycledWaterVolumes :usedBy :CA .

:EstimatedNon-revenueWaterVolumes :usedBy :AUS, :Adelaide, :Canberra, :Melbourne,
    :Perth, :SouthEastQueensland, :Sydney .

:EstimationOfAbstraction :usedBy :AUS, :Perth .

:Morton%27sShallowLakeFormulation :usedBy :AUS, :Adelaide, :Burdekin, :Canberra, :Fitzroy,
    :Melbourne, :MurrayDarling, :SouthEastQueensland, :Sydney .

:EvaporationPanMethod :usedBy :CA .

:PanCoefficient :usedBy :CA .

:SurfaceAreaOfWaterBody :usedBy :CA .

:METRIC-EarthEngineEvapotranspirationFlux :usedBy :CA .

:USGSBasinCharacterizationModel :usedBy :CA .

:CADWRBulletin113%3ACropWaterUse :usedBy :CA .

:MOD16%3AMODISGlobalEvapotranspirationProject :usedBy :CA .

:NOAAOfficeOfSatelliteAndProductOperationsALEXI%3AAtmosphere-LandExchangeInverseModel
  :usedBy :CA .

:NorthAmericanLandDataAssimilationSystem%28NLDAS-2%29 :usedBy :CA .

:OperationalSimplifiedSurfaceEnergyBalance%28SSEBop%29 :usedBy :CA .

:TOPS-SIMS%3ASatelliteIrrigationManagementSupport :usedBy :CA .

:FloodplainModule :usedBy :AUS, :Adelaide, :Burdekin, :Canberra, :Daly, :Fitzroy,
    :Melbourne, :MurrayDarling, :Ord, :Perth, :SouthEastQueensland, :Sydney .

:FlowData :usedBy :AUS, :Daly, :Ord .

:FlowNetAnalysis :usedBy :CA .

:EffectiveThicknessOfTheAquifer%28b%29 :usedBy :CA .

:FlowThroughAVerticalPlaneThatExtendsBeneathTheShorelineOfASurfaceWaterBody%28Q%29
  :usedBy :CA .

:HorizonalHydraulicConductivityOfTheAquiferAtTheBoundary%28K%29 :usedBy :CA .

:NumberOfEquipotentialHeadDropsOverTheAreaOfInterest%28n%29 :usedBy :CA .

:NumberOfStreamtubesAcrossAFlowNet%28M%29 :usedBy :CA .

:GISGroundwaterModelling :usedBy :AUS, :Adelaide .

:PortPhillipCatchmentManagementAuthorityGroundwaterModel :usedBy :AUS, :Melbourne .

:GroundwaterLevel :usedBy :AUS, :Melbourne .

:HydraulicConductivity :usedBy :AUS, :Melbourne .

:Darcy%27sLaw :usedBy :CA .

:GippslandWaterAnnualReport :usedBy :AUS, :Melbourne .

:Peel-HarveyRegionalAquiferModelingSystem%28PHRAMS%29 :usedBy :AUS, :Perth .

:PerthRegionalAquiferModelingSystems%28PRAMS%29 :usedBy :AUS, :Perth .

:LandUseAndAppliedWaterEstimationMethod :usedBy :CA .

:LocalAgencyRecords :usedBy :CA .

:CaliforniaStateWaterResourcesControlBoard%28SWRCB%29UrbanWaterSupplyStatistics :usedBy
    :CA .

:GroundwaterExtractionUnderStatutoryRightsEstimationMethod :usedBy :AUS, :Daly .

:GroundwaterModelling :usedBy :AUS, :MurrayDarling .

:HabitatAcreage :usedBy :CA .

:ExistingWaterRightInformationFromStateWaterResourcesControlBoard%28SWRCB%29 :usedBy
    :CA .

:ManagedWetlandAppliedWater-CA :usedBy :CA .

:OperationalSpill :usedBy :CA .

:UrbanAppliedWater-CA :usedBy :CA .

:IndividualUserLicenses :usedBy :AUS, :Burdekin, :Daly, :Fitzroy, :Melbourne, :MurrayDarling,
    :Ord, :Perth .

:KimberelyAgriculturalInvestment%3AGoomingFarmlands :usedBy :AUS, :Ord .

:OrdIrrigationCooperative%3APacksaddleAndIvanhoePlains :usedBy :AUS, :Ord .

:WaterCorporation%3AM1Channel :usedBy :AUS, :Ord .

:IndustrialWaterUse :usedBy :CA .

:WaterUseSurveys :usedBy :AUS, :CA, :Perth .

:InflowFromContributingOrTributaryStreams :usedBy :CA .

:InflowToWaterTreatmentPlants :usedBy :AUS, :Adelaide .

:GeographicInformationSystem%28GIS%29 :usedBy :AUS, :MurrayDarling .

:MassTransferEquations :usedBy :CA .

:MassTransferCoefficient :usedBy :CA .

:SaturationVaporPressure :usedBy :CA .

:WindFunction :usedBy :CA .

:BottomElevationOfTheLakebedSediments%28HlakebedBottom%29 :usedBy :CA .

:DistanceBetweenTwoPointsWithKnownHead%28I%29 :usedBy :CA .

:GroundwaterLevel%28Haquifer%29 :usedBy :CA .

:SurfaceAreaOfLake%28Al%29 :usedBy :CA .

:VerticalHydraulicConductivityOfTheSurroundingAquifer%28Kv%29 :usedBy :CA .

:WaterLevelInLake%28Hlake%29 :usedBy :CA .

:WettedPerimeterOfLakeMultipliedByTheAverageSaturatedThicknessOfAquiferAroundTheLake%28Awpl%29
  :usedBy :CA .

:USGSPublications :usedBy :CA .

:MassCurve :usedBy :CA .

:ReservoirOperationRuleCurve :usedBy :CA .

:ConsumptiveUseOfPrecipitation%28EP%29 :usedBy :CA .

:LandscapeModelledRunoff :usedBy :AUS, :Adelaide, :Burdekin, :Canberra, :Daly, :Fitzroy,
    :Melbourne, :MurrayDarling, :Ord, :Perth, :SouthEastQueensland, :Sydney .

:LyneAndHollickFilter :usedBy :AUS, :Adelaide .

:MIKE11 :usedBy :AUS, :Daly .

:MeteredWaterData :usedBy :AUS, :Adelaide, :Burdekin, :Canberra, :Daly, :Fitzroy,
    :Melbourne, :MurrayDarling, :Ord, :Perth, :SouthEastQueensland, :Sydney .

:USFWSAndCDFWRefugeWaterManagementPlans :usedBy :CA .

:ManagedWetlandsAppliedWaterEstimation :usedBy :CA .

:UnitETOfAppliedWater :usedBy :CA .

:StreamflowAtDownstreamGauge :usedBy :CA .

:StreamflowAtUpstreamGauge :usedBy :CA .

:MelbourneWaterAnnualReport :usedBy :AUS, :Melbourne .

:SnowyHydro :usedBy :AUS, :MurrayDarling .

:SouthEastWaterAnnualReport :usedBy :AUS, :Melbourne .

:UltrasonicFlowMeters :usedBy :AUS, :Sydney .

:YarraValleyWaterAnnualReport :usedBy :AUS, :Melbourne .

:ModelledRunoff :usedBy :AUS, :Adelaide, :Burdekin, :Canberra, :Daly, :Fitzroy, :Melbourne,
    :MurrayDarling, :Ord, :Perth, :SouthEastQueensland, :Sydney .

:MoretonAndLoganBasinResourceOperatingLicenses :usedBy :AUS, :SouthEastQueensland .

:NetworkRealLossesAndApparentLossesModelingSoftware :usedBy :AUS, :Adelaide, :Melbourne,
    :Perth, :SouthEastQueensland, :Sydney .

:NewSouthWalesDepartmentOfWater :usedBy :AUS, :Canberra .

:Observation :usedBy :AUS, :Melbourne, :SouthEastQueensland .

:OnsiteRe-useMeters :usedBy :AUS, :Adelaide, :Canberra, :Melbourne, :SouthEastQueensland .

:OtherSupplySystemDecreases-AUS :usedBy :AUS, :Adelaide, :Melbourne, :Perth, :Sydney .

:RealLossesEquation :usedBy :AUS, :Canberra, :Melbourne, :Sydney .

:OtherWastewaterDecreases-AUS :usedBy :AUS, :Adelaide, :Canberra, :Melbourne, :SouthEastQueensland .

:StreamGages :usedBy :AUS, :Canberra, :SouthEastQueensland .

:PopulationAndPer-CapitaWaterUse :usedBy :CA .

:CentralValleySpatialDatabase-partOfTheCentralValleyHydrologicModel%5BCVHM%5DProject
  :usedBy :CA .

:SpatialAveragingTechniques :usedBy :CA .

:PropertyAreaEstimationMethodsForSurfaceWaterDiversions :usedBy :AUS, :Daly .

:UnmeteredAuthorisedConsumption :usedBy :AUS, :Canberra, :Melbourne, :Sydney .

:RechargeAsPercentageOfRainfall :usedBy :AUS, :MurrayDarling .

:RechargeCreditBalance :usedBy :AUS, :Adelaide .

:AUSDepartmentForEnvironmentAndWater%28DEW%29 :usedBy :AUS, :Adelaide .

:WaterRecyclingSurvey%282015%29 :usedBy :CA .

:ReportFromBowenBrokenAndBurdekinHaughtonWaterSupplySchemes :usedBy :AUS, :Burdekin .

:ResourceOperatingLicenseTables :usedBy :AUS, :SouthEastQueensland .

:ReturnFlowEstimationMethod :usedBy :CA .

:RiparianWaterAuthorisations :usedBy :AUS, :SouthEastQueensland .

:RiverAndGroundwaterInteractionModule :usedBy :AUS, :Canberra, :Perth, :Sydney .

:RiverLosses-AUS :usedBy :AUS, :Perth .

:CaliforniaDepartmentOfTransportation%27sHighwayDesignManual :usedBy :CA .

:RunoffCurveNumberMethod :usedBy :CA .

:U.C.DavisSoilResourceLab :usedBy :CA .

:Precipitation-RunoffModelingSystem%28PRMS%29 :usedBy :CA .

:PublicPolicyInstituteOfCalifornia%28PPIC%29Map :usedBy :CA .

:SAWaterStorageVolumeRelationship :usedBy :AUS, :Adelaide .

:SWRCBElectronicAnnualReport :usedBy :CA .

:SWRCBMonthlyUrbanWaterProductionReporting :usedBy :CA .

:Seqwater :usedBy :AUS, :SouthEastQueensland .

:SpatialAssessments :usedBy :AUS, :Daly .

:AverageThicknessOfStreambed%28Bstream%29 :usedBy :CA .

:BottomElevationOfStreambedSediments%28HstreambedBottom%29 :usedBy :CA .

:EffectiveAreaOfFlowExchange%28Awps%29 :usedBy :CA .

:HydraulicConductivityOfTheStreambedMaterial%28Ks%29 :usedBy :CA .

:WaterStageInStream%28Hstream%29 :usedBy :CA .

:USGSDR3M :usedBy :CA .

:WaterResourceAssociatesHYSIM :usedBy :CA .

<http://purl.org/iow/WaterBudgetingFramework/UniversityOfWashington%E2%80%99sVariableInfiltrationCapacityModel%28VIC%29.>
  :usedBy :CA .

:Vieux%26Associates%27Vflo :usedBy :CA .

:DescriptiveDataOfTopography%2CSoils%2CAndVegetation :usedBy :CA .

:Cross-sectionalAreaSubjectToBoundaryFlow%28Ab%29 :usedBy :CA .

:DepthOfCrossSection%28b%29 :usedBy :CA .

:HydraulicConductivityOfTheAquiferBoundary%28K%29 :usedBy :CA .

:HydraulicGradientThroughTheCrossSection%28i%29 :usedBy :CA .

:KnownGroundwaterElevationInsideTheBoundary%28hg%29 :usedBy :CA .

:KnownGroundwaterElevationOutsideTheBoundary%28hb%29 :usedBy :CA .

:SubsurfaceFlowAcrossTheBoundary%28Qb%29 :usedBy :CA .

:TransmissivityOfTheAquiferAtTheBoundary%28T%29 :usedBy :CA .

:WidthOfCrossSection%28w%29 :usedBy :CA .

:SurplusIrrigationAssumption :usedBy :AUS, :Perth .

:USGSExtensometer :usedBy :CA .

:VerticalFluxModel :usedBy :AUS, :Perth .

:VirginiaPipelineSchemePumpStation :usedBy :AUS, :Adelaide .

:WaterAllocationPlans :usedBy :AUS, :Daly .

:WaterCorporationSurveys :usedBy :AUS, :Perth .

:WaterSharingPlanForTheGreaterMetropolitanRegionUnregulatedRiverWaterSources :usedBy
    :AUS, :Sydney .

:WaterTableFluctuationModelling :usedBy :AUS, :MurrayDarling .

:WillungaBasinWaterCompany :usedBy :AUS, :Adelaide .

:WaterIndustryLicensingManagementDatabase%28WILMA%29 :usedBy :AUS, :Adelaide .

:SupervisoryControlAndDataAcquisitions%28SCADA%29 :usedBy :AUS, :Perth .

:CARecycledWaterDataFromLocal%2FMunicipalWaterSuppliers :usedBy :CA .

:BarossaInfrastructureLimited%28BIL%29AnnualReport :usedBy :AUS, :Adelaide .

:FiniteElementSubsurfaceFlowSystem%28FEFLOW%29 :usedBy :AUS, :Daly .

:WaterTrackingAndElectronicReportingSystem%28WaTERS%29 :usedBy :AUS, :SouthEastQueensland .

:Losses%3AManagementOfTreatedWater-AUS :usedBy :AUS, :Sydney .

:Losses%3AWastewaterTreatmentSystem-AUS :usedBy :AUS, :Sydney .

:Non-allocatedDiversion%3AUrbanWaterSystemEstimationMethod :usedBy :AUS, :Adelaide .

:SAWater%27sTotalLicensedDiversionVolumeFromWesternMountLoftyRangesPWRA :usedBy :AUS,
    :Adelaide .

:RecycledWaterDelivery%3AIrrigation-AUS :usedBy :AUS, :Melbourne .

:SupplySystemDelivery%3AIrrigation-AUS :usedBy :AUS, :Melbourne .

:SupplySystemDischarge%3ASurfaceWater-AUS :usedBy :AUS, :Canberra .

:WastewaterAndRecycledWaterDischarge%3ASurfaceWater-AUS :usedBy :AUS, :Sydney .

:WastewaterDischarge%3ASurfaceWater-AUS :usedBy :AUS, :Canberra, :Melbourne, :SouthEastQueensland .

:CropConsumptiveUse-CO skos:isExactMatch :IrrigatedAgricultureDepletions-NMOSE .

:MunicipalAndIndustrialConsumptiveUse-CO skos:isExactMatch :MunicipalAndIndustrialDepeltion-UT .

:AgriculturalConsumptiveUse-WY skos:isExactMatch :CropConsumptiveUse-CO .

:TotalDiversions-WY skos:isExactMatch :SurfaceWaterDiversions-CA .

:AgriculturalDepletions-UT skos:isExactMatch :AgriculturalConsumptiveUse-WY, :CropConsumptiveUse-CO .

:SurfaceDiversionToCropland-UT skos:isExactMatch :IrrigationSurfaceWaterDiversions-WY .

:AreaOutflows skos:isExactMatch :TotalSurfaceWaterOutflow-CA .

:BasinOutflow-UT skos:isExactMatch :StreamOutfow-CA .

:GagedStreamOutflow-WY skos:isExactMatch :GagedSurfaceWaterOutflow-CO .

:BasinInflow-UT skos:isExactMatch :StreamInflow-CA .

:RiverInflow-UT skos:isExactMatch :StreamInflow-CA .

:GagedStreamInflow-WY skos:isExactMatch :GagedSurfaceWaterInflow-CO .

:ChangeInGroundWaterStorage-CO skos:isExactMatch :ChangeInGroundwaterStorage-CA .

:ChangeInSurfaceWaterStorage-CO skos:isExactMatch :ChangeInSurfaceWaterStorage-CA .

:Precipitation-CO skos:isExactMatch :Precipitation-CA, :Precipitation-NM .

:Precipitation-UT skos:isExactMatch :Precipitation-CA, :Precipitation-CO, :Precipitation-WY .

:Precipitation-WY skos:isExactMatch :Precipitation-CA, :Precipitation-CO, :Precipitation-NM,
    :Precipitation-UT .

:IrrigatedAgricultureDepletions-NMOSE skos:isExactMatch :AgriculturalConsumptiveUse-WY,
    :AgriculturalDepletions-UT, :CropConsumptiveUse-CO .

:EvaporationFromReservoirs-NMOSE skos:isExactMatch :ReservoirEvaporation-CO, :ReservoirEvaporation-UT .

:ReservoirEvaporation-CO skos:isExactMatch :ReservoirEvaporation-UT .

:ReservoirEvaporation-UT skos:isExactMatch :ReservoirEvaporation-CO, :ReservoirEvaporation-WY .

:GroundWaterInflow-CO skos:isExactMatch :SubsurfaceInflow-CA .

:GroundWaterOutflow-CO skos:isExactMatch :SubsurfaceOutflow-CA .

:GroundwaterInflows-NM skos:isExactMatch :SubsurfaceInflow-CA .

:GroundwaterUse-UT skos:isExactMatch :GroundwaterExtraction-CA .

:PumpedGroundwater-UT skos:isExactMatch :GroundwaterExtraction-CA .

:Imports-CO skos:isExactMatch :ImportedWater-CA .

:Livestock-NMOSE skos:isExactMatch :LivestockConsumptiveUse-WY .

:LivestockConsumptiveUse-WY skos:isExactMatch :LivestockConsumptiveUse-CO .

:Mining-NMOSE skos:isExactMatch :Industrial%3AMineProduction-WY .

:Power-NMOSE skos:isExactMatch :Industrial%3AElectricalGeneration-WY .

:NaturalSystemUse-UT skos:isExactMatch :Evapotranspiration-CA, :NativeVegetationConsumptiveUse-CO .

:ReservoirEvaporation-WY skos:isExactMatch :ReservoirEvaporation-CO, :ReservoirEvaporation-UT .

:Runoff-NM skos:isExactMatch :Runoff-CA .

:SurfaceWaterEvaporation-NM skos:isExactMatch :StreamEvaporation-CA .

:SurfaceWaterInflows-NM skos:isExactMatch :StreamInflow-CA .

:TotalLandReturnFlow-UT skos:isExactMatch :ReturnFlow-CA .

:isPartialSubComponentOf dct:modified "2020-10-07T16:43:40.747Z"^^xsd:dateTime .

:isSubComponentOf dct:modified "2020-10-07T16:43:28.956Z"^^xsd:dateTime .

skos:isExactMatch dct:modified "2020-12-07T03:10:24.157Z"^^xsd:dateTime .

:CaliforniaStateWaterResourcesControlBoardUrbanWaterSupplyStatistics dct:created "2020-10-16T01:50:05.943Z"^^xsd:dateTime;
  dct:modified "2020-10-16T01:52:59.113Z"^^xsd:dateTime .

<http://purl.org/iow/WaterBudgetingFramework/California_State_Water_Resources_Control_Board_(SWRCB)_Urban_Water_Supply_Statistics>
  dct:created "2020-10-16T01:49:18.606Z"^^xsd:dateTime .

_:node1e55oknkkx773 a owl:Restriction;
  owl:onProperty :isFlowType;
  owl:someValuesFrom <http://geoconnex.us/iow/WaterBudgetingFramework/ClosureTerm> .

_:node1e55oknkkx775 a owl:Restriction;
  owl:onProperty :isFlowType;
  owl:someValuesFrom <http://geoconnex.us/iow/WaterBudgetingFramework/ClosureTerm> .

_:node1e55oknkkx777 a owl:Restriction;
  owl:onProperty :isFlowType;
  owl:someValuesFrom <http://geoconnex.us/iow/WaterBudgetingFramework/ClosureTerm> .

_:node1e55oknkkx779 a owl:Restriction;
  owl:onProperty :isFlowType;
  owl:someValuesFrom <http://geoconnex.us/iow/WaterBudgetingFramework/ClosureTerm> .

_:node1e55oknkkx676 owl:onProperty :isFlowType;
  owl:someValuesFrom <http://geoconnex.us/iow/WaterBudgetingFramework/ClosureTerm> .

_:node1e55oknkkx678 owl:onProperty :isFlowType;
  owl:someValuesFrom <http://geoconnex.us/iow/WaterBudgetingFramework/ClosureTerm> .

_:node1e55oknkkx680 owl:onProperty :isFlowType;
  owl:someValuesFrom <http://geoconnex.us/iow/WaterBudgetingFramework/ClosureTerm> .

_:node1e55oknkkx682 owl:onProperty :isFlowType;
  owl:someValuesFrom <http://geoconnex.us/iow/WaterBudgetingFramework/ClosureTerm> .

_:node2 rdf:first skos:Concept;
  rdf:rest _:node3 .

_:node3 rdf:first skos:Collection;
  rdf:rest rdf:nil .

_:node1 owl:unionOf _:node2 .
